@prefix :      <http://publications.europa.eu/ontology/cdm#> .
@prefix cdm:      <http://publications.europa.eu/ontology/cdm#> .
@prefix annotation: <http://publications.europa.eu/ontology/annotation#> .
@prefix dct:   <http://purl.org/dc/terms/> .
@prefix rdf:   <http://www.w3.org/1999/02/22-rdf-syntax-ns#> .
@prefix org:   <http://www.w3.org/ns/org#> .
@prefix owl:   <http://www.w3.org/2002/07/owl#> .
@prefix xsd:   <http://www.w3.org/2001/XMLSchema#> .
@prefix cmr:   <http://publications.europa.eu/ontology/cdm/cmr#> .
@prefix skos:  <http://www.w3.org/2004/02/skos/core#> .
@prefix rdfs:  <http://www.w3.org/2000/01/rdf-schema#> .
@prefix foaf:  <http://xmlns.com/foaf/0.1/> .
@prefix dc:    <http://purl.org/dc/elements/1.1/> .

:dossier_involves_agent
        a                   owl:ObjectProperty ;
        rdfs:comment        "This dossier involves a given agent. To be decided which subtypes (if any) of this property might be needed, mapped from /ns4:ec_transmission_request/transmission/workflow/extension/ns3:workflow_agent" ;
        rdfs:domain         :dossier ;
        rdfs:label          "Dossier involves agent" ;
        rdfs:range          :agent ;
        rdfs:subPropertyOf  :involves .

<http://publications.europa.eu/resource/authority/fd_607>
        a       owl:NamedIndividual .

<http://publications.europa.eu/resource/authority/corporate-body/EP>
        a       owl:NamedIndividual .

:measure_national_implementing_number_official_journal
        a                   owl:DatatypeProperty ;
        rdfs:comment        "Number of national or regional official journal in which this NIM was published" ;
        rdfs:domain         :measure_national_implementing ;
        rdfs:label          "Number of national or regional Official Journal" ;
        rdfs:range          xsd:string ;
        rdfs:subPropertyOf  :number_official_journal .

:prereleased_in  a     owl:ObjectProperty ;
        rdfs:comment   "An entity being released in a pre-release version" ;
        rdfs:label     "Prereleased in" ;
        owl:inverseOf  :prereleases .

:resource_legal_declared_void_by_preliminary_ruling_case-law
        a                   owl:ObjectProperty ;
        rdfs:comment        "Calculated. Relevant for legal analysis: true." ;
        rdfs:domain         :resource_legal ;
        rdfs:label          "Legal resource declared void by preliminary ruling" ;
        rdfs:range          :case-law ;
        rdfs:subPropertyOf  :declared_void_by_preliminary_ruling ;
        owl:inverseOf       :case-law_declares_void_by_preliminary_ruling_resource_legal .

:resource_legal_judgement_corrected_by_case-law
        a                   owl:ObjectProperty ;
        rdfs:comment        "14 cases (2012-07-31). Example: 62007CA0161: \"Corrigendum 62008TN0509\". Relevant for legal analysis: true." ;
        rdfs:domain         :resource_legal ;
        rdfs:label          "Judgement corrected by case law" ;
        rdfs:range          :case-law ;
        rdfs:subPropertyOf  :judgement_corrected_by ;
        owl:inverseOf       :case-law_corrects_judgement_resource_legal .

:work_id_obsolete_notice
        a                   owl:DatatypeProperty ;
        rdfs:comment        "Place to store the old DORIS_KEY or PROCAT_KEY. Really obsolete, only for backwards compatibility for existing notices, not to be used for new notices" ;
        rdfs:domain         :work ;
        rdfs:label          "Obsolete notice id" ;
        rdfs:range          xsd:positiveInteger ;
        rdfs:subPropertyOf  :id_obsolete_notice .

:person  a               owl:Class ;
        rdfs:comment     "The FOAF vocabulary http://xmlns.com/foaf/spec can be used to specify other attributes such as name, email addresses etc. as applicable and needed. Such attributes are however currently not covered in Procat. http://xmlns.com/foaf/0.1/Person If we want to map a person specifically to an authority table (e.g. FD table 013 or 014) this works with inScheme to the appropriate table, e.g. FD 014 in this case: <CMROntology:document_budget_ep_reported_by_person><CMROntology:ATTO_FD_014 rdf:about=\"http://publications.europa.eu/resource/authority/fd_014/AALTONEN\"><skos:inScheme xmlns:skos=\"http://www.w3.org/2004/02/skos/core#\" rdf:resource=\"&cellar-authority;/fd_014\"/></CMROntology:ATTO_FD_014></CMROntology:document_budget_ep_reported_by_person> The person is then correctly decoded using the authority table in question" ;
        rdfs:label       "Person" ;
        rdfs:subClassOf  :agent ;
        rdfs:subClassOf  [ a                owl:Restriction ;
                           owl:cardinality  "1"^^xsd:nonNegativeInteger ;
                           owl:onProperty   cmr:lastModificationDate
                         ] ;
        rdfs:subClassOf  [ a                   owl:Restriction ;
                           owl:maxCardinality  "1"^^xsd:nonNegativeInteger ;
                           owl:onProperty      cmr:creationDate
                         ] .

:agent_addressed_by_resource_legal
        a                   owl:ObjectProperty ;
        rdfs:domain         :agent ;
        rdfs:label          "Agent addressed by legal resource" ;
        rdfs:range          :resource_legal ;
        rdfs:subPropertyOf  :addressed_by ;
        owl:inverseOf       :resource_legal_addresses_agent .

:preface  a              owl:Class ;
        rdfs:comment     "\"A foreword or preface addressed to the reader in which the author or publisher explains the content, purpose, or origin of the text\" (TEI 4.5)" ;
        rdfs:label       "Preface" ;
        rdfs:subClassOf  :front .

:creates  a         owl:ObjectProperty ;
        rdfs:label  "Creates" .

:sitting  a              owl:Class ;
        rdfs:comment     "This class represents the sitting of an institution in the scope of a meeting or session" ;
        rdfs:label       "Sitting" ;
        rdfs:subClassOf  :event .

:measure_national_implementing_date_notification
        a                   owl:DatatypeProperty ;
        rdfs:comment        "NIMs is at a given date addressed to an organization through a notification, given by the SecGen of the Commission" ;
        rdfs:domain         :measure_national_implementing ;
        rdfs:label          "Date of notification for a NIM" ;
        rdfs:range          xsd:date ;
        rdfs:subPropertyOf  :date_notification .

:manifestation_system_requirements
        a                   owl:DatatypeProperty ;
        rdfs:comment        "system requirements of this manifestation. based on 538 $a" ;
        rdfs:domain         :manifestation ;
        rdfs:label          "System requirements" ;
        rdfs:range          xsd:string ;
        rdfs:subPropertyOf  :system_requirements .

:non-opposition_joint-venture_notified
        a                owl:Class ;
        rdfs:comment     "Non-opposition to a notified joint venture (= subsector 3J of sector 3). At present 43 notices. Examples: 31998J0001, 32000J0048" ;
        rdfs:label       "Non-opposition to notified joint venture" ;
        rdfs:subClassOf  :legislation_secondary .

:dossier_category  a        owl:DatatypeProperty ;
        rdfs:comment        "Codes allowing to categorize the dossier. two possible values, CWP and REFIT." ;
        rdfs:domain         :dossier ;
        rdfs:label          "Dossier category" ;
        rdfs:range          xsd:string ;
        rdfs:subPropertyOf  :category .

:released_in  a             owl:ObjectProperty ;
        rdfs:comment        "An entity being released in a release version" ;
        rdfs:label          "Released in" ;
        rdfs:subPropertyOf  :published_in ;
        owl:inverseOf       :releases .

:resource_legal_suspends_resource_legal
        a                   owl:ObjectProperty ;
        rdfs:comment        "Relevant for legal analysis: true" ;
        rdfs:domain         :resource_legal ;
        rdfs:label          "Legal resource suspends legal resource. SP (2) / subsequent related instrument" ;
        rdfs:range          :resource_legal ;
        rdfs:subPropertyOf  :suspends ;
        owl:inverseOf       :resource_legal_suspended_by_resource_legal .

:manifestation_special-official-journal-act_pages_total
        a             owl:DatatypeProperty ;
        rdfs:comment  "Total number of pages in a Special Official Journal act document" ;
        rdfs:domain   :manifestation_special-official-journal-act ;
        rdfs:label    "Manifestation Special Official Journal act pages total" ;
        rdfs:range    xsd:positiveInteger .

:agent  a                owl:Class ;
        rdfs:comment     "\"A resource that acts or has the power to act. Examples of Agent include person, organization, and software agent\" (Dublin Core)" ;
        rdfs:label       "Agent" ;
        rdfs:subClassOf  [ a                            owl:Restriction ;
                           owl:maxQualifiedCardinality  "1"^^xsd:nonNegativeInteger ;
                           owl:onClass                  :role-qualifier ;
                           owl:onProperty               :agent_has_role-qualifier
                         ] ;
        rdfs:subClassOf  [ a                   owl:Restriction ;
                           owl:maxCardinality  "1"^^xsd:nonNegativeInteger ;
                           owl:onProperty      :agent_embargo
                         ] .

:manifestation_distribution_description_editorial
        a                   owl:DatatypeProperty ;
        rdfs:comment        "Distribution description" ;
        rdfs:domain         :manifestation_distribution ;
        rdfs:label          "Distribution description" ;
        rdfs:range          xsd:string ;
        rdfs:subPropertyOf  :description_editorial .

:archive_package_reference_internal
        a                   owl:DatatypeProperty ;
        rdfs:label          "Archive package reference internal" ;
        rdfs:subPropertyOf  :work_reference_internal .

[ a            owl:AllDisjointClasses ;
  owl:members  ( :procedure_without_code_interinstitutional :procedure_code_interinstitutional )
] .

:work_published_in_work
        a                   owl:ObjectProperty ;
        rdfs:comment        "The work published in another work. Meant to eventually replace resource_legal_published_in..." ;
        rdfs:domain         :work ;
        rdfs:label          "Work published by another work" ;
        rdfs:range          :work ;
        rdfs:subPropertyOf  :published_in ;
        owl:inverseOf       :work_publishes_work .

:work_version  a            owl:DatatypeProperty ;
        rdfs:comment        "Relevant for legal analysis: true. Version of a work, expressed in terms specific to a class of work (e.g. final/2, draft, definitive...). Relevant for legal analysis: true" ;
        rdfs:domain         :work ;
        rdfs:label          "Work version" ;
        rdfs:range          xsd:string ;
        rdfs:subPropertyOf  :version .

:evolutive_work_nature_classification
        a            owl:DatatypeProperty ;
        rdfs:domain  :evolutive_work ;
        rdfs:label   "Evolutive work nature classification" ;
        rdfs:range   xsd:anyURI .

:event_joint-responsibility_of_person
        a                   owl:ObjectProperty ;
        rdfs:comment        "Relevant for legal analysis: true. This event is under joint responsibility of a given person. Relevant for legal analysis: true" ;
        rdfs:domain         :event ;
        rdfs:label          "Event under joint responsibility of person" ;
        rdfs:range          :person ;
        rdfs:subPropertyOf  :joint-responsibility_of ;
        owl:inverseOf       :person_jointly-responsible_for_event .

:expression_table_of_contents_uses_language
        a                   owl:ObjectProperty ;
        rdfs:comment        "The language of the table of contents" ;
        rdfs:domain         :expression ;
        rdfs:label          "Expression's table of contents uses language" ;
        rdfs:range          :language ;
        rdfs:subPropertyOf  :table_of_contents_uses ;
        owl:inverseOf       :language_used_by_table_of_contents_expression .

:year_decision  a   owl:DatatypeProperty ;
        rdfs:label  "Year decision" .

:document_court_efta  a  owl:Class ;
        rdfs:comment     "Document of the European Free Trade Association (EFTA) Court (= subsector J of sector E in EUR-Lex)" ;
        rdfs:label       "Document of EFTA Court" ;
        rdfs:subClassOf  :document_efta .

:manifestation_has_item
        a                   owl:ObjectProperty ;
        rdfs:comment        "A manifestation has a given item (typically a datastream in the CCR). Some manifestations have no content (e.g. print manifestations)" ;
        rdfs:domain         :manifestation ;
        rdfs:label          "Manifestation has item" ;
        rdfs:range          :item ;
        rdfs:subPropertyOf  :has .

:position_eesc  a   owl:DatatypeProperty ;
        rdfs:label  "Position eesc" .

:judge_delivers_case-law
        a                   owl:ObjectProperty ;
        rdfs:domain         :judge ;
        rdfs:label          "Judge delivers case law" ;
        rdfs:range          :case-law ;
        rdfs:subPropertyOf  :delivers ;
        owl:inverseOf       :case-law_delivered_by_judge .

:proposal_other  a       owl:Class ;
        rdfs:comment     "Other Proposal, e.g. of the Commission or the Joint Staff" ;
        rdfs:label       "Other proposal for an act" ;
        rdfs:subClassOf  :proposal_act .

:efta   a             owl:DatatypeProperty ;
        rdfs:comment  "Entities with relation to EFTA" ;
        rdfs:label    "EFTA" .

:identifier_year  a  owl:DatatypeProperty ;
        rdfs:label  "Identifier year" .

:reads  a           owl:ObjectProperty ;
        rdfs:label  "Reads" .

:identifier_extension
        a           owl:DatatypeProperty ;
        rdfs:label  "Identifier extension" .

:requests_opinion  a  owl:ObjectProperty ;
        rdfs:label  "Requests opinion" .

:xml-schema-definition_reference
        a           owl:DatatypeProperty ;
        rdfs:label  "Xml schema definition reference" .

:work_includes_expression
        a                   owl:ObjectProperty ;
        rdfs:comment        "Relevant for legal analysis: true. This property associates an instance of work with an instance of expression belonging to a distinct instance of work. Relevant for legal analysis: true" ;
        rdfs:domain         :work ;
        rdfs:label          "Work includes expression" ;
        rdfs:range          :expression ;
        rdfs:subPropertyOf  :includes .

<http://publications.europa.eu/resource/authority/target_audience>
        a       owl:NamedIndividual .

:act_reference_european
        a           owl:DatatypeProperty ;
        rdfs:label  "Act reference european" .

:volume  a          owl:DatatypeProperty ;
        rdfs:label  "Volume" .

<http://publications.europa.eu/resource/authority/fd_602>
        a       owl:NamedIndividual .

:session  a              owl:Class ;
        rdfs:comment     "A meeting or session of an institution or working body." ;
        rdfs:label       "Session" ;
        rdfs:subClassOf  :dossier .

:title  a             owl:DatatypeProperty ;
        rdfs:comment  "Any type of title" ;
        rdfs:label    "Title" .

:parties  a         owl:DatatypeProperty ;
        rdfs:label  "Parties" .

:formatting  a      owl:DatatypeProperty ;
        rdfs:label  "Formatting" .

:ATTO_FD_613  a              owl:Class ;
        rdfs:label           "FD_613 ATTO table" ;
        rdfs:subClassOf      skos:Concept ;
        owl:equivalentClass  [ a               owl:Restriction ;
                               owl:hasValue    <http://publications.europa.eu/resource/authority/fd_613> ;
                               owl:onProperty  skos:inScheme
                             ] .

:event_initiated_by_institution
        a                   owl:ObjectProperty ;
        rdfs:comment        "Relevant for legal analysis: true. This event is initiated by a given institution. Examples include Discussions at the Council or the transmission of a COM from the Commission to Council. Relevant for legal analysis: true" ;
        rdfs:domain         :event ;
        rdfs:label          "Event initiated by institution" ;
        rdfs:range          :institution ;
        rdfs:subPropertyOf  :initiated_by ;
        owl:inverseOf       :institution_initiates_event .

:manifestation_official-journal-act_legal_effect_paper
        a                   owl:DatatypeProperty ;
        rdfs:comment        "Legal effect paper applying to an Official Journal act's manifestation" ;
        rdfs:domain         :manifestation_official-journal-act ;
        rdfs:label          "Manifestation Official Journal act legal effect paper" ;
        rdfs:range          xsd:boolean ;
        rdfs:subPropertyOf  :legal_effect_paper .

:date_document  a           owl:DatatypeProperty ;
        rdfs:label          "Date document" ;
        rdfs:range          xsd:date ;
        rdfs:subPropertyOf  :date .

:manifestation_special-official-journal-act_date_publication
        a                   owl:DatatypeProperty ;
        rdfs:comment        "Publication date of a Special Official Journal act's manifestation" ;
        rdfs:domain         :manifestation_special-official-journal-act ;
        rdfs:label          "Manifestation Special official journal act date publication" ;
        rdfs:range          xsd:date ;
        rdfs:subPropertyOf  :date_publication .

:resource_legal_affected_by_case-law
        a                   owl:ObjectProperty ;
        rdfs:comment        "Relevant for legal analysis: true. The case law in some way affects a legal resource. CD Here according to spec of advanced search the *celex* of the base act is to be indexed (= a language independent textual information). This information will be provided in the indexation notice. Relevant for legal analysis: true" ;
        rdfs:domain         :resource_legal ;
        rdfs:label          "Legal resource is affected by case law" ;
        rdfs:range          :case-law ;
        rdfs:subPropertyOf  :affected_by .

:concept_prelex_council
        a                owl:Class ;
        rdfs:comment     "Concept used in Prelex to classify events in Council sessions" ;
        rdfs:label       "Prelex concept" ;
        rdfs:subClassOf  :concept .

:case-law_national_affaire_jurisdiction
        a                   owl:DatatypeProperty ;
        rdfs:comment        "DEPRECATED, Jurisdiction of the affaire. coded" ;
        rdfs:domain         :case-law_national ;
        rdfs:label          "National affaire: Jurisdiction" ;
        rdfs:range          xsd:string ;
        rdfs:subPropertyOf  :affaire_jurisdiction ;
        owl:deprecated      true .

<http://publications.europa.eu/resource/authority/fd_013>
        a       owl:NamedIndividual .

:judge  a                owl:Class ;
        rdfs:comment     "Judge or rapporteur at the Court of Justice" ;
        rdfs:label       "Judge" ;
        rdfs:subClassOf  :person ;
        rdfs:subClassOf  [ a                            owl:Restriction ;
                           owl:minQualifiedCardinality  "1"^^xsd:nonNegativeInteger ;
                           owl:onClass                  :case-law ;
                           owl:onProperty               :judge_delivers_case-law
                         ] .

:authors-report  a  owl:ObjectProperty ;
        rdfs:label  "Authors report" .

:subject_to_appeal_in
        a           owl:ObjectProperty ;
        rdfs:label  "Subject to appeal in" .

:work_contains_part_legal
        a                   owl:ObjectProperty ;
        rdfs:domain         :work ;
        rdfs:label          "Work contains part (legal)" ;
        rdfs:range          :part_legal ;
        rdfs:subPropertyOf  :work_contains_subdivision , :contains .

:has_part  a        owl:ObjectProperty ;
        rdfs:label  "Has part" .

:work_dataset_has_part_work_dataset
        a                   owl:ObjectProperty ;
        rdfs:comment        "The described dataset includes the referenced dataset" ;
        rdfs:domain         :work_dataset ;
        rdfs:label          "Dataset has part" ;
        rdfs:range          :work_dataset ;
        rdfs:subPropertyOf  :has_part ;
        owl:inverseOf       :work_dataset_is_part_of_work_dataset .

:cpv_original_link_type
        a           owl:DatatypeProperty ;
        rdfs:label  "Cpv original link type" .

:act_consolidated_layer_constituted_by_version_act_consolidated
        a             owl:ObjectProperty ;
        rdfs:comment  "This property links the layer work with all the consolidated sublayer transmissions concerning this layer." ;
        rdfs:domain   :act_consolidated ;
        rdfs:label    "Act consolidated layer constituted by version act consolidated" ;
        rdfs:range    :act_consolidated .

:case-law_defers_application_of_resource_legal
        a                   owl:ObjectProperty ;
        rdfs:comment        "This property points to legal act quoted in the operative part of Court decisions" ;
        rdfs:domain         :case-law ;
        rdfs:label          "Case law defers application of legal resource" ;
        rdfs:range          :resource_legal ;
        rdfs:subPropertyOf  :defers_application_of ;
        owl:inverseOf       :resource_legal_application_deferred_by_case-law .

:manifestation_official-journal-act
        a                owl:Class ;
        rdfs:comment     "Manifestation of an Official Journal act" ;
        rdfs:label       "Manifestation Official Journal act" ;
        rdfs:subClassOf  :manifestation ;
        rdfs:subClassOf  [ a                   owl:Restriction ;
                           owl:maxCardinality  "1"^^xsd:nonNegativeInteger ;
                           owl:onProperty      :manifestation_official-journal-act_pages_total
                         ] ;
        rdfs:subClassOf  [ a                   owl:Restriction ;
                           owl:maxCardinality  "1"^^xsd:nonNegativeInteger ;
                           owl:onProperty      :manifestation_official-journal-act_legal_effect_paper
                         ] ;
        rdfs:subClassOf  [ a                   owl:Restriction ;
                           owl:maxCardinality  "1"^^xsd:nonNegativeInteger ;
                           owl:onProperty      :manifestation_official-journal-act_date_publication
                         ] .

:work_age  a                owl:DatatypeProperty ;
        rdfs:comment        "Age in years IMMC2CDM-OJ" ;
        rdfs:domain         :work ;
        rdfs:label          "Age of work" ;
        rdfs:range          xsd:positiveInteger ;
        rdfs:subPropertyOf  :age .

:information_miscellaneous
        a           owl:DatatypeProperty ;
        rdfs:label  "Information miscellaneous" .

:status  a                   owl:Class ;
        rdfs:comment         "Status of a (legal) file" ;
        rdfs:label           "Status" ;
        rdfs:subClassOf      skos:Concept ;
        owl:equivalentClass  [ a               owl:Restriction ;
                               owl:hasValue    <http://publications.europa.eu/resource/authority/file-status> ;
                               owl:onProperty  skos:inScheme
                             ] .

:communication_request_opinion_requests_opinion_on_resource_legal
        a                   owl:ObjectProperty ;
        rdfs:comment        "This property points to legal act quoted in the communication on a new case published in OJ. Relevant for legal analysis: true" ;
        rdfs:domain         :communication_request_opinion ;
        rdfs:label          "Communication requests opinion on legal resource" ;
        rdfs:range          :resource_legal ;
        rdfs:subPropertyOf  :requests_opinion_on ;
        owl:inverseOf       :resource_legal_opinion_requested_by_communication_request_opinion .

:date_expiration  a  owl:DatatypeProperty ;
        rdfs:label  "Date expiration" .

:consultation_objective
        a           owl:DatatypeProperty ;
        rdfs:label  "Consultation objective" .

:reported_by  a       owl:ObjectProperty ;
        rdfs:comment  "Rapporteur" ;
        rdfs:label    "Reported by" .

:case-law_delivered_by_institution
        a                   owl:ObjectProperty ;
        rdfs:comment        "Court delivering this case law. Should coincide with author encoded in sector code. In case of conflict AU has priority" ;
        rdfs:domain         :case-law ;
        rdfs:label          "Case law delivered by court" ;
        rdfs:range          :institution ;
        rdfs:subPropertyOf  :delivered_by ;
        owl:inverseOf       :institution_delivers_case-law .

<http://publications.europa.eu/resource/authority/fd_050>
        a       owl:NamedIndividual .

:advocate-general_responsible_for_event_case
        a              owl:ObjectProperty ;
        rdfs:comment   "The Advocate-General (agent) responsible for the execution of an event in a Court case" ;
        rdfs:domain    :advocate-general ;
        rdfs:label     "Responsible Advocat-General" ;
        rdfs:range     :event_case ;
        owl:inverseOf  :event_case_responsibility_of_advocate-general .

:concept_directory-code_subject_of_dossier
        a                   owl:ObjectProperty ;
        rdfs:domain         :concept_directory-code ;
        rdfs:label          "Directory code concept is subject of a dossier" ;
        rdfs:range          :dossier ;
        rdfs:subPropertyOf  :subject_of ;
        owl:inverseOf       :dossier_is_about_concept_directory-code .

:recommendation_date_transposition
        a                   owl:DatatypeProperty ;
        rdfs:comment        "Date of transposition applicable to recommendation; can contain multiple values as different parts of a dirctive can be implemented by various pieces of national legislation, coming with different dates (TP_DATE). TP_COMMENT is mixed content, coded with fd_361. Relevant for legal analysis: true." ;
        rdfs:domain         :recommendation ;
        rdfs:label          "Date of transposition of a recommendation" ;
        rdfs:range          xsd:date ;
        rdfs:subPropertyOf  :date_transposition .

:resource_legal_application_extended_by_resource_legal
        a                   owl:ObjectProperty ;
        rdfs:comment        "Relevant for legal analysis: true" ;
        rdfs:domain         :resource_legal ;
        rdfs:label          "Legal resource has application extended by legal resource" ;
        rdfs:range          :resource_legal ;
        rdfs:subPropertyOf  :application_extended_by ;
        owl:inverseOf       :resource_legal_extends_application_resource_legal .

:initiating  a      owl:DatatypeProperty ;
        rdfs:label  "Initiating" .

:associated_to  a   owl:ObjectProperty ;
        rdfs:label  "Associated to" .

:manifestation_distribution_byte_size
        a                   owl:DatatypeProperty ;
        rdfs:comment        "This property contains the size of a distribution in bytes" ;
        rdfs:domain         :manifestation_distribution ;
        rdfs:label          "Distribution byte size" ;
        rdfs:range          xsd:string ;
        rdfs:subPropertyOf  :byte_size .

:target_audience_belongs_to_publication_general
        a                   owl:ObjectProperty ;
        rdfs:domain         :target_audience ;
        rdfs:label          "Target audience belongs to general publication" ;
        rdfs:range          :publication_general ;
        rdfs:subPropertyOf  :belongs_to ;
        owl:inverseOf       :publication_general_has_target_audience .

:dossier_mandatory_information_provided_by_work
        a              owl:ObjectProperty ;
        rdfs:comment   "dossier mandatory information provided by work" ;
        rdfs:domain    :dossier ;
        rdfs:label     "dossier mandatory information provided by work" ;
        rdfs:range     :work ;
        owl:inverseOf  :work_provides_mandatory_information_to_dossier .

:suspends  a        owl:ObjectProperty ;
        rdfs:label  "Suspends" .

:agreement_other  a      owl:Class ;
        rdfs:comment     "Other type of acts (subsector X of sector 2 in Eur-Lex)" ;
        rdfs:label       "Other agreement" ;
        rdfs:subClassOf  :agreement_international .

:work_dataset_has_frequency_publication_frequency
        a                   owl:ObjectProperty ;
        rdfs:comment        "This property refers to the frequency at which dataset is updated" ;
        rdfs:domain         :work_dataset ;
        rdfs:label          "Dataset frequency" ;
        rdfs:range          :publication_frequency ;
        rdfs:subPropertyOf  :has_frequency ;
        owl:inverseOf       :publication_frequency_is_frequency_of_work_dataset .

:title_alternative  a       owl:DatatypeProperty ;
        rdfs:label          "Title alternative" ;
        rdfs:subPropertyOf  :title .

:ATTO_FD_040  a              owl:Class ;
        rdfs:label           "FD_040 ATTO table" ;
        rdfs:subClassOf      skos:Concept ;
        owl:equivalentClass  [ a               owl:Restriction ;
                               owl:hasValue    <http://publications.europa.eu/resource/authority/fd_040> ;
                               owl:onProperty  skos:inScheme
                             ] .

:part_of  a         owl:ObjectProperty ;
        rdfs:label  "Part of" .

:clause_legal  a         owl:Class ;
        rdfs:comment     "A close in a legal document. Created to have correspondance to the subdivision NAL" ;
        rdfs:label       "Clause" ;
        rdfs:subClassOf  :subdivision .

:event_case_framework_procedural_has_nature_concept_court_procedure
        a                   owl:ObjectProperty ;
        rdfs:comment        "Case event has a procedural framework with a given nature. Codes taken from the table \"Procédures juridictionelles\"" ;
        rdfs:domain         :event_case ;
        rdfs:label          "Case event has a procedural framework with a given nature" ;
        rdfs:range          :concept_court_procedure ;
        rdfs:subPropertyOf  :framework_procedural_has_nature .

:manifestation_identifier
        a                   owl:DatatypeProperty ;
        rdfs:comment        "Relevant for legal analysis: true. identifier of this manifestation. mapped from 035 $a. Relevant for legal analysis: true" ;
        rdfs:domain         :manifestation ;
        rdfs:label          "Manifestation identifier" ;
        rdfs:range          xsd:string ;
        rdfs:subPropertyOf  :identifier .

:extends_application  a  owl:ObjectProperty ;
        rdfs:label  "Extends application" .

:work_contains_article_legal
        a                   owl:ObjectProperty ;
        rdfs:comment        "The legal article of this work" ;
        rdfs:domain         :work ;
        rdfs:label          "Work contains article (legal)" ;
        rdfs:range          :article_legal ;
        rdfs:subPropertyOf  :work_contains_subdivision , :contains .

:resource_legal_implements_resource_legal
        a                   owl:ObjectProperty ;
        rdfs:comment        "Relevant for legal analysis: true" ;
        rdfs:domain         :resource_legal ;
        rdfs:label          "Legal resource implements legal resource" ;
        rdfs:range          :resource_legal ;
        rdfs:subPropertyOf  :implements ;
        owl:inverseOf       :resource_legal_implemented_by_resource_legal .

<http://publications.europa.eu/resource/authority/fd_406>
        a       owl:NamedIndividual .

:event_legal_basis_legal
        a                   owl:DatatypeProperty ;
        rdfs:comment        "DEPRECATED, Link to a legal basis that cannot be automatically translated into a link to the corresponding work. Relevant for legal analysis: true." ;
        rdfs:domain         :event_legal ;
        rdfs:label          "Legal basis of legal event" ;
        rdfs:range          xsd:string ;
        rdfs:subPropertyOf  :basis_legal ;
        owl:deprecated      true .

:transliterated_attention
        a           owl:DatatypeProperty ;
        rdfs:label  "Transliterated attention" .

:date_publication  a  owl:DatatypeProperty ;
        rdfs:comment  "PD (type as annotation)" ;
        rdfs:label    "Date publication" .

:act_other_cor  a        owl:Class ;
        rdfs:comment     "29 Committee of the Regions' other acts (5XR)" ;
        rdfs:label       "Committee of the Regions' other act" ;
        rdfs:subClassOf  :act_preparatory_cor ;
        rdfs:subClassOf  [ a                   owl:Restriction ;
                           owl:maxCardinality  "1"^^xsd:nonNegativeInteger ;
                           owl:onProperty      :act_other_cor_number_session
                         ] .

:resource_legal_repeals_resource_legal
        a                   owl:ObjectProperty ;
        rdfs:comment        "This property points to act that is repealed. Relevant for legal analysis: true" ;
        rdfs:domain         :resource_legal ;
        rdfs:label          "Legal resource repeals legal resource" ;
        rdfs:range          :resource_legal ;
        rdfs:subPropertyOf  :repeals ;
        owl:inverseOf       :resource_legal_repealed_by_resource_legal .

:container_case-law_id_numpub
        a                   owl:DatatypeProperty ;
        rdfs:comment        "Numpub" ;
        rdfs:domain         :container_case-law ;
        rdfs:label          "Numpub" ;
        rdfs:range          xsd:string ;
        rdfs:subPropertyOf  :id_numpub .

:point  a                owl:Class ;
        rdfs:label       "Point" ;
        rdfs:subClassOf  :subdivision .

:resource_legal_amendment_proposed_by_resource_legal
        a                   owl:ObjectProperty ;
        rdfs:comment        "Calculated. Relevant for legal analysis: true." ;
        rdfs:domain         :resource_legal ;
        rdfs:label          "Legal resource has amendment proposed by legal resource" ;
        rdfs:range          :resource_legal ;
        rdfs:subPropertyOf  :amendment_proposed_by ;
        owl:inverseOf       :resource_legal_proposes_to_amend_resource_legal .

:case_court_identifier_extension_number
        a                   owl:DatatypeProperty ;
        rdfs:comment        "Number of the extension of the identifier in the case identifier, needed to make the identifier unique in some cases. per default 1, to be discussed if still needed" ;
        rdfs:domain         :case_court ;
        rdfs:label          "Number of the identifier of the extension in the case identifier" ;
        rdfs:range          xsd:positiveInteger ;
        rdfs:subPropertyOf  :identifier_extension_number .

:work_associated_to_work
        a              owl:ObjectProperty ;
        rdfs:domain    :work ;
        rdfs:label     "Work associated to work" ;
        rdfs:range     :work ;
        owl:inverseOf  :work_associates_work .

:case_court_reexamines_case-law
        a                   owl:ObjectProperty ;
        rdfs:domain         :case_court ;
        rdfs:label          "Case reexamines an existing case law document" ;
        rdfs:range          :case-law ;
        rdfs:subPropertyOf  :reexamines .

:act_consolidated_layer_max_version
        a                   owl:DatatypeProperty ;
        rdfs:comment        "Positive integer indicating how many versions are received for this specific layer/dateof activation" ;
        rdfs:domain         :act_consolidated ;
        rdfs:label          "Act consolidated layer max version" ;
        rdfs:range          xsd:positiveInteger ;
        rdfs:subPropertyOf  :layer .

:mandatorily-consults
        a           owl:ObjectProperty ;
        rdfs:label  "Mandatorily consults" .

:xml-schema-definition_link_type
        a           owl:DatatypeProperty ;
        rdfs:label  "Xml schema definition link type" .

:joined_to  a       owl:ObjectProperty ;
        rdfs:label  "Joined to" .

:case-status  a              owl:Class ;
        rdfs:comment         "Values currently used in the Court schema: ENC, CLOT, SUSP, DESIST Traced in MDR-1938" ;
        rdfs:label           "Concept representing the status of a court case" ;
        rdfs:subClassOf      skos:Concept , :concept_decoding ;
        owl:equivalentClass  [ a               owl:Restriction ;
                               owl:hasValue    <http://publications.europa.eu/resource/authority/case-status> ;
                               owl:onProperty  skos:inScheme
                             ] .

:manifestation_is_logical_successor_manifestation
        a                   owl:ObjectProperty ;
        rdfs:comment        "manifestation succeeds another manifestation" ;
        rdfs:domain         :manifestation ;
        rdfs:label          "Manifestation is logical successor of manifestation" ;
        rdfs:range          :manifestation ;
        rdfs:subPropertyOf  :is_logical_successor .

:implicitly_repealed_by
        a           owl:ObjectProperty ;
        rdfs:label  "Implicitly repealed by" .

:procurement_public_transliterated_contact-point
        a                   owl:DatatypeProperty ;
        rdfs:domain         :procurement_public ;
        rdfs:label          "Procurement public transliterated contact point" ;
        rdfs:range          xsd:string ;
        rdfs:subPropertyOf  :transliterated_contact-point .

:case-law_requested_by_agent
        a                   owl:ObjectProperty ;
        rdfs:comment        "This lists the applying party in Court proceeding or party lodging the appeal (institutions, bodies, Member States, companies, individuals). Currently coded with FD_Table_110" ;
        rdfs:domain         :case-law ;
        rdfs:label          "Case law requested by agent" ;
        rdfs:range          :agent ;
        rdfs:subPropertyOf  :requested_by ;
        owl:inverseOf       :agent_requests_case-law .

:term_parliamentary  a  owl:DatatypeProperty ;
        rdfs:comment  "LG" ;
        rdfs:label    "Term parliamentary" .

:datetime_request  a  owl:DatatypeProperty ;
        rdfs:label  "Datetime request" .

:resource_legal_adopts_resource_legal
        a                   owl:ObjectProperty ;
        rdfs:comment        "This points to proposal or draft of the legal act. Relevant for legal analysis: true" ;
        rdfs:domain         :resource_legal ;
        rdfs:label          "Legal resource adopts legal resource" ;
        rdfs:range          :resource_legal ;
        rdfs:subPropertyOf  :adopts ;
        owl:inverseOf       :resource_legal_adopted_by_resource_legal .

:communication_cjeu_defended_by_agent
        a                   owl:ObjectProperty ;
        rdfs:comment        "This lists the defending party in Court proceeding (institutions, bodies, Member States, companies, individuals) the communication_cjeu published in OJ informs about. Currently coded with FD_Table 110. Relevant for legal analysis: true" ;
        rdfs:domain         :communication_cjeu ;
        rdfs:label          "Communication on case law defended by agent" ;
        rdfs:range          :agent ;
        rdfs:subPropertyOf  :defended_by ;
        owl:inverseOf       :agent_defends_in_communication_cjeu .

:resource_legal_partially_referred_to_resource_legal
        a                   owl:ObjectProperty ;
        rdfs:comment        "Calculated. Relevant for legal analysis: true." ;
        rdfs:domain         :resource_legal ;
        rdfs:label          "Legal resource is partially referred to by legal resource" ;
        rdfs:range          :resource_legal ;
        rdfs:subPropertyOf  :partially_referred_to ;
        owl:inverseOf       :resource_legal_partially_refers_to_resource_legal .

:resource_legal_partially_adopts_resource_legal
        a                   owl:ObjectProperty ;
        rdfs:comment        "This points to proposal or draft of the legal act. Relevant for legal analysis: true" ;
        rdfs:domain         :resource_legal ;
        rdfs:label          "Legal resource partially adopts legal resource" ;
        rdfs:range          :resource_legal ;
        rdfs:subPropertyOf  :partially_adopts ;
        owl:inverseOf       :resource_legal_partially_adopted_by_resource_legal .

:meeting_doc_council  a  owl:Class ;
        rdfs:comment     "The majority of these documents are related to Council meetings (minutes, list of items, ...), where resource_legal_type = none, resource_legal_id_sector = 5, work_created_by_agent = CONSIL, work_has_resource-type = (VOTING_RES, NOTE)" ;
        rdfs:label       "Council meeting document" ;
        rdfs:subClassOf  :act_preparatory_council .

:manifestation_print_reference_title
        a                   owl:DatatypeProperty ;
        rdfs:comment        "DEPRECATED, Title of the print manifestation that is referenced. e.g. Débats du PE (éd. française) or Verhandlungen des EP (deutsche Ausgabe). Use manifestion_title" ;
        rdfs:domain         :manifestation_print_reference ;
        rdfs:label          "Title" ;
        rdfs:range          rdfs:Literal ;
        rdfs:subPropertyOf  :title , :manifestation_title ;
        owl:deprecated      true .

:case-law_reexamined_by_case_court
        a                   owl:ObjectProperty ;
        rdfs:comment        "This property points to Court decision quoted in the operative part of Court decisions" ;
        rdfs:domain         :case-law ;
        rdfs:label          "Case law reexamined by a new court case" ;
        rdfs:range          :case_court ;
        rdfs:subPropertyOf  :reexamined_by ;
        owl:inverseOf       :case_court_reexamins_case-law .

:directive_implementing
        a                owl:Class ;
        rdfs:comment     "24 Implementing directives (DTS=3 AND FM=DIRIMP)" ;
        rdfs:label       "Implementing directive" ;
        rdfs:subClassOf  :legislation_secondary .

:authority_local  a      owl:Class ;
        rdfs:comment     "Local authority / town. The list of instances of this class is provided by the Metadata Registry" ;
        rdfs:label       "Local authority" ;
        rdfs:subClassOf  :unit_administrative .

:operative_part  a  owl:DatatypeProperty ;
        rdfs:label  "Operative part" .

:explained_by  a    owl:ObjectProperty ;
        rdfs:label  "Explained by" .

:event_legal_taken_over_person
        a                   owl:ObjectProperty ;
        rdfs:comment        "Relevant for legal analysis: true. This legal event is taken over by a given person. The XML contains two persons, the person handing over and the person taking over. This is the second of the two. Person role: Taking over. Relevant for legal analysis: true" ;
        rdfs:domain         :event_legal ;
        rdfs:label          "Legal event taken over by person" ;
        rdfs:range          :person ;
        rdfs:subPropertyOf  :taken_over ;
        owl:inverseOf       :person_takes_over_event_legal .

:notice_prior-information_main-activities_label
        a                   owl:DatatypeProperty ;
        rdfs:domain         :notice_prior-information ;
        rdfs:label          "Label of main activities" ;
        rdfs:range          xsd:string ;
        rdfs:subPropertyOf  :main-activities_label .

:expression_belongs_to_work
        a                   owl:ObjectProperty ;
        rdfs:comment        "Expression of a given work. Implicit in the current notice structure. Relevant for legal analysis: true." ;
        rdfs:domain         :expression ;
        rdfs:label          "Expression belongs to a work" ;
        rdfs:range          :work ;
        rdfs:subPropertyOf  :belongs_to ;
        owl:inverseOf       :work_has_expression .

:amendment_proposed_by
        a           owl:ObjectProperty ;
        rdfs:label  "Amendment proposed by" .

:group_parliamentary_asks_question_parliamentary
        a                   owl:ObjectProperty ;
        rdfs:comment        "The question is asked by a member of a given parliamentary group" ;
        rdfs:domain         :group_parliamentary ;
        rdfs:label          "Parliamentary group asks a parliamentary question" ;
        rdfs:range          :question_parliamentary ;
        rdfs:subPropertyOf  :asks ;
        owl:inverseOf       :question_parliamentary_asked_by_group_parliamentary .

:national-judgement  a  owl:DatatypeProperty ;
        rdfs:label  "National judgement" .

:summary_legislation_eu_obsolete
        a                   owl:DatatypeProperty ;
        rdfs:comment        "An summary is considered obsolete if its basic act (= summarizes) is out of force. Is this summary obsolete?" ;
        rdfs:domain         :summary_legislation_eu ;
        rdfs:label          "Summary obsolete?" ;
        rdfs:range          xsd:boolean ;
        rdfs:subPropertyOf  :obsolete .

<http://publications.europa.eu/resource/authority/fd_401>
        a       owl:NamedIndividual .

<http://publications.europa.eu/resource/authority/fd_395>
        a       owl:NamedIndividual .

:dossier_is_logical_successor_of_dossier
        a                   owl:ObjectProperty ;
        rdfs:comment        "This property associates an instance of a dossier which logically continues the content of an other instance of dossier with the latter (in analogy to FRBRoo)" ;
        rdfs:domain         :dossier ;
        rdfs:label          "Dossier is logical successor of dossier" ;
        rdfs:range          :dossier ;
        rdfs:subPropertyOf  :is_logical_successor_of .

:reference_act_consolidated
        a           owl:DatatypeProperty ;
        rdfs:label  "Reference act consolidated" .

:expression_publication_general_date_processing
        a                   owl:DatatypeProperty ;
        rdfs:comment        "Date of processing (Record identifier)" ;
        rdfs:domain         :expression_publication_general ;
        rdfs:label          "Processing date" ;
        rdfs:range          xsd:date ;
        rdfs:subPropertyOf  :date_processing .

:used_by_accompanying_material
        a                   owl:ObjectProperty ;
        rdfs:label          "Used by accompanying material" ;
        rdfs:subPropertyOf  :used_by .

:legislative-package  a  owl:Class ;
        rdfs:comment     "Legislative package" ;
        rdfs:label       "Legislative package" ;
        rdfs:subClassOf  :dossier .

:work_dataset_asset_content
        a            owl:DatatypeProperty ;
        rdfs:domain  :work_dataset ;
        rdfs:label   "Work dataset asset content" ;
        rdfs:range   xsd:anyURI .

:decision_service_associated
        a                   owl:DatatypeProperty ;
        rdfs:comment        "This field indicates the Commission DG or DGs co-responsible for drafting of an act. DEPRECATED, In the instance data, the property is planned to be replaced with cdm:resource_legal_service_associated at beginning 2019. When this is done this property the property will be removed from CDM. Relevant for legal analysis: true" ;
        rdfs:domain         :decision ;
        rdfs:label          "Service associated" ;
        rdfs:range          xsd:string ;
        rdfs:subPropertyOf  :service_associated , :resource_legal_service_associated ;
        owl:deprecated      true .

:institution_validates_summary_legislation_eu
        a                   owl:ObjectProperty ;
        rdfs:domain         :institution ;
        rdfs:label          "Institution validates a summary of EU legislation" ;
        rdfs:range          :summary_legislation_eu ;
        rdfs:subPropertyOf  :validates ;
        owl:inverseOf       :summary_legislation_eu_validated_by_institution .

:alinea_part_of_work  a     owl:ObjectProperty ;
        rdfs:comment        "This property associates an instance of a work with an instance of ALINEA that forms part of it." ;
        rdfs:domain         :alinea ;
        rdfs:label          "Alinea part of work" ;
        rdfs:range          :work ;
        rdfs:subPropertyOf  :subdivision_part_of_work , :part_of ;
        owl:inverseOf       :work_contains_alinea .

:decision_internal_ep
        a                owl:Class ;
        rdfs:label       "European Parliament internal decision" ;
        rdfs:subClassOf  :act_preparatory_ep ;
        rdfs:subClassOf  [ a                owl:Restriction ;
                           owl:cardinality  "1"^^xsd:nonNegativeInteger ;
                           owl:onProperty   :decision_internal_ep_term_parliamentary
                         ] .

:institution_jointly-responsible_for_event
        a             owl:ObjectProperty ;
        rdfs:comment  "An institution is responsible for an event together with other agent(s)" ;
        rdfs:domain   :institution ;
        rdfs:label    "Institution jointly responsible for event" ;
        rdfs:range    :event .

:communicates_on  a  owl:ObjectProperty ;
        rdfs:label  "Communicates on" .

:corrected_by  a    owl:ObjectProperty ;
        rdfs:label  "Corrected by" .

:extent_illustration  a  owl:DatatypeProperty ;
        rdfs:label  "Extent illustration" .

<http://publications.europa.eu/resource/authority/corporate-body>
        a       owl:NamedIndividual .

:concept_op_theme_subject_of_publication_general
        a              owl:ObjectProperty ;
        rdfs:comment   "A concept representing an OP theme as subject of a general publication" ;
        rdfs:domain    :concept_op_theme ;
        rdfs:label     "Concept representing an OP theme as subject of a general publication" ;
        rdfs:range     :publication_general ;
        owl:inverseOf  :publication_general_is_about_concept_op_theme .

:dossier_consults_agent
        a                   owl:ObjectProperty ;
        rdfs:comment        "This dossier consults a given consultative agent. mapped from /ns4:ec_transmission_request/transmission/workflow/extension/ns3:workflow_agent , subproperty of involves" ;
        rdfs:domain         :dossier ;
        rdfs:label          "Dossier consults agent" ;
        rdfs:range          :agent ;
        rdfs:subPropertyOf  :dossier_involves_agent , :consults .

:manifestation_case-law_operative_part
        a                   owl:DatatypeProperty ;
        rdfs:comment        "Operative part associated with this judgement. Sector 6 Text Index Field DI" ;
        rdfs:domain         :manifestation_case-law ;
        rdfs:label          "Operative part of court decision" ;
        rdfs:range          rdf:XMLLiteral ;
        rdfs:subPropertyOf  :operative_part .

:opinion_other_cor  a    owl:Class ;
        rdfs:comment     "291 Committee of the Regions' other opinions (5IR)" ;
        rdfs:label       "Committee of the Regions' other opinion" ;
        rdfs:subClassOf  :act_preparatory_cor ;
        rdfs:subClassOf  [ a                   owl:Restriction ;
                           owl:maxCardinality  "1"^^xsd:nonNegativeInteger ;
                           owl:onProperty      :opinion_other_cor_number_session
                         ] .

:work_dataset_has_theme_concept_theme_dataset
        a                   owl:ObjectProperty ;
        rdfs:comment        "This property refers to the theme of the dataset" ;
        rdfs:domain         :work_dataset ;
        rdfs:label          "Dataset theme" ;
        rdfs:range          :concept_theme_dataset ;
        rdfs:subPropertyOf  :has_theme .

:part_of_acquis  a  owl:ObjectProperty ;
        rdfs:label  "Part of acquis" .

:institution_addressed_by_event
        a             owl:ObjectProperty ;
        rdfs:comment  "An institution which is being addressed by execution of an event" ;
        rdfs:domain   :institution ;
        rdfs:label    "Institution addressed by event" ;
        rdfs:range    :event .

:event_has_type_concept_type_event
        a                   owl:ObjectProperty ;
        rdfs:comment        "Event has a certain type of event. Relevant for legal analysis: true." ;
        rdfs:domain         :event ;
        rdfs:label          "Event has type concept type event" ;
        rdfs:range          :concept_type_event ;
        rdfs:subPropertyOf  :has_type .

:language  a                 owl:Class ;
        rdfs:comment         "The list of languages is provided by a common authority table in scheme cat:languages or cat:multilingual" ;
        rdfs:label           "Language" ;
        rdfs:subClassOf      skos:Concept ;
        owl:equivalentClass  [ a               owl:Restriction ;
                               owl:hasValue    <http://publications.europa.eu/resource/authority/language> ;
                               owl:onProperty  skos:inScheme
                             ] .

:resource_legal_eea  a      owl:DatatypeProperty ;
        rdfs:comment        "Legal act relevant for European Economic Area. Added in the context of IMMC2CDM-OJ. Relevant for legal analysis: true" ;
        rdfs:domain         :resource_legal ;
        rdfs:label          "Legal resource European Economic Area" ;
        rdfs:range          xsd:boolean ;
        rdfs:subPropertyOf  :eea .

:question_written  a     owl:Class ;
        rdfs:comment     "Written parliamentary question (= subsector E sector 9 in EUR-Lex, 89929 notices on 2010-07-27)" ;
        rdfs:label       "Written question" ;
        rdfs:subClassOf  :question_parliamentary .

:procedure_number  a  owl:DatatypeProperty ;
        rdfs:label  "Procedure number" .

:agent_contributes_work
        a              owl:ObjectProperty ;
        rdfs:comment   "Agent acts as a contributor of a work" ;
        rdfs:domain    :agent ;
        rdfs:label     "Agent is a contributor of a work" ;
        rdfs:range     :work ;
        owl:inverseOf  :work_contributed_to_by_agent .

:manifestation_published_by_agent
        a             owl:ObjectProperty ;
        rdfs:comment  "Manifestation was published by an agent entity" ;
        rdfs:domain   :manifestation ;
        rdfs:label    "Manifestation published by agent" ;
        rdfs:range    :agent .

:summary_legislation_eu_summarizes_act_consolidated
        a                   owl:ObjectProperty ;
        rdfs:comment        "A legislative summarizes an act from consolidated legislation" ;
        rdfs:domain         :summary_legislation_eu ;
        rdfs:label          "Legislative summary summarizes consolidated act" ;
        rdfs:range          :act_consolidated ;
        rdfs:subPropertyOf  :summary_legislation_eu_summarizes_resource_legal ;
        owl:inverseOf       :act_consolidated_summarized_by_summary_legislation_eu .

:date_dispatch  a           owl:DatatypeProperty ;
        rdfs:label          "Date dispatch" ;
        rdfs:range          xsd:date ;
        rdfs:subPropertyOf  :date .

:partially_adopted_by
        a           owl:ObjectProperty ;
        rdfs:label  "Partially adopted by" .

:document_com_other_ec_service_associated
        a                   owl:DatatypeProperty ;
        rdfs:comment        "This field indicates the Commission DG or DGs co-responsible for drafting of an act. DEPRECATED, In the instance data, the property is planned to be replaced with cdm:resource_legal_service_associated at beginning 2019. When this is done this property the property will be removed from CDM. Relevant for legal analysis: true" ;
        rdfs:domain         :document_com_other_ec ;
        rdfs:label          "Service associated" ;
        rdfs:range          xsd:string ;
        rdfs:subPropertyOf  :service_associated , :resource_legal_service_associated ;
        owl:deprecated      true .

<http://publications.europa.eu/resource/authority/country>
        a       owl:NamedIndividual .

:case-law_amends_resource_legal
        a                   owl:ObjectProperty ;
        rdfs:comment        "This points to the legal act that is amended by a case law. Relevant for legal analysis: true" ;
        rdfs:domain         :case-law ;
        rdfs:label          "Case law amends legal resource" ;
        rdfs:range          :resource_legal ;
        rdfs:subPropertyOf  :amends ;
        owl:inverseOf       :resource_legal_amended_by_case-law .

:signature_digital_signs_manifestation
        a                   owl:ObjectProperty ;
        rdfs:comment        "This digital signature signs the following manifestation" ;
        rdfs:domain         :signature_digital ;
        rdfs:label          "Digital signature signs manifestation" ;
        rdfs:range          :manifestation ;
        rdfs:subPropertyOf  :signs ;
        owl:inverseOf       :manifestation_signed_by_signature_digital .

:concept_directory-code_subject_of_summary_legislation_eu
        a              owl:ObjectProperty ;
        rdfs:comment   "A concept from the directory of EU legal acts is one of the subjects of a legislative summary" ;
        rdfs:domain    :concept_directory-code ;
        rdfs:label     "Directory code concept is subject of a legislative summary" ;
        rdfs:range     :summary_legislation_eu ;
        owl:inverseOf  :summary_legislation_eu_is_about_concept_directory-code .

:person_reports_on_act_other_cor
        a                   owl:ObjectProperty ;
        rdfs:domain         :person ;
        rdfs:label          "Person reports on act_other_cor" ;
        rdfs:range          :act_other_cor ;
        rdfs:subPropertyOf  :reports_on .

:dossier_comment  a         owl:DatatypeProperty ;
        rdfs:comment        "Comment on the dossier as a whole. Relevant for legal analysis: true." ;
        rdfs:domain         :dossier ;
        rdfs:label          "Comment on dossier" ;
        rdfs:range          rdf:PlainLiteral ;
        rdfs:subPropertyOf  :comment .

:work_part_of_work  a       owl:ObjectProperty ;
        rdfs:comment        "The work is part of another work (e.g. an article in a volume of proceedings or a split COM that is part of a multipart COM). In theory also LNK_CES, LNK_CDR, but those have 0% of usage." ;
        rdfs:domain         :work ;
        rdfs:label          "Work is part of work" ;
        rdfs:range          :work ;
        rdfs:subPropertyOf  :part_of ;
        owl:inverseOf       :work_contains_work .

:expression_manifested_by_manifestation
        a                   owl:ObjectProperty ;
        rdfs:comment        "Implicit in the current notice structure" ;
        rdfs:domain         :expression ;
        rdfs:label          "Expression is manifested by manifestation" ;
        rdfs:range          :manifestation ;
        rdfs:subPropertyOf  :manifested_by ;
        owl:inverseOf       :manifestation_manifests_expression .

:ATTO_FD_380  a              owl:Class ;
        rdfs:label           "FD_380 ATTO table" ;
        rdfs:subClassOf      skos:Concept ;
        owl:equivalentClass  [ a               owl:Restriction ;
                               owl:hasValue    <http://publications.europa.eu/resource/authority/fd_380> ;
                               owl:onProperty  skos:inScheme
                             ] .

:report_eca  a           owl:Class ;
        rdfs:comment     "215 Court of Auditors reports, usually the annual report (5TA)" ;
        rdfs:label       "Court of Auditors report" ;
        rdfs:subClassOf  :act_preparatory_eca .

:concept_case_court_domain
        a                owl:Class ;
        rdfs:label       "Concept representing the domain of a court case" ;
        rdfs:subClassOf  :concept_decoding .

:resource_legal_renders_obsolete_resource_legal
        a                   owl:ObjectProperty ;
        rdfs:comment        "Relevant for legal analysis: true" ;
        rdfs:domain         :resource_legal ;
        rdfs:label          "Legal resource renders obsolete legal resource" ;
        rdfs:range          :resource_legal ;
        rdfs:subPropertyOf  :renders_obsolete ;
        owl:inverseOf       :resource_legal_rendered_obsolete_by_resource_legal .

:affects  a           owl:ObjectProperty ;
        rdfs:comment  "Super property (as inverse of cdm#affected_by)" ;
        rdfs:label    "Affects" .

:dossier_adopted-proposal
        a                   owl:DatatypeProperty ;
        rdfs:comment        "Adopted proposal. Relevant for legal analysis: true." ;
        rdfs:domain         :dossier ;
        rdfs:label          "Dossier is already adopted?" ;
        rdfs:range          xsd:boolean ;
        rdfs:subPropertyOf  :adopted-proposal .

:demed_reference  a  owl:DatatypeProperty ;
        rdfs:label  "Demed reference" .

:ATTO_FD_301  a              owl:Class ;
        rdfs:label           "FD_301 ATTO table" ;
        rdfs:subClassOf      skos:Concept ;
        owl:equivalentClass  [ a               owl:Restriction ;
                               owl:hasValue    <http://publications.europa.eu/resource/authority/fd_301> ;
                               owl:onProperty  skos:inScheme
                             ] .

:container_work  a       owl:Class ;
        rdfs:comment     "Works whose essence is to enhance or add value to expressions from one or more other works without altering them, by the selection, arrangement and or addition of features of different form (FRBRoo)" ;
        rdfs:label       "Container work" ;
        rdfs:subClassOf  :work .

:resource_legal_establishes_failure_to_fulfill_obligation_requested_by_case-law
        a                   owl:ObjectProperty ;
        rdfs:comment        "553 cases (2012-07-31). Example: 62007CN0475: \"request to establish failure to fulfil an obligation 32003L0096 Article 21.5\". Relevant for legal analysis: true." ;
        rdfs:domain         :resource_legal ;
        rdfs:label          "Legal resource establishes failure to fulfill obligation" ;
        rdfs:range          :case-law ;
        rdfs:subPropertyOf  :establishes_failure_to_fulfill_obligation_requested_by ;
        owl:inverseOf       :case-law_requests_for_failure_to_fulfill_an_obligation_for_resource_legal .

:agent_publishes_work_dataset
        a              owl:ObjectProperty ;
        rdfs:comment   "Agent acts as publisher of a dataset work" ;
        rdfs:domain    :agent ;
        rdfs:label     "Agent publishes a dataset work" ;
        rdfs:range     :work_dataset ;
        owl:inverseOf  :work_dataset_published_by_agent .

:resource_legal_associates_agreement_international
        a                   owl:ObjectProperty ;
        rdfs:comment        "Decision or regulation associates an international agreement. Relevant for legal analysis: true" ;
        rdfs:domain         :resource_legal ;
        rdfs:label          "Decision or regulation associates an international agreement" ;
        rdfs:range          :agreement_international ;
        rdfs:subPropertyOf  :associates ;
        owl:inverseOf       :agreement_international_associated_to_resource_legal .

:measure_national_implementing_reference_member-state
        a                   owl:DatatypeProperty ;
        rdfs:comment        "Reference to the NIM allocated by the member state" ;
        rdfs:domain         :measure_national_implementing ;
        rdfs:label          "Reference Member States" ;
        rdfs:range          xsd:string ;
        rdfs:subPropertyOf  :reference_member-state .

:report_case  a          owl:Class ;
        rdfs:comment     "Case report in sector 6 (6CP)" ;
        rdfs:label       "Case report" ;
        rdfs:subClassOf  :case-law .

:resolution_initiative_own_ep
        a                owl:Class ;
        rdfs:comment     "5094 Parliament own-initiative resolution (DTT=IP OR AP AND FM=OWNINI_RES)" ;
        rdfs:label       "Parliament own-initiative resolution" ;
        rdfs:subClassOf  :act_preparatory_ep .

:proposal_directive_implementing_ec
        a                owl:Class ;
        rdfs:label       "Commission proposal for an implementing directive" ;
        rdfs:subClassOf  :proposal_act , :act_preparatory_ec .

:commented_by  a    owl:ObjectProperty ;
        rdfs:label  "Commented by" .

:case-law_declares_void_resource_legal
        a                   owl:ObjectProperty ;
        rdfs:comment        "This property points to legal act quoted in the operative part of Court decisions" ;
        rdfs:domain         :case-law ;
        rdfs:label          "Case law declares void legal resource" ;
        rdfs:range          :resource_legal ;
        rdfs:subPropertyOf  :declares_void ;
        owl:inverseOf       :resource_legal_declared_void_by_case-law .

:section_oj  a      owl:DatatypeProperty ;
        rdfs:label  "Section oj" .

:interpretes_judgement
        a           owl:ObjectProperty ;
        rdfs:label  "Interpretes judgement" .

:act_body_agreement_international
        a                owl:Class ;
        rdfs:comment     "Act of body created by international agreement (subsector D of sector 2 in Eur-Lex)" ;
        rdfs:label       "Act of body created by international agreement" ;
        rdfs:subClassOf  :agreement_international .

:expression_abstract  a     owl:DatatypeProperty ;
        rdfs:comment        "Abstract of expression" ;
        rdfs:domain         :expression ;
        rdfs:label          "Abstract of expression" ;
        rdfs:range          rdf:XMLLiteral ;
        rdfs:subPropertyOf  :abstract .

:proposal_act_id_com  a     owl:DatatypeProperty ;
        rdfs:comment        "COM catalogue number. Relevant for legal analysis: true." ;
        rdfs:domain         :proposal_act ;
        rdfs:label          "COM identifier for proposals" ;
        rdfs:range          xsd:string ;
        rdfs:subPropertyOf  :id_com .

:role-qualifier  a           owl:Class ;
        rdfs:comment         "Values currently used in the Court schema: INDIV, TC, IO, MS, CI, STAFF Traced in MDR-1937" ;
        rdfs:label           "Concept representing possible role qualifiers" ;
        rdfs:subClassOf      skos:Concept , :concept_decoding , :agent ;
        owl:equivalentClass  [ a               owl:Restriction ;
                               owl:hasValue    <http://publications.europa.eu/resource/authority/role-qualifier> ;
                               owl:onProperty  skos:inScheme
                             ] .

:opinion_eesc  a         owl:Class ;
        rdfs:comment     "European Economic and Social Committee opinions, usually on non-obligatory consultation on draft legislation or communications (5AC)" ;
        rdfs:label       "European Economic and Social Committee opinion" ;
        rdfs:subClassOf  :act_preparatory_eesc ;
        rdfs:subClassOf  [ a                   owl:Restriction ;
                           owl:maxCardinality  "1"^^xsd:nonNegativeInteger ;
                           owl:onProperty      :opinion_eesc_number_session
                         ] .

:procurement_public_url_etendering
        a                   owl:DatatypeProperty ;
        rdfs:domain         :procurement_public ;
        rdfs:label          "eTendering URL" ;
        rdfs:range          xsd:anyURI ;
        rdfs:subPropertyOf  :url_etendering .

cmr:lang  a                 owl:DatatypeProperty ;
        rdfs:comment        "May be applied on several objects. When applied on the cellar URI of an expression, it indicated the used language of that expression."@en ;
        rdfs:label          "CMR used language"@en ;
        rdfs:range          xsd:language ;
        rdfs:subPropertyOf  owl:topDataProperty .

:replaced_by  a     owl:ObjectProperty ;
        rdfs:label  "Replaced by" .

:has_feature  a     owl:ObjectProperty ;
        rdfs:label  "Has feature" .

:resource_legal_signatory_function
        a                   owl:DatatypeProperty ;
        rdfs:comment        "Legal resource signatory function. Added in the context of IMMC2CDM-OJ. Relevant for legal analysis: true." ;
        rdfs:domain         :resource_legal ;
        rdfs:label          "Function of first signatory of the legal resource" ;
        rdfs:range          xsd:string ;
        rdfs:subPropertyOf  :signatory_function .

:resource_legal_application_deferred_by_case-law
        a                   owl:ObjectProperty ;
        rdfs:comment        "Calculated. Relevant for legal analysis: true." ;
        rdfs:domain         :resource_legal ;
        rdfs:label          "Application of legal resource deferred by" ;
        rdfs:range          :case-law ;
        rdfs:subPropertyOf  :application_deferred_by .

:version  a         owl:DatatypeProperty ;
        rdfs:label  "Version" .

:requests_establishment_of_failure_of_obligation
        a           owl:ObjectProperty ;
        rdfs:label  "Requests establishment of failure of obligation" .

:event_case_framework_procedural_sequential-number_nature
        a                   owl:DatatypeProperty ;
        rdfs:comment        "The sequential number related to the nature in the identifier of the procedural framework of the case event" ;
        rdfs:domain         :event_case ;
        rdfs:label          "Sequential number related to the nature in the identifier of the procedural framework" ;
        rdfs:range          xsd:positiveInteger ;
        rdfs:subPropertyOf  :framework_procedural_sequential-number_nature .

:corrects_judgement  a  owl:ObjectProperty ;
        rdfs:label  "Corrects judgement" .

<http://publications.europa.eu/resource/authority/multilingual>
        a       owl:NamedIndividual .

:is_about  a        owl:ObjectProperty ;
        rdfs:label  "Is about" .

:archive_package_eesc_document_part_of_archive_package_eesc
        a                   owl:ObjectProperty ;
        rdfs:domain         :archive_package_eesc ;
        rdfs:label          "Archive package document from the European Economic and Social Committee is part of archive package." ;
        rdfs:range          :archive_package_eesc_document ;
        rdfs:subPropertyOf  :archive_package_document_part_of_archive_package .

:institution_informed_by_event
        a            owl:ObjectProperty ;
        rdfs:domain  :institution ;
        rdfs:label   "Institution informed by event" ;
        rdfs:range   :event .

:official-journal-act_year
        a                   owl:DatatypeProperty ;
        rdfs:comment        "The year of publication of the Official Journal act; corresponds to the year part of the publication date; the year information makes part of the Official Journal act identification" ;
        rdfs:domain         :official-journal-act ;
        rdfs:label          "Official Journal act year" ;
        rdfs:range          xsd:gYear ;
        rdfs:subPropertyOf  :year .

:regulation_delegated
        a                owl:Class ;
        rdfs:comment     "229 Delegated regulation (DTS=3 AND FM=REGDEL)" ;
        rdfs:label       "Delegated regulation" ;
        rdfs:subClassOf  :legislation_secondary .

:opinion_eesc_reported_by_person
        a                   owl:ObjectProperty ;
        rdfs:comment        "Name of the person (EP member or member of CoR or EESC) who reports on the relevant act. This property will be deprecated and replaced with work_reported_by_person. Role RAPP. Relevant for legal analysis: true" ;
        rdfs:domain         :opinion_eesc ;
        rdfs:label          "European Economic and Social Committee opinion has rapporteur" ;
        rdfs:range          :person ;
        rdfs:subPropertyOf  :work_reported_by_person ;
        owl:inverseOf       :person_reports_on_opinion_eesc .

:reference_commission
        a           owl:DatatypeProperty ;
        rdfs:label  "Reference commission" .

:proposal_directive_ec
        a                owl:Class ;
        rdfs:comment     "where its resource_legal_type = (PC or NONE), resource_legal_id_sector = 5, work_has_resource-type = (PROP_DIR, AMEND_PROP_DIR, DIR_DRAFT, DIR_DEL_DRAFT, DIR_IMPL_DRAFT, PROP_DIR_IMPL, ANNEX)" ;
        rdfs:label       "Commission proposal for a directive" ;
        rdfs:subClassOf  :proposal_act , :act_preparatory_ec .

:legislation_secondary
        a                owl:Class ;
        rdfs:comment     "Secondary legislation (= sector 3 in EUR-Lex)" ;
        rdfs:label       "Secondary legislation" ;
        rdfs:subClassOf  :resource_legal .

:assent_ceca_council  a  owl:Class ;
        rdfs:comment     "721 Council Assent ECSC (5KG)" ;
        rdfs:label       "Council Assent ECSC (CECA)" ;
        rdfs:subClassOf  :act_preparatory_council .

:manifestation_special-court-report_part_page_first
        a                   owl:DatatypeProperty ;
        rdfs:comment        "DEPRECATED, First page number of the special Court report part related to a court document. Use manifestion_print_page_first" ;
        rdfs:domain         :manifestation_special-court-report_part ;
        rdfs:label          "First page" ;
        rdfs:range          xsd:string ;
        rdfs:subPropertyOf  :page_first , :manifestation_print_page_first ;
        owl:deprecated      true .

:work_dataset_date_end
        a                   owl:DatatypeProperty ;
        rdfs:comment        "This property refers to the end of the period the dataset covers" ;
        rdfs:domain         :work_dataset ;
        rdfs:label          "Dataset end date" ;
        rdfs:range          xsd:date ;
        rdfs:subPropertyOf  :date_end .

:procurement_public_tir_code
        a                   owl:DatatypeProperty ;
        rdfs:comment        "à revoire" ;
        rdfs:domain         :procurement_public ;
        rdfs:label          "Tir code for a country" ;
        rdfs:range          xsd:string ;
        rdfs:subPropertyOf  :tir_code .

:case-law_states_failure_concerning_resource_legal
        a                   owl:ObjectProperty ;
        rdfs:comment        "This property points to legal act quoted in the operative part of Court decisions" ;
        rdfs:domain         :case-law ;
        rdfs:label          "Case law states failure concerning legal resource" ;
        rdfs:range          :resource_legal ;
        rdfs:subPropertyOf  :states_failure_concerning ;
        owl:inverseOf       :resource_legal_failure_stated_by_case-law .

:statement_assurance_eca
        a                owl:Class ;
        rdfs:comment     "Court of Auditors statements of assurance (5XA) All \"other acts\" of the Court of Auditors are statements of assurance" ;
        rdfs:label       "Court of Auditors statement of assurance" ;
        rdfs:subClassOf  :act_preparatory_eca .

:person_associated_with_event
        a                   owl:ObjectProperty ;
        rdfs:domain         :person ;
        rdfs:label          "Person is associated with event" ;
        rdfs:range          :event ;
        rdfs:subPropertyOf  :associated_with .

:manifestation_distribution_has_licence_licence_document
        a                   owl:ObjectProperty ;
        rdfs:comment        "This property refers to the licence under which the distribution is made available" ;
        rdfs:domain         :manifestation_distribution ;
        rdfs:label          "Licence" ;
        rdfs:range          :licence_document ;
        rdfs:subPropertyOf  :has_licence .

:document_com_other_ec_service_responsible
        a                   owl:DatatypeProperty ;
        rdfs:comment        "The Commission DG or DGs responsible for drafting of an act. Relevant for legal analysis: true\" DEPRECATED. In the instance data, the property is planned to be replaced with cdm:resource_legal_service_responsible at beginning 2019. When this is done this property will be removed from CDM. The Commission's DG that brought forward the proposal; to be taken from a closed list of DGs (that might be derived from the RECORD project ?). For the backlog data need to be completed. Cardinality to be restricted to 1 in the future" ;
        rdfs:domain         :document_com_other_ec ;
        rdfs:label          "Service responsible" ;
        rdfs:range          xsd:string ;
        rdfs:subPropertyOf  :service_responsible , :resource_legal_service_responsible ;
        owl:deprecated      true .

:event_legal_consults_institution
        a                   owl:ObjectProperty ;
        rdfs:comment        "Relevant for legal analysis: true. This legal event consults a given institution. Body role: Consultation. Relevant for legal analysis: true" ;
        rdfs:domain         :event_legal ;
        rdfs:label          "Legal event consults institution" ;
        rdfs:range          :institution ;
        rdfs:subPropertyOf  :consults ;
        owl:inverseOf       :institution_consulted_by_event_legal .

:version_notes  a   owl:DatatypeProperty ;
        rdfs:label  "Version notes" .

:ATTO_FD_609  a              owl:Class ;
        rdfs:label           "FD_609 ATTO table" ;
        rdfs:subClassOf      skos:Concept ;
        owl:equivalentClass  [ a               owl:Restriction ;
                               owl:hasValue    <http://publications.europa.eu/resource/authority/fd_609> ;
                               owl:onProperty  skos:inScheme
                             ] .

:case_court_has_case-status
        a                   owl:ObjectProperty ;
        rdfs:comment        "The case has a certain status (ENC, CLOT, SUSP, DESIST). Possible values in the target table ENC, CLOT, SUSP, DESIST" ;
        rdfs:domain         :case_court ;
        rdfs:label          "Case has status" ;
        rdfs:range          :case-status ;
        rdfs:subPropertyOf  :has .

:resource_legal_number_natural
        a                   owl:DatatypeProperty ;
        rdfs:comment        "Number part. e.g. 1 for decision 2014/1" ;
        rdfs:domain         :resource_legal ;
        rdfs:label          "Natural number" ;
        rdfs:range          xsd:positiveInteger ;
        rdfs:subPropertyOf  :number_natural .

:memberList  a        owl:ObjectProperty ;
        rdfs:comment  "Object property indicating on which providing th rdf:List that organizes a set of property values" ;
        rdfs:label    "Property for a sequence of values (memberlist)" ;
        rdfs:range    rdf:List .

:adopted_by  a      owl:ObjectProperty ;
        rdfs:label  "Adopted by" .

:event_legal_part_of_dossier
        a                   owl:ObjectProperty ;
        rdfs:comment        "DEPRECATED , The legal event is part of a dossier. Changed: we assume that an event belongs to exactle one dossier. Relevant for legal analysis: true." ;
        rdfs:domain         :event_legal ;
        rdfs:label          "Legal event is part of dossier" ;
        rdfs:range          :dossier ;
        rdfs:subPropertyOf  :part_of , :event_part_of_dossier ;
        owl:deprecated      true .

:implements  a      owl:ObjectProperty ;
        rdfs:label  "Implements" .

:reference-data_asset_prereleased_in_reference-data_asset_prerelease
        a                   owl:ObjectProperty ;
        rdfs:comment        "The representant of a reference data asset has a prerelease version" ;
        rdfs:domain         :reference-data_asset ;
        rdfs:label          "Reference data asset prereleased in reference data asset prerelease" ;
        rdfs:range          :reference-data_asset_prerelease ;
        rdfs:subPropertyOf  :prereleased_in ;
        owl:inverseOf       :reference-data_asset_prerelease_prereleases_reference-data_asset .

:resource_legal_implicitly_repealed_by_resource_legal
        a                   owl:ObjectProperty ;
        rdfs:comment        "Calculated. Relevant for legal analysis: true." ;
        rdfs:domain         :resource_legal ;
        rdfs:label          "Legal resource implicitly repealed by legal resource" ;
        rdfs:range          :resource_legal ;
        rdfs:subPropertyOf  :implicitly_repealed_by ;
        owl:inverseOf       :resource_legal_implicitly_repeals_resource_legal .

:first_series_historical
        a           owl:DatatypeProperty ;
        rdfs:label  "First series historical" .

:proposal_regulation_ec
        a                owl:Class ;
        rdfs:comment     "where its resource_legal_type = PC, resource_legal_id_sector = 5, work_has_resource-type = (PROP_REG, AMEND_PROP_REG, REG_DRAFT, REG_DEL_DRAFT, REG_IMPL_DRAFT, PROP_REG_IMPL, RECO_REG, ANNEX)" ;
        rdfs:label       "Commission proposal for a regulation" ;
        rdfs:subClassOf  :proposal_act , :act_preparatory_ec .

:publisher  a       owl:DatatypeProperty ;
        rdfs:label  "Publisher" .

:act_other_ep_reported_by_person
        a                   owl:ObjectProperty ;
        rdfs:comment        "Name of the person (EP member or member of CoR or EESC) who reports on the relevant act. This property will be deprecated and replaced with work_reported_by_person. Role RAPP. Relevant for legal analysis: true" ;
        rdfs:domain         :act_other_ep ;
        rdfs:label          "European Parliament other act has rapporteur" ;
        rdfs:range          :person ;
        rdfs:subPropertyOf  :work_reported_by_person ;
        dct:created         "2018-07-16T13:15:44.793+02:00"^^xsd:dateTime ;
        owl:inverseOf       :person_reports_on_act_other_ep .

:manifestation_official-journal_part_section_oj
        a                   owl:DatatypeProperty ;
        rdfs:comment        "Section of the OJ part that this legal resource was published in. Values such as \"L2\"" ;
        rdfs:domain         :manifestation_official-journal_part ;
        rdfs:label          "Section of the OJ" ;
        rdfs:range          xsd:string ;
        rdfs:subPropertyOf  :section_oj .

:consolidates  a    owl:ObjectProperty ;
        rdfs:label  "Consolidates" .

:hands_over  a      owl:ObjectProperty ;
        rdfs:label  "Hands over" .

:reexamined_by  a   owl:ObjectProperty ;
        rdfs:label  "Reexamined by" .

:procedure_internal_planned_adoption_period_date_start
        a                   owl:DatatypeProperty ;
        rdfs:comment        "Start date of the planned adoption period for this internal dossier. Information on the planned period for the public consultation.The information is always a period, so start_date must always be lower than end_date.The information is sent in all events part of the workflow Planning. Therefore the information sent in the most recent event is the most precise and has to prevail on the preceding information sent" ;
        rdfs:domain         :procedure_internal ;
        rdfs:label          "Internal procedure: Start date of the planned adoption period" ;
        rdfs:range          xsd:date ;
        rdfs:subPropertyOf  :planned_adoption_period_date_start .

:procurement_public_published_in_official-journal
        a                   owl:ObjectProperty ;
        rdfs:comment        "The public procurement notice is published in a given official journal (always in the S collection)" ;
        rdfs:domain         :procurement_public ;
        rdfs:label          "Public procurement notice published in official journal" ;
        rdfs:range          :official-journal ;
        rdfs:subPropertyOf  :published_in .

:case_court_identifier_year
        a                   owl:DatatypeProperty ;
        rdfs:comment        "Year in the case identifier. e.g. C-172/97_PV" ;
        rdfs:domain         :case_court ;
        rdfs:label          "Year in identifier of court case" ;
        rdfs:range          xsd:gYear ;
        rdfs:subPropertyOf  :identifier_year .

:optionally-consulted_by
        a           owl:ObjectProperty ;
        rdfs:label  "Optionally consulted by" .

:does_repeal_of  a  owl:ObjectProperty ;
        rdfs:label  "Does repeal of" .

:work_catalogued_by_work
        a                   owl:ObjectProperty ;
        rdfs:comment        "The work is catalogued by another work, e.g. by publishing a list of titles" ;
        rdfs:domain         :work ;
        rdfs:label          "Work is catalogued by work" ;
        rdfs:range          :work ;
        rdfs:subPropertyOf  :catalogued_by ;
        owl:inverseOf       :work_catalogues_work .

:manifestation_distribution_has_status_distribution_status
        a                   owl:ObjectProperty ;
        rdfs:comment        "This property refers to the majority of the distribution" ;
        rdfs:domain         :manifestation_distribution ;
        rdfs:label          "Status" ;
        rdfs:range          :distribution_status ;
        rdfs:subPropertyOf  :has_status .

:manifestation_official-journal_part_durability
        a                   owl:DatatypeProperty ;
        rdfs:comment        "Indication of the durability of the legal resource (as seen by the printer). Values such as \"DUR\"" ;
        rdfs:domain         :manifestation_official-journal_part ;
        rdfs:label          "Durability of the act" ;
        rdfs:range          xsd:string ;
        rdfs:subPropertyOf  :durability .

:procurement_public_transliterated_email
        a                   owl:DatatypeProperty ;
        rdfs:domain         :procurement_public ;
        rdfs:label          "Procurement public transliterated email" ;
        rdfs:range          xsd:string ;
        rdfs:subPropertyOf  :transliterated_email .

:service_responsible  a  owl:DatatypeProperty ;
        rdfs:comment  "RS" ;
        rdfs:label    "Service responsible" .

:expression  a           owl:Class ;
        rdfs:comment     "Realisation of a work in alpha-numeric or cartographic notation, sound, image, object, movement, etc., or any combination of such forms" ;
        rdfs:label       "Expression" ;
        rdfs:subClassOf  [ a                   owl:Restriction ;
                           owl:maxCardinality  "1"^^xsd:nonNegativeInteger ;
                           owl:onProperty      :expression_edition
                         ] ;
        rdfs:subClassOf  [ a                         owl:Restriction ;
                           owl:onClass               :work ;
                           owl:onProperty            :expression_belongs_to_work ;
                           owl:qualifiedCardinality  "1"^^xsd:nonNegativeInteger
                         ] ;
        rdfs:subClassOf  [ a                   owl:Restriction ;
                           owl:minCardinality  "1"^^xsd:nonNegativeInteger ;
                           owl:onProperty      :expression_title
                         ] ;
        rdfs:subClassOf  [ a                   owl:Restriction ;
                           owl:maxCardinality  "1"^^xsd:nonNegativeInteger ;
                           owl:onProperty      :expression_version
                         ] ;
        rdfs:subClassOf  [ a                   owl:Restriction ;
                           owl:maxCardinality  "1"^^xsd:nonNegativeInteger ;
                           owl:onProperty      :expression_date
                         ] ;
        rdfs:subClassOf  [ a                   owl:Restriction ;
                           owl:maxCardinality  "1"^^xsd:nonNegativeInteger ;
                           owl:onProperty      cmr:creationDate
                         ] ;
        rdfs:subClassOf  [ a                   owl:Restriction ;
                           owl:maxCardinality  "1"^^xsd:nonNegativeInteger ;
                           owl:onProperty      :expression_embargo
                         ] ;
        rdfs:subClassOf  [ a                            owl:Restriction ;
                           owl:minQualifiedCardinality  "1"^^xsd:nonNegativeInteger ;
                           owl:onClass                  :language ;
                           owl:onProperty               :expression_uses_language
                         ] ;
        rdfs:subClassOf  [ a                owl:Restriction ;
                           owl:cardinality  "1"^^xsd:nonNegativeInteger ;
                           owl:onProperty   cmr:lastModificationDate
                         ] ;
        rdfs:subClassOf  [ a                   owl:Restriction ;
                           owl:maxCardinality  "1"^^xsd:nonNegativeInteger ;
                           owl:onProperty      :expression_source
                         ] .

<http://publications.europa.eu/resource/authority/fd_110>
        a       owl:NamedIndividual .

:abstract  a        owl:DatatypeProperty ;
        rdfs:label  "Abstract" .

:ATTO_FD_604  a              owl:Class ;
        rdfs:label           "FD_604 ATTO table" ;
        rdfs:subClassOf      skos:Concept ;
        owl:equivalentClass  [ a               owl:Restriction ;
                               owl:hasValue    <http://publications.europa.eu/resource/authority/fd_604> ;
                               owl:onProperty  skos:inScheme
                             ] .

:publication_general_part_of_series
        a           owl:ObjectProperty ;
        rdfs:label  "Publication general part of series" .

:binding  a                  owl:Class ;
        rdfs:comment         "binding of a manifestation" ;
        rdfs:label           "Binding" ;
        rdfs:subClassOf      skos:Concept , :concept ;
        owl:equivalentClass  [ a               owl:Restriction ;
                               owl:hasValue    <http://publications.europa.eu/resource/authority/pub_bind> ;
                               owl:onProperty  skos:inScheme
                             ] .

:work_has_resource-type
        a                   owl:ObjectProperty ;
        rdfs:comment        "Related authority or tables: Resource types NAL, ATTO FD_30. Relevant for legal analysis: true. The resource type of this work. Relevant for legal analysis: trueRelated authority or tables: Resource types NAL, ATTO FD_30" ;
        rdfs:domain         :work ;
        rdfs:label          "Work has resource type" ;
        rdfs:range          :resource-type ;
        rdfs:subPropertyOf  :has .

:act_preparatory_council_qualifier_document
        a                   owl:DatatypeProperty ;
        rdfs:comment        "DEPRECATED; Document qualifier of the identifier the document has at the Council. The document qualifier (suffix) serves the purpose of identifying the original document and the modifications made to it" ;
        rdfs:domain         :act_preparatory_council ;
        rdfs:label          "Document qualifier" ;
        rdfs:range          xsd:string ;
        rdfs:subPropertyOf  :qualifier_document ;
        owl:deprecated      true .

<http://publications.europa.eu/resource/authority/corporate-body/EESC>
        a       owl:NamedIndividual .

:subject-matter_subject_of_summary_legislation_eu
        a                   owl:ObjectProperty ;
        rdfs:comment        "A concept expressed as a subject matter (classification tool) has as its subject a summary on EU legislation. Relevant for legal analysis: true" ;
        rdfs:domain         :subject-matter ;
        rdfs:label          "Subject matter is subject of an EU legislative summary" ;
        rdfs:range          :summary_legislation_eu ;
        rdfs:subPropertyOf  :subject_of ;
        owl:inverseOf       :summary_legislation_eu_is_about_subject-matter .

:referred_to_for_preliminary_ruling
        a           owl:ObjectProperty ;
        rdfs:label  "Referred to for preliminary ruling" .

:act_consolidated_layer_act_consolidated
        a                   owl:DatatypeProperty ;
        rdfs:comment        "DEPRECATED, Consleg couche. Number of the layer (DEPRECATED, use layer instead)" ;
        rdfs:domain         :act_consolidated ;
        rdfs:label          "Consolidated act layer" ;
        rdfs:range          xsd:string ;
        rdfs:subPropertyOf  :layer_act_consolidated ;
        owl:deprecated      true .

:event_legal_was_historically_about_concept_type_dossier
        a                   owl:ObjectProperty ;
        rdfs:comment        "Relevant for legal analysis: true. This dossier was at the time of the event of a certain type, expressed through a dossier type concept. Expressed through a link to the concept_type_dossier, currently FD table 612, previously known as type_dossier_historical. Relevant for legal analysis: true" ;
        rdfs:domain         :event_legal ;
        rdfs:label          "Dossier was about historical dossier type concept" ;
        rdfs:range          :concept_type_dossier ;
        rdfs:subPropertyOf  :was_historically_about .

:ATTO_FD_577  a              owl:Class ;
        rdfs:label           "FD_577 ATTO table" ;
        rdfs:subClassOf      skos:Concept ;
        owl:equivalentClass  [ a               owl:Restriction ;
                               owl:hasValue    <http://publications.europa.eu/resource/authority/fd_577> ;
                               owl:onProperty  skos:inScheme
                             ] .

:typedoc_printer  a  owl:DatatypeProperty ;
        rdfs:label  "Typedoc printer" .

:ATTO_FD_100  a              owl:Class ;
        rdfs:label           "FD_100 ATTO table" ;
        rdfs:subClassOf      skos:Concept ;
        owl:equivalentClass  [ a               owl:Restriction ;
                               owl:hasValue    <http://publications.europa.eu/resource/authority/fd_100> ;
                               owl:onProperty  skos:inScheme
                             ] .

:name_official_journal
        a           owl:DatatypeProperty ;
        rdfs:label  "Name official journal" .

:country_role-qualifier_initiates_case-law
        a              owl:ObjectProperty ;
        rdfs:domain    :country_role-qualifier ;
        rdfs:label     "Country role qualifier initiates case law" ;
        rdfs:range     :case-law ;
        owl:inverseOf  :case-law_originates_in_country_role-qualifier .

:requests_for_failure_to_fulfill_an_obligation_for
        a           owl:ObjectProperty ;
        rdfs:label  "Requests for failure to fulfill an obligation for" .

:signature_digital_authority_certification
        a                   owl:DatatypeProperty ;
        rdfs:comment        "Name or abbreviation of the certification authority. Modelled as a free string" ;
        rdfs:domain         :signature_digital ;
        rdfs:label          "Certification authority" ;
        rdfs:range          xsd:string ;
        rdfs:subPropertyOf  :authority_certification .

:article_legal_part_of_work
        a                   owl:ObjectProperty ;
        rdfs:comment        "This property associates an instance of a work with an instance of a legal article that forms part of it." ;
        rdfs:domain         :article_legal ;
        rdfs:label          "Article (legal) part of work" ;
        rdfs:range          :work ;
        rdfs:subPropertyOf  :subdivision_part_of_work , :part_of ;
        owl:inverseOf       :work_contains_article_legal .

:procurement_public_heading_old
        a                   owl:DatatypeProperty ;
        rdfs:domain         :procurement_public ;
        rdfs:label          "Old heading" ;
        rdfs:range          xsd:string ;
        rdfs:subPropertyOf  :heading_old .

:procurement_public_labels_forms_reference
        a                   owl:DatatypeProperty ;
        rdfs:domain         :procurement_public ;
        rdfs:label          "Reference for label forms" ;
        rdfs:range          xsd:anyURI ;
        rdfs:subPropertyOf  :labels_forms_reference .

:dossier_duration  a        owl:DatatypeProperty ;
        rdfs:comment        "If expressed in days, add d after the value, if expressed in weeks w, e.g. 6w, e.g. /ns4:ec_transmission_request/extension/ns4:delay_in_weeks" ;
        rdfs:domain         :dossier ;
        rdfs:label          "Dossier had to be treated during a given duration / in a given delay" ;
        rdfs:range          xsd:string ;
        rdfs:subPropertyOf  :duration .

:case-law_affaire_number
        a                   owl:DatatypeProperty ;
        rdfs:comment        "Number of the affaire" ;
        rdfs:domain         :case-law ;
        rdfs:label          "Affaire: Number" ;
        rdfs:range          xsd:positiveInteger ;
        rdfs:subPropertyOf  :affaire_number .

<http://publications.europa.eu/resource/authority/pub_them>
        a       owl:NamedIndividual .

:manifestation_has_binding
        a                   owl:ObjectProperty ;
        rdfs:domain         :manifestation ;
        rdfs:label          "Manifestation has binding" ;
        rdfs:range          :binding ;
        rdfs:subPropertyOf  :has .

:stored_by  a       owl:ObjectProperty ;
        rdfs:label  "Stored by" .

:manifestation_confidentiality
        a             owl:DatatypeProperty ;
        rdfs:comment  "This property define the confidentiality level, where the possible values are [UNRESTRICTED | RESTRICTED]. Default: UNRESTRICTED" ;
        rdfs:domain   :manifestation ;
        rdfs:label    "Confidentiality level of manifestation" ;
        rdfs:range    xsd:string ;
        dct:created   "2018-08-13T12:22:20.090+02:00"^^xsd:dateTime .

:event_case_has_type-procedure
        a                   owl:ObjectProperty ;
        rdfs:comment        "DEPRECATED; Case event has a procedural framework with a given type of procedure. Possible values R, I, P" ;
        rdfs:domain         :event_case ;
        rdfs:label          "Case event has a procedural framework with a given type of procedure" ;
        rdfs:range          :type-procedure ;
        rdfs:subPropertyOf  :has ;
        owl:deprecated      true .

:basis_legal  a     owl:DatatypeProperty ;
        rdfs:label  "Basis legal" .

:resolution_legislative_ep
        a                owl:Class ;
        rdfs:comment     "8806 EP legislative resolutions (5AP)" ;
        rdfs:label       "European Parliament legislative resolution" ;
        rdfs:subClassOf  :act_preparatory_ep ;
        rdfs:subClassOf  [ a                owl:Restriction ;
                           owl:cardinality  "1"^^xsd:nonNegativeInteger ;
                           owl:onProperty   :resolution_legislative_ep_term_parliamentary
                         ] .

:informs  a         owl:ObjectProperty ;
        rdfs:label  "Informs" .

:act_preparatory_has_status
        a                   owl:ObjectProperty ;
        rdfs:comment        "Status of a preparatory act" ;
        rdfs:domain         :act_preparatory ;
        rdfs:label          "Act preparatory has status" ;
        rdfs:range          :status ;
        rdfs:subPropertyOf  :has_status .

:manifestation_case-law_keywords
        a                   owl:DatatypeProperty ;
        rdfs:comment        "Keywords associated with this judgement. Sector 6 Text Index Field IX" ;
        rdfs:domain         :manifestation_case-law ;
        rdfs:label          "Keywords for court decision" ;
        rdfs:range          rdf:XMLLiteral ;
        rdfs:subPropertyOf  :keywords .

:procurement_public_contract-nature_code
        a                   owl:DatatypeProperty ;
        rdfs:domain         :procurement_public ;
        rdfs:label          "Natural code of the contract" ;
        rdfs:range          xsd:string ;
        rdfs:subPropertyOf  :contract-nature_code .

:opinion_eesc_number_session
        a                   owl:DatatypeProperty ;
        rdfs:comment        "Number of session during which this act was debated or voted (EP, EESC, CoR, …). Relevant for legal analysis: true" ;
        rdfs:domain         :opinion_eesc ;
        rdfs:label          "Number of session" ;
        rdfs:range          xsd:string ;
        rdfs:subPropertyOf  :number_session , :act_preparatory_number_session ;
        owl:deprecated      true .

:person_jointly-responsible_for_event_legal
        a                   owl:ObjectProperty ;
        rdfs:comment        "DEPRECATED," ;
        rdfs:domain         :person ;
        rdfs:label          "Person jointly responsible for legal event" ;
        rdfs:range          :event_legal ;
        rdfs:subPropertyOf  :jointly-responsible_for ;
        owl:deprecated      true .

:second_series_historical
        a           owl:DatatypeProperty ;
        rdfs:label  "Second series historical" .

:court_national_has_type_concept_class_court_national
        a                   owl:ObjectProperty ;
        rdfs:comment        "e.g. a) Court of first instance, b) Court of appeal, c) Supreme court" ;
        rdfs:domain         :court_national ;
        rdfs:label          "National Court has type classification class" ;
        rdfs:range          :concept_class_court_national ;
        rdfs:subPropertyOf  :has_type .

:work_dataset_version_notes
        a                   owl:DatatypeProperty ;
        rdfs:comment        "This property contains a description of differences between this version and previous version of the dataset." ;
        rdfs:domain         :work_dataset ;
        rdfs:label          "Dataset version note" ;
        rdfs:range          xsd:string ;
        rdfs:subPropertyOf  :version_notes .

:regulation_service_responsible
        a                   owl:DatatypeProperty ;
        rdfs:comment        "The Commission DG or DGs responsible for drafting of an act. Relevant for legal analysis: true DEPRECATED, In the instance data, the property is planned to be replaced with cdm:resource_legal_service_responsible at beginning 2019. When this is done this property the property will be removed from CDM.The Commission's DG that brought f\"The Commission DG or DGs responsible for drafting of an act. For the backlog data need to be completed. Cardinality to be restricted to 1 in the future. orward the proposal; to be taken from a closed list of DGs (that might be derived from the RECORD project ?) For the backlog data need to be completed." ;
        rdfs:domain         :regulation ;
        rdfs:label          "Service responsible" ;
        rdfs:range          xsd:string ;
        rdfs:subPropertyOf  :service_responsible , :resource_legal_service_responsible ;
        owl:deprecated      true .

:ATTO_FD_535  a              owl:Class ;
        rdfs:label           "FD_535 ATTO table" ;
        rdfs:subClassOf      skos:Concept ;
        owl:equivalentClass  [ a               owl:Restriction ;
                               owl:hasValue    <http://publications.europa.eu/resource/authority/fd_535> ;
                               owl:onProperty  skos:inScheme
                             ] .

:case-law_national_keywords
        a                   owl:DatatypeProperty ;
        rdfs:comment        "Formal Description of a case law" ;
        rdfs:domain         :case-law_national ;
        rdfs:label          "Description" ;
        rdfs:range          rdf:XMLLiteral ;
        rdfs:subPropertyOf  :keywords .

:subdivision  a          owl:Class ;
        rdfs:comment     "Super class for grouping subdivision structures Super class for grouping subdivision structures such as legal paragraphs and legal articles. Subdivisions follow the general structure of the subdivision authority table." ;
        rdfs:label       "Subdivision" ;
        rdfs:subClassOf  :textstructure ;
        rdfs:subClassOf  [ a                            owl:Restriction ;
                           owl:maxQualifiedCardinality  "1"^^xsd:nonNegativeInteger ;
                           owl:onClass                  :work ;
                           owl:onProperty               :subdivision_part_of_work
                         ] ;
        rdfs:subClassOf  [ a                            owl:Restriction ;
                           owl:maxQualifiedCardinality  "1"^^xsd:nonNegativeInteger ;
                           owl:onClass                  :subdivision ;
                           owl:onProperty               :subdivision_part_of_subdivision
                         ] .

:prereleases  a             owl:ObjectProperty ;
        rdfs:comment        "This is an intermediate subclass representing the pre release relation which is a specific form of making a version public with an inofficial/unstable status." ;
        rdfs:label          "Prereleases" ;
        rdfs:subPropertyOf  :publishes ;
        owl:inverseOf       :prereleased_in .

:identifier_number  a  owl:DatatypeProperty ;
        rdfs:label  "Identifier number" .

:archive_package_barcode
        a                   owl:DatatypeProperty ;
        rdfs:comment        "a barcode used by the scanning provider to uniquely and automatically identify a physical package to be scanned" ;
        rdfs:domain         :archive_package ;
        rdfs:label          "Archive package barcode" ;
        rdfs:range          xsd:string ;
        rdfs:subPropertyOf  :barcode .

:special-official-journal_first_series_historical
        a                   owl:DatatypeProperty ;
        rdfs:comment        "For old SPs, an indication of the series they appeared in" ;
        rdfs:domain         :special-official-journal ;
        rdfs:label          "First historical series" ;
        rdfs:range          xsd:string ;
        rdfs:subPropertyOf  :first_series_historical .

:manifestation_related_to_manifestation
        a                   owl:SymmetricProperty , owl:ObjectProperty ;
        rdfs:comment        "manifestation related to another manifestation" ;
        rdfs:domain         :manifestation ;
        rdfs:label          "Manifestation related to manifestation" ;
        rdfs:range          :manifestation ;
        rdfs:subPropertyOf  :related_to .

:notice_prior-information
        a                owl:Class ;
        rdfs:label       "Prior information notice" ;
        rdfs:subClassOf  :procurement_public ;
        rdfs:subClassOf  [ a                owl:Restriction ;
                           owl:cardinality  "1"^^xsd:nonNegativeInteger ;
                           owl:onProperty   :notice_prior-information_main-activities_code
                         ] ;
        rdfs:subClassOf  [ a                owl:Restriction ;
                           owl:cardinality  "1"^^xsd:nonNegativeInteger ;
                           owl:onProperty   :notice_prior-information_authority-type_label
                         ] ;
        rdfs:subClassOf  [ a                owl:Restriction ;
                           owl:cardinality  "1"^^xsd:nonNegativeInteger ;
                           owl:onProperty   :notice_prior-information_authority-type_code
                         ] .

:resource_legal_interpretes_authoritatively_resource_legal
        a                   owl:ObjectProperty ;
        rdfs:comment        "Relevant for legal analysis: true" ;
        rdfs:domain         :resource_legal ;
        rdfs:label          "Legal resource interprets authoritatively legal resource" ;
        rdfs:range          :resource_legal ;
        rdfs:subPropertyOf  :interpretes_authoritatively ;
        owl:inverseOf       :resource_legal_interpreted_authoritatively_by_resource_legal .

:preceeding_case-law  a  owl:DatatypeProperty ;
        rdfs:label  "Preceeding case law" .

:expression_case-law_indicator_decision
        a                   owl:DatatypeProperty ;
        rdfs:comment        "Decision indicator in the title of a case law document (language-specific)" ;
        rdfs:domain         :expression_case-law ;
        rdfs:label          "Decision indicator" ;
        rdfs:range          xsd:string ;
        rdfs:subPropertyOf  :indicator_decision .

:manifestation_uri  a       owl:DatatypeProperty ;
        rdfs:comment        "External URI for this manifestation. Use manifestation type URI if this fiels is present. Relevant for legal analysis: true." ;
        rdfs:domain         :manifestation ;
        rdfs:label          "External URI of a representation of this manifestation" ;
        rdfs:range          xsd:anyURI ;
        rdfs:subPropertyOf  :uri .

:act_reference_international
        a           owl:DatatypeProperty ;
        rdfs:label  "Act reference international" .

:manifestation_special-official-journal-act_legal_effect_paper
        a                   owl:DatatypeProperty ;
        rdfs:comment        "Legal effect paper applying to a special Official Journal act's manifestation" ;
        rdfs:domain         :manifestation_special-official-journal-act ;
        rdfs:label          "Manifestation Special Official Journal act legal effect paper" ;
        rdfs:range          xsd:boolean ;
        rdfs:subPropertyOf  :legal_effect_paper .

:ATTO_FD_010  a              owl:Class ;
        rdfs:label           "FD_010 ATTO table" ;
        rdfs:subClassOf      skos:Concept ;
        owl:deprecated       true ;
        owl:equivalentClass  [ a               owl:Restriction ;
                               owl:hasValue    <http://publications.europa.eu/resource/authority/fd_010> ;
                               owl:onProperty  skos:inScheme
                             ] .

:requests_validation  a  owl:ObjectProperty ;
        rdfs:label  "Requests validation" .

:archive_package_internal_number_prefix
        a                   owl:DatatypeProperty ;
        rdfs:comment        "possible (useful) values: SEC, S, G, for the subclassification of the document type" ;
        rdfs:domain         :archive_package ;
        rdfs:label          "Archive package internal number prefix" ;
        rdfs:range          xsd:string ;
        rdfs:subPropertyOf  :internal_number_prefix .

:item   a                owl:Class ;
        rdfs:comment     "\"A single exemplar of a manifestation\" (FRBR). In this context an item corresponds to a data stream in the CCR" ;
        rdfs:label       "Item" ;
        rdfs:subClassOf  [ a                   owl:Restriction ;
                           owl:minCardinality  "1"^^xsd:nonNegativeInteger ;
                           owl:onProperty      :item_identifier
                         ] ;
        rdfs:subClassOf  [ a                   owl:Restriction ;
                           owl:maxCardinality  "1"^^xsd:nonNegativeInteger ;
                           owl:onProperty      :item_embargo
                         ] ;
        rdfs:subClassOf  [ a                   owl:Restriction ;
                           owl:maxCardinality  "1"^^xsd:nonNegativeInteger ;
                           owl:onProperty      :item_doi
                         ] ;
        rdfs:subClassOf  [ a                            owl:Restriction ;
                           owl:minQualifiedCardinality  "1"^^xsd:nonNegativeInteger ;
                           owl:onClass                  :manifestation ;
                           owl:onProperty               :item_belongs_to_manifestation
                         ] .

:location_for  a    owl:ObjectProperty ;
        rdfs:label  "Location for" .

:work_date_creation  a      owl:DatatypeProperty ;
        rdfs:comment        "Date of creation in the CELLAR. Relevant for legal analysis: true." ;
        rdfs:domain         :work ;
        rdfs:label          "Date of creation of work" ;
        rdfs:range          xsd:date ;
        rdfs:subPropertyOf  :date_creation .

:work_dataset_description_editorial
        a                   owl:DatatypeProperty ;
        rdfs:domain         :work_dataset ;
        rdfs:label          "Dataset description" ;
        rdfs:range          xsd:string ;
        rdfs:subPropertyOf  :description_editorial .

:resource_legal_date_deadline
        a                   owl:DatatypeProperty ;
        rdfs:comment        "This refers to various intermediate deadlines relating to the document. DL_COMMENT is mixed content, decoded with fd_335. DL. Relevant for legal analysis: true" ;
        rdfs:domain         :resource_legal ;
        rdfs:label          "Date of deadline" ;
        rdfs:range          xsd:date ;
        rdfs:subPropertyOf  :date_deadline .

:procurement_public_number_document_in_official-journal
        a                   owl:DatatypeProperty ;
        rdfs:domain         :procurement_public ;
        rdfs:label          "Document number in the Official Journal" ;
        rdfs:range          xsd:string ;
        rdfs:subPropertyOf  :number_document_in_official-journal .

:act_consolidated  a     owl:Class ;
        rdfs:comment     "Consolidated acts (= sector 0): Non-official documents integrating acts of sector 3 with their amendments and corrections. Note: The original VOLET_CONSLEG contains also more fields: * CONSOLID_SEQ: Sequence in the list * CONSOLID_ACT set: Logical grouping element: Used if the act is modified * CONSOLID_ROLE: \"IN ou OUT suivant prise en compte dans consolidation\" * CONSOLID_FICHE: contains links from the acts to the consolidating acts * BF_NAT, BF, LE and TM are old Consolidation fields that need to be taken into account The pertinence of these fields must be discussed" ;
        rdfs:label       "Consolidated act" ;
        rdfs:subClassOf  :resource_legal ;
        rdfs:subClassOf  [ a                            owl:Restriction ;
                           owl:minQualifiedCardinality  "1"^^xsd:nonNegativeInteger ;
                           owl:onClass                  :resource_legal ;
                           owl:onProperty               :act_consolidated_based_on_resource_legal
                         ] ;
        rdfs:subClassOf  [ a                            owl:Restriction ;
                           owl:minQualifiedCardinality  "1"^^xsd:nonNegativeInteger ;
                           owl:onClass                  :resource_legal ;
                           owl:onProperty               :act_consolidated_consolidates_resource_legal
                         ] ;
        rdfs:subClassOf  [ a                   owl:Restriction ;
                           owl:maxCardinality  "1"^^xsd:nonNegativeInteger ;
                           owl:onProperty      :act_consolidated_reference_act_consolidated
                         ] ;
        rdfs:subClassOf  [ a                   owl:Restriction ;
                           owl:maxCardinality  "1"^^xsd:nonNegativeInteger ;
                           owl:onProperty      :act_consolidated_version
                         ] ;
        rdfs:subClassOf  [ a                   owl:Restriction ;
                           owl:maxCardinality  "1"^^xsd:nonNegativeInteger ;
                           owl:onProperty      :act_consolidated_layer_act_consolidated
                         ] ;
        rdfs:subClassOf  [ a                owl:Restriction ;
                           owl:cardinality  "1"^^xsd:nonNegativeInteger ;
                           owl:onProperty   :act_consolidated_layer
                         ] ;
        rdfs:subClassOf  [ a                   owl:Restriction ;
                           owl:maxCardinality  "1"^^xsd:nonNegativeInteger ;
                           owl:onProperty      :act_consolidated_date
                         ] ;
        rdfs:subClassOf  [ a                   owl:Restriction ;
                           owl:maxCardinality  "1"^^xsd:nonNegativeInteger ;
                           owl:onProperty      :act_consolidated_number
                         ] .

:work_communicates_on_work
        a                   owl:ObjectProperty ;
        rdfs:domain         :work ;
        rdfs:label          "Work communicates on work" ;
        rdfs:range          :work ;
        rdfs:subPropertyOf  :communicates_on .

:manifestation_official-journal_part_legal_basis_printer
        a                   owl:DatatypeProperty ;
        rdfs:comment        "Legal basis of the legal resource (as seen by the printer). Values such as \"EURATOM\", \"EC\"" ;
        rdfs:domain         :manifestation_official-journal_part ;
        rdfs:label          "Printer's legal basis of the act" ;
        rdfs:range          xsd:string ;
        rdfs:subPropertyOf  :legal_basis_printer .

:case-law_national_reference_publication
        a                   owl:DatatypeProperty ;
        rdfs:comment        "Freetext information on the publication in which this judgement appeared" ;
        rdfs:domain         :case-law_national ;
        rdfs:label          "Publication reference of Court decision" ;
        rdfs:range          rdf:XMLLiteral ;
        rdfs:subPropertyOf  :reference_publication .

:resource_legal_basis_for_event_legal
        a                   owl:ObjectProperty ;
        rdfs:comment        "The legal resource serves as basis for a legal event (typically, but not necessarily a treaty article). Relevant for legal analysis: true." ;
        rdfs:domain         :resource_legal ;
        rdfs:label          "Legal resource is basis for a legal event" ;
        rdfs:range          :event_legal ;
        rdfs:subPropertyOf  :basis_for .

:language_used_originally_by_procurement_public
        a              owl:ObjectProperty ;
        rdfs:domain    :language ;
        rdfs:label     "Language used originally by procurement public" ;
        rdfs:range     :procurement_public ;
        owl:inverseOf  :procurement_public_uses_originally_language .

:non-opposition_concentration_notified_service_responsible
        a                   owl:DatatypeProperty ;
        rdfs:comment        "The Commission DG or DGs responsible for drafting of an act. Relevant for legal analysis: true. DEPRECATED, In the instance data, the property is planned to be replaced with cdm:resource_legal_service_responsible at beginning 2019. When this is done this property the property will be removed from CDM. The Commission's DG that brought forward the proposal; to be taken from a closed list of DGs (that might be derived from the RECORD project ?). For the backlog data need to be completed. Cardinality to be restricted to 1 in the future." ;
        rdfs:domain         :non-opposition_concentration_notified ;
        rdfs:label          "Service responsible" ;
        rdfs:range          xsd:string ;
        rdfs:subPropertyOf  :service_responsible , :resource_legal_service_responsible ;
        owl:deprecated      true .

:procedure_year  a  owl:DatatypeProperty ;
        rdfs:label  "Procedure year" .

<http://publications.europa.eu/resource/authority/com_internal_procedure>
        a       owl:NamedIndividual .

:work_explained_by_work
        a                   owl:ObjectProperty ;
        rdfs:comment        "Relevant for legal analysis: true. The work is explained by another work (e.g. a commentary or a citizen's summary). Relevant for legal analysis: true" ;
        rdfs:domain         :work ;
        rdfs:label          "Work is explained by work" ;
        rdfs:range          :work ;
        rdfs:subPropertyOf  :explained_by ;
        owl:inverseOf       :work_explains_work .

:dossier_pending-proposal
        a                   owl:DatatypeProperty ;
        rdfs:comment        "Pending proposal. Relevant for legal analysis: true." ;
        rdfs:domain         :dossier ;
        rdfs:label          "Dossier is still pending proposal?" ;
        rdfs:range          xsd:boolean ;
        rdfs:subPropertyOf  :pending-proposal .

:measure_national_implementing_declaration_transposition_member-state
        a                   owl:DatatypeProperty ;
        rdfs:comment        "Declaration of the Member State on the state of the transposition. Possible values AU, IN, PA, NN" ;
        rdfs:domain         :measure_national_implementing ;
        rdfs:label          "Transposition declaration by the Member State" ;
        rdfs:range          xsd:string ;
        rdfs:subPropertyOf  :declaration_transposition_member-state .

<http://publications.europa.eu/ontology/cdm>
        a                owl:Ontology ;
        rdfs:seeAlso     "https://op.europa.eu/en/web/eu-vocabularies/cdm" ;
        dc:description   "The human readable version of the Common Data Model (CDM) documents the structure of metadata to be used notably in the Publications Office's Common Metadata Repository (CRM). Its mission is to establish a uniform data model that captures and brings together all of the Office's metadata. In a first phase the focus is on metadata related to legal resources and general publications, in a second phase metadata for TED and CORDIS will follow. This documentation is generated directly from the CDM OWL representation. In collaboration with the business units concerned the model is continually refined. The CDM specifies in addition validation rules that may in the future serve to refine the automated validation of incoming and existing metadata."@en ;
        dct:creator      "Publications Office of the European Union"@en ;
        dct:date         "2023-01-12" ;
        dct:rights       "\n    © European Union, 2014\n\tThe Commission’s reuse policy is implemented by Commission Decision 2011/833/EU of 12 December 2011 on the reuse of Commission documents \n\t(OJ L 330, 14.12.2011, p. 39 – https://eur-lex.europa.eu/eli/dec/2011/833/oj). Unless otherwise noted, the reuse of this document is authorised under the \n\tCreativeCommons Attribution 4.0 International (CC BY 4.0) licence (https://creativecommons.org/licenses/by/4.0/). This means that reuse is allowed, provided \n\tthat appropriate credit is given and any changes are indicated.\n\t" ;
        dct:title        "Common Data Model (CDM)"@en ;
        owl:imports      <http://publications.europa.eu/ontology/cdm/import> ;
        owl:versionInfo  "4.8.1" .

:has_type  a        owl:ObjectProperty ;
        rdfs:label  "Has type" .

:agreement_international_stored_by_agent
        a                   owl:ObjectProperty ;
        rdfs:comment        "International agreement is stored by an agent acting as depositary. DP (2) / depositary. Relevant for legal analysis: true." ;
        rdfs:domain         :agreement_international ;
        rdfs:label          "International agreement stored by agent" ;
        rdfs:range          :agent ;
        rdfs:subPropertyOf  :stored_by ;
        owl:inverseOf       :agent_depositary_for_agreement_international .

:included_in  a     owl:ObjectProperty ;
        rdfs:label  "Included in" .

<http://publications.europa.eu/resource/authority/publication-accessibility>
        a       owl:NamedIndividual .

:repealed_by  a     owl:ObjectProperty ;
        rdfs:label  "Repealed by" .

:contains  a        owl:ObjectProperty ;
        rdfs:label  "Contains" .

:illustrated_by  a  owl:ObjectProperty ;
        rdfs:label  "Illustrated by" .

:access_url  a      owl:DatatypeProperty ;
        rdfs:label  "Access url" .

:internal_number_sequential_number
        a           owl:DatatypeProperty ;
        rdfs:label  "Internal number sequential number" .

:country  a                  owl:Class ;
        rdfs:comment         "Country. The list of instances of this class is provided by the Metadata Registry. A country can in our context both act as an agent and as an administrative unit." ;
        rdfs:label           "Country" ;
        rdfs:subClassOf      skos:Concept , :unit_administrative , :agent ;
        owl:equivalentClass  [ a               owl:Restriction ;
                               owl:hasValue    <http://publications.europa.eu/resource/authority/country> ;
                               owl:onProperty  skos:inScheme
                             ] .

:landing_page  a    owl:DatatypeProperty ;
        rdfs:label  "Landing page" .

:date_vote  a               owl:DatatypeProperty ;
        rdfs:label          "Date vote" ;
        rdfs:range          xsd:date ;
        rdfs:subPropertyOf  :date .

:act_consolidated_version
        a                   owl:DatatypeProperty ;
        rdfs:comment        "Number of the version of a layer. Newly created concept to keep track of consleg versions (= changes within one layer)" ;
        rdfs:domain         :act_consolidated ;
        rdfs:label          "Consolidated act version of a layer" ;
        rdfs:range          xsd:string ;
        rdfs:subPropertyOf  :version .

:work_provides_mandatory_information_to_dossier
        a              owl:ObjectProperty ;
        rdfs:domain    :work ;
        rdfs:label     "work provides mandatory information to dossier" ;
        rdfs:range     :dossier ;
        owl:inverseOf  :dossier_mandatory_information_provided_by_work .

:resource_legal_date_referral
        a                   owl:DatatypeProperty ;
        rdfs:comment        "Date of referral" ;
        rdfs:domain         :resource_legal ;
        rdfs:label          "Date of referral" ;
        rdfs:range          xsd:date ;
        rdfs:subPropertyOf  :date_referral .

:manifestation_official-journal_part_page_last
        a                   owl:DatatypeProperty ;
        rdfs:comment        "DEPRECATED, Last page number of the OJ part related to a legal resource. Use manifestion_print_page_last" ;
        rdfs:domain         :manifestation_official-journal_part ;
        rdfs:label          "Last page" ;
        rdfs:range          xsd:string ;
        rdfs:subPropertyOf  :page_last , :manifestation_print_page_last ;
        owl:deprecated      true .

:swd_package_ec  a       owl:Class ;
        rdfs:comment     "The swd_package_ec class is a generic class for scanned documents from the OIB HAS archives, done in the scope of digiCOM/digiSEC projects. It contains formerly internal or classified documents which have been meanwhile declassified officially or implicitly. These staff working documents usually have SEC, S or G type identifiers which will be represented in their own subclasses." ;
        rdfs:label       "Digitised staff working document" ;
        rdfs:subClassOf  :staff-working-document_ec , :archive_package_ec ;
        rdfs:subClassOf  [ a                            owl:Restriction ;
                           owl:maxQualifiedCardinality  "1"^^xsd:nonNegativeInteger ;
                           owl:onDataRange              xsd:boolean ;
                           owl:onProperty               :swd_package_ec_has_title_from_com_final
                         ] ;
        dct:created      "2022-09-01T09:01:22"^^xsd:dateTime .

:regulation_service_associated
        a                   owl:DatatypeProperty ;
        rdfs:comment        "This field indicates the Commission DG or DGs co-responsible for drafting of an act. DEPRECATED, In the instance data, the property is planned to be replaced with cdm:resource_legal_service_associated at beginning 2019. When this is done this property the property will be removed from CDM. Relevant for legal analysis: true" ;
        rdfs:domain         :regulation ;
        rdfs:label          "Service associated" ;
        rdfs:range          xsd:string ;
        rdfs:subPropertyOf  :service_associated , :resource_legal_service_associated ;
        owl:deprecated      true .

:case-law_national_reference_publication-conclusion
        a                   owl:DatatypeProperty ;
        rdfs:comment        "Freetext information on the publication in which the conclusions of this judgement appeared" ;
        rdfs:domain         :case-law_national ;
        rdfs:label          "Publication reference for conclusions" ;
        rdfs:range          rdf:XMLLiteral ;
        rdfs:subPropertyOf  :reference_publication-conclusion .

:optionally-consults  a  owl:ObjectProperty ;
        rdfs:label  "Optionally consults" .

:archive_package  a      owl:Class ;
        rdfs:comment     "The archive_package class is a generic class for compound digitised documents. As such it is a container for one or more digitised documents." ;
        rdfs:label       "Archive Package" ;
        rdfs:subClassOf  :container_work ;
        rdfs:subClassOf  [ a                   owl:Restriction ;
                           owl:maxCardinality  "1"^^xsd:nonNegativeInteger ;
                           owl:onProperty      :archive_package_reference_volume
                         ] ;
        rdfs:subClassOf  [ a                            owl:Restriction ;
                           owl:maxQualifiedCardinality  "1"^^xsd:nonNegativeInteger ;
                           owl:onDataRange              xsd:string ;
                           owl:onProperty               :archive_package_reference_internal
                         ] ;
        rdfs:subClassOf  [ a                   owl:Restriction ;
                           owl:maxCardinality  "1"^^xsd:nonNegativeInteger ;
                           owl:onProperty      :archive_package_internal_number_prefix
                         ] .

:resource_legal_extends_application_resource_legal
        a                   owl:ObjectProperty ;
        rdfs:comment        "This points to the legal act which application is extended. Relevant for legal analysis: true" ;
        rdfs:domain         :resource_legal ;
        rdfs:label          "Legal resource extends application of legal resource" ;
        rdfs:range          :resource_legal ;
        rdfs:subPropertyOf  :extends_application ;
        owl:inverseOf       :resource_legal_application_extended_by_resource_legal .

:procedure_without_code_interinstitutional_based_on_resource_legal
        a                   owl:ObjectProperty ;
        rdfs:comment        "DEPRECATED, Procedure is based on a legal resource (typically a treaty article, but could also be secondary legislation). Use in the future dossier_based_on_resource_legal. Legal basis (2). Relevant for legal analysis: true." ;
        rdfs:domain         :procedure_without_code_interinstitutional ;
        rdfs:label          "Procedure based on legal resource" ;
        rdfs:range          :resource_legal ;
        rdfs:subPropertyOf  :dossier_based_on_resource_legal , :based_on ;
        owl:deprecated      true ;
        owl:inverseOf       :resource_legal_basis_for_procedure_without_code_interinstitutional .

:is_logical_successor_of
        a           owl:ObjectProperty ;
        rdfs:label  "Is logical successor of" .

:resource_legal_repealed_by_resource_legal
        a                   owl:ObjectProperty ;
        rdfs:comment        "Relevant for legal analysis: true" ;
        rdfs:domain         :resource_legal ;
        rdfs:label          "Legal resource repealed by legal resource" ;
        rdfs:range          :resource_legal ;
        rdfs:subPropertyOf  :repealed_by ;
        owl:inverseOf       :resource_legal_repeals_resource_legal .

:incorporated_by  a  owl:ObjectProperty ;
        rdfs:label  "Incorporated by" .

<http://publications.europa.eu/resource/authority/fd_365>
        a       owl:NamedIndividual .

:act_other_oj_l  a       owl:Class ;
        rdfs:comment     "Other acts published in Official Journal L series (= subsector X of sector 4)" ;
        rdfs:label       "Other acts in OJ L" ;
        rdfs:subClassOf  :legislation_complementary .

:reference_member-state
        a           owl:DatatypeProperty ;
        rdfs:label  "Reference member state" .

:resource_legal_partially_suspends_resource_legal
        a                   owl:ObjectProperty ;
        rdfs:comment        "Partially_suspends and suspends could be handled as subcases of a shared super-property. SP (1) / subsequent related instrument. Relevant for legal analysis: true" ;
        rdfs:domain         :resource_legal ;
        rdfs:label          "Legal resource partially suspends legal resource" ;
        rdfs:range          :resource_legal ;
        rdfs:subPropertyOf  :partially_suspends ;
        owl:inverseOf       :resource_legal_partially_suspended_by_resource_legal .

:comment_converter  a  owl:DatatypeProperty ;
        rdfs:label  "Comment converter" .

:agent_comments_case-law
        a                   owl:ObjectProperty ;
        rdfs:comment        "Agent comments a judgement. OB" ;
        rdfs:domain         :agent ;
        rdfs:label          "Agent comments case law" ;
        rdfs:range          :case-law ;
        rdfs:subPropertyOf  :comments ;
        owl:inverseOf       :case-law_commented_by_agent .

:acknowledgment  a       owl:Class ;
        rdfs:comment     "\"A formal declaration of acknowledgment by the author in which persons and institutions are thanked for their part in the creation of a text\" (TEI 4.5)" ;
        rdfs:label       "Acknowlegement" ;
        rdfs:subClassOf  :front .

:expression_publication_general_duration
        a                   owl:DatatypeProperty ;
        rdfs:comment        "Duration / Extend of expression" ;
        rdfs:domain         :expression_publication_general ;
        rdfs:label          "Duration" ;
        rdfs:range          xsd:duration ;
        rdfs:subPropertyOf  :duration .

:resource_legal_id_obsolete_document
        a                   owl:DatatypeProperty ;
        rdfs:comment        "DEPRECATED, An obsolete identifier (id) that this legal resource may have. Use cdm:work_id_obsolete_document" ;
        rdfs:domain         :resource_legal ;
        rdfs:label          "Obsolete document identifier" ;
        rdfs:range          xsd:string ;
        rdfs:subPropertyOf  :id_obsolete_document ;
        owl:deprecated      true .

:concept_media_type  a   owl:Class ;
        rdfs:comment     "Corresponds to the contents of the MDR authority list media file type" ;
        rdfs:label       "Concept representing the media type of a file" ;
        rdfs:subClassOf  :concept_decoding .

dct:date  a     owl:AnnotationProperty .

:mandatorily-addresses
        a           owl:ObjectProperty ;
        rdfs:label  "Mandatorily addresses" .

:archive_package_ec  a   owl:Class ;
        rdfs:comment     "The archive_package_ec class is a generic class for scanned documents from the OIB HAS archives, done in the scope of digiCOM/digiSEC projects." ;
        rdfs:label       "Archive package from European Commission digitisation projects" ;
        rdfs:subClassOf  :archive_package , :act_preparatory_ec ;
        rdfs:subClassOf  [ a                            owl:Restriction ;
                           owl:maxQualifiedCardinality  "1"^^xsd:nonNegativeInteger ;
                           owl:onDataRange              xsd:boolean ;
                           owl:onProperty               :swd_package_ec_has_title_from_com_final
                         ] ;
        dct:created      "2022-09-01T09:01:22"^^xsd:dateTime .

:judgement_corrected_by
        a           owl:ObjectProperty ;
        rdfs:label  "Judgement corrected by" .

:event_legal_joint-responsibility_of_person
        a                   owl:ObjectProperty ;
        rdfs:comment        "Relevant for legal analysis: true. This legal event is under joint responsibility of a given person. Person role: Jointly responsible. Relevant for legal analysis: true" ;
        rdfs:domain         :event_legal ;
        rdfs:label          "Legal event under joint responsibility of person" ;
        rdfs:range          :person ;
        rdfs:subPropertyOf  :joint-responsibility_of , :event_joint-responsibility_of_person ;
        owl:deprecated      true ;
        owl:inverseOf       :person_jointly-responsible_for_event_legal .

:text-adopted_term_parliamentary
        a                   owl:DatatypeProperty ;
        rdfs:comment        "This indicates the Parliamentary term during which an EP document was voted or EP question was raised. Relevant for legal analysis: true. Currently coded with FD_Table 285. However, only codes are exposed (not decoded), so 01, 02 etc." ;
        rdfs:domain         :text-adopted ;
        rdfs:label          "Parliamentary term" ;
        rdfs:range          xsd:string ;
        rdfs:subPropertyOf  :term_parliamentary , :act_preparatory_term_parliamentary .

:institution_formally-addressed_by_event
        a            owl:ObjectProperty ;
        rdfs:domain  :institution ;
        rdfs:label   "Institution formally addressed by event" ;
        rdfs:range   :event .

:language_used_by_expression
        a                   owl:ObjectProperty ;
        rdfs:comment        "A given language is used by an expression" ;
        rdfs:domain         :language ;
        rdfs:label          "Language used by expression" ;
        rdfs:range          :expression ;
        rdfs:subPropertyOf  :used_by .

:procedure_internal_draft_to_be_published
        a                   owl:DatatypeProperty ;
        rdfs:comment        "Do the better_regulation_requirements require that the draft be published for this internal procedure? /ns4:ec_transmission_request/transmission/workflow/extension/ns3:better_regulation_requirements/ns3:draft_to_be_published" ;
        rdfs:domain         :procedure_internal ;
        rdfs:label          "Internal procedure needs draft to be published?" ;
        rdfs:range          xsd:boolean ;
        rdfs:subPropertyOf  :draft_to_be_published .

:manifestation_official-journal_part_year
        a                   owl:DatatypeProperty ;
        rdfs:comment        "Year of the act (as seen by the printer). values such as 2006, 1991,..." ;
        rdfs:domain         :manifestation_official-journal_part ;
        rdfs:label          "Year number of the act (decomposed)" ;
        rdfs:range          xsd:string ;
        rdfs:subPropertyOf  :year .

:date_processing  a         owl:DatatypeProperty ;
        rdfs:label          "Date processing" ;
        rdfs:range          xsd:date ;
        rdfs:subPropertyOf  :date .

:priority_class  a  owl:DatatypeProperty ;
        rdfs:label  "Priority class" .

:reproduction_of  a  owl:ObjectProperty ;
        rdfs:label  "Reproduction of" .

:dossier_related_to_dossier
        a                   owl:SymmetricProperty , owl:ObjectProperty ;
        rdfs:comment        "This dossier is related in some way to another dossier" ;
        rdfs:domain         :dossier ;
        rdfs:label          "Dossier related to dossier" ;
        rdfs:range          :dossier ;
        rdfs:subPropertyOf  :related_to .

:manifestation_official-journal-act_date_publication
        a                   owl:DatatypeProperty ;
        rdfs:comment        "Publication date of an Official Journal act's manifestation" ;
        rdfs:domain         :manifestation_official-journal-act ;
        rdfs:label          "Manifestation Official Journal act date publication" ;
        rdfs:range          xsd:date ;
        rdfs:subPropertyOf  :date_publication .

:case-law_national_affaire_year
        a                   owl:DatatypeProperty ;
        rdfs:comment        "DEPRECATED, Year of the affaire" ;
        rdfs:domain         :case-law_national ;
        rdfs:label          "National affaire: Year" ;
        rdfs:range          xsd:gYear ;
        rdfs:subPropertyOf  :affaire_year ;
        owl:deprecated      true .

:manifestation_case-law_costs_decisions
        a                   owl:DatatypeProperty ;
        rdfs:comment        "Cost decisions applied to this judgement. Sector 6 Text Index Field CO" ;
        rdfs:domain         :manifestation_case-law ;
        rdfs:label          "Cost decisions" ;
        rdfs:range          rdf:XMLLiteral ;
        rdfs:subPropertyOf  :costs_decisions .

:manifestation_isbn  a      owl:DatatypeProperty ;
        rdfs:comment        "ISBN of this manifestation" ;
        rdfs:domain         :manifestation ;
        rdfs:label          "isbn" ;
        rdfs:range          xsd:string ;
        rdfs:subPropertyOf  :isbn .

:derogated_by  a    owl:ObjectProperty ;
        rdfs:label  "Derogated by" .

:event_legal_is_about_concept_agenda_council
        a                   owl:ObjectProperty ;
        rdfs:comment        "Relevant for legal analysis: true. The subject of the legal event. Relevant for legal analysis: true" ;
        rdfs:domain         :event_legal ;
        rdfs:label          "Legal event is about prelex concept" ;
        rdfs:range          :concept_agenda_council ;
        rdfs:subPropertyOf  :is_about .

:official-forms_link_type
        a           owl:DatatypeProperty ;
        rdfs:label  "Official forms link type" .

:number_corrigendum  a  owl:DatatypeProperty ;
        rdfs:label  "Number corrigendum" .

<http://publications.europa.eu/resource/authority/pub_bind>
        a       owl:NamedIndividual .

:sp_package_ec  a        owl:Class ;
        rdfs:comment     "Internal documents of the European Commission with a SP type identifier, meanwhile declassified." ;
        rdfs:label       "SP package EC" ;
        rdfs:subClassOf  :swd_package_ec ;
        rdfs:subClassOf  [ a               owl:Restriction ;
                           owl:hasValue    "SP" ;
                           owl:onProperty  :archive_package_internal_number_prefix
                         ] ;
        dct:created      "2022-09-28T21:12:47Z"^^xsd:dateTime .

:report_special_eca  a   owl:Class ;
        rdfs:comment     "Court of Auditors special reports (5SA)" ;
        rdfs:label       "Court of Auditors special report" ;
        rdfs:subClassOf  :act_preparatory_eca .

:partially_adopts  a  owl:ObjectProperty ;
        rdfs:label  "Partially adopts" .

:report_ec  a            owl:Class ;
        rdfs:comment     "2573 Commission report (5DC with FM=RAPPORT)" ;
        rdfs:label       "Commission report" ;
        rdfs:subClassOf  :act_preparatory_ec .

:date_archived  a   owl:DatatypeProperty ;
        rdfs:label  "Date archived" .

:case-law_defended_by_agent
        a                   owl:ObjectProperty ;
        rdfs:comment        "This lists the defending party in Court proceeding (institutions, bodies, Member States, companies, individuals). Currently coded with FD_Table 110. The role of the defendant is expressed as property in the agent class." ;
        rdfs:domain         :case-law ;
        rdfs:label          "Case law defended by agent" ;
        rdfs:range          :agent ;
        rdfs:subPropertyOf  :defended_by ;
        owl:inverseOf       :agent_defends_in_case-law .

:heading_old  a     owl:DatatypeProperty ;
        rdfs:label  "Heading old" .

:dossier  a              owl:Class ;
        rdfs:label       "Dossier" ;
        rdfs:subClassOf  :period ;
        rdfs:subClassOf  [ a                owl:Restriction ;
                           owl:cardinality  "1"^^xsd:nonNegativeInteger ;
                           owl:onProperty   :dossier_type_reference
                         ] ;
        rdfs:subClassOf  [ a                   owl:Restriction ;
                           owl:maxCardinality  "1"^^xsd:nonNegativeInteger ;
                           owl:onProperty      :dossier_adopted-proposal
                         ] ;
        rdfs:subClassOf  [ a                owl:Restriction ;
                           owl:cardinality  "1"^^xsd:nonNegativeInteger ;
                           owl:onProperty   :dossier_year_reference
                         ] ;
        rdfs:subClassOf  [ a                   owl:Restriction ;
                           owl:maxCardinality  "1"^^xsd:nonNegativeInteger ;
                           owl:onProperty      :dossier_summary
                         ] ;
        rdfs:subClassOf  [ a                   owl:Restriction ;
                           owl:minCardinality  "1"^^xsd:nonNegativeInteger ;
                           owl:onProperty      :dossier_title
                         ] ;
        rdfs:subClassOf  [ a                            owl:Restriction ;
                           owl:minQualifiedCardinality  "1"^^xsd:nonNegativeInteger ;
                           owl:onClass                  :event ;
                           owl:onProperty               :dossier_contains_event
                         ] ;
        rdfs:subClassOf  [ a                   owl:Restriction ;
                           owl:maxCardinality  "1"^^xsd:nonNegativeInteger ;
                           owl:onProperty      :dossier_embargo
                         ] ;
        rdfs:subClassOf  [ a                   owl:Restriction ;
                           owl:maxCardinality  "1"^^xsd:nonNegativeInteger ;
                           owl:onProperty      :dossier_date_creation_legacy
                         ] ;
        rdfs:subClassOf  [ a                owl:Restriction ;
                           owl:cardinality  "1"^^xsd:nonNegativeInteger ;
                           owl:onProperty   cmr:lastModificationDate
                         ] ;
        rdfs:subClassOf  [ a                   owl:Restriction ;
                           owl:maxCardinality  "1"^^xsd:nonNegativeInteger ;
                           owl:onProperty      :dossier_mandatory_information_provided_by_work
                         ] ;
        rdfs:subClassOf  [ a                   owl:Restriction ;
                           owl:maxCardinality  "1"^^xsd:nonNegativeInteger ;
                           owl:onProperty      :dossier_date_withdrawn
                         ] ;
        rdfs:subClassOf  [ a                   owl:Restriction ;
                           owl:maxCardinality  "1"^^xsd:nonNegativeInteger ;
                           owl:onProperty      :dossier_pending-proposal
                         ] ;
        rdfs:subClassOf  [ a                owl:Restriction ;
                           owl:cardinality  "1"^^xsd:nonNegativeInteger ;
                           owl:onProperty   :dossier_number_reference
                         ] ;
        rdfs:subClassOf  [ a                   owl:Restriction ;
                           owl:maxCardinality  "1"^^xsd:nonNegativeInteger ;
                           owl:onProperty      :dossier_withdrawn-proposal
                         ] ;
        rdfs:subClassOf  [ a                   owl:Restriction ;
                           owl:maxCardinality  "1"^^xsd:nonNegativeInteger ;
                           owl:onProperty      :dossier_duration
                         ] ;
        rdfs:subClassOf  [ a                   owl:Restriction ;
                           owl:maxCardinality  "1"^^xsd:nonNegativeInteger ;
                           owl:onProperty      cmr:creationDate
                         ] ;
        rdfs:subClassOf  [ a                   owl:Restriction ;
                           owl:minCardinality  "1"^^xsd:nonNegativeInteger ;
                           owl:onProperty      :dossier_identifier
                         ] .

:monolanguage  a             owl:Class ;
        rdfs:label           "Monolanguage" ;
        rdfs:subClassOf      skos:Concept ;
        owl:equivalentClass  [ a               owl:Restriction ;
                               owl:hasValue    <http://publications.europa.eu/resource/authority/language> ;
                               owl:onProperty  skos:inScheme
                             ] .

:concept_class_court_national
        a                    owl:Class ;
        rdfs:comment         "Corresponds to the contents of the JURE field court/class.court. It can have the values: - Court of first instance - Court of appeal - Supreme court" ;
        rdfs:label           "Concept representing a Class of a National Court" ;
        rdfs:subClassOf      skos:Concept , :concept_decoding ;
        owl:equivalentClass  [ a               owl:Restriction ;
                               owl:hasValue    <http://publications.europa.eu/resource/authority/court-type> ;
                               owl:onProperty  skos:inScheme
                             ] .

:collection_work  a      owl:Class ;
        rdfs:comment     "This class is use to describe a serial work when the publication project is to publish various monographs belonging to a “collection” which gives the editorial line for the monographs." ;
        rdfs:label       "Collection work" ;
        rdfs:subClassOf  :serial_work .

:resource_legal_parent_document_ref
        a                   owl:DatatypeProperty ;
        rdfs:comment        "Parent document reference. Added in the context of IMMC2CDM-OJ" ;
        rdfs:domain         :resource_legal ;
        rdfs:label          "Reference to the parent document of a legal resource" ;
        rdfs:range          xsd:string ;
        rdfs:subPropertyOf  :parent_document_ref .

:was_historically_about
        a           owl:ObjectProperty ;
        rdfs:label  "Was historically about" .

:paragraph_legal_part_of_work
        a                   owl:ObjectProperty ;
        rdfs:comment        "This property associates an instance of a work with an instance of PARAGRAPH that forms part of it." ;
        rdfs:domain         :paragraph_legal ;
        rdfs:label          "Paragraph (legal) part of work" ;
        rdfs:range          :work ;
        rdfs:subPropertyOf  :subdivision_part_of_work , :part_of ;
        owl:inverseOf       :work_contains_paragraph_legal .

:rule_legal_part_of_work
        a                   owl:ObjectProperty ;
        rdfs:comment        "This property associates an instance of a work with an instance of a rule that forms part of it." ;
        rdfs:domain         :rule_legal ;
        rdfs:label          "Rule (legal) part of work" ;
        rdfs:range          :work ;
        rdfs:subPropertyOf  :subdivision_part_of_work , :part_of ;
        owl:inverseOf       :work_contains_rule_legal .

:dossier_basis_legal  a     owl:DatatypeProperty ;
        rdfs:comment        "A string representing a reference to a legal basis for the dossier. Relevant for legal analysis: to be verified." ;
        rdfs:domain         :dossier ;
        rdfs:label          "Dossier legal basis" ;
        rdfs:range          xsd:string ;
        rdfs:subPropertyOf  :basis_legal ;
        dct:created         "2018-11-02T15:08:43.836+01:00"^^xsd:dateTime .

:ATTO_FD_350  a              owl:Class ;
        rdfs:label           "FD_350 ATTO table" ;
        rdfs:subClassOf      skos:Concept ;
        owl:equivalentClass  [ a               owl:Restriction ;
                               owl:hasValue    <http://publications.europa.eu/resource/authority/fd_350> ;
                               owl:onProperty  skos:inScheme
                             ] .

:resource_legal_declared_valid_by_case-law
        a                   owl:ObjectProperty ;
        rdfs:comment        "Calculated. Relevant for legal analysis: true." ;
        rdfs:domain         :resource_legal ;
        rdfs:label          "Legal resource declared valid by case law" ;
        rdfs:range          :case-law ;
        rdfs:subPropertyOf  :declared_valid_by ;
        owl:inverseOf       :case-law_declares_valid_resource_legal .

:agent_defends_in_communication_cjeu
        a              owl:ObjectProperty ;
        rdfs:domain    :agent ;
        rdfs:label     "Agent defends in communication cjeu" ;
        rdfs:range     :communication_cjeu ;
        owl:inverseOf  :communication_cjeu_defended_by_agent .

:comment  a         owl:DatatypeProperty ;
        rdfs:label  "Comment" .

:act_other_eesc_reported_by_person
        a                   owl:ObjectProperty ;
        rdfs:comment        "Name of the person (EP member or member of CoR or EESC) who reports on the relevant act. This property will be deprecated and replaced with work_reported_by_person. Role RAPP. Relevant for legal analysis: true" ;
        rdfs:domain         :act_other_eesc ;
        rdfs:label          "European Economic and Social Committee other act has rapporteur" ;
        rdfs:range          :person ;
        rdfs:subPropertyOf  :work_reported_by_person ;
        dct:created         "2018-07-16T13:15:18.406+02:00"^^xsd:dateTime ;
        owl:inverseOf       :person_reports_on_act_other_eesc .

:case-law_is_about_concept_case-law
        a                   owl:ObjectProperty ;
        rdfs:comment        "Case law directory code is a specific directory classification for EU case law. This one refers to the classification used before Lisbon treaty. Currently coded with FD_578." ;
        rdfs:domain         :case-law ;
        rdfs:label          "Case law is about case law concept" ;
        rdfs:range          :concept_case-law ;
        rdfs:subPropertyOf  :is_about , :case-law_is_about_concept ;
        owl:inverseOf       :concept_case-law_subject_of_case-law .

:resolution  a           owl:Class ;
        rdfs:comment     "Resolution (subsector G of sector 3). At present 128 notices. Examples: 31962G0420(01), 32002G0124(01), 32009G1030(01)" ;
        rdfs:label       "Resolution" ;
        rdfs:subClassOf  :legislation_secondary .

:procedure_language  a  owl:DatatypeProperty ;
        rdfs:label  "Procedure language" .

:expression_incorporates_expression
        a                   owl:ObjectProperty ;
        rdfs:comment        "Relevant for legal analysis: true. This property associates an instance of Expression with an instance of Expression that was included in it and that is a realization of an independent work. Relevant for legal analysis: true" ;
        rdfs:domain         :expression ;
        rdfs:label          "Expression incorporates expression" ;
        rdfs:range          :expression ;
        rdfs:subPropertyOf  :incorporates ;
        owl:inverseOf       :expression_is_incorporated_in_expression .

:publication-accessibility
        a                    owl:Class ;
        rdfs:comment         "Corresponds to the contents of authority table publication-accessibility (http://publications.europa.eu/resource/authority/publication-accessibility)" ;
        rdfs:label           "Publication accessibility concept" ;
        rdfs:subClassOf      :concept_decoding ;
        owl:equivalentClass  [ a               owl:Restriction ;
                               owl:hasValue    <http://publications.europa.eu/resource/authority/publication-accessibility> ;
                               owl:onProperty  skos:inScheme
                             ] .

:opinion_requested_by
        a           owl:ObjectProperty ;
        rdfs:label  "Opinion requested by" .

:legal_effect_paper  a  owl:DatatypeProperty ;
        rdfs:label  "Legal effect paper" .

:does_deletion_of  a  owl:ObjectProperty ;
        rdfs:label  "Does deletion of" .

:resource_legal_basis_for_dossier
        a            owl:ObjectProperty ;
        rdfs:domain  :resource_legal ;
        rdfs:label   "Resource legal basis for dossier" ;
        rdfs:range   :dossier .

:published_in_erecueil
        a           owl:DatatypeProperty ;
        rdfs:label  "Published in erecueil" .

:directive_service_associated
        a                   owl:DatatypeProperty ;
        rdfs:comment        "This field indicates the Commission DG or DGs co-responsible for drafting of an act. DEPRECATED, In the instance data, the property is planned to be replaced with cdm:resource_legal_service_associated at beginning 2019. When this is done this property the property will be removed from CDM. Relevant for legal analysis: true" ;
        rdfs:domain         :directive ;
        rdfs:label          "Service associated" ;
        rdfs:range          xsd:string ;
        rdfs:subPropertyOf  :service_associated , :resource_legal_service_associated .

:communication_cjeu_has_type_procedure_concept_type_procedure
        a                   owl:ObjectProperty ;
        rdfs:comment        "This field refers to the type of action or procedure and the result of the action or procedure by Court proceedings the communication_cjeu published in OJ informs about. Currently coded by FD_Table 100. This property shall be replaced by: cdm:communication_cjeu_has_procjur (type of action or procedure) and annot:result_decision pointing to procresult. Relevant for legal analysis: true." ;
        rdfs:domain         :communication_cjeu ;
        rdfs:label          "Communication on case law that has a type of procedure" ;
        rdfs:range          :concept_type_procedure ;
        rdfs:subPropertyOf  :has_type_procedure .

:codified_version  a  owl:DatatypeProperty ;
        rdfs:label  "Codified version" .

:manifestation_official-journal_page_first
        a                   owl:DatatypeProperty ;
        rdfs:comment        "DEPRECATED, First page number of the OJ part related to a legal resource. Use manifestion_print_page_first" ;
        rdfs:domain         :manifestation_official-journal ;
        rdfs:label          "First page" ;
        rdfs:range          xsd:string ;
        rdfs:subPropertyOf  :page_first , :manifestation_print_page_first ;
        owl:deprecated      true .

:work_co-reported_by_person
        a                   owl:ObjectProperty ;
        rdfs:domain         :work ;
        rdfs:label          "Work co-reported by person" ;
        rdfs:range          :person ;
        rdfs:subPropertyOf  :co-reported_by ;
        owl:inverseOf       :person_co-reports_work .

:id_obsolete_notice  a      owl:DatatypeProperty ;
        rdfs:label          "Id obsolete notice" ;
        rdfs:subPropertyOf  :identifier .

:chapter_legal  a        owl:Class ;
        rdfs:comment     "A chapter in a legal document. Created to have correspondance to the subdivision NAL" ;
        rdfs:label       "Chapter (legal)" ;
        rdfs:subClassOf  :subdivision .

:refers_for_preliminary_ruling
        a           owl:ObjectProperty ;
        rdfs:label  "Refers for preliminary ruling" .

:manifestation_distribution_access_url
        a                   owl:DatatypeProperty ;
        rdfs:comment        "This property contains an URL that gives access to the distribution of a dataset. The resource at the access URL may contain information about how to get the Dataset" ;
        rdfs:domain         :manifestation_distribution ;
        rdfs:label          "Distribution access URL" ;
        rdfs:range          xsd:anyURI ;
        rdfs:subPropertyOf  :access_url .

:collection_document_contains_official-journal-act
        a                   owl:ObjectProperty ;
        rdfs:domain         :collection_document ;
        rdfs:label          "Collection Document contains Official Journal act" ;
        rdfs:range          :official-journal-act ;
        rdfs:subPropertyOf  :contains ;
        owl:inverseOf       :official-journal-act_part_of_collection_document .

:case-law_national_judgement_reference
        a                   owl:DatatypeProperty ;
        rdfs:comment        "Reference to a judgement, typically on the European level" ;
        rdfs:domain         :case-law_national ;
        rdfs:label          "Reference to a judgement" ;
        rdfs:range          xsd:string ;
        rdfs:subPropertyOf  :judgement_reference .

:declares_void  a   owl:ObjectProperty ;
        rdfs:label  "Declares void" .

:reference-data_asset
        a                owl:Class ;
        rdfs:comment     "A dataset representing a reference data asset like an authority table, a thesaurus, a taxonomy in all of its formats (provided in the different manifestations). When holding both this class and the cdm:evolutive_work class, the object is the representant of the asset in its latest version. The documentation of a publication is represented by a linked object with class cdm:documentation and refers to documentation on the represented asset as a whole and not for a specific version." ;
        rdfs:label       "Reference data asset" ;
        rdfs:subClassOf  :work_dataset ;
        rdfs:subClassOf  [ a                owl:Restriction ;
                           owl:cardinality  "1"^^xsd:nonNegativeInteger ;
                           owl:onProperty   :reference-data_asset_published_in_reference-data_publication
                         ] .

:preamble  a             owl:Class ;
        rdfs:label       "Preamble" ;
        rdfs:subClassOf  :subdivision .

:cited_by  a        owl:ObjectProperty ;
        rdfs:label  "Cited by" .

:concept_case-law_result
        a                owl:Class ;
        rdfs:label       "Concept representing the result of a case event" ;
        rdfs:subClassOf  :concept_decoding .

:institution_initiates_event
        a            owl:ObjectProperty ;
        rdfs:domain  :institution ;
        rdfs:label   "Institution initiates event" ;
        rdfs:range   :event .

:work_dataset_nature_classification
        a            owl:DatatypeProperty ;
        rdfs:domain  :work_dataset ;
        rdfs:label   "Work dataset nature classification" ;
        rdfs:range   xsd:anyURI .

:work_archived  a           owl:DatatypeProperty ;
        rdfs:comment        "This work is considered to be no longer applicable on the business level. The document remains visible even if archived" ;
        rdfs:domain         :work ;
        rdfs:label          "Work archived" ;
        rdfs:range          xsd:boolean ;
        rdfs:subPropertyOf  :archived .

:manifestation_print_reference
        a                owl:Class ;
        rdfs:comment     "Reference to a print manifestation or a part of a print manifestation. Not to be used for specific types of print publication references listed below" ;
        rdfs:label       "Reference to a print manifestation" ;
        rdfs:subClassOf  :manifestation_print ;
        rdfs:subClassOf  [ a                   owl:Restriction ;
                           owl:maxCardinality  "1"^^xsd:nonNegativeInteger ;
                           owl:onProperty      :manifestation_print_reference_volume
                         ] ;
        rdfs:subClassOf  [ a                   owl:Restriction ;
                           owl:maxCardinality  "1"^^xsd:nonNegativeInteger ;
                           owl:onProperty      :manifestation_print_reference_title
                         ] ;
        rdfs:subClassOf  [ a                   owl:Restriction ;
                           owl:maxCardinality  "1"^^xsd:nonNegativeInteger ;
                           owl:onProperty      :manifestation_print_reference_pages_total
                         ] ;
        rdfs:subClassOf  [ a                   owl:Restriction ;
                           owl:maxCardinality  "1"^^xsd:nonNegativeInteger ;
                           owl:onProperty      :manifestation_print_reference_page_last
                         ] ;
        rdfs:subClassOf  [ a                owl:Restriction ;
                           owl:cardinality  "1"^^xsd:nonNegativeInteger ;
                           owl:onProperty   :manifestation_print_reference_page_first
                         ] .

:archive_package_has_title_from_com_final
        a               owl:DatatypeProperty ;
        rdfs:comment    "indication if the title(s) of the package from the final document in the package or if the scanning provider (in absence of a final document) took the title from a substitute final document" ;
        rdfs:domain     :archive_package ;
        rdfs:label      "Archive package has title from COM final" ;
        rdfs:range      xsd:boolean ;
        owl:deprecated  true .

:event_legal_handed_over_person
        a                   owl:ObjectProperty ;
        rdfs:comment        "Relevant for legal analysis: true. This legal event is handed over by a given person. The XML contains two persons, the person handing over and the person taking over. This is the first of the two. Relevant for legal analysis: true" ;
        rdfs:domain         :event_legal ;
        rdfs:label          "Legal event handed over by person" ;
        rdfs:range          :person ;
        rdfs:subPropertyOf  :handed_over ;
        owl:inverseOf       :person_hands_over_event_legal .

:date_signature_xades-t
        a           owl:DatatypeProperty ;
        rdfs:label  "Date signature xades t" .

:resource_legal_does_impact_of_resource_legal
        a                   owl:ObjectProperty ;
        rdfs:comment        "Legal resources does impact a legal resource, in term of consolidation, the impact can be: deletion, insertion, renumbering, repeal and replacement" ;
        rdfs:domain         :resource_legal ;
        rdfs:label          "Legal resources does impact of legal resource" ;
        rdfs:range          :resource_legal ;
        rdfs:subPropertyOf  :does_impact_of .

:special-official-journal_second_series_historical
        a                   owl:DatatypeProperty ;
        rdfs:comment        "Used for english and danish special editions containing thematic volumes (the series \"II\"). FYI, the themes for the volumes of the second_series are like follows: I. External Relations II. Agriculture and Food Aid III. European Agricultural Guidance and Guarantee Fund IV.Transport IX. Resolutions of the Council and of the Representatives of the Member States V. Euratom VI. Competition (a) and (b) VII. Institutional questions VIII. European Coal and Steel Community X. Miscellaneous" ;
        rdfs:domain         :special-official-journal ;
        rdfs:label          "Second historical series" ;
        rdfs:range          xsd:string ;
        rdfs:subPropertyOf  :second_series_historical .

:case-law_refers_to_for_preliminary_ruling_case-law
        a              owl:ObjectProperty ;
        rdfs:domain    :case-law ;
        rdfs:label     "Case law refers to for preliminary ruling case law" ;
        rdfs:range     :case-law ;
        owl:inverseOf  :case-law_referred_to_for_preliminary_ruling_case-law .

:procurement_public_official-forms_link_title
        a                   owl:DatatypeProperty ;
        rdfs:domain         :procurement_public ;
        rdfs:label          "Link title for the official forms" ;
        rdfs:range          xsd:string ;
        rdfs:subPropertyOf  :official-forms_link_title .

:resource_legal_signatory_name2
        a                   owl:DatatypeProperty ;
        rdfs:comment        "Legal resource additional signatory name. Added in the context of IMMC2CDM-OJ. Relevant for legal analysis: true" ;
        rdfs:domain         :resource_legal ;
        rdfs:label          "Additional name of signatory of the legal resource" ;
        rdfs:range          xsd:string ;
        rdfs:subPropertyOf  :signatory_name2 .

:page_first  a      owl:DatatypeProperty ;
        rdfs:label  "Page first" .

:official-forms_link_title
        a           owl:DatatypeProperty ;
        rdfs:label  "Official forms link title" .

:uri    a           owl:DatatypeProperty ;
        rdfs:label  "Uri" .

:includes  a        owl:ObjectProperty ;
        rdfs:label  "Includes" .

:asks   a           owl:ObjectProperty ;
        rdfs:label  "Asks" .

<http://publications.europa.eu/resource/authority/fd_605>
        a       owl:NamedIndividual .

:manifestation_official-journal_part_volume_oj
        a                   owl:DatatypeProperty ;
        rdfs:comment        "Volume of the OJ part that this legal resource was published in. Exceptionally used for very long OJ's., e.g. for the budget to disambiguate page numbers, DEPRECATED, use manifestion_print_volume" ;
        rdfs:domain         :manifestation_official-journal_part ;
        rdfs:label          "Volume of the OJ" ;
        rdfs:range          xsd:string ;
        rdfs:subPropertyOf  :volume_oj ;
        owl:deprecated      true .

:cfsp   a                owl:Class ;
        rdfs:comment     "Common Foreign and Security Policy (CFSP). Subsector E of sector 3. At present 642 notices. Examples: 31994E0779, 32004E0794" ;
        rdfs:label       "Common Foreign and Security Policy" ;
        rdfs:subClassOf  :legislation_secondary .

:resource_legal_basis_referral
        a                   owl:DatatypeProperty ;
        rdfs:comment        "Basis / method of referral (mode de saisine) under which this legal resource was produced" ;
        rdfs:domain         :resource_legal ;
        rdfs:label          "Basis of referral" ;
        rdfs:range          xsd:string ;
        rdfs:subPropertyOf  :basis_referral .

:person_reports_on_act_other_ep
        a                   owl:ObjectProperty ;
        rdfs:domain         :person ;
        rdfs:label          "Person reports on act_other_ep" ;
        rdfs:range          :act_other_ep ;
        rdfs:subPropertyOf  :reports_on .

:case-law_refers_for_preliminary_ruling_case-law
        a                   owl:ObjectProperty ;
        rdfs:comment        "Used in sector 6 (EU case law) notices/ the value placed is the national judgment that was referred to the Court of Justice of the EU for the preliminary rulling" ;
        rdfs:domain         :case-law ;
        rdfs:label          "Case law refers for preliminary ruling to another case law" ;
        rdfs:range          :case-law ;
        rdfs:subPropertyOf  :refers_for_preliminary_ruling .

:year_procedure  a  owl:DatatypeProperty ;
        rdfs:label  "Year procedure" .

:directive  a            owl:Class ;
        rdfs:comment     "Subsector L of sector 3. At present 5330 notices. Examples: 31959L0221, 31961L1513, 31964L0433R(02), 32010L0016" ;
        rdfs:label       "Directive" ;
        rdfs:subClassOf  :legislation_secondary .

:event_internal_objection_period_extension
        a                   owl:DatatypeProperty ;
        rdfs:comment        "Possible extension to the period (in months) where the European Parliament and the Council have the right to object on a delegated act of the Commission" ;
        rdfs:domain         :event_internal ;
        rdfs:label          "Objection period extension" ;
        rdfs:range          xsd:positiveInteger ;
        rdfs:subPropertyOf  :objection_period_extension .

:order_cjeu  a           owl:Class ;
        rdfs:comment     "Order in sector 6 (6CO/6TO/6FO)" ;
        rdfs:label       "Court order" ;
        rdfs:subClassOf  :case-law .

:person_name  a             owl:NamedIndividual , owl:DatatypeProperty ;
        rdfs:comment        "Name of this person" ;
        rdfs:domain         :person ;
        rdfs:label          "Person name" ;
        rdfs:range          xsd:string ;
        rdfs:subPropertyOf  :name ;
        owl:sameAs          foaf:name .

:resource_legal_interpreted_by_judgement_case-law
        a                   owl:ObjectProperty ;
        rdfs:comment        "6 cases (2012-07-31). Example: 62007CA0402: \"interprets the judgment 32004R0261 Article 2 PT L)\". Relevant for legal analysis: true." ;
        rdfs:domain         :resource_legal ;
        rdfs:label          "Judgement interpreted by case law" ;
        rdfs:range          :case-law ;
        rdfs:subPropertyOf  :interpreted_by_judgement ;
        owl:inverseOf       :case-law_interpretes_judgement_resource_legal .

:budget  a               owl:Class ;
        rdfs:comment     "Subsector B of sector 3. At present 912 notices. Examples: 31970B0183,31979B0476.32010B0117R(01), 32010B0162" ;
        rdfs:label       "Budget" ;
        rdfs:subClassOf  :legislation_secondary .

<http://publications.europa.eu/resource/authority/fd_578>
        a       owl:NamedIndividual .

:manifestation_doi  a       owl:DatatypeProperty ;
        rdfs:comment        "DOI of this manifestation. mapped from 024 7 $a" ;
        rdfs:domain         :manifestation ;
        rdfs:label          "DOI of manifestation" ;
        rdfs:range          xsd:string ;
        rdfs:subPropertyOf  :doi .

:event_case_framework_procedural_identifier
        a                   owl:DatatypeProperty ;
        rdfs:comment        "The identifer of the procedural framework for the case event" ;
        rdfs:domain         :event_case ;
        rdfs:label          "Identifer of the procedural framework" ;
        rdfs:range          xsd:string ;
        rdfs:subPropertyOf  :framework_procedural_identifier .

:procresult  a               owl:Class ;
        rdfs:comment         "Corresponds to the procresult table" ;
        rdfs:label           "Concept representing the resoult of a judicial procedure (résultats de procédure)" ;
        rdfs:subClassOf      skos:Concept , :concept_decoding ;
        owl:equivalentClass  [ a               owl:Restriction ;
                               owl:hasValue    <http://publications.europa.eu/resource/authority/procresult> ;
                               owl:onProperty  skos:inScheme
                             ] .

:dossier_embargo  a         owl:DatatypeProperty ;
        rdfs:comment        "Is this dossier under embargo? This instance must not be shown until the indicated datetime has been reached. In case a release date is not known,9999-12-31 should be used (= absolute embargo)" ;
        rdfs:domain         :dossier ;
        rdfs:label          "Dossier embargo" ;
        rdfs:range          xsd:dateTime ;
        rdfs:subPropertyOf  :embargo .

:position_council  a     owl:Class ;
        rdfs:comment     "Council position after Lisbon treaty and its statement of reasons (= 5AG after 1.12.2009, entry into force of Lisbon Treaty). Its equivalent authority codes are POSIT for position in the OJ workflow (sent by the Council with the code \"ACT_LEGIS\" in the preleg flow) and STAT_REASON for Statement of reasons. Note: Council position in ATTO FD_030 is FM=PO, before the Lisbon treaty it was Council common position FM=POCO. Resource types mapped on this class for the Council: - STAT_REASON - STAT_REASON_DRAFT - POSIT - ACT_LEGIS (if cm:type_event is ADP_R1_POS_byCONSIL and type_interinstitutionaprocedure is OLP)" ;
        rdfs:label       "Council position" ;
        rdfs:subClassOf  :act_preparatory_council .

:case-law_affaire_jurisdiction
        a                   owl:DatatypeProperty ;
        rdfs:comment        "Jurisdiction of the affaire. coded" ;
        rdfs:domain         :case-law ;
        rdfs:label          "Affaire: Jurisdiction" ;
        rdfs:range          xsd:string ;
        rdfs:subPropertyOf  :affaire_jurisdiction .

:concept_case-law_subject_of_case-law
        a                   owl:ObjectProperty ;
        rdfs:domain         :concept_case-law ;
        rdfs:label          "Case law concept is subject of a case law" ;
        rdfs:range          :case-law ;
        rdfs:subPropertyOf  :subject_of ;
        owl:inverseOf       :case-law_is_about_concept_case-law .

:is_corrigendum_printer
        a           owl:DatatypeProperty ;
        rdfs:label  "Is corrigendum printer" .

:expression_edition  a      owl:DatatypeProperty ;
        rdfs:comment        "edition of this expression" ;
        rdfs:domain         :expression ;
        rdfs:label          "Expression edition" ;
        rdfs:range          xsd:string ;
        rdfs:subPropertyOf  :edition .

:expression_publication_general_scale
        a                   owl:DatatypeProperty ;
        rdfs:comment        "Scale, typically of a map (e.g. \"ca. 1:10,000\")" ;
        rdfs:domain         :expression_publication_general ;
        rdfs:label          "Scale" ;
        rdfs:range          xsd:string ;
        rdfs:subPropertyOf  :scale .

:requests_inapplicability
        a           owl:ObjectProperty ;
        rdfs:label  "Requests inapplicability" .

:incidentally_declared_valid
        a           owl:ObjectProperty ;
        rdfs:label  "Incidentally declared valid" .

<http://publications.europa.eu/resource/authority/fd_557>
        a       owl:NamedIndividual .

:requested_by  a    owl:ObjectProperty ;
        rdfs:label  "Requested by" .

:judgement  a            owl:Class ;
        rdfs:comment     "Judgement in sector 6 (6CJ/6TJ/6FJ)" ;
        rdfs:label       "Judgement" ;
        rdfs:subClassOf  :case-law .

:has_originally  a  owl:ObjectProperty ;
        rdfs:label  "Has originally" .

:procedure_internal_has_status
        a             owl:ObjectProperty ;
        rdfs:comment  "Status of an internal procedure" ;
        rdfs:domain   :procedure_internal ;
        rdfs:label    "Procedure internal has status" ;
        rdfs:range    :status .

:case_court_identifier_court
        a                   owl:DatatypeProperty ;
        rdfs:comment        "Code for the court in the case identifier. Possible values C, T or F, e.g. C" ;
        rdfs:domain         :case_court ;
        rdfs:label          "Identifier of the Court" ;
        rdfs:range          xsd:string ;
        rdfs:subPropertyOf  :identifier_court .

:resource_legal_term-of-office
        a                   owl:DatatypeProperty ;
        rdfs:comment        "Period of time, during which, members nominated by national governments and appointed by the Council of the European Union, are mandated to issue opinions on matters of European interest to the Council, the Commission and the European Parliament. The members are acting for a renewable 5-year term of office, can also serve other concepts.\"" ;
        rdfs:domain         :resource_legal ;
        rdfs:label          "Term of Office" ;
        rdfs:range          xsd:string ;
        rdfs:subPropertyOf  :term-of-office .

:institution_delivers_case-law
        a                   owl:ObjectProperty ;
        rdfs:domain         :institution ;
        rdfs:label          "Institution delivers case law" ;
        rdfs:range          :case-law ;
        rdfs:subPropertyOf  :delivers .

:period  a               owl:Class ;
        rdfs:comment     "\"This class comprises sets of coherent phenomena or cultural manifestations bounded in time and space. It is the social or physical coherence of these phenomena that identify an E4 Period and not the associated spatio-temporal bounds.\" (CIDOC CRM)" ;
        rdfs:label       "Period" ;
        rdfs:subClassOf  :entity_temporal ;
        rdfs:subClassOf  [ a                            owl:Restriction ;
                           owl:maxQualifiedCardinality  "1"^^xsd:nonNegativeInteger ;
                           owl:onClass                  :unit_administrative ;
                           owl:onProperty               :period_located_in_unit_administrative
                         ] .

:case-law_joins_case_court
        a                   owl:ObjectProperty ;
        rdfs:comment        "The case law joins a court case" ;
        rdfs:domain         :case-law ;
        rdfs:label          "Case law joins court case" ;
        rdfs:range          :case_court ;
        rdfs:subPropertyOf  :joins .

:staff-working-document_service_responsible
        a                   owl:DatatypeProperty ;
        rdfs:comment        "The Commission DG or DGs responsible for drafting of an act. DEPRECATED. In the instance data, the property is planned to be replaced with cdm:resource_legal_service_responsible at beginning 2019. When this is done this property will be removed from CDM. The Commission's DG that brought forward the proposal; to be taken from a closed list of DGs (that might be derived from the RECORD project ?). For the backlog data need to be completed. Cardinality to be restricted to 1 in the future." ;
        rdfs:domain         :staff-working-document ;
        rdfs:label          "Service responsible" ;
        rdfs:range          xsd:string ;
        rdfs:subPropertyOf  :service_responsible , :resource_legal_service_responsible ;
        owl:deprecated      true .

:resource_legal_year  a     owl:DatatypeProperty ;
        rdfs:comment        "Year of the legal resource in celex identifier (DTA). Relevant for legal analysis: true" ;
        rdfs:domain         :resource_legal ;
        rdfs:label          "Year of the legal resource" ;
        rdfs:range          xsd:gYear ;
        rdfs:subPropertyOf  :year .

:signed_by  a       owl:ObjectProperty ;
        rdfs:label  "Signed by" .

:manifestation_print_pages_total
        a                   owl:DatatypeProperty ;
        rdfs:comment        "Total number of pages of the OJ part related to a legal resource" ;
        rdfs:domain         :manifestation_print ;
        rdfs:label          "Total pages" ;
        rdfs:range          xsd:string ;
        rdfs:subPropertyOf  :pages_total .

<http://publications.europa.eu/resource/authority/fd_600>
        a       owl:NamedIndividual .

:container_case-law_number
        a                   owl:DatatypeProperty ;
        rdfs:domain         :container_case-law ;
        rdfs:label          "Sequential number" ;
        rdfs:range          xsd:string ;
        rdfs:subPropertyOf  :number .

:uses   a             owl:ObjectProperty ;
        rdfs:comment  "An entity uses another one" ;
        rdfs:label    "Uses" .

:follow-up  a       owl:DatatypeProperty ;
        rdfs:label  "Follow up" .

:interpretes_authoritatively
        a           owl:ObjectProperty ;
        rdfs:label  "Interpretes authoritatively" .

:ATTO_FD_611  a              owl:Class ;
        rdfs:label           "FD_611 ATTO table" ;
        rdfs:subClassOf      skos:Concept ;
        owl:equivalentClass  [ a               owl:Restriction ;
                               owl:hasValue    <http://publications.europa.eu/resource/authority/fd_611> ;
                               owl:onProperty  skos:inScheme
                             ] .

:joint-responsibility_of
        a           owl:ObjectProperty ;
        rdfs:label  "Joint responsibility of" .

:scale  a           owl:DatatypeProperty ;
        rdfs:label  "Scale" .

:compiled_by  a     owl:ObjectProperty ;
        rdfs:label  "Compiled by" .

:procedure_type  a  owl:DatatypeProperty ;
        rdfs:label  "Procedure type" .

:question_parliamentary_nationality_mep
        a                   owl:DatatypeProperty ;
        rdfs:comment        "Nationality of MEP asking a question. Refers to the nationality of the member of the European Parliament who asked the question. It is mandatory for Parliamentary questions Relevant for legal analysis: true. Currently coded by FD Table 289, could also be a link to a country. Example: 92004E1202. AF (1). AF_GROUP and AF_NAT occur together.\" Relevant for legal analysis: true" ;
        rdfs:domain         :question_parliamentary ;
        rdfs:label          "Nationality of MEP" ;
        rdfs:range          xsd:string ;
        rdfs:subPropertyOf  :nationality_mep .

:resource_legal_date_request_caducity
        a                   owl:DatatypeProperty ;
        rdfs:comment        "Date at which a request for caducity was launched" ;
        rdfs:domain         :resource_legal ;
        rdfs:label          "Date of request for caducity" ;
        rdfs:range          xsd:date ;
        rdfs:subPropertyOf  :date_request_caducity .

:manifestation_number_catalogue_global
        a                   owl:DatatypeProperty ;
        rdfs:comment        "cataglogue number of this manifestation (typically, if it is a general publication). In Formex e.g. <NO.CAT.GLOBAL>QDAB10001ENC</NO.CAT.GLOBAL>. \"The NO.CAT.GLOBAL element is used to mark up the catalogue number for a whole publication which is available in various volumes which are identified separately\"" ;
        rdfs:domain         :manifestation ;
        rdfs:label          "Global catalogue number" ;
        rdfs:range          xsd:string ;
        rdfs:subPropertyOf  :number_catalogue_global .

:directive_implemented_by_measure_national_implementing
        a                   owl:ObjectProperty ;
        rdfs:comment        "Relevant for legal analysis: true" ;
        rdfs:domain         :directive ;
        rdfs:label          "Directive implemented by national implementing measure" ;
        rdfs:range          :measure_national_implementing ;
        rdfs:subPropertyOf  :resource_legal_implemented_by_measure_national_implementing , :implemented_by ;
        owl:inverseOf       :measure_national_implementing_implements_directive .

:source  a          owl:DatatypeProperty ;
        rdfs:label  "Source" .

:spatial  a         owl:ObjectProperty ;
        rdfs:label  "Spatial" .

:object_ccr  a           owl:Class ;
        rdfs:label       "CCR object" ;
        rdfs:subClassOf  :manifestation .

:documentation_has_type_concept_type_documentation
        a                   owl:ObjectProperty ;
        rdfs:comment        "This property indicates the type of documentation" ;
        rdfs:domain         :documentation ;
        rdfs:label          "Type of documentation" ;
        rdfs:range          :concept_type_documentation ;
        rdfs:subPropertyOf  :has_type .

:document_cjeu_published_in_court-report
        a                   owl:ObjectProperty ;
        rdfs:comment        "Case law published in Reports. DEPRECATED; The court document is published in a given edition of the Court report" ;
        rdfs:domain         :document_cjeu ;
        rdfs:label          "Court document published in the Court report" ;
        rdfs:range          :court-report ;
        rdfs:subPropertyOf  :published_in ;
        owl:deprecated      true .

:ATTO_FD_499  a              owl:Class ;
        rdfs:label           "FD_499 ATTO table" ;
        rdfs:subClassOf      skos:Concept ;
        owl:equivalentClass  [ a               owl:Restriction ;
                               owl:hasValue    <http://publications.europa.eu/resource/authority/fd_499> ;
                               owl:onProperty  skos:inScheme
                             ] .

:item_identifier  a         owl:DatatypeProperty ;
        rdfs:comment        "Identifier of this data stream" ;
        rdfs:domain         :item ;
        rdfs:label          "Item or content identifier" ;
        rdfs:range          xsd:string ;
        rdfs:subPropertyOf  :identifier .

:case-law_national_act_reference_international
        a                   owl:DatatypeProperty ;
        rdfs:comment        "Reference to an international convention applied in the national judgment, e.g. INT. - European Convention for the Protection of Human Rights and Fundamental Freedoms of 4 November 1950, Article 7. Use an XML structure to capture the sequence of references" ;
        rdfs:domain         :case-law_national ;
        rdfs:label          "Reference to an international convention" ;
        rdfs:range          rdf:XMLLiteral ;
        rdfs:subPropertyOf  :act_reference_international .

:event_legal  a          owl:Class ;
        rdfs:comment     "Any activity in a legislative process involving a recognizable author and often a recipient . The following types of legal events currently exist (event/id, table Events): || TR_TYPE_EVENEMENT_ABR || TR_TYPE_EVENEMENT_DNM || TYPE_EVENEMENT_CODE || TYPE_EVENEMENT_ID || | Consultation EESC by Comm. | Consultation of European Economic and Social Committee by Commission | CESECOM | 101697 | | Communication du Parlement européen sur les suites données | EP communication on action taken | AAAA | 400026 | | Joint Committee Decision | Decision of the Joint Committee | AAAA | 400027 | | Adoption by EP | Adoption by EP | ADPE | 1290 | | Partial adoption by Council | Partial adoption by Council | APPCS | 1295 | | Court of Justice judgment | Court of Justice judgment | ARCJ | 1310 | | Self-referral by COR | Self-referral by Committee of Regions | AUCDR | 1320 | | European Central Bank opinion | European Central Bank opinion | ABCE | 1325 | | ECSC Consultative Com. opinion | ECSC Consultative Committee opinion | ACCC | 1330 | | ESC opinion | Economic and Social Committee opinion | ACES | 1345 | | Monetary Committee opinion | Monetary Committee opinion | ACMO | 1350 | | Council assent | Council assent | AVCCS | 1355 | | EP assent | EP assent | AVCPE | 1360 | | Council opinion | Council opinion | AVCS | 1365 | | Council opinion budgetary act | Council opinion on budgetary act | ACSAB | 1370 | | Court of Justice opinion | Court of Justice opinion | ACJCE | 1375 | | Court of Auditors opinion | Court of Auditors opinion | ACC | 1380 | | No adoption by Council | No adoption by Council | AACS | 1015 | | No EP opinion at 2nd rdg | No EP opinion on 2nd reading | AAPE2 | 1030 | | Council agreement | Council agreement | APCS | 1235 | | Pol. agreement common position | Agreement on Council common position | APPCCS | 1240 | | Approval by Commission | Approval by Commission | APCOM | 10005 | | Consultation EP by Commission | Consultation European Parliament by Commission | PECOM | 100134 | | Association Council decision | Association Council decision | DECASS | 100154 | | Joint Committee decision | Joint Committee decision | DECOMIX | 100155 | | ACP-EC Coun Ministers Decision | Decision of the ACP-EC Council of Ministers | DECCM | 100434 | | Adoption by Commission | Adoption by Commission | ADC | 1265 | | Adoption of act by Commission | Adoption of act by Commission | ARRCOM | 1315 | | Discussions at Council | Discussions in Council | DISCUSSION | 101234 | | Supplement | Supplement | COMPL | 1470 | | Decision ACP-EC Commit. Ambas. | Decision of the ACP-EC Committee of Ambassadors | DECAMB | 101154 | | Decision Cooperation Committee | Decision of the Cooperation Committee | DECCOOP | 101155 | | Joint Council decision | Joint Council decision | DCCJ | 101214 | | ESC exploratory opinion | Economic and Social Committee exploratory opinion | AECES | 101475 | | Council resolution | Council resolution | RESCS | 100034 | | Council approval 2nd rdg | Council approval on 2nd reading | APRCS2 | 101556 | | Council approval 1st rdg | Council approval on 1st reading | APRCS1 | 101555 | | Council partial approv. 1st rdg | Council partial approval on 1st reading | APRPCS1 | 101557 | | Council partial approv. 2. rdg | Council partial approval on 2nd reading | APRPCS2 | 101558 | | EESC opinion | European Economic and Social Committee opinion | ACESE | 101675 | | EESC own-initiative opinion | European Economic and Social Committee own-initiative opinion | AICESE | 101676 | | EESC exploratory opinion | European Economic and Social Committee exploratory opinion | AECESE | 101677 | | EESC resolution | European Economic and Social Committee resolution | RESCESE | 101678 | | Decision on follow-up action | Decision on follow-up action | AAAA | 400025 | | Commission communication on the action taken | Commission communication on the action taken | AAAA | 400028 | | Signature of budget by EP | Signature of budget by EP | SIGNBUD | 1810 | | Transmis. re-exam. prop. to CS | Transmission of the re-examined proposal to the Council | TCSREX | 1835 | | Transm. amended prop. to EP | Transmission to EP of amended proposal | TPEM | 1845 | | Cooperation Council decision | Cooperation Council decision | DECCO | 100275 | | EP Cttee report 1st rdg | EP Committee report on 1st reading | RCPE1 | 1700 | | EP Cttee report 2nd rdg | EP Committee report on 2nd reading | RCPE2 | 1705 | | EP Cttee report 3rd rdg | EP Committee report on 3rd reading | RCPE3 | 1710 | | EP Cttee report on assent | EP Committee report on assent | RCPEAVC | 1715 | | EP Cttee report - resolution | EP Committee report - resolution | RCPEAI | 1720 | | EP Cttee report single rdg | EP Committee report on single reading | RCPEUN | 1725 | | EP Cttee report budgetary act | EP Committee report on budgetary act | RCPEAC | 1730 | | Replacement | Replacement | REMPL | 1755 | | Implicit replacement | Implicit replacement | REMPLI | 1760 | | Partial replacement | Partial replacement | REMPLP | 1765 | | Partial signature by EP and Council | Partial signature by EP and Council | SPPECS | 101902 | | Opinion of the European Data Protection Supervisor | Opinion of the European Data Protection Supervisor | PE | 101901 | | Consultation of EP | Consultation of European Parliament by Council | CONSPE | 1540 | | Convening Conciliation Comm. | Convening of Conciliation Committee | CONVCCO | 1545 | | Corrigendum | Corrigendum | CORR | 1550 | | Conciliation Comm. decision | Conciliation Committee decision | DECCCO | 1570 | | Council decision at 3rd rdg | Council decision on 3rd reading | DCCS3 | 1575 | | Cncl decision budgetary act | Council decision on budgetary act | DCSAB | 1580 | | EP decision budgetary discharg | European Parliament decision on budgetary discharge | DECHBUD | 1585 | | EP decision on 3rd rdg | EP decision on 3rd reading | DECPE3 | 1590 | | EP decision on budgetary act | EP decision on budgetary act | DPEAB | 1595 | | Discuss. budget Council 1st rdg | Discussion of budget by Council on 1st reading | BUDCS1 | 1605 | | Discuss. budget EP 1st rdg | Discussion of budget by EP on 1st reading | BUDPE1 | 1615 | | EP discuss. budget 2nd rdg | Discussion of budget by EP on 2nd reading | BUDPE2 | 1620 | | ESC own-initiative opinion | Economic and Social Committee own-initiative opinion | AICES | 1425 | | EMI opinion | European Monetary Institute opinion | AIME | 1435 | | EP opinion 1st rdg | EP opinion on 1st reading | APE1 | 1440 | | EP opinion 2nd rdg | EP opinion on 2nd reading | APE2 | 1445 | | Transmission to EP | Transmission to European Parliament | TPE | 1895 | | Trans. EP decl. cmn posn | Transmission to EP of declaration on common position | TPEDPC | 1900 | | Adoption common position | Adoption of common position by Council | APCCS | 1300 | | Council conclusions | Council conclusions | CONCS | 1475 | | Discuss. budget Council 2nd rdg | Discussion of budget by Council on 2nd reading | BUDCS2 | 1610 | | Committ. of Regions resolution | Committee of Regions resolution | RESCDR | 1775 | | ESC resolution | Economic and Social Committee resolution | RESCES | 1780 | | EP resolution | EP resolution | RESPE | 1785 | | Withdrawal by Commission | Withdrawal by Commission | RCOM | 1790 | | Partial withdrawal by Commiss. | Partial withdrawal by Commission | RPCOM | 1795 | | Signature by EP and Council | Signature by EP and Council | SIGNPECS | 1815 | | Trans. Council decl. cmn posn | Transmission to Council of declaration on common position | TCSDPC | 1830 | | Transm. re-exam.prop. to EP | Transmission to EP of re-examined proposal | TPEREX | 1850 | | Transmission to Council | Transmission to Council | TCS | 1880 | | Trans. amend. prop. to Council | Transmission of the amended proposal to the Council | TCSM | 1890 | | Information EP rejection 2nd rdg | Information concerning EP rejection on 2nd reading | IRPE | 1675 | | Commission position on EP amendments on 2nd reading | Commission position on EP amendments on 2nd reading | PCOM2 | 1685 | | Commission position on EP amendments on 1st reading | Commission position on EP amendments on 1st reading | PCOM1 | 1690 | | Outlook opinion of the Committee of the Regions | Outlook opinion of the Committee of the Regions | OUTOCOMR | 400090 | | Commission position on EP amendments on single reading | Commission position on EP amendments on single reading | PCOMUN | 1695 | | EP receipt of common position | Receipt by EP of Council common position | RPEPC | 1745 | | Rejection by Council | Rejection by Council | RJCS | 1750 | | EP opinion single rdg | EP opinion on single reading | APEUN | 1450 | | EP opinion on budgetary act | EP opinion on budgetary act | APEAB | 1455 | | Change of legal basis by Comm. | Change of legal basis by Commission | CBJCOM | 1460 | | Change of legal basis by Cncl | Change of legal basis by Council | CBJCS | 1465 | | Transm. EP Commiss. opinion | Transmission to EP of Commission opinion on EP amendments on 2nd reading | TPEAPE | 1840 | | Addendum | Addendum | ADD | 1250 | | Formal adoption by Council | Adoption by Council | AFCS | 1260 | | Adopt. declaration comn posit. | Adoption by Commission of declaration on common position | ADDPC | 1275 | | Adoption amended proposal | Adoption by Commission of amended proposal | ADCM | 1280 | | Adoption re-examined proposal | Adoption by Commission of re-examined proposal | ADCREX | 1285 | | Trans. Council Comm. opinion | Transmission to Council of Commission opinion on EP amendments on 2nd reading | TCSAPE | 1885 | | EIB opinion | European Investment Bank opinion | ABEI | 100875 | | Transmission to European Ombudsman | Transmission to European Ombudsman | TME | 101775 | | Adoption of Commission opinion | Adoption by Commission of opinion on EP amendments on 2nd reading | AVISCOM | 1270 | | CDR own-initiative opinion | Committee of Regions own-initiative opinion | AICDR | 1420 | | Committee of Regions opinion | Committee of Regions opinion | ACDR | 1335 | | Consultation of ESC | Consultation of Economic and Social Committee | CONSCES | 1520 | | Consultation Court of Justice | Consultation of Court of Justice by Council | CONSCJ | 1525 | | Consultation Monetary Committ. | Consultation of Monetary Committee by Council | CONSCMO | 1530 | | Consultation of EMI | Consultation of European Monetary Institute by Council | CONSIME | 1535 | | EP Cttee opinion 1st rdg | EP Committee opinion on 1st reading | ACPE1 | 1385 | | EP Cttee opinion 2nd rdg | EP Committee opinion on 2nd reading | ACPE2 | 1390 | | EP Cttee opinion 3rd rdg | EP Committee opinion on 3rd reading | ACPE3 | 1395 | | EP Cttee opinion on assent | EP Committee opinion on assent | AVCPEAVC | 1400 | | EP Cttee opinion - resolution | EP Committee opinion - resolution | AVCPEAI | 1405 | | CPE opinion single rdg | EP Committee opinion on single reading | ACPEUN | 1410 | | EP Cttee opinion budgetary act | EP Committee opinion on budgetary act | ACPEAB | 1415 | | Confirmation common position | Confirmation of common position by Council | CONPCCS | 1480 | | Consultation ECB | Consultation of the European Central Bank by the Council | CONSBCE | 1485 | | Consultation Court of Auditors | Consultation of Court of Auditors by Council | CONSCC | 1490 | | Consultation ESC by Comm. | Consultation of Economic and Social Committee by Commission | CESCOM | 1515 | | Consultation of EESC | Consultation of European Economic and Social Committee | CONSCESE | 101696 | The following changes come into effect following entry into force of the Lisbon Treaty * 400095: Changes following entry into force of the Lisbon Treaty * 400097: Adoption of Council's position at 1st reading * 400112: Adoption by Commission of its communication on Council's position at 1st reading * 400113: Transmission to Council of Commission communication on Council's position at 1st reading * 400114: Transmission to Parliament of Commission communication on Council's position at 1st reading * 400108: Receipt by the European Parliament of the Council's position at 1st reading * 400107: Withdrawal by the Commission following entry into force of the Lisbon Treaty Decision modes in Prelex (== event/mode_decision, table decision_mode): || MODE_DECISION_ID || TR_MODE_DECISION_ABR || TR_MODE_DECISION_CODE || TR_MODE_DECISION_DNM || | 1005 | Oral procedure | ORALE | Oral procedure | | 1010 | Written procedure | ECRITE | Written procedure | | 1015 | Empowerment procedure | HABIL. | Empowerment procedure | | 1020 | Adoption without debate | SSDEB | Adoption without debate | | 1025 | Procedure without report | PSR | Procedure without report | | 1030 | Qualified majority | MAJQUAL | Qualified majority | | 1035 | Unanimity | UNANIMITE | Unanimity | | 100001 | Procedure without debate | PSD | Procedure without debate | | 100040 | Majority | MAJ | Majority | | 100060 | Delegation procedure | DELEGATION | Delegation procedure | Decision types in Prelex (event/decision/id, table decision): || DECISION_ID || LANGUE_CODE || TR_DECISION_ABR || TR_DECISION_CODE || TR_DECISION_DNM || | 1005 | EN | Approval without amendment | APSAAM | Approval without amendment | | 1010 | EN | Approval with amendments | APAVAM | Approval with amendments | | 1015 | EN | Sending to parliamentary committee | REPR | Sending to parliamentary committee | | 1020 | EN | Agreement | ACTOAM | Agreement | | 1025 | EN | Partial agreement | ACCEAM | Partial agreement | | 1030 | EN | Refusal | RETOAM | Refusal | | 1035 | EN | Approval | APPROB. | Approval | | 1040 | EN | Approv. of Con.Cte joint text | APPRJCCO | Approval of joint text of Conciliation Committee | | 1045 | EN | Reject. Conc. Cttee joint text | RJPRJCCO | Rejection of joint text of Conciliation Committee | | 1050 | EN | Agreement on joint text | ACCPROJ | Agreement on joint text | | 1055 | EN | No agreement on joint text | ABSACCPROJ | No agreement on joint text | | 1060 | EN | Approval of joint text | APPRJCOM | Approval of joint text | | 1065 | EN | Rejection of joint text | RJPRJCOM | Rejection of joint text | | 1070 | EN | Adoption | ADOPTION | Adoption | | 1075 | EN | Amendment | AMENDEMENT | Amendment | | 10000 | EN | Reject.of confir. comm. posit. | RPEPC | Rejection of confirmed common position | | 20000 | EN | Follow-up action | SUITE | Follow-up on a non-legislative opinion | | 20001 | EN | No follow-up | PAS SUITE | No follow-up on a non-legislative opinion | | 100040 | EN | Amending opinion | AVMOD | Amending opinion | | 100041 | EN | Non-amending opinion | AVNMOD | Non-amending opinion | | 100042 | EN | Waiting | ATTENTE | Waiting | | 100043 | EN | Rejection | 100043 | Rejection | Remarks in Prelex (event/remarks, table remark): || DESCRIPTEUR_ID || LANGUE_CODE || TR_DESCRIPTEUR_ABR || TR_DESCRIPTEUR_CODE || TR_DESCRIPTEUR_DNM || | 1005 | EN | Procedure terminated | AF | Procedure terminated | | 1020 | EN | CHANG. LEGAL BASIS by LET/AA/.. | CLBLET/aa/ | Change of legal basis by LET/87/.. | | 1025 | EN | Automatic conciliation | CDD | Automatic conciliation | | 1030 | EN | Conciliation not suggest. Comm | CNSCOM | Conciliation not suggested by Commission | | 1035 | EN | Possible conciliation | CP | Possible conciliation | | 1040 | EN | Confidential | CONF | Confidential | | 1045 | EN | European Council | CSE | European Council | | 1060 | EN | Downgr. from conf. to internal | DECOFIN | Downgraded from confidential to internal | | 1065 | EN | Downgr. from secr. to internal | DESECIN | Downgraded from secret to internal | | 1070 | EN | Internal | IN | Internal | | 1075 | EN | White Paper | LB | White Paper | | 1080 | EN | EUR-OP | OPOCE | EUR-OP | | 1100 | EN | Proposal adopted in parts | PAP | Proposal adopted in parts | | 1105 | EN | Proposal not adopted | PNAP | Proposal not adopted | | 1110 | EN | Proposal partially adopted | PPA | Proposal partially adopted | | 1115 | EN | Restricted | RES | Restricted | | 1120 | EN | Secret | SEC | Secret | | 1155 | EN | Follow-up EP opin.2nd rdg | SAVPE2L | Follow-up to EP opinion on 2nd reading | | 1195 | EN | EP opinion given by EPC | APECPE | EP opinion given by EPC | | 1210 | EN | Opin.deliv. after adopt.by Cnc | ARAACS | Opinion delivered after adoption by Council | | 1215 | EN | Conciliation requested by EP | CDPE | Conciliation requested by EP | | 1220 | EN | Conciliation not requested EP | CNDPE | Conciliation not requested by EP | | 1225 | EN | Conciliation possible for EP | CPPE | Conciliation possible for EP | | 1230 | EN | Request for withdrawal | DRET | Request for withdrawal | | 1235 | EN | Undertaking respected | ER | Undertaking respected | | 1240 | EN | Undertkg respected 2nd rd | ER2 | Undertaking respected after 2nd reading | | 1250 | EN | Prop. upheld by Comm | PMCOM | Prop. upheld by Comm | | 1255 | EN | Prop. upheld by Comm 2nd reading | PMCOM2 | Prop. upheld by Comm 2nd reading | | 1260 | EN | EP part.renunc. of conciliat. | RPPEC | Partial renunciation of conciliation by EP | | 1265 | EN | Change of legal basis Council | CBJCS | Change of legal basis by Council | | 1270 | EN | Change of type by Council | CTYCS | Change of type by Council | | 1275 | EN | Conciliation refused by Cncl | CRCS | Conciliation refused by Council | | 1280 | EN | Conciliation accepted by Counc | CACS | Conciliation accepted by Council | | 1285 | EN | Consultation of EP on initiative of Council | CPEICS | Consultation of EP on initiative of Council | | 1290 | EN | Consultation of ESC on initiative of Council | CECIS | Consultation of ESC on initiative of Council | | 1305 | EN | LATE TRANSMISSION | TT | LATE TRANSMISSION | | 1545 | EN | Follow-up Council proceedings | STRVCS | Follow-up to Council proceedings | | 1555 | EN | Follow-up CFI judgment | SARTR1 | Follow-up to Court of First Instance judgment | | 1560 | EN | Follow-up COR opinion | SAVCDR | Follow-up to Committee of the Regions opinion | | 1565 | EN | Follow-up to Court of Auditors | SAVCC80 | Follow-up to Court of Auditors opinion | | 1585 | EN | Follow-up Court Justice jdgt | SARCJ | Follow-up to Court of Justice judgment | | 1625 | EN | Follow-up Court of Justice op. | SAVCJ94 | Follow-up to Court of Justice opinion | | 10000 | EN | EP renunciation of conciliat. | RPEC | Renunciation of conciliation by EP | | 10001 | EN | MEMORANDUM COMP. 78/111 | MEMO78/111 | COMPLEMENTARY MEMORANDUM 78/111 | | 10002 | EN | EP sending to EPC | REV PE CPE | EP sending to EPC | | 100023 | EN | Social protocol | PROT | Social protocol | | 100064 | EN | Follow-up CFI jdgt 98 | SART1L9 | Follow-up to Court of First Instance judgment 98 | | 100246 | EN | AGENDA 2000 | A2000 | AGENDA 2000 | | 100343 | EN | Follow-up Commission decision | SDCCOM | Follow-up to Commission decision | | 100363 | EN | Follow-up Council discussions | SDSCS | Follow-up to Council discussions | | 100383 | EN | CHANG. LEGAL BASIS by EP and Cnc | CBJPECS | Change of legal basis by EP and Cnc | | 100423 | EN | Follow-up to EP opinion | SAVPE | Follow-up to EP opinion | | 100424 | EN | Follow-up to ESC opinion | SAVCES | Follow-up to Economic and Social Committee opinion | | 100463 | EN | Follow-up to EESC opinion | SAVCESE | Follow-up to EESC opinion | Bibliographic references are encoded through the table series: || Sigle || Full title || | 1,2,3,4,5 | Old European Parliament documents | | A2,A3,A4,A5, A6 | Reports adopted in Parliamentary committee | | B4,B5 | Documents for European Parliament plenary session | | BULL | Bulletin of the European Union | | C | Commission document relating to official acts within the Commission's own areas of responsibility (\"autonomous acts\"). Some of these are sent to the Council or Parliament for information, in which case they are cited in PreLex. | | C2,C3,C4, C5 | Documents from the other institutions, distributed by the European Parliament | | CES-CESE | Opinion of the European Economic and Social Committee | | COM | Commission documents for the other institutions (legislative proposals, communications, reports, etc.) | | COR | Opinion of the Committee of the Regions | | CSE | Old documents for the European Council | | IP | Commission press releases | | JO | Official Journal | | JO C | Official Journal C series | | JO C E | Official Journal C electronic | | JO L | Official Journal L series | | LET | Old Commission documents (\"Letter\") sent to the Council without annexes or with an unnumbered document | | PE | Single number given to all European Parliament documents | | PRES | Council press release | | SEC | Miscellaneous Commission documents | | TA | European Parliament texts (texts adopted) | Note: The legal activities (table \"activities of the insitutions\") can be used to filter the events based on the key actor for an event" ;
        rdfs:label       "Legal event" ;
        rdfs:subClassOf  :event ;
        rdfs:subClassOf  [ a                         owl:Restriction ;
                           owl:onClass               :dossier ;
                           owl:onProperty            :event_legal_part_of_dossier ;
                           owl:qualifiedCardinality  "1"^^xsd:nonNegativeInteger
                         ] ;
        rdfs:subClassOf  [ a                         owl:Restriction ;
                           owl:onClass               :concept_type_event_legal ;
                           owl:onProperty            :event_legal_has_type_concept_type_event_legal ;
                           owl:qualifiedCardinality  "1"^^xsd:nonNegativeInteger
                         ] ;
        rdfs:subClassOf  [ a                   owl:Restriction ;
                           owl:maxCardinality  "1"^^xsd:nonNegativeInteger ;
                           owl:onProperty      :event_legal_type
                         ] ;
        rdfs:subClassOf  [ a                            owl:Restriction ;
                           owl:maxQualifiedCardinality  "1"^^xsd:nonNegativeInteger ;
                           owl:onClass                  :concept_type_decision ;
                           owl:onProperty               :event_legal_uses_concept_type_decision
                         ] ;
        rdfs:subClassOf  [ a                   owl:Restriction ;
                           owl:maxCardinality  "1"^^xsd:nonNegativeInteger ;
                           owl:onProperty      :event_legal_comment
                         ] ;
        rdfs:subClassOf  [ a                   owl:Restriction ;
                           owl:maxCardinality  "1"^^xsd:nonNegativeInteger ;
                           owl:onProperty      :event_legal_session_council
                         ] ;
        rdfs:subClassOf  [ a                            owl:Restriction ;
                           owl:maxQualifiedCardinality  "1"^^xsd:nonNegativeInteger ;
                           owl:onClass                  :concept_type_procedure_code_interinstitutional ;
                           owl:onProperty               :event_legal_was_historically_about_concept_type_procedure_code_interinstitutional
                         ] ;
        rdfs:subClassOf  [ a                   owl:Restriction ;
                           owl:maxCardinality  "1"^^xsd:nonNegativeInteger ;
                           owl:onProperty      :event_legal_initiating
                         ] ;
        rdfs:subClassOf  [ a                            owl:Restriction ;
                           owl:maxQualifiedCardinality  "1"^^xsd:nonNegativeInteger ;
                           owl:onClass                  :concept_agenda_council ;
                           owl:onProperty               :event_legal_on_agenda_concept_agenda_council
                         ] ;
        rdfs:subClassOf  [ a                owl:Restriction ;
                           owl:cardinality  "1"^^xsd:nonNegativeInteger ;
                           owl:onProperty   :event_legal_date
                         ] ;
        rdfs:subClassOf  [ a                            owl:Restriction ;
                           owl:maxQualifiedCardinality  "1"^^xsd:nonNegativeInteger ;
                           owl:onClass                  :concept_mode_decision ;
                           owl:onProperty               :event_legal_uses_concept_mode_decision
                         ] .

:partially_refers_to  a  owl:ObjectProperty ;
        rdfs:label  "Partially refers to" .

:person_takes_over_event_legal
        a                   owl:ObjectProperty ;
        rdfs:domain         :person ;
        rdfs:label          "Person takes over legal event" ;
        rdfs:range          :event_legal ;
        rdfs:subPropertyOf  :takes_over .

:catalogued_by  a   owl:ObjectProperty ;
        rdfs:label  "Catalogued by" .

:complex_work  a         owl:Class ;
        rdfs:comment     "This class comprises works that have more than one work as members (FRBRoo)" ;
        rdfs:label       "Complex Work" ;
        rdfs:subClassOf  :work .

:manifestation_publisher
        a                   owl:DatatypeProperty ;
        rdfs:comment        "DEPRECATED, Publisher of this manifestation. mapped from MARC21 field 260 $b" ;
        rdfs:domain         :manifestation ;
        rdfs:label          "Publisher" ;
        rdfs:range          xsd:string ;
        rdfs:subPropertyOf  :publisher ;
        owl:deprecated      true .

:concept_field_activity
        a                    owl:Class ;
        rdfs:comment         "Now coded with table 604 Pegase extract: <DOMAINE id=\"1140\">Politique industrielle et marché intérieur</DOMAINE> ATTO translation tables: <LIBELLE CODE=\"1140\">Politique industrielle et marché intérieur</LIBELLE><LIBELLE CODE=\"1140\">Industriepolitik und Binnenmarkt</LIBELLE>" ;
        rdfs:label           "Concept representing the field of activity" ;
        rdfs:subClassOf      skos:Concept , :concept_decoding ;
        owl:equivalentClass  [ a               owl:Restriction ;
                               owl:hasValue    <http://publications.europa.eu/resource/authority/fd_604> ;
                               owl:onProperty  skos:inScheme
                             ] .

:agent_relates_to_event
        a                   owl:ObjectProperty ;
        rdfs:domain         :agent ;
        rdfs:label          "Agent related to event" ;
        rdfs:range          :event ;
        rdfs:subPropertyOf  :relates_to ;
        owl:inverseOf       :event_related_with_agent .

:act_legislative_other_oj_l
        a                owl:Class ;
        rdfs:label       "OJ L other legislative act" ;
        rdfs:subClassOf  :legislation_secondary .

:special-official-journal_volume
        a                   owl:DatatypeProperty ;
        rdfs:comment        "Volume of the Special Edition. Consciously not a positiveInteger due to a special case, DD_1981_01_004S_SOM" ;
        rdfs:domain         :special-official-journal ;
        rdfs:label          "Volume of Special Edition of the Official Journal" ;
        rdfs:range          xsd:string ;
        rdfs:subPropertyOf  :volume .

:resource_legal_basis_for_procedure_code_interinstitutional
        a                   owl:ObjectProperty ;
        rdfs:comment        "The legal resource serves as basis for a procedure (typically, but not necessarily a treaty article). Relevant for legal analysis: true" ;
        rdfs:domain         :resource_legal ;
        rdfs:label          "Legal resource is basis for a procedure with interinstitutional code" ;
        rdfs:range          :procedure_code_interinstitutional ;
        rdfs:subPropertyOf  :basis_for .

:objection_period_extension
        a           owl:DatatypeProperty ;
        rdfs:label  "Objection period extension" .

:number_catalogue_other
        a           owl:DatatypeProperty ;
        rdfs:label  "Number catalogue other" .

:work_embargo  a            owl:DatatypeProperty ;
        rdfs:comment        "Is this work under embargo? This instance must not be shown until the indicated datetime has been reached. In case a release date is not known,9999-12-31 should be used (= absolute embargo)" ;
        rdfs:domain         :work ;
        rdfs:label          "Work embargo" ;
        rdfs:range          xsd:dateTime ;
        rdfs:subPropertyOf  :embargo .

:decision_internal_identifier
        a           owl:DatatypeProperty ;
        rdfs:label  "Decision internal identifier" .

:id_reception  a    owl:DatatypeProperty ;
        rdfs:label  "Id reception" .

:work_contains_section_legal
        a                   owl:ObjectProperty ;
        rdfs:domain         :work ;
        rdfs:label          "Work contains section (legal)" ;
        rdfs:range          :section_legal ;
        rdfs:subPropertyOf  :work_contains_subdivision , :contains .

:layer_act_consolidated
        a           owl:DatatypeProperty ;
        rdfs:label  "Layer act consolidated" .

:dossier_initiated_by_act_preparatory
        a                   owl:ObjectProperty ;
        rdfs:comment        "Relevant for legal analysis: true. This dossier is initiated by a preparatory act, typically a COM. Link to the work that created this dossier (to be embedded). Relevant for legal analysis: true" ;
        rdfs:domain         :dossier ;
        rdfs:label          "Dossier initiated by preparatory act" ;
        rdfs:range          :act_preparatory ;
        rdfs:subPropertyOf  :initiated_by .

:affaire_type  a      owl:DatatypeProperty ;
        rdfs:comment  "Type part of the Court case identification" ;
        rdfs:label    "Type of case" .

:communication_request_opinion
        a                owl:Class ;
        rdfs:comment     "Communication on a request for an opinion in sector 6" ;
        rdfs:label       "Communication on a request for an opinion" ;
        rdfs:subClassOf  :communication_cjeu .

:act_other_ep_term_parliamentary
        a                   owl:DatatypeProperty ;
        rdfs:comment        "This indicates the Parliamentary term during which an EP document was voted or EP question was raised. Relevant for legal analysis: true. Currently coded with FD_Table 285. However, only codes are exposed (not decoded), so 01, 02 etc" ;
        rdfs:domain         :act_other_ep ;
        rdfs:label          "Parliamentary term" ;
        rdfs:range          xsd:string ;
        rdfs:subPropertyOf  :term_parliamentary , :act_preparatory_term_parliamentary .

:transliterated_postal_code
        a           owl:DatatypeProperty ;
        rdfs:label  "Transliterated postal code" .

:country_is_about_work_dataset
        a              owl:ObjectProperty ;
        rdfs:domain    :country ;
        rdfs:label     "Country is about work dataset" ;
        rdfs:range     :work_dataset ;
        owl:inverseOf  :work_dataset_spatial_country .

:ruling_cjeu  a          owl:Class ;
        rdfs:comment     "Ruling of the Court of Justice in sector 6 (6CX)" ;
        rdfs:label       "Court ruling" ;
        rdfs:subClassOf  :case-law .

:case-law_requests_for_failure_to_fulfill_an_obligation_for_resource_legal
        a                   owl:ObjectProperty ;
        rdfs:comment        "This property points to legal act quoted in the operative part of Court decisions" ;
        rdfs:domain         :case-law ;
        rdfs:label          "Case law requests to establish failure to fulfill an obligation" ;
        rdfs:range          :resource_legal ;
        rdfs:subPropertyOf  :requests_for_failure_to_fulfill_an_obligation_for ;
        owl:inverseOf       :resource_legal_establishes_failure_to_fulfill_obligation_requested_by_case-law .

:projection  a      owl:DatatypeProperty ;
        rdfs:label  "Projection" .

[ a            owl:AllDisjointClasses ;
  owl:members  ( :event :dossier )
] .

:procurement_public_url_general
        a                   owl:DatatypeProperty ;
        rdfs:domain         :procurement_public ;
        rdfs:label          "General URL" ;
        rdfs:range          xsd:anyURI ;
        rdfs:subPropertyOf  :url_general .

:summary_legislation_eu
        a                owl:Class ;
        rdfs:comment     "Summary of EU legislation as pusblished on http://europa.eu/legislation_summaries/index_en.htm, treated as a separate bibliographic item (= LEGIS_SUM). Usage: &#xA;| summary relationship of class summary | Summarizes basic act: 3xxxxYzzzz | &#xA;| \"summary summarizes modifying act\" relationship of class summary of EU legislaiton | Summarizes modifying act: 3xxxyYzzzz | &#xA;| \"summary summarizes consolidated act\" | Summarizes consolidated act: 0xxxxYzzzz | &#xA;| Links to other documents (e.g. a related COM) | work_related_to_work | The summaries of legislation have a unique identifier in the sumleg scheme (cf. https://webgate.ec.europa.eu/publications/jira/browse/CELLAR-420) Note: Descriptor_ipg and classification_ipg, that currently exist, will not be converted Date of document represents always the date of the latest version." ;
        rdfs:label       "Summary of EU legislation" ;
        rdfs:subClassOf  :summary ;
        rdfs:subClassOf  [ a                   owl:Restriction ;
                           owl:maxCardinality  "1"^^xsd:nonNegativeInteger ;
                           owl:onProperty      :summary_legislation_eu_version
                         ] ;
        rdfs:subClassOf  [ a                   owl:Restriction ;
                           owl:maxCardinality  "1"^^xsd:nonNegativeInteger ;
                           owl:onProperty      :summary_legislation_eu_obsolete
                         ] ;
        rdfs:subClassOf  [ a                   owl:Restriction ;
                           owl:minCardinality  "1"^^xsd:nonNegativeInteger ;
                           owl:onProperty      :summary_legislation_eu_id_legissum
                         ] .

:act_consolidated_date
        a                   owl:DatatypeProperty ;
        rdfs:comment        "Consleg date" ;
        rdfs:domain         :act_consolidated ;
        rdfs:label          "Consolidated act date" ;
        rdfs:range          xsd:date ;
        rdfs:subPropertyOf  :date .

:concept_directory-code_subject_of_manifestation_special-official-journal-act
        a                   owl:ObjectProperty ;
        rdfs:domain         :concept_directory-code ;
        rdfs:label          "Concept directory code subject of manifestation special official journal act" ;
        rdfs:range          :manifestation_special-official-journal-act ;
        rdfs:subPropertyOf  :subject_of ;
        owl:inverseOf       :manifestation_special-official-journal-act_is_about_concept_directory-code .

:title_short  a     owl:DatatypeProperty ;
        rdfs:label  "Title short" .

:ATTO_FD_500  a              owl:Class ;
        rdfs:label           "FD_500 ATTO table" ;
        rdfs:subClassOf      skos:Concept ;
        owl:equivalentClass  [ a               owl:Restriction ;
                               owl:hasValue    <http://publications.europa.eu/resource/authority/fd_500> ;
                               owl:onProperty  skos:inScheme
                             ] .

:resource_legal_partially_annulled_by_case-law
        a                   owl:ObjectProperty ;
        rdfs:comment        "34 cases (2012-07-31). Example: 62009TN0293: \"Partial annulment request 52009XC0521(05)\". Relevant for legal analysis: true." ;
        rdfs:domain         :resource_legal ;
        rdfs:label          "Legal resource partially annulled by case law" ;
        rdfs:range          :case-law ;
        rdfs:subPropertyOf  :partially_annulled_by ;
        owl:inverseOf       :case-law_partially_annuls_resource_legal .

:signatory_function2  a  owl:DatatypeProperty ;
        rdfs:label  "Signatory function2" .

:dossier_based_on_resource_legal
        a                   owl:ObjectProperty ;
        rdfs:comment        "Dossier is based on a legal resource (typically a treaty article, but could also be secondary legislation)" ;
        rdfs:domain         :dossier ;
        rdfs:label          "Dossier based on legal resource" ;
        rdfs:range          :resource_legal ;
        rdfs:subPropertyOf  :based_on ;
        owl:inverseOf       :resource_legal_basis_for_dossier .

:dossier_title  a           owl:DatatypeProperty ;
        rdfs:comment        "Relevant for legal analysis: true. the title of the dossier. language encoded in triple as ^^ISO-Code, on Prelex typically title of initiating document, but can change e.g. in case of JAI dossiers. Datatype is rdf:PlainLiteral. Relevant for legal analysis: true" ;
        rdfs:domain         :dossier ;
        rdfs:label          "Dossier title" ;
        rdfs:range          rdf:PlainLiteral ;
        rdfs:subPropertyOf  :title .

:has_member  a      owl:ObjectProperty ;
        rdfs:label  "Has member" .

:used_originally_by  a      owl:ObjectProperty ;
        rdfs:label          "Used originally by" ;
        rdfs:subPropertyOf  :used_by .

:event_legal_responsibility_of_person
        a                   owl:ObjectProperty ;
        rdfs:comment        "DEPRECATED, This legal event is under responsibility of a given person. Person role: Responsible. Relevant for legal analysis: true." ;
        rdfs:domain         :event_legal ;
        rdfs:label          "Legal event under responsibility of person" ;
        rdfs:range          :person ;
        rdfs:subPropertyOf  :responsibility_of , :event_responsibility_of_person ;
        owl:deprecated      true ;
        owl:inverseOf       :person_responsible_for_event_legal .

:case-law_affects_resource_legal
        a                   owl:ObjectProperty ;
        rdfs:comment        "This property points to legal act quoted in the operative part of Court decisions" ;
        rdfs:domain         :case-law ;
        rdfs:label          "Case law affects legal resource" ;
        rdfs:range          :resource_legal ;
        rdfs:subPropertyOf  :affects ;
        owl:inverseOf       :resource_legal_affected_by_case-law .

:implementation_plan_needed
        a           owl:DatatypeProperty ;
        rdfs:label  "Implementation plan needed" .

:concept_case_event_result
        a                owl:Class ;
        rdfs:label       "Concept representing the result of a case event" ;
        rdfs:subClassOf  :concept_decoding .

:open_public_consultation_needed
        a           owl:DatatypeProperty ;
        rdfs:label  "Open public consultation needed" .

:manifestation_date_publication
        a                   owl:DatatypeProperty ;
        rdfs:comment        "The date of publication/distribution of the manifestation. This date can be a full date in ISO format, a year only or a year and a month." ;
        rdfs:domain         :manifestation ;
        rdfs:label          "Publication date of manifestation" ;
        rdfs:range          <http://publications.europa.eu/ontology/datatype#date> ;
        rdfs:subPropertyOf  :date_publication .

:article_journal_related
        a           owl:DatatypeProperty ;
        rdfs:label  "Article journal related" .

:authors-opinion  a  owl:ObjectProperty ;
        rdfs:label  "Authors opinion" .

:date_deadline  a           owl:DatatypeProperty ;
        rdfs:label          "Date deadline" ;
        rdfs:range          xsd:date ;
        rdfs:subPropertyOf  :date .

:notice_prior-information_authority-type_label
        a                   owl:DatatypeProperty ;
        rdfs:domain         :notice_prior-information ;
        rdfs:label          "Label of authority type" ;
        rdfs:range          xsd:string ;
        rdfs:subPropertyOf  :authority-type_label .

:act_preparatory_term_parliamentary
        a                   owl:DatatypeProperty ;
        rdfs:comment        "This indicates the Parliamentary term during which an EP document was voted or EP question was raised. Relevant for legal analysis: true. Currently coded with FD_Table 285. However, only codes are exposed (not decoded), so 01, 02 etc" ;
        rdfs:domain         :act_preparatory ;
        rdfs:label          "Parliamentary term" ;
        rdfs:range          xsd:string ;
        rdfs:subPropertyOf  :term_parliamentary .

:implicitly_repeals  a  owl:ObjectProperty ;
        rdfs:label  "Implicitly repeals" .

:case-law_delivered_by_court_national
        a                   owl:ObjectProperty ;
        rdfs:comment        "Reference to the national court who delivered the judgement" ;
        rdfs:domain         :case-law ;
        rdfs:label          "Case law delivered by national court" ;
        rdfs:range          :court_national ;
        rdfs:subPropertyOf  :delivered_by ;
        owl:inverseOf       :court_national_delivers_case-law .

:validity_extended_by
        a           owl:ObjectProperty ;
        rdfs:label  "Validity extended by" .

:interpreted_by_judgement
        a           owl:ObjectProperty ;
        rdfs:label  "Interpreted by judgement" .

<http://publications.europa.eu/resource/authority/fd_335>
        a       owl:NamedIndividual .

:committee  a            owl:Class ;
        rdfs:comment     "A group of representatives from EU countries assisting the Commission for implementing acts during the internal decision-making process" ;
        rdfs:label       "Committee" ;
        rdfs:subClassOf  :agent ;
        rdfs:subClassOf  [ a                owl:Restriction ;
                           owl:cardinality  "1"^^xsd:nonNegativeInteger ;
                           owl:onProperty   cmr:lastModificationDate
                         ] ;
        rdfs:subClassOf  [ a                   owl:Restriction ;
                           owl:maxCardinality  "1"^^xsd:nonNegativeInteger ;
                           owl:onProperty      cmr:creationDate
                         ] .

:product-form_is-product-form-of_manifestation
        a             owl:ObjectProperty ;
        rdfs:comment  "A Concept product form representing the product form of manifestation" ;
        rdfs:domain   :product-form ;
        rdfs:label    "Concept product form is product form of manifestation" ;
        rdfs:range    :manifestation ;
        dct:created   "2022-08-01T16:18:31.50"^^xsd:dateTime .

:affected_by  a       owl:ObjectProperty ;
        rdfs:comment  "Super property (as inverse of cdm#affects)" ;
        rdfs:label    "Affected by" .

:manifestation_issn  a      owl:DatatypeProperty ;
        rdfs:comment        "ISSN of this manifestation. In Formex e.g. <NO.ISSN>18318029</NO.ISSN>" ;
        rdfs:domain         :manifestation ;
        rdfs:label          "issn" ;
        rdfs:range          xsd:string ;
        rdfs:subPropertyOf  :issn .

:reference-data_asset_release_basis_for_reference-data_asset_prerelease
        a              owl:ObjectProperty ;
        rdfs:comment   "A given version of a reference data (release) is the basis of prerelease version of the same reference data asset" ;
        rdfs:label     "Reference data asset release is basis for reference data asset prerelease" ;
        owl:inverseOf  :reference-data_asset_prerelease_based_on_reference-data_asset_release .

:opinion_ep_reported_by_associated_agent
        a                   owl:ObjectProperty ;
        rdfs:comment        "Name of the person (EP member or member of CoR or EESC) who reports on the relevant act. This property will be deprecated and replaced with work_reported_by_person. Role CMT_OPIN_ASSOC. Relevant for legal analysis: true" ;
        rdfs:domain         :opinion_ep ;
        rdfs:label          "European Parliament opinion has associated rapporteur" ;
        rdfs:range          :agent ;
        rdfs:subPropertyOf  :reported_by_associated .

:question_parliamentary_question_time
        a                owl:Class ;
        rdfs:comment     "Parliamentary question at question time (= subsector H sector 9 in EUR-Lex, 20873 notices on 2010-07-27)" ;
        rdfs:label       "Question at question time" ;
        rdfs:subClassOf  :question_parliamentary_with-debate .

:text-adopted  a         owl:Class ;
        rdfs:comment     "Texts adopted by the European Parliament" ;
        rdfs:label       "Text adopted" ;
        rdfs:subClassOf  :resource_legal ;
        rdfs:subClassOf  [ a                owl:Restriction ;
                           owl:cardinality  "1"^^xsd:nonNegativeInteger ;
                           owl:onProperty   :text-adopted_term_parliamentary
                         ] .

:dossier_number_reference
        a                   owl:DatatypeProperty ;
        rdfs:comment        "Relevant for legal analysis: true. reference number of the dossier. Taken from Prelex, e.g. numero=\"471\" split=\"1\", should contain information on the split. Procedure reference number. Relevant for legal analysis: true" ;
        rdfs:domain         :dossier ;
        rdfs:label          "Dossier number of reference" ;
        rdfs:range          xsd:string ;
        rdfs:subPropertyOf  :number_reference .

:resource_legal_involves_agent
        a             owl:ObjectProperty ;
        rdfs:comment  "An agent (organization, ...) involves an act(often private). Relevant for legal analysis: true." ;
        rdfs:domain   :resource_legal ;
        rdfs:label    "Legal resource involves agent" ;
        rdfs:range    :agent .

:person_responsible_for_event_legal
        a                   owl:ObjectProperty ;
        rdfs:comment        "DEPRECATED," ;
        rdfs:domain         :person ;
        rdfs:label          "Person responsible for legal event" ;
        rdfs:range          :event_legal ;
        rdfs:subPropertyOf  :responsible_for ;
        owl:deprecated      true .

:event_legal_joint-responsibility_of_institution
        a                   owl:ObjectProperty ;
        rdfs:comment        "DEPRECATED, A given institution is jointly responsible for this legal event. Body role:Jointly responsible. Relevant for legal analysis: true." ;
        rdfs:domain         :event_legal ;
        rdfs:label          "Legal event under joint responsibility of an institution" ;
        rdfs:range          :institution ;
        rdfs:subPropertyOf  :joint-responsibility_of , :event_joint-responsibility_of_institution ;
        owl:deprecated      true ;
        owl:inverseOf       :institution_jointly-responsible_for_event_legal .

:info_decision_cjeu  a   owl:Class ;
        rdfs:label       "Information on a non-published decision of the Court of Justice" ;
        rdfs:subClassOf  :case-law .

:summary_legislation_eu_id_legissum
        a                   owl:DatatypeProperty ;
        rdfs:comment        "Identifier for the summary of EU legislation (id_legissum)" ;
        rdfs:domain         :summary_legislation_eu ;
        rdfs:label          "Identifier for the summary of EU legislation (sumleg)" ;
        rdfs:range          xsd:string ;
        rdfs:subPropertyOf  :id_legissum .

:procurement_public_issued_by_concept_place
        a                   owl:ObjectProperty ;
        rdfs:domain         :procurement_public ;
        rdfs:label          "Public procurement value issued by a given town / place" ;
        rdfs:range          :concept_place ;
        rdfs:subPropertyOf  :issued_by .

:manifestation-mobile-app_date-modified
        a                   owl:DatatypeProperty ;
        rdfs:comment        "This property contains the most recent date on which the mobile application dissemination status was changed or modified. Based on 008 positions 11-14." ;
        rdfs:domain         :manifestation-mobile-app ;
        rdfs:label          "Mobile application dissemination status modification date" ;
        rdfs:range          <http://publications.europa.eu/ontology/datatype#date> ;
        rdfs:subPropertyOf  :date_modified ;
        dct:created         "2022-08-01T16:18:31.50"^^xsd:dateTime .

:resource_legal_annulment_requested_by_case-law
        a                   owl:ObjectProperty ;
        rdfs:comment        "757 cases (2012-07-31). Example: 62011CN0429: \"Annulment request 62008TA0208\". Relevant for legal analysis: true." ;
        rdfs:domain         :resource_legal ;
        rdfs:label          "Annulment of legal resource requested by case law" ;
        rdfs:range          :case-law ;
        rdfs:subPropertyOf  :annulment_requested_by ;
        owl:inverseOf       :case-law_requests_annulment_of_resource_legal .

:number_session_planned
        a           owl:DatatypeProperty ;
        rdfs:label  "Number session planned" .

:institution_optionally-consulted_by_event_legal
        a                   owl:ObjectProperty ;
        rdfs:comment        "An institution is optionally consulted in the scope of a legal event" ;
        rdfs:domain         :institution ;
        rdfs:label          "Institution optionally consulted by legal event" ;
        rdfs:range          :event_legal ;
        rdfs:subPropertyOf  :optionally-consulted_by .

:concept_directory-code_subject_of_legislation_secondary
        a                   owl:ObjectProperty ;
        rdfs:comment        "DEPRECATED" ;
        rdfs:domain         :concept_directory-code ;
        rdfs:label          "Directory code concept is subject of secondary legislation" ;
        rdfs:range          :legislation_secondary ;
        rdfs:subPropertyOf  :subject_of ;
        owl:deprecated      true ;
        owl:inverseOf       :legislation_secondary_is_about_concept_directory-code .

:g_package_ec  a         owl:Class ;
        rdfs:comment     "Internal documents of the European Commission with a G type identifier, meanwhile declassified." ;
        rdfs:label       "G package EC" ;
        rdfs:subClassOf  :swd_package_ec ;
        rdfs:subClassOf  [ a               owl:Restriction ;
                           owl:hasValue    "G" ;
                           owl:onProperty  :archive_package_internal_number_prefix
                         ] ;
        dct:created      "2022-09-28T21:13:12Z"^^xsd:dateTime .

:interpretation_requested_by
        a           owl:ObjectProperty ;
        rdfs:label  "Interpretation requested by" .

:date_referral  a   owl:DatatypeProperty ;
        rdfs:label  "Date referral" .

:has_successor  a   owl:ObjectProperty ;
        rdfs:label  "Has successor" .

:proposal_regulation_implementing_ec
        a                owl:Class ;
        rdfs:comment     "Note: There is consciously no proposal for an delegated regulation (in Procat: 5PC with FM = PDIRDEL), an delegated directive (FM = PDIRIMP) and a delegated decision (FM = PDECIMP)" ;
        rdfs:label       "Commission proposal for an implementing regulation" ;
        rdfs:subClassOf  :proposal_act , :act_preparatory_ec .

:work   a                owl:Class ;
        rdfs:comment     "\"A distinct intellectual creation\" (Definition) \"an abstract notion of an artistic or intellectual creation\" (FRBR)"@en ;
        rdfs:label       "Work" ;
        rdfs:subClassOf  [ a                   owl:Restriction ;
                           owl:maxCardinality  "1"^^xsd:nonNegativeInteger ;
                           owl:onProperty      :work_date_creation_legacy
                         ] ;
        rdfs:subClassOf  [ a                   owl:Restriction ;
                           owl:maxCardinality  "1"^^xsd:nonNegativeInteger ;
                           owl:onProperty      :work_date_creation
                         ] ;
        rdfs:subClassOf  [ a                            owl:Restriction ;
                           owl:minQualifiedCardinality  "1"^^xsd:nonNegativeInteger ;
                           owl:onClass                  :expression ;
                           owl:onProperty               :work_has_expression
                         ] ;
        rdfs:subClassOf  [ a                   owl:Restriction ;
                           owl:maxCardinality  "1"^^xsd:nonNegativeInteger ;
                           owl:onProperty      :work_embargo
                         ] ;
        rdfs:subClassOf  [ a                owl:Restriction ;
                           owl:cardinality  "1"^^xsd:nonNegativeInteger ;
                           owl:onProperty   cmr:lastModificationDate
                         ] ;
        rdfs:subClassOf  [ a                   owl:Restriction ;
                           owl:maxCardinality  "1"^^xsd:nonNegativeInteger ;
                           owl:onProperty      :work_version
                         ] ;
        rdfs:subClassOf  [ a                   owl:Restriction ;
                           owl:maxCardinality  "1"^^xsd:nonNegativeInteger ;
                           owl:onProperty      :work_table-of-contents
                         ] ;
        rdfs:subClassOf  [ a                   owl:Restriction ;
                           owl:maxCardinality  "1"^^xsd:nonNegativeInteger ;
                           owl:onProperty      :work_archived
                         ] ;
        rdfs:subClassOf  [ a                   owl:Restriction ;
                           owl:maxCardinality  "1"^^xsd:nonNegativeInteger ;
                           owl:onProperty      :work_date_archived
                         ] ;
        rdfs:subClassOf  [ a                owl:Restriction ;
                           owl:cardinality  "1"^^xsd:nonNegativeInteger ;
                           owl:onProperty   :work_date_document
                         ] ;
        rdfs:subClassOf  [ a                   owl:Restriction ;
                           owl:maxCardinality  "1"^^xsd:nonNegativeInteger ;
                           owl:onProperty      cmr:creationDate
                         ] ;
        rdfs:subClassOf  [ a                            owl:Restriction ;
                           owl:minQualifiedCardinality  "1"^^xsd:nonNegativeInteger ;
                           owl:onClass                  :agent ;
                           owl:onProperty               :work_created_by_agent
                         ] ;
        rdfs:subClassOf  [ a                   owl:Restriction ;
                           owl:maxCardinality  "1"^^xsd:nonNegativeInteger ;
                           owl:onProperty      :work_datetime_transmission
                         ] ;
        rdfs:subClassOf  [ a                   owl:Restriction ;
                           owl:maxCardinality  "1"^^xsd:nonNegativeInteger ;
                           owl:onProperty      :work_complex_work_group_id
                         ] .

:date_notification  a       owl:DatatypeProperty ;
        rdfs:comment        "NF" ;
        rdfs:label          "Date notification" ;
        rdfs:range          xsd:date ;
        rdfs:subPropertyOf  :date .

:title_part  a              owl:DatatypeProperty ;
        rdfs:label          "Title part" ;
        rdfs:subPropertyOf  :title .

:guideline_ecb  a        owl:Class ;
        rdfs:comment     "Guideline of the European Central Bank (ECB) (subsector O of sector 3). At present 106 notices. Examples: 31998O0017, 31998O0010, 32009O0023" ;
        rdfs:label       "ECB guidelines" ;
        rdfs:subClassOf  :legislation_secondary .

:resource_legal_addresses_agent
        a                   owl:ObjectProperty ;
        rdfs:comment        "Name of an individual or other entity to which the act is addressed. Relevant for legal analysis: true" ;
        rdfs:domain         :resource_legal ;
        rdfs:label          "Legal resource addresses agent" ;
        rdfs:range          :agent ;
        rdfs:subPropertyOf  :addresses .

:resource_legal_basis_legal
        a            owl:DatatypeProperty ;
        rdfs:domain  :resource_legal ;
        rdfs:label   "Resource legal basis legal" ;
        rdfs:range   xsd:string .

:case-law_national_delivered_by_court_depending_on_agent
        a                   owl:ObjectProperty ;
        rdfs:comment        "The Agent is a country or supranational organisation on which the court delivering the judgment depends (e.g. EU Member States, Third Country, European Court of Human Rights, EFTA Court, International Court of Justice). Values are taken either from the table corporate body (for international courts) or country (otherwise). For JURE always from the country table." ;
        rdfs:domain         :case-law_national ;
        rdfs:label          "Case law delivered by court depending on" ;
        rdfs:range          :agent ;
        rdfs:subPropertyOf  :delivered_by_court_depending_on .

:case_court_identifier_extension
        a                   owl:DatatypeProperty ;
        rdfs:comment        "Code for the extension of the identifier in the case identifier, needed to make the identifier unique in some cases. possible values NONE, AVIS, PV, RX" ;
        rdfs:domain         :case_court ;
        rdfs:label          "Identifier of the extension in the case identifier" ;
        rdfs:range          xsd:string ;
        rdfs:subPropertyOf  :identifier_extension .

:drafted_in  a      owl:ObjectProperty ;
        rdfs:label  "Drafted in" .

<http://publications.europa.eu/resource/authority/fd_330>
        a       owl:NamedIndividual .

:manifestation_distribution_source
        a                   owl:DatatypeProperty ;
        rdfs:comment        "This property refers to a related resource from which the described resource is derived" ;
        rdfs:domain         :manifestation_distribution ;
        rdfs:label          "Distribution source" ;
        rdfs:range          xsd:string ;
        rdfs:subPropertyOf  :source .

:document_budget_ep  a   owl:Class ;
        rdfs:comment     "885 EP Budget documents, usually resolutions (5BP)" ;
        rdfs:label       "European Parliament budget document" ;
        rdfs:subClassOf  :act_preparatory_ep ;
        rdfs:subClassOf  [ a                owl:Restriction ;
                           owl:cardinality  "1"^^xsd:nonNegativeInteger ;
                           owl:onProperty   :document_budget_ep_term_parliamentary
                         ] .

:case_court_has_joined_conclusion_opinion_advocate-general
        a                   owl:ObjectProperty ;
        rdfs:comment        "The property to be used to issue a link between an opinion of the advocate general and a case or several cases from the Court (no matter if those are joined or not)" ;
        rdfs:domain         :case_court ;
        rdfs:label          "Case has joined conclusions" ;
        rdfs:range          :opinion_advocate-general ;
        rdfs:subPropertyOf  :has_joined_conclusion ;
        owl:inverseOf       :opinion_advocate-general_joined_to_case_court .

:defers_application_of
        a           owl:ObjectProperty ;
        rdfs:label  "Defers application of" .

:manifestation_date  a      owl:DatatypeProperty ;
        rdfs:comment        "Date of manifestation. CADMOS-2597" ;
        rdfs:domain         :manifestation ;
        rdfs:label          "Date of manifestation" ;
        rdfs:range          xsd:date ;
        rdfs:subPropertyOf  :date .

:proposal_decision_implementing_ec
        a                owl:Class ;
        rdfs:label       "Commission proposal for an implementing decision" ;
        rdfs:subClassOf  :proposal_act , :act_preparatory_ec .

:id_sector  a         owl:DatatypeProperty ;
        rdfs:comment  "DT_SEC" ;
        rdfs:label    "Id sector" .

:resource_legal_date_vote
        a                   owl:DatatypeProperty ;
        rdfs:comment        "Date of vote on decisions or resolutions of the European Parliament or on committees (EESC/CoR) opinions. Relevant for legal analysis: true" ;
        rdfs:domain         :resource_legal ;
        rdfs:label          "Date of vote" ;
        rdfs:range          xsd:date ;
        rdfs:subPropertyOf  :date_vote .

:expression_included_in_work
        a                   owl:ObjectProperty ;
        rdfs:comment        "Expression included in a given work" ;
        rdfs:domain         :expression ;
        rdfs:label          "Expression included in a work" ;
        rdfs:range          :work ;
        rdfs:subPropertyOf  :included_in ;
        owl:inverseOf       :work_includes_expression .

:resource_legal_incidentally_declared_void_by_case-law
        a                   owl:ObjectProperty ;
        rdfs:comment        "Calculated. Relevant for legal analysis: true." ;
        rdfs:domain         :resource_legal ;
        rdfs:label          "Legal resource incidentally declared void by case law" ;
        rdfs:range          :case-law ;
        rdfs:subPropertyOf  :incidentally_declared_void_by ;
        owl:inverseOf       :case-law_incidentally_declares_void_resource_legal .

:urgent_procedure  a  owl:DatatypeProperty ;
        rdfs:label  "Urgent procedure" .

:institution_responsible_for_event
        a             owl:ObjectProperty ;
        rdfs:comment  "An institution is responsible for the execution of an event" ;
        rdfs:domain   :institution ;
        rdfs:label    "Institution responsible for event" ;
        rdfs:range    :event .

:resource_legal_basis_for_procedure_without_code_interinstitutional
        a                   owl:ObjectProperty ;
        rdfs:comment        "The legal resource serves as basis for a procedure (typically, but not necessarily a treaty article). Relevant for legal analysis: true." ;
        rdfs:domain         :resource_legal ;
        rdfs:label          "Legal resource is basis for a procedure without interinstitutional code" ;
        rdfs:range          :procedure_without_code_interinstitutional ;
        rdfs:subPropertyOf  :basis_for .

:resource_legal_partially_refers_to_resource_legal
        a                   owl:ObjectProperty ;
        rdfs:comment        "Relevant for legal analysis: true" ;
        rdfs:domain         :resource_legal ;
        rdfs:label          "Legal resource partially refers to legal resource" ;
        rdfs:range          :resource_legal ;
        rdfs:subPropertyOf  :partially_refers_to ;
        owl:inverseOf       :resource_legal_partially_referred_to_resource_legal .

:manifestation_official-journal_part_formatting
        a                   owl:DatatypeProperty ;
        rdfs:comment        "Formatting for natural number and year. values such as YN (first year then natural number) and NY (first natural number then year)" ;
        rdfs:domain         :manifestation_official-journal_part ;
        rdfs:label          "Desired formatting for the year and number sequence" ;
        rdfs:range          xsd:string ;
        rdfs:subPropertyOf  :formatting .

:date_end-of-validity
        a                   owl:DatatypeProperty ;
        rdfs:label          "Date end of validity" ;
        rdfs:range          xsd:date ;
        rdfs:subPropertyOf  :date .

dct:created  a  owl:AnnotationProperty .

:communication_joint  a  owl:Class ;
        rdfs:comment     "where its resource_legal_type = (JC or DC), resource_legal_id_sector = 5, work_has_resource-type = JOINT_COMMUNIC" ;
        rdfs:label       "Joint communication" ;
        rdfs:subClassOf  :act_preparatory_joint .

:procurement_public_id_reception
        a                   owl:DatatypeProperty ;
        rdfs:comment        "Identifier of the reception" ;
        rdfs:domain         :procurement_public ;
        rdfs:label          "Reception identifier" ;
        rdfs:range          xsd:string ;
        rdfs:subPropertyOf  :id_reception .

:manifestation_extent_illustration
        a                   owl:DatatypeProperty ;
        rdfs:comment        "illustration extent of this manifestation. based on 300 $b. ultiple codes that refer to table PUB_PHYS" ;
        rdfs:domain         :manifestation ;
        rdfs:label          "Extent illustration" ;
        rdfs:range          xsd:string ;
        rdfs:subPropertyOf  :extent_illustration .

:resource_legal_rendered_obsolete_by_resource_legal
        a                   owl:ObjectProperty ;
        rdfs:comment        "Relevant for legal analysis: true." ;
        rdfs:domain         :resource_legal ;
        rdfs:label          "Legal resource rendered obsolete by legal resource" ;
        rdfs:range          :resource_legal ;
        rdfs:subPropertyOf  :rendered_obsolete_by ;
        owl:inverseOf       :resource_legal_renders_obsolete_resource_legal .

:person_jointly-responsible_for_event
        a                   owl:ObjectProperty ;
        rdfs:domain         :person ;
        rdfs:label          "Person jointly responsible for event" ;
        rdfs:range          :event ;
        rdfs:subPropertyOf  :jointly-responsible_for .

:reference_procedure  a  owl:DatatypeProperty ;
        rdfs:label  "Reference procedure" .

:resource_legal_addresses_country
        a             owl:ObjectProperty ;
        rdfs:comment  "Name of country to which the act is addressed. Relevant for legal analysis: true" ;
        rdfs:domain   :resource_legal ;
        rdfs:label    "resource legal addresses country" ;
        rdfs:range    :country .

:is_product_form_of  a  owl:ObjectProperty ;
        rdfs:label  "Is product form of" .

:target_audience_old_belongs_to_publication_general
        a           owl:ObjectProperty ;
        rdfs:label  "Target audience old belongs to publication general" .

:summary_case-law  a     owl:Class ;
        rdfs:comment     "Summary of case law, treated as a separate bibliographic item. Note: Title of the summary of case law: title furnished by the Court in Canvas, or if not available, type of document (e.g. \"Sommaire de l'Arrêt\" or \"Sommaire de l'Ordonnance\")" ;
        rdfs:label       "Summary of case law" ;
        rdfs:subClassOf  :summary ;
        rdfs:subClassOf  [ a                   owl:Restriction ;
                           owl:minCardinality  "1"^^xsd:nonNegativeInteger ;
                           owl:onProperty      :summary_case-law_id_celex
                         ] .

:concept_type_event_legal
        a                    owl:Class ;
        rdfs:comment         "Corresponds to the contents authority table event (http://publications.europa.eu/resource/authority/event)" ;
        rdfs:label           "Concept representing the type of an event" ;
        rdfs:subClassOf      :concept_type_event , :concept_decoding ;
        owl:equivalentClass  [ a               owl:Restriction ;
                               owl:hasValue    <http://publications.europa.eu/resource/authority/event> ;
                               owl:onProperty  skos:inScheme
                             ] .

:case-law_partially_annuls_resource_legal
        a                   owl:ObjectProperty ;
        rdfs:comment        "This property points to legal act quoted in the operative part of Court decisions" ;
        rdfs:domain         :case-law ;
        rdfs:label          "Case law partially annuls a legal resource" ;
        rdfs:range          :resource_legal ;
        rdfs:subPropertyOf  :partially_annuls ;
        owl:inverseOf       :resource_legal_partially_annulled_by_case-law .

:sequence  a        owl:DatatypeProperty ;
        rdfs:label  "Sequence" .

:case-law_national_affaire_number
        a                   owl:DatatypeProperty ;
        rdfs:comment        "DEPRECATED, Number of the affaire" ;
        rdfs:domain         :case-law_national ;
        rdfs:label          "National affaire: Number" ;
        rdfs:range          xsd:positiveInteger ;
        rdfs:subPropertyOf  :affaire_number ;
        owl:deprecated      true .

:case_court_reexamins_case-law
        a              owl:ObjectProperty ;
        rdfs:domain    :case_court ;
        rdfs:label     "Case court reexamins case law" ;
        rdfs:range     :case-law ;
        owl:inverseOf  :case-law_reexamined_by_case_court .

:event_internal_eu_survey_identifier
        a                   owl:DatatypeProperty ;
        rdfs:comment        "Indicates the eu_survey_identifier" ;
        rdfs:domain         :event_internal ;
        rdfs:label          "Eu survey identifier" ;
        rdfs:range          xsd:string ;
        rdfs:subPropertyOf  :eu_survey_identifier .

:resource_legal_immediately_enforced_by_case-law
        a                   owl:ObjectProperty ;
        rdfs:comment        "Calculated. Relevant for legal analysis: true." ;
        rdfs:domain         :resource_legal ;
        rdfs:label          "Legal resource immediately inforced by case law" ;
        rdfs:range          :case-law ;
        rdfs:subPropertyOf  :immediately_enforced_by ;
        owl:inverseOf       :case-law_immediately_enforces_resource_legal .

:table_of_contents_uses
        a                   owl:ObjectProperty ;
        rdfs:label          "Table of contents uses" ;
        rdfs:subPropertyOf  :uses .

:work_dataset_is_part_of_work_dataset
        a             owl:ObjectProperty ;
        rdfs:comment  "The dataset is part of another dataset." ;
        rdfs:domain   :work_dataset ;
        rdfs:label    "Dataset work is part of dataset work" ;
        rdfs:range    :work_dataset .

:work_associates_work
        a              owl:ObjectProperty ;
        rdfs:domain    :work ;
        rdfs:label     "Work associates work" ;
        rdfs:range     :work ;
        owl:inverseOf  :work_associated_to_work .

:event_internal_target_groups
        a                   owl:DatatypeProperty ;
        rdfs:comment        "Indicates the target groups of the internal event" ;
        rdfs:domain         :event_internal ;
        rdfs:label          "Target groups" ;
        rdfs:range          rdf:PlainLiteral ;
        rdfs:subPropertyOf  :target_groups .

:range_maximal  a   owl:DatatypeProperty ;
        rdfs:label  "Range maximal" .

:resource_legal_reestablished_by_resource_legal
        a                   owl:ObjectProperty ;
        rdfs:comment        "Calculated. Relevant for legal analysis: true." ;
        rdfs:domain         :resource_legal ;
        rdfs:label          "Legal resource reestablished by legal resource" ;
        rdfs:range          :resource_legal ;
        rdfs:subPropertyOf  :reestablished_by ;
        owl:inverseOf       :resource_legal_reestablishes_resource_legal .

:back   a                owl:Class ;
        rdfs:comment     "back matter contains any appendixes, etc. following the main part of a text (TEI, description of back element). Cf. http://www.tei-c.org/release/doc/tei-p5-doc/en/html/DS.html#DSBACK for documentation" ;
        rdfs:label       "Back matter" ;
        rdfs:subClassOf  :textstructure .

:part_legal  a           owl:Class ;
        rdfs:comment     "A part in a legal document" ;
        rdfs:label       "Part (legal)" ;
        rdfs:subClassOf  :subdivision .

:url_general  a     owl:DatatypeProperty ;
        rdfs:label  "Url general" .

:document_com_other_ec_id_com
        a                   owl:DatatypeProperty ;
        rdfs:comment        "COM catalogue number" ;
        rdfs:domain         :document_com_other_ec ;
        rdfs:label          "COM identifier" ;
        rdfs:range          xsd:string ;
        rdfs:subPropertyOf  :id_com .

:institution_responsible_for_event_legal
        a                   owl:ObjectProperty ;
        rdfs:comment        "An institution is responsible for the execution of a legal event" ;
        rdfs:domain         :institution ;
        rdfs:label          "Institution responsible for legal event" ;
        rdfs:range          :event_legal ;
        rdfs:subPropertyOf  :responsible_for .

:category  a        owl:DatatypeProperty ;
        rdfs:label  "Category" .

:incidentally_declares_void
        a           owl:ObjectProperty ;
        rdfs:label  "Incidentally declares void" .

:document_budget_ep_reported_by_person
        a                   owl:ObjectProperty ;
        rdfs:comment        "Name of the person (EP member or member of CoR or EESC) who reports on the relevant act. This property will be deprecated and replaced with work_reported_by_person. Role RAPP. Relevant for legal analysis: true" ;
        rdfs:domain         :document_budget_ep ;
        rdfs:label          "European Parliament budget document has rapporteur" ;
        rdfs:range          :person ;
        rdfs:subPropertyOf  :work_reported_by_person ;
        dct:created         "2018-07-16T13:17:46.888+02:00"^^xsd:dateTime ;
        owl:inverseOf       :person_reports_on_document_budget_ep .

:legislation_complementary
        a                owl:Class ;
        rdfs:comment     "Complementary legislation (= sector 4)" ;
        rdfs:label       "Complementary legislation" ;
        rdfs:subClassOf  :resource_legal .

:do_not_index  a      owl:DatatypeProperty ;
        rdfs:comment  "Do not index any object marked with this property, if the value is true. By default, treat the value as false" ;
        rdfs:label    "do not index" ;
        rdfs:range    xsd:boolean .

:agreement_international_efta
        a                owl:Class ;
        rdfs:comment     "European Free Trade Association (EFTA) international agreement (= subsector A of sector E in EUR-Lex). The EFTA international agreement is implicitly also a subclass of agreement_international and can use the relationships stored_by and has_type_comment (cf. below)" ;
        rdfs:label       "EFTA international agreement" ;
        rdfs:subClassOf  :document_efta .

:resource_legal_type  a     owl:DatatypeProperty ;
        rdfs:comment        "Indication of the legal type in celex identifier (DTT). Relevant for legal analysis: true" ;
        rdfs:domain         :resource_legal ;
        rdfs:label          "Type of legal resource" ;
        rdfs:range          xsd:string ;
        rdfs:subPropertyOf  :type .

:communication_case_new_requests_annulment_of_resource_legal
        a                   owl:ObjectProperty ;
        rdfs:comment        "This property points to legal act quoted in the communication on a new case published in OJ. Relevant for legal analysis: true" ;
        rdfs:domain         :communication_case_new ;
        rdfs:label          "Communication requests annulment of legal resource" ;
        rdfs:range          :resource_legal ;
        rdfs:subPropertyOf  :requests_annulment_of ;
        owl:inverseOf       :resource_legal_annulment_requested_by_communication_case_new .

:used_by_table_of_contents
        a                   owl:ObjectProperty ;
        rdfs:label          "Used by table of contents" ;
        rdfs:subPropertyOf  :used_by .

:initiative_eums  a      owl:Class ;
        rdfs:comment     "86 MS - initiatives (5IG)" ;
        rdfs:label       "Member States - initiatives" ;
        rdfs:subClassOf  :act_preparatory .

:manifestation_special-official-journal-act
        a                owl:Class ;
        rdfs:comment     "The manifestation of an act document from a Special Official Journal" ;
        rdfs:label       "Manifestation Special Official Journal act" ;
        rdfs:subClassOf  :manifestation ;
        rdfs:subClassOf  [ a                owl:Restriction ;
                           owl:cardinality  "1"^^xsd:nonNegativeInteger ;
                           owl:onProperty   :manifestation_special-official-journal-act_pages_total
                         ] ;
        rdfs:subClassOf  [ a                   owl:Restriction ;
                           owl:maxCardinality  "1"^^xsd:nonNegativeInteger ;
                           owl:onProperty      :manifestation_special-official-journal-act_legal_effect_paper
                         ] ;
        rdfs:subClassOf  [ a                   owl:Restriction ;
                           owl:minCardinality  "1"^^xsd:nonNegativeInteger ;
                           owl:onProperty      :manifestation_special-official-journal-act_is_about_concept_directory-code
                         ] ;
        rdfs:subClassOf  [ a                owl:Restriction ;
                           owl:cardinality  "1"^^xsd:nonNegativeInteger ;
                           owl:onProperty   :manifestation_special-official-journal-act_date_publication
                         ] .

:renders_obsolete  a  owl:ObjectProperty ;
        rdfs:label  "Renders obsolete" .

:work_catalogues_work
        a                   owl:ObjectProperty ;
        rdfs:comment        "The work catalogues by another work, e.g. by listing its titles" ;
        rdfs:domain         :work ;
        rdfs:label          "Work catalogues a work" ;
        rdfs:range          :work ;
        rdfs:subPropertyOf  :catalogues ;
        owl:inverseOf       :work_catalogued_by_work .

:internal_number_year
        a           owl:DatatypeProperty ;
        rdfs:label  "Internal number year" .

:number_catalogue  a  owl:DatatypeProperty ;
        rdfs:label  "Number catalogue" .

:ATTO_FD_607  a              owl:Class ;
        rdfs:label           "FD_607 ATTO table" ;
        rdfs:subClassOf      skos:Concept ;
        owl:equivalentClass  [ a               owl:Restriction ;
                               owl:hasValue    <http://publications.europa.eu/resource/authority/fd_607> ;
                               owl:onProperty  skos:inScheme
                             ] .

:official-journal-act_subsubsection_oj
        a                   owl:DatatypeProperty ;
        rdfs:comment        "Section heading (level 3) under which an Official Journal act is published." ;
        rdfs:domain         :official-journal-act ;
        rdfs:label          "Official Journal act subsubsection oj" ;
        rdfs:range          xsd:positiveInteger ;
        rdfs:subPropertyOf  :subsubsection_oj .

:expression_uses_language
        a                   owl:ObjectProperty ;
        rdfs:comment        "Relevant for legal analysis: true. The expression uses a given language (can be repeated to cover expressions in several languages). Implicit in the TIT_XX, Marc field 41 a. Relevant for legal analysis: true" ;
        rdfs:domain         :expression ;
        rdfs:label          "Expression uses language" ;
        rdfs:range          :language ;
        rdfs:subPropertyOf  :uses ;
        owl:inverseOf       :language_used_by_expression .

:place_publishes_manifestation
        a                   owl:ObjectProperty ;
        rdfs:domain         :place ;
        rdfs:label          "Place publishes manifestation" ;
        rdfs:range          :manifestation ;
        rdfs:subPropertyOf  :publishes .

<http://publications.europa.eu/resource/authority/treaty>
        a       owl:NamedIndividual .

:number_session  a  owl:DatatypeProperty ;
        rdfs:label  "Number session" .

:act_preparatory_eesc_priority_class
        a                   owl:DatatypeProperty ;
        rdfs:comment        "Priority class under which this document is treated at the EESC. Possible values A, B, B+, C, cf. Procedure of the Committee, rule 30, celex 32010Q1209(01)" ;
        rdfs:domain         :act_preparatory_eesc ;
        rdfs:label          "Priority class for this preparatory act" ;
        rdfs:range          xsd:string ;
        rdfs:subPropertyOf  :priority_class .

:case_court_identifier_number
        a                   owl:DatatypeProperty ;
        rdfs:comment        "Number in the case identifier. e.g. 172" ;
        rdfs:domain         :case_court ;
        rdfs:label          "Number in identifier of court case" ;
        rdfs:range          xsd:positiveInteger ;
        rdfs:subPropertyOf  :identifier_number .

:case-law_decision_review_requested_by_communication_case_new
        a              owl:ObjectProperty ;
        rdfs:domain    :case-law ;
        rdfs:label     "Case law decision review requested by communication case new" ;
        rdfs:range     :communication_case_new ;
        owl:inverseOf  :communication_case_new_requests_review_of_decision_case-law .

:case-law_national-judgement
        a                   owl:DatatypeProperty ;
        rdfs:comment        "Reference of previous and subsequent orders or decisions of national courts in the case of a preliminary ruling" ;
        rdfs:domain         :case-law ;
        rdfs:label          "National judgement" ;
        rdfs:range          rdf:XMLLiteral ;
        rdfs:subPropertyOf  :national-judgement .

:act_preparatory_ecb  a  owl:Class ;
        rdfs:comment     "Preparatory act by the European Central Bank" ;
        rdfs:label       "Preparatory act by ECB" ;
        rdfs:subClassOf  :act_preparatory ;
        rdfs:subClassOf  [ a               owl:Restriction ;
                           owl:hasValue    <http://publications.europa.eu/resource/authority/corporate-body/ECB> ;
                           owl:onProperty  :work_created_by_agent
                         ] ;
        dct:created      "2022-09-01T09:01:22"^^xsd:dateTime .

:resource_legal_relevant_for_unit_administrative
        a                   owl:ObjectProperty ;
        rdfs:comment        "Relevant especially for national legislation, for EU legislation implicitly EU" ;
        rdfs:domain         :resource_legal ;
        rdfs:label          "Legal resource is relevant for an administrative unit" ;
        rdfs:range          :unit_administrative ;
        rdfs:subPropertyOf  :relevant_for .

:act_other_cor_number_session
        a                   owl:DatatypeProperty ;
        rdfs:comment        "DEPRECATED. Number of session during which this act was debated or voted (EP.EESC,CoR, …). Relevant for legal analysis: true.\" Mixed content, decoded with fd_345. Use cdm:act_preparatory_number_session" ;
        rdfs:domain         :act_other_cor ;
        rdfs:label          "Number of session" ;
        rdfs:range          xsd:string ;
        rdfs:subPropertyOf  :number_session , :act_preparatory_number_session ;
        owl:deprecated      true .

:communicated_on_by  a  owl:ObjectProperty ;
        rdfs:label  "Communicated on by" .

:application_extended_by
        a           owl:ObjectProperty ;
        rdfs:label  "Application extended by" .

:opinion_consultation_eesc
        a                owl:Class ;
        rdfs:comment     "European Economic and Social Committee Opinion on consultation (5AE)" ;
        rdfs:label       "European Economic and Social Committee opinion on consultation" ;
        rdfs:subClassOf  :act_preparatory_eesc ;
        rdfs:subClassOf  [ a                   owl:Restriction ;
                           owl:maxCardinality  "1"^^xsd:nonNegativeInteger ;
                           owl:onProperty      :opinion_consultation_eesc_number_session
                         ] .

:item_embargo  a            owl:DatatypeProperty ;
        rdfs:comment        "Is this item under embargo? This instance must not be shown until the indicated datetime has been reached. In case a release date is not known,9999-12-31 should be used (= absolute embargo)" ;
        rdfs:domain         :item ;
        rdfs:label          "Item embargo" ;
        rdfs:range          xsd:dateTime ;
        rdfs:subPropertyOf  :embargo .

:manifestation_special-official-journal_part
        a                owl:Class ;
        rdfs:comment     "Information on the print manifestation of an act" ;
        rdfs:label       "Part of an manifestation of a Special Edition of the Official Journal" ;
        rdfs:subClassOf  :manifestation_print ;
        rdfs:subClassOf  [ a                   owl:Restriction ;
                           owl:maxCardinality  "1"^^xsd:nonNegativeInteger ;
                           owl:onProperty      :manifestation_special-official-journal_part_pages_total
                         ] ;
        rdfs:subClassOf  [ a                owl:Restriction ;
                           owl:cardinality  "1"^^xsd:nonNegativeInteger ;
                           owl:onProperty   :manifestation_special-official-journal_part_page_last
                         ] ;
        rdfs:subClassOf  [ a                owl:Restriction ;
                           owl:cardinality  "1"^^xsd:nonNegativeInteger ;
                           owl:onProperty   :manifestation_special-official-journal_part_page_first
                         ] .

:resource_legal_date_start_handling
        a                   owl:DatatypeProperty ;
        rdfs:comment        "Start of processing of this legal resource. It corresponds to corext:date_activation, at this stage only relevant for internal handling for EESC, but could also be considered for external handling. If needed, the distinction could be made via an annotation." ;
        rdfs:domain         :resource_legal ;
        rdfs:label          "Date at which work on this legal resource has actively started" ;
        rdfs:range          xsd:date ;
        rdfs:subPropertyOf  :date_start_handling .

:dossier_year_reference
        a                   owl:DatatypeProperty ;
        rdfs:comment        "Relevant for legal analysis: true. starting year of the dossier. Year part of the reference number. Procedure reference year. Relevant for legal analysis: true" ;
        rdfs:domain         :dossier ;
        rdfs:label          "Dossier year of reference" ;
        rdfs:range          xsd:string ;
        rdfs:subPropertyOf  :year_reference .

<http://publications.europa.eu/resource/authority/fd_612>
        a       owl:NamedIndividual .

:defended_by  a     owl:ObjectProperty ;
        rdfs:label  "Defended by" .

:embargo  a           owl:DatatypeProperty ;
        rdfs:comment  "Base class for embargo properties on every level of the FRBR hierarchy or dossiers/events/agents." ;
        rdfs:label    "Embargo" .

:barcode  a           owl:DatatypeProperty ;
        rdfs:comment  "The barcode on a document or transmission" ;
        rdfs:label    "Barcode" ;
        dct:created   "2022-09-29T07:25:14Z"^^xsd:dateTime .

:treaty_name  a       owl:DatatypeProperty ;
        rdfs:comment  "Common name of a treaty" ;
        rdfs:domain   :treaty ;
        rdfs:label    "Treaty name" ;
        rdfs:range    xsd:string ;
        dct:created   "2018-05-25T10:45:59.663+02:00"^^xsd:dateTime .

:draft_to_be_published
        a           owl:DatatypeProperty ;
        rdfs:label  "Draft to be published" .

:series_contains_publication_general
        a           owl:ObjectProperty ;
        rdfs:label  "Series contains publication general" .

<http://publications.europa.eu/resource/authority/dissemination-status>
        a       owl:NamedIndividual .

:taken_over  a      owl:ObjectProperty ;
        rdfs:label  "Taken over" .

:institution_informed_by_event_legal
        a                   owl:ObjectProperty ;
        rdfs:domain         :institution ;
        rdfs:label          "Institution informed by legal event" ;
        rdfs:range          :event_legal ;
        rdfs:subPropertyOf  :informed_by .

:act_legislative_other_oj_l_service_responsible
        a                   owl:DatatypeProperty ;
        rdfs:comment        "The Commission DG or DGs responsible for drafting of an act. Relevant for legal analysis: true. DEPRECATED. In the instance data, the property is planned to be replaced with cdm:resource_legal_service_responsible at beginning 2019. When this is done this property will be removed from CDM. The Commission's DG that brought forward the proposal; to be taken from a closed list of DGs (that might be derived from the RECORD project ?). For the backlog data need to be completed. Cardinality to be restricted to 1 in the future. Relevant for legal analysis: true" ;
        rdfs:domain         :act_legislative_other_oj_l ;
        rdfs:label          "Service responsible" ;
        rdfs:range          xsd:string ;
        rdfs:subPropertyOf  :service_responsible , :resource_legal_service_responsible ;
        owl:deprecated      true .

:type_consultation  a        owl:Class ;
        rdfs:comment         "Concept representing the type of the consultation (internal procedure European Commission)" ;
        rdfs:label           "Type of the consultation (COM)" ;
        rdfs:subClassOf      skos:Concept , :concept_decoding ;
        owl:equivalentClass  [ a               owl:Restriction ;
                               owl:hasValue    <http://publications.europa.eu/resource/authority/com_internal_consultation_type> ;
                               owl:onProperty  skos:inScheme
                             ] .

:ATTO_FD_602  a              owl:Class ;
        rdfs:label           "FD_602 ATTO table" ;
        rdfs:subClassOf      skos:Concept ;
        owl:equivalentClass  [ a               owl:Restriction ;
                               owl:hasValue    <http://publications.europa.eu/resource/authority/fd_602> ;
                               owl:onProperty  skos:inScheme
                             ] .

:recommendation_ecsc  a  owl:Class ;
        rdfs:comment     "Recommendation of the European Coal and Steel Community (ECSC) (subsector K of sector 3). At present 152 notices. Examples: 31959K0211, 31978K0617, 31996K2393R(01)" ;
        rdfs:label       "ECSC recommendation" ;
        rdfs:subClassOf  :legislation_secondary .

:concept  a              owl:Class ;
        rdfs:comment     "a cognitive unit of meaning (Wikipedia). Note: Being the \"subject\" (http://purl.org/dc/terms/subject) of a particular work is a specific role of a given concept Note: Concept is a subclass of skos:Concept (= http://www.w3.org/2004/02/skos/core#Concept) A concept will typically be encoded using a suitable vocabulary encoding scheme (controlled vocabulary, taxonomy, or thesaurus)" ;
        rdfs:label       "Concept" ;
        rdfs:subClassOf  skos:Concept .

:recommendation_ec  a    owl:Class ;
        rdfs:comment     "419 Commission recommendation for an act work_has_resource-type = (RECO_DEC, RECO, CORRIGENDUM) resource_legal_type= (DC OR SC OR PC OR XC)" ;
        rdfs:label       "Commission recommendation for an act" ;
        rdfs:subClassOf  :act_preparatory_ec .

:number  a          owl:DatatypeProperty ;
        rdfs:label  "Number" .

:resource-type  a            owl:Class ;
        rdfs:comment         "Corresponds to the resource type as codified by the resource type table" ;
        rdfs:label           "Concept representing the resource type of an act" ;
        rdfs:subClassOf      skos:Concept , :concept_decoding ;
        owl:equivalentClass  [ a               owl:Restriction ;
                               owl:hasValue    <http://publications.europa.eu/resource/authority/resource-type> ;
                               owl:onProperty  skos:inScheme
                             ] .

:frequency_expected  a  owl:DatatypeProperty ;
        rdfs:label  "Frequency expected" .

:act_other_council  a    owl:Class ;
        rdfs:comment     "Where its (resource_legal_type = XG, resource_legal_id_sector = 5, work_created_by_agent = CONSIL) OR (resource_legal_id_sector = C, work_created_by_agent = CONSIL)" ;
        rdfs:label       "Other act of the Council" ;
        rdfs:subClassOf  :act_preparatory_council .

:agreement_international_associated_to_resource_legal
        a                   owl:ObjectProperty ;
        rdfs:comment        "International agreement associated to a decision or regulation. Relevant for legal analysis: true" ;
        rdfs:domain         :agreement_international ;
        rdfs:label          "International agreement associated to a decision and regulation" ;
        rdfs:range          :resource_legal ;
        rdfs:subPropertyOf  :associated_to ;
        owl:inverseOf       :resource_legal_associates_agreement_international .

:event_internal_consultation_duration
        a                   owl:DatatypeProperty ;
        rdfs:comment        "Indicates the consultation duration of the internal event" ;
        rdfs:domain         :event_internal ;
        rdfs:label          "Consultation duration" ;
        rdfs:range          xsd:string ;
        rdfs:subPropertyOf  :consultation_duration ;
        dct:created         "2018-05-24T13:09:27.052+02:00"^^xsd:dateTime .

:yearbook_work  a        owl:Class ;
        rdfs:comment     "This class describes a serial_work composed of set of works, each works is a periodical actualization of the content of the preceding work." ;
        rdfs:label       "Yearbook Work" ;
        rdfs:subClassOf  :serial_work .

:work_contains_indent
        a                   owl:ObjectProperty ;
        rdfs:comment        "The indent of this work" ;
        rdfs:domain         :work ;
        rdfs:label          "Work contains indent" ;
        rdfs:range          :indent ;
        rdfs:subPropertyOf  :work_contains_subdivision , :contains .

:work_compiled_by_agent
        a                   owl:ObjectProperty ;
        rdfs:comment        "The work is compiled an agent" ;
        rdfs:domain         :work ;
        rdfs:label          "Work is compiled by agent" ;
        rdfs:range          :agent ;
        rdfs:subPropertyOf  :work_created_by_agent , :compiled_by ;
        dct:created         "2018-08-30T11:08:56.144+02:00"^^xsd:dateTime .

:ATTO_FD_013  a              owl:Class ;
        rdfs:label           "FD_013 ATTO table" ;
        rdfs:subClassOf      skos:Concept ;
        owl:equivalentClass  [ a               owl:Restriction ;
                               owl:hasValue    <http://publications.europa.eu/resource/authority/fd_013> ;
                               owl:onProperty  skos:inScheme
                             ] .

:endorsements  a    owl:DatatypeProperty ;
        rdfs:label  "Endorsements" .

:expert-group  a         owl:Class ;
        rdfs:comment     "A group of representatives from EU countries assisting the Commission for implementing acts during the internal decision-making process" ;
        rdfs:label       "Expert group" ;
        rdfs:subClassOf  :agent ;
        rdfs:subClassOf  [ a                owl:Restriction ;
                           owl:cardinality  "1"^^xsd:nonNegativeInteger ;
                           owl:onProperty   cmr:lastModificationDate
                         ] ;
        rdfs:subClassOf  [ a                   owl:Restriction ;
                           owl:maxCardinality  "1"^^xsd:nonNegativeInteger ;
                           owl:onProperty      cmr:creationDate
                         ] .

:concept_eurovoc_subject_of_work
        a                   owl:ObjectProperty ;
        rdfs:comment        "terminology inspired by Property cidoc p129F.is_about. For a completed notice at least one concept should be present, but unforunately that is not always the case" ;
        rdfs:domain         :concept_eurovoc ;
        rdfs:label          "Eurovoc concept is subject of a work" ;
        rdfs:range          :work ;
        rdfs:subPropertyOf  :subject_of ;
        owl:inverseOf       :work_is_about_concept_eurovoc .

:work_contains_appendix
        a                   owl:ObjectProperty ;
        rdfs:domain         :work ;
        rdfs:label          "Work contains appendix" ;
        rdfs:range          :appendix ;
        rdfs:subPropertyOf  :work_contains_subdivision , :contains .

:act_preparatory_joint
        a                owl:Class ;
        rdfs:label       "Joint preparatory act" ;
        rdfs:subClassOf  :act_preparatory ;
        dct:created      "2022-09-01T09:01:22"^^xsd:dateTime .

:manifestation_reproduced_as_manifestation
        a                   owl:ObjectProperty ;
        rdfs:comment        "manifestation that reproduces another manifestation embodying the same expression of a work. Reciprocal relationship: reproduction of (manifestation) (after RDA J.4.2.)" ;
        rdfs:domain         :manifestation ;
        rdfs:label          "Manifestation reproduced as manifestation" ;
        rdfs:range          :manifestation ;
        rdfs:subPropertyOf  :reproduced_as ;
        owl:inverseOf       :manifestation_reproduction_of_manifestation .

:resource_legal_signatory_name
        a                   owl:DatatypeProperty ;
        rdfs:comment        "Legal resource signatory name. Added in the context of IMMC2CDM-OJ. Relevant for legal analysis: true" ;
        rdfs:domain         :resource_legal ;
        rdfs:label          "Name of signatory of the legal resource" ;
        rdfs:range          xsd:string ;
        rdfs:subPropertyOf  :signatory_name .

:range_minimal  a   owl:DatatypeProperty ;
        rdfs:label  "Range minimal" .

:resource_legal_validation_requested_by_case-law
        a                   owl:ObjectProperty ;
        rdfs:comment        "4 cases (2012-07-31). Example: 62008CN0373: \"validation request 32004R0398\". Relevant for legal analysis: true." ;
        rdfs:domain         :resource_legal ;
        rdfs:label          "Validation of legal resource requested by case law" ;
        rdfs:range          :case-law ;
        rdfs:subPropertyOf  :validation_requested_by .

:manifestation_official-journal_part_typedoc_printer
        a                   owl:DatatypeProperty ;
        rdfs:comment        "Typedoc of the legal resource (as seen by the printer). Values such as \"DEC\", the values are stored as is. They will at a future stage likely be replaced by a value for the resource type table" ;
        rdfs:domain         :manifestation_official-journal_part ;
        rdfs:label          "Printer's typedoc of the act" ;
        rdfs:range          xsd:string ;
        rdfs:subPropertyOf  :typedoc_printer .

:nuts_original_link_title
        a           owl:DatatypeProperty ;
        rdfs:label  "Nuts original link title" .

:event_case_framework_procedural_sequential-number_type_procedure
        a                   owl:DatatypeProperty ;
        rdfs:comment        "The sequential number related to the type of procedure in the identifier of the procedural framework of the case event" ;
        rdfs:domain         :event_case ;
        rdfs:label          "Sequential number related to the type of procedure in the identifier of the procedural framework" ;
        rdfs:range          xsd:positiveInteger ;
        rdfs:subPropertyOf  :framework_procedural_sequential-number_type_procedure .

:question_parliamentary_with-debate_published
        a                   owl:DatatypeProperty ;
        rdfs:comment        "Has this debate ever been published in \"EP debates\"? Indicates if this debate has ever been published in \"EP Debates\"" ;
        rdfs:domain         :question_parliamentary_with-debate ;
        rdfs:label          "Debate published?" ;
        rdfs:range          xsd:boolean ;
        rdfs:subPropertyOf  :published .

:procedure_internal_has_type_procedure_internal
        a                   owl:ObjectProperty ;
        rdfs:comment        "This internal procedure is of a certain type. Table com_internal_procedure" ;
        rdfs:domain         :procedure_internal ;
        rdfs:label          "Internal procedure has a type" ;
        rdfs:range          :type_procedure_internal ;
        rdfs:subPropertyOf  :has ;
        owl:inverseOf       :type_procedure_internal_is_type_of_procedure_internal .

:report_ep  a            owl:Class ;
        rdfs:comment     "Report issued by a committee conformant to the Rules of Procedure of the European Parliament, Rule 47/1)" ;
        rdfs:label       "European Parliament report" ;
        rdfs:subClassOf  :act_preparatory_ep .

:event_reported_by_person
        a                   owl:ObjectProperty ;
        rdfs:comment        "This event is reported on by a given person" ;
        rdfs:domain         :event ;
        rdfs:label          "Event reported on by person" ;
        rdfs:range          :person ;
        rdfs:subPropertyOf  :reported_by ;
        owl:inverseOf       :person_reports_on_event .

:opinion_consultation_cor
        a                owl:Class ;
        rdfs:comment     "709 Committee of the Regions' opinions on consultation (5AR)" ;
        rdfs:label       "Committee of the Regions' opinion on consultation" ;
        rdfs:subClassOf  :act_preparatory_cor ;
        rdfs:subClassOf  [ a                   owl:Restriction ;
                           owl:maxCardinality  "1"^^xsd:nonNegativeInteger ;
                           owl:onProperty      :opinion_consultation_cor_number_session
                         ] .

:event_case_responsibility_of_institution
        a                   owl:ObjectProperty ;
        rdfs:comment        "A given institution is primarily responsible for this case event" ;
        rdfs:domain         :event_case ;
        rdfs:label          "Case event under responsibility of an institution" ;
        rdfs:range          :institution ;
        rdfs:subPropertyOf  :responsibility_of ;
        owl:inverseOf       :institution_responsible_for_event_case .

:co-reports  a      owl:ObjectProperty ;
        rdfs:label  "Co reports" .

:labels_forms_link_type
        a           owl:DatatypeProperty ;
        rdfs:label  "Labels forms link type" .

:document_com_other_ec
        a                owl:Class ;
        rdfs:comment     "The natural number of the COM can be encoded as id. The class document_com_other_ec should NOT include more specific COMs. In terms of the expert search the resulting query for document_com_other_ec being: where its resource_legal_type = (DC or JC), resource_legal_id_sector = 5, work_has_resource-type = (REPORT, COMMUNIC, OPIN, PAPER_GREEN, PAPER_WHITE, RECO, RECO_RECO, PAPER_REFLEC, PROGRAM, MEMORANDUM_UNDERST, MEMORANDUM)" ;
        rdfs:label       "Other Commission COM document" ;
        rdfs:subClassOf  :act_preparatory_ec ;
        rdfs:subClassOf  [ a                   owl:Restriction ;
                           owl:maxCardinality  "1"^^xsd:nonNegativeInteger ;
                           owl:onProperty      :document_com_other_ec_id_com
                         ] .

:ATTO_FD_050  a              owl:Class ;
        rdfs:label           "FD_050 ATTO table" ;
        rdfs:subClassOf      skos:Concept , :agent ;
        owl:equivalentClass  [ a               owl:Restriction ;
                               owl:hasValue    <http://publications.europa.eu/resource/authority/fd_050> ;
                               owl:onProperty  skos:inScheme
                             ] .

:internal_number_suffix
        a           owl:DatatypeProperty ;
        rdfs:label  "Internal number suffix" .

:special-official-journal_legal_effect_paper
        a                   owl:DatatypeProperty ;
        rdfs:comment        "Does the paper version of this OJ issue have legal effect? To be included after the adoption of a regulation on electronic publication of OJ" ;
        rdfs:domain         :special-official-journal ;
        rdfs:label          "Legal effect for paper version of the special edition of the Official Journal" ;
        rdfs:range          xsd:boolean ;
        rdfs:subPropertyOf  :legal_effect_paper .

<http://publications.europa.eu/resource/authority/fd_501>
        a       owl:NamedIndividual .

:date_request_caducity
        a                   owl:DatatypeProperty ;
        rdfs:label          "Date request caducity" ;
        rdfs:range          xsd:date ;
        rdfs:subPropertyOf  :date .

:concept_court_procedure
        a                owl:Class ;
        rdfs:comment     "Table des procédures juridictionelles" ;
        rdfs:label       "Concept representing a court procedure" ;
        rdfs:subClassOf  :concept_decoding .

:resource_legal_eli  a      owl:DatatypeProperty ;
        rdfs:comment        "ELI identifier of an act. Relevant for legal analysis: true" ;
        rdfs:domain         :resource_legal ;
        rdfs:label          "European legislation identifier (ELI)" ;
        rdfs:range          xsd:anyURI ;
        rdfs:subPropertyOf  :eli .

:evolutive_work_asset_content
        a            owl:DatatypeProperty ;
        rdfs:domain  :evolutive_work ;
        rdfs:label   "Evolutive work asset content" ;
        rdfs:range   xsd:anyURI .

<http://publications.europa.eu/resource/authority/product-form>
        a       owl:NamedIndividual .

:textstructure  a        owl:Class ;
        rdfs:comment     "Works that are part of other works Classes to support access to substructures of the text as freestanding works. The class hierarchie is modelled on TEI P5, chapter 4, in particular TEI 4.5 and TEI 4.7 Relationships between these works and their container work are modelled via the generic work_part_of_work relationship." ;
        rdfs:label       "Superclass for all text structures" ;
        rdfs:subClassOf  :work .

:expression_includes_manifestation
        a                   owl:ObjectProperty ;
        rdfs:comment        "Relevant for legal analysis: true. This property associates an instance of an expression with an instance of manifestation belonging to a distinct instance of the expression. Relevant for legal analysis: true" ;
        rdfs:domain         :expression ;
        rdfs:label          "Expression includes manifestation" ;
        rdfs:range          :manifestation ;
        rdfs:subPropertyOf  :includes ;
        owl:inverseOf       :manifestation_is_included_in_expression .

:manifestation_title  a     owl:DatatypeProperty ;
        rdfs:comment        "title of this manifestation. Optional title of this manifestation (if different from the expression title)" ;
        rdfs:domain         :manifestation ;
        rdfs:label          "Manifestation title" ;
        rdfs:range          rdfs:Literal ;
        rdfs:subPropertyOf  :title .

:ATTO_FD_406  a              owl:Class ;
        rdfs:label           "FD_406 ATTO table" ;
        rdfs:subClassOf      skos:Concept ;
        owl:equivalentClass  [ a               owl:Restriction ;
                               owl:hasValue    <http://publications.europa.eu/resource/authority/fd_406> ;
                               owl:onProperty  skos:inScheme
                             ] .

:resolution_other_ep  a  owl:Class ;
        rdfs:comment     "8512 EP other resolutions, usually own-initiative (5IP)" ;
        rdfs:label       "European Parliament other resolution" ;
        rdfs:subClassOf  :act_preparatory_ep ;
        rdfs:subClassOf  [ a                owl:Restriction ;
                           owl:cardinality  "1"^^xsd:nonNegativeInteger ;
                           owl:onProperty   :resolution_other_ep_term_parliamentary
                         ] .

:resource_legal_uses_originally_language
        a                   owl:ObjectProperty ;
        rdfs:comment        "It indicates authentic language version of an act or a European Court case. It indicates also the language of the international agreements, treaties and corrigenda. This property used to point to both fd_060 and language tables. Our instance data is now fully pointing to the language table. Authentic language version of an act or a European Court case. Relevant for legal analysis: true" ;
        rdfs:domain         :resource_legal ;
        rdfs:label          "Legal resource uses originally language" ;
        rdfs:range          :language ;
        rdfs:subPropertyOf  :uses_originally ;
        dct:created         "2018-07-24T10:12:05.168+02:00"^^xsd:dateTime ;
        owl:inverseOf       :language_used_originally_by_resource_legal .

:resource_legal_based_on_resource_legal
        a                   owl:ObjectProperty ;
        rdfs:comment        "Link to the legal act(s) constituting the legal basis of the document. Additional information (LB_DNPLUS, LB_DN_COMMENT) to be stored as annotation properties. Relevant for legal analysis: true" ;
        rdfs:domain         :resource_legal ;
        rdfs:label          "Legal resource is based on legal resource" ;
        rdfs:range          :resource_legal ;
        rdfs:subPropertyOf  :based_on ;
        owl:inverseOf       :resource_legal_basis_for_resource_legal .

:resource_legal_responsibility_of_agent
        a                   owl:ObjectProperty ;
        rdfs:domain         :resource_legal ;
        rdfs:label          "Legal resource under responsibility of an agent" ;
        rdfs:range          :agent ;
        rdfs:subPropertyOf  :responsibility_of ;
        owl:inverseOf       :agent_responsible_for_resource_legal .

:opinion_eca  a          owl:Class ;
        rdfs:comment     "145 Court of Auditors opinions, usually on draft legislation and requested by another institution (5AA)" ;
        rdfs:label       "Court of Auditors opinion" ;
        rdfs:subClassOf  :act_preparatory_eca .

:fragment_resource_legal_part_of_resource_legal
        a                   owl:ObjectProperty ;
        rdfs:domain         :fragment_resource_legal ;
        rdfs:label          "Legal fragment is part of a legal resource" ;
        rdfs:range          :resource_legal ;
        rdfs:subPropertyOf  :part_of ;
        owl:inverseOf       :resource_legal_contains_fragment_resource_legal .

:resource_legal_does_replacement_of_resource_legal
        a                   owl:ObjectProperty ;
        rdfs:comment        "Legal resources does replacement a legal resource, in term of consolidation" ;
        rdfs:domain         :resource_legal ;
        rdfs:label          "Legal resources does replacement of legal resource" ;
        rdfs:range          :resource_legal ;
        rdfs:subPropertyOf  :does_replacement_of .

:modifies  a        owl:ObjectProperty ;
        rdfs:label  "Modifies" .

:court_national_delivers_case-law
        a                   owl:ObjectProperty ;
        rdfs:domain         :court_national ;
        rdfs:label          "National Court delivers case law" ;
        rdfs:range          :case-law ;
        rdfs:subPropertyOf  :delivers ;
        owl:inverseOf       :case-law_delivered_by_court_national .

:part1  a           owl:DatatypeProperty ;
        rdfs:label  "Part1" .

:expression_case-law_identifier_case
        a                   owl:DatatypeProperty ;
        rdfs:comment        "Case identifier in the title of a case law document (language-specific)" ;
        rdfs:domain         :expression_case-law ;
        rdfs:label          "Case identifier" ;
        rdfs:range          xsd:string ;
        rdfs:subPropertyOf  :identifier_case .

:resource_legal_defers_application_of_resource_legal
        a                   owl:ObjectProperty ;
        rdfs:comment        "Relevant for legal analysis: true." ;
        rdfs:domain         :resource_legal ;
        rdfs:label          "Legal resource defers application of legal resource" ;
        rdfs:range          :resource_legal ;
        rdfs:subPropertyOf  :defers_application_of ;
        owl:inverseOf       :resource_legal_application_deferred_by_resource_legal .

:serial_work  a          owl:Class ;
        rdfs:comment     "This class comprises works that are, or have been, planned to result in sequences of manifestations with common features. (Definition FRBRoo)" ;
        rdfs:label       "Serial Work" ;
        rdfs:subClassOf  :complex_work .

:article_publishing  a   owl:Class ;
        rdfs:comment     "A piece of nonfictional prose that is an independent part of a publication (wikipedia). The naming is inspired by Wikipedia's terminology (https://en.wikipedia.org/wiki/Article_%28publishing%29)" ;
        rdfs:label       "Article in publishing" ;
        rdfs:subClassOf  :publication_general .

:work_dataset_has_status-dataset
        a             owl:ObjectProperty ;
        rdfs:comment  "The concept representing a dataset status on work level" ;
        rdfs:domain   :work_dataset ;
        rdfs:label    "Dataset work has dataset status" ;
        rdfs:range    :dataset-status .

:procurement_public_regulation_label
        a                   owl:DatatypeProperty ;
        rdfs:domain         :procurement_public ;
        rdfs:label          "Regulation label of the contract" ;
        rdfs:range          xsd:string ;
        rdfs:subPropertyOf  :regulation_label .

:work_part_of_event  a  owl:ObjectProperty ;
        rdfs:comment   "Work documents (the outcome of) an event" ;
        rdfs:domain    :work ;
        rdfs:label     "Work is part of event" ;
        rdfs:range     :event ;
        owl:inverseOf  :event_contains_work .

:affaire_number  a    owl:DatatypeProperty ;
        rdfs:comment  "Number part of the Court case identification" ;
        rdfs:label    "Number of case" .

:resource_legal_confirmed_by_resource_legal
        a                   owl:ObjectProperty ;
        rdfs:comment        "Calculated. Relevant for legal analysis: true." ;
        rdfs:domain         :resource_legal ;
        rdfs:label          "Legal resource confirmed by legal resource" ;
        rdfs:range          :resource_legal ;
        rdfs:subPropertyOf  :confirmed_by ;
        owl:inverseOf       :resource_legal_confirms_resource_legal .

:id_local  a        owl:DatatypeProperty ;
        rdfs:label  "Id local" .

:manifestation_has_dimension
        a           owl:ObjectProperty ;
        rdfs:label  "Manifestation has dimension" .

:formally-addressed_by
        a           owl:ObjectProperty ;
        rdfs:label  "Formally addressed by" .

:datetime_transmission
        a           owl:DatatypeProperty ;
        rdfs:label  "Datetime transmission" .

:isbn   a           owl:DatatypeProperty ;
        rdfs:label  "Isbn" .

:adopts  a          owl:ObjectProperty ;
        rdfs:label  "Adopts" .

:event_internal_planned_objection_period_date_end
        a            owl:DatatypeProperty ;
        rdfs:domain  :event_internal ;
        rdfs:label   "Event internal planned objection period date end" ;
        rdfs:range   xsd:date ;
        dct:created  "2018-07-16T13:02:45.218+02:00"^^xsd:dateTime .

:related_with  a    owl:ObjectProperty ;
        rdfs:label  "Related with" .

:planned_consultation_period_date_end
        a           owl:DatatypeProperty ;
        rdfs:label  "Planned consultation period date end" .

:work_title  a              owl:DatatypeProperty ;
        rdfs:comment        "A title for the work itself (domain specific). Multiple usage to gather all language versions if necessary. Relevant for legal analysis: true." ;
        rdfs:domain         :work ;
        rdfs:label          "Work title" ;
        rdfs:range          rdfs:Literal ;
        rdfs:subPropertyOf  :title .

:in-force  a          owl:DatatypeProperty ;
        rdfs:comment  "Indicator whether a piece of legislation is currently in force or not in force. It is calculated based on the date_entry-into-force and date_end-of-validity. This can be used for the sector 1,2,3,4. It should not be used for legislative proposals or drafts. For these an extra property is going to be added in a next version of the CDM. Relevant for legal analysis: true. More information can be found in EUR-Lex legal analysis methodology." ;
        rdfs:label    "In force" .

:resource_legal_cor_opinion_contained_in_resource_legal
        a                   owl:ObjectProperty ;
        rdfs:comment        "451 cases (2010-07-27). Relevant for legal analysis: true." ;
        rdfs:domain         :resource_legal ;
        rdfs:label          "Committee of the Regions opinion on legal resource contained in legal resource" ;
        rdfs:range          :resource_legal ;
        rdfs:subPropertyOf  :cor_opinion_contained_in ;
        owl:inverseOf       :resource_legal_contains_cor_opinion_on_resource_legal .

:opinion_consultation_eesc_reported_by_person
        a                   owl:ObjectProperty ;
        rdfs:comment        "Name of the person (EP member or member of CoR or EESC) who reports on the relevant act. This property will be deprecated and replaced with work_reported_by_person. Role RAPP. Relevant for legal analysis: true" ;
        rdfs:domain         :opinion_consultation_eesc ;
        rdfs:label          "European Economic and Social Committee opinion on consultation has rapporteur" ;
        rdfs:range          :person ;
        rdfs:subPropertyOf  :work_reported_by_person ;
        dct:created         "2018-07-16T13:18:52.228+02:00"^^xsd:dateTime ;
        owl:inverseOf       :person_reports_on_opinion_consultation_eesc .

:declares_valid  a  owl:ObjectProperty ;
        rdfs:label  "Declares valid" .

:manifestation_official-journal_part_pages_total
        a                   owl:DatatypeProperty ;
        rdfs:comment        "DEPRECATED, Total number of pages of the OJ part related to a legal resource. Use manifestion_print_pages_total" ;
        rdfs:domain         :manifestation_official-journal_part ;
        rdfs:label          "Total pages" ;
        rdfs:range          xsd:string ;
        rdfs:subPropertyOf  :pages_total , :manifestation_print_pages_total ;
        owl:deprecated      true .

:influenced_by  a   owl:ObjectProperty ;
        rdfs:label  "Influenced by" .

:unit_administrative_contains_unit_administrative
        a                   owl:ObjectProperty ;
        rdfs:comment        "The administrative unit contains another administrative unit" ;
        rdfs:domain         :unit_administrative ;
        rdfs:label          "Administrative unit contains administrative unit" ;
        rdfs:range          :unit_administrative ;
        rdfs:subPropertyOf  :contains ;
        owl:inverseOf       :unit_administrative_part_of_unit_administrative .

:reference-data_asset_released_in_reference-data_asset_release
        a              owl:ObjectProperty ;
        rdfs:comment   "The representant of a reference data asset has a release version" ;
        rdfs:domain    :reference-data_asset ;
        rdfs:label     "Reference data asset released in reference data asset release" ;
        rdfs:range     :reference-data_asset_release ;
        owl:inverseOf  :reference-data_asset_release_releases_reference-data_asset .

:place  a                    owl:Class ;
        rdfs:label           "Place" ;
        rdfs:subClassOf      skos:Concept , :concept ;
        owl:equivalentClass  [ a               owl:Restriction ;
                               owl:hasValue    <http://publications.europa.eu/resource/authority/place> ;
                               owl:onProperty  skos:inScheme
                             ] .

:resource_legal_does_insertion_of_resource_legal
        a                   owl:ObjectProperty ;
        rdfs:comment        "Legal resources does insertion a legal resource, in term of consolidation" ;
        rdfs:domain         :resource_legal ;
        rdfs:label          "Legal resources does insertion of legal resource" ;
        rdfs:range          :resource_legal ;
        rdfs:subPropertyOf  :does_insertion_of .

<http://publications.europa.eu/resource/authority/fd_305>
        a       owl:NamedIndividual .

:manifestation_special-court-report_part_pages_total
        a                   owl:DatatypeProperty ;
        rdfs:comment        "DEPRECATED, Total number of pages of the special Court report part related to a court document. Use manifestion_print_pages_total" ;
        rdfs:domain         :manifestation_special-court-report_part ;
        rdfs:label          "Total pages" ;
        rdfs:range          xsd:string ;
        rdfs:subPropertyOf  :pages_total , :manifestation_print_pages_total ;
        owl:deprecated      true .

:fascicule  a       owl:DatatypeProperty ;
        rdfs:label  "Fascicule" .

:ATTO_FD_401  a              owl:Class ;
        rdfs:label           "FD_401 ATTO table" ;
        rdfs:subClassOf      skos:Concept ;
        owl:equivalentClass  [ a               owl:Restriction ;
                               owl:hasValue    <http://publications.europa.eu/resource/authority/fd_401> ;
                               owl:onProperty  skos:inScheme
                             ] .

:ATTO_FD_395  a              owl:Class ;
        rdfs:label           "FD_395 ATTO table" ;
        rdfs:subClassOf      skos:Concept ;
        owl:equivalentClass  [ a               owl:Restriction ;
                               owl:hasValue    <http://publications.europa.eu/resource/authority/fd_395> ;
                               owl:onProperty  skos:inScheme
                             ] .

:work_reference_internal
        a                   owl:DatatypeProperty ;
        rdfs:comment        "Possible subdivisions can be noted using the annotation properties sequence_number, prefix, /cortrans:cor_transmission_request/cmt:transmission/cmt:workflow/cm:work/cm:extension/corext:reference_internal" ;
        rdfs:domain         :work ;
        rdfs:label          "Internal reference" ;
        rdfs:range          xsd:string ;
        rdfs:subPropertyOf  :reference_internal .

:resource_legal_partially_adopted_by_resource_legal
        a                   owl:ObjectProperty ;
        rdfs:comment        "Calculated. Relevant for legal analysis: true." ;
        rdfs:domain         :resource_legal ;
        rdfs:label          "Legal resource is partially adopted by legal resource" ;
        rdfs:range          :resource_legal ;
        rdfs:subPropertyOf  :partially_adopted_by ;
        owl:inverseOf       :resource_legal_partially_adopts_resource_legal .

:completes  a       owl:ObjectProperty ;
        rdfs:label  "Completes" .

:manifestation-publication-general
        a                owl:Class ;
        rdfs:comment     "Manifestation is an (unspecific) general publication" ;
        rdfs:label       "Manifestation of a general publication" ;
        rdfs:subClassOf  :manifestation .

:work_contains_alinea
        a                   owl:ObjectProperty ;
        rdfs:comment        "The alinea of this work" ;
        rdfs:domain         :work ;
        rdfs:label          "Work contains alinea" ;
        rdfs:range          :alinea ;
        rdfs:subPropertyOf  :work_contains_subdivision , :contains .

:number_reference  a  owl:DatatypeProperty ;
        rdfs:label  "Number reference" .

:document_efta  a        owl:Class ;
        rdfs:comment     "European Free Trade Association (EFTA) document (= sector E in EUR-Lex)" ;
        rdfs:label       "EFTA document" ;
        rdfs:subClassOf  :resource_legal .

:has_result  a      owl:ObjectProperty ;
        rdfs:label  "Has result" .

:procurement_public_cpv_original_link_type
        a                   owl:DatatypeProperty ;
        rdfs:domain         :procurement_public ;
        rdfs:label          "CPV original type" ;
        rdfs:range          xsd:string ;
        rdfs:subPropertyOf  :cpv_original_link_type .

:listedProperty  a    owl:ObjectProperty ;
        rdfs:comment  "Object property identifying the property from which object values are listed" ;
        rdfs:domain   rdf:List ;
        rdfs:label    "Property with list as range" ;
        rdfs:range    rdf:Property .

:institution_mandatorily-addressed_by_event_legal
        a                   owl:ObjectProperty ;
        rdfs:comment        "An institution is mandatorily addressed in the scope of a legal event" ;
        rdfs:domain         :institution ;
        rdfs:label          "Institution mandatorily addressed by legal event" ;
        rdfs:range          :event_legal ;
        rdfs:subPropertyOf  :mandatorily-addressed_by .

:language_used_for_drafting_work
        a                   owl:ObjectProperty ;
        rdfs:domain         :language ;
        rdfs:label          "Language used for drafting a work" ;
        rdfs:range          :work ;
        rdfs:subPropertyOf  :used_for_drafting ;
        owl:inverseOf       :work_drafted_in_language .

:sec_package_ec  a       owl:Class ;
        rdfs:comment     "Internal documents of the European Commission with a SEC type identifier, meanwhile declassified." ;
        rdfs:label       "SEC package EC" ;
        rdfs:subClassOf  :swd_package_ec ;
        rdfs:subClassOf  [ a               owl:Restriction ;
                           owl:hasValue    "SEC" ;
                           owl:onProperty  :archive_package_internal_number_prefix
                         ] ;
        dct:created      "2022-09-28T21:13:02Z"^^xsd:dateTime .

:modified_by  a     owl:ObjectProperty ;
        rdfs:label  "Modified by" .

:case-law_delivered_by_advocate-general
        a                   owl:ObjectProperty ;
        rdfs:comment        "Name of the Advocate General who delivered the opinion on the case. Currently coded with FD_Table 100." ;
        rdfs:domain         :case-law ;
        rdfs:label          "Case law delivered by advocate general" ;
        rdfs:range          :advocate-general ;
        rdfs:subPropertyOf  :delivered_by ;
        owl:inverseOf       :advocate-general_delivers_case-law .

:case-law_communicated_on_by_communication_cjeu
        a              owl:ObjectProperty ;
        rdfs:comment   "A Court case is communicated by a Court communication in the Official Journal" ;
        rdfs:domain    :case-law ;
        rdfs:label     "Case law is communicated by a Court communication" ;
        rdfs:range     :communication_cjeu ;
        owl:inverseOf  :communication_cjeu_communicates_on_case-law .

:summary_legislation_eu_is_about_concept_directory-code
        a                   owl:ObjectProperty ;
        rdfs:comment        "Summary of EU legislation is about a concept expressed in the directory code" ;
        rdfs:domain         :summary_legislation_eu ;
        rdfs:label          "Summary of EU legislation is about directory code concept" ;
        rdfs:range          :concept_directory-code ;
        rdfs:subPropertyOf  :is_about .

:concept_type_dossier
        a                    owl:Class ;
        rdfs:comment         "Now coded with table 612 Pegase extract: <TYPE_DOSSIER id=\"1095\">Proposition de décision</TYPE_DOSSIER> Pegase translation tables: 1095 1005 PRDC PROPOSITION DE DECISION Proposition de décision 22-JUL-04 8888 1095 1010 PRDC Vorschlag Beschluss/Entscheid. Vorschlag für eine Entschließung 03-JUN-98 2000 22-DEC-06 1" ;
        rdfs:label           "Concept representing the type of a dossier" ;
        rdfs:subClassOf      skos:Concept , :concept_decoding ;
        owl:equivalentClass  [ a               owl:Restriction ;
                               owl:hasValue    <http://publications.europa.eu/resource/authority/fd_612> ;
                               owl:onProperty  skos:inScheme
                             ] .

:date_transposition  a      owl:DatatypeProperty ;
        rdfs:comment        "TP" ;
        rdfs:label          "Date transposition" ;
        rdfs:range          xsd:date ;
        rdfs:subPropertyOf  :date .

:procurement_public_uses_originally_language
        a                   owl:ObjectProperty ;
        rdfs:comment        "Authentic language version of a public procurement notice" ;
        rdfs:domain         :procurement_public ;
        rdfs:label          "Public procurement uses originally language" ;
        rdfs:range          :language ;
        rdfs:subPropertyOf  :uses_originally .

:event_legal_formally-addresses_institution
        a                   owl:ObjectProperty ;
        rdfs:comment        "DEPRECATED, This legal event formally addresses a given institution. Examples include the transmission of a COM from the Commission to Council. Body role:Addressee for formal act. Relevant for legal analysis: true." ;
        rdfs:domain         :event_legal ;
        rdfs:label          "Legal event formally addresses institution" ;
        rdfs:range          :institution ;
        rdfs:subPropertyOf  :formally-addresses , :event_formally-addresses_institution ;
        owl:deprecated      true ;
        owl:inverseOf       :institution_formally-addressed_by_event_legal .

:dossier_contains_event_legal
        a                   owl:ObjectProperty ;
        rdfs:comment        "DEPRECATED, This dossier contains a legal event. Relevant for legal analysis: true." ;
        rdfs:domain         :dossier ;
        rdfs:label          "Dossier contains legal event" ;
        rdfs:range          :event_legal ;
        rdfs:subPropertyOf  :dossier_contains_event , :contains ;
        owl:deprecated      true ;
        owl:inverseOf       :event_legal_part_of_dossier .

:act_standing-committee_efta
        a                owl:Class ;
        rdfs:comment     "Act of European Free Trade Association (EFTA) Standing Committee (= subsector G of sector E in EUR-Lex)" ;
        rdfs:label       "Act of EFTA Standing Committee" ;
        rdfs:subClassOf  :document_efta .

:court-report_number  a     owl:DatatypeProperty ;
        rdfs:comment        "Number of the Court report" ;
        rdfs:domain         :court-report ;
        rdfs:label          "Court report number" ;
        rdfs:range          xsd:positiveInteger ;
        rdfs:subPropertyOf  :number .

:act_preparatory_date_debate
        a                   owl:DatatypeProperty ;
        rdfs:comment        "Date of debate on the proposed secondary legislation in the European Parliament, European Economic and Social Committee or European Committee of Regions. Relevant for legal analysis: true" ;
        rdfs:domain         :act_preparatory ;
        rdfs:label          "Date of debate" ;
        rdfs:range          xsd:date ;
        rdfs:subPropertyOf  :date_debate .

:declaration_transposition_member-state
        a           owl:DatatypeProperty ;
        rdfs:label  "Declaration transposition member state" .

:dossier_date_adopted
        a                   owl:DatatypeProperty ;
        rdfs:comment        "Relevant for legal analysis: true" ;
        rdfs:domain         :dossier ;
        rdfs:label          "Dossier was adopted on a given date" ;
        rdfs:range          xsd:date ;
        rdfs:subPropertyOf  :date_adopted .

:concept_type_comment
        a                    owl:Class ;
        rdfs:comment         "Corresponds to the contents of the Procat field CI, coded with FD_Table 301" ;
        rdfs:label           "Concept representing the type of a comment" ;
        rdfs:subClassOf      skos:Concept , :concept_decoding ;
        owl:equivalentClass  [ a               owl:Restriction ;
                               owl:hasValue    <http://publications.europa.eu/resource/authority/fd_301> ;
                               owl:onProperty  skos:inScheme
                             ] .

:institution_authors-report_event_legal
        a                   owl:ObjectProperty ;
        rdfs:domain         :institution ;
        rdfs:label          "Institution authors report on legal event" ;
        rdfs:range          :event_legal ;
        rdfs:subPropertyOf  :authors-report .

:agreement_international
        a                owl:Class ;
        rdfs:comment     "International agreements (= sector 2 in EUR-Lex)" ;
        rdfs:label       "International agreement" ;
        rdfs:subClassOf  :resource_legal .

:expression_original_translation_uses_language
        a                   owl:ObjectProperty ;
        rdfs:comment        "Relevant for legal analysis: true. The language of the of original and/or intermediate translations of text. Relevant for legal analysis: true" ;
        rdfs:domain         :expression ;
        rdfs:label          "Expression's original translation uses language" ;
        rdfs:range          :language ;
        rdfs:subPropertyOf  :original_translation_uses ;
        owl:inverseOf       :language_used_by_original_translation_expression .

:case-law_confirms_resource_legal
        a                   owl:ObjectProperty ;
        rdfs:comment        "This property points to legal act quoted in the operative part of Court decisions" ;
        rdfs:domain         :case-law ;
        rdfs:label          "Case law confirms legal resource" ;
        rdfs:range          :resource_legal ;
        rdfs:subPropertyOf  :confirms ;
        owl:inverseOf       :resource_legal_confirmed_by_case-law .

<http://publications.europa.eu/resource/authority/fd_300>
        a       owl:NamedIndividual .

:dossier_type_reference
        a                   owl:DatatypeProperty ;
        rdfs:comment        "Reference to this procedure. This will serve for the search in files. Procedure reference type. Relevant for legal analysis: true." ;
        rdfs:domain         :dossier ;
        rdfs:label          "Reference type" ;
        rdfs:range          xsd:string ;
        rdfs:subPropertyOf  :type_reference .

<http://publications.europa.eu/resource/authority/dataset-status>
        a       owl:NamedIndividual .

:declared_void_by  a  owl:ObjectProperty ;
        rdfs:label  "Declared void by" .

:resource_legal_published_in_court-report
        a             owl:ObjectProperty ;
        rdfs:comment  "RECUEIL and subfields RECUEIL_ANNE RECUEIL_PARTIE RECUEIL_PAGE_DEB are exposed as annotations of this link between the legal resource and the official journal" ;
        rdfs:domain   :resource_legal ;
        rdfs:label    "Legal resource published in Court report" ;
        rdfs:range    :court-report .

:si_package_ec  a        owl:Class ;
        rdfs:comment     "Internal documents of the European Commission with a SI type identifier, meanwhile declassified." ;
        rdfs:label       "SI package EC" ;
        rdfs:subClassOf  :swd_package_ec ;
        rdfs:subClassOf  [ a               owl:Restriction ;
                           owl:hasValue    "SI" ;
                           owl:onProperty  :archive_package_internal_number_prefix
                         ] ;
        dct:created      "2022-09-28T21:12:47Z"^^xsd:dateTime .

:legislation_secondary_modified_by_legislation_secondary
        a                   owl:ObjectProperty ;
        rdfs:comment        "Relevant for legal analysis: true" ;
        rdfs:domain         :legislation_secondary ;
        rdfs:label          "Secondary legislation is modified by legislation_secondary" ;
        rdfs:range          :legislation_secondary ;
        rdfs:subPropertyOf  :modified_by ;
        owl:inverseOf       :legislation_secondary_modifies_legislation_secondary .

:contract-nature_label
        a           owl:DatatypeProperty ;
        rdfs:label  "Contract nature label" .

:summary_legislation_eu_is_about_subject-matter
        a                   owl:ObjectProperty ;
        rdfs:comment        "A summary on EU legislation is about a concept expressed as a subject matter (classification tool). Refers to a concept from AT subject-matter, previously ATTO table FD_070 (with same codes). Relevant for legal analysis: true" ;
        rdfs:domain         :summary_legislation_eu ;
        rdfs:label          "Legislative summary EU is about subject matter" ;
        rdfs:range          :subject-matter ;
        rdfs:subPropertyOf  :is_about ;
        owl:inverseOf       :subject-matter_subject_of_summary_legislation_eu .

:expression_inherited
        a             owl:DatatypeProperty ;
        rdfs:comment  "Indication if the expression is inherited from another version of the document" ;
        rdfs:domain   :expression ;
        rdfs:label    "Expression inherited" ;
        rdfs:range    xsd:boolean .

:resource_legal_opinion_requested_by_communication_request_opinion
        a              owl:ObjectProperty ;
        rdfs:domain    :resource_legal ;
        rdfs:label     "Resource legal opinion requested by communication request opinion" ;
        rdfs:range     :communication_request_opinion ;
        owl:inverseOf  :communication_request_opinion_requests_opinion_on_resource_legal .

:recital_part_of_work
        a                   owl:ObjectProperty ;
        rdfs:comment        "This property associates an instance of a work with an instance of a recital that forms part of it." ;
        rdfs:domain         :recital ;
        rdfs:label          "Recital part of work" ;
        rdfs:range          :work ;
        rdfs:subPropertyOf  :subdivision_part_of_work , :part_of ;
        owl:inverseOf       :work_contains_recital .

:basis_for  a       owl:ObjectProperty ;
        rdfs:label  "Basis for" .

:official-journal-act_date_publication
        a                   owl:DatatypeProperty ;
        rdfs:comment        "Publication date of a special Official Journal act" ;
        rdfs:domain         :official-journal-act ;
        rdfs:label          "Official Journal act date publication" ;
        rdfs:range          xsd:date ;
        rdfs:subPropertyOf  :date_publication .

:amends  a          owl:ObjectProperty ;
        rdfs:label  "Amends" .

:event_internal_consultation_objective
        a                   owl:DatatypeProperty ;
        rdfs:comment        "Indicates the consultation objective of the internal event" ;
        rdfs:domain         :event_internal ;
        rdfs:label          "Consultation objective" ;
        rdfs:range          rdf:PlainLiteral ;
        rdfs:subPropertyOf  :consultation_objective .

:summary_legislation_eu_summarizes_resource_legal
        a                   owl:ObjectProperty ;
        rdfs:comment        "A legislative summarizes a legal resource (document)" ;
        rdfs:domain         :summary_legislation_eu ;
        rdfs:label          "Legislative summary summarizes legal resource" ;
        rdfs:range          :resource_legal ;
        rdfs:subPropertyOf  :summary_summarizes_work ;
        owl:inverseOf       :resource_legal_summarized_by_summary_legislation_eu .

:event_legal_mandatorily-consults_institution
        a                   owl:ObjectProperty ;
        rdfs:comment        "Relevant for legal analysis: true. This legal event mandatorily consults a given institution. Body role: Mandatory consultation. Relevant for legal analysis: true" ;
        rdfs:domain         :event_legal ;
        rdfs:label          "Legal event mandatorily consults institution" ;
        rdfs:range          :institution ;
        rdfs:subPropertyOf  :mandatorily-consults ;
        owl:inverseOf       :institution_mandatorily-consulted_by_event_legal .

:resource_legal_incidentally_declared_valid_case-law
        a                   owl:ObjectProperty ;
        rdfs:comment        "Calculated. Relevant for legal analysis: true." ;
        rdfs:domain         :resource_legal ;
        rdfs:label          "Legal resource incidentally declared valid by case law" ;
        rdfs:range          :case-law ;
        rdfs:subPropertyOf  :incidentally_declared_valid ;
        owl:inverseOf       :case-law_declares_incidentally_valid_resource_legal .

:non-opposition_concentration_notified
        a                owl:Class ;
        rdfs:comment     "Non-opposition to a notified concentration (= subsector 3M of sector 3). At present 3924 notices. Examples: 31990M0004, 31991M0021, 32010M5760" ;
        rdfs:label       "Non-opposition to notified concentration" ;
        rdfs:subClassOf  :legislation_secondary .

:official-forms_reference
        a           owl:DatatypeProperty ;
        rdfs:label  "Official forms reference" .

:resource_legal_confirmed_by_case-law
        a                   owl:ObjectProperty ;
        rdfs:comment        "Relevant for legal analysis: true" ;
        rdfs:domain         :resource_legal ;
        rdfs:label          "Legal resource confirmed by case law" ;
        rdfs:range          :case-law ;
        rdfs:subPropertyOf  :confirmed_by ;
        owl:inverseOf       :case-law_confirms_resource_legal .

:event_case_part1  a        owl:DatatypeProperty ;
        rdfs:comment        "Part 1 of the legal basis of the procedure. typical values PROT" ;
        rdfs:domain         :event_case ;
        rdfs:label          "Part 1 of the legal basis of the procedure" ;
        rdfs:range          xsd:string ;
        rdfs:subPropertyOf  :part1 .

:event_legal_date  a        owl:DatatypeProperty ;
        rdfs:comment        "DEPRECATED, The date of the legal event, Date of event. Relevant for legal analysis: true." ;
        rdfs:domain         :event_legal ;
        rdfs:label          "Date of legal event" ;
        rdfs:range          xsd:date ;
        rdfs:subPropertyOf  :event_date , :date ;
        owl:deprecated      true .

:has_licence  a     owl:ObjectProperty ;
        rdfs:label  "Has licence" .

:advocate-general_delivers_case-law
        a                   owl:ObjectProperty ;
        rdfs:comment        "AG" ;
        rdfs:domain         :advocate-general ;
        rdfs:label          "Advocate general delivers case law" ;
        rdfs:range          :case-law ;
        rdfs:subPropertyOf  :delivers ;
        owl:inverseOf       :case-law_delivered_by_advocate-general .

:communication_case_new
        a                owl:Class ;
        rdfs:comment     "Communication on a New Case in sector 6" ;
        rdfs:label       "Communication on a new case" ;
        rdfs:subClassOf  :communication_cjeu .

:work_id_obsolete_document
        a                   owl:DatatypeProperty ;
        rdfs:domain         :work ;
        rdfs:label          "Obsolete document identifier" ;
        rdfs:range          xsd:string ;
        rdfs:subPropertyOf  :id_obsolete_document .

:responsible_for  a  owl:ObjectProperty ;
        rdfs:label  "Responsible for" .

:report_ep_reported_by_agent
        a                   owl:ObjectProperty ;
        rdfs:comment        "Name of the person (EP member or member of CoR or EESC) who reports on the relevant act. This property will be deprecated and replaced with work_reported_by_person. Role RAPP. Relevant for legal analysis: true" ;
        rdfs:domain         :report_ep ;
        rdfs:label          "European Parliament report has rapporteur" ;
        rdfs:range          :agent ;
        rdfs:subPropertyOf  :reported_by ;
        owl:inverseOf       :agent_reports_on_report_ep .

:labels_forms_link_title
        a           owl:DatatypeProperty ;
        rdfs:label  "Labels forms link title" .

:cor_opinion_contained_in
        a           owl:ObjectProperty ;
        rdfs:label  "Cor opinion contained in" .

:requests  a        owl:ObjectProperty ;
        rdfs:label  "Requests" .

<http://publications.europa.eu/resource/authority/corporate-body/ECB>
        a       owl:NamedIndividual .

:publication_general_title_part
        a                   owl:DatatypeProperty ;
        rdfs:comment        "Name of part or section of a work. Marc fields 700 p, 710 p and 711 n | How do fields 700 p, 710 p and 711 n differ? 700 = Personal name (of the author); p = Name of part/section of a work 710 = Corporate name (of the author); p = Name of part/section of a work 711 = Meeting name; n = Number of part/section/meeting" ;
        rdfs:domain         :publication_general ;
        rdfs:label          "Title of part" ;
        rdfs:range          rdfs:Literal ;
        rdfs:subPropertyOf  :title_part .

:publication_general_is_about_concept_op_theme
        a                   owl:ObjectProperty ;
        rdfs:comment        "Subject of the publication" ;
        rdfs:domain         :publication_general ;
        rdfs:label          "General publication is about concept op theme" ;
        rdfs:range          :concept_op_theme ;
        rdfs:subPropertyOf  :is_about ;
        owl:inverseOf       :concept_op_theme_subject_of_publication_general .

:publication_general_is_about_concept_udc
        a                   owl:ObjectProperty ;
        rdfs:domain         :publication_general ;
        rdfs:label          "General publication is about udc concept" ;
        rdfs:range          :concept_udc ;
        rdfs:subPropertyOf  :is_about .

:authority_certification
        a           owl:DatatypeProperty ;
        rdfs:label  "Authority certification" .

:based_on  a        owl:ObjectProperty ;
        rdfs:label  "Based on" .

:work_dataset  a         owl:Class ;
        rdfs:comment     "Equivalent class in the cdm model to dcat:Dataset" ;
        rdfs:label       "Work dataset" ;
        rdfs:subClassOf  :work ;
        rdfs:subClassOf  [ a                            owl:Restriction ;
                           owl:maxQualifiedCardinality  "1"^^xsd:nonNegativeInteger ;
                           owl:onClass                  :concept_type_dataset ;
                           owl:onProperty               :work_dataset_has_type_concept_type_dataset
                         ] ;
        rdfs:subClassOf  [ a                   owl:Restriction ;
                           owl:maxCardinality  "1"^^xsd:nonNegativeInteger ;
                           owl:onProperty      :work_dataset_date_start
                         ] ;
        rdfs:subClassOf  [ a                   owl:Restriction ;
                           owl:maxCardinality  "1"^^xsd:nonNegativeInteger ;
                           owl:onProperty      :work_dataset_nature_classification
                         ] ;
        rdfs:subClassOf  [ a                   owl:Restriction ;
                           owl:maxCardinality  "1"^^xsd:nonNegativeInteger ;
                           owl:onProperty      :work_dataset_date_end
                         ] ;
        rdfs:subClassOf  [ a                            owl:Restriction ;
                           owl:minQualifiedCardinality  "1"^^xsd:nonNegativeInteger ;
                           owl:onClass                  :agent ;
                           owl:onProperty               :work_dataset_published_by_agent
                         ] ;
        rdfs:subClassOf  [ a                            owl:Restriction ;
                           owl:maxQualifiedCardinality  "1"^^xsd:nonNegativeInteger ;
                           owl:onClass                  :publication_frequency ;
                           owl:onProperty               :work_dataset_has_frequency_publication_frequency
                         ] ;
        rdfs:subClassOf  [ a                            owl:Restriction ;
                           owl:maxQualifiedCardinality  "1"^^xsd:nonNegativeInteger ;
                           owl:onClass                  :concept_theme_dataset ;
                           owl:onProperty               :work_dataset_has_theme_concept_theme_dataset
                         ] ;
        rdfs:subClassOf  [ a                   owl:Restriction ;
                           owl:maxCardinality  "1"^^xsd:nonNegativeInteger ;
                           owl:onProperty      :work_dataset_date_modified
                         ] .

:concept_op_theme  a         owl:Class ;
        rdfs:comment         "Used to classify general publications" ;
        rdfs:label           "OP Theme concept" ;
        rdfs:subClassOf      skos:Concept , :concept ;
        owl:equivalentClass  [ a               owl:Restriction ;
                               owl:hasValue    <http://publications.europa.eu/resource/authority/pub-theme> ;
                               owl:onProperty  skos:inScheme
                             ] .

:case-law_interpretes_resource_legal
        a                   owl:ObjectProperty ;
        rdfs:comment        "This property points to legal act quoted in the operative part of Court decisions." ;
        rdfs:domain         :case-law ;
        rdfs:label          "Case law interprets legal resource" ;
        rdfs:range          :resource_legal ;
        rdfs:subPropertyOf  :interpretes ;
        owl:inverseOf       :resource_legal_interpreted_by_case-law .

:resource_legal_efta  a     owl:DatatypeProperty ;
        rdfs:domain         :resource_legal ;
        rdfs:label          "Resource legal efta" ;
        rdfs:range          xsd:boolean ;
        rdfs:subPropertyOf  :efta .

:repeals  a         owl:ObjectProperty ;
        rdfs:label  "Repeals" .

:case-law_is_about_concept_new_case-law
        a                   owl:ObjectProperty ;
        rdfs:comment        "Case law directory code is a specific directory classification for EU case law. This one refers to the classification used after Lisbon treaty. Currently coded with FD_578." ;
        rdfs:domain         :case-law ;
        rdfs:label          "Case law is about new case law concept" ;
        rdfs:range          :concept_new_case-law ;
        rdfs:subPropertyOf  :is_about , :case-law_is_about_concept ;
        owl:inverseOf       :concept_new_case-law_subject_of_case-law .

:resource_legal_adds_to_resource_legal
        a                   owl:ObjectProperty ;
        rdfs:comment        "This property points to act which some new provisions are added. Relevant for legal analysis: true" ;
        rdfs:domain         :resource_legal ;
        rdfs:label          "Legal resource adds to legal resource" ;
        rdfs:range          :resource_legal ;
        rdfs:subPropertyOf  :adds_to ;
        owl:inverseOf       :resource_legal_added_to_resource_legal .

:on_agenda  a       owl:ObjectProperty ;
        rdfs:label  "On agenda" .

:concept_type_documentation
        a                owl:Class ;
        rdfs:comment     "Corresponds to the contents of the MDR authority list documentation type" ;
        rdfs:label       "Concept representing the documentation of a dataset" ;
        rdfs:subClassOf  :concept_decoding .

:concept_type_event_legal_is_type_of_event_legal
        a                   owl:ObjectProperty ;
        rdfs:comment        "type of event associated to the event" ;
        rdfs:domain         :concept_type_event_legal ;
        rdfs:label          "concept type event associated to the legal event" ;
        rdfs:range          :event_legal ;
        rdfs:subPropertyOf  :is_type_of ;
        owl:inverseOf       :event_legal_has_type_concept_type_event_legal .

:agent_responsible_for_resource_legal
        a              owl:ObjectProperty ;
        rdfs:comment   "Agent is responsible for a legal resource" ;
        rdfs:domain    :agent ;
        rdfs:label     "Agent responsible for a legal resource" ;
        rdfs:range     :resource_legal ;
        owl:inverseOf  :resource_legal_responsibility_of_agent .

:dossier_summary  a   owl:DatatypeProperty ;
        rdfs:comment  "a summary of the dossier" ;
        rdfs:domain   :dossier ;
        rdfs:label    "Dossier summary" ;
        rdfs:range    rdf:PlainLiteral .

:date_creation  a   owl:DatatypeProperty ;
        rdfs:label  "Date creation" .

:expression_procurement_public_authority-type_name
        a                   owl:DatatypeProperty ;
        rdfs:comment        "Suitable authority type" ;
        rdfs:domain         :expression_procurement_public ;
        rdfs:label          "Authority type name" ;
        rdfs:range          xsd:string ;
        rdfs:subPropertyOf  :authority-type_name .

<http://publications.europa.eu/resource/authority/language>
        a       owl:NamedIndividual .

:declaration  a          owl:Class ;
        rdfs:comment     "Subsector C of sector 3. At present 23 notices. Examples: 31995C0907, 32003C0929(01), 32007C0630(01), 32005C0295" ;
        rdfs:label       "Declaration" ;
        rdfs:subClassOf  :legislation_secondary .

:id_legissum  a     owl:DatatypeProperty ;
        rdfs:label  "Id legissum" .

<http://publications.europa.eu/resource/authority/fd_608>
        a       owl:NamedIndividual .

:concept_directory-code
        a                    owl:Class ;
        rdfs:comment         "Concept in the directory code. Currently coded using FD Table 555" ;
        rdfs:label           "Directory code concept" ;
        rdfs:subClassOf      skos:Concept , :concept ;
        owl:equivalentClass  [ a               owl:Restriction ;
                               owl:hasValue    <http://publications.europa.eu/resource/authority/fd_555> ;
                               owl:onProperty  skos:inScheme
                             ] ;
        owl:equivalentClass  [ a               owl:Restriction ;
                               owl:hasValue    <http://publications.europa.eu/resource/authority/dir-eu-legal-act> ;
                               owl:onProperty  skos:inScheme
                             ] .

:event_legal_informs_institution
        a                   owl:ObjectProperty ;
        rdfs:comment        "DEPRECATED, This legal event addresses for information a given institution. Body role:Addressee for information. Relevant for legal analysis: true." ;
        rdfs:domain         :event_legal ;
        rdfs:label          "Legal event informs institution" ;
        rdfs:range          :institution ;
        rdfs:subPropertyOf  :informs , :event_informs_institution ;
        owl:deprecated      true ;
        owl:inverseOf       :institution_informed_by_event_legal .

:staff-working-document
        a                owl:Class ;
        rdfs:comment     "resource_legal_type = (SC or JC or none), resource_legal_id_sector = 5, work_has_resource-type = (SWD, JOINT_SWD, IMPACT_ASSESS, IMPACT_ASSESS_SUM, WORK_DOC, REPORT, COMMUNIC, COMMUNIC_POSIT, OPIN, ACT_OTHER,OPIN_IMPACT_ASSESS, JOINT_TEXT, JOINT_IMPACT_ASSESS, JOINT_IMPACT_ASSESS_SUM)" ;
        rdfs:label       "Staff Working document" ;
        rdfs:subClassOf  :act_preparatory ;
        rdfs:subClassOf  [ a                   owl:Restriction ;
                           owl:maxCardinality  "1"^^xsd:nonNegativeInteger ;
                           owl:onProperty      :staff-working-document_id_com
                         ] .

:resource_legal_failure_stated_by_case-law
        a                   owl:ObjectProperty ;
        rdfs:comment        "Calculated. Relevant for legal analysis: true." ;
        rdfs:domain         :resource_legal ;
        rdfs:label          "Legal resource failure stated by case law" ;
        rdfs:range          :case-law ;
        rdfs:subPropertyOf  :failure_stated_by ;
        owl:inverseOf       :case-law_states_failure_concerning_resource_legal .

:communication_opinion
        a                owl:Class ;
        rdfs:comment     "Communication opinion in sector 6" ;
        rdfs:label       "Communication opinion" ;
        rdfs:subClassOf  :communication_cjeu .

:number_edition  a  owl:DatatypeProperty ;
        rdfs:label  "Number edition" .

:work_dataset_spatial_country
        a                   owl:ObjectProperty ;
        rdfs:comment        "This property refers to a geographic region that is covered by the dataset" ;
        rdfs:domain         :work_dataset ;
        rdfs:label          "Dataset spatial" ;
        rdfs:range          :country ;
        rdfs:subPropertyOf  :spatial .

:language_used_by_original_translation_expression
        a                   owl:ObjectProperty ;
        rdfs:comment        "A given language is used for the original translation of an expression (typically of a general publication)" ;
        rdfs:domain         :language ;
        rdfs:label          "Language used by original translation" ;
        rdfs:range          :expression ;
        rdfs:subPropertyOf  :used_by_original_translation .

:work_authored_by_agent
        a                   owl:ObjectProperty ;
        rdfs:comment        "The work is authored by an agent" ;
        rdfs:domain         :work ;
        rdfs:label          "Work is authored by agent" ;
        rdfs:range          :agent ;
        rdfs:subPropertyOf  :work_created_by_agent , :authored_by ;
        dct:created         "2018-08-30T11:07:33.027+02:00"^^xsd:dateTime ;
        owl:inverseOf       :agent_authors_work .

:resource_legal_interpreted_authoritatively_by_resource_legal
        a                   owl:ObjectProperty ;
        rdfs:comment        "Calculated. Relevant for legal analysis: true." ;
        rdfs:domain         :resource_legal ;
        rdfs:label          "Legal resource interpreted authoritatively by legal resource" ;
        rdfs:range          :resource_legal ;
        rdfs:subPropertyOf  :interpreted_authoritatively_by ;
        owl:inverseOf       :resource_legal_interpretes_authoritatively_resource_legal .

:case-law_uses_procedure_language
        a                   owl:ObjectProperty ;
        rdfs:comment        "The case uses a given language of procedure" ;
        rdfs:domain         :case-law ;
        rdfs:label          "Case law uses language of procedure" ;
        rdfs:range          :language ;
        rdfs:subPropertyOf  :uses_procedure .

:event_title  a             owl:DatatypeProperty ;
        rdfs:comment        "Title text of an event" ;
        rdfs:domain         :event ;
        rdfs:label          "Event title" ;
        rdfs:range          rdf:PlainLiteral ;
        rdfs:subPropertyOf  :title .

:container_case-law_year_decision
        a                   owl:DatatypeProperty ;
        rdfs:domain         :container_case-law ;
        rdfs:label          "Year of the decision" ;
        rdfs:range          xsd:gYear ;
        rdfs:subPropertyOf  :year_decision .

:institution_initiates_event_legal
        a                   owl:ObjectProperty ;
        rdfs:comment        "The institution initiates a legal event" ;
        rdfs:domain         :institution ;
        rdfs:label          "Institution initiates legal event" ;
        rdfs:range          :event_legal ;
        rdfs:subPropertyOf  :initiates .

:citation  a             owl:Class ;
        rdfs:comment     "A citation in a legal document. Created to have correspondance to the subdivision NAL" ;
        rdfs:label       "Citation" ;
        rdfs:subClassOf  :subdivision .

:read_by  a         owl:ObjectProperty ;
        rdfs:label  "Read by" .

:signature_digital_date_signature_xades-a
        a                   owl:DatatypeProperty ;
        rdfs:comment        "Date and time this signature got its XAdES-A" ;
        rdfs:domain         :signature_digital ;
        rdfs:label          "XAdES-A date and time" ;
        rdfs:range          xsd:dateTime ;
        rdfs:subPropertyOf  :date_signature_xades-a .

:institution_formally-addressed_by_event_legal
        a                   owl:ObjectProperty ;
        rdfs:domain         :institution ;
        rdfs:label          "Institution formally-addressed by legal event" ;
        rdfs:range          :event_legal ;
        rdfs:subPropertyOf  :formally-addressed_by .

:cooperation_police-and-judicial
        a                owl:Class ;
        rdfs:comment     "Police and judicial cooperation in criminal matters (subsector F of sector 3). At present 142 notices. Examples: 31995F0073, 31995F0401, 32009F0905" ;
        rdfs:label       "Police and judicial cooperation" ;
        rdfs:subClassOf  :legislation_secondary .

:work_contains_rule_legal
        a                   owl:ObjectProperty ;
        rdfs:domain         :work ;
        rdfs:label          "Work contains rule (legal)" ;
        rdfs:range          :rule_legal ;
        rdfs:subPropertyOf  :work_contains_subdivision , :contains .

:act_preparatory_eesc
        a                owl:Class ;
        rdfs:comment     "Preparatory act by the European Economic and Social Committee" ;
        rdfs:label       "Preparatory act by EESC" ;
        rdfs:subClassOf  :act_preparatory ;
        rdfs:subClassOf  [ a               owl:Restriction ;
                           owl:hasValue    <http://publications.europa.eu/resource/authority/corporate-body/EESC> ;
                           owl:onProperty  :work_created_by_agent
                         ] ;
        rdfs:subClassOf  [ a                   owl:Restriction ;
                           owl:maxCardinality  "1"^^xsd:nonNegativeInteger ;
                           owl:onProperty      :act_preparatory_eesc_priority_class
                         ] .

:work_contains_annex  a     owl:ObjectProperty ;
        rdfs:comment        "The annex of this work" ;
        rdfs:domain         :work ;
        rdfs:label          "Work contains annex" ;
        rdfs:range          :annex ;
        rdfs:subPropertyOf  :work_contains_subdivision , :contains .

:expression_is_included_in_work
        a             owl:ObjectProperty ;
        rdfs:comment  "Indication if the expression has to be considered included in a work different from its parent work" ;
        rdfs:label    "Expression is included in work" .

:group_parliamentary  a      owl:Class ;
        rdfs:label           "Parliamentary group" ;
        rdfs:subClassOf      skos:Concept , :agent ;
        owl:equivalentClass  [ a               owl:Restriction ;
                               owl:hasValue    <http://publications.europa.eu/resource/authority/corporate-body> ;
                               owl:onProperty  skos:inScheme
                             ] .

:work_has_successor_work
        a                   owl:ObjectProperty ;
        rdfs:comment        "cf. above" ;
        rdfs:domain         :work ;
        rdfs:label          "Work has successor work" ;
        rdfs:range          :work ;
        rdfs:subPropertyOf  :has_successor ;
        owl:inverseOf       :work_is_logical_successor_of_work .

:work_is_about_concept_eurovoc
        a                   owl:ObjectProperty ;
        rdfs:comment        "Relevant for legal analysis: true. The work is about a concept, typically expressed as a Eurovoc concept, but also through other taxonomies and thesauri. It represents thus mainly the information currently contained in the VOLET_EUROVOC. Eurovoc descriptors are not used for all Legal ressources, name changed at request of IRIS. DC. Relevant for legal analysis: true" ;
        rdfs:domain         :work ;
        rdfs:label          "Work is about a Eurovoc concept" ;
        rdfs:range          :concept_eurovoc ;
        rdfs:subPropertyOf  :is_about ;
        owl:inverseOf       :concept_eurovoc_subject_of_work .

:evolutive_work_business_classification
        a            owl:DatatypeProperty ;
        rdfs:domain  :evolutive_work ;
        rdfs:label   "Evolutive work business classification" ;
        rdfs:range   xsd:anyURI .

[ a            owl:AllDisjointClasses ;
  owl:members  ( :document_efta :case-law )
] .

:identifier  a        owl:DatatypeProperty ;
        rdfs:comment  "Any type of identifier:" ;
        rdfs:label    "Any type of identifier" .

:work_datetime_transmission
        a                   owl:DatatypeProperty ;
        rdfs:comment        "Date on which a work was transmitted" ;
        rdfs:domain         :work ;
        rdfs:label          "Datetime Transmission" ;
        rdfs:range          xsd:dateTime ;
        rdfs:subPropertyOf  :datetime_transmission .

:has_theme  a       owl:ObjectProperty ;
        rdfs:label  "Has theme" .

:recommendation_ecsc_date_transposition
        a                   owl:DatatypeProperty ;
        rdfs:comment        "Date of transposition applicable to recommendation of the European Coal and Steel community; can contain multiple values as different parts of a directive can be implemented by various pieces of national legislation, coming with different dates (TP_DATE). TP_COMMENT is mixed content, coded with fd_361. Relevant for legal analysis: true" ;
        rdfs:domain         :recommendation_ecsc ;
        rdfs:label          "Date of transposition of a ECSC recommendation" ;
        rdfs:range          xsd:date ;
        rdfs:subPropertyOf  :date_transposition .

:resource_legal_id_sector
        a                   owl:DatatypeProperty ;
        rdfs:comment        "Identifier of the sector (DT_SEC). Relevant for legal analysis: true." ;
        rdfs:domain         :resource_legal ;
        rdfs:label          "Sector identifier" ;
        rdfs:range          xsd:string ;
        rdfs:subPropertyOf  :id_sector .

:reference-data_publication_publishes_reference-data_asset_release
        a                   owl:ObjectProperty ;
        rdfs:comment        "This predicate describes the relation between a representant of a reference data asset version and the publications in which it was made public. " ;
        rdfs:domain         :reference-data_publication ;
        rdfs:label          "Reference data publication publishes reference data asset release" ;
        rdfs:range          :reference-data_asset_release ;
        rdfs:subPropertyOf  :publishes ;
        owl:inverseOf       :reference-data_asset_release_published_in_reference-data_publication .

:confirmed_by  a    owl:ObjectProperty ;
        rdfs:label  "Confirmed by" .

:ep_opinion_contained_in
        a           owl:ObjectProperty ;
        rdfs:label  "Ep opinion contained in" .

:resource_legal_confirms_resource_legal
        a                   owl:ObjectProperty ;
        rdfs:comment        "Relevant for legal analysis: true" ;
        rdfs:domain         :resource_legal ;
        rdfs:label          "Legal resource confirms resource_legal" ;
        rdfs:range          :resource_legal ;
        rdfs:subPropertyOf  :confirms ;
        owl:inverseOf       :resource_legal_confirmed_by_resource_legal .

:product-form  a             owl:Class ;
        rdfs:comment         "Corresponds to the contents of authority table product-form (http://publications.europa.eu/resource/authority/product-form)" , "Concept of a product form from authority table product-form (http://publications.europa.eu/resource/authority/product-form)" ;
        rdfs:label           "Product form concept" ;
        rdfs:subClassOf      :concept_decoding ;
        owl:equivalentClass  [ a               owl:Restriction ;
                               owl:hasValue    <http://publications.europa.eu/resource/authority/product-form> ;
                               owl:onProperty  skos:inScheme
                             ] .

:resource_legal_demed_reference
        a                   owl:DatatypeProperty ;
        rdfs:comment        "Demande d'editon. Added in the context of IMMC2CDM-OJ" ;
        rdfs:domain         :resource_legal ;
        rdfs:label          "This element is used to mark up the Demed number" ;
        rdfs:range          xsd:string ;
        rdfs:subPropertyOf  :demed_reference .

:type_event_interinstitutional
        a                    owl:Class ;
        rdfs:comment         "Concept representing the type of an event in the interinstitutional procedure" ;
        rdfs:label           "Type of an interinstitutional event" ;
        rdfs:subClassOf      skos:Concept ;
        owl:equivalentClass  [ a               owl:Restriction ;
                               owl:hasValue    <http://publications.europa.eu/resource/authority/event> ;
                               owl:onProperty  skos:inScheme
                             ] .

:resource_legal_replaced_by_resource_legal
        a                   owl:ObjectProperty ;
        rdfs:comment        "Calculated. Relevant for legal analysis: true." ;
        rdfs:domain         :resource_legal ;
        rdfs:label          "Legal resource replaced by legal resource" ;
        rdfs:range          :resource_legal ;
        rdfs:subPropertyOf  :replaced_by ;
        owl:inverseOf       :resource_legal_replaces_resource_legal .

:subsection_oj  a   owl:DatatypeProperty ;
        rdfs:label  "Subsection oj" .

:date_request_opinion
        a                   owl:DatatypeProperty ;
        rdfs:label          "Date request opinion" ;
        rdfs:range          xsd:date ;
        rdfs:subPropertyOf  :date .

:case-law_source_ruling_preliminary
        a                   owl:DatatypeProperty ;
        rdfs:comment        "Identifier of the source of the preliminary ruling in the title of a case law document (language-specific)" ;
        rdfs:domain         :case-law ;
        rdfs:label          "Source of preliminary ruling" ;
        rdfs:range          xsd:string ;
        rdfs:subPropertyOf  :source_ruling_preliminary .

:is_logical_successor
        a           owl:ObjectProperty ;
        rdfs:label  "Is logical successor" .

:explains  a        owl:ObjectProperty ;
        rdfs:label  "Explains" .

:expression_description_editorial
        a                   owl:DatatypeProperty ;
        rdfs:comment        "editorial content that further elaborates the abstract with other editorial content" ;
        rdfs:domain         :expression ;
        rdfs:label          "Expression editorial description" ;
        rdfs:range          <http://publications.europa.eu/ontology/datatype#string_or_xml> ;
        rdfs:subPropertyOf  :description_editorial .

<http://publications.europa.eu/resource/authority/fd_603>
        a       owl:NamedIndividual .

:manifestation_distribution
        a                owl:Class ;
        rdfs:label       "Distribution of a dataset" ;
        rdfs:subClassOf  :manifestation ;
        rdfs:subClassOf  [ a                            owl:Restriction ;
                           owl:maxQualifiedCardinality  "1"^^xsd:nonNegativeInteger ;
                           owl:onClass                  :distribution_status ;
                           owl:onProperty               :manifestation_distribution_has_status_distribution_status
                         ] ;
        rdfs:subClassOf  [ a                            owl:Restriction ;
                           owl:maxQualifiedCardinality  "1"^^xsd:nonNegativeInteger ;
                           owl:onClass                  :licence_document ;
                           owl:onProperty               :manifestation_distribution_has_licence_licence_document
                         ] ;
        rdfs:subClassOf  [ a                   owl:Restriction ;
                           owl:maxCardinality  "1"^^xsd:nonNegativeInteger ;
                           owl:onProperty      :manifestation_distribution_date_modified
                         ] ;
        rdfs:subClassOf  [ a                   owl:Restriction ;
                           owl:maxCardinality  "1"^^xsd:nonNegativeInteger ;
                           owl:onProperty      :manifestation_distribution_byte_size
                         ] ;
        rdfs:subClassOf  [ a                            owl:Restriction ;
                           owl:maxQualifiedCardinality  "1"^^xsd:nonNegativeInteger ;
                           owl:onDataRange              xsd:anyURI ;
                           owl:onProperty               :manifestation_distribution_access_url
                         ] .

:resource_legal_internal_number_suffix
        a                   owl:DatatypeProperty ;
        rdfs:comment        "Suffix of the unique internal identifier of the resource legal. The suffix serves the purpose of identifying the original document and the modifications made to it" ;
        rdfs:domain         :resource_legal ;
        rdfs:label          "Internal number suffix" ;
        rdfs:range          xsd:string ;
        rdfs:subPropertyOf  :internal_number_suffix .

:communication_cjeu  a   owl:Class ;
        rdfs:comment     "Communication of the court of justice (in sector 6)" ;
        rdfs:label       "Court communication" ;
        rdfs:subClassOf  :document_cjeu .

:assessment_impact_summary_ec
        a                owl:Class ;
        rdfs:comment     "Summary of Impact Assessment documents for the European Commission" ;
        rdfs:label       "European Commission Summary of Impact Assessment" ;
        rdfs:subClassOf  :staff-working-document_ec .

:swd_package_ec_has_title_from_com_final
        a                   owl:DatatypeProperty ;
        rdfs:domain         :swd_package_ec ;
        rdfs:label          "SWD package EC has title from COM final" ;
        rdfs:range          xsd:boolean ;
        rdfs:subPropertyOf  :archive_package_ec_has_title_from_com_final .

:id_celex  a                owl:DatatypeProperty ;
        rdfs:comment        "Former CELEX number (= DN and DN2)" ;
        rdfs:label          "Id celex" ;
        rdfs:subPropertyOf  :identifier .

:communication_order_cjeu
        a                owl:Class ;
        rdfs:comment     "Communication on a court order in sector 6" ;
        rdfs:label       "Communication on a court order" ;
        rdfs:subClassOf  :communication_cjeu .

:publication_general_source_information_additional
        a                   owl:DatatypeProperty ;
        rdfs:comment        "Additional source of information relating to this general publication" ;
        rdfs:domain         :publication_general ;
        rdfs:label          "Additional source of information" ;
        rdfs:range          xsd:string ;
        rdfs:subPropertyOf  :source_information_additional .

:procedure_code_interinstitutional_year_procedure
        a                   owl:DatatypeProperty ;
        rdfs:comment        "Relevant for legal analysis: true. Year of this procedure. Relevant for legal analysis: true" ;
        rdfs:domain         :procedure_code_interinstitutional ;
        rdfs:label          "Year of procedure" ;
        rdfs:range          xsd:gYear ;
        rdfs:subPropertyOf  :year_procedure .

:derogates  a       owl:ObjectProperty ;
        rdfs:label  "Derogates" .

:manifestation_year  a      owl:DatatypeProperty ;
        rdfs:comment        "Relevant for legal analysis: true. year of this manifestation. mapped from 260 $c. Relevant for legal analysis: true" ;
        rdfs:domain         :manifestation ;
        rdfs:label          "Manifestation year" ;
        rdfs:range          xsd:gYear ;
        rdfs:subPropertyOf  :year .

:manifestation_embargo
        a                   owl:DatatypeProperty ;
        rdfs:comment        "Is this manifestation under embargo? This instance must not be shown until the indicated datetime has been reached. In case a release date is not known,9999-12-31 should be used (= absolute embargo)" ;
        rdfs:domain         :manifestation ;
        rdfs:label          "Manifestation embargo" ;
        rdfs:range          xsd:dateTime ;
        rdfs:subPropertyOf  :embargo .

:act_preparatory  a      owl:Class ;
        rdfs:comment     "As per the decision of the meeting of 2010-05-11 the works in sector 5 will be split in real preparatory acts and others such as the report of the Court of Auditors. They will be distinguished by document type and author (e.g. the opinion of the ECB). The preparatory acts have thus been restructured to clearly distinguish between preparatory acts in a strict sense (COMs etc.) and other types of documents that have traditionally been grouped in sector 5." ;
        rdfs:label       "Preparatory act" ;
        rdfs:subClassOf  :resource_legal ;
        rdfs:subClassOf  [ a                   owl:Restriction ;
                           owl:maxCardinality  "1"^^xsd:nonNegativeInteger ;
                           owl:onProperty      :act_preparatory_term_parliamentary
                         ] ;
        rdfs:subClassOf  [ a                   owl:Restriction ;
                           owl:maxCardinality  "1"^^xsd:nonNegativeInteger ;
                           owl:onProperty      :act_preparatory_number_session_planned
                         ] ;
        rdfs:subClassOf  [ a                   owl:Restriction ;
                           owl:maxCardinality  "1"^^xsd:nonNegativeInteger ;
                           owl:onProperty      :act_preparatory_number_session
                         ] ;
        rdfs:subClassOf  [ a                   owl:Restriction ;
                           owl:maxCardinality  "1"^^xsd:nonNegativeInteger ;
                           owl:onProperty      :act_preparatory_has_status
                         ] .

:work_reported_by_agent
        a             owl:ObjectProperty ;
        rdfs:comment  "Work is the report of a reporting agent (AT corporate body, AT country, other agent entities)" ;
        rdfs:domain   :work ;
        rdfs:label    "Work reported by agent" ;
        rdfs:range    :agent .

:work_is_logical_predecessor_of_work
        a            owl:ObjectProperty ;
        rdfs:domain  :work ;
        rdfs:label   "work_is_logical_predecessor_of_work " ;
        rdfs:range   :work .

:duration  a        owl:DatatypeProperty ;
        rdfs:label  "Duration" .

:notice_prior-information_authority-type_code
        a                   owl:DatatypeProperty ;
        rdfs:domain         :notice_prior-information ;
        rdfs:label          "Code of authority type" ;
        rdfs:range          xsd:string ;
        rdfs:subPropertyOf  :authority-type_code .

:communication_case_new_requests_review_of_decision_case-law
        a                   owl:ObjectProperty ;
        rdfs:comment        "This property points to legal act quoted in the communication on a new case published in OJ. Relevant for legal analysis: true" ;
        rdfs:domain         :communication_case_new ;
        rdfs:label          "Communication requesting the review of a order or judgement" ;
        rdfs:range          :case-law ;
        rdfs:subPropertyOf  :requests_review_of_decision ;
        owl:inverseOf       :case-law_decision_review_requested_by_communication_case_new .

<http://publications.europa.eu/resource/authority/fd_014>
        a       owl:NamedIndividual .

:ATTO_FD_110  a              owl:Class ;
        rdfs:label           "FD_110 ATTO table" ;
        rdfs:subClassOf      skos:Concept ;
        owl:equivalentClass  [ a               owl:Restriction ;
                               owl:hasValue    <http://publications.europa.eu/resource/authority/fd_110> ;
                               owl:onProperty  skos:inScheme
                             ] .

:adopted-proposal  a  owl:DatatypeProperty ;
        rdfs:label  "Adopted proposal" .

:manifestation-issue  a  owl:Class ;
        rdfs:comment     "Manifestation is the issue of a serial publication or series" ;
        rdfs:label       "Manifestation issue" ;
        rdfs:subClassOf  :manifestation-publication-general .

:decision_delegated  a   owl:Class ;
        rdfs:comment     "0 Delegated decision (DTS=3 AND FM=DECDEL). Examples: 32012D0186, 32012D0207" ;
        rdfs:label       "Delegated decision" ;
        rdfs:subClassOf  :legislation_secondary .

:work_sender_transmission
        a                   owl:DatatypeProperty ;
        rdfs:comment        "Sender at the source of the work transmitted" ;
        rdfs:domain         :work ;
        rdfs:label          "Sender of the transmission" ;
        rdfs:range          xsd:string ;
        rdfs:subPropertyOf  :sender_transmission .

:number_sequence  a  owl:DatatypeProperty ;
        rdfs:label  "Number sequence" .

:event_addresses_institution
        a                   owl:ObjectProperty ;
        rdfs:comment        "Relevant for legal analysis: true. This event addresses a given institution. Relevant for legal analysis: true" ;
        rdfs:domain         :event ;
        rdfs:label          "Event addresses institution" ;
        rdfs:range          :institution ;
        rdfs:subPropertyOf  :addresses ;
        owl:inverseOf       :institution_addressed_by_event .

:work_contains_work  a      owl:ObjectProperty ;
        rdfs:comment        "The work contains another work (e.g. a law contains many articles or a COM or CES document contains a number of split proposals)" ;
        rdfs:domain         :work ;
        rdfs:label          "Work contains work" ;
        rdfs:range          :work ;
        rdfs:subPropertyOf  :contains ;
        owl:inverseOf       :work_part_of_work .

:case-law_has_type_procedure_concept_type_procedure
        a                   owl:ObjectProperty ;
        rdfs:comment        "This field refers to the type of action or procedure and the result of the action or procedure by Court proceedings. Currently coded by FD_Table 100. This property shall be replaced by: cdm:case-law_has_procjur (type of action or procedure) and annot:result_decision pointing to procresult.\"" ;
        rdfs:domain         :case-law ;
        rdfs:label          "Case law has a type of procedure" ;
        rdfs:range          :concept_type_procedure ;
        rdfs:subPropertyOf  :has_type_procedure .

:concept_type_dataset
        a                owl:Class ;
        rdfs:comment     "Corresponds to the contents of the MDR authority list ADMS Asset type (http://purl.org/adms/assetype)" ;
        rdfs:label       "Concept representing the type of a dataset" ;
        rdfs:subClassOf  :concept_decoding .

<http://publications.europa.eu/resource/authority/fd_555>
        a       owl:NamedIndividual .

:person_co-reports_event
        a                   owl:ObjectProperty ;
        rdfs:domain         :person ;
        rdfs:label          "Person co-reports event" ;
        rdfs:range          :event ;
        rdfs:subPropertyOf  :co-reports .

:has    a           owl:ObjectProperty ;
        rdfs:label  "Has" .

:work_translated_by_agent
        a                   owl:ObjectProperty ;
        rdfs:comment        "The work is translated by an agent (AU)" ;
        rdfs:domain         :work ;
        rdfs:label          "Work is translated by agent" ;
        rdfs:range          :agent ;
        rdfs:subPropertyOf  :work_contributed_to_by_agent , :translated_by ;
        dct:created         "2018-08-30T11:11:48.160+02:00"^^xsd:dateTime ;
        owl:inverseOf       :agent_translates_work .

:publication_general  a  owl:Class ;
        rdfs:comment     "Any type of general publications, generally characterized currently by an ID_PUB. Cf. also the page [CMR Marc21 Mapping], now superseded by marc21_usage_and_frbr_mapping_harmonization_1.2.xls (cf. attachments). The following manifestation identifiers for general publications need to be covered in the CCR (including mappings): || Type in Marc 21 || Field in Marc 21 || Subfield / position in Marc 21 || Number of occrrences || Entity || FRBR mapping || Comment || Property || DC elements || Class / AttributeoF || Example || Systems || Use || Remarks || | Varfield | 20 | a | 1229 | manifestation | Manifestation identifier | IsIdOf - ISBN | identifier | references | identifier | 92-825-4954-2, 978-92-78-40510-6 | OJ, PUB, CORDIS | search | ISBN | | Varfield | 20 | z | 59 | manifestation | Manifestation identifier | IsIdOf - ISBN | identifier | references | identifier | 92-825-4954-X, 978-92-78-40510-7 | OJ, PUB, CORDIS | search | cancelled/invalid ISBN | | Varfield | 22 | a | 758 | manifestation | Manifestation identifier | IsIdOf - ISSN | identifier | references | identifier | 1022-842X | OJ, PUB, CORDIS | search | ISSN | | Varfield | 22 | y | 69 | manifestation | Manifestation identifier | IsIdOf - ISSN | identifier | references | identifier | 1022-8422 | OJ, PUB, CORDIS | search | incorrect ISSN | | Varfield | 22 | z | 2 | manifestation | Manifestation identifier | IsIdOf - ISSN | identifier | references | identifier | 1028-8422 | OJ, PUB, CORDIS | search | cancelled ISSN | | Varfield | 24 | a | 1223 | manifestation | Manifestation identifier | IsIdOf - DOI | identifier | references | identifier | 10.2830/41254 | OJ, PUB, CORDIS | search | DOI | | Varfield | 24 | z | 2 | manifestation | Manifestation identifier | IsIdOf - DOI | identifier | references | identifier | 10.2831/41254 | OJ, PUB, CORDIS | search | cancelled/invalid DOI | | Varfield | 30 | a | 40 | manifestation | Manifestation identifier | CODEN 6 char. - not used at OP | identifier | references | identifier | N/A | N/A | search | CODEN \"The CODEN is assigned by the International CODEN Section of Chemical Abstracts Service\" | | Varfield | 30 | b | 2 | manifestation | Manifestation identifier | 6 char. - not used at OP | identifier | references | identifier | N/A | N/A | search | | | Varfield | 86 | a | 31 | manifestation | Manifestation identifier | Government Document Classification Number ?? Should not be used | classification | subject | concept | N/A | N/A | search | index | | | Varfield | 29 | a | 6288 | manifestation | identifier (Not mapped in table 3) | IsIdOf - NumCat | identifier | references | identifier | OA-81-08-353-EN-C | OJ, PUB, CORDIS | search | Catalogue number | | | | Varfield | 29 | z | 17 | manifestation | identifier (Not mapped in table 3) | IsIdOf - NumCat | identifier | references | identifier | OA-81-08-353-EN-J | OJ, PUB, CORDIS | search | cancelled/invalid Catnum ? | | Varfield | 765 | z | 20 | manifestation | Manifestation identifier | hasId - ISBN | link | references | relation | | | | | | Varfield | 245 | a | 5866 | manifestation | Manifestation - Title | hasTitle - only for serials | title | title | title | Deutsche Bibliographie | | search | index | | | Varfield | 765 | z | 20 | manifestation | Manifestation identifier | hasId - ISBN | link | references | relation | | | | | | Varfield | 775 | x | 198 | manifestation | Manifestation identifier | hasId - ISSN | link | references | relation | | PUB | | | Varfield | 776 | x | 1 | manifestation | Manifestation identifier | hasId - ISSN | link | references | relation | | PUB | | | Varfield | 780 | x | 14 | manifestation | Manifestation identifier | hasId - ISSN | link | references | relation | | PUB | | | Varfield | 785 | x | 10 | manifestation | Manifestation identifier | hasId - ISSN | link | references | relation | | PUB | | | Varfield | 787 | x | 20 | manifestation | Manifestation identifier | hasId - ISSN | link | references | relation | | PUB | | | Varfield | 856 | u | 843 | manifestation | Manifestation identifier | isLocated | URL | URI | identifier | identifier | | | | Altogether the following fields needs to be covered for the manifestations of general publications: || Type in Marc 21 || Field in Marc 21 || Subfield / position in Marc 21 || Number of occrrences || Entity || FRBR mapping || Comment || Property || DC elements || Class / AttributeoF || Example || Systems || Use || Remarks || | Varfield | 20 | a | 1229 | manifestation | Manifestation identifier | IsIdOf - ISBN | identifier | references | identifier | 92-825-4954-2, 978-92-78-40510-6 | OJ, PUB CORDIS | search | ISBN | | Varfield | 20 | z | 59 | manifestation | Manifestation identifier | IsIdOf - ISBN | identifier | references | identifier | 92-825-4954-X, 978-92-78-40510-7 | OJ, PUB, CORDIS | search | cancelled/invalid ISBN | | Varfield | 22 | a | 758 | manifestation | Manifestation identifier | IsIdOf - ISSN | identifier | references | identifier | 1022-842X | OJ, PUB, CORDIS | search | ISSN | | Varfield | 22 | y | 69 | manifestation | Manifestation identifier | IsIdOf - ISSN | identifier | references | identifier | 1022-8422 | OJ, PUB, CORDIS | search | incorrect ISSN | | Varfield | 22 | z | 2 | manifestation | Manifestation identifier | IsIdOf - ISSN | identifier | references | identifier | 1028-8422 | OJ, PUB, CORDIS | search | cancelled ISSN | | Varfield | 24 | a | 1223 | manifestation | Manifestation identifier | IsIdOf - DOI | identifier | references | identifier | 10.2830/41254 | OJ, PUB, CORDIS | search | DOI | | Varfield | 24 | z | 2 | manifestation | Manifestation identifier | IsIdOf - DOI | identifier | references | identifier | 10.2831/41254 | OJ, PUB, CORDIS | search | cancelled/invalid DOI | | Varfield | 29 | a | 6288 | manifestation | identifier (Not mapped in table 3) | IsIdOf - NumCat | identifier | references | identifier | OA-81-08-353-EN-C | OJ, PUB, CORDIS | search | Catalogue number | | Varfield | 29 | z | 17 | manifestation | identifier (Not mapped in table 3) | IsIdOf - NumCat | identifier | references | identifier | OA-81-08-353-EN-J | OJ, PUB, CORDIS | search | cancelled/invalid Catnum ? | | Varfield | 30 | a | 40 | manifestation | Manifestation identifier | CODEN 6 char. - not used at OP | identifier | references | identifier | N/A | N/A | search | CODEN \"The CODEN is assigned by the International CODEN Section of Chemical Abstracts Service\" | | Varfield | 30 | b | 2 | manifestation | Manifestation identifier | 6 char. - not used at OP | identifier | references | identifier | N/A | N/A | search | | | Varfield | 86 | a | 31 | manifestation | Manifestation identifier | Government Document Classification Number ?? Should not be used | classification | subject | concept | N/A | N/A | search, index | | Varfield | 210 | a | 26 | manifestation | Title of manifestation | hasTitle - abbreviated title - only for serials | title | title | title | Plant prot. bull. (used for Plant protection bulletin) | | search, index | | Varfield | 222 | a | 40 | manifestation | Title of manifestation | hasTitle - only for serials | title | title | title | Der Öffentliche Dienst | | search, index | | | Varfield | 245 | a | 5866 | manifestation | Manifestation - Title | hasTitle - only for serials | title | title | title | Deutsche Bibliographie | | search, index | | | Varfield | 245 | b | 943 | manifestation | Remainder of title of manifestation (Not mapped in table 3) | | subtitle | title | title | Amtsblatt der Deutschen Bibliothek | | search, index | | | Varfield | 245 | h | 589 | manifestation | Manifestation - Form of carrier | hasFormat - medium - always indicated between \\[opoce: \\] | format | format | format_medium | \"ER\" used for (electronic resource) | | identify | | | Varfield | 245 | n | 471 | manifestation | Manifestation - Title | IsPartOf | number_title | title | title | Reihe B | | search, index | | | Varfield | 245 | p | 134 | manifestation | Manifestation - Title | IsPartOf | part_title | title | title | Wöchentliches Verzeichnis | | search, index | | | Varfield | 246 | a | 4591 | manifestation | Manifestation - Title | IsVaryingTitle | varying_title | title | title | \"Four corners power review\" when in 245 field \"4 corners power review\" | | search, index | | | Varfield | 246 | b | 128 | manifestation | Remainder of title of manifestation (Not mapped in table 3) | IsVaryingTitle | subtitle | title | title | | | search | | | Varfield | 246 | h | 94 | manifestation | Manifestation - Form of carrier | hasFormat | format | format | format_medium | \"ER\" used for (electronic resource) | | | | | Varfield | 246 | n | 31 | manifestation | Manifestation - Title | IsPartOf | number_title | title | title | Vol. 1 & 2 rev. | | search, index | | | Varfield | 250 | a | 82 | manifestation | Manifestation - Edition/issue designation | IsPartOf | number_title | title | title | 2nd rev. edition | | identify | | | Varfield | 250 | b | 85 | manifestation / person | Manifestation - Edition/issue designation | isRealizedBy | note | description | description | revised by J.G. Le Mesurier, Repr. with corrections | | identify | | | Varfield | 300 | 3 | 129 | manifestation | Manifestation designation - Material specified | hasFormat | product | type | product | | | ISBD presentation | | Varfield | 300 | a | 6956 | manifestation | Manifestation - Extent of carrier | isAttributeOf | physical description | format | format_extent | xv, 149 p., 15 slides, 1 map | | identify | | | Varfield | 300 | b | 1047 | manifestation | Manifestation - Various | isAttributeOf | physical description | format | format_extent | ill. | col. | | identify | | Varfield | 300 | c | 2710 | manifestation | Manifestation - Dimensions of carrier | isAttributeOf | physical description | format | format_extent | \"A4\" used for 21 x 29,7 cm | CORDIS, PUB | identify | | | Varfield | 300 | d | 579 | manifestation | Finition (Not mapped in table 3) | isAttributeOf | physical description | format | format_extent | \"BR\" used for softcover | | identify | | | Varfield | 300 | e | 19 | manifestation | Accompanying material (Not mapped in table 3) | | product | type | product | 1 atlas, 1 manual | | | | Varfield | 300 | f | 1 | manifestation | Manifestation - Type of component unit | checK if not an error | product | type | product | 1 box | | | | Varfield | 362 | a | 53 | manifestation | Manifestation - Numbering | isAttributeOf | numbering | coverage | format_extent | Vol. 1 (Mar. 1980)- , Ceased with 2 (1964) | | identify | | | Varfield | 440 | a | 539 | manifestation | Manifestation - Series statement / Whole/part | hasTitle | series_title | title | title | Journal of polymer science | | search, index | | | Varfield | 440 | p | 1 | manifestation | Manifestation - Series statement / Whole/part | IsPartOf | part_title | title | title | Polymer symposia | | search, index | | | Varfield | 440 | v | 468 | manifestation | Manifestation - Series statement / Whole/part | IsPartOf | number_title | title | title | no. 39 | | | | | Varfield | 440 | x | 3229 | manifestation | Manifestation - Series statement / Whole/part | isIdOf - ISSN | link | references | relation | 0080-3863 | PUB | | | | Varfield | 500 | 3 | 42 | manifestation | Materials specified (Manifestation designation) | hasFormat | document | references | relation | | | | | | Varfield | 500 | a | 91 | manifestation | General note (Not mapped in table 3) | | note | description | description | | | identify | | | Varfield | 506 | a | 1 | manifestation | Manifest./Item-- Access restrictions | | note | description | description | | | search | | | Varfield | 538 | a | 1 | manifestation | Manifestation - System requirements | | note | description | description | | | identify | | | Varfield | 540 | 3 | 434 | manifestation | Materials specified (Manifestation - Manifestation designation) | hasFormat | document | references | relation | | | | | | Varfield | 540 | a | 1833 | manifestation | Manifest./Item-- Access restrictions | | copyright | rights | rights | | | management | | | Varfield | 540 | b | 1464 | manifestation | Manifest./Item-- Access restrictions | | author_corporate | creator | agent | | | search, index | | | Varfield | 540 | c | 1 | manifestation | Manifest./Item-- Access restrictions | | N/A | N/A | N/A | | | | | | Varfield | 765 | z | 20 | manifestation | Manifestation identifier | hasId - ISBN | link | references | relation | | | | | | Varfield | 772 | t | 11 | manifestation | Supplement Parent Entry (Title of manifestation) | IsSupplementOf - See also varfield \"770\" that provides the inverse \"Has supplement\" - IsSupplementOf | title | title | title | \"research*eu results supplement\" is the supplement to \"research*eu magazine\" - and vice-versa: \"research*eu magazine\" has a supplement \"research*eu magazine\" | | | | Varfield | 773 | q | 938 | Manifestation | Enumeration and first page (Title of manifestation) | isAttributeOf | numbering | coverage | format_extent | No. 63, April 2010, pp. 8-19 | | identify | | | Varfield | 773 | t | 1027 | Manifestation | Title of manifestation | BelongsTo | title | title | title | \"Copenhage, a missed chance?\" in \"research *eu magazine\", No. 63, April 2010, pp. 8-19, cf. ftp://ftp.cordis.europa.eu/pub/news/research-eu/docs/researcheu-supplement26_en.pdf | | search, index | | | Varfield | 775 | e | 591 | manifestation | Language code (Not mapped in table 3) | hasVersion | | | | | | | | Varfield | 775 | t | 591 | manifestation | Title of manifestation | hasVaryingTitle - Other edition entry - link to other manifestations | title | title | title | | | search, index | | | Varfield | 775 | x | 198 | manifestation | Manifestation identifier | hasId - ISSN | link | references | relation | | PUB | | | Varfield | 776 | h | 2 | manifestation | Physical description (Manifestation --(Various) (sic!)) | hasFormat | format | format | format_medium | | | | | Varfield | 776 | t | 3 | manifestation | Title of manifestation - see varfield 245 | Available in other form: (for non-serials) or Issued in other form: (for serials). | | | | | | | | Varfield | 776 | x | 1 | manifestation | Manifestation identifier | hasId - ISSN | link | references | relation | | PUB | | | Varfield | 777 | h | 533 | manifestation | Physical description (Manifestation --(Various) (sic!)) | hasFormat | format | format | format_medium | | | | | Varfield | 777 | t | 533 | manifestation | Issued With Entry (Title of manifestation) | hasRelationTo | title | title | title | | | | | Varfield | 780 | t | 14 | manifestation | Preceding entry (Title of manifestation) | hasVaryingTitle - only for serials | | | | | | | | Varfield | 780 | x | 14 | manifestation | Manifestation identifier | hasId - ISSN | link | references | relation | | PUB | | | Varfield | 785 | t | 10 | manifestation | Succeeding entry (Title of manifestation) | HasVaryingTitle - only for serials | | | | | | | | Varfield | 785 | x | 10 | manifestation | Manifestation identifier | hasId - ISSN | link | references | relation | | PUB | | | Varfield | 787 | t | 20 | manifestation | Title of manifestation | hasRelationTo | title | title | title | Reports of cases before the Court of Justice and the Court of First Instance has a related entry European Court reports. Reports of European Community staff cases | | | | Varfield | 787 | x | 20 | manifestation | Manifestation identifier | hasId - ISSN | link | references | relation | | PUB | | | Varfield | 856 | n | 11 | manifestation | Name of location of host (Manifestation - Source for acquisition) | IsLocated | source | references | relation | | | identify | | Varfield | 856 | q | 630 | manifestation | Format (Manifestation - File characteristics) | hasFormat | format | format | format_extent | 850 Kb | | | | Varfield | 856 | s | 173 | manifestation | File size (Not mapped in table 3) | hasFormat | physical description | format | format_extent | | | | | Varfield | 856 | u | 843 | manifestation | Manifestation identifier | isLocated | URL | URI | identifier | identifier | | | | | Varfield | 880 | a | 5 | manifestation | Other scripts (Not mapped in table 3) | isOtherScript | | | | | | | | Varfield | 44 | c | 231 | manifestation | Place in which this manifestation was published (always eu) | | | | | | | |" ;
        rdfs:label       "General publication" ;
        rdfs:subClassOf  :work ;
        rdfs:subClassOf  [ a                   owl:Restriction ;
                           owl:maxCardinality  "1"^^xsd:nonNegativeInteger ;
                           owl:onProperty      :publication_general_title_part
                         ] ;
        rdfs:subClassOf  [ a                   owl:Restriction ;
                           owl:maxCardinality  "1"^^xsd:nonNegativeInteger ;
                           owl:onProperty      :publication_general_name_meeting
                         ] ;
        rdfs:subClassOf  [ a                   owl:Restriction ;
                           owl:maxCardinality  "1"^^xsd:nonNegativeInteger ;
                           owl:onProperty      :publication_general_date_publication
                         ] .

:case-law_affaire_year
        a                   owl:DatatypeProperty ;
        rdfs:comment        "Year of the affaire" ;
        rdfs:domain         :case-law ;
        rdfs:label          "Affaire: Year" ;
        rdfs:range          xsd:gYear ;
        rdfs:subPropertyOf  :affaire_year .

:type_court-report  a        owl:Class ;
        rdfs:comment         "Values currently used in the Court schema: RG1, RG2, SC Traced in MDR-1940" ;
        rdfs:label           "Concept representing the types of court reports" ;
        rdfs:subClassOf      skos:Concept , :concept_decoding ;
        owl:equivalentClass  [ a               owl:Restriction ;
                               owl:hasValue    <http://publications.europa.eu/resource/authority/court-report> ;
                               owl:onProperty  skos:inScheme
                             ] .

:expression_embargo  a      owl:DatatypeProperty ;
        rdfs:comment        "Is this expression under embargo? This instance must not be shown until the indicated datetime has been reached. In case a release date is not known,9999-12-31 should be used (= absolute embargo)" ;
        rdfs:domain         :expression ;
        rdfs:label          "Expression embargo" ;
        rdfs:range          xsd:dateTime ;
        rdfs:subPropertyOf  :embargo .

:transliterated_country
        a           owl:DatatypeProperty ;
        rdfs:label  "Transliterated country" .

<http://publications.europa.eu/resource/authority/com_internal_event>
        a       owl:NamedIndividual .

:resource_legal_annulment_requested_by_communication_case_new
        a              owl:ObjectProperty ;
        rdfs:domain    :resource_legal ;
        rdfs:label     "Resource legal annulment requested by communication case new" ;
        rdfs:range     :communication_case_new ;
        owl:inverseOf  :communication_case_new_requests_annulment_of_resource_legal .

:case-law_national_based_on_resource_legal
        a                   owl:ObjectProperty ;
        rdfs:comment        "Possible values: Brussels Convention → 41968A0927(01), Lugano Convention → 22009A0610(01), Brussels I regulation → 32001R0044, Brussels II regulation → 32000R1347, New Brussels II regulation → 32003R2201" ;
        rdfs:domain         :case-law_national ;
        rdfs:label          "Case law based on a legal instrument" ;
        rdfs:range          :resource_legal ;
        rdfs:subPropertyOf  :based_on ;
        owl:inverseOf       :resource_legal_basis_for_case-law_national .

:event_mandatorily-addresses_institution
        a                   owl:ObjectProperty ;
        rdfs:comment        "This event mandatorily addresses a given institution. Corresponds to role type ADDRESSEE_MANDATORY" ;
        rdfs:domain         :event ;
        rdfs:label          "event mandatorily addresses institution" ;
        rdfs:range          :institution ;
        rdfs:subPropertyOf  :mandatorily-addresses ;
        owl:deprecated      true ;
        owl:inverseOf       :institution_addressed_by_event .

:application_suspended_by
        a           owl:ObjectProperty ;
        rdfs:label  "Application suspended by" .

:has_conclusions  a  owl:ObjectProperty ;
        rdfs:label  "Has conclusions" .

:container_case-law_section
        a                   owl:DatatypeProperty ;
        rdfs:domain         :container_case-law ;
        rdfs:label          "Section of case law publication" ;
        rdfs:range          xsd:positiveInteger ;
        rdfs:subPropertyOf  :section .

:eu_survey_identifier
        a           owl:DatatypeProperty ;
        rdfs:label  "Eu survey identifier" .

<http://publications.europa.eu/resource/authority/fd_030>
        a       owl:NamedIndividual .

:dossier_part_of_dossier
        a                   owl:ObjectProperty ;
        rdfs:comment        "This dossier is part of another dossier" ;
        rdfs:domain         :dossier ;
        rdfs:label          "Dossier part of dossier" ;
        rdfs:range          :dossier ;
        rdfs:subPropertyOf  :part_of .

:procurement_public_labels_forms_link_title
        a                   owl:DatatypeProperty ;
        rdfs:domain         :procurement_public ;
        rdfs:label          "Labels forms title" ;
        rdfs:range          xsd:string ;
        rdfs:subPropertyOf  :labels_forms_link_title .

:case_court_domain  a       owl:DatatypeProperty ;
        rdfs:comment        "This case is about a given domain, e.g. Energie or Agriculture, expressed as a string" ;
        rdfs:domain         :case_court ;
        rdfs:label          "Domain of the court case" ;
        rdfs:range          xsd:string ;
        rdfs:subPropertyOf  :domain .

:documents  a       owl:ObjectProperty ;
        rdfs:label  "Documents" .

:resource_legal_contains_eesc_opinion_on_resource_legal
        a                   owl:ObjectProperty ;
        rdfs:comment        "This points to proposal on which EESC provides its opinion. Relevant for legal analysis: true" ;
        rdfs:domain         :resource_legal ;
        rdfs:label          "Legal resource contains Economic and Social Committee opinion on legal resource" ;
        rdfs:range          :resource_legal ;
        rdfs:subPropertyOf  :contains_eesc_opinion_on ;
        owl:inverseOf       :resource_legal_eesc_opinion_contained_in_resource_legal .

:decision_ecsc  a        owl:Class ;
        rdfs:comment     "European Coal and Steel Community (ECSC) decisions of general interest (subsector S of sector 3). At present 589 notices. Examples: 31960S0022, 31962S0719, 31952S0004, 32001S2443" ;
        rdfs:label       "ECSC decision" ;
        rdfs:subClassOf  :legislation_secondary .

:partially_annuls  a  owl:ObjectProperty ;
        rdfs:label  "Partially annuls" .

:link-package  a         owl:Class ;
        rdfs:comment     "A dossier acting as a grouping of arbitrarily assigned documents (works)" ;
        rdfs:label       "Link package" ;
        rdfs:subClassOf  :dossier .

:resource_legal_does_renumbering_of_resource_legal
        a                   owl:ObjectProperty ;
        rdfs:comment        "Legal resources does renumbering a legal resource, in term of consolidation" ;
        rdfs:domain         :resource_legal ;
        rdfs:label          "Legal resources does renumbering of legal resource" ;
        rdfs:range          :resource_legal ;
        rdfs:subPropertyOf  :does_renumbering_of .

:resource_legal_eesc_opinion_contained_in_resource_legal
        a                   owl:ObjectProperty ;
        rdfs:comment        "4603 cases (2010-07-27). Relevant for legal analysis: true." ;
        rdfs:domain         :resource_legal ;
        rdfs:label          "Economic and Social Committee opinion on legal resource contained in legal resource" ;
        rdfs:range          :resource_legal ;
        rdfs:subPropertyOf  :eesc_opinion_contained_in ;
        owl:inverseOf       :resource_legal_contains_eesc_opinion_on_resource_legal .

:has_frequency  a   owl:ObjectProperty ;
        rdfs:label  "Has frequency" .

:transliterated_address
        a           owl:DatatypeProperty ;
        rdfs:label  "Transliterated address" .

:case-law_delivered_by_judge
        a                   owl:ObjectProperty ;
        rdfs:comment        "Name of the Judge-Rapporteur for the case. Currently coded with FD_Table 130." ;
        rdfs:domain         :case-law ;
        rdfs:label          "Case law delivered by judge" ;
        rdfs:range          :judge ;
        rdfs:subPropertyOf  :delivered_by ;
        owl:inverseOf       :judge_delivers_case-law .

:resource_legal_basis_for_case-law_national
        a              owl:ObjectProperty ;
        rdfs:domain    :resource_legal ;
        rdfs:label     "Resource legal basis for case law national" ;
        rdfs:range     :case-law_national ;
        owl:inverseOf  :case-law_national_based_on_resource_legal .

:case-law_subject_to_appeal_in_case_court
        a                   owl:ObjectProperty ;
        rdfs:comment        "The case law subject to appeal in a new court case" ;
        rdfs:domain         :case-law ;
        rdfs:label          "Case law subject to appeal in a new court case" ;
        rdfs:range          :case_court ;
        rdfs:subPropertyOf  :subject_to_appeal_in ;
        owl:inverseOf       :case_court_subject_to_appeal_in_case-law .

:manifestation_reproduction_of_manifestation
        a                   owl:ObjectProperty ;
        rdfs:comment        "manifestation used as the basis for a reproduction. Reciprocal relationship: reproduced as (after RDA J.4.2.)" ;
        rdfs:domain         :manifestation ;
        rdfs:label          "Manifestation reproduction of manifestation" ;
        rdfs:range          :manifestation ;
        rdfs:subPropertyOf  :reproduction_of .

:related_question_to  a  owl:ObjectProperty ;
        rdfs:label  "Related question to" .

:expression_version  a      owl:DatatypeProperty ;
        rdfs:comment        "Freeform information on the version of this expression" ;
        rdfs:domain         :expression ;
        rdfs:label          "Expression version" ;
        rdfs:range          xsd:string ;
        rdfs:subPropertyOf  :version .

:roadmap_needed  a  owl:DatatypeProperty ;
        rdfs:label  "Roadmap needed" .

:signs  a           owl:ObjectProperty ;
        rdfs:label  "Signs" .

:resource_legal_completes_resource_legal
        a                   owl:ObjectProperty ;
        rdfs:comment        "This property points to act which provision(s) are completed. Relevant for legal analysis: true" ;
        rdfs:domain         :resource_legal ;
        rdfs:label          "Legal resource completes legal resource" ;
        rdfs:range          :resource_legal ;
        rdfs:subPropertyOf  :completes ;
        owl:inverseOf       :resource_legal_completed_by_resource_legal .

:event_based_on_resource_legal
        a                   owl:ObjectProperty ;
        rdfs:comment        "Relevant for legal analysis: true. This event is based on a legal resource (typically a treaty article, but could also be secondary legislation). Relevant for legal analysis: true" ;
        rdfs:domain         :event ;
        rdfs:label          "Event based on legal resource" ;
        rdfs:range          :resource_legal ;
        rdfs:subPropertyOf  :based_on ;
        owl:inverseOf       :resource_legal_basis_for_event .

:resource_legal_referred_to_by_agent
        a                   owl:ObjectProperty ;
        rdfs:comment        "corext:author_referral, is often provided in combination with corext:date_referral. In this case this date of referral is stored in the annotation property \"date\"" ;
        rdfs:domain         :resource_legal ;
        rdfs:label          "Legal resource referred to by agent" ;
        rdfs:range          :agent ;
        rdfs:subPropertyOf  :referred_to_by .

:consulted_by  a    owl:ObjectProperty ;
        rdfs:label  "Consulted by" .

:official-journal_class
        a                   owl:DatatypeProperty ;
        rdfs:comment        "OJ class \"R\" / \"A\" / \"E\" / \"M\"/ \"I\". Distinction between the issues: the regular (R), the CE (E), the CA (A), Malte but also Gaïlique edition (M) and Urgent edition (I)" ;
        rdfs:domain         :official-journal ;
        rdfs:label          "Class of OJ" ;
        rdfs:range          xsd:string ;
        rdfs:subPropertyOf  :class .

:confirms  a        owl:ObjectProperty ;
        rdfs:label  "Confirms" .

:resource_legal_implemented_by_resource_legal
        a                   owl:ObjectProperty ;
        rdfs:comment        "Relevant for legal analysis: true." ;
        rdfs:domain         :resource_legal ;
        rdfs:label          "Legal resource implemented_by legal resource" ;
        rdfs:range          :resource_legal ;
        rdfs:subPropertyOf  :implemented_by ;
        owl:inverseOf       :resource_legal_implements_resource_legal .

:added_to  a        owl:ObjectProperty ;
        rdfs:label  "Added to" .

:procurement_public_originates_in_concept_ntu
        a                   owl:ObjectProperty ;
        rdfs:domain         :procurement_public ;
        rdfs:label          "Public procurement originates in territorial unit (expressed as NTU concept)" ;
        rdfs:range          :concept_ntu ;
        rdfs:subPropertyOf  :originates_in .

:case-law_national_decision_internal_identifier
        a                   owl:DatatypeProperty ;
        rdfs:comment        "Internal identifier from the Court for the national decisions. limited to sector 8" ;
        rdfs:domain         :case-law_national ;
        rdfs:label          "Internal identifier" ;
        rdfs:range          xsd:string ;
        rdfs:subPropertyOf  :decision_internal_identifier .

:submits_preliminary_question
        a           owl:ObjectProperty ;
        rdfs:label  "Submits preliminary question" .

:european_union_competence_type
        a           owl:DatatypeProperty ;
        rdfs:label  "European union competence type" .

:decision_service_responsible
        a                   owl:DatatypeProperty ;
        rdfs:comment        "The Commission DG or DGs responsible for drafting of an act. Relevant for legal analysis: true. DEPRECATED. In the instance data, the property is planned to be replaced with cdm:resource_legal_service_responsible at beginning 2019. When this is done this property will be removed from CDM. The Commission's DG that brought forward the proposal; to be taken from a closed list of DGs (that might be derived from the RECORD project ?). For the backlog data need to be completed. Cardinality to be restricted to 1 in the future." ;
        rdfs:domain         :decision ;
        rdfs:label          "Service responsible" ;
        rdfs:range          xsd:string ;
        rdfs:subPropertyOf  :service_responsible , :resource_legal_service_responsible ;
        owl:deprecated      true .

:resource_legal  a       owl:Class ;
        rdfs:comment     "Resources created for legal and legislative purposes. Remarks: * All relationships resource_legal_XXX_resource_legal can be seen as sub-properties of a general property \"affects\" * The role of linking tables and the VOLET_JUR_LNK are more fully explained below in relation to the link target class. * EV_VV field is not used in practice * Elements VOLET_JUR/PP, PP_PP, PP_TYPE, PP_ORGANE, PP_COMMENT to be integrated in general Prelex model * \"Legal resource belongs to legislative procedure\" should not be restricted to secondary legislation as acts other than secondary legislation may belong to legislative procedures. * In VOLET_JUR_LNK, LNK_PLACE_P might be decoded with fd_370, ROLE_2 with fd_375." ;
        rdfs:label       "Legal resource" ;
        rdfs:subClassOf  :work ;
        rdfs:subClassOf  [ a                   owl:Restriction ;
                           owl:maxCardinality  "1"^^xsd:nonNegativeInteger ;
                           owl:onProperty      :resource_legal_number_natural_celex
                         ] ;
        rdfs:subClassOf  [ a                   owl:Restriction ;
                           owl:maxCardinality  "1"^^xsd:nonNegativeInteger ;
                           owl:onProperty      :resource_legal_reference_oj-act
                         ] ;
        rdfs:subClassOf  [ a                   owl:Restriction ;
                           owl:maxCardinality  "1"^^xsd:nonNegativeInteger ;
                           owl:onProperty      :resource_legal_date_start_handling
                         ] ;
        rdfs:subClassOf  [ a                   owl:Restriction ;
                           owl:maxCardinality  "1"^^xsd:nonNegativeInteger ;
                           owl:onProperty      :resource_legal_repertoire
                         ] ;
        rdfs:subClassOf  [ a                   owl:Restriction ;
                           owl:maxCardinality  "1"^^xsd:nonNegativeInteger ;
                           owl:onProperty      :resource_legal_number_natural
                         ] ;
        rdfs:subClassOf  [ a                   owl:Restriction ;
                           owl:maxCardinality  "1"^^xsd:nonNegativeInteger ;
                           owl:onProperty      :resource_legal_date_request_caducity
                         ] ;
        rdfs:subClassOf  [ a                   owl:Restriction ;
                           owl:maxCardinality  "1"^^xsd:nonNegativeInteger ;
                           owl:onProperty      :resource_legal_number_corrigendum_eli
                         ] ;
        rdfs:subClassOf  [ a                   owl:Restriction ;
                           owl:maxCardinality  "1"^^xsd:nonNegativeInteger ;
                           owl:onProperty      :resource_legal_date_vote
                         ] ;
        rdfs:subClassOf  [ a                   owl:Restriction ;
                           owl:maxCardinality  "1"^^xsd:nonNegativeInteger ;
                           owl:onProperty      :resource_legal_id_sector
                         ] ;
        rdfs:subClassOf  [ a                   owl:Restriction ;
                           owl:maxCardinality  "1"^^xsd:nonNegativeInteger ;
                           owl:onProperty      :resource_legal_number_sequence_celex
                         ] ;
        rdfs:subClassOf  [ a                   owl:Restriction ;
                           owl:maxCardinality  "1"^^xsd:nonNegativeInteger ;
                           owl:onProperty      :resource_legal_internal_number_sequential_number
                         ] ;
        rdfs:subClassOf  [ a                   owl:Restriction ;
                           owl:maxCardinality  "1"^^xsd:nonNegativeInteger ;
                           owl:onProperty      :resource_legal_internal_number_prefix
                         ] ;
        rdfs:subClassOf  [ a                   owl:Restriction ;
                           owl:maxCardinality  "1"^^xsd:nonNegativeInteger ;
                           owl:onProperty      :resource_legal_basis_referral
                         ] ;
        rdfs:subClassOf  [ a                   owl:Restriction ;
                           owl:maxCardinality  "1"^^xsd:nonNegativeInteger ;
                           owl:onProperty      :resource_legal_number_sequence
                         ] ;
        rdfs:subClassOf  [ a                   owl:Restriction ;
                           owl:maxCardinality  "1"^^xsd:nonNegativeInteger ;
                           owl:onProperty      :resource_legal_number_corrigendum
                         ] ;
        rdfs:subClassOf  [ a                   owl:Restriction ;
                           owl:maxCardinality  "1"^^xsd:nonNegativeInteger ;
                           owl:onProperty      :resource_legal_internal_number_suffix
                         ] ;
        rdfs:subClassOf  [ a                   owl:Restriction ;
                           owl:maxCardinality  "1"^^xsd:nonNegativeInteger ;
                           owl:onProperty      :resource_legal_term-of-office
                         ] ;
        rdfs:subClassOf  [ a                   owl:Restriction ;
                           owl:maxCardinality  "1"^^xsd:nonNegativeInteger ;
                           owl:onProperty      :resource_legal_in-force
                         ] .

:manifestation_case-law_endorsements
        a                   owl:DatatypeProperty ;
        rdfs:comment        "Endorsements associated with this judgement. Sector 6 Text Index Field VS" ;
        rdfs:domain         :manifestation_case-law ;
        rdfs:label          "Endorsements in court decision" ;
        rdfs:range          rdf:XMLLiteral ;
        rdfs:subPropertyOf  :endorsements .

:issn   a           owl:DatatypeProperty ;
        rdfs:label  "Issn" .

:event_legal_associated_with_person
        a                   owl:ObjectProperty ;
        rdfs:comment        "Relevant for legal analysis: true. This legal event is associated with a given person. Body role:Associated. Relevant for legal analysis: true" ;
        rdfs:domain         :event_legal ;
        rdfs:label          "Legal event associated with person" ;
        rdfs:range          :person ;
        rdfs:subPropertyOf  :event_associated_with_person , :associated_with ;
        owl:deprecated      true ;
        owl:inverseOf       :person_associated_with_event_legal .

:reference-data_asset_prerelease_based_on_reference-data_asset_release
        a                   owl:ObjectProperty ;
        rdfs:comment        "This predicate describes the relation between an official/stable reference data asset version as derivation basis for a prerelease version." ;
        rdfs:domain         :reference-data_asset_prerelease ;
        rdfs:label          "Reference data asset prerelease based on reference data asset release" ;
        rdfs:range          :reference-data_asset_release ;
        rdfs:subPropertyOf  :based_on ;
        owl:inverseOf       :reference-data_asset_release_basis_for_reference-data_asset_prerelease .

:joint-assessment_impact_summary
        a                owl:Class ;
        rdfs:label       "Summary of Joint Impact Assessment" ;
        rdfs:subClassOf  :joint-staff-working-document .

:reference-data_asset_release_published_in_reference-data_publication
        a              owl:ObjectProperty ;
        rdfs:comment   " " ;
        rdfs:domain    :reference-data_asset_release ;
        rdfs:label     "reference data asset release published in reference data publication" ;
        rdfs:range     :reference-data_publication ;
        owl:inverseOf  :reference-data_publication_publishes_reference-data_asset_release .

:delivers  a        owl:ObjectProperty ;
        rdfs:label  "Delivers" .

:glossary  a             owl:Class ;
        rdfs:comment     "\"A list of terms associated with definition texts (‘glosses’)\" (TEI 4.7) Add notes, bibliogr., index, colophon if needed at a later stage" ;
        rdfs:label       "Glossary" ;
        rdfs:subClassOf  :back .

:concept_agenda_council
        a                    owl:Class ;
        rdfs:label           "Concept representing the council agenda in Prelex" ;
        rdfs:subClassOf      skos:Concept , :concept_decoding ;
        owl:equivalentClass  [ a               owl:Restriction ;
                               owl:hasValue    <http://publications.europa.eu/resource/authority/fd_600> ;
                               owl:onProperty  skos:inScheme
                             ] .

:manifestation_print_volume
        a                   owl:DatatypeProperty ;
        rdfs:comment        "Volume of the publication. e.g. for DEBAT_PUB_NO or other indication of volumes" ;
        rdfs:domain         :manifestation_print ;
        rdfs:label          "Volume of the print manifestation" ;
        rdfs:range          xsd:string ;
        rdfs:subPropertyOf  :volume .

:official-journal-act_section_oj
        a                   owl:DatatypeProperty ;
        rdfs:comment        "Section heading (level 1) under which an Official Journal act is published." ;
        rdfs:domain         :official-journal-act ;
        rdfs:label          "Official Journal act section oj" ;
        rdfs:range          xsd:string ;
        rdfs:subPropertyOf  :section_oj .

:act_preparatory_ec  a   owl:Class ;
        rdfs:comment     "Preparatory act by the European Commission. A common superclass for all documents of the European Commission emerging from the preparatory work in legislative and non-legislative procedures. All documents from that hierarchy have the European Commission or one of their subentities as author." ;
        rdfs:label       "Preparatory act by EC" ;
        rdfs:subClassOf  :act_preparatory ;
        rdfs:subClassOf  [ a               owl:Restriction ;
                           owl:hasValue    <http://publications.europa.eu/resource/authority/corporate-body/COM> ;
                           owl:onProperty  :work_created_by_agent
                         ] ;
        dct:created      "2022-09-01T09:01:22"^^xsd:dateTime .

:expression_source  a       owl:DatatypeProperty ;
        rdfs:comment        "Freeform source information on this expression. maps e.g. from oibext:reference_volume" ;
        rdfs:domain         :expression ;
        rdfs:label          "Source of expression" ;
        rdfs:range          xsd:string ;
        rdfs:subPropertyOf  :source .

:agent_requests_case-law
        a                   owl:ObjectProperty ;
        rdfs:comment        "Agent requests a judgement. AP" ;
        rdfs:domain         :agent ;
        rdfs:label          "Agent requests case law" ;
        rdfs:range          :case-law ;
        rdfs:subPropertyOf  :requests ;
        owl:inverseOf       :case-law_requested_by_agent .

:resource_legal_produced_by_dossier
        a                   owl:ObjectProperty ;
        rdfs:comment        "The legal resource is the result of a dossier. Never directly specified, inverse property. Relevant for legal analysis: true" ;
        rdfs:domain         :resource_legal ;
        rdfs:label          "Legal resource is produced by a dossier" ;
        rdfs:range          :dossier ;
        rdfs:subPropertyOf  :produced_by ;
        owl:inverseOf       :dossier_produces_resource_legal .

:manifestation_case-law_parties
        a                   owl:DatatypeProperty ;
        rdfs:comment        "Parties associated with this judgement. Sector 6 Text Index Field I1" ;
        rdfs:domain         :manifestation_case-law ;
        rdfs:label          "Parties of court decision" ;
        rdfs:range          rdf:XMLLiteral ;
        rdfs:subPropertyOf  :parties .

:event_embargo  a           owl:DatatypeProperty ;
        rdfs:comment        "Is this event under embargo? This instance must not be shown until the indicated datetime has been reached. In case a release date is not known,9999-12-31 should be used (= absolute embargo)" ;
        rdfs:domain         :event ;
        rdfs:label          "Event embargo" ;
        rdfs:range          xsd:dateTime ;
        rdfs:subPropertyOf  :embargo .

:source-pool  a     owl:DatatypeProperty ;
        rdfs:label  "Source pool" .

<http://publications.europa.eu/resource/authority/fd_396>
        a       owl:NamedIndividual .

:framework_procedural_has_nature
        a           owl:ObjectProperty ;
        rdfs:label  "Framework procedural has nature" .

:originates_in  a   owl:ObjectProperty ;
        rdfs:label  "Originates in" .

:transliterated_organisation_official-name
        a           owl:DatatypeProperty ;
        rdfs:label  "Transliterated organisation official name" .

:procurement_public_range_maximal
        a                   owl:DatatypeProperty ;
        rdfs:domain         :procurement_public ;
        rdfs:label          "Maximimal value of a range" ;
        rdfs:range          xsd:decimal ;
        rdfs:subPropertyOf  :range_maximal .

:event_formally-addresses_institution
        a                   owl:ObjectProperty ;
        rdfs:comment        "Relevant for legal analysis: true. This event formally addresses a given institution. Examples include the transmission of a COM from the Commission to Council. Relevant for legal analysis: true" ;
        rdfs:domain         :event ;
        rdfs:label          "Event formally addresses institution" ;
        rdfs:range          :institution ;
        rdfs:subPropertyOf  :formally-addresses ;
        owl:inverseOf       :institution_formally-addressed_by_event .

:event_legal_uses_concept_mode_decision
        a                   owl:ObjectProperty ;
        rdfs:comment        "Change from the mode_decision data property, encoded via FD_606. Decision mode. Relevant for legal analysis: true." ;
        rdfs:domain         :event_legal ;
        rdfs:label          "The event operates under a given decision mode" ;
        rdfs:range          :concept_mode_decision ;
        rdfs:subPropertyOf  :uses .

:id     a                   owl:DatatypeProperty ;
        rdfs:label          "Id" ;
        rdfs:subPropertyOf  :identifier .

:event_responsibility_of_person
        a                   owl:ObjectProperty ;
        rdfs:comment        "Relevant for legal analysis: true. This event is under responsibility of a given person. Relevant for legal analysis: true" ;
        rdfs:domain         :event ;
        rdfs:label          "Event under responsibility of person" ;
        rdfs:range          :person ;
        rdfs:subPropertyOf  :responsibility_of ;
        owl:inverseOf       :person_responsible_for_event .

:official-journal-act_durability
        a                   owl:DatatypeProperty ;
        rdfs:comment        "Durability of a legal resource published as Official Journal act" ;
        rdfs:domain         :official-journal-act ;
        rdfs:label          "Official Journal act durability" ;
        rdfs:range          xsd:string ;
        rdfs:subPropertyOf  :durability .

:country_role-qualifier
        a                    owl:Class ;
        rdfs:label           "Country role qualifier" ;
        rdfs:subClassOf      skos:Concept ;
        owl:disjointUnionOf  ( :country :role-qualifier ) .

:procurement_public_transliterated_fax
        a                   owl:DatatypeProperty ;
        rdfs:domain         :procurement_public ;
        rdfs:label          "Procurement public transliterated fax" ;
        rdfs:range          xsd:string ;
        rdfs:subPropertyOf  :transliterated_fax .

:manifestation_official-journal_part_natural_number
        a                   owl:DatatypeProperty ;
        rdfs:comment        "Natural number of the act (as seen by the printer). values such as 36, 127,..." ;
        rdfs:domain         :manifestation_official-journal_part ;
        rdfs:label          "Natural number of the act (decomposed)" ;
        rdfs:range          xsd:string ;
        rdfs:subPropertyOf  :natural_number .

:archive_package_contains_archive_package_document
        a                   owl:ObjectProperty ;
        rdfs:comment        "An archive package can contain a list of digitised documents which as such are not separately digitised. This relation characterises an included work as part of an archive package and offers the possibility to specify by an owl:Axiom the sequence of the included documents." ;
        rdfs:domain         :archive_package ;
        rdfs:label          "Archive package contains archive package document" ;
        rdfs:range          :archive_package_document ;
        rdfs:subPropertyOf  :work_contains_work ;
        owl:inverseOf       :archive_package_document_part_of_archive_package .

<http://publications.europa.eu/resource/authority/fd_375>
        a       owl:NamedIndividual .

:green-paper_joint  a    owl:Class ;
        rdfs:label       "Joint Green Paper" ;
        rdfs:subClassOf  :act_preparatory_joint .

:dossier_produces_resource_legal
        a                   owl:ObjectProperty ;
        rdfs:comment        "Relevant for legal analysis: true. This dossier results in a legal resource in force at the end of the process. This implies the URL (dossier/details/community_legislation_in_force_url which belongs to the manifestation of the legislation in force. Relevant for legal analysis: true" ;
        rdfs:domain         :dossier ;
        rdfs:label          "Dossier produces legal resource" ;
        rdfs:range          :resource_legal ;
        rdfs:subPropertyOf  :produces ;
        owl:inverseOf       :resource_legal_produced_by_dossier .

:resource_legal_partially_suspended_by_resource_legal
        a                   owl:ObjectProperty ;
        rdfs:comment        "Calculated. Relevant for legal analysis: true." ;
        rdfs:domain         :resource_legal ;
        rdfs:label          "Legal resource partially suspended by legal resource" ;
        rdfs:range          :resource_legal ;
        rdfs:subPropertyOf  :partially_suspended_by ;
        owl:inverseOf       :resource_legal_partially_suspends_resource_legal .

:manifestation_special-court-report_part_year
        a                   owl:DatatypeProperty ;
        rdfs:comment        "Year in which this special court report was published. Temporary solution, should in the future be part of the court report object itself" ;
        rdfs:domain         :manifestation_special-court-report_part ;
        rdfs:label          "Year of special court report" ;
        rdfs:range          xsd:string ;
        rdfs:subPropertyOf  :year .

:opinion_other_eesc  a   owl:Class ;
        rdfs:comment     "European Economic and Social Committee other opinions, usually own-initiative (celex 5IE)" ;
        rdfs:label       "European Economic and Social Committee other opinion" ;
        rdfs:subClassOf  :act_preparatory_eesc ;
        rdfs:subClassOf  [ a                   owl:Restriction ;
                           owl:maxCardinality  "1"^^xsd:nonNegativeInteger ;
                           owl:onProperty      :opinion_other_eesc_number_session
                         ] .

:resource_legal_suspended_by_resource_legal
        a                   owl:ObjectProperty ;
        rdfs:comment        "Calculated. Relevant for legal analysis: true." ;
        rdfs:domain         :resource_legal ;
        rdfs:label          "Legal resource suspended by legal resource" ;
        rdfs:range          :resource_legal ;
        rdfs:subPropertyOf  :suspended_by ;
        owl:inverseOf       :resource_legal_suspends_resource_legal .

:measure_national_implementing_type_act
        a                   owl:DatatypeProperty ;
        rdfs:comment        "Type of act in the national system. e.g. Acte juridique: Règlement" ;
        rdfs:domain         :measure_national_implementing ;
        rdfs:label          "Act type" ;
        rdfs:range          xsd:string ;
        rdfs:subPropertyOf  :type_act .

:agent_related_to_work
        a              owl:ObjectProperty ;
        rdfs:comment   "This generic relation relates the agents to the work, in considering all possible ROLES of the agent (person, institution, ...), which does a work (any type of works)" ;
        rdfs:domain    :agent ;
        rdfs:label     "Agent related to work" ;
        rdfs:range     :work ;
        owl:inverseOf  :work_related_with_agent .

:dossier_withdrawn-proposal
        a                   owl:DatatypeProperty ;
        rdfs:comment        "Relevant for legal analysis: true. Withdrawn proposal. Relevant for legal analysis: true" ;
        rdfs:domain         :dossier ;
        rdfs:label          "Dossier is already withdrawn?" ;
        rdfs:range          xsd:boolean ;
        rdfs:subPropertyOf  :withdrawn-proposal .

:date   a             owl:DatatypeProperty ;
        rdfs:comment  "Any type of date (inferred superproperty of all dates)" ;
        rdfs:label    "Date" ;
        rdfs:range    xsd:date .

:ATTO_FD_365  a              owl:Class ;
        rdfs:label           "FD_365 ATTO table" ;
        rdfs:subClassOf      skos:Concept ;
        owl:equivalentClass  [ a               owl:Restriction ;
                               owl:hasValue    <http://publications.europa.eu/resource/authority/fd_365> ;
                               owl:onProperty  skos:inScheme
                             ] .

:repertoire  a      owl:DatatypeProperty ;
        rdfs:label  "Repertoire" .

:framework_procedural_identifier
        a           owl:DatatypeProperty ;
        rdfs:label  "Framework procedural identifier" .

:joint-proposal_regulation
        a                owl:Class ;
        rdfs:comment     "where its resource_legal_type = JC, resource_legal_id_sector = 5, work_has_resource-type = JOINT_PROP_REG" ;
        rdfs:label       "Joint proposal for a regulation" ;
        rdfs:subClassOf  :proposal_act , :act_preparatory_joint .

:non-opposition_joint-venture_notified_service_responsible
        a                   owl:DatatypeProperty ;
        rdfs:comment        "The Commission DG or DGs responsible for drafting of an act. Relevant for legal analysis: true\" DEPRECATED. In the instance data, the property is planned to be replaced with cdm:resource_legal_service_responsible at beginning 2019. When this is done this property will be removed from CDM. The Commission's DG that brought forward the proposal; to be taken from a closed list of DGs (that might be derived from the RECORD project ?). For the backlog data need to be completed. Cardinality to be restricted to 1 in the future." ;
        rdfs:domain         :non-opposition_joint-venture_notified ;
        rdfs:label          "Service responsible" ;
        rdfs:range          xsd:string ;
        rdfs:subPropertyOf  :service_responsible , :resource_legal_service_responsible ;
        owl:deprecated      true .

:resource_legal_based_on_concept_treaty
        a                   owl:ObjectProperty ;
        rdfs:comment        "Name of the treaty/treaties that form the legal basis under which the document has been adopted. This field is linked to NAL treaty; no CELEX numbers are used. Relevant for legal analysis: true" ;
        rdfs:domain         :resource_legal ;
        rdfs:label          "Legal resource based on treaty concept" ;
        rdfs:range          :concept_treaty ;
        rdfs:subPropertyOf  :based_on ;
        owl:inverseOf       :concept_treaty_basis_for_resource_legal .

:special-official-journal
        a                owl:Class ;
        rdfs:comment     "Special Edition of the Official Journal used to complement existing OJ issues upon accession of a memberstate candidate bringing in a new lingustic version." ;
        rdfs:label       "Special Edition" ;
        rdfs:subClassOf  :publication_general ;
        rdfs:subClassOf  [ a                owl:Restriction ;
                           owl:cardinality  "1"^^xsd:nonNegativeInteger ;
                           owl:onProperty   :special-official-journal_volume
                         ] ;
        rdfs:subClassOf  [ a                   owl:Restriction ;
                           owl:maxCardinality  "1"^^xsd:nonNegativeInteger ;
                           owl:onProperty      :special-official-journal_second_series_historical
                         ] ;
        rdfs:subClassOf  [ a                   owl:Restriction ;
                           owl:maxCardinality  "1"^^xsd:nonNegativeInteger ;
                           owl:onProperty      :special-official-journal_legal_effect_paper
                         ] ;
        rdfs:subClassOf  [ a                   owl:Restriction ;
                           owl:maxCardinality  "1"^^xsd:nonNegativeInteger ;
                           owl:onProperty      :special-official-journal_first_series_historical
                         ] .

:resource_legal_basis_for_act_consolidated
        a                   owl:ObjectProperty ;
        rdfs:comment        "This legal resource is the base act for a consolidation" ;
        rdfs:domain         :resource_legal ;
        rdfs:label          "Legal resources basis for a consolidated act" ;
        rdfs:range          :act_consolidated ;
        rdfs:subPropertyOf  :basis_for ;
        owl:inverseOf       :act_consolidated_based_on_resource_legal .

:responsibility_of  a  owl:ObjectProperty ;
        rdfs:label  "Responsibility of" .

:expression_subtitle  a     owl:DatatypeProperty ;
        rdfs:comment        "Relevant for legal analysis: true. Subtitle of the expression. Relevant for legal analysis: true" ;
        rdfs:domain         :expression ;
        rdfs:label          "Expression Subtitle" ;
        rdfs:range          rdfs:Literal ;
        rdfs:subPropertyOf  :subtitle .

:directive_name  a  owl:DatatypeProperty ;
        rdfs:label  "Directive name" .

:manifestation_official-journal_part_page_first
        a                   owl:DatatypeProperty ;
        rdfs:comment        "DEPRECATED, First page number of the OJ part related to a legal resource. Use manifestion_print_page_first" ;
        rdfs:domain         :manifestation_official-journal_part ;
        rdfs:label          "First page" ;
        rdfs:range          xsd:string ;
        rdfs:subPropertyOf  :page_first , :manifestation_print_page_first ;
        owl:deprecated      true .

:date_start  a      owl:DatatypeProperty ;
        rdfs:label  "Date start" .

:uses_procedure  a  owl:ObjectProperty ;
        rdfs:label  "Uses procedure" .

:case-law_national_act_reference_european
        a                   owl:DatatypeProperty ;
        rdfs:comment        "Reference to an European act in free text, e.g. Richtlinie 88/361/EWG des Rates vom 24. Juni 1988. VOLET_JUR_NAT/SUIVI is mapped on the element abstract of the corresponding expression" ;
        rdfs:domain         :case-law_national ;
        rdfs:label          "Reference to a European act in free text" ;
        rdfs:range          xsd:string ;
        rdfs:subPropertyOf  :act_reference_european .

:event_related_with_agent
        a                   owl:ObjectProperty ;
        rdfs:comment        "This generic relation relates the event to the agent, in considering all possible ROLES of the agent (person, institution, ...), which does an event (all type of events)" ;
        rdfs:domain         :event ;
        rdfs:label          "Event related with agent" ;
        rdfs:range          :agent ;
        rdfs:subPropertyOf  :related_with .

:referred_to_by  a  owl:ObjectProperty ;
        rdfs:label  "Referred to by" .

:reference-data_asset_release_is_basis_for_reference-data_asset_prerelease
        a              owl:ObjectProperty ;
        rdfs:comment   "A given version of a reference data (release) is the basis of prerelease version of the same reference data asset. This is a duplicate of cdm#reference-data_asset_release_basis_for_reference-data_asset_prerelease and should be deleted/deprecated." ;
        rdfs:domain    :reference-data_asset_release ;
        rdfs:label     "Reference data asset release is basis for reference data asset prerelease" ;
        rdfs:range     :reference-data_asset_prerelease ;
        owl:inverseOf  :reference-data_asset_prerelease_based_on_reference-data_asset_release .

:licence_document_is_licence_of_manifestation_distribution
        a              owl:ObjectProperty ;
        rdfs:comment   "A licence document representing the licence of a dataset distribution manifestation" ;
        rdfs:domain    :licence_document ;
        rdfs:label     "Licence document representing the licence of a distribution manifestation" ;
        rdfs:range     :manifestation_distribution ;
        owl:inverseOf  :manifestation_distribution_has_licence_licence_document .

<http://publications.europa.eu/resource/authority/fd_370>
        a       owl:NamedIndividual .

:subdivision_contains_subdivision
        a                   owl:ObjectProperty ;
        rdfs:comment        "A subdivision is hierarchically above another subdivision" ;
        rdfs:domain         :subdivision ;
        rdfs:label          "Subdivision contains subdivision" ;
        rdfs:range          :subdivision ;
        rdfs:subPropertyOf  :work_contains_work , :contains ;
        owl:inverseOf       :subdivision_part_of_subdivision .

:byte_size  a       owl:DatatypeProperty ;
        rdfs:label  "Byte size" .

:decision_representatives_member-states
        a                owl:Class ;
        rdfs:comment     "Decision of the representatives of the governments of the Member States (= subsector D of sector 4)" ;
        rdfs:label       "Decision of member state representatives" ;
        rdfs:subClassOf  :legislation_complementary .

:declared_valid_by  a  owl:ObjectProperty ;
        rdfs:label  "Declared valid by" .

:measure_national_implementing_implements_resource_legal
        a                   owl:ObjectProperty ;
        rdfs:comment        "Link to the act (directive or framework decision) that this NIM implements" ;
        rdfs:domain         :measure_national_implementing ;
        rdfs:label          "National implementing measure implements legal resource" ;
        rdfs:range          :resource_legal ;
        rdfs:subPropertyOf  :implements ;
        owl:inverseOf       :resource_legal_implemented_by_measure_national_implementing .

<http://publications.europa.eu/resource/authority/fd_285>
        a       owl:NamedIndividual .

:official-journal_year
        a                   owl:DatatypeProperty ;
        rdfs:comment        "Year in which this OJ number appeared" ;
        rdfs:domain         :official-journal ;
        rdfs:label          "Year of OJ" ;
        rdfs:range          xsd:gYear ;
        rdfs:subPropertyOf  :year .

:document_cjeu  a        owl:Class ;
        rdfs:comment     "Case law / jurisprudence and other communications of the Court of Justice (= sector 6). In contrast to the original structure a further subdevision by author is not represented in the class structure itself, but will be done by linking it to the author property. This does not preclude that we could calculate these classes based on that information and suitable inference rules. The following table --- which is based on the new structure of case law as proposed for the ongoing reunumerotation --- specifies the combination of case-law classes and the court handing out these type of case law (English translations of types based on a mail from Jean-Philippe Loucheur): || Type (en français) || Type (in English) || Sigle || Cour || TPI || TFP || Subclass || | | | | C | T | F | | | arrêt | judgement | J | CJ | TJ | FJ | | ordonnance | order | O | CO | TO | FO | | conclusion | Opinion of the advocate-general of the court of Justice | C | CC | TC | | saisie-arrêt | seizure | S | CS | | | tierce opposition | third-party proceedings | T | CT | TT | FT | | avis | Opinion of the Court of justice | V | CV | | | | délibération | ruling | X | CX | | | | décision | decision | D | CD | | | | prises de position | case report | P | CP | | | | communication nouvelle affaire | communication new case | N | CN | TN | FN | | communication arrêt | communication judgement | A | CA | TA | FA | | communication ordonnance | communication order | B | CB | TB | FB | | communication demande avis | communication request for an opinion | U | CU | | | | communication avis | communication opinion | G | CG | | | Sector 6 documents can be either case law or communications of the Court of Justice." ;
        rdfs:label       "Court of Justice document" ;
        rdfs:subClassOf  :resource_legal .

:reference_volume  a  owl:DatatypeProperty ;
        rdfs:label  "Reference volume" .

:number_official_journal
        a           owl:DatatypeProperty ;
        rdfs:label  "Number official journal" .

:resource_legal_published_in_special-official-journal
        a                   owl:ObjectProperty ;
        rdfs:comment        "The legal resource is published in a given special edition" ;
        rdfs:domain         :resource_legal ;
        rdfs:label          "Legal resource published in special edition" ;
        rdfs:range          :special-official-journal ;
        rdfs:subPropertyOf  :published_in ;
        owl:inverseOf       :special-official-journal_publishes_resource_legal .

:target_audience  a          owl:Class ;
        rdfs:comment         "Used to classify target audience" ;
        rdfs:label           "Target audience" ;
        rdfs:subClassOf      skos:Concept , :concept ;
        owl:equivalentClass  [ a               owl:Restriction ;
                               owl:hasValue    <http://publications.europa.eu/resource/authority/target_audience> ;
                               owl:onProperty  skos:inScheme
                             ] .

:manifestation_has_thumbnail
        a                   owl:ObjectProperty ;
        rdfs:comment        "A manifestation has a thumbnail (typically a jpg in the CCR). Needed for general publications" ;
        rdfs:domain         :manifestation ;
        rdfs:label          "Manifestation has thumbnail" ;
        rdfs:range          :thumbnail ;
        rdfs:subPropertyOf  :has ;
        owl:inverseOf       :thumbnail_belongs_to_manifestation .

:id_fragment  a             owl:DatatypeProperty ;
        rdfs:label          "Id fragment" ;
        rdfs:subPropertyOf  :identifier .

:institution_addressed_by_event_legal
        a                   owl:ObjectProperty ;
        rdfs:comment        "An institution which is being addressed by execution of a legal event" ;
        rdfs:domain         :institution ;
        rdfs:label          "Institution addressed by legal event" ;
        rdfs:range          :event_legal ;
        rdfs:subPropertyOf  :addressed_by .

:court-report_class  a      owl:DatatypeProperty ;
        rdfs:domain         :court-report ;
        rdfs:label          "Part of court report" ;
        rdfs:range          xsd:string ;
        rdfs:subPropertyOf  :class .

:archive_package_eesc_document
        a                owl:Class ;
        rdfs:comment     "The archive packages created in the scope of the EESC digitisation project(s) will provide in their metadata also the list of documents contained in the archive package in form of an ordered list of titles. Additional information (like EESC internal identifiers or the starting page of the different documents) may be provided to enrich the information on an EESC archive package document." ;
        rdfs:label       "Archive package document by EESC" ;
        rdfs:subClassOf  :archive_package_document ;
        rdfs:subClassOf  [ a                            owl:Restriction ;
                           owl:minQualifiedCardinality  "1"^^xsd:nonNegativeInteger ;
                           owl:onClass                  :archive_package_eesc ;
                           owl:onProperty               :archive_package_eesc_document_part_of_archive_package_eesc
                         ] ;
        dct:created      "2022-09-01T09:01:22" .

:subdivision_part_of_subdivision
        a                   owl:ObjectProperty ;
        rdfs:comment        "A subdivision is hierarchically below another subdivision" ;
        rdfs:domain         :subdivision ;
        rdfs:label          "Subdivision part of subdivision" ;
        rdfs:range          :subdivision ;
        rdfs:subPropertyOf  :work_part_of_work , :part_of .

:measure_national_implementing_implemented_by_country
        a                   owl:ObjectProperty ;
        rdfs:comment        "Link to the country that has implemented this NIM. For the data received from SecGen only information on the implementing country is available. In the future with ELI agents might be indicated more precisely (e.g. regions as legislators) and will be stored in work_created_by_agent" ;
        rdfs:domain         :measure_national_implementing ;
        rdfs:label          "National implementing measure implemented by country" ;
        rdfs:range          :country ;
        rdfs:subPropertyOf  :implemented_by ;
        owl:inverseOf       :country_implements_measure_national_implementing .

:work_part_of_collection_document
        a                   owl:ObjectProperty ;
        rdfs:comment        "DEPRECATED, The work is part of a document collection. COLL" ;
        rdfs:domain         :work ;
        rdfs:label          "Work is part of a document collection" ;
        rdfs:range          :collection_document ;
        rdfs:subPropertyOf  :part_of ;
        owl:deprecated      true ;
        owl:inverseOf       :collection_document_contains_work .

:resource_legal_proposes_to_amend_resource_legal
        a                   owl:ObjectProperty ;
        rdfs:comment        "This property points to act which provision(s) are proposed to be amended. Relevant for legal analysis: true" ;
        rdfs:domain         :resource_legal ;
        rdfs:label          "Legal resource proposes to amend legal resource" ;
        rdfs:range          :resource_legal ;
        rdfs:subPropertyOf  :proposes_to_amend ;
        owl:inverseOf       :resource_legal_amendment_proposed_by_resource_legal .

:resolution_legislative_term_parliamentary
        a                   owl:DatatypeProperty ;
        rdfs:comment        "This indicates the Parliamentary term during which an EP document was voted or EP question was raised. Relevant for legal analysis: true. Currently coded with FD_Table 285. However, only codes are exposed (not decoded), so 01, 02 etc." ;
        rdfs:domain         :resolution_legislative ;
        rdfs:label          "Parliamentary term" ;
        rdfs:range          xsd:string ;
        rdfs:subPropertyOf  :term_parliamentary , :act_preparatory_term_parliamentary .

:manifestation_contains_manifestation
        a                   owl:ObjectProperty ;
        rdfs:comment        "Relevant for legal analysis: true. The manfestation contains another manifestation. Relevant for legal analysis: true" ;
        rdfs:domain         :manifestation ;
        rdfs:label          "Manifestation contains manifestation" ;
        rdfs:range          :manifestation ;
        rdfs:subPropertyOf  :contains ;
        owl:inverseOf       :manifestation_part_of_manifestation .

:opinion  a              owl:Class ;
        rdfs:comment     "Opinion (subsector A of sector 3). Examples: 31968A0336, 31977A0674, 32009A1013(03)R(01),32009A1121(01)" ;
        rdfs:label       "Opinion" ;
        rdfs:subClassOf  :legislation_secondary .

:agent_reports_on_report_ep
        a              owl:ObjectProperty ;
        rdfs:comment   "Agent is an EP committee member reporting to the plenary about a topic (by a report)" ;
        rdfs:domain    :agent ;
        rdfs:label     "Agent reports on an EP report" ;
        rdfs:range     :report_ep ;
        owl:inverseOf  :report_ep_reported_by_agent .

:work_reported_by_person
        a                   owl:ObjectProperty ;
        rdfs:comment        "Work is the report of a reporting personal agent" ;
        rdfs:domain         :work ;
        rdfs:label          "Work reported by person" ;
        rdfs:range          :person ;
        rdfs:subPropertyOf  :work_reported_by_agent ;
        dct:created         "2018-05-25T10:35:36.108+02:00"^^xsd:dateTime .

:court-type  a               owl:Class ;
        rdfs:comment         "The type of Court handling a case" ;
        rdfs:label           "Court type" ;
        rdfs:subClassOf      skos:Concept ;
        owl:equivalentClass  [ a               owl:Restriction ;
                               owl:hasValue    <http://publications.europa.eu/resource/authority/court-type> ;
                               owl:onProperty  skos:inScheme
                             ] .

:pending-proposal  a  owl:DatatypeProperty ;
        rdfs:label  "Pending proposal" .

:authority-type_label
        a           owl:DatatypeProperty ;
        rdfs:label  "Authority type label" .

:concept_ntu  a          owl:Class ;
        rdfs:comment     "CAT NTU" ;
        rdfs:label       "Concept representing a territorial unit / NTU code in Ted" ;
        rdfs:subClassOf  :concept .

:resource_legal_number_sequence_celex
        a                   owl:DatatypeProperty ;
        rdfs:comment        "Sequence number part of the Celex identifier (id). For backlog based on ID_CELEX, currently provided by legal analysis contractor. Relevant for legal analysis: true" ;
        rdfs:domain         :resource_legal ;
        rdfs:label          "Celex sequence number" ;
        rdfs:range          xsd:positiveInteger ;
        rdfs:subPropertyOf  :number_sequence_celex .

:resource_legal_contains_cor_opinion_on_resource_legal
        a                   owl:ObjectProperty ;
        rdfs:comment        "This points to proposal on which CoR provides its opinion. Relevant for legal analysis: true." ;
        rdfs:domain         :resource_legal ;
        rdfs:label          "Legal resource contains Committee of the Regions opinion on legal resource" ;
        rdfs:range          :resource_legal ;
        rdfs:subPropertyOf  :contains_cor_opinion_on ;
        owl:inverseOf       :resource_legal_cor_opinion_contained_in_resource_legal .

:procurement_public_range_minimal
        a                   owl:DatatypeProperty ;
        rdfs:domain         :procurement_public ;
        rdfs:label          "Minimal value of a range" ;
        rdfs:range          xsd:decimal ;
        rdfs:subPropertyOf  :range_minimal .

:resource_legal_is_about_concept_directory-code
        a                   owl:ObjectProperty ;
        rdfs:comment        "A legal resource is about a concept expressed in the directory code (numerical classification tool; it offers access to EU law by subject). Use instead of secondary_legislation_is_about_concept_directory-code. CC, coded separatedly (FD table 555). Relevant for legal analysis: true" ;
        rdfs:domain         :resource_legal ;
        rdfs:label          "Legal resource is about directory code concept" ;
        rdfs:range          :concept_directory-code ;
        rdfs:subPropertyOf  :is_about ;
        owl:inverseOf       :concept_directory-code_subject_of_resource_legal .

:expression_procurement_public
        a                owl:Class ;
        rdfs:label       "Expression for public procurement" ;
        rdfs:subClassOf  :expression ;
        rdfs:subClassOf  [ a                   owl:Restriction ;
                           owl:minCardinality  "1"^^xsd:nonNegativeInteger ;
                           owl:onProperty      :expression_procurement_public_authority-type_name
                         ] .

:dossier_responsibility_of_agent
        a                   owl:ObjectProperty ;
        rdfs:comment        "This dossier is under the responsibility of a given agent. mapped from /ns4:ec_transmission_request/transmission/workflow/extension/ns3:workflow_agent , subproperty of involves" ;
        rdfs:domain         :dossier ;
        rdfs:label          "Dossier under responsibility of agent" ;
        rdfs:range          :agent ;
        rdfs:subPropertyOf  :responsibility_of , :dossier_involves_agent .

:depositary_for  a  owl:ObjectProperty ;
        rdfs:label  "Depositary for" .

:case-law_originates_in_country
        a                   owl:ObjectProperty ;
        rdfs:comment        "This property refers to country of origin of a question referred for a preliminary ruling. Coded with http://publications.europa.eu/resource/authority/country. This property used to point to both fd_140 which is deprecated. Our instance data is now fully pointing to the country table. A few records pointing to a temporary code have to be cleaned" ;
        rdfs:domain         :case-law ;
        rdfs:label          "Case law originates in country" ;
        rdfs:range          :country ;
        rdfs:subPropertyOf  :originates_in ;
        dct:created         "2018-07-24T10:14:29.237+02:00"^^xsd:dateTime ;
        owl:inverseOf       :country_initiates_case-law .

:thumbnail_belongs_to_manifestation
        a             owl:ObjectProperty ;
        rdfs:comment  "A thumbnail item is the effective thumbnail image of file(s) for another manifestation (e.g. PDF)" ;
        rdfs:domain   :thumbnail ;
        rdfs:label    "Thumbnail belongs to manifestation" ;
        rdfs:range    :manifestation .

:resource_legal_reference_oj-act
        a             owl:DatatypeProperty ;
        rdfs:comment  "An OJ act's reference string" ;
        rdfs:domain   :resource_legal ;
        rdfs:label    "OJ act reference of legal resource" ;
        rdfs:range    xsd:string .

:resource_legal_basis_for_event
        a            owl:ObjectProperty ;
        rdfs:domain  :resource_legal ;
        rdfs:label   "Resource legal basis for event" ;
        rdfs:range   :event .

:work_id  a                 owl:DatatypeProperty ;
        rdfs:comment        "DEPRECATED, A domain specific way to formally identify this resource. Relevant for legal analysis: true." ;
        rdfs:domain         :work ;
        rdfs:label          "Work identifier" ;
        rdfs:range          xsd:string ;
        rdfs:subPropertyOf  :id ;
        owl:deprecated      true .

:cites  a           owl:ObjectProperty ;
        rdfs:label  "Cites" .

:case-law_national_affaire_type
        a                   owl:DatatypeProperty ;
        rdfs:comment        "DEPRECATED, Type of the affaire, coded" ;
        rdfs:domain         :case-law_national ;
        rdfs:label          "National affaire: Type" ;
        rdfs:range          xsd:string ;
        rdfs:subPropertyOf  :affaire_type ;
        owl:deprecated      true .

:number_natural_celex
        a           owl:DatatypeProperty ;
        rdfs:label  "Number natural celex" .

:reference-data_asset_release
        a                owl:Class ;
        rdfs:comment     "A dataset representing a specific version of a reference data asset which has an unversioned representant in cdm:reference-data_asset/evolutive work. The documentation of a publication is represented by a linked object with class cdm:documentation." ;
        rdfs:label       "Release of reference data asset" ;
        rdfs:subClassOf  :work_dataset ;
        rdfs:subClassOf  [ a                owl:Restriction ;
                           owl:cardinality  "1"^^xsd:nonNegativeInteger ;
                           owl:onProperty   :reference-data_asset_release_releases_reference-data_asset
                         ] .

:s_package_ec  a         owl:Class ;
        rdfs:comment     "Internal documents of the European Commission with a S type identifier, meanwhile declassified." ;
        rdfs:label       "S package EC" ;
        rdfs:subClassOf  :swd_package_ec ;
        rdfs:subClassOf  [ a               owl:Restriction ;
                           owl:hasValue    "S" ;
                           owl:onProperty  :archive_package_internal_number_prefix
                         ] ;
        dct:created      "2022-09-28T21:12:47Z"^^xsd:dateTime .

:resource_legal_corrected_by_resource_legal
        a                   owl:ObjectProperty ;
        rdfs:comment        "Calculated. Relevant for legal analysis: true." ;
        rdfs:domain         :resource_legal ;
        rdfs:label          "Legal resource is corrected by legal resource" ;
        rdfs:range          :resource_legal ;
        rdfs:subPropertyOf  :corrected_by ;
        owl:inverseOf       :resource_legal_corrects_resource_legal .

:failure_stated_by  a  owl:ObjectProperty ;
        rdfs:label  "Failure stated by" .

:case-law_incidentally_declares_void_resource_legal
        a                   owl:ObjectProperty ;
        rdfs:comment        "This property points to legal act quoted in the operative part of Court decisions." ;
        rdfs:domain         :case-law ;
        rdfs:label          "Case law incidentally declares void legal resource" ;
        rdfs:range          :resource_legal ;
        rdfs:subPropertyOf  :incidentally_declares_void ;
        owl:inverseOf       :resource_legal_incidentally_declared_void_by_case-law .

:type_procedure_internal_is_type_of_procedure_internal
        a                   owl:ObjectProperty ;
        rdfs:comment        "the type of internal procedure associated to the internal procedure. Table com_internal_procedure" ;
        rdfs:domain         :type_procedure_internal ;
        rdfs:label          "Type procedure internal of internal procedure" ;
        rdfs:range          :procedure_internal ;
        rdfs:subPropertyOf  :is_type_of .

:concept_type_documentation_is_type_of_documentation
        a              owl:ObjectProperty ;
        rdfs:domain    :concept_type_documentation ;
        rdfs:label     "Concept type documentation is type of documentation" ;
        rdfs:range     :documentation ;
        owl:inverseOf  :documentation_has_type_concept_type_documentation .

:dossier_identifier  a      owl:DatatypeProperty ;
        rdfs:comment        "Relevant for legal analysis: true. the identifier of the dossier. Any type of identifier for this dossier. Dossier ID. Relevant for legal analysis: true" ;
        rdfs:domain         :dossier ;
        rdfs:label          "Dossier identifier" ;
        rdfs:range          rdf:PlainLiteral ;
        rdfs:subPropertyOf  :identifier .

:resolution_legislative_ep_reported_by_person
        a                   owl:ObjectProperty ;
        rdfs:comment        "Name of the person (EP member or member of CoR or EESC) who reports on the relevant act. This property will be deprecated and replaced with work_reported_by_person. Role RAPP. Relevant for legal analysis: true" ;
        rdfs:domain         :resolution_legislative_ep ;
        rdfs:label          "European Parliament legislative resolution has rapporteur" ;
        rdfs:range          :person ;
        rdfs:subPropertyOf  :reported_by ;
        dct:created         "2018-07-16T13:21:29.255+02:00"^^xsd:dateTime ;
        owl:inverseOf       :person_reports_on_resolution_legislative_ep .

:act_consolidated_number
        a                   owl:DatatypeProperty ;
        rdfs:comment        "Consleg number" ;
        rdfs:domain         :act_consolidated ;
        rdfs:label          "Consolidated act number" ;
        rdfs:range          xsd:string ;
        rdfs:subPropertyOf  :number .

:has_joined_conclusion
        a           owl:ObjectProperty ;
        rdfs:label  "Has joined conclusion" .

:serials_periodical  a   owl:Class ;
        rdfs:label       "Periodical serials" ;
        rdfs:subClassOf  :publication_general .

:procedure_without_code_interinstitutional_basis_legal
        a                   owl:DatatypeProperty ;
        rdfs:comment        "Legal basis of the procedure (as text). Relevant for legal analysis: true." ;
        rdfs:domain         :procedure_without_code_interinstitutional ;
        rdfs:label          "Legal basis of procedure without interinstitutional code" ;
        rdfs:range          xsd:string ;
        rdfs:subPropertyOf  :dossier_basis_legal ;
        dct:created         "2018-11-02T15:09:44.597+01:00"^^xsd:dateTime .

:decision  a             owl:Class ;
        rdfs:comment     "Subsector D of sector 3. At present 27222 notices" ;
        rdfs:label       "Decision" ;
        rdfs:subClassOf  :legislation_secondary .

:application_deferred_by
        a           owl:ObjectProperty ;
        rdfs:label  "Application deferred by" .

:summary  a              owl:Class ;
        rdfs:comment     "Not all summaries are necessarily treated as separate works, but when this is desired as e.g. in the case of the summaries of case law, this is the class to be used Note that summaries should whenever possible indicate which work(s) they summarize" ;
        rdfs:label       "Summary of another work" ;
        rdfs:subClassOf  :auxiliary-work .

:resource_legal_amended_by_case-law
        a                   owl:ObjectProperty ;
        rdfs:comment        "Calculated. MD. Relevant for legal analysis: true." ;
        rdfs:domain         :resource_legal ;
        rdfs:label          "Legal resource amended by case law" ;
        rdfs:range          :case-law ;
        rdfs:subPropertyOf  :amended_by ;
        owl:inverseOf       :case-law_amends_resource_legal .

:produces  a        owl:ObjectProperty ;
        rdfs:label  "Produces" .

:manuscript_ref  a  owl:DatatypeProperty ;
        rdfs:label  "Manuscript ref" .

:located_in  a      owl:ObjectProperty ;
        rdfs:label  "Located in" .

:advocate-general  a     owl:Class ;
        rdfs:comment     "Advocate general at the Court of Justice" ;
        rdfs:label       "Advocate general" ;
        rdfs:subClassOf  :person ;
        rdfs:subClassOf  [ a                            owl:Restriction ;
                           owl:minQualifiedCardinality  "1"^^xsd:nonNegativeInteger ;
                           owl:onClass                  :case-law ;
                           owl:onProperty               :advocate-general_delivers_case-law
                         ] .

:proposal_decision_ec
        a                owl:Class ;
        rdfs:comment     "where its resource_legal_type = (PC or DC or NONE), resource_legal_id_sector = 5, work_has_resource-type = (PROP_DEC, AMEND_PROP_DEC, DEC_DRAFT, DEC_DEL_DRAFT, DEC_FRAMW_DRAFT, PROP_DEC_NO_ADDRESSEE, PROP_DEC_FRAMW, PROP_DEC_IMPL, RECO_DEC)" ;
        rdfs:label       "Commission proposal for a decision" ;
        rdfs:subClassOf  :proposal_act , :act_preparatory_ec .

:table-of-contents  a    owl:Class ;
        rdfs:comment     "A separate table of contents for a general publication (e.g. the TOC of the official journal)" ;
        rdfs:label       "Table of contents" ;
        rdfs:subClassOf  :front .

:work_is_logical_successor_of_work
        a                   owl:ObjectProperty ;
        rdfs:comment        "This property associates an instance of Work which logically continues the content of another instance of Work with the latter (FRBRoo)" ;
        rdfs:domain         :work ;
        rdfs:label          "Work is logical successor of work" ;
        rdfs:range          :work ;
        rdfs:subPropertyOf  :is_logical_successor_of ;
        owl:inverseOf       :work_has_successor_work .

:rendered_obsolete_by
        a           owl:ObjectProperty ;
        rdfs:label  "Rendered obsolete by" .

:procedure_internal_impact_assessment_needed
        a                   owl:DatatypeProperty ;
        rdfs:comment        "Do the better_regulation_requirements require an impact assessment for this internal procedure? /ns4:ec_transmission_request/transmission/workflow/extension/ns3:better_regulation_requirements/ns3:impact_assessment" ;
        rdfs:domain         :procedure_internal ;
        rdfs:label          "Internal procedure needs impact assessment?" ;
        rdfs:range          xsd:boolean ;
        rdfs:subPropertyOf  :impact_assessment_needed .

:event_place  a      owl:DatatypeProperty ;
        rdfs:domain  :event ;
        rdfs:label   "Event place" ;
        rdfs:range   xsd:anyURI .

:tackles_similar_question_as
        a           owl:ObjectProperty ;
        rdfs:label  "Tackles similar question as" .

:staff-working-document_ec
        a                owl:Class ;
        rdfs:comment     "Where its resource_legal_type =(SC or none), resource_legal_id_sector = 5, work_has_resource-type = (SWD, JOINT_SWD, IMPACT_ASSESS, IMPACT_ASSESS_SUM, WORK_DOC, REPORT, COMMUNIC, COMMUNIC_POSIT, DEC_DRAFT, OPIN, ACT_OTHER,OPIN_IMPACT_ASSESS), work_created_by_agent = COM" ;
        rdfs:label       "European Commission Staff Working document" ;
        rdfs:subClassOf  :staff-working-document , :act_preparatory_ec .

:event_legal_based_on_resource_legal
        a                   owl:ObjectProperty ;
        rdfs:comment        "DEPRECATED, This legal event is based on a legal resource (typically a treaty article, but could also be secondary legislation). Relevant for legal analysis: true." ;
        rdfs:domain         :event_legal ;
        rdfs:label          "Legal event based on legal resource" ;
        rdfs:range          :resource_legal ;
        rdfs:subPropertyOf  :event_based_on_resource_legal , :based_on ;
        owl:deprecated      true ;
        owl:inverseOf       :resource_legal_basis_for_event_legal .

:documentation_documents_work_dataset
        a                   owl:ObjectProperty ;
        rdfs:comment        "The described resource documents dataset" ;
        rdfs:domain         :documentation ;
        rdfs:label          "Documents" ;
        rdfs:range          :work_dataset ;
        rdfs:subPropertyOf  :work_explains_work , :documents ;
        owl:inverseOf       :work_dataset_has_documentation_documentation .

:article_legal  a        owl:Class ;
        rdfs:comment     "An article in a legal document" ;
        rdfs:label       "Article" ;
        rdfs:subClassOf  :subdivision .

:procurement_public_comment_converter
        a                   owl:DatatypeProperty ;
        rdfs:domain         :procurement_public ;
        rdfs:label          "Comment convertor" ;
        rdfs:range          xsd:string ;
        rdfs:subPropertyOf  :comment_converter .

:publishes  a       owl:ObjectProperty ;
        rdfs:label  "Publishes" .

:basis_referral  a  owl:DatatypeProperty ;
        rdfs:label  "Basis referral" .

:case-law_published_in_erecueil
        a                   owl:DatatypeProperty ;
        rdfs:comment        "Is this case law document published in the eRecueil" ;
        rdfs:domain         :case-law ;
        rdfs:label          "Published in eRecueil" ;
        rdfs:range          xsd:boolean ;
        rdfs:subPropertyOf  :published_in_erecueil .

:manifestation_court-report_part_number
        a                   owl:DatatypeProperty ;
        rdfs:comment        "Number of the Court report." ;
        rdfs:domain         :manifestation_court-report_part ;
        rdfs:label          "Number of the Court report" ;
        rdfs:range          xsd:string ;
        rdfs:subPropertyOf  :number .

:comments  a        owl:ObjectProperty ;
        rdfs:label  "Comments" .

:opinion_consultation_cor_number_session
        a                   owl:DatatypeProperty ;
        rdfs:comment        "DEPRECATED. Number of session during which this act was debated or voted (EP.EESC,CoR, …). Relevant for legal analysis: true. Mixed content, decoded with fd_345. Use cdm:act_preparatory_number_session" ;
        rdfs:domain         :opinion_consultation_cor ;
        rdfs:label          "Number of session" ;
        rdfs:range          xsd:string ;
        rdfs:subPropertyOf  :number_session , :act_preparatory_number_session ;
        owl:deprecated      true .

:act_other_ec  a         owl:Class ;
        rdfs:comment     "7868 Other Commission acts (5XC)" ;
        rdfs:label       "Commission other act" ;
        rdfs:subClassOf  :act_preparatory_ec .

:date_withdrawn  a  owl:DatatypeProperty ;
        rdfs:label  "Date withdrawn" .

:transliterated_town  a  owl:DatatypeProperty ;
        rdfs:label  "Transliterated town" .

:archive_package_reference_volume
        a                   owl:DatatypeProperty ;
        rdfs:comment        "The reference of the volume to which this package belongs (one volume can consist of one or more packages)" ;
        rdfs:domain         :archive_package ;
        rdfs:label          "Archive package reference volume" ;
        rdfs:range          xsd:string ;
        rdfs:subPropertyOf  :reference_volume .

:procedure_without_code_interinstitutional
        a                owl:Class ;
        rdfs:comment     "A procedure initiated usually by the Commission, but not having an inter-institutional procedure code. The dossier does not follow one of the (non-)legislative procedures represented in this data model. In any case, a dossier consists of one or more events. Such a dossier could also lead to the adoption of a new act (Eg.: COM (2010) 2010))" ;
        rdfs:label       "Procedure without interinstitutional code" ;
        rdfs:subClassOf  :dossier ;
        rdfs:subClassOf  [ a                   owl:Restriction ;
                           owl:maxCardinality  "1"^^xsd:nonNegativeInteger ;
                           owl:onProperty      :procedure_without_code_interinstitutional_has_status
                         ] .

:agent_depositary_for_legislation_complementary
        a                   owl:ObjectProperty ;
        rdfs:comment        "Agent is depositary for complementary legislation" ;
        rdfs:domain         :agent ;
        rdfs:label          "Agent is depositary for complementary legislation" ;
        rdfs:range          :legislation_complementary ;
        rdfs:subPropertyOf  :depositary_for ;
        owl:inverseOf       :legislation_complementary_stored_by_agent .

:act_preparatory_number_session
        a                   owl:DatatypeProperty ;
        rdfs:comment        "Number of session during which this act was debated or voted (EP, EESC, CoR, …). Relevant for legal analysis: true" ;
        rdfs:domain         :act_preparatory ;
        rdfs:label          "Number of session" ;
        rdfs:range          xsd:string ;
        rdfs:subPropertyOf  :number_session .

:communication_cjeu_has_procjur
        a                   owl:ObjectProperty ;
        rdfs:comment        "The communication has a type of judicial procedure (procédures juridictionnelles). http://publications.europa.eu/mdr/resource/authority/procjur/html/procjur-eng.html" ;
        rdfs:domain         :communication_cjeu ;
        rdfs:label          "Communication on case law has a judicial procedure type" ;
        rdfs:range          :procjur ;
        rdfs:subPropertyOf  :has .

:resource_legal_procedure_number
        a                   owl:DatatypeProperty ;
        rdfs:comment        "Number of the corresponding legal procedure. Obsolete, only maintained for backwards compatibility. Relevant for legal analysis: true" ;
        rdfs:domain         :resource_legal ;
        rdfs:label          "Legal procedure number" ;
        rdfs:range          xsd:string ;
        rdfs:subPropertyOf  :procedure_number .

:file_act_consolidated
        a           owl:DatatypeProperty ;
        rdfs:label  "File act consolidated" .

:transliterated_phone
        a           owl:DatatypeProperty ;
        rdfs:label  "Transliterated phone" .

:manifestation_has-feature-accessibility_publication-accessibility
        a                   owl:ObjectProperty ;
        rdfs:comment        "A note describing assistive features and/or adaptations to improve the accessibility of this general publication for particular needs of some audiences." ;
        rdfs:domain         :manifestation ;
        rdfs:label          "Manifestation has feature publication accessiblity" ;
        rdfs:range          :publication-accessibility ;
        rdfs:subPropertyOf  :has_feature ;
        dct:created         "2022-08-01T16:18:31.50"^^xsd:dateTime ;
        owl:inverseOf       :publication-accessibility_is-feature-accessibility-of_manifestation .

:dataset-status  a           owl:Class ;
        rdfs:comment         "Status of the dataset (values from AT dataset-status)" ;
        rdfs:label           "Dataset status" ;
        rdfs:subClassOf      :concept_decoding ;
        owl:equivalentClass  [ a               owl:Restriction ;
                               owl:hasValue    <http://publications.europa.eu/resource/authority/dataset-status> ;
                               owl:onProperty  skos:inScheme
                             ] .

:legal-act-domain  a         owl:Class ;
        rdfs:label           "Legal act domain" ;
        rdfs:subClassOf      skos:Concept ;
        owl:equivalentClass  [ a               owl:Restriction ;
                               owl:hasValue    <http://publications.europa.eu/resource/authority/legal-act-domain> ;
                               owl:onProperty  skos:inScheme
                             ] .

:act_reference_national
        a           owl:DatatypeProperty ;
        rdfs:label  "Act reference national" .

:case_court_treats_appeal_case-law
        a                   owl:ObjectProperty ;
        rdfs:comment        "An appeal against an existing case law is discussed in this case" ;
        rdfs:domain         :case_court ;
        rdfs:label          "Case treats the appeal against a case law document" ;
        rdfs:range          :case-law ;
        rdfs:subPropertyOf  :treats_appeal .

:unit_administrative_location_for_period
        a                   owl:ObjectProperty ;
        rdfs:comment        "The period takes place in a given administrative unit" ;
        rdfs:domain         :unit_administrative ;
        rdfs:label          "Administrative unit is location for period" ;
        rdfs:range          :period ;
        rdfs:subPropertyOf  :location_for .

:resource_legal_does_repeal_of_resource_legal
        a                   owl:ObjectProperty ;
        rdfs:comment        "Legal resources does repeal a legal resource, in term of consolidation" ;
        rdfs:domain         :resource_legal ;
        rdfs:label          "Legal resources does repeal of legal resource" ;
        rdfs:range          :resource_legal ;
        rdfs:subPropertyOf  :does_repeal_of .

:ATTO_FD_605  a              owl:Class ;
        rdfs:label           "FD_605 ATTO table" ;
        rdfs:subClassOf      skos:Concept ;
        owl:equivalentClass  [ a               owl:Restriction ;
                               owl:hasValue    <http://publications.europa.eu/resource/authority/fd_605> ;
                               owl:onProperty  skos:inScheme
                             ] .

:event_legal_associated_with_institution
        a                   owl:ObjectProperty ;
        rdfs:comment        "DEPRECATED, This legal event is associated with a given institution. Relevant for legal analysis: true." ;
        rdfs:domain         :event_legal ;
        rdfs:label          "Legal event associated with institution" ;
        rdfs:range          :institution ;
        rdfs:subPropertyOf  :event_associated_with_institution , :associated_with ;
        owl:deprecated      true ;
        owl:inverseOf       :institution_associated_with_event_legal .

:has_type_comment  a  owl:ObjectProperty ;
        rdfs:label  "Has type comment" .

:value_type  a      owl:DatatypeProperty ;
        rdfs:label  "Value type" .

:event_legal_comment  a     owl:DatatypeProperty ;
        rdfs:comment        "Comment on the legal event. Not to be displayed. Relevant for legal analysis: true." ;
        rdfs:domain         :event_legal ;
        rdfs:label          "Comment on legal event" ;
        rdfs:range          rdf:PlainLiteral ;
        rdfs:subPropertyOf  :comment .

:resource_legal_date_entry-into-force
        a                   owl:DatatypeProperty ;
        rdfs:comment        "Date of the entry into force of a legal resource IF_COMMENT and IF_TYPE are mixed content, decoded with fd_335. IF (type as annotation). Relevant for legal analysis: true" ;
        rdfs:domain         :resource_legal ;
        rdfs:label          "Date of entry into force" ;
        rdfs:range          xsd:date ;
        rdfs:subPropertyOf  :date_entry-into-force .

:published_in  a    owl:ObjectProperty ;
        rdfs:label  "Published in" .

:belongs_to  a      owl:ObjectProperty ;
        rdfs:label  "Belongs to" .

:expression_publication_general_projection
        a                   owl:DatatypeProperty ;
        rdfs:comment        "Projection, typically of a map (e.g. \"Gauss proj.\")" ;
        rdfs:domain         :expression_publication_general ;
        rdfs:label          "Projection of a map" ;
        rdfs:range          xsd:string ;
        rdfs:subPropertyOf  :projection .

:session_date_end_planned
        a           owl:DatatypeProperty ;
        rdfs:label  "Session date end planned" .

:manifestation_number_catalogue
        a                   owl:DatatypeProperty ;
        rdfs:comment        "cataglogue number of this manifestation (typically, if it is a general publication). In Formex e.g. <NO.CAT>QDAB1001AENC</NO.CAT>" ;
        rdfs:domain         :manifestation ;
        rdfs:label          "Catalogue number" ;
        rdfs:range          xsd:string ;
        rdfs:subPropertyOf  :number_catalogue .

:ATTO_FD_578  a              owl:Class ;
        rdfs:label           "FD_578 ATTO table" ;
        rdfs:subClassOf      skos:Concept ;
        owl:equivalentClass  [ a               owl:Restriction ;
                               owl:hasValue    <http://publications.europa.eu/resource/authority/fd_578> ;
                               owl:onProperty  skos:inScheme
                             ] .

:person_reports_on_act_other_eesc
        a                   owl:ObjectProperty ;
        rdfs:domain         :person ;
        rdfs:label          "Person reports on act_other_eesc" ;
        rdfs:range          :act_other_eesc ;
        rdfs:subPropertyOf  :reports_on .

:signature_digital_date_expiration
        a                   owl:DatatypeProperty ;
        rdfs:comment        "Date and time this signature loses its validity. Can be updated in case of renewal" ;
        rdfs:domain         :signature_digital ;
        rdfs:label          "Expiration date and time" ;
        rdfs:range          xsd:dateTime ;
        rdfs:subPropertyOf  :date_expiration .

:procedure_internal_planned_adoption_period_date_end
        a                   owl:DatatypeProperty ;
        rdfs:comment        "End date of the planned adoption period for this internal dossier. Information on the planned period for the public consultation. The information is always a period, so end_date must always be higher than start_date.The information is sent in all events part of the workflow Planning. Therefore the information sent in the most recent event is the most precise and has to prevail on the preceding information sent." ;
        rdfs:domain         :procedure_internal ;
        rdfs:label          "Internal procedure: End date of the planned adoption period" ;
        rdfs:range          xsd:date ;
        rdfs:subPropertyOf  :planned_adoption_period_date_end .

:number_contract  a  owl:DatatypeProperty ;
        rdfs:label  "Number contract" .

:official-journal  a     owl:Class ;
        rdfs:comment     "The Official Journal itself" ;
        rdfs:label       "Official Journal" ;
        rdfs:subClassOf  :resource_legal , :publication_general ;
        rdfs:subClassOf  [ a                owl:Restriction ;
                           owl:cardinality  "1"^^xsd:nonNegativeInteger ;
                           owl:onProperty   :official-journal_year
                         ] ;
        rdfs:subClassOf  [ a                         owl:Restriction ;
                           owl:onClass               :collection_document ;
                           owl:onProperty            :official-journal_part_of_collection_document ;
                           owl:qualifiedCardinality  "1"^^xsd:nonNegativeInteger
                         ] ;
        rdfs:subClassOf  [ a                   owl:Restriction ;
                           owl:maxCardinality  "1"^^xsd:nonNegativeInteger ;
                           owl:onProperty      :official-journal_volume
                         ] ;
        rdfs:subClassOf  [ a                   owl:Restriction ;
                           owl:maxCardinality  "1"^^xsd:nonNegativeInteger ;
                           owl:onProperty      :official-journal_legal_effect_paper
                         ] ;
        rdfs:subClassOf  [ a                owl:Restriction ;
                           owl:cardinality  "1"^^xsd:nonNegativeInteger ;
                           owl:onProperty   :official-journal_number
                         ] ;
        rdfs:subClassOf  [ a                   owl:Restriction ;
                           owl:maxCardinality  "1"^^xsd:nonNegativeInteger ;
                           owl:onProperty      :official-journal_class
                         ] .

:act_consolidated_summarized_by_summary_legislation_eu
        a                   owl:ObjectProperty ;
        rdfs:comment        "Consolidated act is summarized by summary of EU legislation" ;
        rdfs:domain         :act_consolidated ;
        rdfs:label          "Consolidated act is summarized by summary of EU legislation" ;
        rdfs:range          :summary_legislation_eu ;
        rdfs:subPropertyOf  :resource_legal_summarized_by_summary_legislation_eu ;
        owl:inverseOf       :summary_legislation_eu_summarizes_act_consolidated .

:proposal_regulation_codified_ec
        a                owl:Class ;
        rdfs:comment     "Commission Proposal Codified Regulation (5EC)" ;
        rdfs:label       "Commission proposal for a codified regulation" ;
        rdfs:subClassOf  :act_preparatory_ec .

:manifestation_special-official-journal
        a                owl:Class ;
        rdfs:comment     "Information on the print manifestation of a special edition of the official journal" ;
        rdfs:label       "Manifestation of a Special Edition of the Official Journal" ;
        rdfs:subClassOf  :manifestation_print .

:class  a           owl:DatatypeProperty ;
        rdfs:label  "Class" .

:doi    a           owl:DatatypeProperty ;
        rdfs:label  "Doi" .

:dossier_is_about_concept_field_activity
        a                   owl:ObjectProperty ;
        rdfs:comment        "Relevant for legal analysis: true. This dossier is about a certain field of activity. Relevant for legal analysis: true" ;
        rdfs:domain         :dossier ;
        rdfs:label          "Dossier touches a field of activity" ;
        rdfs:range          :concept_field_activity ;
        rdfs:subPropertyOf  :is_about .

:ATTO_FD_557  a              owl:Class ;
        rdfs:label           "FD_557 ATTO table" ;
        rdfs:subClassOf      skos:Concept ;
        owl:equivalentClass  [ a               owl:Restriction ;
                               owl:hasValue    <http://publications.europa.eu/resource/authority/fd_557> ;
                               owl:onProperty  skos:inScheme
                             ] .

:received  a        owl:ObjectProperty ;
        rdfs:label  "Received" .

:dossier_has_successor_dossier
        a                   owl:ObjectProperty ;
        rdfs:comment        "cf. above" ;
        rdfs:domain         :dossier ;
        rdfs:label          "Dossier has successor dossier" ;
        rdfs:range          :dossier ;
        rdfs:subPropertyOf  :has_successor ;
        owl:inverseOf       :dossier_is_logical_successor_of_dossier .

:authority-type_code  a  owl:DatatypeProperty ;
        rdfs:label  "Authority type code" .

:communication_case_new_requests_establishment_of_failure_of_obligation_resource_legal
        a                   owl:ObjectProperty ;
        rdfs:comment        "This property points to legal act quoted in the communication on a new case published in OJ. Relevant for legal analysis: true" ;
        rdfs:domain         :communication_case_new ;
        rdfs:label          "Communication requests to establish failure to fulfill an obligation" ;
        rdfs:range          :resource_legal ;
        rdfs:subPropertyOf  :requests_establishment_of_failure_of_obligation ;
        owl:inverseOf       :resource_legal_establishment_of_failure_of_obligation_requested_by_communication_case_new .

<http://publications.europa.eu/resource/authority/fd_610>
        a       owl:NamedIndividual .

:dimension  a       owl:DatatypeProperty ;
        rdfs:label  "Dimension" .

:reference-data_asset_prerelease
        a                owl:Class ;
        rdfs:comment     "A prerelease version of the a reference data asset, marked as not being \"official\". It has no documentation link and is not linked to any publication but only to a reference data asset release as base version from which it is derived." ;
        rdfs:label       "Pre-release of reference data asset" ;
        rdfs:subClassOf  :work_dataset ;
        rdfs:subClassOf  [ a                owl:Restriction ;
                           owl:cardinality  "1"^^xsd:nonNegativeInteger ;
                           owl:onProperty   :reference-data_asset_prerelease_prereleases_reference-data_asset
                         ] ;
        rdfs:subClassOf  [ a                owl:Restriction ;
                           owl:cardinality  "1"^^xsd:nonNegativeInteger ;
                           owl:onProperty   :reference-data_asset_prerelease_based_on_reference-data_asset_release
                         ] .

:resource_legal_part_of_acquis_language
        a                   owl:ObjectProperty ;
        rdfs:comment        "Resource legal is considered to be part of the acquis for a given language at a given moment" ;
        rdfs:domain         :resource_legal ;
        rdfs:label          "Resource legal is part of acquis for a language" ;
        rdfs:range          :language ;
        rdfs:subPropertyOf  :part_of_acquis ;
        owl:deprecated      true .

:work_dataset_has_type_concept_type_dataset
        a                   owl:ObjectProperty ;
        rdfs:comment        "This property indicates the type of dataset" ;
        rdfs:domain         :work_dataset ;
        rdfs:label          "Type of dataset" ;
        rdfs:range          :concept_type_dataset ;
        rdfs:subPropertyOf  :has_type ;
        owl:inverseOf       :concept_type_dataset_is_type_of_work_dataset .

:manifestation-mobile-app
        a                owl:Class ;
        rdfs:comment     "Mobile applications are a product type in the scope of General Publications. Their metadata refers to the app store from which the application can be downloaded. Mobile app manifestions are not stored in different versions, only the current version is exposed." ;
        rdfs:label       "Mobile application manifestation" ;
        rdfs:subClassOf  :manifestation-publication-general ;
        rdfs:subClassOf  [ a                            owl:Restriction ;
                           owl:maxQualifiedCardinality  "1"^^xsd:nonNegativeInteger ;
                           owl:onDataRange              xsd:string ;
                           owl:onProperty               :manifestation-mobile-app_version
                         ] ;
        rdfs:subClassOf  [ a                            owl:Restriction ;
                           owl:maxQualifiedCardinality  "1"^^xsd:nonNegativeInteger ;
                           owl:onClass                  :dissemination-status ;
                           owl:onProperty               :manifestation-mobile-app_has-status_dissemination-status
                         ] ;
        rdfs:subClassOf  [ a                            owl:Restriction ;
                           owl:maxQualifiedCardinality  "1"^^xsd:nonNegativeInteger ;
                           owl:onDataRange              <http://publications.europa.eu/ontology/datatype#date> ;
                           owl:onProperty               :manifestation-mobile-app_date-modified
                         ] ;
        rdfs:subClassOf  [ a                            owl:Restriction ;
                           owl:minQualifiedCardinality  "1"^^xsd:nonNegativeInteger ;
                           owl:onDataRange              xsd:anyURI ;
                           owl:onProperty               :manifestation-mobile-app_access-url
                         ] .

<http://publications.europa.eu/resource/authority/case-status>
        a       owl:NamedIndividual .

:implemented_by  a  owl:ObjectProperty ;
        rdfs:label  "Implemented by" .

:resource_legal_date_signature
        a                   owl:DatatypeProperty ;
        rdfs:comment        "Date or dates of the signing of a legislative act, agreement or EU budget. This field may also contain a reference to the place where the agreement was signed. SG_COMMENT is mixed content, decoded with fd_325.SG. Relevant for legal analysis: true" ;
        rdfs:domain         :resource_legal ;
        rdfs:label          "Date of signature" ;
        rdfs:range          xsd:date ;
        rdfs:subPropertyOf  :date_signature .

:concept_udc  a          owl:Class ;
        rdfs:comment     "Universal Decimal Classification (UDC), used to classify general publications" ;
        rdfs:label       "UDC concept" ;
        rdfs:subClassOf  :concept .

:resource_legal_establishment_of_failure_of_obligation_requested_by_communication_case_new
        a              owl:ObjectProperty ;
        rdfs:domain    :resource_legal ;
        rdfs:label     "Resource legal establishment of failure of obligation requested by communication case new" ;
        rdfs:range     :communication_case_new ;
        owl:inverseOf  :communication_case_new_requests_establishment_of_failure_of_obligation_resource_legal .

:institution_associated_with_event
        a             owl:ObjectProperty ;
        rdfs:comment  "An institution is associated with the execution of an event" ;
        rdfs:domain   :institution ;
        rdfs:label    "Institution associated with event" ;
        rdfs:range    :event .

:official-journal-act_number
        a                   owl:DatatypeProperty ;
        rdfs:comment        "The number of the Official Journal act as assigned by the production unit; this makes part of the Official Journal act identification" ;
        rdfs:domain         :official-journal-act ;
        rdfs:label          "Official Journal act number" ;
        rdfs:range          xsd:positiveInteger ;
        rdfs:subPropertyOf  :number .

:decision_internal_ep_reported_by_person
        a                   owl:ObjectProperty ;
        rdfs:comment        "Name of the person (EP member or member of CoR or EESC) who reports on the relevant act. This property will be deprecated and replaced with work_reported_by_person. Role RAPP. Relevant for legal analysis: true" ;
        rdfs:domain         :decision_internal_ep ;
        rdfs:label          "European Parliament internal decision" ;
        rdfs:range          :person ;
        rdfs:subPropertyOf  :work_reported_by_person ;
        dct:created         "2018-07-16T13:17:23.176+02:00"^^xsd:dateTime ;
        owl:inverseOf       :person_reports_on_decision_internal_ep .

:ATTO_FD_600  a              owl:Class ;
        rdfs:label           "FD_600 ATTO table" ;
        rdfs:subClassOf      skos:Concept ;
        owl:equivalentClass  [ a               owl:Restriction ;
                               owl:hasValue    <http://publications.europa.eu/resource/authority/fd_600> ;
                               owl:onProperty  skos:inScheme
                             ] .

:defends_in  a      owl:ObjectProperty ;
        rdfs:label  "Defends in" .

:act_preparatory_number_session_planned
        a                   owl:DatatypeProperty ;
        rdfs:comment        "Number of session during which this preparatory act will most likely be debated or voted (EO, EESC, CoR, …)" ;
        rdfs:domain         :act_preparatory ;
        rdfs:label          "Number of planned session" ;
        rdfs:range          xsd:string ;
        rdfs:subPropertyOf  :number_session_planned .

:event_number_session
        a                   owl:DatatypeProperty ;
        rdfs:comment        "A number of a session during which this event took place, e.g. in the Council or the Committee of the Regions" ;
        rdfs:domain         :event ;
        rdfs:label          "Number of a session for event" ;
        rdfs:range          xsd:positiveInteger ;
        rdfs:subPropertyOf  :number_session .

:event_co-reported_by_person
        a                   owl:ObjectProperty ;
        rdfs:domain         :event ;
        rdfs:label          "Event co-reported by person" ;
        rdfs:range          :person ;
        rdfs:subPropertyOf  :co-reported_by ;
        owl:inverseOf       :person_co-reports_event .

:opinion_consultation_cor_reported_by_person
        a                   owl:ObjectProperty ;
        rdfs:comment        "Name of the person (EP member or member of CoR or EESC) who reports on the relevant act. This property will be deprecated and replaced with work_reported_by_person. Role RAPP. Relevant for legal analysis: true" ;
        rdfs:domain         :opinion_consultation_cor ;
        rdfs:label          "Committee of the Regions' opinion on consultation has rapporteur" ;
        rdfs:range          :person ;
        rdfs:subPropertyOf  :reported_by ;
        dct:created         "2018-07-16T13:18:25.010+02:00"^^xsd:dateTime ;
        owl:inverseOf       :person_reports_on_opinion_consultation_cor .

:authority-type_name  a  owl:DatatypeProperty ;
        rdfs:label  "Authority type name" .

:manifestation_special-official-journal_part_pages_total
        a                   owl:DatatypeProperty ;
        rdfs:comment        "DEPRECATED, Total number of pages of the SE part related to a legal resource. Use manifestion_print_pages_total" ;
        rdfs:domain         :manifestation_special-official-journal_part ;
        rdfs:label          "Total pages" ;
        rdfs:range          xsd:string ;
        rdfs:subPropertyOf  :pages_total , :manifestation_print_pages_total ;
        owl:deprecated      true .

:treaty  a               owl:Class ;
        rdfs:comment     "The class treaty does has concrete treaty instances that correspond to the subsectors of sector 1" ;
        rdfs:label       "Treaty" ;
        rdfs:subClassOf  :resource_legal .

:work_related_to_work
        a                   owl:SymmetricProperty , owl:ObjectProperty ;
        rdfs:comment        "Relevant for legal analysis: true. The work is related to another work, the relationship being not further typed (including links such as LNK_CELEX_DN). Relevant for legal analysis: true" ;
        rdfs:domain         :work ;
        rdfs:label          "Work related to work" ;
        rdfs:range          :work ;
        rdfs:subPropertyOf  :related_to .

:annex  a                owl:Class ;
        rdfs:comment     "an addition to a document\" (OED)" ;
        rdfs:label       "Annex" ;
        rdfs:subClassOf  :subdivision , :auxiliary-work .

:agent_authors_work  a  owl:ObjectProperty ;
        rdfs:domain    :agent ;
        rdfs:label     "Agent acts as author of a work" ;
        rdfs:range     :work ;
        owl:inverseOf  :work_authored_by_agent .

:handed_over  a     owl:ObjectProperty ;
        rdfs:label  "Handed over" .

:judgement_reference  a  owl:DatatypeProperty ;
        rdfs:label  "Judgement reference" .

:person_reports_on_document_budget_ep
        a                   owl:ObjectProperty ;
        rdfs:domain         :person ;
        rdfs:label          "Person reports on documention_budget_ep" ;
        rdfs:range          :document_budget_ep ;
        rdfs:subPropertyOf  :reports_on ;
        owl:inverseOf       :document_budget_ep_reported_by_person .

:procurement_public_transliterated_organisation_official-name
        a                   owl:DatatypeProperty ;
        rdfs:domain         :procurement_public ;
        rdfs:label          "Procurement public transliterated organisation official name" ;
        rdfs:range          xsd:string ;
        rdfs:subPropertyOf  :transliterated_organisation_official-name .

:resource_legal_information_miscellaneous
        a                   owl:DatatypeProperty ;
        rdfs:comment        "Various miscellaneous information. Mixed content, decoded with fd_400. MI. Relevant for legal analysis: true" ;
        rdfs:domain         :resource_legal ;
        rdfs:label          "Miscellaneous information" ;
        rdfs:range          xsd:string ;
        rdfs:subPropertyOf  :information_miscellaneous .

:official-journal_part_of_collection_document
        a                   owl:ObjectProperty ;
        rdfs:comment        "OJ Series" ;
        rdfs:domain         :official-journal ;
        rdfs:label          "Official journal is part of a document collection" ;
        rdfs:range          :collection_document ;
        rdfs:subPropertyOf  :part_of ;
        owl:inverseOf       :collection_document_contains_official-journal .

:judgement_national  a  owl:DatatypeProperty ;
        rdfs:label  "Judgement national" .

:consults  a        owl:ObjectProperty ;
        rdfs:label  "Consults" .

:title_legal  a          owl:Class ;
        rdfs:comment     "A title in a legal document. Created to have correspondance to the subdivision NAL" ;
        rdfs:label       "Title in a legal resource" ;
        rdfs:subClassOf  :subdivision .

:act_consolidated_consolidates_resource_legal
        a                   owl:ObjectProperty ;
        rdfs:comment        "Here according to spec of advanced search the *celexs* of the consolidating acts is to be indexed (= a language independent textual information). This information will be provided in the indexation notice (BF)" ;
        rdfs:domain         :act_consolidated ;
        rdfs:label          "Consolidated act consolidates legal resource" ;
        rdfs:range          :resource_legal ;
        rdfs:subPropertyOf  :consolidates ;
        owl:inverseOf       :resource_legal_consolidated_by_act_consolidated .

:complex_work_group_id
        a           owl:DatatypeProperty ;
        rdfs:label  "Complex work group id" .

:indent_part_of_work  a     owl:ObjectProperty ;
        rdfs:comment        "This property associates an instance of a work with an instance of INDENT that forms part of it." ;
        rdfs:domain         :indent ;
        rdfs:label          "Indent part of work" ;
        rdfs:range          :work ;
        rdfs:subPropertyOf  :subdivision_part_of_work , :part_of ;
        owl:inverseOf       :work_contains_indent .

:com_package_reference_volume
        a                   owl:DatatypeProperty ;
        rdfs:comment        "Reference of the volume in which this COM package is contained" ;
        rdfs:domain         :com_package ;
        rdfs:label          "COM package volume reference" ;
        rdfs:range          xsd:string ;
        rdfs:subPropertyOf  :reference_volume .

:procurement_public_has_originally_concept_cpv
        a                   owl:ObjectProperty ;
        rdfs:comment        "Public procurement is originally classified against a CPV concept" ;
        rdfs:domain         :procurement_public ;
        rdfs:label          "Public procurement has original CPV concept" ;
        rdfs:range          :concept_cpv ;
        rdfs:subPropertyOf  :has_originally .

:is_type_of  a      owl:ObjectProperty ;
        rdfs:label  "Is type of" .

:act_surveillance-authority_efta
        a                owl:Class ;
        rdfs:comment     "Act of the European Free Trade Association (EFTA) Surveillance Authority (= subsector C of sector E in EUR-Lex)" ;
        rdfs:label       "Act of EFTA Surveillance Authority" ;
        rdfs:subClassOf  :document_efta .

:work_contains_preamble
        a                   owl:ObjectProperty ;
        rdfs:domain         :work ;
        rdfs:label          "Work contains preamble" ;
        rdfs:range          :preamble ;
        rdfs:subPropertyOf  :work_contains_subdivision , :contains .

:comment_internal  a  owl:DatatypeProperty ;
        rdfs:label  "Comment internal" .

:language_used_by_accompanying_material_expression
        a                   owl:ObjectProperty ;
        rdfs:comment        "A given language is used for the accompanying material of an expression (typically of a general publication)" ;
        rdfs:domain         :language ;
        rdfs:label          "Language used by accompanying material" ;
        rdfs:range          :expression ;
        rdfs:subPropertyOf  :used_by_accompanying_material .

:datetime_submission  a  owl:DatatypeProperty ;
        rdfs:label  "Datetime submission" .

:description_editorial
        a           owl:DatatypeProperty ;
        rdfs:label  "Description editorial" .

:manifestation_court-report_part_page_last
        a                   owl:DatatypeProperty ;
        rdfs:comment        "DEPRECATED, Last page number of the Court report part related to a court document. Use manifestion_print_page_last" ;
        rdfs:domain         :manifestation_court-report_part ;
        rdfs:label          "Last page" ;
        rdfs:range          xsd:string ;
        rdfs:subPropertyOf  :page_last , :manifestation_print_page_last ;
        owl:deprecated      true .

:summary_case-law_jure_id_celex
        a                   owl:DatatypeProperty ;
        rdfs:comment        "Identifier for the summary of case law (build on Celex identifier in sector 8 followed by _SUMJURE)" ;
        rdfs:domain         :summary_case-law_jure ;
        rdfs:label          "Identifier for case law in JURE" ;
        rdfs:range          xsd:string ;
        rdfs:subPropertyOf  :id_celex .

:resource_legal_addresses_organization
        a                   owl:ObjectProperty ;
        rdfs:comment        "Name of an organization (often private) to which the act is addressed. Relevant for legal analysis: true" ;
        rdfs:domain         :resource_legal ;
        rdfs:label          "Legal resource addresses organization" ;
        rdfs:range          :organization ;
        rdfs:subPropertyOf  :addresses ;
        owl:inverseOf       :organization_addressed_by_resource_legal .

:drafted_by  a      owl:ObjectProperty ;
        rdfs:label  "Drafted by" .

:date_deletion  a           owl:DatatypeProperty ;
        rdfs:label          "Date deletion" ;
        rdfs:range          xsd:date ;
        rdfs:subPropertyOf  :date .

:labels_forms_reference
        a           owl:DatatypeProperty ;
        rdfs:label  "Labels forms reference" .

:reproduced_as  a   owl:ObjectProperty ;
        rdfs:label  "Reproduced as" .

cmr:creationDate  a   owl:DatatypeProperty ;
        rdfs:comment  "The date when an entity was introduced/created the first time in the Common Metadata Repository." ;
        rdfs:label    "CMR creation date" ;
        rdfs:range    xsd:dateTime .

:contains_cor_opinion_on
        a           owl:ObjectProperty ;
        rdfs:label  "Contains cor opinion on" .

:case-law_commented_by_agent
        a                   owl:ObjectProperty ;
        rdfs:comment        "This lists the institutions, bodies or Member States having presented observations on the case in a preliminary ruling. We are in the process of cleaning some temporary values for that property and are planning to switch values following fd_160 table (deprecated) to one value of the NAL country, corporate-body or role-qualifier." ;
        rdfs:domain         :case-law ;
        rdfs:label          "Case law commented by agent" ;
        rdfs:range          :agent ;
        rdfs:subPropertyOf  :commented_by ;
        dct:created         "2018-07-24T10:15:26.014+02:00"^^xsd:dateTime ;
        owl:inverseOf       :agent_comments_case-law .

:resolution_legislative
        a                owl:Class ;
        rdfs:comment     "8806 EP legislative resolutions (5AP) NOT TO BE USED YET, because Text Adopted is in \"preliminary\" status?" ;
        rdfs:label       "Legislative resolution" ;
        rdfs:subClassOf  :text-adopted ;
        rdfs:subClassOf  [ a                owl:Restriction ;
                           owl:cardinality  "1"^^xsd:nonNegativeInteger ;
                           owl:onProperty   :resolution_legislative_term_parliamentary
                         ] .

:act_consolidated_file_act_consolidated
        a                   owl:DatatypeProperty ;
        rdfs:comment        "DEPRECATED, Consleg file. Logical grouping" ;
        rdfs:domain         :act_consolidated ;
        rdfs:label          "Consolidated act file" ;
        rdfs:range          xsd:string ;
        rdfs:subPropertyOf  :file_act_consolidated ;
        owl:deprecated      true .

:work_is_another_publication_of_work
        a                   owl:SymmetricProperty , owl:ObjectProperty ;
        rdfs:comment        "The work in its entirety is another publication of another work. Meant for cases where one work is republished entirely elsewhere, but where for some reasons those two works should not be considered identical" ;
        rdfs:domain         :work ;
        rdfs:label          "Work is another publication of another work" ;
        rdfs:range          :work ;
        rdfs:subPropertyOf  :is_another_publication_of .

:measure_national_implementing_page_official_journal
        a                   owl:DatatypeProperty ;
        rdfs:comment        "Page in the national or regional official journal on which this NIM was published" ;
        rdfs:domain         :measure_national_implementing ;
        rdfs:label          "Page in the national or regional Official Journal" ;
        rdfs:range          xsd:string ;
        rdfs:subPropertyOf  :page_official_journal .

:opinion_advocate-general
        a                owl:Class ;
        rdfs:comment     "Opinion of the advocate general in sector 6 (6CC/6TC). Currently encoded by table FD" ;
        rdfs:label       "Opinion of advocate general" ;
        rdfs:subClassOf  :case-law .

:multilanguage  a            owl:Class ;
        rdfs:label           "Multilanguage" ;
        rdfs:subClassOf      skos:Concept ;
        owl:equivalentClass  [ a               owl:Restriction ;
                               owl:hasValue    <http://publications.europa.eu/resource/authority/multilingual> ;
                               owl:onProperty  skos:inScheme
                             ] .

:summary_case-law_id_celex
        a                   owl:DatatypeProperty ;
        rdfs:comment        "Identifier for the summary of case law (build on Celex identifier followed by _SOM)" ;
        rdfs:domain         :summary_case-law ;
        rdfs:label          "Identifier for case law" ;
        rdfs:range          xsd:string ;
        rdfs:subPropertyOf  :id_celex .

:concept_decoding  a     owl:Class ;
        rdfs:comment     "Concept standing as a placeholder for skos:Concepts used for decoding texts" ;
        rdfs:label       "Decoding concept" ;
        rdfs:subClassOf  :concept .

:resolution_other_ep_reported_by_person
        a                   owl:ObjectProperty ;
        rdfs:comment        "Name of the person (EP member or member of CoR or EESC) who reports on the relevant act. This property will be deprecated and replaced with work_reported_by_person. Role RAPP. Relevant for legal analysis: true" ;
        rdfs:domain         :resolution_other_ep ;
        rdfs:label          "European Parliament other resolution has rapporteur" ;
        rdfs:range          :person ;
        rdfs:subPropertyOf  :reported_by ;
        dct:created         "2018-07-16T13:21:52.971+02:00"^^xsd:dateTime ;
        owl:inverseOf       :person_reports_on_resolution_other_ep .

:concept_eurovoc_subject_of_dossier
        a                   owl:ObjectProperty ;
        rdfs:domain         :concept_eurovoc ;
        rdfs:label          "Eurovoc concept is subject of a dossier" ;
        rdfs:range          :dossier ;
        rdfs:subPropertyOf  :subject_of ;
        owl:inverseOf       :dossier_is_about_concept_eurovoc .

:expression_title_alternative
        a                   owl:DatatypeProperty ;
        rdfs:comment        "Any alternative title(s) that this expression might have (obsolete titles, ...). Relevant for legal analysis: true." ;
        rdfs:domain         :expression ;
        rdfs:label          "Alternative title" ;
        rdfs:range          rdfs:Literal ;
        rdfs:subPropertyOf  :title_alternative .

:published  a       owl:DatatypeProperty ;
        rdfs:label  "Published" .

:reference_internal  a  owl:DatatypeProperty ;
        rdfs:label  "Reference internal" .

<http://publications.europa.eu/resource/authority/corporate-body/ECSC>
        a       owl:NamedIndividual .

:work_cited_by_work  a      owl:ObjectProperty ;
        rdfs:comment        "Relevant for legal analysis: true. The work is cited by another work. Relevant for legal analysis: true" ;
        rdfs:domain         :work ;
        rdfs:label          "Work cited by work" ;
        rdfs:range          :work ;
        rdfs:subPropertyOf  :cited_by ;
        owl:inverseOf       :work_cites_work .

:initiates  a       owl:ObjectProperty ;
        rdfs:label  "Initiates" .

:assessment_impact_ec
        a                owl:Class ;
        rdfs:label       "European Commission Impact Assessment" ;
        rdfs:subClassOf  :staff-working-document_ec .

:publication_frequency_is_frequency_of_work_dataset
        a              owl:ObjectProperty ;
        rdfs:domain    :publication_frequency ;
        rdfs:label     "Publication frequency is frequency of work dataset" ;
        rdfs:range     :work_dataset ;
        owl:inverseOf  :work_dataset_has_frequency_publication_frequency .

:manifestation_distribution_title
        a                   owl:DatatypeProperty ;
        rdfs:comment        "Distribution title" ;
        rdfs:domain         :manifestation_distribution ;
        rdfs:label          "Distribution title" ;
        rdfs:range          xsd:string ;
        rdfs:subPropertyOf  :title .

<http://publications.europa.eu/resource/authority/procjur>
        a       owl:NamedIndividual .

:date_adopted  a    owl:DatatypeProperty ;
        rdfs:label  "Date adopted" .

:expression_corrected_by_expression
        a                   owl:ObjectProperty ;
        rdfs:comment        "Expression corrected by another expression (e.g. in the case of language-specific corrigenda). Relevant for legal analysis: true." ;
        rdfs:domain         :expression ;
        rdfs:label          "Expression corrected by another expression" ;
        rdfs:range          :expression ;
        rdfs:subPropertyOf  :corrected_by ;
        owl:inverseOf       :expression_corrects_expression .

:work_contributed_to_by_agent
        a                   owl:ObjectProperty ;
        rdfs:comment        "The work is contributed to by an agent" ;
        rdfs:domain         :work ;
        rdfs:label          "Work is contributed to by agent" ;
        rdfs:range          :agent ;
        rdfs:subPropertyOf  :contributed_to_by ;
        owl:inverseOf       :agent_contributes_work .

:resource_legal_ep_opinion_contained_in_resource_legal
        a                   owl:ObjectProperty ;
        rdfs:comment        "8028 cases (2010-07-27). Relevant for legal analysis: true." ;
        rdfs:domain         :resource_legal ;
        rdfs:label          "European Parliament opinion on legal resource contained in legal resource" ;
        rdfs:range          :resource_legal ;
        rdfs:subPropertyOf  :ep_opinion_contained_in ;
        owl:inverseOf       :resource_legal_contains_ep_opinion_on_resource_legal .

:expression_case-law  a  owl:Class ;
        rdfs:comment     "Expression with specific elements to a case law element" ;
        rdfs:label       "Expression for a case law document" ;
        rdfs:subClassOf  :expression ;
        rdfs:subClassOf  [ a                   owl:Restriction ;
                           owl:maxCardinality  "1"^^xsd:nonNegativeInteger ;
                           owl:onProperty      :expression_case-law_source_ruling_preliminary
                         ] ;
        rdfs:subClassOf  [ a                   owl:Restriction ;
                           owl:maxCardinality  "1"^^xsd:nonNegativeInteger ;
                           owl:onProperty      :expression_case-law_procedure_language
                         ] ;
        rdfs:subClassOf  [ a                   owl:Restriction ;
                           owl:maxCardinality  "1"^^xsd:nonNegativeInteger ;
                           owl:onProperty      :expression_case-law_parties
                         ] ;
        rdfs:subClassOf  [ a                   owl:Restriction ;
                           owl:maxCardinality  "1"^^xsd:nonNegativeInteger ;
                           owl:onProperty      :expression_case-law_indicator_decision
                         ] ;
        rdfs:subClassOf  [ a                   owl:Restriction ;
                           owl:maxCardinality  "1"^^xsd:nonNegativeInteger ;
                           owl:onProperty      :expression_case-law_identifier_case
                         ] .

:manifestation_print  a  owl:Class ;
        rdfs:label       "Print manifestation" ;
        rdfs:subClassOf  :manifestation ;
        rdfs:subClassOf  [ a                   owl:Restriction ;
                           owl:maxCardinality  "1"^^xsd:nonNegativeInteger ;
                           owl:onProperty      :manifestation_print_volume
                         ] ;
        rdfs:subClassOf  [ a                   owl:Restriction ;
                           owl:maxCardinality  "1"^^xsd:nonNegativeInteger ;
                           owl:onProperty      :manifestation_print_pages_total
                         ] ;
        rdfs:subClassOf  [ a                   owl:Restriction ;
                           owl:maxCardinality  "1"^^xsd:nonNegativeInteger ;
                           owl:onProperty      :manifestation_print_page_last
                         ] ;
        rdfs:subClassOf  [ a                   owl:Restriction ;
                           owl:maxCardinality  "1"^^xsd:nonNegativeInteger ;
                           owl:onProperty      :manifestation_print_page_first
                         ] .

:language_used_by_table_of_contents_expression
        a                   owl:ObjectProperty ;
        rdfs:comment        "A given language is used for the table of contents of an expression (typically of a general publication)" ;
        rdfs:domain         :language ;
        rdfs:label          "Language used by table of contents expression" ;
        rdfs:range          :expression ;
        rdfs:subPropertyOf  :used_by_table_of_contents .

<http://publications.europa.eu/resource/authority/fd_345>
        a       owl:NamedIndividual .

:act_consolidated_file
        a                   owl:DatatypeProperty ;
        rdfs:comment        "DEPRECATED, Consleg file. Logical grouping" ;
        rdfs:domain         :act_consolidated ;
        rdfs:label          "Consolidated act file" ;
        rdfs:range          xsd:string ;
        rdfs:subPropertyOf  :file ;
        owl:deprecated      true .

:edited_by  a       owl:ObjectProperty ;
        rdfs:label  "Edited by" .

:event_case_has_result_concept_case_event_result
        a                   owl:ObjectProperty ;
        rdfs:comment        "Case event has a result" ;
        rdfs:domain         :event_case ;
        rdfs:label          "Case event has a result" ;
        rdfs:range          :concept_case_event_result ;
        rdfs:subPropertyOf  :has_result .

:manifestation-mobile-app_version
        a                   owl:DatatypeProperty ;
        rdfs:comment        "Current version of the mobile application" ;
        rdfs:domain         :manifestation-mobile-app ;
        rdfs:label          "Mobile application version" ;
        rdfs:range          xsd:string ;
        rdfs:subPropertyOf  :version ;
        dct:created         "2022-09-11T12:34:56.789"^^xsd:dateTime .

:resource_legal_procedure_comment
        a                   owl:DatatypeProperty ;
        rdfs:comment        "Comment on the corresponding legal procedure. Obsolete, only maintained for backwards compatibility. Relevant for legal analysis: true." ;
        rdfs:domain         :resource_legal ;
        rdfs:label          "Legal procedure comment" ;
        rdfs:range          xsd:string ;
        rdfs:subPropertyOf  :procedure_comment .

:session_date_start  a  owl:DatatypeProperty ;
        rdfs:label  "Session date start" .

:summary_legislation_eu_id_doc_summarized
        a                   owl:DatatypeProperty ;
        rdfs:comment        "Natural number of document summarized" ;
        rdfs:domain         :summary_legislation_eu ;
        rdfs:label          "Natural number of document summarized (basic or modifying)" ;
        rdfs:range          xsd:string ;
        rdfs:subPropertyOf  :id_doc_summarized .

:manifestation_special-official-journal_part_page_last
        a                   owl:DatatypeProperty ;
        rdfs:comment        "DEPRECATED, Last page number of the SE part related to a legal resource. Use manifestion_print_page_last" ;
        rdfs:domain         :manifestation_special-official-journal_part ;
        rdfs:label          "Last page" ;
        rdfs:range          xsd:string ;
        rdfs:subPropertyOf  :page_last , :manifestation_print_page_last ;
        owl:deprecated      true .

:concept_treaty  a           owl:Class ;
        rdfs:comment         "Concept used for a treaty. The value of the field is taken from the treaty authority table" ;
        rdfs:label           "Treaty concept" ;
        rdfs:subClassOf      skos:Concept , :concept ;
        owl:equivalentClass  [ a               owl:Restriction ;
                               owl:hasValue    <http://publications.europa.eu/resource/authority/treaty> ;
                               owl:onProperty  skos:inScheme
                             ] .

:section_legal_part_of_work
        a                   owl:ObjectProperty ;
        rdfs:comment        "This property associates an instance of a work with an instance of a section_legal that forms part of it." ;
        rdfs:domain         :section_legal ;
        rdfs:label          "Section (legal) part of work" ;
        rdfs:range          :work ;
        rdfs:subPropertyOf  :subdivision_part_of_work , :part_of ;
        owl:inverseOf       :work_contains_section_legal .

:concept_agenda_council_subject_of_event_legal
        a                   owl:ObjectProperty ;
        rdfs:comment        "Now coded with table 600" ;
        rdfs:domain         :concept_agenda_council ;
        rdfs:label          "Agenda concept is subject of a legal event" ;
        rdfs:range          :event_legal ;
        rdfs:subPropertyOf  :subject_of ;
        owl:inverseOf       :event_legal_is_about_concept_agenda_council .

:releases  a                owl:ObjectProperty ;
        rdfs:comment        "This is an intermediate subclass representing the release relation which is a specific form of making a version public." ;
        rdfs:label          "Releases" ;
        rdfs:subPropertyOf  :publishes ;
        owl:inverseOf       :released_in .

:ATTO_FD_335  a              owl:Class ;
        rdfs:label           "FD_335 ATTO table" ;
        rdfs:subClassOf      skos:Concept ;
        owl:equivalentClass  [ a               owl:Restriction ;
                               owl:hasValue    <http://publications.europa.eu/resource/authority/fd_335> ;
                               owl:onProperty  skos:inScheme
                             ] .

:court_national  a       owl:Class ;
        rdfs:comment     "National court, used esp. in the context of JURE" ;
        rdfs:label       "National court" ;
        rdfs:subClassOf  :agent ;
        rdfs:subClassOf  [ a                owl:Restriction ;
                           owl:cardinality  "1"^^xsd:nonNegativeInteger ;
                           owl:onProperty   cmr:lastModificationDate
                         ] ;
        rdfs:subClassOf  [ a                   owl:Restriction ;
                           owl:maxCardinality  "1"^^xsd:nonNegativeInteger ;
                           owl:onProperty      cmr:creationDate
                         ] ;
        rdfs:subClassOf  [ a                   owl:Restriction ;
                           owl:minCardinality  "1"^^xsd:nonNegativeInteger ;
                           owl:onProperty      :court_national_name
                         ] ;
        rdfs:subClassOf  [ a                            owl:Restriction ;
                           owl:maxQualifiedCardinality  "1"^^xsd:nonNegativeInteger ;
                           owl:onClass                  :concept_class_court_national ;
                           owl:onProperty               :court_national_has_type_concept_class_court_national
                         ] .

:manifestation_special-official-journal_part_page_first
        a                   owl:DatatypeProperty ;
        rdfs:comment        "DEPRECATED, First page number of the SE part related to a legal resource. Use manifestion_print_page_first" ;
        rdfs:domain         :manifestation_special-official-journal_part ;
        rdfs:label          "First page" ;
        rdfs:range          xsd:string ;
        rdfs:subPropertyOf  :page_first , :manifestation_print_page_first ;
        owl:deprecated      true .

:person_associated_with_event_legal
        a                   owl:ObjectProperty ;
        rdfs:comment        "DEPRECATED," ;
        rdfs:domain         :person ;
        rdfs:label          "Person is associated with legal event" ;
        rdfs:range          :event_legal ;
        rdfs:subPropertyOf  :associated_with ;
        owl:deprecated      true .

:person_hands_over_event_legal
        a                   owl:ObjectProperty ;
        rdfs:domain         :person ;
        rdfs:label          "Person hands over legal event" ;
        rdfs:range          :event_legal ;
        rdfs:subPropertyOf  :hands_over .

:eesc_opinion_contained_in
        a           owl:ObjectProperty ;
        rdfs:label  "Eesc opinion contained in" .

:joint-proposal_directive
        a                owl:Class ;
        rdfs:comment     "where its resource_legal_type = JC, resource_legal_id_sector = 5, work_has_resource-type = JOINT_PROP_DIR" ;
        rdfs:label       "Joint proposal for a directive" ;
        rdfs:subClassOf  :proposal_act , :act_preparatory_joint .

<http://publications.europa.eu/resource/authority/fd_361>
        a       owl:NamedIndividual .

:question_oral  a        owl:Class ;
        rdfs:comment     "Oral parliamentary question (= subsector O sector 9 in EUR-Lex, 2451 notices on 2010-07-27)" ;
        rdfs:label       "Oral question" ;
        rdfs:subClassOf  :question_parliamentary_with-debate .

:question_parliamentary
        a                owl:Class ;
        rdfs:comment     "Parliamentary questions (= sector 9 in EUR-Lex)" ;
        rdfs:label       "Parliamentary question" ;
        rdfs:subClassOf  :resource_legal ;
        rdfs:subClassOf  [ a                owl:Restriction ;
                           owl:cardinality  "1"^^xsd:nonNegativeInteger ;
                           owl:onProperty   :question_parliamentary_term_parliamentary
                         ] ;
        rdfs:subClassOf  [ a                   owl:Restriction ;
                           owl:maxCardinality  "1"^^xsd:nonNegativeInteger ;
                           owl:onProperty      :question_parliamentary_published
                         ] ;
        rdfs:subClassOf  [ a                   owl:Restriction ;
                           owl:maxCardinality  "1"^^xsd:nonNegativeInteger ;
                           owl:onProperty      :question_parliamentary_number_session
                         ] .

:costs_decisions  a  owl:DatatypeProperty ;
        rdfs:label  "Costs decisions" .

:manifestation-audiovisual
        a                owl:Class ;
        rdfs:comment     "Audiovisuals are a product type in the scope of General Publications. They include audiobooks." ;
        rdfs:label       "Audiovisual manifestation" ;
        rdfs:subClassOf  :manifestation-publication-general ;
        rdfs:subClassOf  [ a                            owl:Restriction ;
                           owl:maxQualifiedCardinality  "1"^^xsd:nonNegativeInteger ;
                           owl:onDataRange              xsd:duration ;
                           owl:onProperty               :manifestation-audiovisual_duration-playing-time
                         ] .

:report_joint  a         owl:Class ;
        rdfs:comment     "resource_legal_type = (JC or DC), resource_legal_id_sector = 5, work_has_resource-type = JOINT_REPORT" ;
        rdfs:label       "Joint report" ;
        rdfs:subClassOf  :act_preparatory_joint .

:procurement_public_transliterated_organisation_national-id
        a                   owl:DatatypeProperty ;
        rdfs:domain         :procurement_public ;
        rdfs:label          "Procurement public transliterated organisation national id" ;
        rdfs:range          xsd:string ;
        rdfs:subPropertyOf  :transliterated_organisation_national-id .

:treaty_basis_for_resource_legal
        a                   owl:ObjectProperty ;
        rdfs:comment        ". Relevant for legal analysis: true." ;
        rdfs:domain         :treaty ;
        rdfs:label          "Treaty is basis for legal resource" ;
        rdfs:range          :resource_legal ;
        rdfs:subPropertyOf  :basis_for .

:replaces  a        owl:ObjectProperty ;
        rdfs:label  "Replaces" .

:expression_case-law_procedure_language
        a                   owl:DatatypeProperty ;
        rdfs:comment        "Language of the procedure in the title of a case law document (language-specific)" ;
        rdfs:domain         :expression_case-law ;
        rdfs:label          "Language of procedure" ;
        rdfs:range          xsd:string ;
        rdfs:subPropertyOf  :procedure_language .

:procurement_public_cpv_original_reference
        a                   owl:DatatypeProperty ;
        rdfs:domain         :procurement_public ;
        rdfs:label          "CPV original reference" ;
        rdfs:range          xsd:anyURI ;
        rdfs:subPropertyOf  :cpv_original_reference .

:collection_document  a      owl:Class ;
        rdfs:comment         "A collection of documents. Typical examples might be the collection of documents with a Celex ID, with an ID Pub etc." ;
        rdfs:label           "Document collection" ;
        rdfs:subClassOf      :collection ;
        owl:equivalentClass  [ a               owl:Restriction ;
                               owl:hasValue    <http://publications.europa.eu/resource/authority/document-collection> ;
                               owl:onProperty  skos:inScheme
                             ] .

:work_has_number  a  owl:DatatypeProperty ;
        rdfs:domain  :work ;
        rdfs:label   "Work has number" ;
        rdfs:range   xsd:string .

:interpreted_by  a  owl:ObjectProperty ;
        rdfs:label  "Interpreted by" .

:joint-staff-working-document
        a                owl:Class ;
        rdfs:label       "Joint Staff Working document" ;
        rdfs:subClassOf  :staff-working-document , :act_preparatory_joint .

<http://publications.europa.eu/resource/authority/fd_340>
        a       owl:NamedIndividual .

:communication_cjeu_requested_by_agent
        a                   owl:ObjectProperty ;
        rdfs:comment        "This lists the applying party or party lodging the appeal in Court proceeding (institutions, bodies, Member States, companies, individuals) the communication_cjeu published in OJ informs about. Currently coded with FD_Table_110. Relevant for legal analysis: true" ;
        rdfs:domain         :communication_cjeu ;
        rdfs:label          "Communication on case law requested by agent" ;
        rdfs:range          :agent ;
        rdfs:subPropertyOf  :requested_by ;
        owl:inverseOf       :agent_requests_communication_cjeu .

<http://publications.europa.eu/resource/authority/procresult>
        a       owl:NamedIndividual .

:has_documentation  a  owl:ObjectProperty ;
        rdfs:label  "Has documentation" .

:case-law_reviews_judgement_resource_legal
        a                   owl:ObjectProperty ;
        rdfs:comment        "This property points to the Court decision quoted in the operative part of Court decisions" ;
        rdfs:domain         :case-law ;
        rdfs:label          "Case law reviews judgement" ;
        rdfs:range          :resource_legal ;
        rdfs:subPropertyOf  :reviews_judgement ;
        owl:inverseOf       :resource_legal_reviewed_by_case-law .

:is_status_of  a    owl:ObjectProperty ;
        rdfs:label  "Is status of" .

:layer  a           owl:DatatypeProperty ;
        rdfs:label  "Layer" .

:takes_over  a      owl:ObjectProperty ;
        rdfs:label  "Takes over" .

:case-law_has_conclusions_opinion_advocate-general
        a                   owl:ObjectProperty ;
        rdfs:comment        "Only in IMMC concext" ;
        rdfs:domain         :case-law ;
        rdfs:label          "Case law has conclusions" ;
        rdfs:range          :opinion_advocate-general ;
        rdfs:subPropertyOf  :has_conclusions .

:container_case-law_series
        a                   owl:DatatypeProperty ;
        rdfs:domain         :container_case-law ;
        rdfs:label          "Series of the Court report" ;
        rdfs:range          xsd:string ;
        rdfs:subPropertyOf  :series .

:manifestation_court-report_part_year
        a                   owl:DatatypeProperty ;
        rdfs:comment        "Year in which this court report was published. Temporary solution, should in the future be part of the court report object itself" ;
        rdfs:domain         :manifestation_court-report_part ;
        rdfs:label          "Year of court report" ;
        rdfs:range          xsd:string ;
        rdfs:subPropertyOf  :year .

:signatory_function  a  owl:DatatypeProperty ;
        rdfs:label  "Signatory function" .

:ATTO_FD_330  a              owl:Class ;
        rdfs:label           "FD_330 ATTO table" ;
        rdfs:subClassOf      skos:Concept ;
        owl:equivalentClass  [ a               owl:Restriction ;
                               owl:hasValue    <http://publications.europa.eu/resource/authority/fd_330> ;
                               owl:onProperty  skos:inScheme
                             ] .

:bibliography  a    owl:DatatypeProperty ;
        rdfs:label  "Bibliography" .

:unit_administrative  a  owl:Class ;
        rdfs:comment     "\"Politically defined administrative unit such as a town, a region, a country or the European Union\" (eGov Share Reference ontology). The concept of an administrative unit is linked to CIDOC CRM's http://purl.org/NET/cidoc-crm/core#E53_Place" ;
        rdfs:label       "Administrative unit" ;
        rdfs:subClassOf  [ a                            owl:Restriction ;
                           owl:maxQualifiedCardinality  "1"^^xsd:nonNegativeInteger ;
                           owl:onClass                  :unit_administrative ;
                           owl:onProperty               :unit_administrative_part_of_unit_administrative
                         ] .

:xml-schema-definition_link_title
        a           owl:DatatypeProperty ;
        rdfs:label  "Xml schema definition link title" .

:procedure_internal_has_type_consultation
        a                   owl:ObjectProperty ;
        rdfs:comment        "This internal procedure is a certain type of consultation. Table com_internal_consultation_type" ;
        rdfs:domain         :procedure_internal ;
        rdfs:label          "Internal procedure has a consultation type" ;
        rdfs:range          :type_consultation ;
        rdfs:subPropertyOf  :has ;
        owl:inverseOf       :type_consultation_is_type_of_procedure_internal .

:institution_authors-opinion_event_legal
        a                   owl:ObjectProperty ;
        rdfs:domain         :institution ;
        rdfs:label          "Institution authors opinion on legal event" ;
        rdfs:range          :event_legal ;
        rdfs:subPropertyOf  :authors-opinion .

:procedure_code_interinstitutional
        a                owl:Class ;
        rdfs:comment     "A procedure from its initiation to its conclusion. Procedures cover legislative or non-legislative procedures as defined in this data model from the initial Commission proposal to its eventual adoption and beyond. Procedures with an interinstitutional code are the typical case of procedures leading to new secondary legislation. Pegase file works with the concepts of a * Dossier (element DOSSIER having a certain TYPE_DOSSIER * Each event links to DOCUMENT(s), identified by one (or more) identifiers. Procedure types in Prelex (= procedures_general/procedure/id): || PROCEDURE_ID || LANGUE_ID || TR_PROCEDURE_CODE || TR_PROCEDURE_ABR || TR_PROCEDURE_DNM || DATE_CREATION || AUTEUR_CREATION || DATE_MODIFICATION || AUTEUR_MODIFICATION || | 10000 | 1020 | ACC | Agreement | Agreement | 11.06.98 | 2000 | 36483 | 100162 | | 1030 | 1020 | APP | Special legislative procedure (EP consent required) | Special legislative procedure (EP consent required) | 03.03.10 | 9999 | 40325 | 100162 | | 1020 | 1020 | AVC | Assent procedure | Assent procedure | 11.06.98 | 2000 | 35957 | 2000 | | 100000 | 1020 | CNB | Consultation Eur. Central Bank | Consultation of the European Central Bank | 15.05.00 | 100161 | 36929 | 100162 | | 100060 | 1020 | CNC | Consultation Court of Auditors | Consultation of the Court of Auditors | 18.07.02 | 100482 | 37456 | 100482 | | 1015 | 1020 | CNS | Special legislative procedure (EP consulted) | Special legislative procedure (EP consulted) | 11.06.98 | 2000 | 40325 | 2000 | | 1016 | 1020 | CNS_OLD* | Consultation procedure | Consultation procedure | 26.05.10 | 9999 | 40325 | 100162 | | 1010 | 1020 | COD | Ordinary legislative procedure | Ordinary legislative procedure | 11.06.98 | 2000 | 40325 | 2000 | | 1011 | 1020 | COD_OLD | Codecision procedure | Codecision procedure | 26.05.10 | 9999 | 40325 | 100162 | | 1035 | 1020 | NLE | Non-legislative procedure | Non-legislative procedure | 03.03.10 | 9999 | 40325 | 100162 | | 1025 | 1020 | PRT | Social protocol | Social protocol | 11.06.98 | 2000 | 35957 | 2000 | | 1005 | 1020 | SYN | Cooperation procedure | Cooperation procedure | 11.06.98 | 2000 | 35957 | 2000 | Dossier types in Prelex (= types_of_file/type_of_file/id, table type_of_file): || TR_TYPE_DOSSIER_ABR || TR_TYPE_DOSSIER_CODE || TR_TYPE_DOSSIER_DNM || TYPE_DOSSIER_ID || | Agreement | ACC | Agreement | 1005 | | Draft agreement | PACC | Draft agreement | 1010 | | Agreement betw. Member states | ACCEM | Agreement betw. Member states | 1015 | | Draft agreement Member States | PACCEM | Draft agreement between Member States | 1020 | | Interinstitutional Agreement | ACCIN | Interinstitutional Agreement | 1025 | | Draft interinstitut. agreement | PACCIN | Draft interinstitutional agreement | 1030 | | Joint action | ACT | Joint action | 1035 | | Draft joint action | PACT | Draft joint action | 1040 | | Opinion | AV | Opinion | 1045 | | COR own-initiative opinion | AVCR | COR own-initiative opinion | 1050 | | ESC own-initiative opinion | AVCES | ESC own-initiative opinion | 1055 | | EP own-initiative opinion | AVPE | EP own-initiative opinion | 1060 | | Request for Council Assent | DAVCS | Request for Council Assent | 1065 | | Council Assent | AVCS | Council Assent | 1070 | | Communication | CO | Communication | 1075 | | Draft communication | PCO | Draft communication | 1080 | | Decision | DC | Decision | 1085 | | Proposal for a Decision | PRDC | Proposal for a Decision | 1095 | | Draft decision | PDC | Draft decision | 1100 | | Recommendation for a Decision | RCDC | Recommendation for a Decision | 1105 | | Declaration | DCL | Declaration | 1110 | | Draft declaration | PDCL | Draft declaration | 1115 | | Directive | DI | Directive | 1120 | | Proposal for a Directive | PRDI | Proposal for a Directive | 1130 | | Draft directive | PDI | Draft directive | 1135 | | Recommendation for a Directive | RCDI | Recommendation for a Directive | 1140 | | Working Paper | DT | Commission Working Paper | 1145 | | Staff Working Paper | DTS | Commission Staff Working Paper | 1150 | | Periodic report | EP | Periodic report | 1155 | | Letter | LT | Letter | 1160 | | Green Paper | LV | Green Paper | 1165 | | White Paper | LB | White Paper | 1170 | | Memorandum | MM | Memorandum | 1175 | | Note | NT | Note | 1180 | | Draft Common Position | PPC | Draft Common Position | 1185 | | Proposal for a Common Position | PRPC | Proposal for a Common Position | 1190 | | Common position | PC | Common position | 1195 | | Programme | PRG | Programme | 1200 | | Protocol | PROT | Protocol | 1205 | | Draft protocol | PRT | Draft protocol | 1210 | | Report | RA | Report | 1215 | Recommendation | RC | Recommendation | 1220 | | Draft recommendation | PRC | Draft recommendation | 1230 | | Proposal for a Recommendation | PRRC | Proposal for a Recommendation | 1235 | Recomm. for a Recommendation | RCRC | Recommendation for a Recommendation | 1240 | | Regulation | RG | Regulation | 1245 | | Draft regulation | PRJREG | Draft regulation | 1255 | | Proposal for a Regulation | PRRG | Proposal for a Regulation | 1260 | | Recomm. for a Regulation | RERG | Recomm. for a Regulation | 1265 | | Draft resolution | PRS | Draft resolution | 1270 | | Proposal for a Resolution | PRRS | Proposal for a Resolution | 1275 | | Recommendation for Resolution | RCRS | Recommendation for a Resolution | 1280 | | Resolution of EP | RS | Resolution of EP | 1285 | | Draft Treaty | PTR | Draft Treaty | 1290 | | Treaty | TR | Treaty | 1295 | | Preliminary Draft Budget | APRB | Preliminary Draft Budget | 1300 | | Prelim. Draft supplem. Budget | APRBRS | Preliminary Draft supplementary and amending Budget | 1305 | | Draft budget | PRB | Draft budget | 1310 | | Draft suppl. and amend. budget | PRBRS | Draft supplementary and amending budget | 1315 | | Budget | B | Budget | 1320 | | Supplem. and amending Budet | BRS | Supplementary and amending Budget | 1325 | | Letter of amendment | LR | Letter of amendment | 1330 | | Draft ECSC budget | PRBCECA | Draft ECSC budget | 1335 | | ECSC Budget | BCECA | ECSC Budget | 1340 | | Transfer of appropriations | VICR | Transfer of appropriations | 1345 | | Proposal for a Declaration | PROPDECLAR | Proposal for a Declaration | 10000 | | Resolution | RES | Resolution | 20000 | | Proposal for an Act | PRACT | Proposal for an Act | 100020 | | Draft act | PROJACT | Draft act | 100040 | | Act | ACTE | Act | 100060 | | Proposal for a joint action | PROPACT | Proposal for a joint action | 100100 | | Draft proposal | PPR | Draft proposal | 100120 | | Recommendation for an Opinion | RCA | Recommendation for an Opinion | 100140 | | EESC own-initiative opinion | AVCESE | EESC own-initiative opinion | 100180 | | Proposal for a Council Framework Decision | PROPDECAD | Proposal for a Council Framework Decision | 100182 | | COUNCIL FRAMEWORK DECISION | DECAD | COUNCIL FRAMEWORK DECISION | 100183 | | Draft Council framework decision | PROJDECAD | Draft Council framework decision | 100185 |" ;
        rdfs:label       "Procedure with interinstitutional code" ;
        rdfs:subClassOf  :dossier ;
        rdfs:subClassOf  [ a                   owl:Restriction ;
                           owl:maxCardinality  "1"^^xsd:nonNegativeInteger ;
                           owl:onProperty      :procedure_code_interinstitutional_reference_procedure
                         ] ;
        rdfs:subClassOf  [ a                         owl:Restriction ;
                           owl:onClass               :concept_type_procedure_code_interinstitutional ;
                           owl:onProperty            :procedure_code_interinstitutional_has_type_concept_type_procedure_code_interinstitutional ;
                           owl:qualifiedCardinality  "1"^^xsd:nonNegativeInteger
                         ] ;
        rdfs:subClassOf  [ a                   owl:Restriction ;
                           owl:maxCardinality  "1"^^xsd:nonNegativeInteger ;
                           owl:onProperty      :procedure_code_interinstitutional_has_status
                         ] ;
        rdfs:subClassOf  [ a                owl:Restriction ;
                           owl:cardinality  "1"^^xsd:nonNegativeInteger ;
                           owl:onProperty   :procedure_code_interinstitutional_year_procedure
                         ] ;
        rdfs:subClassOf  [ a                owl:Restriction ;
                           owl:cardinality  "1"^^xsd:nonNegativeInteger ;
                           owl:onProperty   :procedure_code_interinstitutional_number_procedure
                         ] ;
        rdfs:subClassOf  [ a                   owl:Restriction ;
                           owl:maxCardinality  "1"^^xsd:nonNegativeInteger ;
                           owl:onProperty      :procedure_code_interinstitutional_european_union_competence_type
                         ] .

:has_remark  a      owl:ObjectProperty ;
        rdfs:label  "Has remark" .

:case-law_immediately_enforces_resource_legal
        a                   owl:ObjectProperty ;
        rdfs:comment        "This property points to legal act quoted in the operative part of Court decisions." ;
        rdfs:domain         :case-law ;
        rdfs:label          "Case law suspends immediately enforces legal resource" ;
        rdfs:range          :resource_legal ;
        rdfs:subPropertyOf  :immediately_enforces ;
        owl:inverseOf       :resource_legal_immediately_enforced_by_case-law .

:directive_delegated  a  owl:Class ;
        rdfs:comment     "0 Delegated directives (DTS=3 AND FM=DIRDEL)" ;
        rdfs:label       "Delegated directive" ;
        rdfs:subClassOf  :legislation_secondary .

:act_other_oj_c  a       owl:Class ;
        rdfs:comment     "Other acts published in Official Journal C series (= subsector Y of sector 4)" ;
        rdfs:label       "Other acts in OJ C" ;
        rdfs:subClassOf  :legislation_complementary .

:publication_general_number_contract
        a                   owl:DatatypeProperty ;
        rdfs:comment        "Contract number under which this general publication was elaborated" ;
        rdfs:domain         :publication_general ;
        rdfs:label          "Contract number" ;
        rdfs:range          xsd:string ;
        rdfs:subPropertyOf  :number_contract .

:case-law  a             owl:Class ;
        rdfs:comment     "\"Real\" case law in sector 6 (= a subset of the complete sector 6) and sector 8. Changed to subclass of: resource_legal. Case law of the Court of Justice also inherits from document_cjeu Remarks: * case-law_XXX_resource_legal can all be seen as sub-properties of a generic \"affects\" property * These fields by and large correspond to the specific fields of the VOLET_CDJ * NOMUSUEL and NOMUSUEL_XX: Appears as title in the corresponding expression" ;
        rdfs:label       "Case law" ;
        rdfs:subClassOf  :resource_legal ;
        rdfs:subClassOf  [ a                            owl:Restriction ;
                           owl:maxQualifiedCardinality  "1"^^xsd:nonNegativeInteger ;
                           owl:onClass                  :court_national ;
                           owl:onProperty               :case-law_delivered_by_court_national
                         ] ;
        rdfs:subClassOf  [ a                   owl:Restriction ;
                           owl:maxCardinality  "1"^^xsd:nonNegativeInteger ;
                           owl:onProperty      :case-law_source_ruling_preliminary
                         ] ;
        rdfs:subClassOf  [ a                   owl:Restriction ;
                           owl:maxCardinality  "1"^^xsd:nonNegativeInteger ;
                           owl:onProperty      :case-law_national-judgement
                         ] ;
        rdfs:subClassOf  [ a                            owl:Restriction ;
                           owl:maxQualifiedCardinality  "1"^^xsd:nonNegativeInteger ;
                           owl:onClass                  :court-formation ;
                           owl:onProperty               :case-law_delivered_by_court-formation
                         ] ;
        rdfs:subClassOf  [ a                   owl:Restriction ;
                           owl:maxCardinality  "1"^^xsd:nonNegativeInteger ;
                           owl:onProperty      :case-law_ecli
                         ] ;
        rdfs:subClassOf  [ a                            owl:Restriction ;
                           owl:maxQualifiedCardinality  "1"^^xsd:nonNegativeInteger ;
                           owl:onClass                  :judge ;
                           owl:onProperty               :case-law_delivered_by_judge
                         ] ;
        rdfs:subClassOf  [ a                   owl:Restriction ;
                           owl:maxCardinality  "1"^^xsd:nonNegativeInteger ;
                           owl:onProperty      :case-law_judgement_national
                         ] ;
        rdfs:subClassOf  [ a                            owl:Restriction ;
                           owl:maxQualifiedCardinality  "1"^^xsd:nonNegativeInteger ;
                           owl:onClass                  :institution ;
                           owl:onProperty               :case-law_delivered_by_institution
                         ] ;
        rdfs:subClassOf  [ a                   owl:Restriction ;
                           owl:maxCardinality  "1"^^xsd:nonNegativeInteger ;
                           owl:onProperty      :case-law_published_in_erecueil
                         ] .

:organization  a          owl:Class ;
        rdfs:comment      "Organization (typically private)" ;
        rdfs:label        "Organization" ;
        rdfs:subClassOf   :agent ;
        rdfs:subClassOf   [ a                owl:Restriction ;
                            owl:cardinality  "1"^^xsd:nonNegativeInteger ;
                            owl:onProperty   cmr:lastModificationDate
                          ] ;
        rdfs:subClassOf   [ a                   owl:Restriction ;
                            owl:maxCardinality  "1"^^xsd:nonNegativeInteger ;
                            owl:onProperty      cmr:creationDate
                          ] ;
        owl:disjointWith  :person .

:work_complex_work_group_id
        a                   owl:DatatypeProperty ;
        rdfs:comment        "common property to all works related directly or indirectly to a complex work instance" ;
        rdfs:domain         :work ;
        rdfs:label          "Complex work group id" ;
        rdfs:range          xsd:string ;
        rdfs:subPropertyOf  :complex_work_group_id .

:concept_cpv  a          owl:Class ;
        rdfs:comment     "Table to create" ;
        rdfs:label       "Concept representing a CPV code in Ted" ;
        rdfs:subClassOf  :concept .

:event_legal_addresses_institution
        a                   owl:ObjectProperty ;
        rdfs:comment        "DEPRECATED, This legal event addresses a given institution. Body role: Addressee. Relevant for legal analysis: true." ;
        rdfs:domain         :event_legal ;
        rdfs:label          "Legal event addresses institution" ;
        rdfs:range          :institution ;
        rdfs:subPropertyOf  :event_addresses_institution , :addresses ;
        owl:deprecated      true ;
        owl:inverseOf       :institution_addressed_by_event_legal .

:indent  a               owl:Class ;
        rdfs:label       "Indent" ;
        rdfs:subClassOf  :subdivision .

:section  a         owl:DatatypeProperty ;
        rdfs:label  "Section" .

:concept_type_event  a       owl:Class ;
        rdfs:comment         "Corresponds to the contents authority table event (http://publications.europa.eu/resource/authority/event)" ;
        rdfs:label           "Concept representing the type of an event" ;
        rdfs:subClassOf      skos:Concept , :concept_decoding ;
        owl:disjointUnionOf  ( :type_event_interinstitutional :type_event_internal ) .

:white-paper_joint  a    owl:Class ;
        rdfs:label       "Joint White Paper" ;
        rdfs:subClassOf  :act_preparatory_joint .

:work_date_creation_legacy
        a                   owl:DatatypeProperty ;
        rdfs:comment        "Legacy date of creation. Relevant for legal analysis: true. Procat and Pegase legacy creation dates. Relevant for legal analysis: true." ;
        rdfs:domain         :work ;
        rdfs:label          "Legacy date of creation of work" ;
        rdfs:range          xsd:date ;
        rdfs:subPropertyOf  :date_creation_legacy .

:regulation_code  a  owl:DatatypeProperty ;
        rdfs:label  "Regulation code" .

:resource_legal_tackles_similar_question_as_resource_legal
        a                   owl:SymmetricProperty , owl:ObjectProperty ;
        rdfs:comment        "Relevant for legal analysis: true" ;
        rdfs:domain         :resource_legal ;
        rdfs:label          "Legal resource tackles similar question as legal resource" ;
        rdfs:range          :resource_legal ;
        rdfs:subPropertyOf  :tackles_similar_question_as .

:institution_mandatorily-consulted_by_event_legal
        a                   owl:ObjectProperty ;
        rdfs:comment        "An institution is mandatorily consulted in the scope of a legal event" ;
        rdfs:domain         :institution ;
        rdfs:label          "Institution mandatorily consulted by legal event" ;
        rdfs:range          :event_legal ;
        rdfs:subPropertyOf  :mandatorily-consulted_by .

:initiated_by  a    owl:ObjectProperty ;
        rdfs:label  "Initiated by" .

:procurement_public_official-forms_link_type
        a                   owl:DatatypeProperty ;
        rdfs:domain         :procurement_public ;
        rdfs:label          "Link type for the official forms" ;
        rdfs:range          xsd:string ;
        rdfs:subPropertyOf  :official-forms_link_type .

:manifestation_case-law_subject
        a                   owl:DatatypeProperty ;
        rdfs:comment        "Free text subject associated with this judgement. Sector 6 Text Index Field I2" ;
        rdfs:domain         :manifestation_case-law ;
        rdfs:label          "Subject for court decision" ;
        rdfs:range          rdf:XMLLiteral ;
        rdfs:subPropertyOf  :subject .

:official-journal_publishes_resource_legal
        a                   owl:ObjectProperty ;
        rdfs:comment        "No longer 1..* as this property is inferred in many circumstances" ;
        rdfs:domain         :official-journal ;
        rdfs:label          "Official journal publishes a legal resource" ;
        rdfs:range          :resource_legal ;
        rdfs:subPropertyOf  :publishes ;
        owl:inverseOf       :resource_legal_published_in_official-journal .

:nuts_original_link_type
        a           owl:DatatypeProperty ;
        rdfs:label  "Nuts original link type" .

:event_responsibility_of_institution
        a                   owl:ObjectProperty ;
        rdfs:comment        "A given institution is primarily responsible for this event. Relevant for legal analysis: true." ;
        rdfs:domain         :event ;
        rdfs:label          "Event under responsibility of an institution" ;
        rdfs:range          :institution ;
        rdfs:subPropertyOf  :responsibility_of ;
        owl:inverseOf       :institution_responsible_for_event .

:resource_legal_id_local
        a                   owl:DatatypeProperty ;
        rdfs:comment        "Identifier that this legal resource in some other reference system, e.g. in the member states. Does not at present exist in EUR-lex" ;
        rdfs:domain         :resource_legal ;
        rdfs:label          "Local identifier" ;
        rdfs:range          xsd:string ;
        rdfs:subPropertyOf  :id_local .

:communication_case_new_requests_partial_annulment_of_resource_legal
        a                   owl:ObjectProperty ;
        rdfs:comment        "This property points to legal act quoted in the communication on a new case published in OJ. Relevant for legal analysis: true" ;
        rdfs:domain         :communication_case_new ;
        rdfs:label          "Communication requests partial annulment of legal resource" ;
        rdfs:range          :resource_legal ;
        rdfs:subPropertyOf  :requests_partial_annulment_of ;
        owl:inverseOf       :resource_legal_partial_annulment_requested_by_communication_case_new .

:agent_jointly-responsible_for_resource_legal
        a              owl:ObjectProperty ;
        rdfs:comment   "Agent is responsible for a legal resource together with other agent(s)" ;
        rdfs:domain    :agent ;
        rdfs:label     "Agent jointly responsible for a legal resource" ;
        rdfs:range     :resource_legal ;
        owl:inverseOf  :resource_legal_joint-responsibility_of_agent .

:work_cites_work  a         owl:ObjectProperty ;
        rdfs:comment        "Relevant for legal analysis: true." ;
        rdfs:domain         :work ;
        rdfs:label          "Work cites work. CI / CJ" ;
        rdfs:range          :work ;
        rdfs:subPropertyOf  :cites ;
        owl:inverseOf       :work_cited_by_work .

:resource_legal_published_in_official-journal
        a                   owl:ObjectProperty ;
        rdfs:comment        "The legal resource is published in a given official journal. OJ_PUB and subfields NO_OJ NO_OJ_CLASS COLL_OJ YEAR_PUB PAGE_FIRST PAGE_LAST are exposed as annotations of this link between the legal resource and the official journal" ;
        rdfs:domain         :resource_legal ;
        rdfs:label          "Legal resource published in official journal" ;
        rdfs:range          :official-journal ;
        rdfs:subPropertyOf  :published_in ;
        owl:inverseOf       :official-journal_publishes_resource_legal .

:period_located_in_unit_administrative
        a                   owl:ObjectProperty ;
        rdfs:comment        "The period takes place in a given administrative unit (related to CIDOC CRM's P7 P7 took place at (witnessed): E53 Place" ;
        rdfs:domain         :period ;
        rdfs:label          "Period is located in administrative unit" ;
        rdfs:range          :unit_administrative ;
        rdfs:subPropertyOf  :located_in ;
        owl:inverseOf       :unit_administrative_location_for_period .

:resource_legal_interpreted_by_case-law
        a                   owl:ObjectProperty ;
        rdfs:comment        "Calculated. Relevant for legal analysis: true." ;
        rdfs:domain         :resource_legal ;
        rdfs:label          "Legal resource interpreted by case law" ;
        rdfs:range          :case-law ;
        rdfs:subPropertyOf  :interpreted_by ;
        owl:inverseOf       :case-law_interpretes_resource_legal .

:procurement_public_number_edition
        a                   owl:DatatypeProperty ;
        rdfs:comment        "The OJ edition to which the procurement notice belongs to. It will contain a compound of year + number-zero-padded-3-digit (e.g. 2019023) representing the year and the number of the OJ edition" ;
        rdfs:domain         :procurement_public ;
        rdfs:label          "Number edition" ;
        rdfs:range          xsd:positiveInteger ;
        rdfs:subPropertyOf  :number_edition .

:number_sequence_celex
        a           owl:DatatypeProperty ;
        rdfs:label  "Number sequence celex" .

:year   a           owl:DatatypeProperty ;
        rdfs:label  "Year" .

:resource_legal_in-force
        a                   owl:DatatypeProperty ;
        rdfs:comment        "Is this legal resource currently in force? Could be calculated based on end of validity date. Relevant for legal analysis: true" ;
        rdfs:domain         :resource_legal ;
        rdfs:label          "In force?" ;
        rdfs:range          xsd:boolean ;
        rdfs:subPropertyOf  :in-force .

:agent_depositary_for_treaty
        a                   owl:ObjectProperty ;
        rdfs:comment        "Agent (e.g. World Trade Organisation - Director-General) is depositary for a treaty" ;
        rdfs:domain         :agent ;
        rdfs:label          "Agent is depositary for treaty" ;
        rdfs:range          :treaty ;
        rdfs:subPropertyOf  :depositary_for ;
        owl:inverseOf       :treaty_stored_by_agent .

:procurement_public_datetime_submission
        a                   owl:DatatypeProperty ;
        rdfs:domain         :procurement_public ;
        rdfs:label          "Submission date" ;
        rdfs:range          xsd:dateTime ;
        rdfs:subPropertyOf  :datetime_submission .

:natural_number  a  owl:DatatypeProperty ;
        rdfs:label  "Natural number" .

:archive_package_eesc
        a                owl:Class ;
        rdfs:comment     "An archive package of internal/official documents of the EESC in the scope of their contribution to legislative procedures. Besides the manifestation representing the digitised \"folder\" of documents for a given legislative procedure the package also contains metadata referring to the contained singular documents which however are not represented by their own manifestations, but only as metadata." ;
        rdfs:label       "Archive package from the European Economic and Social Committee digitisation projects" ;
        rdfs:subClassOf  :archive_package , :act_preparatory_eesc ;
        dct:created      "2022-09-01T09:01:22"^^xsd:dateTime .

:has_type_procedure  a  owl:ObjectProperty ;
        rdfs:label  "Has type procedure" .

<http://publications.europa.eu/resource/authority/fd_606>
        a       owl:NamedIndividual .

:manifestation_special-official-journal-act_is_about_concept_directory-code
        a                   owl:ObjectProperty ;
        rdfs:comment        "Manifestation of a Special Official Journal act has as subject a concept from legal directory" ;
        rdfs:domain         :manifestation_special-official-journal-act ;
        rdfs:label          "Manifestation Special Official Journal act is about concept directory-code" ;
        rdfs:range          :concept_directory-code ;
        rdfs:subPropertyOf  :is_about ;
        owl:inverseOf       :concept_directory-code_subject_of_manifestation_special-official-journal-act .

:manifested_by  a   owl:ObjectProperty ;
        rdfs:label  "Manifested by" .

:citation_part_of_work
        a                   owl:ObjectProperty ;
        rdfs:comment        "This property associates an instance of a work with an instance of a citation that forms part of it." ;
        rdfs:domain         :citation ;
        rdfs:label          "Citation part of work" ;
        rdfs:range          :work ;
        rdfs:subPropertyOf  :subdivision_part_of_work , :part_of ;
        owl:inverseOf       :work_contains_citation .

:dimension_belongs_to_manifestation
        a           owl:ObjectProperty ;
        rdfs:label  "Dimension belongs to manifestation" .

:question_parliamentary_term_parliamentary
        a                   owl:DatatypeProperty ;
        rdfs:comment        "This indicates the Parliamentary term during which an EP document was voted or EP question was raised. Relevant for legal analysis: true. Currently coded with FD_Table 285. However, only codes are exposed (not decoded), so 01, 02 etc." ;
        rdfs:domain         :question_parliamentary ;
        rdfs:label          "Parliamentary term" ;
        rdfs:range          xsd:string ;
        rdfs:subPropertyOf  :term_parliamentary , :act_preparatory_term_parliamentary .

:amended_by  a      owl:ObjectProperty ;
        rdfs:label  "Amended by" .

:produced_by  a     owl:ObjectProperty ;
        rdfs:label  "Produced by" .

:manifestation_print_reference_page_last
        a                   owl:DatatypeProperty ;
        rdfs:comment        "DEPRECATED, Last page number of the OJ part related to a legal resource. Use manifestion_print_page_last" ;
        rdfs:domain         :manifestation_print_reference ;
        rdfs:label          "Last page" ;
        rdfs:range          xsd:string ;
        rdfs:subPropertyOf  :page_last , :manifestation_print_page_last ;
        owl:deprecated      true .

:resource_legal_procedure_year
        a                   owl:DatatypeProperty ;
        rdfs:comment        "Year of the corresponding legal procedure Obsolete, only maintained for backwards compatibility. Relevant for legal analysis: true" ;
        rdfs:domain         :resource_legal ;
        rdfs:label          "Legal procedure year" ;
        rdfs:range          xsd:gYear ;
        rdfs:subPropertyOf  :procedure_year .

:manifestation-mobile-app_has-status_dissemination-status
        a                   owl:ObjectProperty ;
        rdfs:comment        "This property refers to the dissemination status of a mobile application. Based on 008 position 6." ;
        rdfs:domain         :manifestation-mobile-app ;
        rdfs:label          "Mobile application has dissemination status" ;
        rdfs:range          :dissemination-status ;
        rdfs:subPropertyOf  :has_status ;
        dct:created         "2022-08-01T16:18:31.50"^^xsd:dateTime ;
        owl:inverseOf       :dissemination-status_is-status-of_manifestation-mobile-app .

:pricing_info  a             owl:Class ;
        rdfs:comment         "price info of a manifestation" ;
        rdfs:label           "Pricing info" ;
        rdfs:subClassOf      skos:Concept , :concept ;
        owl:equivalentClass  [ a               owl:Restriction ;
                               owl:hasValue    <http://publications.europa.eu/resource/authority/pub_div> ;
                               owl:onProperty  skos:inScheme
                             ] .

:case-law_national_follow-up
        a                   owl:DatatypeProperty ;
        rdfs:comment        "Follow up to the case by the national Court" ;
        rdfs:domain         :case-law_national ;
        rdfs:label          "Follow up by the national Court" ;
        rdfs:range          rdf:XMLLiteral ;
        rdfs:subPropertyOf  :follow-up .

:procurement_public_directive_number
        a                   owl:DatatypeProperty ;
        rdfs:domain         :procurement_public ;
        rdfs:label          "Directive number" ;
        rdfs:range          xsd:string ;
        rdfs:subPropertyOf  :directive_number .

:related_to  a      owl:SymmetricProperty , owl:ObjectProperty ;
        rdfs:label  "Related to" .

:person_drafts_event_legal
        a                   owl:ObjectProperty ;
        rdfs:domain         :person ;
        rdfs:label          "Person drafts legal event" ;
        rdfs:range          :event_legal ;
        rdfs:subPropertyOf  :drafts .

:has_joined_decisions
        a           owl:ObjectProperty ;
        rdfs:label  "Has joined decisions" .

:act_preparatory_ep  a   owl:Class ;
        rdfs:comment     "Preparatory act by the European Parliament" ;
        rdfs:label       "Preparatory act by EP" ;
        rdfs:subClassOf  :act_preparatory ;
        rdfs:subClassOf  [ a               owl:Restriction ;
                           owl:hasValue    <http://publications.europa.eu/resource/authority/corporate-body/EP> ;
                           owl:onProperty  :work_created_by_agent
                         ] .

:regulation_label  a  owl:DatatypeProperty ;
        rdfs:label  "Regulation label" .

:reestablished_by  a  owl:ObjectProperty ;
        rdfs:label  "Reestablished by" .

:event_legal_uses_concept_type_decision
        a                   owl:ObjectProperty ;
        rdfs:comment        "Change from the type_decision data property. Decision. Relevant for legal analysis: true." ;
        rdfs:domain         :event_legal ;
        rdfs:label          "The event uses a given decision type" ;
        rdfs:range          :concept_type_decision ;
        rdfs:subPropertyOf  :uses .

:delivered_by  a    owl:ObjectProperty ;
        rdfs:label  "Delivered by" .

:official_journal  a  owl:DatatypeProperty ;
        rdfs:label  "Official journal" .

:official-journal-act
        a                owl:Class ;
        rdfs:comment     "This class establishes the Official Journal in its act-by-act publication form; it holds all properties that represent an OJ act, including corrigenda to those. I.e. the properties from which the identification is built have to be represented. In order to hold the business specific aspects of a legal act, the objects having this class here will also be typed as cdm#resource_legal" ;
        rdfs:label       "Official Journal act" ;
        rdfs:subClassOf  :work ;
        rdfs:subClassOf  [ a                   owl:Restriction ;
                           owl:maxCardinality  "1"^^xsd:nonNegativeInteger ;
                           owl:onProperty      :official-journal-act_subsubsection_oj
                         ] ;
        rdfs:subClassOf  [ a                   owl:Restriction ;
                           owl:maxCardinality  "1"^^xsd:nonNegativeInteger ;
                           owl:onProperty      :official-journal-act_subsection_oj
                         ] ;
        rdfs:subClassOf  [ a                owl:Restriction ;
                           owl:cardinality  "1"^^xsd:nonNegativeInteger ;
                           owl:onProperty   :official-journal-act_number
                         ] ;
        rdfs:subClassOf  [ a                owl:Restriction ;
                           owl:cardinality  "1"^^xsd:nonNegativeInteger ;
                           owl:onProperty   :official-journal-act_part_of_collection_document
                         ] ;
        rdfs:subClassOf  [ a                   owl:Restriction ;
                           owl:maxCardinality  "1"^^xsd:nonNegativeInteger ;
                           owl:onProperty      :official-journal-act_durability
                         ] ;
        rdfs:subClassOf  [ a                   owl:Restriction ;
                           owl:maxCardinality  "1"^^xsd:nonNegativeInteger ;
                           owl:onProperty      :official-journal-act_section_oj
                         ] ;
        rdfs:subClassOf  [ a                owl:Restriction ;
                           owl:cardinality  "1"^^xsd:nonNegativeInteger ;
                           owl:onProperty   :official-journal-act_date_publication
                         ] ;
        rdfs:subClassOf  [ a                owl:Restriction ;
                           owl:cardinality  "1"^^xsd:nonNegativeInteger ;
                           owl:onProperty   :official-journal-act_year
                         ] .

:event_legal_drafted_by_person
        a                   owl:ObjectProperty ;
        rdfs:comment        "A given person acts as drafter for this legal event. Person role: Draftsman. Relevant for legal analysis: true." ;
        rdfs:domain         :event_legal ;
        rdfs:label          "Legal event drafted by person" ;
        rdfs:range          :person ;
        rdfs:subPropertyOf  :drafted_by ;
        owl:inverseOf       :person_drafts_event_legal .

:manifestation_published_in_place
        a                   owl:ObjectProperty ;
        rdfs:comment        "Manifestation was published in a place characterized by a concept from AT place" ;
        rdfs:domain         :manifestation ;
        rdfs:label          "Manifestation published in place" ;
        rdfs:range          :place ;
        rdfs:subPropertyOf  :published_in ;
        owl:inverseOf       :place_publishes_manifestation .

:source_ruling_preliminary
        a           owl:DatatypeProperty ;
        rdfs:label  "Source ruling preliminary" .

:summary_legislation_eu_drafted_in_language
        a                   owl:ObjectProperty ;
        rdfs:comment        "Language in which this document is drafted" ;
        rdfs:domain         :summary_legislation_eu ;
        rdfs:label          "Summary drafted in language" ;
        rdfs:range          :language ;
        rdfs:subPropertyOf  :drafted_in ;
        owl:inverseOf       :language_used_for_drafting_summary_legislation_eu .

:service_associated  a  owl:DatatypeProperty ;
        rdfs:comment  "AS" ;
        rdfs:label    "Service associated" .

[ a            owl:AllDisjointClasses ;
  owl:members  ( :item :expression :manifestation :entity_temporal :work :concept )
] .

:name_meeting  a            owl:DatatypeProperty ;
        rdfs:label          "Name meeting" ;
        rdfs:subPropertyOf  :title .

<http://publications.europa.eu/resource/authority/fd_537>
        a       owl:NamedIndividual .

<http://publications.europa.eu/resource/authority/fd_601>
        a       owl:NamedIndividual .

:expression_date  a         owl:DatatypeProperty ;
        rdfs:comment        "Date of this expression according to a suitable methodology" ;
        rdfs:domain         :expression ;
        rdfs:label          "Expression date" ;
        rdfs:range          xsd:date ;
        rdfs:subPropertyOf  :date .

:legal_basis_printer  a  owl:DatatypeProperty ;
        rdfs:label  "Legal basis printer" .

:ATTO_FD_612  a              owl:Class ;
        rdfs:label           "FD_612 ATTO table" ;
        rdfs:subClassOf      skos:Concept ;
        owl:equivalentClass  [ a               owl:Restriction ;
                               owl:hasValue    <http://publications.europa.eu/resource/authority/fd_612> ;
                               owl:onProperty  skos:inScheme
                             ] .

:drafts  a          owl:ObjectProperty ;
        rdfs:label  "Drafts" .

:manifestation_number_catalogue_other
        a                   owl:DatatypeProperty ;
        rdfs:comment        "other cataglogue number of this manifestation (typically, if it is a general publication). based on 029 7 $a iff $2 != 'LU-LuPOE' # $2 is mandatory" ;
        rdfs:domain         :manifestation ;
        rdfs:label          "Catalogue number other" ;
        rdfs:range          xsd:string ;
        rdfs:subPropertyOf  :number_catalogue_other .

:id_obsolete_document
        a                   owl:DatatypeProperty ;
        rdfs:comment        "Former CELEX number (= DN_OLD)" ;
        rdfs:label          "Id obsolete document" ;
        rdfs:subPropertyOf  :identifier .

:work_dataset_published_by_agent
        a                   owl:ObjectProperty ;
        rdfs:comment        "An entity that is responsible for making the Dataset available" ;
        rdfs:domain         :work_dataset ;
        rdfs:label          "Work dataset published by agent" ;
        rdfs:range          :agent ;
        rdfs:subPropertyOf  :published_by ;
        owl:inverseOf       :agent_publishes_work_dataset .

:work_part_of_event_legal
        a                   owl:ObjectProperty ;
        rdfs:comment        "Many works referred to in Pegase are not legal resources. Relevant for legal analysis: true." ;
        rdfs:domain         :work ;
        rdfs:label          "Work is part of legal event" ;
        rdfs:range          :event_legal ;
        rdfs:subPropertyOf  :part_of ;
        owl:inverseOf       :event_legal_contains_work .

:concept_new_case-law
        a                    owl:Class ;
        rdfs:comment         "Concept from the case law directory. The case law concept is currently coded with FD_Table 578" ;
        rdfs:label           "New case law concept" ;
        rdfs:subClassOf      skos:Concept , :concept ;
        owl:equivalentClass  [ a               owl:Restriction ;
                               owl:hasValue    <http://publications.europa.eu/resource/authority/fd_578> ;
                               owl:onProperty  skos:inScheme
                             ] .

:work_related_with_agent
        a                   owl:ObjectProperty ;
        rdfs:comment        "This generic relation relates the work to the agent, in considering all possible ROLES of the agent (person, institution, ...), which does an event (all type of work)" ;
        rdfs:domain         :work ;
        rdfs:label          "Work related with agent" ;
        rdfs:range          :agent ;
        rdfs:subPropertyOf  :related_with .

:target_groups  a   owl:DatatypeProperty ;
        rdfs:label  "Target groups" .

:alinea  a               owl:Class ;
        rdfs:label       "Alinea" ;
        rdfs:subClassOf  :subdivision .

:event_internal_urgent_procedure
        a                   owl:DatatypeProperty ;
        rdfs:comment        "Indicates if the delegated act enters into force immediately as long as no objections are expressed by the European Parliament and the Council. the possible values: (true) urgent procedure, (false) normal procedure" ;
        rdfs:domain         :event_internal ;
        rdfs:label          "Urgent procedure" ;
        rdfs:range          xsd:boolean ;
        rdfs:subPropertyOf  :urgent_procedure .

:case-law_requests_validation_resource_legal
        a                   owl:ObjectProperty ;
        rdfs:comment        "This property points to legal act quoted in the operative part of Court decisions" ;
        rdfs:domain         :case-law ;
        rdfs:label          "Case law requests validation a legal resource" ;
        rdfs:range          :resource_legal ;
        rdfs:subPropertyOf  :requests_validation ;
        owl:inverseOf       :resource_legal_validation_requested_by_case-law .

:qualifier_document  a  owl:DatatypeProperty ;
        rdfs:label  "Qualifier document" .

:fragment_resource_legal_id_fragment
        a                   owl:DatatypeProperty ;
        rdfs:comment        "Identifier of a fragment (typically an article number)" ;
        rdfs:domain         :fragment_resource_legal ;
        rdfs:label          "Fragment identifier" ;
        rdfs:range          xsd:string ;
        rdfs:subPropertyOf  :id_fragment .

:communication_ec  a     owl:Class ;
        rdfs:comment     "3063 Commission communication (5DC or 5SC with FM=COMMUNIC)" ;
        rdfs:label       "Commission communication" ;
        rdfs:subClassOf  :act_preparatory_ec .

:language_used_for_drafting_summary_legislation_eu
        a                   owl:ObjectProperty ;
        rdfs:domain         :language ;
        rdfs:label          "Language used for drafting summary of EU legislation" ;
        rdfs:range          :summary_legislation_eu ;
        rdfs:subPropertyOf  :used_for_drafting ;
        owl:inverseOf       :summary_legislation_eu_drafted_in_language .

<http://publications.europa.eu/resource/authority/legal-act-domain>
        a       owl:NamedIndividual .

:manifestation_official-journal_part_subsection_oj
        a                   owl:DatatypeProperty ;
        rdfs:comment        "Sub section of the OJ part that this legal resource was published in. Added in the context of IMMC2CDM-OJ" ;
        rdfs:domain         :manifestation_official-journal_part ;
        rdfs:label          "Sub section of the OJ" ;
        rdfs:range          xsd:string ;
        rdfs:subPropertyOf  :subsection_oj .

:person_reports_on_opinion_eesc
        a                   owl:ObjectProperty ;
        rdfs:domain         :person ;
        rdfs:label          "Person reports on opinion_eesc" ;
        rdfs:range          :opinion_eesc ;
        rdfs:subPropertyOf  :reports_on ;
        owl:inverseOf       :opinion_eesc_reported_by_person .

:resource_legal_codified_version
        a                   owl:DatatypeProperty ;
        rdfs:comment        "Codified version of the legal resource. Added in the context of IMMC2CDM-OJ" ;
        rdfs:domain         :resource_legal ;
        rdfs:label          "Legal resource codified version" ;
        rdfs:range          xsd:boolean ;
        rdfs:subPropertyOf  :codified_version .

:procedure_code_interinstitutional_european_union_competence_type
        a                   owl:DatatypeProperty ;
        rdfs:comment        "When the Treaties confer on the Union exclusive competence in a specific area, only the Union may legislate and adopt legally binding acts;When the Treaties confer on the Union a competence shared with the Member States in a specific area, the Union and the Member States may legislate and adopt legally binding acts in that area. values: EXCLUSIVE (exclusive competence, articles 3 and 6 TUE), SHARED (shared competence with the Member States, article 4 TUE)" ;
        rdfs:domain         :procedure_code_interinstitutional ;
        rdfs:label          "Type of competence conferred on the European Union" ;
        rdfs:range          xsd:string ;
        rdfs:subPropertyOf  :european_union_competence_type .

:work_edited_by_agent
        a                   owl:ObjectProperty ;
        rdfs:comment        "The work is edited by an agent (AU)" ;
        rdfs:domain         :work ;
        rdfs:label          "Work is edited by agent" ;
        rdfs:range          :agent ;
        rdfs:subPropertyOf  :work_contributed_to_by_agent , :edited_by ;
        dct:created         "2018-08-30T11:12:32.408+02:00"^^xsd:dateTime ;
        owl:inverseOf       :agent_edits_work .

:resource_legal_validity_extended_by_resource_legal
        a                   owl:ObjectProperty ;
        rdfs:comment        "Calculated. Relevant for legal analysis: true." ;
        rdfs:domain         :resource_legal ;
        rdfs:label          "Legal resource has validity extended by legal resource" ;
        rdfs:range          :resource_legal ;
        rdfs:subPropertyOf  :validity_extended_by ;
        owl:inverseOf       :resource_legal_extends_validity_of_resource_legal .

<http://publications.europa.eu/resource/authority/fd_070>
        a       owl:NamedIndividual .

:number_corrigendum_eli
        a           owl:DatatypeProperty ;
        rdfs:label  "Number corrigendum eli" .

:event_case  a           owl:Class ;
        rdfs:comment     "An event in a court case" ;
        rdfs:label       "Case event" ;
        rdfs:subClassOf  :event ;
        rdfs:subClassOf  [ a                   owl:Restriction ;
                           owl:maxCardinality  "1"^^xsd:nonNegativeInteger ;
                           owl:onProperty      :event_case_framework_procedural_sequential-number_nature
                         ] ;
        rdfs:subClassOf  [ a                            owl:Restriction ;
                           owl:maxQualifiedCardinality  "1"^^xsd:nonNegativeInteger ;
                           owl:onClass                  :procjur-type ;
                           owl:onProperty               :event_case_has_procjur-type
                         ] ;
        rdfs:subClassOf  [ a                   owl:Restriction ;
                           owl:maxCardinality  "1"^^xsd:nonNegativeInteger ;
                           owl:onProperty      :event_case_framework_procedural_sequential-number_type_procedure
                         ] ;
        rdfs:subClassOf  [ a                   owl:Restriction ;
                           owl:maxCardinality  "1"^^xsd:nonNegativeInteger ;
                           owl:onProperty      :event_case_part2
                         ] ;
        rdfs:subClassOf  [ a                   owl:Restriction ;
                           owl:maxCardinality  "1"^^xsd:nonNegativeInteger ;
                           owl:onProperty      :event_case_part1
                         ] ;
        rdfs:subClassOf  [ a                            owl:Restriction ;
                           owl:maxQualifiedCardinality  "1"^^xsd:nonNegativeInteger ;
                           owl:onClass                  :concept_court_procedure ;
                           owl:onProperty               :event_case_framework_procedural_has_nature_concept_court_procedure
                         ] ;
        rdfs:subClassOf  [ a                            owl:Restriction ;
                           owl:maxQualifiedCardinality  "1"^^xsd:nonNegativeInteger ;
                           owl:onClass                  :concept_case_event_result ;
                           owl:onProperty               :event_case_has_result_concept_case_event_result
                         ] ;
        rdfs:subClassOf  [ a                            owl:Restriction ;
                           owl:maxQualifiedCardinality  "1"^^xsd:nonNegativeInteger ;
                           owl:onClass                  :type-procedure ;
                           owl:onProperty               :event_case_has_type-procedure
                         ] ;
        rdfs:subClassOf  [ a                   owl:Restriction ;
                           owl:maxCardinality  "1"^^xsd:nonNegativeInteger ;
                           owl:onProperty      :event_case_framework_procedural_identifier
                         ] .

:measure_national_implementing_date_official_journal
        a                   owl:DatatypeProperty ;
        rdfs:comment        "Date of the national or regional official journal on which this NIM was published" ;
        rdfs:domain         :measure_national_implementing ;
        rdfs:label          "Date of the national or regional Official Journal" ;
        rdfs:range          xsd:date ;
        rdfs:subPropertyOf  :date_official_journal .

:opinion_other_cor_number_session
        a                   owl:DatatypeProperty ;
        rdfs:comment        "DEPRECATED. Number of session during which this act was debated or voted (EP.EESC,CoR, …). Relevant for legaa analysis: true. Mixed content, decoded with fd_345. Use cdm:act_preparatory_number_session" ;
        rdfs:domain         :opinion_other_cor ;
        rdfs:label          "Number of session" ;
        rdfs:range          xsd:string ;
        rdfs:subPropertyOf  :number_session , :act_preparatory_number_session ;
        owl:deprecated      true .

:legislation_secondary_is_about_concept_directory-code
        a                   owl:ObjectProperty ;
        rdfs:comment        "DEPRECATED, A secondary legislation is about a concept expressed in the directory code. CC, coded separatedly (FD table 555). Relevant for legal analysis: true." ;
        rdfs:domain         :legislation_secondary ;
        rdfs:label          "Secondary legislation is about directory code concept" ;
        rdfs:range          :concept_directory-code ;
        rdfs:subPropertyOf  :is_about ;
        owl:deprecated      true .

:reference-data_asset_release_releases_reference-data_asset
        a                   owl:ObjectProperty ;
        rdfs:comment        "This predicate describes the relation between an official/stable release version and the related representant asset" ;
        rdfs:domain         :reference-data_asset_release ;
        rdfs:label          "Reference data asset release releases reference data asset" ;
        rdfs:range          :reference-data_asset ;
        rdfs:subPropertyOf  :releases ;
        owl:inverseOf       :reference-data_asset_released_in_reference-data_asset_release .

:event_associated_with_institution
        a                   owl:ObjectProperty ;
        rdfs:comment        "Relevant for legal analysis: true. This event is associated with a given institution. Relevant for legal analysis: true" ;
        rdfs:domain         :event ;
        rdfs:label          "Event associated with institution" ;
        rdfs:range          :institution ;
        rdfs:subPropertyOf  :associated_with ;
        owl:inverseOf       :institution_associated_with_event .

:person_reports_on_resolution_legislative_ep
        a              owl:ObjectProperty ;
        rdfs:domain    :person ;
        rdfs:label     "Person reports on resolution legislative ep" ;
        rdfs:range     :resolution_legislative_ep ;
        owl:inverseOf  :resolution_legislative_ep_reported_by_person .

:eea    a           owl:DatatypeProperty ;
        rdfs:label  "Eea" .

:page_last  a       owl:DatatypeProperty ;
        rdfs:label  "Page last" .

:date_debate  a             owl:DatatypeProperty ;
        rdfs:comment        "DB" ;
        rdfs:label          "Date debate" ;
        rdfs:range          xsd:date ;
        rdfs:subPropertyOf  :date .

:event_legal_has_type_concept_type_event_legal
        a                   owl:ObjectProperty ;
        rdfs:comment        "DEPRECATED, Event has a certain type of event. Relevant for legal analysis: true." ;
        rdfs:domain         :event_legal ;
        rdfs:label          "Legal event has type concept type event" ;
        rdfs:range          :concept_type_event_legal ;
        rdfs:subPropertyOf  :has_type , :event_has_type_concept_type_event ;
        owl:deprecated      true .

:concept_legal_basis_court_procedure
        a                owl:Class ;
        rdfs:label       "Concept representing the legal basis of a Court procedure" ;
        rdfs:subClassOf  :concept_decoding .

:procedure_internal_roadmap_needed
        a                   owl:DatatypeProperty ;
        rdfs:comment        "Do the better_regulation_requirements require a roadmap for this internal procedure? /ns4:ec_transmission_request/transmission/workflow/extension/ns3:better_regulation_requirements/ns3:roadmap" ;
        rdfs:domain         :procedure_internal ;
        rdfs:label          "Internal procedure needs roadmap?" ;
        rdfs:range          xsd:boolean ;
        rdfs:subPropertyOf  :roadmap_needed .

:informed_by  a     owl:ObjectProperty ;
        rdfs:label  "Informed by" .

:special-official-journal_is_about_concept_directory-code
        a                   owl:ObjectProperty ;
        rdfs:domain         :special-official-journal ;
        rdfs:label          "Special Edition is about a Directory code chapter" ;
        rdfs:range          :concept_directory-code ;
        rdfs:subPropertyOf  :is_about ;
        owl:inverseOf       :concept_directory-code_subject_of_special-official-journal .

:event_legal_reported_by_person
        a                   owl:ObjectProperty ;
        rdfs:comment        "Relevant for legal analysis: true. This legal event is reported on by a given person. Relevant for legal analysis: true" ;
        rdfs:domain         :event_legal ;
        rdfs:label          "Legal event reported on by person" ;
        rdfs:range          :person ;
        rdfs:subPropertyOf  :event_reported_by_person ;
        owl:inverseOf       :person_reports_on_event_legal .

:parent_document_ref  a  owl:DatatypeProperty ;
        rdfs:label  "Parent document ref" .

:work_contains_title_legal
        a                   owl:ObjectProperty ;
        rdfs:domain         :work ;
        rdfs:label          "Work contains title (legal)" ;
        rdfs:range          :title_legal ;
        rdfs:subPropertyOf  :work_contains_subdivision , :contains .

:procurement_public_contract-nature_label
        a                   owl:DatatypeProperty ;
        rdfs:domain         :procurement_public ;
        rdfs:label          "Natural label of the contract" ;
        rdfs:range          xsd:string ;
        rdfs:subPropertyOf  :contract-nature_label .

:recommendation_ecb  a   owl:Class ;
        rdfs:comment     "ECB recommendations, usually based on the Statute of the European System of Central Banks and of the ECB (5HB)" ;
        rdfs:label       "European Central Bank recommendation" ;
        rdfs:subClassOf  :act_preparatory_ecb .

:manifestation_court-report_belongs_to_type_court-report
        a                   owl:ObjectProperty ;
        rdfs:domain         :manifestation_court-report ;
        rdfs:label          "Manifestation published in a type of court report" ;
        rdfs:range          :type_court-report ;
        rdfs:subPropertyOf  :belongs_to .

:publication_general_has_target_audience_old
        a           owl:ObjectProperty ;
        rdfs:label  "Publication general has target audience old" .

:reestablishes  a   owl:ObjectProperty ;
        rdfs:label  "Reestablishes" .

:institution_addressed_by_resource_legal
        a                   owl:ObjectProperty ;
        rdfs:comment        "An institution is the addressee of a legal resource (document)" ;
        rdfs:domain         :institution ;
        rdfs:label          "Institution addressed by legal resource" ;
        rdfs:range          :resource_legal ;
        rdfs:subPropertyOf  :addressed_by ;
        owl:inverseOf       :resource_legal_addresses_institution .

:agent_requests_communication_cjeu
        a              owl:ObjectProperty ;
        rdfs:domain    :agent ;
        rdfs:label     "Agent requests communication cjeu" ;
        rdfs:range     :communication_cjeu ;
        owl:inverseOf  :communication_cjeu_requested_by_agent .

<http://publications.europa.eu/resource/authority/pub-theme>
        a       owl:NamedIndividual .

:question_parliamentary_number_session
        a                   owl:DatatypeProperty ;
        rdfs:comment        "DEPRECATED. Number of session during which this act was debated or voted (EP, EESC, CoR, …). Relevant for legal analysis: true" ;
        rdfs:domain         :question_parliamentary ;
        rdfs:label          "Number of session" ;
        rdfs:range          xsd:string ;
        rdfs:subPropertyOf  :number_session , :act_preparatory_number_session ;
        owl:deprecated      true .

:event_internal_planned_objection_period_date_start
        a            owl:DatatypeProperty ;
        rdfs:domain  :event_internal ;
        rdfs:label   "Event internal planned objection period date start" ;
        rdfs:range   xsd:date ;
        dct:created  "2018-07-16T13:03:24.876+02:00"^^xsd:dateTime .

:work_id_document  a        owl:DatatypeProperty ;
        rdfs:comment        "An alternative identifier (id) that this work may have. All identifier-like properties are subproperties of the identifier property." ;
        rdfs:domain         :work ;
        rdfs:label          "Identifier of document" ;
        rdfs:range          xsd:string ;
        rdfs:subPropertyOf  :id_document .

:recital  a              owl:Class ;
        rdfs:comment     "A recital in a legal document . Created to have correspondance to the subdivision NAL" ;
        rdfs:label       "Recital" ;
        rdfs:subClassOf  :subdivision .

:case-law_is_about_concept
        a                   owl:ObjectProperty ;
        rdfs:comment        "This property points to a concept from a directory of case law" ;
        rdfs:label          "Case law is about concept" ;
        rdfs:subPropertyOf  :is_about .

:paragraph_legal  a      owl:Class ;
        rdfs:comment     "A paragraph in a legal document" ;
        rdfs:label       "Paragraph (legal)" ;
        rdfs:subClassOf  :subdivision .

:number_natural  a  owl:DatatypeProperty ;
        rdfs:label  "Number natural" .

:procurement_public_nuts_original_link_type
        a                   owl:DatatypeProperty ;
        rdfs:domain         :procurement_public ;
        rdfs:label          "NUTS original type" ;
        rdfs:range          xsd:string ;
        rdfs:subPropertyOf  :nuts_original_link_type .

:is_another_publication_of
        a           owl:ObjectProperty ;
        rdfs:label  "Is another publication of" .

:opinion_ec_ep-amendments
        a                owl:Class ;
        rdfs:comment     "where its resource_legal_type = (PC or DC), resource_legal_id_sector = 5, work_has_resource-type = OPIN_AMEND_EP" ;
        rdfs:label       "EC Opinion on European Parliament's amendments" ;
        rdfs:subClassOf  :act_preparatory_ec .

:ATTO_FD_501  a              owl:Class ;
        rdfs:label           "FD_501 ATTO table" ;
        rdfs:subClassOf      skos:Concept ;
        owl:equivalentClass  [ a               owl:Restriction ;
                               owl:hasValue    <http://publications.europa.eu/resource/authority/fd_501> ;
                               owl:onProperty  skos:inScheme
                             ] .

:court-report_publishes_document_cjeu
        a                   owl:ObjectProperty ;
        rdfs:domain         :court-report ;
        rdfs:label          "Court report publishes a court document" ;
        rdfs:range          :document_cjeu ;
        rdfs:subPropertyOf  :publishes ;
        owl:inverseOf       :document_cjeu_published_in_court-report .

:consultation_duration
        a           owl:DatatypeProperty ;
        rdfs:label  "Consultation duration" .

:declares_incidentally_valid
        a           owl:ObjectProperty ;
        rdfs:label  "Declares incidentally valid" .

:resource_legal_amends_resource_legal
        a                   owl:ObjectProperty ;
        rdfs:comment        "A change or alteration in existing provisions of an act. This property points to act which provision(s) are amended. Relevant for legal analysis: true" ;
        rdfs:domain         :resource_legal ;
        rdfs:label          "Legal resource amends legal resource" ;
        rdfs:range          :resource_legal ;
        rdfs:subPropertyOf  :amends ;
        owl:inverseOf       :resource_legal_amended_by_resource_legal .

:thumbnail  a            owl:Class ;
        rdfs:comment     "A thumbnail item. Other properties of the item class are the technical metadata associated with the item in question (defined in the TMD ontology)" ;
        rdfs:label       "Thumbnail" ;
        rdfs:subClassOf  :item .

:manifestation_dimension
        a                   owl:DatatypeProperty ;
        rdfs:comment        "dimension of this manifestation. mapped from 300 $c" ;
        rdfs:domain         :manifestation ;
        rdfs:label          "Dimension of manifestation" ;
        rdfs:range          xsd:string ;
        rdfs:subPropertyOf  :dimension .

:measure_national_implementing_implements_directive
        a                   owl:ObjectProperty ;
        rdfs:comment        "DEPRECATED, Link to the directive that this NIM implements. Use mesure_national_implementing_implements_resource_legal" ;
        rdfs:domain         :measure_national_implementing ;
        rdfs:label          "National implementing measure implements directive" ;
        rdfs:range          :directive ;
        rdfs:subPropertyOf  :measure_national_implementing_implements_resource_legal , :implements ;
        owl:deprecated      true ;
        owl:inverseOf       :directive_implemented_by_measure_national_implementing .

:evolutive_work  a       owl:Class ;
        rdfs:comment     "This class describes a set of works where each work member of the evolutive_work instance is an evolution of the preceding one." ;
        rdfs:label       "Evolutive Work" ;
        rdfs:subClassOf  :serial_work ;
        rdfs:subClassOf  [ a                   owl:Restriction ;
                           owl:maxCardinality  "1"^^xsd:nonNegativeInteger ;
                           owl:onProperty      :evolutive_work_nature_classification
                         ] ;
        rdfs:subClassOf  [ a                owl:Restriction ;
                           owl:cardinality  "1"^^xsd:nonNegativeInteger ;
                           owl:onProperty   :datetime_negotiation
                         ] .

:staff-working-document_service_associated
        a                   owl:DatatypeProperty ;
        rdfs:comment        "This field indicates the Commission DG or DGs co-responsible for drafting of an act. DEPRECATED, In the instance data, the property is planned to be replaced with cdm:resource_legal_service_associated at beginning 2019. When this is done this property the property will be removed from CDM. Relevant for legal analysis: true" ;
        rdfs:domain         :staff-working-document ;
        rdfs:label          "Service associated" ;
        rdfs:range          xsd:string ;
        rdfs:subPropertyOf  :service_associated , :resource_legal_service_associated ;
        owl:deprecated      true .

:procedure_code_interinstitutional_basis_legal
        a                   owl:DatatypeProperty ;
        rdfs:comment        "Legal basis of the procedure (as text). Relevant for legal analysis: true." ;
        rdfs:domain         :procedure_code_interinstitutional ;
        rdfs:label          "Legal basis of the procedure" ;
        rdfs:range          xsd:string ;
        rdfs:subPropertyOf  :dossier_basis_legal ;
        dct:created         "2018-11-02T15:09:26.258+01:00"^^xsd:dateTime .

:event_part_of_dossier
        a                   owl:ObjectProperty ;
        rdfs:comment        "Relevant for legal analysis: true. The event is part of a dossier. Relevant for legal analysis: true" ;
        rdfs:domain         :event ;
        rdfs:label          "Event is part of dossier" ;
        rdfs:range          :dossier ;
        rdfs:subPropertyOf  :part_of .

:communication_case_new_submits_preliminary_question_resource_legal
        a                   owl:ObjectProperty ;
        rdfs:comment        "This property points to legal act quoted in the communication on a new case published in OJ (preliminary ruling). Relevant for legal analysis: true" ;
        rdfs:domain         :communication_case_new ;
        rdfs:label          "Communication submits a question on interpretation or validation" ;
        rdfs:range          :resource_legal ;
        rdfs:subPropertyOf  :submits_preliminary_question ;
        owl:inverseOf       :resource_legal_preliminary_question-submitted_by_communication_case_new .

:manifestation_print_page_last
        a                   owl:DatatypeProperty ;
        rdfs:comment        "Last page number of the OJ part related to a legal resource" ;
        rdfs:domain         :manifestation_print ;
        rdfs:label          "Last page" ;
        rdfs:range          xsd:string ;
        rdfs:subPropertyOf  :page_last .

:resource_legal_partial_annulment_requested_by_communication_case_new
        a              owl:ObjectProperty ;
        rdfs:domain    :resource_legal ;
        rdfs:label     "Resource legal partial annulment requested by communication case new" ;
        rdfs:range     :communication_case_new ;
        owl:inverseOf  :communication_case_new_requests_partial_annulment_of_resource_legal .

:work_table-of-contents
        a             owl:DatatypeProperty ;
        rdfs:comment  "Table of contents." ;
        rdfs:domain   :work ;
        rdfs:label    "Table of contents" ;
        rdfs:range    rdf:XMLLiteral .

:manifestation_distribution_has_media_type_concept_media_type
        a                   owl:ObjectProperty ;
        rdfs:comment        "Distribution media type" ;
        rdfs:domain         :manifestation_distribution ;
        rdfs:label          "Distribution media type" ;
        rdfs:range          :concept_media_type ;
        rdfs:subPropertyOf  :has_media_type .

:requests_opinion_on  a  owl:ObjectProperty ;
        rdfs:label  "Requests opinion on" .

:act_other_cor_reported_by_person
        a                   owl:ObjectProperty ;
        rdfs:comment        "Name of the person (EP member or member of CoR or EESC) who reports on the relevant act. This property will be deprecated and replaced with work_reported_by_person. Role RAPP. Relevant for legal analysis: true" ;
        rdfs:domain         :act_other_cor ;
        rdfs:label          "Committee of the Regions' other act has rapporteur" ;
        rdfs:range          :person ;
        rdfs:subPropertyOf  :work_reported_by_person ;
        dct:created         "2018-07-16T13:14:40.407+02:00"^^xsd:dateTime ;
        owl:inverseOf       :person_reports_on_act_other_cor .

:chapter_legal_part_of_work
        a                   owl:ObjectProperty ;
        rdfs:comment        "This property associates an instance of a work with an instance of a chapter that forms part of it." ;
        rdfs:domain         :chapter_legal ;
        rdfs:label          "Chapter (legal) part of work" ;
        rdfs:range          :work ;
        rdfs:subPropertyOf  :subdivision_part_of_work , :part_of ;
        owl:inverseOf       :work_contains_chapter_legal .

:manifestation_official-journal_part_is_corrigendum_printer
        a                   owl:DatatypeProperty ;
        rdfs:comment        "Is this a corrigendum? values can be C (corrigendum) or O (not a corrigendum), removed range restriction for IMMC2CDM-OJ" ;
        rdfs:domain         :manifestation_official-journal_part ;
        rdfs:label          "Printer's view if this is a corrigendum or not" ;
        rdfs:range          xsd:string ;
        rdfs:subPropertyOf  :is_corrigendum_printer .

:requests_annulment_of
        a           owl:ObjectProperty ;
        rdfs:label  "Requests annulment of" .

:name   a           owl:DatatypeProperty ;
        rdfs:label  "Name" .

:complex_work_has_member_work
        a                   owl:ObjectProperty ;
        rdfs:comment        "This property associates an instance of complex_work with an instance of work that forms part of it." ;
        rdfs:domain         :complex_work ;
        rdfs:label          "Work has member" ;
        rdfs:range          :work ;
        rdfs:subPropertyOf  :has_member ;
        owl:inverseOf       :work_is_member_of_complex_work .

:interpretes  a     owl:ObjectProperty ;
        rdfs:label  "Interpretes" .

:agent_reads_manifestation-audiovisual
        a                   owl:ObjectProperty ;
        rdfs:comment        "this refers to the narrator of an audiovisual manifestation, e.g., an audiobook" ;
        rdfs:domain         :agent ;
        rdfs:label          "Agent reads audiovisual manifestation" ;
        rdfs:range          :manifestation-audiovisual ;
        rdfs:subPropertyOf  :reads ;
        dct:created         "2022-08-01T16:18:31.50"^^xsd:dateTime ;
        owl:inverseOf       :manifestation-audiovisual_read-by_agent .

:resource_legal_incorporates_resource_legal
        a                   owl:ObjectProperty ;
        rdfs:comment        "Relevant for legal analysis: true" ;
        rdfs:domain         :resource_legal ;
        rdfs:label          "Legal resource incorporates legal resource" ;
        rdfs:range          :resource_legal ;
        rdfs:subPropertyOf  :incorporates ;
        owl:inverseOf       :resource_legal_incorporated_by_resource_legal .

:resource_legal_id_celex
        a                   owl:DatatypeProperty ;
        rdfs:comment        "Celex identifier. CELEX number (= DN and DN2). Relevant for legal analysis: true." ;
        rdfs:domain         :resource_legal ;
        rdfs:label          "Celex identifier" ;
        rdfs:range          xsd:string ;
        rdfs:subPropertyOf  :id_celex .

:resource_legal_service_responsible
        a                   owl:DatatypeProperty ;
        rdfs:comment        "The Commission DG or DGs responsible for drafting of an act. Relevant for legal analysis: true" ;
        rdfs:domain         :resource_legal ;
        rdfs:label          "Service responsible" ;
        rdfs:range          xsd:string ;
        rdfs:subPropertyOf  :service_responsible .

:expression_corrects_expression
        a                   owl:ObjectProperty ;
        rdfs:comment        "Expression corrects another expression. Relevant for legal analysis: true." ;
        rdfs:domain         :expression ;
        rdfs:label          "Expression corrects another expression" ;
        rdfs:range          :expression ;
        rdfs:subPropertyOf  :corrects .

:procurement_public_xml-schema-definition_link_title
        a                   owl:DatatypeProperty ;
        rdfs:domain         :procurement_public ;
        rdfs:label          "Link title for the schema definition" ;
        rdfs:range          xsd:string ;
        rdfs:subPropertyOf  :xml-schema-definition_link_title .

:relevant_for  a    owl:ObjectProperty ;
        rdfs:label  "Relevant for" .

:event_internal_has_type_consultation
        a                   owl:ObjectProperty ;
        rdfs:comment        "This property describes the type of consultation of the internal event" ;
        rdfs:domain         :event_internal ;
        rdfs:label          "Event internal has type consultation" ;
        rdfs:range          :type_consultation ;
        rdfs:subPropertyOf  :has .

:event_date  a              owl:DatatypeProperty ;
        rdfs:comment        "The date of the event" ;
        rdfs:domain         :event ;
        rdfs:label          "Date of event" ;
        rdfs:range          xsd:date ;
        rdfs:subPropertyOf  :date .

:partially_suspended_by
        a           owl:ObjectProperty ;
        rdfs:label  "Partially suspended by" .

:summary_legislation_eu_validated_by_institution
        a                   owl:ObjectProperty ;
        rdfs:comment        "Corporate body which validated this summary" ;
        rdfs:domain         :summary_legislation_eu ;
        rdfs:label          "Summary validated by a corporate body" ;
        rdfs:range          :institution ;
        rdfs:subPropertyOf  :validated_by ;
        owl:inverseOf       :institution_validates_summary_legislation_eu .

:official-journal_publishes_procurement_public
        a              owl:ObjectProperty ;
        rdfs:comment   "An Official Journal edition in Series S publishes a publication procurement document." ;
        rdfs:domain    :official-journal ;
        rdfs:label     "Official journal publishes public procurement" ;
        rdfs:range     :procurement_public ;
        owl:inverseOf  :procurement_public_published_in_official-journal .

<http://publications.europa.eu/resource/authority/fd_400>
        a       owl:NamedIndividual .

:periodical_work  a      owl:Class ;
        rdfs:comment     "This class describes a serial work such as news-paper, news-letter, journal… Each work member of the periodical_work has the same name but a completely new content." ;
        rdfs:label       "Periodical Work" ;
        rdfs:subClassOf  :serial_work .

:dossier_contains_event
        a                   owl:ObjectProperty ;
        rdfs:comment        "Relevant for legal analysis: true. This dossier contains an event. Relevant for legal analysis: true" ;
        rdfs:domain         :dossier ;
        rdfs:label          "Dossier contains event" ;
        rdfs:range          :event ;
        rdfs:subPropertyOf  :contains ;
        owl:inverseOf       :event_part_of_dossier .

:date_signature_xades-a
        a           owl:DatatypeProperty ;
        rdfs:label  "Date signature xades a" .

:manifestation_court-report_part_type
        a                   owl:DatatypeProperty ;
        rdfs:comment        "Type of the court report (Court report of the Court of Justice, parts I and II, Cour de la fonction publique). Temporary solution, should in the future be part of the court report object itself. We need the type as some judgements of the Tribual of first instance can appear both in RJII and TP" ;
        rdfs:domain         :manifestation_court-report_part ;
        rdfs:label          "Type of the court report" ;
        rdfs:range          xsd:string ;
        rdfs:subPropertyOf  :type .

:declared_void_by_preliminary_ruling
        a           owl:ObjectProperty ;
        rdfs:label  "Declared void by preliminary ruling" .

:act_legislative_other_oj_c
        a                owl:Class ;
        rdfs:comment     "Other legislative acts published in Official Journal C series (subsector Y of sector 3) Examples: 31960Y0317(02), 31962Y1109(03), 31970Y0721(01), 31991Y0419(01), 31990Y0303(03). Remark: There are at present 1189 notices. Other than in sector C the notices referes to legislative acts and they have a real CELEX sector 3 number." ;
        rdfs:label       "OJ C other legislative act" ;
        rdfs:subClassOf  :legislation_secondary .

:event_contains_work  a     owl:ObjectProperty ;
        rdfs:comment        "Any event contains one or more works. Relevant for legal analysis: true." ;
        rdfs:domain         :event ;
        rdfs:label          "Event contains a work" ;
        rdfs:range          :work ;
        rdfs:subPropertyOf  :contains ;
        owl:inverseOf       :work_part_of_event .

:white-paper_ec  a       owl:Class ;
        rdfs:comment     "European commission White Paper" ;
        rdfs:label       "White paper EC" ;
        rdfs:subClassOf  :act_preparatory_ec .

:resource_legal_joint-responsibility_of_agent
        a                   owl:ObjectProperty ;
        rdfs:domain         :resource_legal ;
        rdfs:label          "Legal resource under joint responsibility of an agent" ;
        rdfs:range          :agent ;
        rdfs:subPropertyOf  :joint-responsibility_of .

:partially_annulled_by
        a           owl:ObjectProperty ;
        rdfs:label  "Partially annulled by" .

:immediately_enforced_by
        a           owl:ObjectProperty ;
        rdfs:label  "Immediately enforced by" .

:act_other_ecb  a        owl:Class ;
        rdfs:comment     "ECB other acts (5XB)" ;
        rdfs:label       "European Central Bank other act" ;
        rdfs:subClassOf  :act_preparatory_ecb .

:act_other_ep  a         owl:Class ;
        rdfs:label       "European Parliament other act" ;
        rdfs:subClassOf  :act_preparatory_ep ;
        rdfs:subClassOf  [ a                owl:Restriction ;
                           owl:cardinality  "1"^^xsd:nonNegativeInteger ;
                           owl:onProperty   :act_other_ep_term_parliamentary
                         ] .

:ATTO_FD_305  a              owl:Class ;
        rdfs:label           "FD_305 ATTO table" ;
        rdfs:subClassOf      skos:Concept ;
        owl:equivalentClass  [ a               owl:Restriction ;
                               owl:hasValue    <http://publications.europa.eu/resource/authority/fd_305> ;
                               owl:onProperty  skos:inScheme
                             ] .

:manifestation_representation_type
        a            owl:DatatypeProperty ;
        rdfs:domain  :manifestation ;
        rdfs:label   "Manifestation representation type" ;
        rdfs:range   xsd:anyURI .

:archive_package_document
        a                owl:Class ;
        rdfs:comment     "An archive package document is a document contained in an archive package but most probably not available in/with a separate manifestation. However, a minimum level of metadata has to be available for such a document in order to establish a work with at least one expression (e.g. titles, identfiers)." ;
        rdfs:label       "Archive package document" ;
        rdfs:subClassOf  :auxiliary-work ;
        rdfs:subClassOf  [ a                            owl:Restriction ;
                           owl:minQualifiedCardinality  "1"^^xsd:nonNegativeInteger ;
                           owl:onClass                  :archive_package ;
                           owl:onProperty               :archive_package_document_part_of_archive_package
                         ] ;
        dct:created      "2022-09-01T09:01:22" .

:communication_ec_council-position
        a                owl:Class ;
        rdfs:comment     "Communication on Council's position, where work_has_resource-type = COMMUNIC_POSIT" ;
        rdfs:label       "EC Communication on Council's position" ;
        rdfs:subClassOf  :act_preparatory_ec .

:transliterated_contact-point
        a           owl:DatatypeProperty ;
        rdfs:label  "Transliterated contact point" .

:country_implements_measure_national_implementing
        a                   owl:ObjectProperty ;
        rdfs:domain         :country ;
        rdfs:label          "Country implements national implementing measure" ;
        rdfs:range          :measure_national_implementing ;
        rdfs:subPropertyOf  :implements ;
        owl:inverseOf       :measure_national_implementing_implemented_by_country .

:reference-data_asset_prerelease_prereleases_reference-data_asset
        a                   owl:ObjectProperty ;
        rdfs:comment        "This predicate describes the relation between an inofficial/unstable prerelease version and the related representant asset" ;
        rdfs:domain         :reference-data_asset_prerelease ;
        rdfs:label          "Reference data asset prerelease prereleases reference data asset" ;
        rdfs:range          :reference-data_asset ;
        rdfs:subPropertyOf  :prereleases ;
        owl:inverseOf       :reference-data_asset_prereleased_in_reference-data_asset_prerelease .

:manifestation_case-law_grounds
        a                   owl:DatatypeProperty ;
        rdfs:comment        "Grounds / motivation associated with this judgement. Sector 6 Text Index Field MO" ;
        rdfs:domain         :manifestation_case-law ;
        rdfs:label          "Grounds for court decision" ;
        rdfs:range          rdf:XMLLiteral ;
        rdfs:subPropertyOf  :grounds .

:case-law_interpretes_judgement_resource_legal
        a                   owl:ObjectProperty ;
        rdfs:comment        "This property points to legal act quoted in the operative part of Court decisions." ;
        rdfs:domain         :case-law ;
        rdfs:label          "Case law interpretes judgement" ;
        rdfs:range          :resource_legal ;
        rdfs:subPropertyOf  :interpretes_judgement ;
        owl:inverseOf       :resource_legal_interpreted_by_judgement_case-law .

:procedure_code_interinstitutional_has_type_concept_type_procedure_code_interinstitutional
        a                   owl:ObjectProperty ;
        rdfs:comment        "Procedure has a certain type of procedure. Uses the procedure NAL. Relevant for legal analysis: true." ;
        rdfs:domain         :procedure_code_interinstitutional ;
        rdfs:label          "Procedure has type concept type procedure" ;
        rdfs:range          :concept_type_procedure_code_interinstitutional ;
        rdfs:subPropertyOf  :has_type .

:question_parliamentary_published
        a                   owl:DatatypeProperty ;
        rdfs:comment        "Has this debate ever been published in \"EP debates\"? Indicates if this debate has ever been published in \"EP Debates\" (examples: 91998H0002, 91998H0001). In this case we have a manifestation_print with information on the relevant publication, e.g. \"Debates of the EP (French ed.):No 514 P. 0193\". This type of parliamentary questions was published in the OJ from 1979 to 2000" ;
        rdfs:domain         :question_parliamentary ;
        rdfs:label          "Question published?" ;
        rdfs:range          xsd:boolean ;
        rdfs:subPropertyOf  :published .

:document_budget_ep_term_parliamentary
        a                   owl:DatatypeProperty ;
        rdfs:comment        "This indicates the Parliamentary term during which an EP document was voted or EP question was raised. Relevant for legal analysis: true. Currently coded with FD_Table 285. However, only codes are exposed (not decoded), so 01, 02 etc.\"" ;
        rdfs:domain         :document_budget_ep ;
        rdfs:label          "Parliamentary term" ;
        rdfs:range          xsd:string ;
        rdfs:subPropertyOf  :term_parliamentary , :act_preparatory_term_parliamentary .

:procurement_public_directive_name
        a                   owl:DatatypeProperty ;
        rdfs:domain         :procurement_public ;
        rdfs:label          "Directive name" ;
        rdfs:range          xsd:string ;
        rdfs:subPropertyOf  :directive_name .

:contains_eesc_opinion_on
        a           owl:ObjectProperty ;
        rdfs:label  "Contains eesc opinion on" .

:event_associated_with_person
        a                   owl:ObjectProperty ;
        rdfs:comment        "Relevant for legal analysis: true. This event is associated with a given person. Relevant for legal analysis: true" ;
        rdfs:domain         :event ;
        rdfs:label          "Event associated with person" ;
        rdfs:range          :person ;
        rdfs:subPropertyOf  :associated_with ;
        owl:inverseOf       :person_associated_with_event .

:rule_legal  a           owl:Class ;
        rdfs:comment     "A rule in a legal document. Created to have correspondance to the subdivision NAL" ;
        rdfs:label       "Rule (legal)" ;
        rdfs:subClassOf  :subdivision .

:resource_legal_received_opinion_cjeu
        a                   owl:ObjectProperty ;
        rdfs:comment        "Calculated. Relevant for legal analysis: true." ;
        rdfs:domain         :resource_legal ;
        rdfs:label          "Legal resource received opinion" ;
        rdfs:range          :opinion_cjeu ;
        rdfs:subPropertyOf  :received .

:agent_defends_in_case-law
        a                   owl:ObjectProperty ;
        rdfs:comment        "Agent (typically a country or an organization) defends himself before the court. DF" ;
        rdfs:domain         :agent ;
        rdfs:label          "Agent defends in case law" ;
        rdfs:range          :case-law ;
        rdfs:subPropertyOf  :defends_in ;
        owl:inverseOf       :case-law_defended_by_agent .

:partially_referred_to
        a           owl:ObjectProperty ;
        rdfs:label  "Partially referred to" .

:manifestation_manifests_expression
        a                   owl:ObjectProperty ;
        rdfs:comment        "A Manifestation manifests a given expression. Relevant for legal analysis: true." ;
        rdfs:domain         :manifestation ;
        rdfs:label          "Manifestation manifests expression" ;
        rdfs:range          :expression ;
        rdfs:subPropertyOf  :manifests .

:court  a           owl:DatatypeProperty ;
        rdfs:label  "Court" .

:does_renumbering_of  a  owl:ObjectProperty ;
        rdfs:label  "Does renumbering of" .

:uses_originally  a         owl:ObjectProperty ;
        rdfs:label          "Uses originally" ;
        rdfs:subPropertyOf  :uses .

:event_legal_contains_work
        a                   owl:ObjectProperty ;
        rdfs:comment        "DEPRECATED, Any legal event contains one or more works. LP_EVENT_DOC_CELEX. Relevant for legal analysis: true." ;
        rdfs:domain         :event_legal ;
        rdfs:label          "Legal event contains a work" ;
        rdfs:range          :work ;
        rdfs:subPropertyOf  :event_contains_work , :contains ;
        owl:deprecated      true ;
        owl:inverseOf       :work_part_of_event_legal .

:resource_legal_number_corrigendum
        a                   owl:DatatypeProperty ;
        rdfs:comment        "Sequential number of the nth corrigendum. Relevant for legal analysis: true" ;
        rdfs:domain         :resource_legal ;
        rdfs:label          "Corrigendum number" ;
        rdfs:range          xsd:positiveInteger ;
        rdfs:subPropertyOf  :number_corrigendum .

<http://publications.europa.eu/resource/authority/document-collection>
        a       owl:NamedIndividual .

:work_dataset_date_start
        a                   owl:DatatypeProperty ;
        rdfs:comment        "This property refers to the beginning of the period the dataset covers" ;
        rdfs:domain         :work_dataset ;
        rdfs:label          "Dataset start date" ;
        rdfs:range          xsd:date ;
        rdfs:subPropertyOf  :date_start .

:point_part_of_work  a      owl:ObjectProperty ;
        rdfs:comment        "This property associates an instance of a work with an instance of POINT that forms part of it." ;
        rdfs:domain         :point ;
        rdfs:label          "Point part of work" ;
        rdfs:range          :work ;
        rdfs:subPropertyOf  :subdivision_part_of_work , :part_of ;
        owl:inverseOf       :work_contains_point .

<http://publications.europa.eu/resource/authority/court-report>
        a       owl:NamedIndividual .

:manifestation_part_of_manifestation
        a                   owl:ObjectProperty ;
        rdfs:comment        "Relevant for legal analysis: true. The manifestation is part of another manifestation (e.g. the manifestation of an act is part of the manifestation of the OJ in print). Manifestation is part of another manifestation. In particular relevant for OJ manifestations. Relevant for legal analysis: true" ;
        rdfs:domain         :manifestation ;
        rdfs:label          "Manifestation is part of manifestation" ;
        rdfs:range          :manifestation ;
        rdfs:subPropertyOf  :part_of .

:region  a               owl:Class ;
        rdfs:comment     "Region of a country (e.g. a Land in Germany)" ;
        rdfs:label       "Region" ;
        rdfs:subClassOf  :unit_administrative .

:work_summarized_by_summary
        a                   owl:ObjectProperty ;
        rdfs:comment        "The work is summarized by another work (e.g. the summary of case law)" ;
        rdfs:domain         :work ;
        rdfs:label          "Work is summarized by work" ;
        rdfs:range          :summary ;
        rdfs:subPropertyOf  :summarized_by ;
        owl:inverseOf       :summary_summarizes_work .

:expression_accompanying_material_uses_language
        a                   owl:ObjectProperty ;
        rdfs:comment        "The language of the accompanying material" ;
        rdfs:domain         :expression ;
        rdfs:label          "Expression's accompanying material uses language" ;
        rdfs:range          :language ;
        rdfs:subPropertyOf  :accompanying_material_uses ;
        owl:inverseOf       :language_used_by_accompanying_material_expression .

:work_dataset_is_deprecated
        a             owl:DatatypeProperty ;
        rdfs:comment  "work dataset is deprecated, the property is useful for the MDR team to be able to flag datasets which are not used any more." ;
        rdfs:domain   :work_dataset ;
        rdfs:label    "work dataset is deprecated" ;
        rdfs:range    xsd:boolean .

:addressed_by  a    owl:ObjectProperty ;
        rdfs:label  "Addressed by" .

:series  a          owl:DatatypeProperty ;
        rdfs:label  "Series" .

:ATTO_FD_300  a              owl:Class ;
        rdfs:label           "FD_300 ATTO table" ;
        rdfs:subClassOf      skos:Concept ;
        owl:equivalentClass  [ a               owl:Restriction ;
                               owl:hasValue    <http://publications.europa.eu/resource/authority/fd_300> ;
                               owl:onProperty  skos:inScheme
                             ] .

:concept_place  a        owl:Class ;
        rdfs:comment     "CAT place" ;
        rdfs:label       "Concept representing a place (e.g. a town)" ;
        rdfs:subClassOf  :concept .

:documentation_description_editorial
        a                   owl:DatatypeProperty ;
        rdfs:domain         :documentation ;
        rdfs:label          "Documentation description" ;
        rdfs:range          xsd:string ;
        rdfs:subPropertyOf  :description_editorial .

:dossier_is_about_concept_directory-code
        a             owl:ObjectProperty ;
        rdfs:comment  "The dossier has as subject a concept from the legal act directory. Relevant for legal analysis: to be verified." ;
        rdfs:domain   :dossier ;
        rdfs:label    "Dossier is about directory-code concept" ;
        rdfs:range    :concept_directory-code .

:event_joint-responsibility_of_institution
        a                   owl:ObjectProperty ;
        rdfs:comment        "A given institution is jointly responsible for this event. Relevant for legal analysis: true." ;
        rdfs:domain         :event ;
        rdfs:label          "Event under joint responsibility of an institution" ;
        rdfs:range          :institution ;
        rdfs:subPropertyOf  :joint-responsibility_of ;
        owl:inverseOf       :institution_jointly-responsible_for_event .

:event_legal_session_council
        a                   owl:DatatypeProperty ;
        rdfs:comment        "Relevant for legal analysis: true. council session number. Relevant for legal analysis: true" ;
        rdfs:domain         :event_legal ;
        rdfs:label          "Council session number" ;
        rdfs:range          xsd:positiveInteger ;
        rdfs:subPropertyOf  :session_council .

:resource_legal_domain_reference_oj-act
        a             owl:ObjectProperty ;
        rdfs:comment  "A concept representing the domain of a legal act in the Official Journal" ;
        rdfs:domain   :resource_legal ;
        rdfs:label    "OJ act reference legal domain" ;
        rdfs:range    :legal-act-domain .

:session_date_start_planned
        a           owl:DatatypeProperty ;
        rdfs:label  "Session date start planned" .

:volume_oj  a       owl:DatatypeProperty ;
        rdfs:label  "Volume oj" .

:transliterated_email
        a           owl:DatatypeProperty ;
        rdfs:label  "Transliterated email" .

:act_preparatory_cor  a  owl:Class ;
        rdfs:comment     "Preparatory act by the Committee of the Regions" ;
        rdfs:label       "Preparatory act by COR" ;
        rdfs:subClassOf  :act_preparatory ;
        rdfs:subClassOf  [ a               owl:Restriction ;
                           owl:hasValue    <http://publications.europa.eu/resource/authority/corporate-body/COR> ;
                           owl:onProperty  :work_created_by_agent
                         ] ;
        dct:created      "2022-09-01T09:01:22"^^xsd:dateTime .

:manifestation_has_restriction_on_use
        a           owl:ObjectProperty ;
        rdfs:label  "Manifestation has restriction on use" .

:monograph  a            owl:Class ;
        rdfs:comment     "Any type of monograph" ;
        rdfs:label       "Monograph" ;
        rdfs:subClassOf  :publication_general .

:created_by  a      owl:ObjectProperty ;
        rdfs:label  "Created by" .

:nationality_mep  a  owl:DatatypeProperty ;
        rdfs:label  "Nationality mep" .

<http://publications.europa.eu/resource/authority/corporate-body/CONSIL>
        a       owl:NamedIndividual .

:treats_appeal  a   owl:ObjectProperty ;
        rdfs:label  "Treats appeal" .

:contributed_to_by  a  owl:ObjectProperty ;
        rdfs:label  "Contributed to by" .

:age    a             owl:DatatypeProperty ;
        rdfs:comment  "A generic property to characterize the age of an entity (as count of years)" ;
        rdfs:label    "Age of an entity" .

:type_act  a                owl:DatatypeProperty ;
        rdfs:comment        "Type of a (legal) act" ;
        rdfs:label          "Type of act" ;
        rdfs:subPropertyOf  :type .

dct:rights  a   owl:AnnotationProperty .

:subdivision_part_of_work
        a                   owl:ObjectProperty ;
        rdfs:comment        "A subdivision is part of a work" ;
        rdfs:domain         :subdivision ;
        rdfs:label          "Subdivision part of work" ;
        rdfs:range          :work ;
        rdfs:subPropertyOf  :part_of ;
        owl:inverseOf       :work_contains_subdivision .

:session_date_end  a  owl:DatatypeProperty ;
        rdfs:label  "Session date end" .

<http://publications.europa.eu/resource/authority/pub_repro>
        a       owl:NamedIndividual .

:manifestation_has_successor_manifestation
        a                   owl:ObjectProperty ;
        rdfs:comment        "manifestation succeeds another manifestation" ;
        rdfs:domain         :manifestation ;
        rdfs:label          "Manifestation has successor of manifestation" ;
        rdfs:range          :manifestation ;
        rdfs:subPropertyOf  :has_successor .

:illustrates  a     owl:ObjectProperty ;
        rdfs:label  "Illustrates" .

:catalogues  a      owl:ObjectProperty ;
        rdfs:label  "Catalogues" .

:pricing_info_belongs_to_manifestation
        a                   owl:ObjectProperty ;
        rdfs:domain         :pricing_info ;
        rdfs:label          "Pricing info of a manifestation" ;
        rdfs:range          :manifestation ;
        rdfs:subPropertyOf  :belongs_to .

:manifestation_has_pricing_info
        a                   owl:ObjectProperty ;
        rdfs:domain         :manifestation ;
        rdfs:label          "Manifestation has pricing info" ;
        rdfs:range          :pricing_info ;
        rdfs:subPropertyOf  :has ;
        owl:inverseOf       :pricing_info_belongs_to_manifestation .

:whoiswho_dataset  a     owl:Class ;
        rdfs:comment     "Datasets representing the EU Whoiswho directory of EU institutions" ;
        rdfs:label       "EU Whoiswho dataset" ;
        rdfs:subClassOf  :work_dataset .

:identifier_extension_number
        a           owl:DatatypeProperty ;
        rdfs:label  "Identifier extension number" .

:act_preparatory_initiates_dossier
        a                   owl:ObjectProperty ;
        rdfs:comment        "This preparatory act, typically a COM, initiates a dossier, typically a procedure. Relevant for legal analysis: true" ;
        rdfs:domain         :act_preparatory ;
        rdfs:label          "Preparatory act initiates a dossier" ;
        rdfs:range          :dossier ;
        rdfs:subPropertyOf  :initiates ;
        owl:inverseOf       :dossier_initiated_by_act_preparatory .

:manifestation_official-journal_part_author_printer
        a                   owl:DatatypeProperty ;
        rdfs:comment        "Author of the legal resource (as seen by the printer). Values such as \"CS\", not currently normalized" ;
        rdfs:domain         :manifestation_official-journal_part ;
        rdfs:label          "Printer's author of the act" ;
        rdfs:range          xsd:string ;
        rdfs:subPropertyOf  :author_printer .

:case-law_ecli  a           owl:DatatypeProperty ;
        rdfs:comment        "European Case Law Identifier. Identifier of the decision, including all its summaries (not necessarily unique in the CELLAR)" ;
        rdfs:domain         :case-law ;
        rdfs:label          "ECLI" ;
        rdfs:range          xsd:string ;
        rdfs:subPropertyOf  :ecli .

:type_reference  a  owl:DatatypeProperty ;
        rdfs:label  "Type reference" .

:procedure_internal_planned_consultation_period_date_end
        a                   owl:DatatypeProperty ;
        rdfs:domain         :procedure_internal ;
        rdfs:label          "Internal procedure: Planned consultation period date end" ;
        rdfs:range          xsd:date ;
        rdfs:subPropertyOf  :planned_consultation_period_date_end .

:section_legal  a        owl:Class ;
        rdfs:label       "Section in a legal resource" ;
        rdfs:subClassOf  :subdivision .

:contract-nature_code
        a           owl:DatatypeProperty ;
        rdfs:label  "Contract nature code" .

:ATTO_FD_608  a              owl:Class ;
        rdfs:label           "FD_608 ATTO table" ;
        rdfs:subClassOf      skos:Concept ;
        owl:equivalentClass  [ a               owl:Restriction ;
                               owl:hasValue    <http://publications.europa.eu/resource/authority/fd_608> ;
                               owl:onProperty  skos:inScheme
                             ] .

:resource_legal_implemented_by_measure_national_implementing
        a                   owl:ObjectProperty ;
        rdfs:domain         :resource_legal ;
        rdfs:label          "Legal resource implemented_by national implementing measure" ;
        rdfs:range          :measure_national_implementing ;
        rdfs:subPropertyOf  :implemented_by ;
        owl:inverseOf       :measure_national_implementing_implements_resource_legal .

:procurement_public_date_deletion
        a                   owl:DatatypeProperty ;
        rdfs:domain         :procurement_public ;
        rdfs:label          "Deletion date" ;
        rdfs:range          xsd:date ;
        rdfs:subPropertyOf  :date_deletion .

:procurement_public_transliterated_attention
        a                   owl:DatatypeProperty ;
        rdfs:domain         :procurement_public ;
        rdfs:label          "Procurement public transliterated attention" ;
        rdfs:range          xsd:string ;
        rdfs:subPropertyOf  :transliterated_attention .

:person_reports_on_opinion_other_cor
        a                   owl:ObjectProperty ;
        rdfs:domain         :person ;
        rdfs:label          "Person reports on opinion_other_cor" ;
        rdfs:range          :opinion_other_cor ;
        rdfs:subPropertyOf  :reports_on .

:planned_adoption_period_date_end
        a           owl:DatatypeProperty ;
        rdfs:label  "Planned adoption period date end" .

:resource_legal_number_corrigendum_eli
        a                   owl:DatatypeProperty ;
        rdfs:comment        "Sequential number of the nth corrigendum in the ELI, needed to disambigutate corrigendum ELIS" ;
        rdfs:domain         :resource_legal ;
        rdfs:label          "Corrigendum number ELI" ;
        rdfs:range          xsd:positiveInteger ;
        rdfs:subPropertyOf  :number_corrigendum_eli .

:page_seq  a        owl:DatatypeProperty ;
        rdfs:label  "Page seq" .

:treaty_stored_by_agent
        a                   owl:ObjectProperty ;
        rdfs:comment        "This points to the name of the depositary of an international agreement. Relevant for legal analysis: true" ;
        rdfs:domain         :treaty ;
        rdfs:label          "Treaty stored by agent" ;
        rdfs:range          :agent ;
        rdfs:subPropertyOf  :stored_by .

:fragment_resource_legal
        a                owl:Class ;
        rdfs:comment     "Fragment of a legal resource (e.g. §2 of the Treaty on European Union and the Treaty establishing the European Community, always linked to that resource)" ;
        rdfs:label       "Legal fragment" ;
        rdfs:subClassOf  :resource_legal ;
        rdfs:subClassOf  [ a                         owl:Restriction ;
                           owl:onClass               :resource_legal ;
                           owl:onProperty            :fragment_resource_legal_part_of_resource_legal ;
                           owl:qualifiedCardinality  "1"^^xsd:nonNegativeInteger
                         ] ;
        rdfs:subClassOf  [ a                owl:Restriction ;
                           owl:cardinality  "1"^^xsd:nonNegativeInteger ;
                           owl:onProperty   :fragment_resource_legal_id_fragment
                         ] .

:event_reported_by_agent
        a             owl:ObjectProperty ;
        rdfs:comment  "The event is reported by a reporting agent (AT corporate body, AT country, other agent entities)" ;
        rdfs:domain   :event ;
        rdfs:label    "Event reported by agent" ;
        rdfs:range    :agent .

:institution_consulted_by_event_legal
        a                   owl:ObjectProperty ;
        rdfs:domain         :institution ;
        rdfs:label          "Institution consulted by legal event" ;
        rdfs:range          :event_legal ;
        rdfs:subPropertyOf  :consulted_by .

:resource_legal_derogates_resource_legal
        a                   owl:ObjectProperty ;
        rdfs:comment        "This property points to act which provision(s) are derogated. Relevant for legal analysis: true" ;
        rdfs:domain         :resource_legal ;
        rdfs:label          "Legal resource derogates legal resource" ;
        rdfs:range          :resource_legal ;
        rdfs:subPropertyOf  :derogates ;
        owl:inverseOf       :resource_legal_derogated_by_resource_legal .

:manifestation_official-journal_pages_total
        a                   owl:DatatypeProperty ;
        rdfs:comment        "DEPRECATED, Total number of pages of the OJ part related to a legal resource. Use manifestion_print_pages_total" ;
        rdfs:domain         :manifestation_official-journal ;
        rdfs:label          "Total pages" ;
        rdfs:range          xsd:string ;
        rdfs:subPropertyOf  :pages_total , :manifestation_print_pages_total ;
        owl:deprecated      true .

:concept_udc_subject_of_publication_general
        a                   owl:ObjectProperty ;
        rdfs:domain         :concept_udc ;
        rdfs:label          "UDC concept is subject of a general publication" ;
        rdfs:range          :publication_general ;
        rdfs:subPropertyOf  :subject_of ;
        owl:inverseOf       :publication_general_is_about_concept_udc .

:joins  a           owl:ObjectProperty ;
        rdfs:label  "Joins" .

:manifestation_rights
        a                   owl:DatatypeProperty ;
        rdfs:comment        "rights on this manifestation. mapped from 540 $a" ;
        rdfs:domain         :manifestation ;
        rdfs:label          "Rights on manifestation" ;
        rdfs:range          xsd:string ;
        rdfs:subPropertyOf  :rights .

:tir_code  a        owl:DatatypeProperty ;
        rdfs:label  "Tir code" .

:domain  a          owl:DatatypeProperty ;
        rdfs:label  "Domain" .

:act_preparatory_council_prefix
        a                   owl:DatatypeProperty ;
        rdfs:comment        "DEPRECATED; Prefix of the identifier the document has at the Council. Standard and official document with the Council logo. E.g. legislative acts, working documents, information notes, agendas, minute, outcome of proceedings and other reports, Standard documents without the Council logo, e.g. EUCO, PE-CONS, ACP-CE, EUROMED, EU-AL, These documents are numbered from 1 to 5000" ;
        rdfs:domain         :act_preparatory_council ;
        rdfs:label          "Prefix" ;
        rdfs:range          xsd:string ;
        rdfs:subPropertyOf  :prefix ;
        owl:deprecated      true .

:transliterated_fax  a  owl:DatatypeProperty ;
        rdfs:label  "Transliterated fax" .

<http://publications.europa.eu/resource/authority/fd_613>
        a       owl:NamedIndividual .

:proposal_act_service_associated
        a                   owl:DatatypeProperty ;
        rdfs:comment        "This field indicates the Commission DG or DGs co-responsible for drafting of an act. DEPRECATED, In the instance data, the property is planned to be replaced with cdm:resource_legal_service_associated at beginning 2019. When this is done this property the property will be removed from CDM. Relevant for legal analysis: true" ;
        rdfs:domain         :proposal_act ;
        rdfs:label          "Service associated" ;
        rdfs:range          xsd:string ;
        rdfs:subPropertyOf  :service_associated , :resource_legal_service_associated ;
        owl:deprecated      true .

:case-law_has_procjur
        a                   owl:ObjectProperty ;
        rdfs:comment        "This field refers to the type of action or procedure by Court proceedings. Coded with http://publications.europa.eu/resource/authority/procjur. It could be annotated by annot:result_decision indicating the results of the action or procedure and pointing to http://publications.europa.eu/resource/authority/procresult." ;
        rdfs:domain         :case-law ;
        rdfs:label          "Case law has a judicial procedure type" ;
        rdfs:range          :procjur ;
        rdfs:subPropertyOf  :has .

<http://publications.europa.eu/resource/authority/class-sum-leg>
        a       owl:NamedIndividual .

:gets_report_of  a  owl:ObjectProperty ;
        rdfs:label  "Gets report of" .

<http://publications.europa.eu/resource/authority/procedure>
        a       owl:NamedIndividual .

:person_reports_on_event_legal
        a                   owl:ObjectProperty ;
        rdfs:comment        "DEPRECATED," ;
        rdfs:domain         :person ;
        rdfs:label          "Person reports on legal event" ;
        rdfs:range          :event_legal ;
        rdfs:subPropertyOf  :reports_on ;
        owl:deprecated      true .

:requests_partial_annulment_of
        a           owl:ObjectProperty ;
        rdfs:label  "Requests partial annulment of" .

:requests_review_of_decision
        a           owl:ObjectProperty ;
        rdfs:label  "Requests review of decision" .

:impact_assessment_needed
        a           owl:DatatypeProperty ;
        rdfs:label  "Impact assessment needed" .

:case-law_delivered_by_court-formation
        a                   owl:ObjectProperty ;
        rdfs:comment        "Reference to the Court formation who delivered the judgement (e.g. AP for Assemblée plénière). cm:work/cm:agent_work/@role=\"FORM_JUG\"" ;
        rdfs:domain         :case-law ;
        rdfs:label          "Case law delivered by court formation" ;
        rdfs:range          :court-formation ;
        rdfs:subPropertyOf  :delivered_by ;
        owl:inverseOf       :court-formation_delivers_case-law .

:event_legal_optionally-consults_institution
        a                   owl:ObjectProperty ;
        rdfs:comment        "Relevant for legal analysis: true. This legal event optionally consults a given institution. Body role:Optional consultation. Relevant for legal analysis: true" ;
        rdfs:domain         :event_legal ;
        rdfs:label          "Legal event optionally consults institution" ;
        rdfs:range          :institution ;
        rdfs:subPropertyOf  :optionally-consults ;
        owl:inverseOf       :institution_optionally-consulted_by_event_legal .

:agent_illustrates_work
        a                   owl:ObjectProperty ;
        rdfs:domain         :agent ;
        rdfs:label          "Agent illustrates a work" ;
        rdfs:range          :work ;
        rdfs:subPropertyOf  :illustrates ;
        owl:inverseOf       :work_illustrated_by_agent .

:resource_legal_date_dispatch
        a                   owl:DatatypeProperty ;
        rdfs:comment        "Contains the date of transmission of: Commission proposals to the Council; European Parliament resolutions to parties concerned; EESC, CoR opinions to the Council and the Commission. DH_COMMENT is mixed content, coded with fd_340. Date of delivery / DH_DATE. Relevant for legal analysis: true" ;
        rdfs:domain         :resource_legal ;
        rdfs:label          "Date of dispatch" ;
        rdfs:range          xsd:date ;
        rdfs:subPropertyOf  :date_dispatch .

:case_court_has_joined_decisions_case-law
        a                   owl:ObjectProperty ;
        rdfs:comment        "Only in IMMC concext" ;
        rdfs:domain         :case_court ;
        rdfs:label          "Case has joined decision" ;
        rdfs:range          :case-law ;
        rdfs:subPropertyOf  :has_joined_decisions .

:ATTO_FD_603  a              owl:Class ;
        rdfs:label           "FD_603 ATTO table" ;
        rdfs:subClassOf      skos:Concept ;
        owl:equivalentClass  [ a               owl:Restriction ;
                               owl:hasValue    <http://publications.europa.eu/resource/authority/fd_603> ;
                               owl:onProperty  skos:inScheme
                             ] .

:agent_publishes_manifestation
        a                   owl:ObjectProperty ;
        rdfs:comment        "Agent acts as publisher of a manifestation" ;
        rdfs:domain         :agent ;
        rdfs:label          "Agent publishes a manifestation" ;
        rdfs:range          :manifestation ;
        rdfs:subPropertyOf  :publishes ;
        owl:inverseOf       :manifestation_published_by_agent .

:document_link  a   owl:DatatypeProperty ;
        rdfs:label  "Document link" .

:court_national_name  a     owl:DatatypeProperty ;
        rdfs:comment        "Name of this national court, possibly qualified by language. e.g. <name.court>High Court</name.court> in JURE" ;
        rdfs:domain         :court_national ;
        rdfs:label          "Name of national Court" ;
        rdfs:range          xsd:string ;
        rdfs:subPropertyOf  :name .

:act_preparatory_organ_other
        a                owl:Class ;
        rdfs:comment     "810 Other organs' or bodies' preparatory acts, e.g. national governments (5XX)" ;
        rdfs:label       "Other organ preparatory act" ;
        rdfs:subClassOf  :act_preparatory .

:manifestation_official-journal_page_last
        a                   owl:DatatypeProperty ;
        rdfs:comment        "DEPRECATED, Last page number of the OJ part related to a legal resource. Use manifestion_print_page_last" ;
        rdfs:domain         :manifestation_official-journal ;
        rdfs:label          "Last page" ;
        rdfs:range          xsd:string ;
        rdfs:subPropertyOf  :page_last , :manifestation_print_page_last ;
        owl:deprecated      true .

:work_is_member_of_complex_work
        a              owl:ObjectProperty ;
        rdfs:comment   "The work is grouped into a complex work" ;
        rdfs:domain    :work ;
        rdfs:label     "Work is member of complex work" ;
        rdfs:range     :complex_work ;
        owl:inverseOf  :complex_work_has_member_work .

:resource_legal_reestablishes_resource_legal
        a                   owl:ObjectProperty ;
        rdfs:comment        "Relevant for legal analysis: true" ;
        rdfs:domain         :resource_legal ;
        rdfs:label          "Legal resource reestablishes legal resource" ;
        rdfs:range          :resource_legal ;
        rdfs:subPropertyOf  :reestablishes ;
        owl:inverseOf       :resource_legal_reestablished_by_resource_legal .

:event_legal_document_link
        a                   owl:DatatypeProperty ;
        rdfs:comment        "Link to an external document / work e.g. in the Council or Parliament register that does not also exist in EUR-Lex. Relevant for legal analysis: true." ;
        rdfs:domain         :event_legal ;
        rdfs:label          "Document link" ;
        rdfs:range          xsd:anyURI ;
        rdfs:subPropertyOf  :document_link .

:case-law_national_act_reference_national
        a                   owl:DatatypeProperty ;
        rdfs:comment        "Reference to provisions of national law applied in the national judgment, e.g. \"Codice di procedura civile, art. 360, 737 e 738\", \"Legge 24/07/1954 no. 722\". Use an XML structure to capture the sequence of references" ;
        rdfs:domain         :case-law_national ;
        rdfs:label          "Reference to provisions of national law" ;
        rdfs:range          rdf:XMLLiteral ;
        rdfs:subPropertyOf  :act_reference_national .

:ATTO_FD_014  a              owl:Class ;
        rdfs:label           "FD_014 ATTO table" ;
        rdfs:subClassOf      skos:Concept ;
        owl:equivalentClass  [ a               owl:Restriction ;
                               owl:hasValue    <http://publications.europa.eu/resource/authority/fd_014> ;
                               owl:onProperty  skos:inScheme
                             ] .

:act_body_parliamentary_agreement_international
        a                owl:Class ;
        rdfs:comment     "Act of parliamentary body created by international agreement (subsector P of sector 2 in Eur-Lex)" ;
        rdfs:label       "Act of parliamentary body created by international agreement" ;
        rdfs:subClassOf  :agreement_international .

:ATTO_FD_555  a              owl:Class ;
        rdfs:label           "FD_555 ATTO table" ;
        rdfs:subClassOf      skos:Concept ;
        owl:equivalentClass  [ a               owl:Restriction ;
                               owl:hasValue    <http://publications.europa.eu/resource/authority/fd_555> ;
                               owl:onProperty  skos:inScheme
                             ] .

:act_preparatory_council
        a                owl:Class ;
        rdfs:comment     "Where: resource_legal_type = (AG; KG; XG), resource_legal_id_sector = 5, work_created_by_agent = CONSIL, work_has_resource-type = (COMMUNIC, COMPOS, POSIT, STAT_REASON, ACT_PREP, PROP_ACT, ASSENT)" , "Preparatory act by the Council of the European Union" ;
        rdfs:label       "Preparatory act by Council" ;
        rdfs:subClassOf  :act_preparatory ;
        rdfs:subClassOf  [ a               owl:Restriction ;
                           owl:hasValue    <http://publications.europa.eu/resource/authority/corporate-body/CONSIL> ;
                           owl:onProperty  :work_created_by_agent
                         ] ;
        rdfs:subClassOf  [ a                   owl:Restriction ;
                           owl:maxCardinality  "1"^^xsd:nonNegativeInteger ;
                           owl:onProperty      :act_preparatory_council_qualifier_document
                         ] ;
        rdfs:subClassOf  [ a                   owl:Restriction ;
                           owl:maxCardinality  "1"^^xsd:nonNegativeInteger ;
                           owl:onProperty      :act_preparatory_council_prefix
                         ] .

:manifestation_court-report_part_pages_total
        a                   owl:DatatypeProperty ;
        rdfs:comment        "DEPRECATED, Total number of pages of the Court report part related to a court document. Use manifestion_print_pages_total" ;
        rdfs:domain         :manifestation_court-report_part ;
        rdfs:label          "Total pages" ;
        rdfs:range          xsd:string ;
        rdfs:subPropertyOf  :pages_total , :manifestation_print_pages_total ;
        owl:deprecated      true .

:has_media_type  a  owl:ObjectProperty ;
        rdfs:label  "Has media type" .

:manifestation_official-journal
        a                owl:Class ;
        rdfs:comment     "Information on the print manifestation of an official journal" ;
        rdfs:label       "Manifestation of the Official Journal" ;
        rdfs:subClassOf  :manifestation_print ;
        rdfs:subClassOf  [ a                   owl:Restriction ;
                           owl:maxCardinality  "1"^^xsd:nonNegativeInteger ;
                           owl:onProperty      :manifestation_official-journal_pages_total
                         ] ;
        rdfs:subClassOf  [ a                   owl:Restriction ;
                           owl:maxCardinality  "1"^^xsd:nonNegativeInteger ;
                           owl:onProperty      :manifestation_official-journal_page_last
                         ] ;
        rdfs:subClassOf  [ a                   owl:Restriction ;
                           owl:maxCardinality  "1"^^xsd:nonNegativeInteger ;
                           owl:onProperty      :manifestation_official-journal_page_first
                         ] .

:resource_legal_reviewed_by_case-law
        a                   owl:ObjectProperty ;
        rdfs:comment        "0 cases (2012-07-31). No example currently existing. Relevant for legal analysis: true." ;
        rdfs:domain         :resource_legal ;
        rdfs:label          "Judgement reviewed by case law" ;
        rdfs:range          :case-law ;
        rdfs:subPropertyOf  :reviewed_by ;
        owl:inverseOf       :case-law_reviews_judgement_resource_legal .

:official-journal-act_part_of_collection_document
        a                   owl:ObjectProperty ;
        rdfs:comment        "The Official Journal act belongs to an OJ collection identified by a concept from AT document-collection." ;
        rdfs:domain         :official-journal-act ;
        rdfs:label          "Official Journal act part of collection document" ;
        rdfs:range          :collection_document ;
        rdfs:subPropertyOf  :part_of ;
        owl:inverseOf       :collection_document_contains_official-journal-act .

:procedure_without_code_interinstitutional_has_status
        a             owl:ObjectProperty ;
        rdfs:comment  "Status of a procedure without an interinstitutional code" ;
        rdfs:domain   :procedure_without_code_interinstitutional ;
        rdfs:label    "Procedure without interinstitutional code has status" ;
        rdfs:range    :status .

<http://publications.europa.eu/resource/authority/fd_040>
        a       owl:NamedIndividual .

:manifestation_signed_by_signature_digital
        a                   owl:ObjectProperty ;
        rdfs:comment        "This manifestation is signed by the following manifestation" ;
        rdfs:domain         :manifestation ;
        rdfs:label          "Manifestation signed by digital signature" ;
        rdfs:range          :signature_digital ;
        rdfs:subPropertyOf  :signed_by ;
        owl:inverseOf       :signature_digital_signs_manifestation .

:opinion_other_committee_ecsc
        a                owl:Class ;
        rdfs:comment     "where its resource_legal_type = AK, resource_legal_id_sector = 5, work_has_resource-type = OPIN" ;
        rdfs:label       "ECSC Committee other opinion" ;
        rdfs:subClassOf  :act_preparatory_ecsc .

:resource_legal_summarized_by_summary_legislation_eu
        a                   owl:ObjectProperty ;
        rdfs:comment        "Resource legal is summarized by summary of EU legislation" ;
        rdfs:domain         :resource_legal ;
        rdfs:label          "Resource legal is summarized by summary of EU legislation" ;
        rdfs:range          :summary_legislation_eu ;
        rdfs:subPropertyOf  :work_summarized_by_summary ;
        owl:inverseOf       :summary_legislation_eu_summarizes_resource_legal .

:agreement_non-member-states
        a                owl:Class ;
        rdfs:comment     "Agreement with non-member states or international organizations (subsector A of sector 2 in Eur-Lex)" ;
        rdfs:label       "Agreement with non-member states" ;
        rdfs:subClassOf  :agreement_international .

:manifestation-audiovisual_read-by_agent
        a                   owl:ObjectProperty ;
        rdfs:comment        "This refers to the narrator of an audiovisual manifestation, e.g., an audiobook" ;
        rdfs:domain         :manifestation-audiovisual ;
        rdfs:label          "Audiovisual manifestation read by agent" ;
        rdfs:range          :agent ;
        rdfs:subPropertyOf  :read_by ;
        dct:created         "2022-08-01T16:18:31.50"^^xsd:dateTime ;
        owl:inverseOf       :agent_reads_manifestation-audiovisual .

:publication_general_source_information
        a                   owl:DatatypeProperty ;
        rdfs:comment        "source of information relating to this general publication" ;
        rdfs:domain         :publication_general ;
        rdfs:label          "Source of information" ;
        rdfs:range          xsd:string ;
        rdfs:subPropertyOf  :source_information .

:container_case-law_type_court_report
        a                   owl:DatatypeProperty ;
        rdfs:comment        "possible values: RG1, RG2, SC" ;
        rdfs:domain         :container_case-law ;
        rdfs:label          "Type court report" ;
        rdfs:range          xsd:string ;
        rdfs:subPropertyOf  :type_court_report .

:act_legislative_other_oj_c_service_responsible
        a                   owl:DatatypeProperty ;
        rdfs:comment        "The Commission DG or DGs responsible for drafting of an act. Relevant for legal analysis: true. DEPRECATED. In the instance data, the property is planned to be replaced with cdm:resource_legal_service_responsible at beginning 2019. When this is done this property will be removed from CDM. The Commission's DG that brought forward the proposal; to be taken from a closed list of DGs (that might be derived from the RECORD project ?). For the backlog data need to be completed. Cardinality to be restricted to 1 in the future." ;
        rdfs:domain         :act_legislative_other_oj_c ;
        rdfs:label          "Service responsible" ;
        rdfs:range          xsd:string ;
        rdfs:subPropertyOf  :service_responsible , :resource_legal_service_responsible ;
        owl:deprecated      true .

:expression_publication_general
        a                owl:Class ;
        rdfs:comment     "Expression specifically of a general publication" ;
        rdfs:label       "General publication expression" ;
        rdfs:subClassOf  :expression ;
        rdfs:subClassOf  [ a                   owl:Restriction ;
                           owl:maxCardinality  "1"^^xsd:nonNegativeInteger ;
                           owl:onProperty      :expression_publication_general_scale
                         ] ;
        rdfs:subClassOf  [ a                   owl:Restriction ;
                           owl:maxCardinality  "1"^^xsd:nonNegativeInteger ;
                           owl:onProperty      :expression_publication_general_projection
                         ] ;
        rdfs:subClassOf  [ a                   owl:Restriction ;
                           owl:maxCardinality  "1"^^xsd:nonNegativeInteger ;
                           owl:onProperty      :expression_publication_general_frequency_expected
                         ] ;
        rdfs:subClassOf  [ a                   owl:Restriction ;
                           owl:maxCardinality  "1"^^xsd:nonNegativeInteger ;
                           owl:onProperty      :expression_publication_general_duration
                         ] ;
        rdfs:subClassOf  [ a                   owl:Restriction ;
                           owl:maxCardinality  "1"^^xsd:nonNegativeInteger ;
                           owl:onProperty      :expression_publication_general_date_processing
                         ] .

:institution  a              owl:Class ;
        rdfs:comment         "Institution (typically public). The class institution has as instances institutions like the European Commission, the European Parliament, the European Council, the Council of the Regions etc. Institutions are defined by the corporate-body table" ;
        rdfs:label           "Institution" ;
        rdfs:subClassOf      skos:Concept , :agent ;
        owl:equivalentClass  [ a               owl:Restriction ;
                               owl:hasValue    <http://publications.europa.eu/resource/authority/corporate-body> ;
                               owl:onProperty  skos:inScheme
                             ] .

<http://eurovoc.europa.eu/100141>
        a       owl:NamedIndividual .

:ATTO_FD_030  a              owl:Class ;
        rdfs:label           "FD_030 ATTO table" ;
        rdfs:subClassOf      skos:Concept ;
        owl:equivalentClass  [ a               owl:Restriction ;
                               owl:hasValue    <http://publications.europa.eu/resource/authority/fd_030> ;
                               owl:onProperty  skos:inScheme
                             ] .

:court-formation_delivers_case-law
        a              owl:ObjectProperty ;
        rdfs:domain    :court-formation ;
        rdfs:label     "Court formation delivers case law" ;
        rdfs:range     :case-law ;
        owl:inverseOf  :case-law_delivered_by_court-formation .

:procurement_public_has_concept_cpv
        a                   owl:ObjectProperty ;
        rdfs:comment        "Public procurement is currently classified against a CPV concept" ;
        rdfs:domain         :procurement_public ;
        rdfs:label          "Public procurement has current CPV concept" ;
        rdfs:range          :concept_cpv ;
        rdfs:subPropertyOf  :has .

:manifestation_type  a      owl:DatatypeProperty ;
        rdfs:comment        "Relevant for legal analysis: true. Type of this manifestation. Possible values are defined in the naming conventions document. Optional as some manifestations might be untyped. Untyped manifestations would, however, only be retrievale through dedicated SPARQL queries. Relevant for legal analysis: true" ;
        rdfs:domain         :manifestation ;
        rdfs:label          "Manifestation type" ;
        rdfs:range          xsd:string ;
        rdfs:subPropertyOf  :type .

:delivered_by_court_depending_on
        a           owl:ObjectProperty ;
        rdfs:label  "Delivered by court depending on" .

:opinion_other_eesc_number_session
        a                   owl:DatatypeProperty ;
        rdfs:comment        "DEPRECATED. Number of session during which this act was debated or voted (EP, EESC, CoR, …). Relevant for legal analysis: true. Mixed content, decoded with fd_345. Use cdm:act_preparatory_number_session" ;
        rdfs:domain         :opinion_other_eesc ;
        rdfs:label          "Number of session" ;
        rdfs:range          xsd:string ;
        rdfs:subPropertyOf  :number_session , :act_preparatory_number_session ;
        owl:deprecated      true .

:manifestation_print_reference_volume
        a                   owl:DatatypeProperty ;
        rdfs:comment        "Volume of the publication. e.g. for DEBAT_PUB_NO or other indication of volumes, DEPRECATED, use manifestion_print_volume" ;
        rdfs:domain         :manifestation_print_reference ;
        rdfs:label          "Volume" ;
        rdfs:range          xsd:string ;
        rdfs:subPropertyOf  :volume , :manifestation_print_volume ;
        owl:deprecated      true .

:co-reported_by  a  owl:ObjectProperty ;
        rdfs:label  "Co reported by" .

:subtitle  a                owl:DatatypeProperty ;
        rdfs:label          "Subtitle" ;
        rdfs:subPropertyOf  :title .

:is-signed  a       owl:DatatypeProperty ;
        rdfs:label  "Is signed" .

:case-law_declares_valid_resource_legal
        a                   owl:ObjectProperty ;
        rdfs:comment        "This property points to legal act quoted in the operative part of Court decisions" ;
        rdfs:domain         :case-law ;
        rdfs:label          "Case law declares valid legal resource" ;
        rdfs:range          :resource_legal ;
        rdfs:subPropertyOf  :declares_valid ;
        owl:inverseOf       :resource_legal_declared_valid_by_case-law .

:documentation_nature_classification
        a            owl:DatatypeProperty ;
        rdfs:domain  :documentation ;
        rdfs:label   "Documentation nature classification" ;
        rdfs:range   xsd:anyURI .

:case-law_declares_void_by_preliminary_ruling_resource_legal
        a                   owl:ObjectProperty ;
        rdfs:comment        "This property points to legal act quoted in the operative part of Court decisions" ;
        rdfs:domain         :case-law ;
        rdfs:label          "Case law declares void by preliminary ruling legal resource" ;
        rdfs:range          :resource_legal ;
        rdfs:subPropertyOf  :declares_void_by_preliminary_ruling ;
        owl:inverseOf       :resource_legal_declared_void_by_preliminary_ruling_case-law .

<http://publications.europa.eu/resource/authority/procjur-type>
        a       owl:NamedIndividual .

:mandatorily-consulted_by
        a           owl:ObjectProperty ;
        rdfs:label  "Mandatorily consulted by" .

:prefix  a          owl:DatatypeProperty ;
        rdfs:label  "Prefix" .

:appendix  a             owl:Class ;
        rdfs:comment     "An ancillary self-contained section of a work, often providing additional but in some sense extra-canonical text (TEI 4.7)" ;
        rdfs:label       "Appendix" ;
        rdfs:subClassOf  :back .

:procedure_internal  a   owl:Class ;
        rdfs:comment     "An arbitrary internal workflow in an institution, e.g. used to model internal workflows in the Commission. Internal procedures will be primariy produced by Institutoins. Whenever mapping IMMC transmissions, whenever possible the corresponding elements of dossier should be used, e.g. - dossier_identifier for the IMMC element /ns4:ec_transmission_request/transmission/workflow/extension/ns3:workflow_id - dossier_is_logical_successor_of_dossier /ns4:ec_transmission_request/transmission/workflow/extension/ns3:workflow_preceding_info - Note that the details of modelling the workflow_id in IMMC is still an open issue (precomposed / decomposed) and that the use of the workflow_type of the preceding workflow needs to be clarified" ;
        rdfs:label       "Internal procedure" ;
        rdfs:subClassOf  :dossier ;
        rdfs:subClassOf  [ a                   owl:Restriction ;
                           owl:maxCardinality  "1"^^xsd:nonNegativeInteger ;
                           owl:onProperty      :procedure_internal_implementation_plan_needed
                         ] ;
        rdfs:subClassOf  [ a                   owl:Restriction ;
                           owl:maxCardinality  "1"^^xsd:nonNegativeInteger ;
                           owl:onProperty      :procedure_internal_impact_assessment_needed
                         ] ;
        rdfs:subClassOf  [ a                   owl:Restriction ;
                           owl:maxCardinality  "1"^^xsd:nonNegativeInteger ;
                           owl:onProperty      :procedure_internal_roadmap_needed
                         ] ;
        rdfs:subClassOf  [ a                   owl:Restriction ;
                           owl:maxCardinality  "1"^^xsd:nonNegativeInteger ;
                           owl:onProperty      :procedure_internal_planned_adoption_period_date_end
                         ] ;
        rdfs:subClassOf  [ a                   owl:Restriction ;
                           owl:maxCardinality  "1"^^xsd:nonNegativeInteger ;
                           owl:onProperty      :procedure_internal_open_public_consultation_needed
                         ] ;
        rdfs:subClassOf  [ a                   owl:Restriction ;
                           owl:maxCardinality  "1"^^xsd:nonNegativeInteger ;
                           owl:onProperty      :procedure_internal_has_status
                         ] ;
        rdfs:subClassOf  [ a                            owl:Restriction ;
                           owl:maxQualifiedCardinality  "1"^^xsd:nonNegativeInteger ;
                           owl:onClass                  :type_procedure_internal ;
                           owl:onProperty               :procedure_internal_has_type_procedure_internal
                         ] ;
        rdfs:subClassOf  [ a                   owl:Restriction ;
                           owl:maxCardinality  "1"^^xsd:nonNegativeInteger ;
                           owl:onProperty      :procedure_internal_planned_consultation_period_date_start
                         ] ;
        rdfs:subClassOf  [ a                   owl:Restriction ;
                           owl:maxCardinality  "1"^^xsd:nonNegativeInteger ;
                           owl:onProperty      :procedure_internal_planned_consultation_period_date_end
                         ] ;
        rdfs:subClassOf  [ a                            owl:Restriction ;
                           owl:maxQualifiedCardinality  "1"^^xsd:nonNegativeInteger ;
                           owl:onClass                  :type_consultation ;
                           owl:onProperty               :procedure_internal_has_type_consultation
                         ] ;
        rdfs:subClassOf  [ a                   owl:Restriction ;
                           owl:maxCardinality  "1"^^xsd:nonNegativeInteger ;
                           owl:onProperty      :procedure_internal_planned_adoption_period_date_start
                         ] ;
        rdfs:subClassOf  [ a                   owl:Restriction ;
                           owl:maxCardinality  "1"^^xsd:nonNegativeInteger ;
                           owl:onProperty      :procedure_internal_draft_to_be_published
                         ] .

:opinion_ecb  a          owl:Class ;
        rdfs:comment     "European Central Bank opinions, usually on draft legislation and requested by another institution (5AB)" ;
        rdfs:label       "European Central Bank opinion" ;
        rdfs:subClassOf  :act_preparatory_ecb .

:case-law_affaire_type
        a                   owl:DatatypeProperty ;
        rdfs:comment        "Type of the affaire. coded" ;
        rdfs:domain         :case-law ;
        rdfs:label          "Affaire: Type" ;
        rdfs:range          xsd:string ;
        rdfs:subPropertyOf  :affaire_type .

:date_modified  a   owl:DatatypeProperty ;
        rdfs:label  "Date modified" .

:resource_legal_derogated_by_resource_legal
        a                   owl:ObjectProperty ;
        rdfs:comment        "Relevant for legal analysis: true" ;
        rdfs:domain         :resource_legal ;
        rdfs:label          "Legal resource derogated by legal resource" ;
        rdfs:range          :resource_legal ;
        rdfs:subPropertyOf  :derogated_by ;
        owl:inverseOf       :resource_legal_derogates_resource_legal .

:part2  a           owl:DatatypeProperty ;
        rdfs:label  "Part2" .

:indicator_decision  a  owl:DatatypeProperty ;
        rdfs:label  "Indicator decision" .

:court-report  a         owl:Class ;
        rdfs:comment     "The Reports of Cases before the Court of Justice and the General Court. The Reports of Cases before the Court of Justice and the General Court, generally known as Court Reports, publishes the collections of documents that belong to one case (e.g. Summary of the Judgment, Opinion of Advocate General and Judgment of the Court). Structually, one publication consists of: - the front matter including the index of subject matter and the table of contents - a series of cases, each in turn composed of the individual documents Some of these documents are already part of sector 6 (e.g. Opinion of Advocate General and Judgment of the Court), others not, e.g. the front matter and the summary. The CDM must therefore model some parts of the court documents as well. To make things more complicated, the summary of the case is in the Court Report separated from the judgement and introduces the complete case (e.g. ECR 2010-1, p. 1f) and joined to the judgement itself in EUR-Lex (e.g. celex 62008CJ0229). A number of key properties such as catalogue number and issn are modelled on the manifestation level as they can vary according to the type of manifestation chosen (e.g. print vs. eBook). One number (= fascicle) of the Court Report can be split over multiple volumes that are conventionally numbered with Latin capital letters, e.g. \"2010 - 1 (A)\" and \"2010 - 1 (B)\". They are consecutively numbered so that \"2010 - 1 (A)\" ends with page 486 and \"2010 - 1 (B)\" starts with page 487. Only the first volume has the front-matter (except for the title page). The CDM therefore treats these volumes as part of one work and only distinguishes the parts of the full Court Report at the item level (i.e. as parts of the various manifestation of the full Court Report). This is, however, probably not in line with the current practice in EU-Bookshop. However, as long as the partial catalogue numbers are stored, the Court Reports would be finable both by the \"global catalogue number\" that is manifestation wide (i.e. for one manifestation of the complete fascicle) and by a catalogue number essentially on item level. The page numbers that an legal resource appears on are part of the legal resource's print publication. So, an individual case law expression will be linked to a manifestation_print that in turn is lnked to the work of the Court Report." ;
        rdfs:label       "Court report" ;
        rdfs:subClassOf  :publication_general ;
        rdfs:subClassOf  [ a                owl:Restriction ;
                           owl:cardinality  "1"^^xsd:nonNegativeInteger ;
                           owl:onProperty   :court-report_year
                         ] ;
        rdfs:subClassOf  [ a                            owl:Restriction ;
                           owl:minQualifiedCardinality  "1"^^xsd:nonNegativeInteger ;
                           owl:onClass                  :document_cjeu ;
                           owl:onProperty               :court-report_publishes_document_cjeu
                         ] ;
        rdfs:subClassOf  [ a                owl:Restriction ;
                           owl:cardinality  "1"^^xsd:nonNegativeInteger ;
                           owl:onProperty   :court-report_number
                         ] ;
        rdfs:subClassOf  [ a                   owl:Restriction ;
                           owl:maxCardinality  "1"^^xsd:nonNegativeInteger ;
                           owl:onProperty      :court-report_class
                         ] .

:cpv_original_link_title
        a           owl:DatatypeProperty ;
        rdfs:label  "Cpv original link title" .

:reexamines  a      owl:ObjectProperty ;
        rdfs:label  "Reexamines" .

:resource_legal_related_to_resource_legal
        a                   owl:SymmetricProperty , owl:ObjectProperty ;
        rdfs:comment        "There is no semantic difference between codes K and L. DEPRECATED in favour of work_related_to_work. Relevant for legal analysis: true" ;
        rdfs:domain         :resource_legal ;
        rdfs:label          "Legal resource is related to legal resource" ;
        rdfs:range          :resource_legal ;
        rdfs:subPropertyOf  :work_related_to_work , :related_to ;
        owl:deprecated      true .

:type_event_internal  a      owl:Class ;
        rdfs:comment         "The type of an event in the internal procedure (draft legislation) of the European Commission" ;
        rdfs:label           "Type of event internal (COM)" ;
        rdfs:subClassOf      skos:Concept , :concept_decoding ;
        owl:equivalentClass  [ a               owl:Restriction ;
                               owl:hasValue    <http://publications.europa.eu/resource/authority/com_internal_event> ;
                               owl:onProperty  skos:inScheme
                             ] .

:procedure_internal_implementation_plan_needed
        a                   owl:DatatypeProperty ;
        rdfs:comment        "Do the better_regulation_requirements require an impact assessment for this internal procedure? /ns4:ec_transmission_request/transmission/workflow/extension/ns3:better_regulation_requirements/ns3:implementation_plan" ;
        rdfs:domain         :procedure_internal ;
        rdfs:label          "Internal procedure needs implementation plan?" ;
        rdfs:range          xsd:boolean ;
        rdfs:subPropertyOf  :implementation_plan_needed .

:resource_legal_number_sequence
        a                   owl:DatatypeProperty ;
        rdfs:comment        "Sequence number of this document. Used to disambiguate ELIs sharing the same natural number, many cases different from number_sequence_celex" ;
        rdfs:domain         :resource_legal ;
        rdfs:label          "Sequence number" ;
        rdfs:range          xsd:positiveInteger ;
        rdfs:subPropertyOf  :number_sequence .

:legislation_secondary_modifies_legislation_secondary
        a                   owl:ObjectProperty ;
        rdfs:comment        "A change or alteration in existing provisions of an act. This property points to act which provision(s) are modified. Relevant for legal analysis: true" ;
        rdfs:domain         :legislation_secondary ;
        rdfs:label          "Secondary legislation modifies secondary legislation" ;
        rdfs:range          :legislation_secondary ;
        rdfs:subPropertyOf  :modifies ;
        owl:inverseOf       :legislation_secondary_modified_by_legislation_secondary .

:case-law_requests_opinion_resource_legal
        a                   owl:ObjectProperty ;
        rdfs:comment        "This property points to legal act quoted in the operative part of Court decisions." ;
        rdfs:domain         :case-law ;
        rdfs:label          "Case law requests an opinion" ;
        rdfs:range          :resource_legal ;
        rdfs:subPropertyOf  :requests_opinion ;
        owl:inverseOf       :resource_legal_opinion_requested_by_case-law .

:manifestation_extent
        a                   owl:DatatypeProperty ;
        rdfs:comment        "extent of this manifestation. mapped from 300 $a" ;
        rdfs:domain         :manifestation ;
        rdfs:label          "Extent of manifeststion" ;
        rdfs:range          xsd:string ;
        rdfs:subPropertyOf  :pages_total , :extent .

:manifestation_print_reference_pages_total
        a                   owl:DatatypeProperty ;
        rdfs:comment        "DEPRECATED, Total number of pages of the OJ part related to a legal resource. Use manifestion_print_pages_total" ;
        rdfs:domain         :manifestation_print_reference ;
        rdfs:label          "Total pages" ;
        rdfs:range          xsd:string ;
        rdfs:subPropertyOf  :pages_total , :manifestation_print_pages_total ;
        owl:deprecated      true .

:procedure_internal_planned_consultation_period_date_start
        a                   owl:DatatypeProperty ;
        rdfs:domain         :procedure_internal ;
        rdfs:label          "Internal procedure: Planned consultation period date start" ;
        rdfs:range          xsd:date ;
        rdfs:subPropertyOf  :planned_consultation_period_date_start .

:pages_total  a     owl:DatatypeProperty ;
        rdfs:label  "Pages total" .

:translated_by  a   owl:ObjectProperty ;
        rdfs:label  "Translated by" .

<http://publications.europa.eu/resource/authority/pub_div>
        a       owl:NamedIndividual .

:part-session_ep  a      owl:Class ;
        rdfs:comment     "This class represents the actual session weeks of the European Parliament, the term part-session is used by the EP" ;
        rdfs:label       "EP part-session" ;
        rdfs:subClassOf  :session .

:resource_legal_incorporated_by_resource_legal
        a                   owl:ObjectProperty ;
        rdfs:comment        "Calculated" ;
        rdfs:domain         :resource_legal ;
        rdfs:label          "Legal resource is incorporated by legal resource" ;
        rdfs:range          :resource_legal ;
        rdfs:subPropertyOf  :incorporated_by ;
        owl:inverseOf       :resource_legal_incorporates_resource_legal .

:resource_legal_consolidated_by_act_consolidated
        a                   owl:ObjectProperty ;
        rdfs:comment        "A set of legal resources consolidated by a Consolidated Act of that resource (typically sector 0) . Typically a consolidated legal resource will be secondary legislation. How do CONSOLID_FICHE and VOLET_DOC_LNK/LNK_CONSLEG play together? According to spec of advanced search the *celexs* of the consolidating acts is to be indexed (= a language independent textual information). This information will be provided in the indexation notice" ;
        rdfs:domain         :resource_legal ;
        rdfs:label          "Legal resources consolidated by Consolidated Act" ;
        rdfs:range          :act_consolidated ;
        rdfs:subPropertyOf  :consolidated_by ;
        owl:inverseOf       :act_consolidated_consolidates_resource_legal .

:dossier_contains_dossier
        a                   owl:ObjectProperty ;
        rdfs:comment        "This dossier contains another dossier" ;
        rdfs:domain         :dossier ;
        rdfs:label          "Dossier contains dossier" ;
        rdfs:range          :dossier ;
        rdfs:subPropertyOf  :contains ;
        owl:inverseOf       :dossier_part_of_dossier .

:concept_new_case-law_subject_of_case-law
        a                   owl:ObjectProperty ;
        rdfs:domain         :concept_new_case-law ;
        rdfs:label          "New case law concept is subject of a case law" ;
        rdfs:range          :case-law ;
        rdfs:subPropertyOf  :subject_of ;
        owl:inverseOf       :case-law_is_about_concept_new_case-law .

:addresses  a       owl:ObjectProperty ;
        rdfs:label  "Addresses" .

<http://publications.europa.eu/resource/authority/event>
        a       owl:NamedIndividual .

:collection  a           owl:Class ;
        rdfs:comment     "An aggregation of resources. A collection is described as a group; its parts may also be separately described." ;
        rdfs:label       "Collection" ;
        rdfs:subClassOf  skos:Concept .

:term-of-office  a  owl:DatatypeProperty ;
        rdfs:label  "Term of office" .

:publication_general_name_meeting
        a                   owl:DatatypeProperty ;
        rdfs:comment        "Meeting name (treated as a special type of title). Marc field 711 a and 711 c | Example: Council of Trent" ;
        rdfs:domain         :publication_general ;
        rdfs:label          "Meeting name" ;
        rdfs:range          rdfs:Literal ;
        rdfs:subPropertyOf  :name_meeting .

:case_court_affects_case_court
        a                   owl:ObjectProperty ;
        rdfs:comment        "This case affects another case" ;
        rdfs:domain         :case_court ;
        rdfs:label          "Case affects case" ;
        rdfs:range          :case_court ;
        rdfs:subPropertyOf  :affects .

:ATTO_FD_396  a              owl:Class ;
        rdfs:label           "FD_396 ATTO table" ;
        rdfs:subClassOf      skos:Concept ;
        owl:equivalentClass  [ a               owl:Restriction ;
                               owl:hasValue    <http://publications.europa.eu/resource/authority/fd_396> ;
                               owl:onProperty  skos:inScheme
                             ] .

:concept_theme_dataset
        a                owl:Class ;
        rdfs:comment     "Corresponds to the contents of the MDR authority list dataset-theme" ;
        rdfs:label       "Concept representing the theme of a dataset" ;
        rdfs:subClassOf  :concept_decoding .

:preamble_part_of_work
        a                   owl:ObjectProperty ;
        rdfs:comment        "This property associates an instance of a work with an instance of a preamble that forms part of it." ;
        rdfs:domain         :preamble ;
        rdfs:label          "Preamble part of work" ;
        rdfs:range          :work ;
        rdfs:subPropertyOf  :subdivision_part_of_work , :part_of ;
        owl:inverseOf       :work_contains_preamble .

:measure_national_implementing_name_official_journal
        a                   owl:DatatypeProperty ;
        rdfs:comment        "National or regional official journal in which this NIM was published" ;
        rdfs:domain         :measure_national_implementing ;
        rdfs:label          "National or regional Official Journal" ;
        rdfs:range          xsd:string ;
        rdfs:subPropertyOf  :name_official_journal .

:event_legal_initiating
        a                   owl:DatatypeProperty ;
        rdfs:comment        "Is this legal event initiating?. Relevant for legal analysis: true." ;
        rdfs:domain         :event_legal ;
        rdfs:label          "Initiating event" ;
        rdfs:range          xsd:boolean ;
        rdfs:subPropertyOf  :initiating .

:resource_legal_amended_by_resource_legal
        a                   owl:ObjectProperty ;
        rdfs:comment        "Calculated. Relevant for legal analysis: true." ;
        rdfs:domain         :resource_legal ;
        rdfs:label          "Legal resource amended by legal resource" ;
        rdfs:range          :resource_legal ;
        rdfs:subPropertyOf  :amended_by ;
        owl:inverseOf       :resource_legal_amends_resource_legal .

:court-formation  a      owl:Class ;
        rdfs:comment     "Formation of a court delivering a decision, e.g.CP Cour plénière" ;
        rdfs:label       "Court formation" ;
        rdfs:subClassOf  :agent ;
        rdfs:subClassOf  [ a                owl:Restriction ;
                           owl:cardinality  "1"^^xsd:nonNegativeInteger ;
                           owl:onProperty   cmr:lastModificationDate
                         ] ;
        rdfs:subClassOf  [ a                   owl:Restriction ;
                           owl:maxCardinality  "1"^^xsd:nonNegativeInteger ;
                           owl:onProperty      cmr:creationDate
                         ] .

:accompanying_material_uses
        a                   owl:ObjectProperty ;
        rdfs:label          "Accompanying material uses" ;
        rdfs:subPropertyOf  :uses .

:work_created_by_agent
        a                   owl:ObjectProperty ;
        rdfs:comment        "Our legacy data was pointing to concepts of fd_010, corporate-body and country table. We have now mapped them all to either corportate-body or country table. Relevant for legal analysis: true.\\\\nRelated authority or tables: Corporate bodies NAL, Countries NAL\\\\nEntries previously using FD_010 have been mapped to either Corporate bodies NAL, Countries NAL. AU. Related authority or tables: Corporate bodies NAL, Countries NAL, ATTO FD_010. Relevant for legal analysis: true" ;
        rdfs:domain         :work ;
        rdfs:label          "Work is created by agent (AU)" ;
        rdfs:range          :agent ;
        rdfs:subPropertyOf  :created_by ;
        dct:created         "2018-07-24T10:04:52.365+02:00"^^xsd:dateTime ;
        owl:inverseOf       :agent_creates_work .

:concept_type_procedure
        a                    owl:Class ;
        rdfs:comment         "Corresponds to the contents of the Procat field PR, coded with FD_Table 100" ;
        rdfs:label           "Concept representing the type of a procedure in case law" ;
        rdfs:subClassOf      skos:Concept , :concept_decoding ;
        owl:equivalentClass  [ a               owl:Restriction ;
                               owl:hasValue    <http://publications.europa.eu/resource/authority/fd_100> ;
                               owl:onProperty  skos:inScheme
                             ] .

:procurement_public_transliterated_country
        a                   owl:DatatypeProperty ;
        rdfs:domain         :procurement_public ;
        rdfs:label          "Procurement public transliterated country" ;
        rdfs:range          xsd:string ;
        rdfs:subPropertyOf  :transliterated_country .

:suspends_application_of
        a           owl:ObjectProperty ;
        rdfs:label  "Suspends application of" .

:ATTO_FD_375  a              owl:Class ;
        rdfs:label           "FD_375 ATTO table" ;
        rdfs:subClassOf      skos:Concept ;
        owl:equivalentClass  [ a               owl:Restriction ;
                               owl:hasValue    <http://publications.europa.eu/resource/authority/fd_375> ;
                               owl:onProperty  skos:inScheme
                             ] .

:expression_case-law_source_ruling_preliminary
        a                   owl:DatatypeProperty ;
        rdfs:comment        "Identifier of the source of the preliminary ruling in the title of a case law document (language-specific)" ;
        rdfs:domain         :expression_case-law ;
        rdfs:label          "Source of preliminary ruling (expression)" ;
        rdfs:range          xsd:string ;
        rdfs:subPropertyOf  :source_ruling_preliminary .

:resource_legal_adopted_by_resource_legal
        a                   owl:ObjectProperty ;
        rdfs:comment        "Never directly specified, inverse property. Relevant for legal analysis: true" ;
        rdfs:domain         :resource_legal ;
        rdfs:label          "Legal resource is adopted by legal resource" ;
        rdfs:range          :resource_legal ;
        rdfs:subPropertyOf  :adopted_by ;
        owl:inverseOf       :resource_legal_adopts_resource_legal .

:opinion_ec  a           owl:Class ;
        rdfs:comment     "313 Commission opinions (5, not PC, with FM=AVIS OR OPIN). Examples: 52011SC1503: Commission opinion appointment of members of the european economic and social committee 52011DC0816: Commission Opinion on the independent expert evaluation on the EIT" ;
        rdfs:label       "Commission opinion" ;
        rdfs:subClassOf  :act_preparatory_ec .

<http://publications.europa.eu/resource/authority/corporate-body/COR>
        a       owl:NamedIndividual .

:green-paper_ec  a       owl:Class ;
        rdfs:label       "Commission Green Paper" ;
        rdfs:subClassOf  :act_preparatory_ec .

:id_doc_related  a  owl:DatatypeProperty ;
        rdfs:label  "Id doc related" .

:partially_suspends  a  owl:ObjectProperty ;
        rdfs:label  "Partially suspends" .

:work_date_document  a      owl:DatatypeProperty ;
        rdfs:comment        "Relevant for legal analysis: true. The date of document (possibly including annotation properties). Relevant for legal analysis: true. DD (comment as annotation). DD_COMMENT is mixed content, decoded with fd_365. DD (comment as annotation). Relevant for legal analysis: true" ;
        rdfs:domain         :work ;
        rdfs:label          "Date of document" ;
        rdfs:range          xsd:date ;
        rdfs:subPropertyOf  :date_document .

:type_court_report  a  owl:DatatypeProperty ;
        rdfs:label  "Type of Court report" .

:source_information  a  owl:DatatypeProperty ;
        rdfs:label  "Source information" .

:communication_judgement
        a                owl:Class ;
        rdfs:comment     "Communication on a Judgement in sector 6" ;
        rdfs:label       "Communication on a judgement" ;
        rdfs:subClassOf  :communication_cjeu .

:used_by_original_translation
        a                   owl:ObjectProperty ;
        rdfs:label          "Used by original translation" ;
        rdfs:subPropertyOf  :used_by .

:date_start_handling  a  owl:DatatypeProperty ;
        rdfs:label  "Date start handling" .

<http://publications.europa.eu/resource/authority/resource-type>
        a       owl:NamedIndividual .

:opinion_consultation_eesc_number_session
        a                   owl:DatatypeProperty ;
        rdfs:comment        "DEPRECATED. Number of session during which this act was debated or voted (EP. EESC, CoR, …). Relevant for legal analysis: true" ;
        rdfs:domain         :opinion_consultation_eesc ;
        rdfs:label          "Number of session" ;
        rdfs:range          xsd:string ;
        rdfs:subPropertyOf  :number_session , :act_preparatory_number_session ;
        owl:deprecated      true .

:following_case-law  a  owl:DatatypeProperty ;
        rdfs:label  "Following case law" .

:expression_case-law_parties
        a                   owl:DatatypeProperty ;
        rdfs:comment        "Parties in the title of a case law document (language-specific)" ;
        rdfs:domain         :expression_case-law ;
        rdfs:label          "Parties" ;
        rdfs:range          xsd:string ;
        rdfs:subPropertyOf  :parties .

<http://publications.europa.eu/resource/authority/fd_380>
        a       owl:NamedIndividual .

:resource_legal_extends_validity_of_resource_legal
        a                   owl:ObjectProperty ;
        rdfs:comment        "This property points to act which validity is extended. Relevant for legal analysis: true" ;
        rdfs:domain         :resource_legal ;
        rdfs:label          "Legal resource extends validity of legal resource" ;
        rdfs:range          :resource_legal ;
        rdfs:subPropertyOf  :extends_validity_of ;
        owl:inverseOf       :resource_legal_validity_extended_by_resource_legal .

:procurement_public_transliterated_address
        a                   owl:DatatypeProperty ;
        rdfs:domain         :procurement_public ;
        rdfs:label          "Procurement public transliterated address" ;
        rdfs:range          xsd:string ;
        rdfs:subPropertyOf  :transliterated_address .

:issued_by  a       owl:ObjectProperty ;
        rdfs:label  "Issued by" .

<http://publications.europa.eu/resource/authority/fd_301>
        a       owl:NamedIndividual .

:work_dataset_date_modified
        a                   owl:DatatypeProperty ;
        rdfs:comment        "This property contains the most recent data on which the dataset was changed or modified" ;
        rdfs:domain         :work_dataset ;
        rdfs:label          "Dataset date modified" ;
        rdfs:range          xsd:date ;
        rdfs:subPropertyOf  :date_modified .

:resource_legal_sequence
        a                   owl:DatatypeProperty ;
        rdfs:comment        "Legal resource sequence number. Added in the context of IMMC2CDM-OJ" ;
        rdfs:domain         :resource_legal ;
        rdfs:label          "Sequence number of the legal resource" ;
        rdfs:range          xsd:positiveInteger ;
        rdfs:subPropertyOf  :sequence .

:publication_other  a    owl:Class ;
        rdfs:comment     "Other types of publications that do not fall into one of the previous classes (e.g. gadgets serving as advertisements, but not contents)" ;
        rdfs:label       "Other publication" ;
        rdfs:subClassOf  :publication_general .

:reference_publication-conclusion
        a           owl:DatatypeProperty ;
        rdfs:label  "Reference publication conclusion" .

:file   a           owl:DatatypeProperty ;
        rdfs:label  "File" .

:relates_to  a      owl:ObjectProperty ;
        rdfs:label  "Relates to" .

:concept_directory-code_subject_of_resource_legal
        a                   owl:ObjectProperty ;
        rdfs:domain         :concept_directory-code ;
        rdfs:label          "Directory code concept is subject of a legal resource" ;
        rdfs:range          :resource_legal ;
        rdfs:subPropertyOf  :subject_of ;
        owl:inverseOf       :resource_legal_is_about_concept_directory-code .

:corrects  a        owl:ObjectProperty ;
        rdfs:label  "Corrects" .

:work_contains_paragraph_legal
        a                   owl:ObjectProperty ;
        rdfs:comment        "The paragraph of this work" ;
        rdfs:domain         :work ;
        rdfs:label          "Work contains paragraph (legal)" ;
        rdfs:range          :paragraph_legal ;
        rdfs:subPropertyOf  :work_contains_subdivision , :contains .

:ATTO_FD_370  a              owl:Class ;
        rdfs:label           "FD_370 ATTO table" ;
        rdfs:subClassOf      skos:Concept ;
        owl:equivalentClass  [ a               owl:Restriction ;
                               owl:hasValue    <http://publications.europa.eu/resource/authority/fd_370> ;
                               owl:onProperty  skos:inScheme
                             ] .

:resource_legal_opinion_requested_by_case-law
        a                   owl:ObjectProperty ;
        rdfs:comment        "2 cases (2012-07-31). Example: 62008CU0001: \"request for opinion 12006E133 P1\". Relevant for legal analysis: true" ;
        rdfs:domain         :resource_legal ;
        rdfs:label          "Opinion on legal resource requested by case law" ;
        rdfs:range          :case-law ;
        rdfs:subPropertyOf  :opinion_requested_by ;
        owl:inverseOf       :case-law_requests_opinion_resource_legal .

:manifestation_special-court-report_part_type
        a                   owl:DatatypeProperty ;
        rdfs:comment        "Type of the special court report. Temporary solution" ;
        rdfs:domain         :manifestation_special-court-report_part ;
        rdfs:label          "Type of the special court report" ;
        rdfs:range          xsd:string ;
        rdfs:subPropertyOf  :type .

:reference-data_publication_publishes_reference-data_asset
        a                   owl:ObjectProperty ;
        rdfs:comment        "A publication containing a specific reference data asset" ;
        rdfs:domain         :reference-data_publication ;
        rdfs:label          "Reference data publication published reference data asset" ;
        rdfs:range          :reference-data_asset ;
        rdfs:subPropertyOf  :publishes ;
        owl:inverseOf       :reference-data_asset_published_in_reference-data_publication .

<http://publications.europa.eu/resource/authority/corporate-body/COM>
        a       owl:NamedIndividual .

:type_procedure_internal
        a                    owl:Class ;
        rdfs:comment         "Type of an internal procedure (draft legislation) of the European Commission" ;
        rdfs:label           "Type of internal procedure (COM)" ;
        rdfs:subClassOf      skos:Concept , :concept_decoding ;
        rdfs:subClassOf      [ a                            owl:Restriction ;
                               owl:maxQualifiedCardinality  "1"^^xsd:nonNegativeInteger ;
                               owl:onClass                  :procedure_internal ;
                               owl:onProperty               :type_procedure_internal_is_type_of_procedure_internal
                             ] ;
        owl:equivalentClass  [ a               owl:Restriction ;
                               owl:hasValue    <http://publications.europa.eu/resource/authority/com_internal_procedure> ;
                               owl:onProperty  skos:inScheme
                             ] .

:item_belongs_to_manifestation
        a                   owl:ObjectProperty ;
        rdfs:comment        "An item belongs to a given manifestation" ;
        rdfs:domain         :item ;
        rdfs:label          "Item belongs to manifestation" ;
        rdfs:range          :manifestation ;
        rdfs:subPropertyOf  :belongs_to ;
        owl:inverseOf       :manifestation_has_item .

:id_numpub  a       owl:DatatypeProperty ;
        rdfs:label  "Id numpub" .

:decision_review_cjeu
        a                owl:Class ;
        rdfs:comment     "Corresponds to DEC_REVIEW in resource-type table" ;
        rdfs:label       "Decision to review of the Court of Justice" ;
        rdfs:subClassOf  :case-law .

:event_case_part2  a        owl:DatatypeProperty ;
        rdfs:comment        "Part 2 of the legal basis of the procedure. typical values such as BCE" ;
        rdfs:domain         :event_case ;
        rdfs:label          "Part 2 of the legal basis of the procedure" ;
        rdfs:range          xsd:string ;
        rdfs:subPropertyOf  :part2 .

:ATTO_FD_285  a              owl:Class ;
        rdfs:label           "FD_285 ATTO table" ;
        rdfs:subClassOf      skos:Concept ;
        owl:equivalentClass  [ a               owl:Restriction ;
                               owl:hasValue    <http://publications.europa.eu/resource/authority/fd_285> ;
                               owl:onProperty  skos:inScheme
                             ] .

:clause_legal_part_of_work
        a                   owl:ObjectProperty ;
        rdfs:comment        "This property associates an instance of a work with an instance of a close that forms part of it." ;
        rdfs:domain         :clause_legal ;
        rdfs:label          "Clause (legal) part of work" ;
        rdfs:range          :work ;
        rdfs:subPropertyOf  :subdivision_part_of_work , :part_of ;
        owl:inverseOf       :work_contains_clause_legal .

:authored_by  a     owl:ObjectProperty ;
        rdfs:label  "Authored by" .

:system_requirements  a  owl:DatatypeProperty ;
        rdfs:label  "System requirements" .

:publication_general_has_target_audience
        a                   owl:ObjectProperty ;
        rdfs:comment        "Intended audience of a publication" ;
        rdfs:domain         :publication_general ;
        rdfs:label          "General publication has target audience" ;
        rdfs:range          :target_audience ;
        rdfs:subPropertyOf  :has ;
        owl:inverseOf       :target_audience_belongs_to_publication_general .

:regulation  a           owl:Class ;
        rdfs:comment     "Regulation (subsector R of sector 3). At present 75662 notices" ;
        rdfs:label       "Regulation" ;
        rdfs:subClassOf  :legislation_secondary .

:published_by  a    owl:ObjectProperty ;
        rdfs:label  "Published by" .

:event_involves_agent
        a                   owl:ObjectProperty ;
        rdfs:comment        "Relevant for legal analysis: true. This event involves a specific agent (related to CIDOC CRM's P11 had participant (participated in): E39 Actor). Relevant for legal analysis: true" ;
        rdfs:domain         :event ;
        rdfs:label          "Event involves agent" ;
        rdfs:range          :agent ;
        rdfs:subPropertyOf  :involves .

:directive_service_responsible
        a                   owl:DatatypeProperty ;
        rdfs:comment        "The Commission DG or DGs responsible for drafting of an act. DEPRECATED, In the instance data, the property is planned to be replaced with cdm:resource_legal_service_responsible at beginning 2019. When this is done this property the property will be removed from CDM. The Commission's DG that brought forward the proposal; to be taken from a closed list of DGs (that might be derived from the RECORD project ?). For the backlog data need to be completed. Cardinality to be restricted to 1 in the future. Relevant for legal analysis: true" ;
        rdfs:domain         :directive ;
        rdfs:label          "Service responsible" ;
        rdfs:range          xsd:string ;
        rdfs:subPropertyOf  :service_responsible , :resource_legal_service_responsible .

:type_consultation_is_type_of_procedure_internal
        a             owl:ObjectProperty ;
        rdfs:comment  "Consultation type of an internal procedure. procedure_internal associated to com_internal_consultation_type" ;
        rdfs:domain   :type_consultation ;
        rdfs:label    "Consultation type of an internal procedure" ;
        rdfs:range    :procedure_internal .

:manifestation_is_included_in_expression
        a            owl:ObjectProperty ;
        rdfs:domain  :manifestation ;
        rdfs:label   "Manifestation is included in expression" ;
        rdfs:range   :expression ;
        dct:created  "2018-08-13T12:30:59.225+02:00"^^xsd:dateTime .

:procurement_public_regulation_code
        a                   owl:DatatypeProperty ;
        rdfs:domain         :procurement_public ;
        rdfs:label          "Regulation code of the contract" ;
        rdfs:range          xsd:string ;
        rdfs:subPropertyOf  :regulation_code .

:objection_period  a  owl:DatatypeProperty ;
        rdfs:label  "Objection period" .

:associates  a      owl:ObjectProperty ;
        rdfs:label  "Associates" .

:case_court_subject_to_appeal_in_case-law
        a              owl:ObjectProperty ;
        rdfs:domain    :case_court ;
        rdfs:label     "Case court subject to appeal in case law" ;
        rdfs:range     :case-law ;
        owl:inverseOf  :case-law_subject_to_appeal_in_case_court .

:case-law_judgement_national
        a                   owl:DatatypeProperty ;
        rdfs:comment        "DEPRECATED, Reference a un jugement prononce par un tribunal national ayant donne lieu à un renvoi. NC / national court" ;
        rdfs:domain         :case-law ;
        rdfs:label          "National judgement" ;
        rdfs:range          xsd:string ;
        rdfs:subPropertyOf  :judgement_national ;
        owl:deprecated      true .

:document_other_efta  a  owl:Class ;
        rdfs:comment     "Other documents from the European Free Trade Association (EFTA) (= subsector O of sector E in EUR-Lex)" ;
        rdfs:label       "Other EFTA document" ;
        rdfs:subClassOf  :document_efta .

:communication_case_new_requests_inapplicability_resource_legal
        a                   owl:ObjectProperty ;
        rdfs:comment        "This property points to legal act quoted in the communication on a new case published in OJ. Relevant for legal analysis: true" ;
        rdfs:domain         :communication_case_new ;
        rdfs:label          "Communication requesting the inapplicability of a legal resource" ;
        rdfs:range          :resource_legal ;
        rdfs:subPropertyOf  :requests_inapplicability ;
        owl:inverseOf       :resource_legal_inapplicability_requested_by_communication_case_new .

:proposal_act_service_responsible
        a                   owl:DatatypeProperty ;
        rdfs:comment        "The Commission DG or DGs responsible for drafting of an act. Relevant for legal analysis: true. DEPRECATED. In the instance data, the property is planned to be replaced with cdm:resource_legal_service_responsible at beginning 2019. When this is done this property will be removed from CDM. The Commission's DG that brought forward the proposal; to be taken from a closed list of DGs (that might be derived from the RECORD project ?). For the backlog data need to be completed. Cardinality to be restricted to 1 in the future" ;
        rdfs:domain         :proposal_act ;
        rdfs:label          "Service responsible" ;
        rdfs:range          xsd:string ;
        rdfs:subPropertyOf  :service_responsible , :resource_legal_service_responsible ;
        owl:deprecated      true .

:resource_legal_signatory_function2
        a                   owl:DatatypeProperty ;
        rdfs:comment        "Legal resource signatory function. Added in the context of IMMC2CDM-OJ. Relevant for legal analysis: true" ;
        rdfs:domain         :resource_legal ;
        rdfs:label          "Function of second signatory of the legal resource" ;
        rdfs:range          xsd:string ;
        rdfs:subPropertyOf  :signatory_function2 .

:obsolete  a        owl:DatatypeProperty ;
        rdfs:label  "Obsolete" .

:procurement_public_xml-schema-definition_reference
        a                   owl:DatatypeProperty ;
        rdfs:domain         :procurement_public ;
        rdfs:label          "Reference for the schema definition" ;
        rdfs:range          xsd:anyURI ;
        rdfs:subPropertyOf  :xml-schema-definition_reference .

:entity_temporal  a   owl:Class ;
        rdfs:comment  "Cf. [http://cidoc.ics.forth.gr/official_release_cidoc.html] for the specification of the CIDOC CRM itself and [http://bloody-byte.net/rdf/cidoc-crm/core_5.0.1.rdf] for its OWL mapping" ;
        rdfs:label    "Temporal entity" .

:framework_procedural_sequential-number_type_procedure
        a           owl:DatatypeProperty ;
        rdfs:label  "Framework procedural sequential number type procedure" .

:information-communication_efta
        a                owl:Class ;
        rdfs:comment     "European Free Trade Association (EFTA) information and communication (= subsector X of sector E in EUR-Lex)" ;
        rdfs:label       "EFTA information and communication" ;
        rdfs:subClassOf  :document_efta .

<http://publications.europa.eu/resource/authority/fd_609>
        a       owl:NamedIndividual .

:planned_adoption_period_date_start
        a           owl:DatatypeProperty ;
        rdfs:label  "Planned adoption period date start" .

:procurement_public_datetime_request
        a                   owl:DatatypeProperty ;
        rdfs:domain         :procurement_public ;
        rdfs:label          "Request date" ;
        rdfs:range          xsd:dateTime ;
        rdfs:subPropertyOf  :datetime_request .

:expression_is_incorporated_in_expression
        a             owl:ObjectProperty ;
        rdfs:comment  "Indication if the expression has to be considered a part of another expression" ;
        rdfs:domain   :expression ;
        rdfs:label    "Expression is incorporated in expression" ;
        rdfs:range    :expression .

:resource_legal_number_natural_celex
        a                   owl:DatatypeProperty ;
        rdfs:comment        "Number part of the Celex identifier (DTN). Relevant for legal analysis: true" ;
        rdfs:domain         :resource_legal ;
        rdfs:label          "Natural number (celex)" ;
        rdfs:range          xsd:positiveInteger ;
        rdfs:subPropertyOf  :number_natural_celex .

:manifestation-mobile-app_access-url
        a                   owl:DatatypeProperty ;
        rdfs:comment        "This property contains an URL that gives access to the mobile application in the app store. The resource at the access URL may contain information about how to get the mobile application." ;
        rdfs:domain         :manifestation-mobile-app ;
        rdfs:label          "Mobile application access URL" ;
        rdfs:range          xsd:anyURI ;
        rdfs:subPropertyOf  :access_url ;
        dct:created         "2022-08-01T16:18:31.50"^^xsd:dateTime .

:procurement_public_cpv_original_link_title
        a                   owl:DatatypeProperty ;
        rdfs:domain         :procurement_public ;
        rdfs:label          "CPV orignal title" ;
        rdfs:range          xsd:string ;
        rdfs:subPropertyOf  :cpv_original_link_title .

:work_dataset_has_documentation_documentation
        a                   owl:ObjectProperty ;
        rdfs:comment        "Indicates the resource which documents the dataset" ;
        rdfs:domain         :work_dataset ;
        rdfs:label          "Documentation" ;
        rdfs:range          :documentation ;
        rdfs:subPropertyOf  :work_explained_by_work , :has_documentation ;
        owl:inverseOf       :documentation_documents_work_dataset .

:expressed_in  a    owl:ObjectProperty ;
        rdfs:label  "Expressed in" .

:incidentally_declared_void_by
        a           owl:ObjectProperty ;
        rdfs:label  "Incidentally declared void by" .

:session_council  a   owl:DatatypeProperty ;
        rdfs:comment  "Council session" ;
        rdfs:label    "Session council" .

:datetime_negotiation
        a             owl:ObjectProperty ;
        rdfs:comment  "This object property indicates which metadata field should be taken into account during datetime negotiation. The property is part of the instance data" ;
        rdfs:domain   :evolutive_work ;
        rdfs:label    "Datetime negotiation" ;
        rdfs:range    owl:DatatypeProperty .

dct:title  a    owl:AnnotationProperty .

:procedure_code_interinstitutional_has_status
        a             owl:ObjectProperty ;
        rdfs:comment  "Status of a procedure with an interinstitutional code" ;
        rdfs:domain   :procedure_code_interinstitutional ;
        rdfs:label    "Procedure with interinstitutional code has status" ;
        rdfs:range    :status .

:case-law_national_preceeding_case-law
        a                   owl:DatatypeProperty ;
        rdfs:comment        "The case law has a predecessor. see 81986DE0828(01) or 81998UK0408(01)" ;
        rdfs:domain         :case-law_national ;
        rdfs:label          "Preceeding case law" ;
        rdfs:range          xsd:string ;
        rdfs:subPropertyOf  :preceeding_case-law .

:case_court_efta_pending
        a                owl:Class ;
        rdfs:comment     "Pending case of the EFTA Court (= subsector P of sector E)" ;
        rdfs:label       "EFTA pending court case" ;
        rdfs:subClassOf  :document_efta .

:does_impact_of  a  owl:ObjectProperty ;
        rdfs:label  "Does impact of" .

:establishes_failure_to_fulfill_obligation_requested_by
        a           owl:ObjectProperty ;
        rdfs:label  "Establishes failure to fulfill obligation requested by" .

:work_dataset_landing_page
        a                   owl:DatatypeProperty ;
        rdfs:comment        "This property refers to a Web page that provide access to the dataset, its distributions and/or additional information" ;
        rdfs:domain         :work_dataset ;
        rdfs:label          "Dataset landing page" ;
        rdfs:range          xsd:anyURI ;
        rdfs:subPropertyOf  :landing_page .

:procurement_public_issued_by_country
        a                   owl:ObjectProperty ;
        rdfs:comment        "Public procurement notice issued by a given country" ;
        rdfs:domain         :procurement_public ;
        rdfs:label          "Public procurement issued by country" ;
        rdfs:range          :country ;
        rdfs:subPropertyOf  :issued_by .

:manifestation_court-report
        a                owl:Class ;
        rdfs:comment     "Information on the print manifestation of a court report" ;
        rdfs:label       "Manifestation of the Court report" ;
        rdfs:subClassOf  :manifestation_print ;
        rdfs:subClassOf  [ a                            owl:Restriction ;
                           owl:maxQualifiedCardinality  "1"^^xsd:nonNegativeInteger ;
                           owl:onClass                  :type_court-report ;
                           owl:onProperty               :manifestation_court-report_belongs_to_type_court-report
                         ] .

:concept_type_procedure_code_interinstitutional
        a                    owl:Class ;
        rdfs:comment         "Now coded with table 609 In Pegase <COTEII proc=\"COD\" libproc=\"Procédure législative ordinaire\" annee=\"2010\" numero=\"36\"/><COTEII proc=\"APP\" libproc=\"procédure législative spéciale (approbation du PE)\" annee=\"2010\" numero=\"48\"/> In PROCEDURE prelex translation table <LIBELLE CODE=\"1010\">Procédure de codécision</LIBELLE><LIBELLE CODE=\"1030\">procédure législative spéciale (approbation du PE)</LIBELLE><LIBELLE CODE=\"1010_CODE\">COD</LIBELLE><LIBELLE CODE=\"1030_CODE\">APP</LIBELLE>" ;
        rdfs:label           "Concept representing the type of a procedure with interinstitutional code" ;
        rdfs:subClassOf      skos:Concept , :concept_decoding ;
        owl:equivalentClass  [ a               owl:Restriction ;
                               owl:hasValue    <http://publications.europa.eu/resource/authority/procedure> ;
                               owl:onProperty  skos:inScheme
                             ] .

:manifestation_official-journal_part
        a                owl:Class ;
        rdfs:comment     "Information on the print manifestation of an act. These values are set by the printer in the production process, are incoporated in the prenotice and (except for the page numbers) not necessarily very reliable. The juridical analysis has always priority" ;
        rdfs:label       "Part of an manifestation of the Official Journal" ;
        rdfs:subClassOf  :manifestation_print ;
        rdfs:subClassOf  [ a                   owl:Restriction ;
                           owl:maxCardinality  "1"^^xsd:nonNegativeInteger ;
                           owl:onProperty      :manifestation_official-journal_part_section_oj
                         ] ;
        rdfs:subClassOf  [ a                   owl:Restriction ;
                           owl:maxCardinality  "1"^^xsd:nonNegativeInteger ;
                           owl:onProperty      :manifestation_official-journal_part_durability
                         ] ;
        rdfs:subClassOf  [ a                owl:Restriction ;
                           owl:cardinality  "1"^^xsd:nonNegativeInteger ;
                           owl:onProperty   :manifestation_official-journal_part_page_first
                         ] ;
        rdfs:subClassOf  [ a                   owl:Restriction ;
                           owl:maxCardinality  "1"^^xsd:nonNegativeInteger ;
                           owl:onProperty      :manifestation_official-journal_part_typedoc_printer
                         ] ;
        rdfs:subClassOf  [ a                   owl:Restriction ;
                           owl:maxCardinality  "1"^^xsd:nonNegativeInteger ;
                           owl:onProperty      :manifestation_official-journal_part_page_seq
                         ] ;
        rdfs:subClassOf  [ a                   owl:Restriction ;
                           owl:maxCardinality  "1"^^xsd:nonNegativeInteger ;
                           owl:onProperty      :manifestation_official-journal_part_year
                         ] ;
        rdfs:subClassOf  [ a                   owl:Restriction ;
                           owl:maxCardinality  "1"^^xsd:nonNegativeInteger ;
                           owl:onProperty      :manifestation_official-journal_part_natural_number
                         ] ;
        rdfs:subClassOf  [ a                   owl:Restriction ;
                           owl:maxCardinality  "1"^^xsd:nonNegativeInteger ;
                           owl:onProperty      :manifestation_official-journal_part_volume_oj
                         ] ;
        rdfs:subClassOf  [ a                   owl:Restriction ;
                           owl:maxCardinality  "1"^^xsd:nonNegativeInteger ;
                           owl:onProperty      :manifestation_official-journal_part_subsection_oj
                         ] ;
        rdfs:subClassOf  [ a                   owl:Restriction ;
                           owl:maxCardinality  "1"^^xsd:nonNegativeInteger ;
                           owl:onProperty      :manifestation_official-journal_part_pages_total
                         ] ;
        rdfs:subClassOf  [ a                owl:Restriction ;
                           owl:cardinality  "1"^^xsd:nonNegativeInteger ;
                           owl:onProperty   :manifestation_official-journal_part_page_last
                         ] ;
        rdfs:subClassOf  [ a                   owl:Restriction ;
                           owl:maxCardinality  "1"^^xsd:nonNegativeInteger ;
                           owl:onProperty      :manifestation_official-journal_part_formatting
                         ] .

:subject-matter  a           owl:Class ;
        rdfs:comment         "Concept used for a subject heading. Currently, subject headings are captured in the VOLET_DOC_BIB/CT field and are coded according to FD_TABLE 070. The field is in the methodology manual also referred to as ET" ;
        rdfs:label           "Subject matter" ;
        rdfs:subClassOf      skos:Concept , :concept ;
        owl:equivalentClass  [ a               owl:Restriction ;
                               owl:hasValue    <http://publications.europa.eu/resource/authority/subject-matter> ;
                               owl:onProperty  skos:inScheme
                             ] ;
        owl:equivalentClass  [ a               owl:Restriction ;
                               owl:hasValue    <http://publications.europa.eu/resource/authority/fd_070> ;
                               owl:onProperty  skos:inScheme
                             ] .

:expression_publication_general_information_miscellaneous
        a                   owl:DatatypeProperty ;
        rdfs:comment        "Miscellaneous information" ;
        rdfs:domain         :expression_publication_general ;
        rdfs:label          "Miscellaneous information for a general publication" ;
        rdfs:range          xsd:string ;
        rdfs:subPropertyOf  :information_miscellaneous .

:procurement_public_official-forms_reference
        a                   owl:DatatypeProperty ;
        rdfs:domain         :procurement_public ;
        rdfs:label          "Reference for the official forms" ;
        rdfs:range          xsd:anyURI ;
        rdfs:subPropertyOf  :official-forms_reference .

:resource_legal_added_to_resource_legal
        a                   owl:ObjectProperty ;
        rdfs:comment        "DEPRECATED Never directly specified, inverse property. Relevant for legal analysis: true" ;
        rdfs:domain         :resource_legal ;
        rdfs:label          "Legal resource added to legal resource" ;
        rdfs:range          :resource_legal ;
        rdfs:subPropertyOf  :added_to ;
        owl:inverseOf       :resource_legal_adds_to_resource_legal .

:case_court_affected_by_case_court
        a                   owl:ObjectProperty ;
        rdfs:comment        "This case affected by another case" ;
        rdfs:domain         :case_court ;
        rdfs:label          "Case affected by case" ;
        rdfs:range          :case_court ;
        rdfs:subPropertyOf  :affected_by ;
        owl:inverseOf       :case_court_affects_case_court .

:consolidated_by  a  owl:ObjectProperty ;
        rdfs:label  "Consolidated by" .

:nuts_original_reference
        a           owl:DatatypeProperty ;
        rdfs:label  "Nuts original reference" .

:concept_mode_decision
        a                    owl:Class ;
        rdfs:comment         "Now coded with table 606 Example: <MODE_DECISION id=\"1005\">Procédure orale</MODE_DECISION><LIBELLE CODE=\"1005\">Procédure orale</LIBELLE>" ;
        rdfs:label           "Concept representing the decision mode in Prelex" ;
        rdfs:subClassOf      skos:Concept , :concept_decoding ;
        owl:equivalentClass  [ a               owl:Restriction ;
                               owl:hasValue    <http://publications.europa.eu/resource/authority/fd_606> ;
                               owl:onProperty  skos:inScheme
                             ] .

:keywords  a        owl:DatatypeProperty ;
        rdfs:label  "Keywords" .

:original_translation_uses
        a                   owl:ObjectProperty ;
        rdfs:label          "Original translation uses" ;
        rdfs:subPropertyOf  :uses .

:event_legal_has_remark_concept_type_remark
        a                   owl:ObjectProperty ;
        rdfs:comment        "Legal event has a remark, taken from FD table 600. Relevant for legal analysis: true.. Remarks" ;
        rdfs:domain         :event_legal ;
        rdfs:label          "Legal event has remark" ;
        rdfs:range          :concept_type_remark ;
        rdfs:subPropertyOf  :has_remark .

:procjur-type  a             owl:Class ;
        rdfs:comment         "Values currently used in the Court schema: R, I, P Traced in MDR-1936" ;
        rdfs:label           "Concept representing types of procedures in a court case" ;
        rdfs:subClassOf      skos:Concept , :concept_decoding ;
        owl:equivalentClass  [ a               owl:Restriction ;
                               owl:hasValue    <http://publications.europa.eu/resource/authority/procjur-type> ;
                               owl:onProperty  skos:inScheme
                             ] .

:signature_digital  a    owl:Class ;
        rdfs:comment     "A digital signature in the Commission model is a standalone signature file related to (typically) one OJ, Special Edition of the OJ or Court report with all its expressions and pdf manifestations (full and toc) as well as all its acts. It is a plain vanilla work with the only special relationship \"signs\". No specific properties are defined for their expressions (per default, the language \"English\" should be set) and manifestations. Manifestations point to XML files with names such as CE2010256.sig.xml Two signatures are sent, one being the main signature itself (signature XAdES-T and XAdES-A = archival electronic signatures). At the date of publishing of the electronic OJ (pdf on eurlex) only XAdES-T signature will be available, XAdES-A signatures will be added to the CELLAR as soon as they become available. It will replace the original XAdES-T file of the manifestation. In principle, it is always the individual PDF/A-1a manifestation that is signed: {code} +--------------------------------------+ +-----------------------------------------+ | +-----------------------+ | | +--------------------------------+ | | | Digital Signature | |-- | | Work (e.g. OJ or act) | | | +-----------------------+ | \\- . | +--------------------------------+ | | | \\- | | +--------------------------------------+ \\- +-----------------------------------------+ \\- \\- - +--------------------------------------+ \\- Signs / +-----------------------------------------+ | +-----------------------+ | \\- | +-------------------------------+ | | | Expression | | \\- Signed by | | Expression | | | +-----------------------+ | \\- | +-------------------------------+ | | Fixed title | \\- | | +--------------------------------------+ \\- +-----------------------------------------+ \\- \\- +--------------------------------------+ \\- +-------------------------------------------+ | +-----------------------+ | \\- | +-----------------------------+ | | | Manifestation - | | \\+ | Manifestation (pdfa1a) | | - | +-----------------------+ | | +-----------------------------+ | | Signature (xml), Type | | | +--------------------------------------+ +-------------------------------------------+ +--------------------------------------+ | +-----------------------+ | | | Item | | | +-----------------------+ | | | +--------------------------------------+ {code} Once signatures are up for renewal, typically after a period of four years, this might be captured e.g. by adding a new manifestation encapsulating this file. Alternatively, the current manifestation might be updated to contain the renewed signature. This question will be clarified at the appropriate moment in collaboration with Dokumenta, the company providing the signature system." ;
        rdfs:label       "Digital signature" ;
        rdfs:subClassOf  :work ;
        rdfs:subClassOf  [ a                   owl:Restriction ;
                           owl:maxCardinality  "1"^^xsd:nonNegativeInteger ;
                           owl:onProperty      :signature_digital_authority_certification
                         ] ;
        rdfs:subClassOf  [ a                owl:Restriction ;
                           owl:cardinality  "1"^^xsd:nonNegativeInteger ;
                           owl:onProperty   :signature_digital_date_signature_xades-t
                         ] ;
        rdfs:subClassOf  [ a                            owl:Restriction ;
                           owl:minQualifiedCardinality  "1"^^xsd:nonNegativeInteger ;
                           owl:onClass                  :manifestation ;
                           owl:onProperty               :signature_digital_signs_manifestation
                         ] ;
        rdfs:subClassOf  [ a                   owl:Restriction ;
                           owl:maxCardinality  "1"^^xsd:nonNegativeInteger ;
                           owl:onProperty      :signature_digital_date_signature_xades-a
                         ] ;
        rdfs:subClassOf  [ a                owl:Restriction ;
                           owl:cardinality  "1"^^xsd:nonNegativeInteger ;
                           owl:onProperty   :signature_digital_type
                         ] ;
        rdfs:subClassOf  [ a                owl:Restriction ;
                           owl:cardinality  "1"^^xsd:nonNegativeInteger ;
                           owl:onProperty   :signature_digital_date_expiration
                         ] .

:manifestation  a        owl:Class ;
        rdfs:comment     "\"A class whose members are the physical embodiment of one or more expressions\" (FRBR) Digital Objects will be stored as such in the CCR. They will bundle all electronic formats of a given expression (\"data streams\") and the CMR will just contain a placeholder object that references the digital object. As per the 2010-08-09 meeting with IRIS this will include the represtation of the manifestations representing physical objects (e.g. JO-L 123 of 1999), linked to the physical object in question. For information, here the list of original manifestation classes: * Manifestation of Official Journal: Component (based on information from VOLET_DOC_LNK) * Manifestation of Print Publication * Manifestation of Official Journal: Aggregation * Manifestation of Recueil de la Jurisprudence * Other Manifestation" ;
        rdfs:label       "Manifestation" ;
        rdfs:subClassOf  [ a                         owl:Restriction ;
                           owl:onClass               :expression ;
                           owl:onProperty            :manifestation_manifests_expression ;
                           owl:qualifiedCardinality  "1"^^xsd:nonNegativeInteger
                         ] ;
        rdfs:subClassOf  [ a                   owl:Restriction ;
                           owl:maxCardinality  "1"^^xsd:nonNegativeInteger ;
                           owl:onProperty      cmr:creationDate
                         ] ;
        rdfs:subClassOf  [ a                   owl:Restriction ;
                           owl:maxCardinality  "1"^^xsd:nonNegativeInteger ;
                           owl:onProperty      :manifestation_source-pool
                         ] ;
        rdfs:subClassOf  [ a                   owl:Restriction ;
                           owl:maxCardinality  "1"^^xsd:nonNegativeInteger ;
                           owl:onProperty      :manifestation_embargo
                         ] ;
        rdfs:subClassOf  [ a                   owl:Restriction ;
                           owl:maxCardinality  "1"^^xsd:nonNegativeInteger ;
                           owl:onProperty      :manifestation_number_catalogue_global
                         ] ;
        rdfs:subClassOf  [ a                   owl:Restriction ;
                           owl:maxCardinality  "1"^^xsd:nonNegativeInteger ;
                           owl:onProperty      :manifestation_dimension
                         ] ;
        rdfs:subClassOf  [ a                owl:Restriction ;
                           owl:cardinality  "1"^^xsd:nonNegativeInteger ;
                           owl:onProperty   cmr:lastModificationDate
                         ] ;
        rdfs:subClassOf  [ a                owl:Restriction ;
                           owl:cardinality  "1"^^xsd:nonNegativeInteger ;
                           owl:onProperty   :manifestation_type
                         ] ;
        rdfs:subClassOf  [ a                   owl:Restriction ;
                           owl:maxCardinality  "1"^^xsd:nonNegativeInteger ;
                           owl:onProperty      :manifestation_is-signed
                         ] ;
        rdfs:subClassOf  [ a                   owl:Restriction ;
                           owl:maxCardinality  "1"^^xsd:nonNegativeInteger ;
                           owl:onProperty      :manifestation_date_publication
                         ] ;
        rdfs:subClassOf  [ a                            owl:Restriction ;
                           owl:maxQualifiedCardinality  "1"^^xsd:nonNegativeInteger ;
                           owl:onClass                  :manifestation ;
                           owl:onProperty               :manifestation_reproduction_of_manifestation
                         ] ;
        rdfs:subClassOf  [ a                   owl:Restriction ;
                           owl:maxCardinality  "1"^^xsd:nonNegativeInteger ;
                           owl:onProperty      :manifestation_date
                         ] ;
        rdfs:subClassOf  [ a                   owl:Restriction ;
                           owl:maxCardinality  "1"^^xsd:nonNegativeInteger ;
                           owl:onProperty      :manifestation_title
                         ] ;
        rdfs:subClassOf  [ a                   owl:Restriction ;
                           owl:maxCardinality  "1"^^xsd:nonNegativeInteger ;
                           owl:onProperty      :manifestation_representation_type
                         ] ;
        rdfs:subClassOf  [ a                            owl:Restriction ;
                           owl:maxQualifiedCardinality  "1"^^xsd:nonNegativeInteger ;
                           owl:onClass                  :signature_digital ;
                           owl:onProperty               :manifestation_signed_by_signature_digital
                         ] ;
        rdfs:subClassOf  [ a                            owl:Restriction ;
                           owl:maxQualifiedCardinality  "1"^^xsd:nonNegativeInteger ;
                           owl:onClass                  :product-form ;
                           owl:onProperty               :manifestation_has-product-form_product-form
                         ] .

:procurement_public_transliterated_town
        a                   owl:DatatypeProperty ;
        rdfs:domain         :procurement_public ;
        rdfs:label          "Procurement public transliterated town" ;
        rdfs:range          xsd:string ;
        rdfs:subPropertyOf  :transliterated_town .

:resource_legal_implicitly_repeals_resource_legal
        a                   owl:ObjectProperty ;
        rdfs:comment        "This property points to act that is implicitly repealed. Relevant for legal analysis: true" ;
        rdfs:domain         :resource_legal ;
        rdfs:label          "Legal resource implicitly repeals legal resource" ;
        rdfs:range          :resource_legal ;
        rdfs:subPropertyOf  :implicitly_repeals ;
        owl:inverseOf       :resource_legal_implicitly_repealed_by_resource_legal .

:procedure_code_interinstitutional_based_on_resource_legal
        a                   owl:ObjectProperty ;
        rdfs:comment        "DEPRECATED, Procedure is based on a legal resource (typically a treaty article, but could also be secondary legislation). Use in the future dossier_based_on_resource_legal. Legal basis (1). Relevant for legal analysis: true." ;
        rdfs:domain         :procedure_code_interinstitutional ;
        rdfs:label          "Procedure based on legal resource" ;
        rdfs:range          :resource_legal ;
        rdfs:subPropertyOf  :dossier_based_on_resource_legal , :based_on ;
        owl:deprecated      true ;
        owl:inverseOf       :resource_legal_basis_for_procedure_code_interinstitutional .

<http://publications.europa.eu/resource/authority/fd_604>
        a       owl:NamedIndividual .

:event_internal  a       owl:Class ;
        rdfs:comment     "Event in an internal procedure, e.g of the Commission. The two metadata elements of in the corresponding IMMC elements, event_date and event_has_type_concept_type_event are already present at the event level. To link an internal event to its internal procedure, event_part_of_dossier should be used Corresponding data will be delivered in particular via the new publicAccess chain in the element /ns4:ec_transmission_request/transmission/workflow/extension/ns3:workflow_event and its subelements." ;
        rdfs:label       "Internal event" ;
        rdfs:subClassOf  :event ;
        rdfs:subClassOf  [ a                            owl:Restriction ;
                           owl:maxQualifiedCardinality  "1"^^xsd:nonNegativeInteger ;
                           owl:onClass                  :concept_mode_decision ;
                           owl:onProperty               :event_internal_uses_concept_mode_decision
                         ] ;
        rdfs:subClassOf  [ a                   owl:Restriction ;
                           owl:maxCardinality  "1"^^xsd:nonNegativeInteger ;
                           owl:onProperty      :event_internal_urgent_procedure
                         ] ;
        rdfs:subClassOf  [ a                   owl:Restriction ;
                           owl:maxCardinality  "1"^^xsd:nonNegativeInteger ;
                           owl:onProperty      :event_internal_objection_period_extension
                         ] ;
        rdfs:subClassOf  [ a                   owl:Restriction ;
                           owl:maxCardinality  "1"^^xsd:nonNegativeInteger ;
                           owl:onProperty      :event_internal_objection_period
                         ] ;
        rdfs:subClassOf  [ a                   owl:Restriction ;
                           owl:maxCardinality  "1"^^xsd:nonNegativeInteger ;
                           owl:onProperty      :event_internal_eu_survey_identifier
                         ] .

:dossier_is_about_concept_eurovoc
        a             owl:ObjectProperty ;
        rdfs:comment  "The dossier has as subject a concept from the Eurovoc thesaurus. Relevant for legal analysis: to be verified." ;
        rdfs:domain   :dossier ;
        rdfs:label    "Dossier is about Eurovoc concept" ;
        rdfs:range    :concept_eurovoc .

:number_document_in_official-journal
        a           owl:DatatypeProperty ;
        rdfs:label  "Number document in official journal" .

:resource_legal_inapplicability_requested_by_communication_case_new
        a              owl:ObjectProperty ;
        rdfs:domain    :resource_legal ;
        rdfs:label     "Resource legal inapplicability requested by communication case new" ;
        rdfs:range     :communication_case_new ;
        owl:inverseOf  :communication_case_new_requests_inapplicability_resource_legal .

:event_legal_was_historically_about_concept_type_procedure_code_interinstitutional
        a                   owl:ObjectProperty ;
        rdfs:comment        "At the time of the event the procedure had a certain type of procedure. Change from the type_procedure_historical data property. Relevant for legal analysis: true." ;
        rdfs:domain         :event_legal ;
        rdfs:label          "Procedure had type concept type procedure" ;
        rdfs:range          :concept_type_procedure_code_interinstitutional ;
        rdfs:subPropertyOf  :was_historically_about .

:manifestation_special-court-report_part_page_last
        a                   owl:DatatypeProperty ;
        rdfs:comment        "DEPRECATED, Last page number of the special Court report part related to a court document. Use manifestion_print_page_last" ;
        rdfs:domain         :manifestation_special-court-report_part ;
        rdfs:label          "Last page" ;
        rdfs:range          xsd:string ;
        rdfs:subPropertyOf  :page_last , :manifestation_print_page_last ;
        owl:deprecated      true .

:jointly-responsible_for
        a           owl:ObjectProperty ;
        rdfs:label  "Jointly responsible for" .

<http://publications.europa.eu/resource/authority/fd_577>
        a       owl:NamedIndividual .

<http://publications.europa.eu/resource/authority/fd_100>
        a       owl:NamedIndividual .

:work_drafted_in_language
        a                   owl:ObjectProperty ;
        rdfs:comment        "The work was originally drafted in a given language" ;
        rdfs:domain         :work ;
        rdfs:label          "Work drafted in a given language" ;
        rdfs:range          :language ;
        rdfs:subPropertyOf  :drafted_in ;
        owl:inverseOf       :language_used_for_drafting_work .

:concept_type_act  a         owl:Class ;
        rdfs:comment         "Corresponds to the contents of the Procat field FM, coded with FD_Table 030. This concept belonging to the deprecated NAL fd_030 is not anymore fed. Please use the concept resource-type which has replaced it." ;
        rdfs:label           "Concept representing the type of an act" ;
        rdfs:subClassOf      skos:Concept , :concept_decoding ;
        owl:equivalentClass  [ a               owl:Restriction ;
                               owl:hasValue    <http://publications.europa.eu/resource/authority/fd_030> ;
                               owl:onProperty  skos:inScheme
                             ] .

:event_legal_initiated_by_institution
        a                   owl:ObjectProperty ;
        rdfs:comment        "DEPRECATED, This legal event is initiated by a given institution. Examples include Discussions at the Council or the transmission of a COM from the Commission to Council. Body role:Primarily responsible. Relevant for legal analysis: true." ;
        rdfs:domain         :event_legal ;
        rdfs:label          "Legal event initiated by institution" ;
        rdfs:range          :institution ;
        rdfs:subPropertyOf  :initiated_by , :event_initiated_by_institution ;
        owl:deprecated      true ;
        owl:inverseOf       :institution_initiates_event_legal .

:case-law_national_following_case-law
        a                   owl:DatatypeProperty ;
        rdfs:comment        "The case law has a follow up. see 82003UK1021(01)" ;
        rdfs:domain         :case-law_national ;
        rdfs:label          "Following case law" ;
        rdfs:range          xsd:string ;
        rdfs:subPropertyOf  :following_case-law .

:concept_currency  a     owl:Class ;
        rdfs:comment     "CAT currency" ;
        rdfs:label       "Concept representing currency" ;
        rdfs:subClassOf  :concept .

:agreement_member-states
        a                owl:Class ;
        rdfs:comment     "Agreement between member states (= subsector A of sector 4)" ;
        rdfs:label       "Agreement between member states" ;
        rdfs:subClassOf  :legislation_complementary .

:case-law_declares_incidentally_valid_resource_legal
        a                   owl:ObjectProperty ;
        rdfs:comment        "This property points to legal act quoted in the operative part of Court decisions" ;
        rdfs:domain         :case-law ;
        rdfs:label          "Case law declares incidentally valid legal resource" ;
        rdfs:range          :resource_legal ;
        rdfs:subPropertyOf  :declares_incidentally_valid ;
        owl:inverseOf       :resource_legal_incidentally_declared_valid_case-law .

:decision_date_transposition
        a                   owl:DatatypeProperty ;
        rdfs:comment        "Date of transposition applicable to decisions; can contain multiple values as different parts of a dirctive can be implemented by various pieces of national legislation, coming with different dates (TP_DATE). TP_COMMENT is mixed content, coded with fd_361. Relevant for legal analysis: true." ;
        rdfs:domain         :decision ;
        rdfs:label          "Date of transposition of a decision" ;
        rdfs:range          xsd:date ;
        rdfs:subPropertyOf  :date_transposition .

:person_reports_on_opinion_consultation_eesc
        a                   owl:ObjectProperty ;
        rdfs:domain         :person ;
        rdfs:label          "Person reports on opinion_consultation_eesc" ;
        rdfs:range          :opinion_consultation_eesc ;
        rdfs:subPropertyOf  :reports_on ;
        owl:inverseOf       :opinion_consultation_eesc_reported_by_person .

:summary_legislation_eu_is_about_classification_summary
        a                   owl:ObjectProperty ;
        rdfs:comment        "Summary is about a subject in the classification of summaries of EU legislation." ;
        rdfs:domain         :summary_legislation_eu ;
        rdfs:label          "Summary is about a subject in the classification of summaries of EU legislation" ;
        rdfs:range          :classification_summary ;
        rdfs:subPropertyOf  :is_about ;
        owl:inverseOf       :classification_summary_subject_of_summary_legislation_eu .

:procurement_public_value_type
        a                   owl:DatatypeProperty ;
        rdfs:domain         :procurement_public ;
        rdfs:label          "Type of value" ;
        rdfs:range          xsd:string ;
        rdfs:subPropertyOf  :value_type .

:decision_implementing
        a                owl:Class ;
        rdfs:comment     "93 Implementing decision (DTS=3 AND FM=DECIMP)" ;
        rdfs:label       "Implementing decision" ;
        rdfs:subClassOf  :legislation_secondary .

:procurement_public_xml-schema-definition_link_type
        a                   owl:DatatypeProperty ;
        rdfs:domain         :procurement_public ;
        rdfs:label          "Link type for the schema definition" ;
        rdfs:range          xsd:string ;
        rdfs:subPropertyOf  :xml-schema-definition_link_type .

:regulation_implementing
        a                owl:Class ;
        rdfs:comment     "18 Implementing regulation (DTS=3 AND FM=REGIMP)" ;
        rdfs:label       "Implementing regulation" ;
        rdfs:subClassOf  :legislation_secondary .

<http://publications.europa.eu/resource/authority/fd_535>
        a       owl:NamedIndividual .

:concept_treaty_basis_for_resource_legal
        a                   owl:ObjectProperty ;
        rdfs:domain         :concept_treaty ;
        rdfs:label          "Treaty is basis for a legal resource" ;
        rdfs:range          :resource_legal ;
        rdfs:subPropertyOf  :basis_for ;
        owl:inverseOf       :resource_legal_based_on_concept_treaty .

:case-law_article_journal_related
        a                   owl:DatatypeProperty ;
        rdfs:comment        "Reference to an article which has appeared in a juridical journal and is related to the judgement in question (e.g. <NO>Thompson, James E.: Common Market Law Review 1990 p.589-607</NO>) NO / notes related to the decision" ;
        rdfs:domain         :case-law ;
        rdfs:label          "Related journal article" ;
        rdfs:range          xsd:string ;
        rdfs:subPropertyOf  :article_journal_related .

:com_package_barcode  a     owl:DatatypeProperty ;
        rdfs:comment        "Digitizer's barcode for a COM package" ;
        rdfs:domain         :com_package ;
        rdfs:label          "COM package barcode" ;
        rdfs:range          xsd:string ;
        rdfs:subPropertyOf  :archive_package_barcode .

:question_parliamentary_with-debate
        a                owl:Class ;
        rdfs:comment     "DEPRECATED. Parliamentary question with debate. Examples: 91998H0002, 91998H0001" ;
        rdfs:label       "Parliamentary question with debate" ;
        rdfs:subClassOf  :question_parliamentary ;
        rdfs:subClassOf  [ a                   owl:Restriction ;
                           owl:maxCardinality  "1"^^xsd:nonNegativeInteger ;
                           owl:onProperty      :question_parliamentary_with-debate_published
                         ] ;
        owl:deprecated   true .

:date_signature  a          owl:DatatypeProperty ;
        rdfs:label          "Date signature" ;
        rdfs:range          xsd:date ;
        rdfs:subPropertyOf  :date .

:manifestation_official-journal_part_information_number
        a                   owl:DatatypeProperty ;
        rdfs:comment        "Year and natural number of the act (combined in one string, as seen by the printer). values such as \"2012/C 95/23\", \"2590/1980\" (precomposed) --- in the future only to be used for OJ_NUM_INF in OJ C, not for OJ_DOC_NO" ;
        rdfs:domain         :manifestation_official-journal_part ;
        rdfs:label          "Year and natural number of the act (precomposed)" ;
        rdfs:range          xsd:string ;
        rdfs:subPropertyOf  :information_number .

:resource_legal_date_end-of-validity
        a                   owl:DatatypeProperty ;
        rdfs:comment        "Date of the end of validity of a legal resource. Several end of validity dates are possible, e.g. partial ends of validity - EV_COMMENT is mixed content, decoded with fd_330. EV (type as annotation). Relevant for legal analysis: true" ;
        rdfs:domain         :resource_legal ;
        rdfs:label          "Date of end of validity" ;
        rdfs:range          xsd:date ;
        rdfs:subPropertyOf  :date_end-of-validity .

dc:description  a  owl:AnnotationProperty .

:resource_legal_is_about_subject-matter
        a                   owl:ObjectProperty ;
        rdfs:comment        "A legal resource is about a concept expressed as a subject matter (classification tool). CT, coded according to FD_TABLE 070, also exposed as field ET. CT, coded according to FD_TABLE 070, also exposed as field ET. Relevant for legal analysis: true" ;
        rdfs:domain         :resource_legal ;
        rdfs:label          "Legal resource is about subject matter" ;
        rdfs:range          :subject-matter ;
        rdfs:subPropertyOf  :is_about ;
        owl:inverseOf       :subject-matter_subject_of_resource_legal .

:resource_legal_corrects_resource_legal
        a                   owl:ObjectProperty ;
        rdfs:comment        "Link from corrigendum to corrected act. Relevant for legal analysis: true" ;
        rdfs:domain         :resource_legal ;
        rdfs:label          "Legal resource corrects legal resource" ;
        rdfs:range          :resource_legal ;
        rdfs:subPropertyOf  :corrects ;
        owl:inverseOf       :resource_legal_corrected_by_resource_legal .

:subject-matter_subject_of_resource_legal
        a                   owl:ObjectProperty ;
        rdfs:domain         :subject-matter ;
        rdfs:label          "Subject matter is subject of a legal resource" ;
        rdfs:range          :resource_legal ;
        rdfs:subPropertyOf  :subject_of ;
        owl:inverseOf       :resource_legal_is_about_subject-matter .

:resource_legal_contains_ep_opinion_on_resource_legal
        a                   owl:ObjectProperty ;
        rdfs:comment        "This points to proposal on which EP provides its opinion. Relevant for legal analysis: true" ;
        rdfs:domain         :resource_legal ;
        rdfs:label          "Legal resource contains European Parliament opinion on legal resource" ;
        rdfs:range          :resource_legal ;
        rdfs:subPropertyOf  :contains_ep_opinion_on ;
        owl:inverseOf       :resource_legal_ep_opinion_contained_in_resource_legal .

:date_creation_legacy
        a                   owl:DatatypeProperty ;
        rdfs:comment        "Procat and Pegase legacy creation dates" ;
        rdfs:label          "Date creation legacy" ;
        rdfs:range          xsd:date ;
        rdfs:subPropertyOf  :date .

:item_doi  a                owl:DatatypeProperty ;
        rdfs:comment        "DOI of this item" ;
        rdfs:domain         :item ;
        rdfs:label          "DOI of item" ;
        rdfs:range          xsd:string ;
        rdfs:subPropertyOf  :doi .

:archived  a        owl:DatatypeProperty ;
        rdfs:label  "Archived" .

:resource_legal_based_on_treaty
        a                   owl:ObjectProperty ;
        rdfs:comment        "This property pointing to fd_020 has been deprecated. The instances which used to point to this property are now pointing to cdm:resource_legal_based_on_concept_treaty pointing to treaty table. This property will ultimatively be removed from the CDM. Link to the treaty/treaties that form the legal basis under which the document has been or is being adopted. DEPRECATED. See cdm:resource_legal_based_on_concept_treaty" ;
        rdfs:domain         :resource_legal ;
        rdfs:label          "Legal resource based on treaty" ;
        rdfs:range          :treaty ;
        rdfs:subPropertyOf  :based_on ;
        dct:created         "2018-07-24T10:08:41.793+02:00"^^xsd:dateTime ;
        owl:deprecated      true ;
        owl:inverseOf       :treaty_basis_for_resource_legal .

:event_basis_legal_suggested
        a            owl:DatatypeProperty ;
        rdfs:domain  :event ;
        rdfs:label   "Event basis legal suggested" ;
        rdfs:range   xsd:string ;
        dct:created  "2018-07-20T08:47:25.375+02:00"^^xsd:dateTime .

:ATTO_FD_610  a              owl:Class ;
        rdfs:label           "FD_610 ATTO table" ;
        rdfs:subClassOf      skos:Concept ;
        owl:equivalentClass  [ a               owl:Restriction ;
                               owl:hasValue    <http://publications.europa.eu/resource/authority/fd_610> ;
                               owl:onProperty  skos:inScheme
                             ] .

:joint-assessment_impact
        a                owl:Class ;
        rdfs:label       "Joint Impact Assessment" ;
        rdfs:subClassOf  :joint-staff-working-document .

:agent_edits_work  a   owl:ObjectProperty ;
        rdfs:comment   "Agent acts as an editor of a work" ;
        rdfs:domain    :agent ;
        rdfs:label     "Agent is editor of a work" ;
        rdfs:range     :work ;
        owl:inverseOf  :work_edited_by_agent .

:opinion_ep_reported_by_agent
        a                   owl:ObjectProperty ;
        rdfs:comment        "Name of the person (EP member or member of CoR or EESC) who reports on the relevant act. This property will be deprecated and replaced with work_reported_by_person. Relevant for legal analysis: true. Roles RAPP, RAPP_OPIN, CMT_OPIN.\"" ;
        rdfs:domain         :opinion_ep ;
        rdfs:label          "European Parliament opinion has rapporteur" ;
        rdfs:range          :agent ;
        rdfs:subPropertyOf  :reported_by .

:resource_legal_replaces_resource_legal
        a                   owl:ObjectProperty ;
        rdfs:comment        "This property points to act that is replaced. Relevant for legal analysis: true" ;
        rdfs:domain         :resource_legal ;
        rdfs:label          "Legal resource replaces legal resource" ;
        rdfs:range          :resource_legal ;
        rdfs:subPropertyOf  :replaces ;
        owl:inverseOf       :resource_legal_replaced_by_resource_legal .

:event_legal_on_agenda_concept_agenda_council
        a                   owl:ObjectProperty ;
        rdfs:comment        "Information on the council session this event is related to. Change from the agenda_council data property. Council agenda. Relevant for legal analysis: true." ;
        rdfs:domain         :event_legal ;
        rdfs:label          "The event references to a council agenda" ;
        rdfs:range          :concept_agenda_council ;
        rdfs:subPropertyOf  :on_agenda .

:manifestation_audience
        a             owl:DatatypeProperty ;
        rdfs:comment  "This property describe the audience, where the possible values are: [PUBLIC | NOT_PUBLIC], and by default: PUBLIC" ;
        rdfs:domain   :manifestation ;
        rdfs:label    "Audience of manifestation" ;
        rdfs:range    xsd:string ;
        dct:created   "2018-08-13T12:33:30.273+02:00"^^xsd:dateTime .

<http://publications.europa.eu/resource/authority/fd_010>
        a       owl:NamedIndividual .

dct:creator  a  owl:AnnotationProperty .

:language_used_originally_by_resource_legal
        a                   owl:ObjectProperty ;
        rdfs:comment        "A given language is used for the authentic language version of a legal resource. LF / authentic language" ;
        rdfs:domain         :language ;
        rdfs:label          "Language used originally by legal resource" ;
        rdfs:range          :resource_legal ;
        rdfs:subPropertyOf  :used_originally_by ;
        owl:inverseOf       :resource_legal_uses_originally_language .

:arrangement_institutional
        a                owl:Class ;
        rdfs:comment     "Institutional arrangements: rules of procedure; internal agreements (subsector Q of sector 3). At present 267 notices. Examples: 31953Q0003, 31957Q0002, 31969Q0491, 32009Q0716(02), 32005Q1029(01)" ;
        rdfs:label       "Institutional arrangement" ;
        rdfs:subClassOf  :legislation_secondary .

:agreement_international_has_type_comment_concept_type_comment
        a                   owl:ObjectProperty ;
        rdfs:comment        "Comments and additional details of agreements and decisions taken by bodies created by these agreements. IC. Relevant for legal analysis: true" ;
        rdfs:domain         :agreement_international ;
        rdfs:label          "Type of comment by a body" ;
        rdfs:range          :concept_type_comment ;
        rdfs:subPropertyOf  :has_type_comment .

:given_on  a        owl:ObjectProperty ;
        rdfs:label  "Given on" .

:expression_publication_general_information_language_expression
        a                   owl:DatatypeProperty ;
        rdfs:comment        "Additional information on the language of expression. Textual information on the language of the described materials. A description of the alphabet, script, or other symbol system ..." ;
        rdfs:domain         :expression_publication_general ;
        rdfs:label          "Information on language of expression" ;
        rdfs:range          xsd:string ;
        rdfs:subPropertyOf  :information_language_expression .

:completed_by  a    owl:ObjectProperty ;
        rdfs:label  "Completed by" .

:person_reports_on_opinion_consultation_cor
        a                   owl:ObjectProperty ;
        rdfs:domain         :person ;
        rdfs:label          "Person reports on opinion_consultation_cor" ;
        rdfs:range          :opinion_consultation_cor ;
        rdfs:subPropertyOf  :reports_on ;
        owl:inverseOf       :opinion_consultation_cor_reported_by_person .

:main-activities_label
        a           owl:DatatypeProperty ;
        rdfs:label  "Main activities label" .

:work_contains_recital
        a                   owl:ObjectProperty ;
        rdfs:domain         :work ;
        rdfs:label          "Work contains recital" ;
        rdfs:range          :recital ;
        rdfs:subPropertyOf  :work_contains_subdivision , :contains .

:act_preparatory_ecsc
        a                owl:Class ;
        rdfs:comment     "Preparatory act by the European Coal and Steel Community" ;
        rdfs:label       "Preparatory act by ECSC" ;
        rdfs:subClassOf  :act_preparatory ;
        rdfs:subClassOf  [ a               owl:Restriction ;
                           owl:hasValue    <http://publications.europa.eu/resource/authority/corporate-body/ECSC> ;
                           owl:onProperty  :work_created_by_agent
                         ] ;
        dct:created      "2022-09-01T09:01:22"^^xsd:dateTime .

:date_end  a        owl:DatatypeProperty ;
        rdfs:label  "Date end" .

:publication_frequency
        a                owl:Class ;
        rdfs:comment     "Corresponds to the publication frequency" ;
        rdfs:label       "Concept representing the publication frequency" ;
        rdfs:subClassOf  :concept_decoding .

:documentation_business_classification
        a            owl:DatatypeProperty ;
        rdfs:domain  :documentation ;
        rdfs:label   "Documentation business classification" ;
        rdfs:range   xsd:anyURI .

:com_package  a          owl:Class ;
        rdfs:comment     "Package of digitized documents related to a COM proposal. Historical collection of documents related to a Commission proposal, digitized based on the fonds of the OIB archive. Such COM packages merge typically a number of different documents across linguistic versions in a single multilingual expression. Each expression indicates the languages it uses, each title has in a language tag the corresponding language. The relationship between the COM package and its COM is expressed via work_contains_work. The COM identifier can be built based on ext:prefix_com, ext:year_com and ext:number_com." ;
        rdfs:label       "Digitised COM package document" ;
        rdfs:subClassOf  :archive_package_ec ;
        rdfs:subClassOf  [ a                            owl:Restriction ;
                           owl:maxQualifiedCardinality  "1"^^xsd:nonNegativeInteger ;
                           owl:onDataRange              xsd:string ;
                           owl:onProperty               :com_package_reference_volume
                         ] ;
        rdfs:subClassOf  [ a                            owl:Restriction ;
                           owl:maxQualifiedCardinality  "1"^^xsd:nonNegativeInteger ;
                           owl:onDataRange              xsd:boolean ;
                           owl:onProperty               :com_package_has_title_from_com_final
                         ] .

:institution_associated_with_event_legal
        a                   owl:ObjectProperty ;
        rdfs:comment        "An institution is associated with the execution of a legal event" ;
        rdfs:domain         :institution ;
        rdfs:label          "Institution associated with legal event" ;
        rdfs:range          :event_legal ;
        rdfs:subPropertyOf  :associated_with .

:author_printer  a  owl:DatatypeProperty ;
        rdfs:label  "Author printer" .

:opinion_cjeu_given_on_resource_legal
        a                   owl:ObjectProperty ;
        rdfs:comment        "This property points to act quoted in Court document." ;
        rdfs:domain         :opinion_cjeu ;
        rdfs:label          "Case law Opinion given on legal resource" ;
        rdfs:range          :resource_legal ;
        rdfs:subPropertyOf  :given_on ;
        owl:inverseOf       :resource_legal_received_opinion_cjeu .

:com_package_has_title_from_com_final
        a                   owl:DatatypeProperty ;
        rdfs:comment        "Boolean property representing the information whether the titles for a COM package were taken from a COM final document or (in absence of a COM final document) from another document in the package being defined as substitute." ;
        rdfs:domain         :com_package ;
        rdfs:label          "COM package has title from COM final" ;
        rdfs:range          xsd:boolean ;
        rdfs:subPropertyOf  :archive_package_ec_has_title_from_com_final .

:event_legal_type  a        owl:DatatypeProperty ;
        rdfs:comment        "DEPRECATED, The type of the legal event. Event type. Relevant for legal analysis: true." ;
        rdfs:domain         :event_legal ;
        rdfs:label          "Type of legal event" ;
        rdfs:range          xsd:string ;
        rdfs:subPropertyOf  :type ;
        owl:deprecated      true .

:institution_jointly-responsible_for_event_legal
        a                   owl:ObjectProperty ;
        rdfs:comment        "An institution is responsible for a legal event together with other agent(s)" ;
        rdfs:domain         :institution ;
        rdfs:label          "Institution jointly responsible for legal event" ;
        rdfs:range          :event_legal ;
        rdfs:subPropertyOf  :jointly-responsible_for .

:resource_legal_internal_number_year
        a                   owl:DatatypeProperty ;
        rdfs:domain         :resource_legal ;
        rdfs:label          "Resource legal internal number year" ;
        rdfs:range          xsd:year ;
        rdfs:subPropertyOf  :internal_number_year .

:durability  a      owl:DatatypeProperty ;
        rdfs:label  "Durability" .

:annulment_requested_by
        a           owl:ObjectProperty ;
        rdfs:label  "Annulment requested by" .

:identifier_case  a  owl:DatatypeProperty ;
        rdfs:label  "Identifier case" .

:act_consolidated_layer
        a                   owl:DatatypeProperty ;
        rdfs:comment        "Consleg couche. Number of the layer" ;
        rdfs:domain         :act_consolidated ;
        rdfs:label          "Consolidated act layer" ;
        rdfs:range          xsd:string ;
        rdfs:subPropertyOf  :layer .

:seizure  a              owl:Class ;
        rdfs:comment     "Seizure in sector 6 (6CS)" ;
        rdfs:label       "Seizure" ;
        rdfs:subClassOf  :case-law .

:resource_legal_application_deferred_by_resource_legal
        a                   owl:ObjectProperty ;
        rdfs:comment        "Calculated. Relevant for legal analysis: true." ;
        rdfs:domain         :resource_legal ;
        rdfs:label          "Legal resource has application deferred by legal resource" ;
        rdfs:range          :resource_legal ;
        rdfs:subPropertyOf  :application_deferred_by ;
        owl:inverseOf       :resource_legal_defers_application_of_resource_legal .

:classification_summary
        a                    owl:Class ;
        rdfs:label           "Classification for summaries of EU legislation" ;
        rdfs:subClassOf      skos:Concept , :concept_decoding ;
        owl:equivalentClass  [ a               owl:Restriction ;
                               owl:hasValue    <http://publications.europa.eu/resource/authority/class-sum-leg> ;
                               owl:onProperty  skos:inScheme
                             ] .

:work_dataset_version
        a                   owl:DatatypeProperty ;
        rdfs:comment        "This property contains a version number or other version designation of the Dataset" ;
        rdfs:domain         :work_dataset ;
        rdfs:label          "Dataset version" ;
        rdfs:range          xsd:string ;
        rdfs:subPropertyOf  :version .

:agent_creates_work  a      owl:ObjectProperty ;
        rdfs:domain         :agent ;
        rdfs:label          "Agent creates a work" ;
        rdfs:range          :work ;
        rdfs:subPropertyOf  :creates ;
        owl:inverseOf       :work_created_by_agent .

:summary_legislation_eu_version
        a                   owl:DatatypeProperty ;
        rdfs:comment        "What is the version of this summary? \"v1\", \"v2\", \"v3\"" ;
        rdfs:domain         :summary_legislation_eu ;
        rdfs:label          "Version of summary of legislation" ;
        rdfs:range          xsd:string ;
        rdfs:subPropertyOf  :version .

:dossier_is_about_concept_type_dossier
        a                   owl:ObjectProperty ;
        rdfs:comment        "Relevant for legal analysis: true. This dossier is of a certain type, expressed through a dossier type concept. Expressed through a link to the concept_type_dossier, currently FD table 612. Relevant for legal analysis: true" ;
        rdfs:domain         :dossier ;
        rdfs:label          "Dossier is about dossier type concept" ;
        rdfs:range          :concept_type_dossier ;
        rdfs:subPropertyOf  :is_about .

:agent_translates_work
        a              owl:ObjectProperty ;
        rdfs:comment   "Agent acts as a translator of a work" ;
        rdfs:domain    :agent ;
        rdfs:label     "Agent translates work" ;
        rdfs:range     :work ;
        owl:inverseOf  :work_translated_by_agent .

:resource_legal_has_type_act_concept_type_act
        a                   owl:ObjectProperty ;
        rdfs:comment        "This property pointing to the deprecated NAL fd_030 is not anymore fed. Please use work_has_resource-type pointing to resource-type instead. We will remove it from our instance data and ultimatively from the CDM.. The type of act in legal terms, expressed through a link to a type of act concept. FM, coded with FD_Table 030Related authority or tables: Resource types NAL, ATTO FD_30. Relevant for legal analysis: true\". \"Related authority or tables: Resource types NAL, ATTO FD_30. Relevant for legal analysis: true" ;
        rdfs:domain         :resource_legal ;
        rdfs:label          "Legal resource has type of act" ;
        rdfs:range          :concept_type_act ;
        rdfs:subPropertyOf  :has_type_act ;
        dct:created         "2018-07-24T10:10:14.722+02:00"^^xsd:dateTime .

:procurement_public_nuts_original_reference
        a                   owl:DatatypeProperty ;
        rdfs:domain         :procurement_public ;
        rdfs:label          "NUTS original reference" ;
        rdfs:range          xsd:anyURI ;
        rdfs:subPropertyOf  :nuts_original_reference .

<http://publications.europa.eu/resource/authority/court-type>
        a       owl:NamedIndividual .

:used_by  a           owl:ObjectProperty ;
        rdfs:comment  "An entity is used by another one" ;
        rdfs:label    "Used by" .

:person_responsible_for_event
        a                   owl:ObjectProperty ;
        rdfs:domain         :person ;
        rdfs:label          "Person responsible for event" ;
        rdfs:range          :event ;
        rdfs:subPropertyOf  :responsible_for .

:cooperation_police-and-judicial_date_transposition
        a                   owl:DatatypeProperty ;
        rdfs:comment        "Date of transposition applicable to police and judicial cooperation in criminal matters; can contain multiple values as different parts of a dirctive can be implemented by various pieces of national legislation, coming with different dates (TP_DATE). TP_COMMENT is mixed content, coded with fd_361. Relevant for legal analysis: true." ;
        rdfs:domain         :cooperation_police-and-judicial ;
        rdfs:label          "Date of transposition in police and judicial cooperation" ;
        rdfs:range          xsd:date ;
        rdfs:subPropertyOf  :date_transposition .

:resource_legal_internal_number_sequential_number
        a                   owl:DatatypeProperty ;
        rdfs:comment        "Sequential number of unique internal identifier of the resource legal" ;
        rdfs:domain         :resource_legal ;
        rdfs:label          "Internal number sequential number" ;
        rdfs:range          xsd:positiveInteger ;
        rdfs:subPropertyOf  :internal_number_sequential_number .

:legislation_secondary_date_notification
        a                   owl:DatatypeProperty ;
        rdfs:comment        "This contains the date of notification of directives and decisions which specify to whom they are addressed. Relevant for legal analysis: true" ;
        rdfs:domain         :legislation_secondary ;
        rdfs:label          "Date of notification of the secondary legislation" ;
        rdfs:range          xsd:date ;
        rdfs:subPropertyOf  :date_notification .

:influences  a      owl:ObjectProperty ;
        rdfs:label  "Influences" .

:opinion_other_eesc_reported_by_person
        a                   owl:ObjectProperty ;
        rdfs:comment        "Name of the person (EP member or member of CoR or EESC) who reports on the relevant act. This property will be deprecated and replaced with work_reported_by_person. Role RAPP. Relevant for legal analysis: true" ;
        rdfs:domain         :opinion_other_eesc ;
        rdfs:label          "European Economic and Social Committee other opinion has rapporteur" ;
        rdfs:range          :person ;
        rdfs:subPropertyOf  :work_reported_by_person ;
        dct:created         "2018-07-16T13:21:00.506+02:00"^^xsd:dateTime ;
        owl:inverseOf       :person_reports_on_opinion_other_eesc .

:publication_work  a     owl:Class ;
        rdfs:comment     "publication_work will be used to describe an aggregation of components which form a single publication product" ;
        rdfs:label       "Publication work" ;
        rdfs:subClassOf  :container_work .

:manifestation_court-report_part_page_first
        a                   owl:DatatypeProperty ;
        rdfs:comment        "DEPRECATED, First page number of the Court report part related to a court document. Use manifestion_print_page_first" ;
        rdfs:domain         :manifestation_court-report_part ;
        rdfs:label          "First page" ;
        rdfs:range          xsd:string ;
        rdfs:subPropertyOf  :page_first , :manifestation_print_page_first ;
        owl:deprecated      true .

:official-journal_volume
        a                   owl:DatatypeProperty ;
        rdfs:comment        "Volume of the Official Journal" ;
        rdfs:domain         :official-journal ;
        rdfs:label          "Volume of Official Journal" ;
        rdfs:range          xsd:positiveInteger ;
        rdfs:subPropertyOf  :volume .

:expression_publication_general_frequency_expected
        a                   owl:DatatypeProperty ;
        rdfs:comment        "Expected frequency of the series (e.g. M for monthly)" ;
        rdfs:domain         :expression_publication_general ;
        rdfs:label          "Expected frequency" ;
        rdfs:range          xsd:string ;
        rdfs:subPropertyOf  :frequency_expected .

:event_legal_document_reference
        a                   owl:DatatypeProperty ;
        rdfs:comment        "Relevant for legal analysis: true. Textual reference for a document / work that we do not know anything else about. Technical criteria is absence of any expression that we could establish. Document reference. Relevant for legal analysis: true" ;
        rdfs:domain         :event_legal ;
        rdfs:label          "Document reference" ;
        rdfs:range          xsd:string ;
        rdfs:subPropertyOf  :document_reference .

:distribution_status  a  owl:Class ;
        rdfs:comment     "Corresponds to the contents of the MDR authority list ADMS status vocabulary (http://purl.org/adms/status)" ;
        rdfs:label       "Concept representing the distribution status" ;
        rdfs:subClassOf  :concept_decoding .

:agent_relates_to_work
        a                   owl:ObjectProperty ;
        rdfs:domain         :agent ;
        rdfs:label          "Agent related to work" ;
        rdfs:range          :work ;
        rdfs:subPropertyOf  :relates_to ;
        owl:inverseOf       :work_related_with_agent .

:concept_type_dataset_is_type_of_work_dataset
        a              owl:ObjectProperty ;
        rdfs:domain    :concept_type_dataset ;
        rdfs:label     "Concept type dataset is type of work dataset" ;
        rdfs:range     :work_dataset ;
        owl:inverseOf  :work_dataset_has_type_concept_type_dataset .

:immediately_enforces
        a           owl:ObjectProperty ;
        rdfs:label  "Immediately enforces" .

:resource_legal_does_deletion_of_resource_legal
        a                   owl:ObjectProperty ;
        rdfs:comment        "Legal resources does deletion a legal resource, in term of consolidation." ;
        rdfs:domain         :resource_legal ;
        rdfs:label          "Legal resources does deletion of legal resource" ;
        rdfs:range          :resource_legal ;
        rdfs:subPropertyOf  :does_deletion_of .

:interpreted_authoritatively_by
        a           owl:ObjectProperty ;
        rdfs:label  "Interpreted authoritatively by" .

:event_legal_gets_report_of_institution
        a                   owl:ObjectProperty ;
        rdfs:comment        "Relevant for legal analysis: true. This legal gets the report of given institution. Body role:Author of report. Relevant for legal analysis: true" ;
        rdfs:domain         :event_legal ;
        rdfs:label          "Legal event gets the report of an institution" ;
        rdfs:range          :institution ;
        rdfs:subPropertyOf  :gets_report_of ;
        owl:inverseOf       :institution_authors-report_event_legal .

:proposes_to_amend  a  owl:ObjectProperty ;
        rdfs:label  "Proposes to amend" .

:nestedList  a              owl:ObjectProperty ;
        rdfs:comment        "Object property that is a sub-property of rdf:first. It introduces a nested list (as the first resource) at the current position in the rdf:List" ;
        rdfs:label          "Property to hold nested lists" ;
        rdfs:range          rdf:List ;
        rdfs:subPropertyOf  rdf:first .

:directive_number  a  owl:DatatypeProperty ;
        rdfs:label  "Directive number" .

:has_status  a      owl:ObjectProperty ;
        rdfs:label  "Has status" .

:requests_interpretation
        a           owl:ObjectProperty ;
        rdfs:label  "Requests interpretation" .

:work_communicated_on_by_work
        a                   owl:ObjectProperty ;
        rdfs:domain         :work ;
        rdfs:label          "Work communicated on by work" ;
        rdfs:range          :work ;
        rdfs:subPropertyOf  :communicated_on_by ;
        owl:inverseOf       :work_communicates_on_work .

:work_has_jurisdiction
        a            owl:DatatypeProperty ;
        rdfs:domain  :work ;
        rdfs:label   "Work has jurisdiction" ;
        rdfs:range   xsd:string .

:subject_of  a        owl:ObjectProperty ;
        rdfs:comment  "UDC concept is subject of a general publication" ;
        rdfs:label    "Subject of" .

:part_legal_part_of_work
        a                   owl:ObjectProperty ;
        rdfs:comment        "This property associates an instance of a work with an instance of a part that forms part of it." ;
        rdfs:domain         :part_legal ;
        rdfs:label          "Part (legal) part of work" ;
        rdfs:range          :work ;
        rdfs:subPropertyOf  :subdivision_part_of_work , :part_of ;
        owl:inverseOf       :work_contains_part_legal .

:edition  a         owl:DatatypeProperty ;
        rdfs:label  "Edition" .

:manifestation_is-signed
        a                   owl:DatatypeProperty ;
        rdfs:comment        "Indication, if this manifestation is electronically signed. Is this manifestation signed?" ;
        rdfs:domain         :manifestation ;
        rdfs:label          "Is this manifestation electronically signed?" ;
        rdfs:range          xsd:boolean ;
        rdfs:subPropertyOf  :is-signed .

:official-journal-act_subsection_oj
        a                   owl:DatatypeProperty ;
        rdfs:comment        "Section heading (level 2) under which an Official Journal act is published." ;
        rdfs:domain         :official-journal-act ;
        rdfs:label          "Official journal act subsection oj" ;
        rdfs:range          xsd:string ;
        rdfs:subPropertyOf  :subsection_oj .

:manifestation_has-product-form_product-form
        a                   owl:ObjectProperty ;
        rdfs:comment        "This Manifestation has a specific Product Form." ;
        rdfs:domain         :manifestation ;
        rdfs:label          "Manifestation has Product Form" ;
        rdfs:range          :product-form ;
        rdfs:subPropertyOf  :has_product_form ;
        dct:created         "2022-08-01T16:18:31.50"^^xsd:dateTime ;
        owl:inverseOf       :product-form_is-product-form-of_manifestation .

:ATTO_FD_345  a              owl:Class ;
        rdfs:label           "FD_345 ATTO table" ;
        rdfs:subClassOf      skos:Concept ;
        owl:equivalentClass  [ a               owl:Restriction ;
                               owl:hasValue    <http://publications.europa.eu/resource/authority/fd_345> ;
                               owl:onProperty  skos:inScheme
                             ] .

:resource_legal_influences_resource_legal
        a                   owl:ObjectProperty ;
        rdfs:comment        "This points to subsequent preparatory document influencing a proposal. Relevant for legal analysis: true" ;
        rdfs:domain         :resource_legal ;
        rdfs:label          "Legal resource influenced by legal resource" ;
        rdfs:range          :resource_legal ;
        rdfs:subPropertyOf  :influences ;
        owl:inverseOf       :resource_legal_influenced_by_resource_legal .

:procurement_public_expressed_in_concept_currency
        a                   owl:ObjectProperty ;
        rdfs:domain         :procurement_public ;
        rdfs:label          "Public procurement value expressed in a given currency" ;
        rdfs:range          :concept_currency ;
        rdfs:subPropertyOf  :expressed_in .

:keyword  a         owl:DatatypeProperty ;
        rdfs:label  "Keyword" .

:container_case-law_fascicule
        a                   owl:DatatypeProperty ;
        rdfs:domain         :container_case-law ;
        rdfs:label          "Fascicule" ;
        rdfs:range          xsd:positiveInteger ;
        rdfs:subPropertyOf  :fascicule .

:work_dataset_keyword
        a                   owl:DatatypeProperty ;
        rdfs:comment        "This property contains a keyword or tag describing the dataset" ;
        rdfs:domain         :work_dataset ;
        rdfs:label          "Dataset keyword" ;
        rdfs:range          xsd:string ;
        rdfs:subPropertyOf  :keyword .

:resource_legal_interpretation_requested_by_case-law
        a                   owl:ObjectProperty ;
        rdfs:comment        "1435 cases (2012-07-31). Example: 62011CN0266 : \"request for interpretation 32000L0078\". Relevant for legal analysis: true." ;
        rdfs:domain         :resource_legal ;
        rdfs:label          "Interpretation of legal resource requested by case law" ;
        rdfs:range          :case-law ;
        rdfs:subPropertyOf  :interpretation_requested_by ;
        owl:inverseOf       :case-law_requests_interpretation_resource_legal .

:restriction_on_use  a       owl:Class ;
        rdfs:label           "Restriction on use" ;
        rdfs:subClassOf      skos:Concept ;
        owl:equivalentClass  [ a               owl:Restriction ;
                               owl:hasValue    <http://publications.europa.eu/resource/authority/pub_repro> ;
                               owl:onProperty  skos:inScheme
                             ] .

:resolution_legislative_ep_term_parliamentary
        a                   owl:DatatypeProperty ;
        rdfs:comment        "This indicates the Parliamentary term during which an EP document was voted or EP question was raised. Relevant for legal analysis: true. Currently coded with FD_Table 285. However, only codes are exposed (not decoded), so 01, 02 etc." ;
        rdfs:domain         :resolution_legislative_ep ;
        rdfs:label          "Parliamentary term" ;
        rdfs:range          xsd:string ;
        rdfs:subPropertyOf  :term_parliamentary , :act_preparatory_term_parliamentary .

:date_entry-into-force
        a                   owl:DatatypeProperty ;
        rdfs:label          "Date entry into force" ;
        rdfs:range          xsd:date ;
        rdfs:subPropertyOf  :date .

:planned_consultation_period_date_start
        a           owl:DatatypeProperty ;
        rdfs:label  "Planned consultation period date start" .

:signatory_name  a  owl:DatatypeProperty ;
        rdfs:label  "Signatory name" .

:agent_related_to_event
        a              owl:ObjectProperty ;
        rdfs:comment   "This generic relation relates the agents to the event, in considering all possible ROLES of the agent (person, institution, ...), which does an event (any type of events)" ;
        rdfs:domain    :agent ;
        rdfs:label     "Agent related to event" ;
        rdfs:range     :event ;
        owl:inverseOf  :event_related_with_agent .

:manifests  a       owl:ObjectProperty ;
        rdfs:label  "Manifests" .

:summarizes  a      owl:ObjectProperty ;
        rdfs:label  "Summarizes" .

:dossier_date_creation_legacy
        a                   owl:DatatypeProperty ;
        rdfs:comment        "Legacy date of creation. if possible, original creation date of the Pegase notice. Procat and Pegase legacy creation dates. Relevant for legal analysis: true." ;
        rdfs:domain         :dossier ;
        rdfs:label          "Legacy date of creation for dossier" ;
        rdfs:range          xsd:date ;
        rdfs:subPropertyOf  :date_creation_legacy .

:procjur  a                  owl:Class ;
        rdfs:comment         "Corresponds to the procjur table" ;
        rdfs:label           "Concept representing judicial procedures (procédures juridictionnelles)" ;
        rdfs:subClassOf      skos:Concept , :concept_decoding ;
        owl:equivalentClass  [ a               owl:Restriction ;
                               owl:hasValue    <http://publications.europa.eu/resource/authority/procjur> ;
                               owl:onProperty  skos:inScheme
                             ] .

:manifestation_source-information
        a                   owl:DatatypeProperty ;
        rdfs:comment        "A note describing the source of description for this Manifestation. Based on 588 $a." ;
        rdfs:domain         :manifestation ;
        rdfs:label          "Source of information note for Manifestation" ;
        rdfs:range          xsd:string ;
        rdfs:subPropertyOf  :source_information ;
        dct:created         "2022-08-01T16:18:31.50"^^xsd:dateTime .

:signatory_name2  a  owl:DatatypeProperty ;
        rdfs:label  "Signatory name2" .

:validated_by  a    owl:ObjectProperty ;
        rdfs:label  "Validated by" .

:measure_national_implementing_reference_publication
        a                   owl:DatatypeProperty ;
        rdfs:comment        "DEPRECATED, Local publication reference for this NIM (in the national scheme)." ;
        rdfs:domain         :measure_national_implementing ;
        rdfs:label          "Publication reference" ;
        rdfs:range          xsd:string ;
        rdfs:subPropertyOf  :reference_publication ;
        owl:deprecated      true .

<http://publications.europa.eu/resource/authority/fd_350>
        a       owl:NamedIndividual .

:case-law_requests_interpretation_resource_legal
        a                   owl:ObjectProperty ;
        rdfs:comment        "This property points to legal act quoted in the operative part of Court decisions" ;
        rdfs:domain         :case-law ;
        rdfs:label          "Case law requests interpretation a legal resource" ;
        rdfs:range          :resource_legal ;
        rdfs:subPropertyOf  :requests_interpretation ;
        owl:inverseOf       :resource_legal_interpretation_requested_by_case-law .

:summarized_by  a   owl:ObjectProperty ;
        rdfs:label  "Summarized by" .

:procedure_code_interinstitutional_reference_procedure
        a                   owl:DatatypeProperty ;
        rdfs:comment        "Reference to this procedure. e.g. 1995/0305/COD or 2012/0204/NLE or 2012/0201/COD. Relevant for legal analysis: true." ;
        rdfs:domain         :procedure_code_interinstitutional ;
        rdfs:label          "Procedure reference" ;
        rdfs:range          xsd:string ;
        rdfs:subPropertyOf  :reference_procedure .

:event_informs_institution
        a                   owl:ObjectProperty ;
        rdfs:comment        "Relevant for legal analysis: true. This event addresses for information a given institution. Relevant for legal analysis: true" ;
        rdfs:domain         :event ;
        rdfs:label          "Event informs institution" ;
        rdfs:range          :institution ;
        rdfs:subPropertyOf  :informs ;
        owl:inverseOf       :institution_informed_by_event .

:proposal_act  a         owl:Class ;
        rdfs:comment     "The natural number of the COM can be encoded as id All Commission legislative proposals (proposal) are currently 5PC documents. The class proposal should accordingly NOT take the joint-proposal_decision, joint-proposal_directive and joint-proposal_regulation. They should go to their specific sub-classes." ;
        rdfs:label       "Proposal for an act" ;
        rdfs:subClassOf  :act_preparatory ;
        rdfs:subClassOf  [ a                   owl:Restriction ;
                           owl:maxCardinality  "1"^^xsd:nonNegativeInteger ;
                           owl:onProperty      :proposal_act_id_com
                         ] .

:ATTO_FD_361  a              owl:Class ;
        rdfs:label           "FD_361 ATTO table" ;
        rdfs:subClassOf      skos:Concept ;
        owl:equivalentClass  [ a               owl:Restriction ;
                               owl:hasValue    <http://publications.europa.eu/resource/authority/fd_361> ;
                               owl:onProperty  skos:inScheme
                             ] .

:resource_legal_service_associated
        a                   owl:DatatypeProperty ;
        rdfs:comment        "This field indicates the Commission DG or DGs co-responsible for drafting of an act. Relevant for legal analysis: true" ;
        rdfs:domain         :resource_legal ;
        rdfs:label          "Service associated" ;
        rdfs:range          xsd:string ;
        rdfs:subPropertyOf  :service_associated .

:agent_involved_in_event
        a                   owl:ObjectProperty ;
        rdfs:comment        "A specific agent is involved in this event" ;
        rdfs:domain         :agent ;
        rdfs:label          "Agent involved in event" ;
        rdfs:range          :event ;
        rdfs:subPropertyOf  :involved_in ;
        owl:inverseOf       :event_involves_agent .

:measure_national_implementing_national_website_link
        a                   owl:DatatypeProperty ;
        rdfs:comment        "URI of the national website and / or the concrete work. Can be at any granularity that the sending member states consider applicable, e.g. of the website itself, of the work or of some specific format (EURLEXNEW-2124 / CADMOS-1762)" ;
        rdfs:domain         :measure_national_implementing ;
        rdfs:label          "URI of national website" ;
        rdfs:range          xsd:anyURI ;
        rdfs:subPropertyOf  :national_website_link .

:work_contains_clause_legal
        a                   owl:ObjectProperty ;
        rdfs:domain         :work ;
        rdfs:label          "Work contains clause (legal)" ;
        rdfs:range          :clause_legal ;
        rdfs:subPropertyOf  :work_contains_subdivision , :contains .

:declares_void_by_preliminary_ruling
        a           owl:ObjectProperty ;
        rdfs:label  "Declares void by preliminary ruling" .

:measure_national_implementing_reference_commission
        a                   owl:DatatypeProperty ;
        rdfs:comment        "Reference of the NIM allocated by the Commission" ;
        rdfs:domain         :measure_national_implementing ;
        rdfs:label          "Reference Commission" ;
        rdfs:range          xsd:string ;
        rdfs:subPropertyOf  :reference_commission .

:year_reference  a  owl:DatatypeProperty ;
        rdfs:label  "Year reference" .

:reviews_judgement  a  owl:ObjectProperty ;
        rdfs:label  "Reviews judgement" .

:ATTO_FD_340  a              owl:Class ;
        rdfs:label           "FD_340 ATTO table" ;
        rdfs:subClassOf      skos:Concept ;
        owl:equivalentClass  [ a               owl:Restriction ;
                               owl:hasValue    <http://publications.europa.eu/resource/authority/fd_340> ;
                               owl:onProperty  skos:inScheme
                             ] .

<http://publications.europa.eu/resource/authority/pub_target>
        a       owl:NamedIndividual .

:act_other_eesc  a       owl:Class ;
        rdfs:comment     "5 European Economic and Social Committee other acts, mostly resolutions (5XE)" ;
        rdfs:label       "European Economic and Social Committee other act" ;
        rdfs:subClassOf  :act_preparatory_eesc ;
        rdfs:subClassOf  [ a                   owl:Restriction ;
                           owl:maxCardinality  "1"^^xsd:nonNegativeInteger ;
                           owl:onProperty      :act_other_eesc_number_session
                         ] .

<http://publications.europa.eu/resource/authority/com_internal_consultation_type>
        a       owl:NamedIndividual .

:date_reply  a              owl:DatatypeProperty ;
        rdfs:comment        "RP" ;
        rdfs:label          "Date reply" ;
        rdfs:range          xsd:date ;
        rdfs:subPropertyOf  :date .

:does_replacement_of  a  owl:ObjectProperty ;
        rdfs:label  "Does replacement of" .

:agent_depositary_for_agreement_international
        a                   owl:ObjectProperty ;
        rdfs:comment        "Agent (e.g. World Trade Organisation - Director-General) is depositary for an international agreement" ;
        rdfs:domain         :agent ;
        rdfs:label          "Agent is depositary for international agreement" ;
        rdfs:range          :agreement_international ;
        rdfs:subPropertyOf  :depositary_for ;
        owl:inverseOf       :agreement_international_stored_by_agent .

:url_etendering  a  owl:DatatypeProperty ;
        rdfs:label  "Url etendering" .

:organization_addressed_by_resource_legal
        a                   owl:ObjectProperty ;
        rdfs:domain         :organization ;
        rdfs:label          "Organization addressed by legal resource" ;
        rdfs:range          :resource_legal ;
        rdfs:subPropertyOf  :addressed_by ;
        owl:inverseOf       :resource_legal_addresses_organization .

:manifestation_official-journal_part_page_seq
        a                   owl:DatatypeProperty ;
        rdfs:comment        "Page sequence of the print manifestation of a act. Added in the context of IMMC2CDM-OJ" ;
        rdfs:domain         :manifestation_official-journal_part ;
        rdfs:label          "Page sequence" ;
        rdfs:range          xsd:positiveInteger ;
        rdfs:subPropertyOf  :page_seq .

:container_case-law_court
        a                   owl:DatatypeProperty ;
        rdfs:domain         :container_case-law ;
        rdfs:label          "Court reponsible for the work" ;
        rdfs:range          xsd:string ;
        rdfs:subPropertyOf  :court .

:signature_digital_type
        a                   owl:DatatypeProperty ;
        rdfs:comment        "Possible values XAdES-T and XAdES-A" ;
        rdfs:domain         :signature_digital ;
        rdfs:label          "Type of digital signature" ;
        rdfs:range          xsd:string ;
        rdfs:subPropertyOf  :type .

:summary_case-law_jure
        a                owl:Class ;
        rdfs:comment     "Summary of case law in JURE, treated as a separate bibliographic item Note: Title of the summary of case law: to be extracted from the created XML" ;
        rdfs:label       "Summary of case law in JURE" ;
        rdfs:subClassOf  :summary ;
        rdfs:subClassOf  [ a                   owl:Restriction ;
                           owl:minCardinality  "1"^^xsd:nonNegativeInteger ;
                           owl:onProperty      :summary_case-law_jure_id_celex
                         ] .

:event_internal_objection_period
        a                   owl:DatatypeProperty ;
        rdfs:comment        "Period (expressed in months or weeks to be confirmed) where the European Parliament and the Council have the right to object on a delegated act of the Commission" ;
        rdfs:domain         :event_internal ;
        rdfs:label          "Objection period" ;
        rdfs:range          xsd:positiveInteger ;
        rdfs:subPropertyOf  :objection_period .

:act_preparatory_session_date_end_planned
        a                   owl:DatatypeProperty ;
        rdfs:comment        "Date of session end. Corresponds to corext:date_end" ;
        rdfs:domain         :act_preparatory ;
        rdfs:label          "Planned end date of a session at the EESC" ;
        rdfs:range          xsd:date ;
        rdfs:subPropertyOf  :session_date_end_planned .

:resource_legal_completed_by_resource_legal
        a                   owl:ObjectProperty ;
        rdfs:comment        "Calculated" ;
        rdfs:domain         :resource_legal ;
        rdfs:label          "Legal resource completed by legal resource" ;
        rdfs:range          :resource_legal ;
        rdfs:subPropertyOf  :completed_by ;
        owl:inverseOf       :resource_legal_completes_resource_legal .

:person_reports_on_decision_internal_ep
        a                   owl:ObjectProperty ;
        rdfs:domain         :person ;
        rdfs:label          "Person reports on decision_internal_ep" ;
        rdfs:range          :decision_internal_ep ;
        rdfs:subPropertyOf  :reports_on ;
        owl:inverseOf       :decision_internal_ep_reported_by_person .

:internal_number_prefix
        a           owl:DatatypeProperty ;
        rdfs:label  "Internal number prefix" .

:concept_type_remark  a      owl:Class ;
        rdfs:comment         "Corresponds to the contents of the Prelex field DESCRIPTEUR, now coded with FD_Table 600" ;
        rdfs:label           "Concept representing the type of a remark in Prelex" ;
        rdfs:subClassOf      skos:Concept , :concept_decoding ;
        owl:equivalentClass  [ a               owl:Restriction ;
                               owl:hasValue    <http://publications.europa.eu/resource/authority/fd_600> ;
                               owl:onProperty  skos:inScheme
                             ] .

:question_parliamentary_asked_by_group_parliamentary
        a                   owl:ObjectProperty ;
        rdfs:comment        "This refers to political affiliation and nationality of the Member of the European Parliament who asked the question. Originally coded by FD_290, that shall be replaced by NAL corporate-body. Relevant for legal analysis: true" ;
        rdfs:domain         :question_parliamentary ;
        rdfs:label          "Parliamentary Querstion asked by parliamentary group" ;
        rdfs:range          :group_parliamentary ;
        rdfs:subPropertyOf  :asked_by ;
        owl:inverseOf       :group_parliamentary_asks_question_parliamentary .

:reviewed_by  a     owl:ObjectProperty ;
        rdfs:label  "Reviewed by" .

:case-law_corrects_judgement_resource_legal
        a                   owl:ObjectProperty ;
        rdfs:comment        "This points to the judgment/order that is concerned by the rectification order" ;
        rdfs:domain         :case-law ;
        rdfs:label          "Case law corrects judgement" ;
        rdfs:range          :resource_legal ;
        rdfs:subPropertyOf  :corrects_judgement ;
        owl:inverseOf       :resource_legal_judgement_corrected_by_case-law .

:expression_title  a        owl:DatatypeProperty ;
        rdfs:comment        "Relevant for legal analysis: true. Title of the expression. Any type of title (TI / TJ / TE...), also for case law (NOM_USUEL) and general publications. Relevant for legal analysis: true" ;
        rdfs:domain         :expression ;
        rdfs:label          "Expression Title" ;
        rdfs:range          rdfs:Literal ;
        rdfs:subPropertyOf  :title .

:agent_embargo  a           owl:DatatypeProperty ;
        rdfs:comment        "Is this agent under embargo? This instance must not be shown until the indicated datetime has been reached. In case a release date is not known,9999-12-31 should be used (= absolute embargo)" ;
        rdfs:domain         :agent ;
        rdfs:label          "Agent embargo" ;
        rdfs:range          xsd:dateTime ;
        rdfs:subPropertyOf  :embargo .

:working-document_ec  a  owl:Class ;
        rdfs:comment     "European Commission *working* document is different from a *staff working* document in that it is produced on the level of the Commission as such." ;
        rdfs:label       "Working document EC" ;
        rdfs:subClassOf  :act_preparatory_ec .

:reference-data_asset_published_in_reference-data_publication
        a              owl:ObjectProperty ;
        rdfs:comment   "A reference data asset is published by a reference data publication" ;
        rdfs:domain    :reference-data_asset ;
        rdfs:label     "Reference data asset published in reference data publication" ;
        rdfs:range     :reference-data_publication ;
        owl:inverseOf  :reference-data_publication_publishes_reference-data_asset .

:procurement_public_heading
        a                   owl:DatatypeProperty ;
        rdfs:domain         :procurement_public ;
        rdfs:label          "Heading of the procurement notice" ;
        rdfs:range          xsd:string ;
        rdfs:subPropertyOf  :heading .

:collection_document_contains_official-journal
        a                   owl:ObjectProperty ;
        rdfs:domain         :collection_document ;
        rdfs:label          "Collection contains official journal" ;
        rdfs:range          :official-journal ;
        rdfs:subPropertyOf  :contains ;
        owl:inverseOf       :official-journal_part_of_collection_document .

:act_consolidated_reference_act_consolidated
        a                   owl:DatatypeProperty ;
        rdfs:comment        "DEPRECATED, Consleg reference (example: <CONSOLID_FAMILY>1953D0030</CONSOLID_FAMILY>) ( use based_on instead) Could be used as the basis for links between consolidated acts of one base act." ;
        rdfs:domain         :act_consolidated ;
        rdfs:label          "Consolidated act reference" ;
        rdfs:range          xsd:string ;
        rdfs:subPropertyOf  :reference_act_consolidated ;
        owl:deprecated      true .

:unit_administrative_part_of_unit_administrative
        a                   owl:ObjectProperty ;
        rdfs:comment        "The administrative unit is part of another administrative unit. To be coordinated with the country CAT" ;
        rdfs:domain         :unit_administrative ;
        rdfs:label          "Administrative unit is part of administrative unit" ;
        rdfs:range          :unit_administrative ;
        rdfs:subPropertyOf  :part_of .

:manifestation_distribution_date_modified
        a                   owl:DatatypeProperty ;
        rdfs:comment        "This property contains the most recent data on which the distribution was changed or modified" ;
        rdfs:domain         :manifestation_distribution ;
        rdfs:label          "Distribution date modified" ;
        rdfs:range          xsd:date ;
        rdfs:subPropertyOf  :date_modified .

:id_doc_summarized  a  owl:DatatypeProperty ;
        rdfs:label  "Id doc summarized" .

:resource_legal_position_eesc
        a                   owl:DatatypeProperty ;
        rdfs:comment        "Internal reference of the opinions of the European Economic and Social Committee. Relevant for legal analysis: true" ;
        rdfs:domain         :resource_legal ;
        rdfs:label          "Position of European Economic and Social Committee" ;
        rdfs:range          xsd:string ;
        rdfs:subPropertyOf  :position_eesc .

:decision_cjeu  a        owl:Class ;
        rdfs:comment     "Decision of the Court of Justice (6CD)" ;
        rdfs:label       "Decision of the Court of Justice" ;
        rdfs:subClassOf  :case-law .

:case-law_suspends_application_of_resource_legal
        a                   owl:ObjectProperty ;
        rdfs:comment        "This property points to legal act quoted in the operative part of Court decisions." ;
        rdfs:domain         :case-law ;
        rdfs:label          "Case law suspends application of legal resource" ;
        rdfs:range          :resource_legal ;
        rdfs:subPropertyOf  :suspends_application_of ;
        owl:inverseOf       :resource_legal_application_suspended_by_case-law .

:resource_legal_repertoire
        a                   owl:DatatypeProperty ;
        rdfs:comment        "Indicator for the extraction of titles for the production of the directory of legislation in force. Mandatory for legislation, commission proposals and agreements. REP with the following possible value: \"REP\": legal resource appears in the directory with a full title. \"LIE\": legal resource appears in the directory as a reference. \"CADUC\": legal resource stricken from the directory. In theory this is linked to FD_Table091, but the \"translations\" retake the original codes This will not be translated, there are no labels used in the interface. Only the coded values are exposed" ;
        rdfs:domain         :resource_legal ;
        rdfs:label          "Repertoire of legislation in force" ;
        rdfs:range          xsd:string ;
        rdfs:subPropertyOf  :repertoire .

:person_reports_on_resolution_other_ep
        a              owl:ObjectProperty ;
        rdfs:domain    :person ;
        rdfs:label     "Person reports on resolution other ep" ;
        rdfs:range     :resolution_other_ep ;
        owl:inverseOf  :resolution_other_ep_reported_by_person .

:com_final  a            owl:Class ;
        rdfs:comment     "Digitized COM final document (a Commission proposal), digitized based on the fonds of the OIB archive. For practical purposes this digitization is treated as a separate work from the \"main\" Commission proposal that has undergone full legal analysis. It may be related to this COM using cdm:work_is_another_publication_of_work. The exact type of this COM is indicated via cdm: work_has_resource-type, mapped from /oibtrans:oib_transmission_request/cmt:transmission/cmt:workflow/cm:work/cm:type_work The COM identifier (= cdm:work_id_document) can be built based on cmext:prefix, cmext:year and cmext:number. These are individually mapped to annotations to cdm:work_id_document (annotation:prefix, annotation:year, annotation:sequence_number). <cmext:internal_number><cmext:prefix>COM</cmext:prefix><cmext:year>1983</cmext:year><cmext:number>29</cmext:number></cmext:internal_number> cmext:reference_production is mapped to to cdm:work_reference_internal oibext:reference_volume is mapped to cdm:expression_source for the applicable linguistic versions. oibext:size is mapped to the technical metadata tdm:stream_size, oibext:datetime_creation to tdm:creating_application_date_created_by_application (cf. tdm.rdf for details) The link of a COM final and its COM package(s) is expressed at the manifestation level via cdm:manifestation_part_of_manifestation" ;
        rdfs:label       "Digitised COM final document" ;
        rdfs:subClassOf  :act_preparatory_ec .

:involved_in  a     owl:ObjectProperty ;
        rdfs:label  "Involved in" .

:institution_responsible_for_event_case
        a             owl:ObjectProperty ;
        rdfs:comment  "An institution is responsible for the execution of an event in a Court case" ;
        rdfs:domain   :institution ;
        rdfs:label    "Institution responsible for a Court case event" ;
        rdfs:range    :event_case .

:document_reference  a  owl:DatatypeProperty ;
        rdfs:label  "Document reference" .

:measure_national_implementing
        a                owl:Class ;
        rdfs:comment     "National implementing measures (= sector 7 in EUR-Lex). Information on National implementing measures aka NIMs are currently typically expressed in VOLET_MNE (MNE: mésure nationale d'exécution = NIM). This volet contains references to the national implementing measures enacted in order to comply with European directives. The volet is usually directly fed by data issued by the Secretariat General. Note: Information on National Implementing Measures are currently partially encoded as \"true\" sector 7 document, but for the most part they are stored in the VOLET_MNE of their \"mother\" directive. However, for conversion these must become their own objects, only linked to the directive(s) they implement. As an example the <VOLET_MNE> of the Council directive Council Directive 2009/158/EC of 30 November 2009 (= 32009L0158) on \"animal health conditions governing intra-Community trade in, and imports from third countries of, poultry and hatching eggs\" that shows how the country codes are used to encode the title(s) of the NIMs belonging to a given directive. The number of different implementing measures can vary per country. {code} <VOLET_MNE><DE>1. - Neunte Verordnung zur Änderung der Binnenmarkt-Tiersuchenverordnung vom 27. März 2006</DE><DE>2. - Zehnte Verordnung zur Änderung der Binnenmarkt-Tierseuchenschutzverordnung vom 11. Dezember 2006</DE><DE>3. - Bekanntmachung der Neufassung der Binnenmarkt-Tierseuchenschutzverordnung vom 6. April 2005</DE><LV>1. - Mājputnu un inkubējamo olu aprites kārtība</LV><CZ>1. - Zákon č. 131/2003 Sb., kterým se mění zákon č. 166/1999 Sb., o veterinární péči a o změně některých souvisejících zákonů (veterinární zákon), ve znění pozdějších předpisů, a některé další zákony</CZ> [...] <CZ>8. - Vyhláška č. 12/2010 Sb., kterou se mění vyhláška č. 299/2003 Sb., o opatřeních pro předcházení a zdolávání nákaz a nemocí přenosných ze zvířat na člověka, ve znění pozdějších předpisů</CZ><CZ>9. - Zákon č. 182/2008 Sb., kterým se mění zákon č. 166/1999 Sb., o veterinární péči a o změně některých souvisejících zákonů (veterinární zákon), ve znění pozdějších předpisů, zákon č. 634/2004 Sb., o správních poplatcích, ve znění pozdějších předpisů, a zákon č. 154/2000 Sb., o šlechtění, plemenitbě a evidenci hospodářských zvířat a o změně některých souvisejících zákonů (plemenářský zákon), ve znění pozdějších předpisů</CZ> [...] </VOLET_MNE> {code}" ;
        rdfs:label       "National implementing measures" ;
        rdfs:subClassOf  :resource_legal ;
        rdfs:subClassOf  [ a                   owl:Restriction ;
                           owl:maxCardinality  "1"^^xsd:nonNegativeInteger ;
                           owl:onProperty      :measure_national_implementing_reference_member-state
                         ] ;
        rdfs:subClassOf  [ a                   owl:Restriction ;
                           owl:maxCardinality  "1"^^xsd:nonNegativeInteger ;
                           owl:onProperty      :measure_national_implementing_reference_commission
                         ] ;
        rdfs:subClassOf  [ a                            owl:Restriction ;
                           owl:minQualifiedCardinality  "1"^^xsd:nonNegativeInteger ;
                           owl:onClass                  :resource_legal ;
                           owl:onProperty               :measure_national_implementing_implements_resource_legal
                         ] ;
        rdfs:subClassOf  [ a                            owl:Restriction ;
                           owl:minQualifiedCardinality  "1"^^xsd:nonNegativeInteger ;
                           owl:onClass                  :country ;
                           owl:onProperty               :measure_national_implementing_implemented_by_country
                         ] ;
        rdfs:subClassOf  [ a                   owl:Restriction ;
                           owl:maxCardinality  "1"^^xsd:nonNegativeInteger ;
                           owl:onProperty      :measure_national_implementing_declaration_transposition_member-state
                         ] .

:decision_internal_ep_term_parliamentary
        a                   owl:DatatypeProperty ;
        rdfs:comment        "This indicates the Parliamentary term during which an EP document was voted or EP question was raised. Relevant for legal analysis: true. Currently coded with FD_Table 285. However, only codes are exposed (not decoded), so 01, 02 etc" ;
        rdfs:domain         :decision_internal_ep ;
        rdfs:label          "Parliamentary term" ;
        rdfs:range          xsd:string ;
        rdfs:subPropertyOf  :term_parliamentary , :act_preparatory_term_parliamentary .

:case_court  a           owl:Class ;
        rdfs:comment     "Case at a Court (pending or closed)" ;
        rdfs:label       "Case at a Court" ;
        rdfs:subClassOf  :dossier ;
        rdfs:subClassOf  [ a                owl:Restriction ;
                           owl:cardinality  "1"^^xsd:nonNegativeInteger ;
                           owl:onProperty   :case_court_identifier_year
                         ] ;
        rdfs:subClassOf  [ a                            owl:Restriction ;
                           owl:maxQualifiedCardinality  "1"^^xsd:nonNegativeInteger ;
                           owl:onClass                  :case-status ;
                           owl:onProperty               :case_court_has_case-status
                         ] ;
        rdfs:subClassOf  [ a                   owl:Restriction ;
                           owl:maxCardinality  "1"^^xsd:nonNegativeInteger ;
                           owl:onProperty      :case_court_identifier_extension_number
                         ] ;
        rdfs:subClassOf  [ a                owl:Restriction ;
                           owl:cardinality  "1"^^xsd:nonNegativeInteger ;
                           owl:onProperty   :case_court_identifier_court
                         ] ;
        rdfs:subClassOf  [ a                owl:Restriction ;
                           owl:cardinality  "1"^^xsd:nonNegativeInteger ;
                           owl:onProperty   :case_court_identifier_number
                         ] ;
        rdfs:subClassOf  [ a                   owl:Restriction ;
                           owl:maxCardinality  "1"^^xsd:nonNegativeInteger ;
                           owl:onProperty      :case_court_identifier_extension
                         ] .

:event_case_responsibility_of_advocate-general
        a                   owl:ObjectProperty ;
        rdfs:comment        "The advocate general is responsible for this case event" ;
        rdfs:domain         :event_case ;
        rdfs:label          "Case event under responsibility of the advocate general" ;
        rdfs:range          :advocate-general ;
        rdfs:subPropertyOf  :responsibility_of .

:reported_by_associated
        a           owl:ObjectProperty ;
        rdfs:label  "Reported by associated" .

:incorporates  a    owl:ObjectProperty ;
        rdfs:label  "Incorporates" .

:eli    a                   owl:DatatypeProperty ;
        rdfs:comment        "Entities with relation to the European Legislative Identifier (ELI)" ;
        rdfs:label          "Eli" ;
        rdfs:subPropertyOf  :identifier .

:concept_media_type_is_media_type_of_manifestation_distribution
        a              owl:ObjectProperty ;
        rdfs:comment   "A concept representing the media type of a distribution manifestation of a dataset" ;
        rdfs:domain    :concept_media_type ;
        rdfs:label     "Concept representing the media type of dataset distribution manifestation" ;
        rdfs:range     :manifestation_distribution ;
        owl:inverseOf  :manifestation_distribution_has_media_type_concept_media_type .

<http://publications.europa.eu/resource/authority/place>
        a       owl:NamedIndividual .

:work_sequence  a           owl:DatatypeProperty ;
        rdfs:comment        "Order of the work in a group of works. IMMC2CDM-COM. Relevant for legal analysis: true." ;
        rdfs:domain         :work ;
        rdfs:label          "Sequence of work" ;
        rdfs:range          xsd:positiveInteger ;
        rdfs:subPropertyOf  :sequence .

:procurement_public_version_model
        a                   owl:DatatypeProperty ;
        rdfs:comment        "Version of the procurement public model as modeled in CDM, for EUDOR to distinguish different model versions." ;
        rdfs:domain         :procurement_public ;
        rdfs:label          "Version of the procurement public model" ;
        rdfs:range          xsd:string ;
        rdfs:subPropertyOf  :version .

:event_based_on_suggested_resource_legal
        a            owl:ObjectProperty ;
        rdfs:domain  :event ;
        rdfs:label   "Event based on suggested resource legal" ;
        rdfs:range   :resource_legal ;
        dct:created  "2018-07-20T08:53:56.623+02:00"^^xsd:dateTime .

<http://publications.europa.eu/resource/authority/dir-eu-legal-act>
        a       owl:NamedIndividual .

:suspended_by  a    owl:ObjectProperty ;
        rdfs:label  "Suspended by" .

:manifestation_official-journal-act_pages_total
        a                   owl:DatatypeProperty ;
        rdfs:comment        "Total number of pages in an Official Journal act document" ;
        rdfs:domain         :manifestation_official-journal-act ;
        rdfs:label          "Manifestation Official Journal act pages total" ;
        rdfs:range          xsd:string ;
        rdfs:subPropertyOf  :pages_total , :manifestation_extent .

:information_language_expression
        a           owl:DatatypeProperty ;
        rdfs:label  "Information language expression" .

:act_consolidated_based_on_resource_legal
        a                   owl:ObjectProperty ;
        rdfs:comment        "This consolidated act starts out with this legal resource as its basic act. Could be used as the basis for links between consolidated acts of one base act, use either CONSOLIF_FAMILY or CONSLEG_REFER depending on the type of consolidated act, relating to a layer or to a family." ;
        rdfs:domain         :act_consolidated ;
        rdfs:label          "Consolidated act based on legal resource" ;
        rdfs:range          :resource_legal ;
        rdfs:subPropertyOf  :based_on ;
        owl:inverseOf       :resource_legal_basis_for_act_consolidated .

:publication-accessibility_is-feature-accessibility-of_manifestation
        a                   owl:ObjectProperty ;
        rdfs:comment        "Publication accessibility feature(s) of a manifestion." ;
        rdfs:domain         :publication-accessibility ;
        rdfs:label          "Publication accessibility feature of manifestation" ;
        rdfs:range          :manifestation ;
        rdfs:subPropertyOf  :is_feature_of ;
        dct:created         "2022-08-01T16:18:31.50"^^xsd:dateTime .

:states_failure_concerning
        a           owl:ObjectProperty ;
        rdfs:label  "States failure concerning" .

:ATTO_FD_606  a              owl:Class ;
        rdfs:label           "FD_606 ATTO table" ;
        rdfs:subClassOf      skos:Concept ;
        owl:equivalentClass  [ a               owl:Restriction ;
                               owl:hasValue    <http://publications.europa.eu/resource/authority/fd_606> ;
                               owl:onProperty  skos:inScheme
                             ] .

:act_preparatory_session_date_start_planned
        a                   owl:DatatypeProperty ;
        rdfs:comment        "Date of session start.Corresponds to corext:date_start" ;
        rdfs:domain         :act_preparatory ;
        rdfs:label          "Planned starting date of a session at the EESC" ;
        rdfs:range          xsd:date ;
        rdfs:subPropertyOf  :session_date_start_planned .

:regulation_date_transposition
        a                   owl:DatatypeProperty ;
        rdfs:comment        "Date of transposition applicable to regulations; can contain multiple values as different parts of a dirctive can be implemented by various pieces of national legislation, coming with different dates (TP_DATE). TP_COMMENT is mixed content, coded with fd_361. Relevant for legal analysis: true." ;
        rdfs:domain         :regulation ;
        rdfs:label          "Date of transposition of a regulation" ;
        rdfs:range          xsd:date ;
        rdfs:subPropertyOf  :date_transposition .

:page_official_journal
        a           owl:DatatypeProperty ;
        rdfs:label  "Page official journal" .

<http://publications.europa.eu/resource/authority/subject-matter>
        a       owl:NamedIndividual .

:resource_legal_basis_for_resource_legal
        a                   owl:ObjectProperty ;
        rdfs:comment        "This points to the legal resource that is based on this act. Never directly specified, inverse property of cdm:resource_legal_based_on_resource_legal. Relevant for legal analysis: true" ;
        rdfs:domain         :resource_legal ;
        rdfs:label          "Legal resource is basis for legal resource" ;
        rdfs:range          :resource_legal ;
        rdfs:subPropertyOf  :basis_for ;
        owl:inverseOf       :resource_legal_based_on_resource_legal .

:manifestation-issue_title-series
        a                   owl:DatatypeProperty ;
        rdfs:comment        "Issue manifestation has a series title which points to the series; can be combined with an ant:volume-designation" ;
        rdfs:domain         :manifestation-issue ;
        rdfs:label          "Issue manifestation title series" ;
        rdfs:range          rdf:PlainLiteral ;
        rdfs:subPropertyOf  :title ;
        dct:created         "2022-09-09T09:34:00.000"^^xsd:dateTime .

:proposal_decision_codified_ec
        a                owl:Class ;
        rdfs:comment     "17 Commission Proposal Codified Decision (5GC)" ;
        rdfs:label       "Commission proposal for a codified decision" ;
        rdfs:subClassOf  :act_preparatory_ec .

:manifestation_source-pool
        a                   owl:DatatypeProperty ;
        rdfs:comment        "String that indicates the source pool" ;
        rdfs:domain         :manifestation ;
        rdfs:label          "Source pool" ;
        rdfs:range          xsd:string ;
        rdfs:subPropertyOf  :source-pool .

:case-law_originates_in_country_role-qualifier
        a                   owl:ObjectProperty ;
        rdfs:comment        "Indicates country of origin of the applicant, the defendant or the court referring the case. Only after start of use of IMMC transmission. Currently fill both changes." ;
        rdfs:domain         :case-law ;
        rdfs:label          "Case law originates in country or uses a role qualifier" ;
        rdfs:range          :country_role-qualifier ;
        rdfs:subPropertyOf  :originates_in ;
        owl:inverseOf       :country_role-qualifier_initiates_case-law .

:act_preparatory_eca  a  owl:Class ;
        rdfs:comment     "Preparatory act by the European Court of Auditors" ;
        rdfs:label       "Preparatory act by ECA" ;
        rdfs:subClassOf  :act_preparatory ;
        rdfs:subClassOf  [ a               owl:Restriction ;
                           owl:hasValue    <http://publications.europa.eu/resource/authority/corporate-body/ECA> ;
                           owl:onProperty  :work_created_by_agent
                         ] ;
        dct:created      "2022-09-01T09:01:22"^^xsd:dateTime .

:procurement_public_labels_forms_link_type
        a                   owl:DatatypeProperty ;
        rdfs:domain         :procurement_public ;
        rdfs:label          "Label forms type" ;
        rdfs:range          xsd:string ;
        rdfs:subPropertyOf  :labels_forms_link_type .

:withdrawn-proposal  a  owl:DatatypeProperty ;
        rdfs:label  "Withdrawn proposal" .

:gets_opinion_of  a  owl:ObjectProperty ;
        rdfs:label  "Gets opinion of" .

:adds_to  a         owl:ObjectProperty ;
        rdfs:label  "Adds to" .

:work_contains_point  a     owl:ObjectProperty ;
        rdfs:comment        "The point of this work" ;
        rdfs:domain         :work ;
        rdfs:label          "Work contains point" ;
        rdfs:range          :point ;
        rdfs:subPropertyOf  :work_contains_subdivision , :contains .

:procurement_public  a   owl:Class ;
        rdfs:comment     "Any of the works related to public procurement (Ted)" ;
        rdfs:label       "Public procurement" ;
        rdfs:subClassOf  :work ;
        rdfs:subClassOf  [ a                owl:Restriction ;
                           owl:cardinality  "1"^^xsd:nonNegativeInteger ;
                           owl:onProperty   :procurement_public_number_edition
                         ] ;
        rdfs:subClassOf  [ a                owl:Restriction ;
                           owl:cardinality  "1"^^xsd:nonNegativeInteger ;
                           owl:onProperty   :procurement_public_number_document_in_official-journal
                         ] .

:work_explains_work  a      owl:ObjectProperty ;
        rdfs:comment        "Relevant for legal analysis: true. The work explains another work. Relevant for legal analysis: true" ;
        rdfs:domain         :work ;
        rdfs:label          "Work explains another work" ;
        rdfs:range          :work ;
        rdfs:subPropertyOf  :explains .

:affaire_year  a      owl:DatatypeProperty ;
        rdfs:comment  "Year part of the Court case identification" ;
        rdfs:label    "Year of case" .

:transliterated_organisation_national-id
        a           owl:DatatypeProperty ;
        rdfs:label  "Transliterated organisation national id" .

:archive_package_document_part_of_archive_package
        a                   owl:ObjectProperty ;
        rdfs:domain         :archive_package_document ;
        rdfs:label          "Archive package document part of archive package" ;
        rdfs:range          :archive_package ;
        rdfs:subPropertyOf  :work_part_of_work .

:validation_requested_by
        a           owl:ObjectProperty ;
        rdfs:label  "Validation requested by" .

:event_legal_responsibility_of_institution
        a                   owl:ObjectProperty ;
        rdfs:comment        "DEPRECATED, A given institution is primarily responsible for this legal event. Relevant for legal analysis: true." ;
        rdfs:domain         :event_legal ;
        rdfs:label          "Legal event under responsibility of an institution" ;
        rdfs:range          :institution ;
        rdfs:subPropertyOf  :responsibility_of , :event_responsibility_of_institution ;
        owl:deprecated      true ;
        owl:inverseOf       :institution_responsible_for_event_legal .

:subject  a         owl:DatatypeProperty ;
        rdfs:label  "Subject" .

:summary_legislation_eu_id_doc_related
        a                   owl:DatatypeProperty ;
        rdfs:domain         :summary_legislation_eu ;
        rdfs:label          "Natural number of related documents" ;
        rdfs:range          xsd:string ;
        rdfs:subPropertyOf  :id_doc_related .

:recommendation  a       owl:Class ;
        rdfs:comment     "Recommendation (subsector H of sector 3). At present 706 notices. Examples: 31960H1221,31963H0660, 32004H0705, 32010H0191" ;
        rdfs:label       "Recommendation" ;
        rdfs:subClassOf  :legislation_secondary .

<http://publications.europa.eu/resource/authority/fd_611>
        a       owl:NamedIndividual .

:resource_legal_addresses_institution
        a                   owl:ObjectProperty ;
        rdfs:comment        "Name of institution to which the act is addressed. Relevant for legal analysis: true" ;
        rdfs:domain         :resource_legal ;
        rdfs:label          "Legal resource addresses institution" ;
        rdfs:range          :institution ;
        rdfs:subPropertyOf  :addresses ;
        owl:inverseOf       :institution_addressed_by_resource_legal .

:rights  a          owl:DatatypeProperty ;
        rdfs:label  "Rights" .

:auxiliary-work  a       owl:Class ;
        rdfs:comment     "Works that derive their validity from the existance of another work to which they refer. Relationships between auxiliary works is modelled on FRBR 5.3.1, table 5.1: - has_successor: work_has_successor_work (e.g. sequel, suceeding works) - has_supplement: work_has_supplement_work (e.g. annex) - summarized_by / summarizes: summary_summarizes_work" ;
        rdfs:label       "Auxiliary works" ;
        rdfs:subClassOf  :work .

:work_publishes_work  a     owl:ObjectProperty ;
        rdfs:comment        "The work publishes another work. Meant to eventually replace resource_legal_publishes..." ;
        rdfs:domain         :work ;
        rdfs:label          "Work publishes another work" ;
        rdfs:range          :work ;
        rdfs:subPropertyOf  :publishes ;
        owl:inverseOf       :work_published_in_work .

:concept_theme_dataset_is_theme_of_work_dataset
        a              owl:ObjectProperty ;
        rdfs:domain    :concept_theme_dataset ;
        rdfs:label     "Concept theme dataset is theme of work dataset" ;
        rdfs:range     :work_dataset ;
        owl:inverseOf  :work_dataset_has_theme_concept_theme_dataset .

:classification_summary_subject_of_summary_legislation_eu
        a                   owl:ObjectProperty ;
        rdfs:domain         :classification_summary ;
        rdfs:label          "Classification of a summary of EU legislation is subject of a summary of EU legislation" ;
        rdfs:range          :summary_legislation_eu ;
        rdfs:subPropertyOf  :subject_of ;
        owl:inverseOf       :summary_legislation_eu_is_about_classification_summary .

:procedure_comment  a  owl:DatatypeProperty ;
        rdfs:label  "Procedure comment" .

:event_internal_uses_concept_mode_decision
        a                   owl:ObjectProperty ;
        rdfs:comment        "This property describes the concept mode decision of the internal event" ;
        rdfs:domain         :event_internal ;
        rdfs:label          "Event internal uses concept mode decision" ;
        rdfs:range          :concept_mode_decision ;
        rdfs:subPropertyOf  :uses .

:work_date_archived  a      owl:DatatypeProperty ;
        rdfs:comment        "The document remains visible even if archived" ;
        rdfs:domain         :work ;
        rdfs:label          "Date archived" ;
        rdfs:range          xsd:date ;
        rdfs:subPropertyOf  :date_archived .

:expression_title_information_additional
        a                   owl:DatatypeProperty ;
        rdfs:comment        "Additional information on the type of the title (TIT_QUAL). Relevant for legal analysis: true." ;
        rdfs:domain         :expression ;
        rdfs:label          "Additional information on title" ;
        rdfs:range          rdfs:Literal ;
        rdfs:subPropertyOf  :title_information_additional .

:opinion_ep  a           owl:Class ;
        rdfs:label       "European Parliament opinion" ;
        rdfs:subClassOf  :act_preparatory_ep .

:ATTO_FD_537  a              owl:Class ;
        rdfs:label           "FD_537 ATTO table" ;
        rdfs:subClassOf      skos:Concept ;
        owl:equivalentClass  [ a               owl:Restriction ;
                               owl:hasValue    <http://publications.europa.eu/resource/authority/fd_537> ;
                               owl:onProperty  skos:inScheme
                             ] .

:type   a           owl:DatatypeProperty ;
        rdfs:label  "Any kind of type" .

[ a            owl:AllDisjointClasses ;
  owl:members  ( :concept_case-law :concept_new_case-law :concept_directory-code :concept_eurovoc :subject-matter :concept_prelex_council )
] .

:event_session_date_end
        a                   owl:DatatypeProperty ;
        rdfs:comment        "The end date of the session during which this event took place, e.g. in the Council or the Committee of the Regions" ;
        rdfs:domain         :event ;
        rdfs:label          "End date of a session" ;
        rdfs:range          xsd:date ;
        rdfs:subPropertyOf  :session_date_end .

:resolution_other_ep_term_parliamentary
        a                   owl:DatatypeProperty ;
        rdfs:comment        "This indicates the Parliamentary term during which an EP document was voted or EP question was raised. Relevant for legal analysis: true. Currently coded with FD_Table 285. However, only codes are exposed (not decoded), so 01, 02 etc." ;
        rdfs:domain         :resolution_other_ep ;
        rdfs:label          "Parliamentary term" ;
        rdfs:range          xsd:string ;
        rdfs:subPropertyOf  :term_parliamentary , :act_preparatory_term_parliamentary .

:event_legal_mandatorily-addresses_institution
        a                   owl:ObjectProperty ;
        rdfs:comment        "This legal event mandatorily addresses a given institution. Corresponds to role type ADDRESSEE_MANDATORY" ;
        rdfs:domain         :event_legal ;
        rdfs:label          "Legal event mandatorily addresses institution" ;
        rdfs:range          :institution ;
        rdfs:subPropertyOf  :mandatorily-addresses ;
        owl:inverseOf       :institution_mandatorily-addressed_by_event_legal .

:has_product_form  a  owl:ObjectProperty ;
        rdfs:label  "Has product form" .

:proposal_directive_codified_ec
        a                owl:Class ;
        rdfs:comment     "77 Commission Proposal Codified Directive(5FC)" ;
        rdfs:label       "Commission proposal for a codified directive" ;
        rdfs:subClassOf  :act_preparatory_ec .

foaf:name  a    owl:NamedIndividual .

:official-journal_number
        a                   owl:DatatypeProperty ;
        rdfs:comment        "Number of the OJ" ;
        rdfs:domain         :official-journal ;
        rdfs:label          "OJ number" ;
        rdfs:range          xsd:positiveInteger ;
        rdfs:subPropertyOf  :number .

<http://publications.europa.eu/resource/authority/fd_499>
        a       owl:NamedIndividual .

:ATTO_FD_601  a              owl:Class ;
        rdfs:label           "FD_601 ATTO table" ;
        rdfs:subClassOf      skos:Concept ;
        owl:equivalentClass  [ a               owl:Restriction ;
                               owl:hasValue    <http://publications.europa.eu/resource/authority/fd_601> ;
                               owl:onProperty  skos:inScheme
                             ] .

:resource_legal_procedure_type
        a                   owl:DatatypeProperty ;
        rdfs:comment        "Type of the corresponding legal procedure. Obsolete, only maintained for backwards compatibility. Relevant for legal analysis: true" ;
        rdfs:domain         :resource_legal ;
        rdfs:label          "Legal procedure type" ;
        rdfs:range          xsd:string ;
        rdfs:subPropertyOf  :procedure_type .

:resource_legal_declared_void_by_case-law
        a                   owl:ObjectProperty ;
        rdfs:comment        "Calculated. Relevant for legal analysis: true." ;
        rdfs:domain         :resource_legal ;
        rdfs:label          "Legal resource declared void by case law" ;
        rdfs:range          :case-law ;
        rdfs:subPropertyOf  :declared_void_by ;
        owl:inverseOf       :case-law_declares_void_resource_legal .

:resource_legal_influenced_by_resource_legal
        a                   owl:ObjectProperty ;
        rdfs:domain         :resource_legal ;
        rdfs:label          "Legal resource influences legal resource" ;
        rdfs:range          :resource_legal ;
        rdfs:subPropertyOf  :influenced_by ;
        owl:inverseOf       :resource_legal_influences_resource_legal .

:manifestation-audiovisual_duration-playing-time
        a                   owl:DatatypeProperty ;
        rdfs:comment        "Playing time of an audiobook, video or music in format PT3H21M15S (3 hours, 21 minutes, 15 seconds)" ;
        rdfs:domain         :manifestation-audiovisual ;
        rdfs:label          "Playing time duration of an audiovisual manifestation" ;
        rdfs:range          xsd:duration ;
        rdfs:subPropertyOf  :duration ;
        dct:created         "2022-08-01T16:18:31.50"^^xsd:dateTime .

:concept_eurovoc  a          owl:Class ;
        rdfs:comment         "Eurovoc will retake the SKOS-XL model developed for that. The detailed representation of the subject is out of scope of this datamodel and will have to align with the SKOS-representation of Eurovoc Note: The current elements in VOLET_EUROVOC other than EUROVOC itself, namely EUROVOC_PROP, EUROVOC_PROP_CODE, EUROVOC_PROP_TERM, EUROVOC_OLD, EUROVOC_OLD_CODE and EUROVOC_OLD_TERM seem to be little to not used. They will be ignored" ;
        rdfs:label           "Eurovoc concept" ;
        rdfs:subClassOf      skos:Concept , :concept ;
        owl:equivalentClass  [ a               owl:Restriction ;
                               owl:hasValue    <http://eurovoc.europa.eu/100141> ;
                               owl:onProperty  skos:inScheme
                             ] .

:work_illustrated_by_agent
        a                   owl:ObjectProperty ;
        rdfs:comment        "The work is illustrated by an agent (AU)" ;
        rdfs:domain         :work ;
        rdfs:label          "Work is illustrated by agent" ;
        rdfs:range          :agent ;
        rdfs:subPropertyOf  :work_contributed_to_by_agent , :illustrated_by ;
        dct:created         "2018-08-30T11:10:59.946+02:00"^^xsd:dateTime ;
        owl:inverseOf       :agent_illustrates_work .

:has_type_act  a    owl:ObjectProperty ;
        rdfs:label  "Has type act" .

:id_com  a                  owl:DatatypeProperty ;
        rdfs:label          "Id com" ;
        rdfs:subPropertyOf  :identifier .

:dossier_contains_work
        a                   owl:ObjectProperty ;
        rdfs:comment        "Relevant for legal analysis: true. This dossier contains a work. Relevant for legal analysis: true" ;
        rdfs:domain         :dossier ;
        rdfs:label          "Dossier contains work" ;
        rdfs:range          :work ;
        rdfs:subPropertyOf  :contains ;
        owl:inverseOf       :work_part_of_dossier .

:procedure_code_interinstitutional_number_procedure
        a                   owl:DatatypeProperty ;
        rdfs:comment        "Number of this procedure. Relevant for legal analysis: true." ;
        rdfs:domain         :procedure_code_interinstitutional ;
        rdfs:label          "Number of procedure" ;
        rdfs:range          xsd:string ;
        rdfs:subPropertyOf  :number_procedure .

:oj_c   a                owl:Class ;
        rdfs:comment     "Other documents published in the Official Journal C Series (= sector C in EUR-Lex) . Sector C effectively has only one subsector called again C, so no further subclasses are needed." ;
        rdfs:label       "OJ C series" ;
        rdfs:subClassOf  :resource_legal .

:act_other_committee_ecsc
        a                owl:Class ;
        rdfs:comment     "4 European Coal and Steel Community (ECSC) Consultative Committee's other acts (5XK)" ;
        rdfs:label       "ECSC Committee other act" ;
        rdfs:subClassOf  :act_preparatory_ecsc .

:event_legal_gets_opinion_of_institution
        a                   owl:ObjectProperty ;
        rdfs:comment        "Relevant for legal analysis: true. This legal gets the opinon of given institution. Body role:Author of opinion. Relevant for legal analysis: true" ;
        rdfs:domain         :event_legal ;
        rdfs:label          "Legal event gets the opinion of an institution" ;
        rdfs:range          :institution ;
        rdfs:subPropertyOf  :gets_opinion_of ;
        owl:inverseOf       :institution_authors-opinion_event_legal .

:is_feature_of  a   owl:ObjectProperty ;
        rdfs:label  "Is feature of" .

:joint-proposal_decision
        a                owl:Class ;
        rdfs:comment     "where its resource_legal_type = JC, resource_legal_id_sector = 5, work_has_resource-type = JOINT_PROP_DEC" ;
        rdfs:label       "Joint proposal for a decision" ;
        rdfs:subClassOf  :proposal_act , :act_preparatory_joint .

:dissemination-status_is-status-of_manifestation-mobile-app
        a                   owl:ObjectProperty ;
        rdfs:domain         :dissemination-status ;
        rdfs:label          "Dissemination status is status of manifestation mobile app" ;
        rdfs:range          :manifestation-mobile-app ;
        rdfs:subPropertyOf  :is_status_of ;
        dct:created         "2022-08-01T16:18:31.50"^^xsd:dateTime ;
        owl:inverseOf       :manifestation-mobile-app_has-status_dissemination-status .

:reference-data_publication
        a                owl:Class ;
        rdfs:comment     "A dataset representing a (potentially complex) publication of reference data assets. The manifestations of such a dataset contain the zipped assets. The documentation of a publication is represented by a linked object with class cdm:documentation." ;
        rdfs:label       "Publication of reference data asset(s)" ;
        rdfs:subClassOf  :work_dataset ;
        rdfs:subClassOf  [ a                   owl:Restriction ;
                           owl:minCardinality  "1"^^xsd:nonNegativeInteger ;
                           owl:onProperty      :reference-data_publication_publishes_reference-data_asset
                         ] .

:staff-working-document_id_com
        a                   owl:DatatypeProperty ;
        rdfs:comment        "COM or SEC or SWD catalogue number. Relevant for legal analysis: true" ;
        rdfs:domain         :staff-working-document ;
        rdfs:label          "COM identifier of SEC and SWD" ;
        rdfs:range          xsd:string ;
        rdfs:subPropertyOf  :id_com .

:measure_national_implementing_official_journal
        a                   owl:DatatypeProperty ;
        rdfs:comment        "DEPRECATED, National or regional official journal in which this NIM was published. Replaced by the individual fields name_official_journal, number_official_journal, date_official_journal, page_official_journal" ;
        rdfs:domain         :measure_national_implementing ;
        rdfs:label          "National or regional Official Journal" ;
        rdfs:range          xsd:string ;
        rdfs:subPropertyOf  :official_journal ;
        owl:deprecated      true .

:ATTO_FD_070  a              owl:Class ;
        rdfs:label           "FD_070 ATTO table" ;
        rdfs:subClassOf      skos:Concept ;
        owl:equivalentClass  [ a               owl:Restriction ;
                               owl:hasValue    <http://publications.europa.eu/resource/authority/fd_070> ;
                               owl:onProperty  skos:inScheme
                             ] .

:number_procedure  a  owl:DatatypeProperty ;
        rdfs:label  "Number procedure" .

:does_insertion_of  a  owl:ObjectProperty ;
        rdfs:label  "Does insertion of" .

:procurement_public_transliterated_phone
        a                   owl:DatatypeProperty ;
        rdfs:domain         :procurement_public ;
        rdfs:label          "Procurement public transliterated phone" ;
        rdfs:range          xsd:string ;
        rdfs:subPropertyOf  :transliterated_phone .

:manifestation_print_reference_page_first
        a                   owl:DatatypeProperty ;
        rdfs:comment        "DEPRECATED, First page number of the OJ part related to a legal resource. Use manifestion_print_page_first" ;
        rdfs:domain         :manifestation_print_reference ;
        rdfs:label          "First page" ;
        rdfs:range          xsd:string ;
        rdfs:subPropertyOf  :page_first , :manifestation_print_page_first ;
        owl:deprecated      true .

:person_reports_on_event
        a                   owl:ObjectProperty ;
        rdfs:domain         :person ;
        rdfs:label          "Person reports on event" ;
        rdfs:range          :event ;
        rdfs:subPropertyOf  :reports_on .

:documentation  a        owl:Class ;
        rdfs:comment     "Documentation is used to describe dataset. Equivalent class in the cdm model to void:DatasetDescription" ;
        rdfs:label       "Documentation" ;
        rdfs:subClassOf  :work ;
        rdfs:subClassOf  [ a                   owl:Restriction ;
                           owl:maxCardinality  "1"^^xsd:nonNegativeInteger ;
                           owl:onProperty      :documentation_nature_classification
                         ] ;
        rdfs:subClassOf  [ a                            owl:Restriction ;
                           owl:maxQualifiedCardinality  "1"^^xsd:nonNegativeInteger ;
                           owl:onClass                  :concept_type_documentation ;
                           owl:onProperty               :documentation_has_type_concept_type_documentation
                         ] .

:agent_name  a              owl:DatatypeProperty ;
        rdfs:comment        "What is the name or other designation of this agent? The name can be the name of a person, an organization..., possibly qualified by language or script" ;
        rdfs:domain         :agent ;
        rdfs:label          "Agent name" ;
        rdfs:range          xsd:string ;
        rdfs:subPropertyOf  :name .

<http://publications.europa.eu/resource/authority/file-status>
        a       owl:NamedIndividual .

:resource_legal_related_question_to_resource_legal
        a                   owl:SymmetricProperty , owl:ObjectProperty ;
        rdfs:comment        "Relevant for legal analysis: true" ;
        rdfs:domain         :resource_legal ;
        rdfs:label          "Legal resource raises related question to legal resource" ;
        rdfs:range          :resource_legal ;
        rdfs:subPropertyOf  :related_question_to .

:signature_digital_date_signature_xades-t
        a                   owl:DatatypeProperty ;
        rdfs:comment        "Date and time this signature got its XAdES-T" ;
        rdfs:domain         :signature_digital ;
        rdfs:label          "XAdES-T date and time" ;
        rdfs:range          xsd:dateTime ;
        rdfs:subPropertyOf  :date_signature_xades-t .

:case-law_requests_annulment_of_resource_legal
        a                   owl:ObjectProperty ;
        rdfs:comment        "This property points to legal act quoted in the operative part of Court decisions" ;
        rdfs:domain         :case-law ;
        rdfs:label          "Case law requests annulment of legal resource" ;
        rdfs:range          :resource_legal ;
        rdfs:subPropertyOf  :requests_annulment_of ;
        owl:inverseOf       :resource_legal_annulment_requested_by_case-law .

<http://publications.europa.eu/resource/authority/fd_500>
        a       owl:NamedIndividual .

:manifestation_print_page_first
        a                   owl:DatatypeProperty ;
        rdfs:comment        "First page number of the OJ part related to a legal resource" ;
        rdfs:domain         :manifestation_print ;
        rdfs:label          "First page" ;
        rdfs:range          xsd:string ;
        rdfs:subPropertyOf  :page_first .

:front  a                owl:Class ;
        rdfs:comment     "\"distinct sections of a text (usually, but not necessarily, a printed one), prefixed to it by way of introduction or identification as a part of its production\" (TEI 4.5)" ;
        rdfs:label       "Front matter" ;
        rdfs:subClassOf  :textstructure .

:dossier_date_withdrawn
        a                   owl:DatatypeProperty ;
        rdfs:comment        "Relevant for legal analysis: true" ;
        rdfs:domain         :dossier ;
        rdfs:label          "Dossier was withdrawn on a given date" ;
        rdfs:range          xsd:date ;
        rdfs:subPropertyOf  :date_withdrawn .

:expression_title_short
        a                   owl:DatatypeProperty ;
        rdfs:comment        "Established short title of the expression (if any)" ;
        rdfs:domain         :expression ;
        rdfs:label          "Short title" ;
        rdfs:range          xsd:string ;
        rdfs:subPropertyOf  :title_short .

:case-law_national  a    owl:Class ;
        rdfs:comment     "National case law with relevance to EU law (sector 8)" ;
        rdfs:label       "National case law" ;
        rdfs:subClassOf  :case-law ;
        rdfs:subClassOf  [ a                   owl:Restriction ;
                           owl:maxCardinality  "1"^^xsd:nonNegativeInteger ;
                           owl:onProperty      :case-law_national_parties
                         ] ;
        rdfs:subClassOf  [ a                   owl:Restriction ;
                           owl:maxCardinality  "1"^^xsd:nonNegativeInteger ;
                           owl:onProperty      :case-law_national_judgement_reference
                         ] ;
        rdfs:subClassOf  [ a                            owl:Restriction ;
                           owl:maxQualifiedCardinality  "1"^^xsd:nonNegativeInteger ;
                           owl:onClass                  :agent ;
                           owl:onProperty               :case-law_national_delivered_by_court_depending_on_agent
                         ] .

:resource_legal_application_suspended_by_case-law
        a                   owl:ObjectProperty ;
        rdfs:comment        "Calculated. Relevant for legal analysis: true." ;
        rdfs:domain         :resource_legal ;
        rdfs:label          "Legal resource has application suspended by case law" ;
        rdfs:range          :case-law ;
        rdfs:subPropertyOf  :application_suspended_by ;
        owl:inverseOf       :case-law_suspends_application_of_resource_legal .

:publication_general_date_publication
        a                   owl:DatatypeProperty ;
        rdfs:comment        "The date that this resource was released to the public" ;
        rdfs:domain         :publication_general ;
        rdfs:label          "Publication date of general publication" ;
        rdfs:range          xsd:date ;
        rdfs:subPropertyOf  :date_publication .

:directive_date_transposition
        a                   owl:DatatypeProperty ;
        rdfs:comment        "Deadline for the transposition applicable to directives; can contain multiple values as different parts of a dirctive can be implemented by various pieces of national legislation, coming with different dates (TP_DATE). TP_COMMENT is mixed content, coded with fd_361. Relevant for legal analysis: true" ;
        rdfs:domain         :directive ;
        rdfs:label          "Date of transposition of a directive" ;
        rdfs:range          xsd:date ;
        rdfs:subPropertyOf  :date_transposition .

:collection_document_contains_work
        a                   owl:ObjectProperty ;
        rdfs:domain         :collection_document ;
        rdfs:label          "Document collection contains work" ;
        rdfs:range          :work ;
        rdfs:subPropertyOf  :contains ;
        owl:inverseOf       :work_part_of_collection_document .

:ecli   a           owl:DatatypeProperty ;
        rdfs:label  "Ecli" .

:id_document  a             owl:DatatypeProperty ;
        rdfs:label          "Id document" ;
        rdfs:subPropertyOf  :identifier .

:procurement_public_transliterated_postal_code
        a                   owl:DatatypeProperty ;
        rdfs:domain         :procurement_public ;
        rdfs:label          "Procurement public transliterated postal code" ;
        rdfs:range          xsd:string ;
        rdfs:subPropertyOf  :transliterated_postal_code .

:manifestation_court-report_part
        a                owl:Class ;
        rdfs:comment     "Information on the print manifestation of a court report. cf. http://curia.europa.eu/jcms/jcms/Jo2_10203/contenu" ;
        rdfs:label       "Part of an manifestation of a court report" ;
        rdfs:subClassOf  :manifestation_print ;
        rdfs:subClassOf  [ a                   owl:Restriction ;
                           owl:maxCardinality  "1"^^xsd:nonNegativeInteger ;
                           owl:onProperty      :manifestation_court-report_part_pages_total
                         ] ;
        rdfs:subClassOf  [ a                owl:Restriction ;
                           owl:cardinality  "1"^^xsd:nonNegativeInteger ;
                           owl:onProperty   :manifestation_court-report_part_page_first
                         ] ;
        rdfs:subClassOf  [ a                   owl:Restriction ;
                           owl:maxCardinality  "1"^^xsd:nonNegativeInteger ;
                           owl:onProperty      :manifestation_court-report_part_number
                         ] ;
        rdfs:subClassOf  [ a                   owl:Restriction ;
                           owl:maxCardinality  "1"^^xsd:nonNegativeInteger ;
                           owl:onProperty      :manifestation_court-report_part_page_last
                         ] ;
        rdfs:subClassOf  [ a                   owl:Restriction ;
                           owl:maxCardinality  "1"^^xsd:nonNegativeInteger ;
                           owl:onProperty      :manifestation_court-report_part_type
                         ] ;
        rdfs:subClassOf  [ a                   owl:Restriction ;
                           owl:maxCardinality  "1"^^xsd:nonNegativeInteger ;
                           owl:onProperty      :manifestation_court-report_part_year
                         ] .

:treaty_consolidated  a  owl:Class ;
        rdfs:comment     "Consolidated treaty (= sector 1E in EUR-Lex)" ;
        rdfs:label       "Consolidated treaty" ;
        rdfs:subClassOf  :treaty .

:validates  a       owl:ObjectProperty ;
        rdfs:label  "Validates" .

:summary_summarizes_work
        a                   owl:ObjectProperty ;
        rdfs:comment        "The work is summarized by another work (e.g. the summary of case law, to be embedded)" ;
        rdfs:domain         :summary ;
        rdfs:label          "Summary summarizes another work" ;
        rdfs:range          :work ;
        rdfs:subPropertyOf  :summarizes ;
        owl:inverseOf       :work_summarized_by_summary .

:work_dataset_business_classification
        a            owl:DatatypeProperty ;
        rdfs:domain  :work_dataset ;
        rdfs:label   "Work dataset business classification" ;
        rdfs:range   xsd:anyURI .

:main-activities_code
        a           owl:DatatypeProperty ;
        rdfs:label  "Main activities code" .

:heading  a         owl:DatatypeProperty ;
        rdfs:label  "Heading" .

:annex_part_of_work  a      owl:ObjectProperty ;
        rdfs:comment        "This property associates an instance of a work with an instance of ANNEX that forms part of it." ;
        rdfs:domain         :annex ;
        rdfs:label          "Annex part of work" ;
        rdfs:range          :work ;
        rdfs:subPropertyOf  :subdivision_part_of_work , :part_of ;
        owl:inverseOf       :work_contains_annex .

:manifestation_special-court-report_part
        a                owl:Class ;
        rdfs:comment     "Information on the print manifestation of a special edition of a court report. cf. http://curia.europa.eu/jcms/jcms/Jo2_10203/contenu" ;
        rdfs:label       "Part of an manifestation of a special edition of a court report" ;
        rdfs:subClassOf  :manifestation_print ;
        rdfs:subClassOf  [ a                   owl:Restriction ;
                           owl:maxCardinality  "1"^^xsd:nonNegativeInteger ;
                           owl:onProperty      :manifestation_special-court-report_part_year
                         ] ;
        rdfs:subClassOf  [ a                   owl:Restriction ;
                           owl:maxCardinality  "1"^^xsd:nonNegativeInteger ;
                           owl:onProperty      :manifestation_special-court-report_part_type
                         ] ;
        rdfs:subClassOf  [ a                   owl:Restriction ;
                           owl:maxCardinality  "1"^^xsd:nonNegativeInteger ;
                           owl:onProperty      :manifestation_special-court-report_part_pages_total
                         ] ;
        rdfs:subClassOf  [ a                   owl:Restriction ;
                           owl:maxCardinality  "1"^^xsd:nonNegativeInteger ;
                           owl:onProperty      :manifestation_special-court-report_part_page_last
                         ] ;
        rdfs:subClassOf  [ a                owl:Restriction ;
                           owl:cardinality  "1"^^xsd:nonNegativeInteger ;
                           owl:onProperty   :manifestation_special-court-report_part_page_first
                         ] .

:resource_legal_date_request_opinion
        a                   owl:DatatypeProperty ;
        rdfs:comment        "For the Court of Justice of the European Union documents: the field indicates when the document was lodged with the Registrar of the EU Court of Justice (or EFTA Court). For the Committee of Regions, European Economic and Social Committee: Date on which a proposal is submitted for consultation. LO_COMMENT is mixed content, coded with fd_305. Date lodged / LO_DATE. Relevant for legal analysis: true" ;
        rdfs:domain         :resource_legal ;
        rdfs:label          "Date of request for an opinion" ;
        rdfs:range          xsd:date ;
        rdfs:subPropertyOf  :date_request_opinion .

<http://publications.europa.eu/resource/authority/role-qualifier>
        a       owl:NamedIndividual .

:concept_case-law  a         owl:Class ;
        rdfs:comment         "Concept from the case law directory. The case law concept is currently coded with FD_Table 577" ;
        rdfs:label           "Case law concept" ;
        rdfs:subClassOf      skos:Concept , :concept ;
        owl:equivalentClass  [ a               owl:Restriction ;
                               owl:hasValue    <http://publications.europa.eu/resource/authority/fd_577> ;
                               owl:onProperty  skos:inScheme
                             ] .

:formally-addresses  a  owl:ObjectProperty ;
        rdfs:label  "Formally addresses" .

:distribution_status_is_status_of_manifestation_distribution
        a              owl:ObjectProperty ;
        rdfs:domain    :distribution_status ;
        rdfs:label     "Distribution status is status of manifestation distribution" ;
        rdfs:range     :manifestation_distribution ;
        owl:inverseOf  :manifestation_distribution_has_status_distribution_status .

:reports_on  a      owl:ObjectProperty ;
        rdfs:label  "Reports on" .

:concept_directory-code_subject_of_special-official-journal
        a                   owl:ObjectProperty ;
        rdfs:comment        "A concept from the directory of EU legal acts is one of the subjects of a special edition of the Official Journal" ;
        rdfs:domain         :concept_directory-code ;
        rdfs:label          "Directory code concept is subject of special edition" ;
        rdfs:range          :special-official-journal ;
        rdfs:subPropertyOf  :subject_of ;
        owl:inverseOf       :special-official-journal_is_about_concept_directory-code .

:person_reports_on_opinion_other_eesc
        a              owl:ObjectProperty ;
        rdfs:domain    :person ;
        rdfs:label     "Person reports on opinion other eesc" ;
        rdfs:range     :opinion_other_eesc ;
        owl:inverseOf  :opinion_other_eesc_reported_by_person .

:framework_procedural_sequential-number_nature
        a           owl:DatatypeProperty ;
        rdfs:label  "Framework procedural sequential number nature" .

:procedure_internal_open_public_consultation_needed
        a                   owl:DatatypeProperty ;
        rdfs:comment        "Do the better_regulation_requirements require an open public consultation for this internal procedure? /ns4:ec_transmission_request/transmission/workflow/extension/ns3:better_regulation_requirements/ns3:open_public_consultation" ;
        rdfs:domain         :procedure_internal ;
        rdfs:label          "Internal procedure needs open public consultation?" ;
        rdfs:range          xsd:boolean ;
        rdfs:subPropertyOf  :open_public_consultation_needed .

:used_for_drafting  a  owl:ObjectProperty ;
        rdfs:label  "Used for drafting" .

:resource_legal_manuscript_ref
        a                   owl:DatatypeProperty ;
        rdfs:comment        "Manuscript reference. Added in the context of IMMC2CDM-OJ" ;
        rdfs:domain         :resource_legal ;
        rdfs:label          "This element is used to mark up the reference of the manuscript sent to the printer" ;
        rdfs:range          xsd:string ;
        rdfs:subPropertyOf  :manuscript_ref .

:court-report_year  a       owl:DatatypeProperty ;
        rdfs:comment        "Year in which this Court report appeared" ;
        rdfs:domain         :court-report ;
        rdfs:label          "Year of court report" ;
        rdfs:range          xsd:gYear ;
        rdfs:subPropertyOf  :year .

:extent  a          owl:DatatypeProperty ;
        rdfs:label  "Extent" .

:concept_type_decision
        a                    owl:Class ;
        rdfs:comment         "Now coded with table 602 Example: <DECISION id=\"1070\">Adoption</DECISION><LIBELLE CODE=\"1070\">Adoption</LIBELLE>" ;
        rdfs:label           "Concept representing the decision type in Prelex" ;
        rdfs:subClassOf      skos:Concept , :concept_decoding ;
        owl:equivalentClass  [ a               owl:Restriction ;
                               owl:hasValue    <http://publications.europa.eu/resource/authority/fd_602> ;
                               owl:onProperty  skos:inScheme
                             ] .

:appendix_part_of_work
        a                   owl:ObjectProperty ;
        rdfs:comment        "An appendix (representing a subdivision) is part of another work" ;
        rdfs:domain         :appendix ;
        rdfs:label          "Appendix part of work" ;
        rdfs:range          :work ;
        rdfs:subPropertyOf  :subdivision_part_of_work ;
        owl:inverseOf       :work_contains_appendix .

:special-official-journal_publishes_resource_legal
        a                   owl:ObjectProperty ;
        rdfs:domain         :special-official-journal ;
        rdfs:label          "Special official journal publishes a legal resource" ;
        rdfs:range          :resource_legal ;
        rdfs:subPropertyOf  :publishes ;
        owl:inverseOf       :resource_legal_published_in_special-official-journal .

cmr:lastModificationDate
        a             owl:DatatypeProperty ;
        rdfs:comment  "The last date/time at which an entity in the Common Metadata Repository was modified." ;
        rdfs:label    "CMR last modification date" ;
        rdfs:range    xsd:dateTime .

:notice_prior-information_main-activities_code
        a                   owl:DatatypeProperty ;
        rdfs:domain         :notice_prior-information ;
        rdfs:label          "Code of main activities" ;
        rdfs:range          xsd:string ;
        rdfs:subPropertyOf  :main-activities_code .

:source_information_additional
        a           owl:DatatypeProperty ;
        rdfs:label  "Source information additional" .

:agent_has_role-qualifier
        a                   owl:ObjectProperty ;
        rdfs:domain         :agent ;
        rdfs:label          "Agent has a role" ;
        rdfs:range          :role-qualifier ;
        rdfs:subPropertyOf  :has .

cmr:manifestationMimeType
        a                   owl:DatatypeProperty ;
        rdfs:comment        "The MIME type associated with a manifestation, and thus with all principal content streams of that manifestation. \"principal\" here means the top level content stream MIME type. (e.g. a principal or content stream may be in xhtml, while this xhtml may carry images in tiff, png or other formats). Such top level content streams are in the PO metsMessage accessed with: - mets/fileSec/fileGrp/file"@en ;
        rdfs:label          "CMR manifestation MIME-type"@en ;
        rdfs:range          xsd:string ;
        rdfs:subPropertyOf  owl:topDataProperty .

:ATTO_FD_400  a              owl:Class ;
        rdfs:label           "FD_400 ATTO table" ;
        rdfs:subClassOf      skos:Concept ;
        owl:equivalentClass  [ a               owl:Restriction ;
                               owl:hasValue    <http://publications.europa.eu/resource/authority/fd_400> ;
                               owl:onProperty  skos:inScheme
                             ] .

:manifestation_edition
        a                   owl:DatatypeProperty ;
        rdfs:comment        "edition of this manifestation. mapped from 250 $a" ;
        rdfs:domain         :manifestation ;
        rdfs:label          "Manifestation edition" ;
        rdfs:range          xsd:string ;
        rdfs:subPropertyOf  :edition .

:resource_legal_internal_number_prefix
        a                   owl:DatatypeProperty ;
        rdfs:comment        "Prefix of the unique internal identifier of the resource legal. Standard and official document with the Council logo. E.g. legislative acts, working documents, information notes, agendas, minute, outcome of proceedings and other reports, Standard documents without the Council logo, e.g. EUCO, PE-CONS, ACP-CE, EUROMED, EU-AL, These documents are numbered from 1 to 5000" ;
        rdfs:domain         :resource_legal ;
        rdfs:label          "Internal number prefix" ;
        rdfs:range          xsd:string ;
        rdfs:subPropertyOf  :internal_number_prefix .

:question_parliamentary_date_reply
        a                   owl:DatatypeProperty ;
        rdfs:comment        "Date of the answer of the institution to a parliamentary question. Relevant for legal analysis: true" ;
        rdfs:domain         :question_parliamentary ;
        rdfs:label          "Date of reply" ;
        rdfs:range          xsd:date ;
        rdfs:subPropertyOf  :date_reply .

:publication_general_bibliography
        a                   owl:DatatypeProperty ;
        rdfs:comment        "Bibliography" ;
        rdfs:domain         :publication_general ;
        rdfs:label          "Bibliography" ;
        rdfs:range          xsd:string ;
        rdfs:subPropertyOf  :bibliography .

:archive_package_eesc_contains_archive_package_eesc_document
        a                   owl:ObjectProperty ;
        rdfs:comment        "Archive package from the European Economic and Social Committee contains a sub document (=section)." ;
        rdfs:domain         :archive_package_eesc ;
        rdfs:label          "Archive package from the European Economic and Social Committee contains a singular document." ;
        rdfs:range          :archive_package_eesc_document ;
        rdfs:subPropertyOf  :archive_package_contains_archive_package_document ;
        owl:inverseOf       :archive_package_eesc_document_part_of_archive_package_eesc .

:subsubsection_oj  a  owl:DatatypeProperty ;
        rdfs:label  "subsubsection oj" .

:binding_belongs_to_manifestation
        a                   owl:ObjectProperty ;
        rdfs:domain         :binding ;
        rdfs:label          "Binding of a manifestation" ;
        rdfs:range          :manifestation ;
        rdfs:subPropertyOf  :belongs_to ;
        owl:inverseOf       :manifestation_has_binding .

:dissemination-status
        a                    owl:Class ;
        rdfs:comment         "Corresponds to the contents of authority table dissemination-status (http://publications.europa.eu/resource/authority/dissemination-status)" ;
        rdfs:label           "Concept representing the dissemination status of any FRBR entity" ;
        rdfs:subClassOf      :concept_decoding ;
        owl:equivalentClass  [ a               owl:Restriction ;
                               owl:hasValue    <http://publications.europa.eu/resource/authority/dissemination-status> ;
                               owl:onProperty  skos:inScheme
                             ] .

:country_initiates_case-law
        a                   owl:ObjectProperty ;
        rdfs:domain         :country ;
        rdfs:label          "Country initiates / is origin of case law" ;
        rdfs:range          :case-law ;
        rdfs:subPropertyOf  :initiates ;
        owl:inverseOf       :case-law_originates_in_country .

:information_number  a  owl:DatatypeProperty ;
        rdfs:label  "Information number" .

:work_contains_chapter_legal
        a                   owl:ObjectProperty ;
        rdfs:domain         :work ;
        rdfs:label          "Work contains chapter (legal)" ;
        rdfs:range          :chapter_legal ;
        rdfs:subPropertyOf  :work_contains_subdivision , :contains .

:legislation_complementary_stored_by_agent
        a                   owl:ObjectProperty ;
        rdfs:comment        "Complementary lesiglation is stored by an agent acting as depositary. DP (1) / depositary. Relevant for legal analysis: true." ;
        rdfs:domain         :legislation_complementary ;
        rdfs:label          "Complementary legislation stored by agent" ;
        rdfs:range          :agent ;
        rdfs:subPropertyOf  :stored_by ;
        owl:inverseOf       :agent_depositary_for_legislation_complementary .

:case-law_referred_to_for_preliminary_ruling_case-law
        a                   owl:ObjectProperty ;
        rdfs:comment        "Used in sector 8 (national case law) notices. The value placed is the preliminary ruling from the Court of Justice of the EU." ;
        rdfs:domain         :case-law ;
        rdfs:label          "Case law referred to for preliminary ruling from another case law" ;
        rdfs:range          :case-law ;
        rdfs:subPropertyOf  :referred_to_for_preliminary_ruling ;
        owl:inverseOf       :case-law_refers_to_for_preliminary_ruling_case-law .

:contains_ep_opinion_on
        a           owl:ObjectProperty ;
        rdfs:label  "Contains ep opinion on" .

:event_case_has_procjur-type
        a                   owl:ObjectProperty ;
        rdfs:comment        "Case event has a procedural framework with a given type of procedure. Possible values taken from authority table procjur-types, corresponds to R, I, P" ;
        rdfs:domain         :event_case ;
        rdfs:label          "Case event has a procedural framework with a given type of procedure" ;
        rdfs:range          :procjur-type ;
        rdfs:subPropertyOf  :has .

:licence_document  a     owl:Class ;
        rdfs:comment     "Corresponds to the contents of the MDR authority list licence" ;
        rdfs:label       "Concept representing the licence" ;
        rdfs:subClassOf  :concept_decoding .

:event  a                owl:Class ;
        rdfs:comment     "\"This class comprises changes of states in cultural, social or physical systems, regardless of scale, brought about by a series or group of coherent physical, cultural, technological or legal phenomena.\" (CIDOC CRM)" ;
        rdfs:label       "Event" ;
        rdfs:subClassOf  :period ;
        rdfs:subClassOf  [ a                owl:Restriction ;
                           owl:cardinality  "1"^^xsd:nonNegativeInteger ;
                           owl:onProperty   cmr:lastModificationDate
                         ] ;
        rdfs:subClassOf  [ a                   owl:Restriction ;
                           owl:maxCardinality  "1"^^xsd:nonNegativeInteger ;
                           owl:onProperty      :event_session_date_start
                         ] ;
        rdfs:subClassOf  [ a                         owl:Restriction ;
                           owl:onClass               :concept_type_event ;
                           owl:onProperty            :event_has_type_concept_type_event ;
                           owl:qualifiedCardinality  "1"^^xsd:nonNegativeInteger
                         ] ;
        rdfs:subClassOf  [ a                            owl:Restriction ;
                           owl:maxQualifiedCardinality  "1"^^xsd:nonNegativeInteger ;
                           owl:onClass                  :dossier ;
                           owl:onProperty               :event_part_of_dossier
                         ] ;
        rdfs:subClassOf  [ a                   owl:Restriction ;
                           owl:maxCardinality  "1"^^xsd:nonNegativeInteger ;
                           owl:onProperty      cmr:creationDate
                         ] ;
        rdfs:subClassOf  [ a                owl:Restriction ;
                           owl:cardinality  "1"^^xsd:nonNegativeInteger ;
                           owl:onProperty   :event_date
                         ] ;
        rdfs:subClassOf  [ a                   owl:Restriction ;
                           owl:maxCardinality  "1"^^xsd:nonNegativeInteger ;
                           owl:onProperty      :event_embargo
                         ] ;
        rdfs:subClassOf  [ a                   owl:Restriction ;
                           owl:maxCardinality  "1"^^xsd:nonNegativeInteger ;
                           owl:onProperty      :event_session_date_end
                         ] ;
        rdfs:subClassOf  [ a                   owl:Restriction ;
                           owl:maxCardinality  "1"^^xsd:nonNegativeInteger ;
                           owl:onProperty      :event_number_session
                         ] .

:proceeding_third-party
        a                owl:Class ;
        rdfs:comment     "Third party proceeding in sector 6 (6CT/6TT/6FT)" ;
        rdfs:label       "Third party proceeding" ;
        rdfs:subClassOf  :case-law .

:archive_package_ec_has_title_from_com_final
        a            owl:DatatypeProperty ;
        rdfs:domain  :archive_package_ec ;
        rdfs:label   "Archive package EC has title from COM final" ;
        rdfs:range   xsd:boolean .

:involves  a        owl:ObjectProperty ;
        rdfs:label  "Involves" .

:person_co-reports_work
        a                   owl:ObjectProperty ;
        rdfs:domain         :person ;
        rdfs:label          "Person co-reports work" ;
        rdfs:range          :work ;
        rdfs:subPropertyOf  :co-reports ;
        owl:inverseOf       :work_co-reported_by_person .

:associated_with  a  owl:ObjectProperty ;
        rdfs:label  "Associated with" .

:container_case-law  a   owl:Class ;
        rdfs:comment     "A container work regrouping multiple case law documents for publication purposes. This work in particular regroups multiple related case law documents for publication and display on EUR-Lex. Typically, the case law container is identified by a numpub. Use the general work_part_of_work relationship to indicate that a case law is part of a case law collection" ;
        rdfs:label       "Container work for case law" ;
        rdfs:subClassOf  :container_work ;
        rdfs:subClassOf  [ a                   owl:Restriction ;
                           owl:maxCardinality  "1"^^xsd:nonNegativeInteger ;
                           owl:onProperty      :container_case-law_section
                         ] ;
        rdfs:subClassOf  [ a                   owl:Restriction ;
                           owl:maxCardinality  "1"^^xsd:nonNegativeInteger ;
                           owl:onProperty      :container_case-law_fascicule
                         ] ;
        rdfs:subClassOf  [ a                   owl:Restriction ;
                           owl:maxCardinality  "1"^^xsd:nonNegativeInteger ;
                           owl:onProperty      :container_case-law_number
                         ] ;
        rdfs:subClassOf  [ a                   owl:Restriction ;
                           owl:maxCardinality  "1"^^xsd:nonNegativeInteger ;
                           owl:onProperty      :container_case-law_year_decision
                         ] ;
        rdfs:subClassOf  [ a                   owl:Restriction ;
                           owl:maxCardinality  "1"^^xsd:nonNegativeInteger ;
                           owl:onProperty      :container_case-law_type_court_report
                         ] ;
        rdfs:subClassOf  [ a                   owl:Restriction ;
                           owl:maxCardinality  "1"^^xsd:nonNegativeInteger ;
                           owl:onProperty      :container_case-law_court
                         ] ;
        rdfs:subClassOf  [ a                owl:Restriction ;
                           owl:cardinality  "1"^^xsd:nonNegativeInteger ;
                           owl:onProperty   :container_case-law_id_numpub
                         ] ;
        rdfs:subClassOf  [ a                   owl:Restriction ;
                           owl:maxCardinality  "1"^^xsd:nonNegativeInteger ;
                           owl:onProperty      :container_case-law_series
                         ] .

:sender_transmission  a  owl:DatatypeProperty ;
        rdfs:label  "Sender transmission" .

:target_audience_old  a      owl:Class ;
        rdfs:label           "Target audience old" ;
        rdfs:subClassOf      skos:Concept ;
        owl:equivalentClass  [ a               owl:Restriction ;
                               owl:hasValue    <http://publications.europa.eu/resource/authority/pub_target> ;
                               owl:onProperty  skos:inScheme
                             ] .

:communication_cjeu_communicates_on_case-law
        a                   owl:ObjectProperty ;
        rdfs:comment        "If communication_cjeu published in OJ informs about the content of case-law document from the Court, this property points to this Court document. Relevant for legal analysis: true." ;
        rdfs:domain         :communication_cjeu ;
        rdfs:label          "Communication communicates on case law" ;
        rdfs:range          :case-law ;
        rdfs:subPropertyOf  :communicates_on ;
        owl:deprecated      true ;
        owl:inverseOf       :case-law_communicated_on_by_communication_cjeu .

:event_session_date_start
        a                   owl:DatatypeProperty ;
        rdfs:comment        "The start date of the session during which this event took place, e.g. in the Council or the Committee of the Regions" ;
        rdfs:domain         :event ;
        rdfs:label          "Start date of a session" ;
        rdfs:range          xsd:date ;
        rdfs:subPropertyOf  :session_date_start .

:opinion_other_cor_reported_by_person
        a                   owl:ObjectProperty ;
        rdfs:comment        "Name of the person (EP member or member of CoR or EESC) who reports on the relevant act. This property will be deprecated and replaced with work_reported_by_person. Role RAPP. Relevant for legal analysis: true" ;
        rdfs:domain         :opinion_other_cor ;
        rdfs:label          "Committee of the Regions' other opinion has rapporteur" ;
        rdfs:range          :person ;
        rdfs:subPropertyOf  :work_reported_by_person ;
        dct:created         "2018-07-16T13:20:03.944+02:00"^^xsd:dateTime ;
        owl:inverseOf       :person_reports_on_opinion_other_cor .

:resource_legal_comment_internal
        a                   owl:DatatypeProperty ;
        rdfs:comment        "Internal comment on this resource. CM. Relevant for legal analysis: true." ;
        rdfs:domain         :resource_legal ;
        rdfs:label          "Internal comment" ;
        rdfs:range          xsd:string ;
        rdfs:subPropertyOf  :comment_internal .

:restriction_on_use_belongs_to_manifestation
        a           owl:ObjectProperty ;
        rdfs:label  "Restriction on use belongs to manifestation" .

:proposal_recommendation_ec
        a                owl:Class ;
        rdfs:label       "Commission proposal for a recommendation" ;
        rdfs:subClassOf  :proposal_act , :act_preparatory_ec .

:number_catalogue_global
        a           owl:DatatypeProperty ;
        rdfs:label  "Number catalogue global" .

:case-law_national_parties
        a                   owl:DatatypeProperty ;
        rdfs:comment        "Reference to the parties involved in this case law. Use an XML structure to capture the sequence of references" ;
        rdfs:domain         :case-law_national ;
        rdfs:label          "Parties of the case law" ;
        rdfs:range          rdf:XMLLiteral ;
        rdfs:subPropertyOf  :parties .

:type-procedure  a    owl:Class ;
        rdfs:comment  "Type of an (institutional) procedure" ;
        rdfs:label    "Type of procedure" .

:title_legal_part_of_work
        a                   owl:ObjectProperty ;
        rdfs:comment        "This property associates an instance of a work with an instance of a title_legal that forms part of it." ;
        rdfs:domain         :title_legal ;
        rdfs:label          "Title (legal) part of work" ;
        rdfs:range          :work ;
        rdfs:subPropertyOf  :subdivision_part_of_work , :part_of ;
        owl:inverseOf       :work_contains_title_legal .

:mandatorily-addressed_by
        a           owl:ObjectProperty ;
        rdfs:label  "Mandatorily addressed by" .

:work_part_of_dossier
        a                       owl:ObjectProperty ;
        rdfs:comment            ". Relevant for legal analysis: true." ;
        rdfs:domain             :work ;
        rdfs:label              "Work is part of dossier" ;
        rdfs:range              :dossier ;
        rdfs:subPropertyOf      :part_of ;
        owl:inverseOf           :dossier_contains_work ;
        owl:propertyChainAxiom  ( :work_part_of_event_legal :event_legal_part_of_dossier ) .

:opinion_cjeu  a         owl:Class ;
        rdfs:comment     "Opinion of the Court of Justice in sector 6 (= type 6CV)" ;
        rdfs:label       "Opinion of the Court of Justice" ;
        rdfs:subClassOf  :case-law .

:session_ep  a           owl:Class ;
        rdfs:comment     "DEPRECATED, This class represents a session of the European Parliament; it refers to the parliamentary term in which the session takes place." ;
        rdfs:label       "EP session" ;
        rdfs:subClassOf  :session ;
        owl:deprecated   true .

:work_contains_citation
        a                   owl:ObjectProperty ;
        rdfs:domain         :work ;
        rdfs:label          "Work contains citation" ;
        rdfs:range          :citation ;
        rdfs:subPropertyOf  :work_contains_subdivision , :contains .

:sitting_part_of_session
        a                   owl:ObjectProperty ;
        rdfs:comment        "This relation links a sitting to the session of the respective institution or working body, e.g. committee" ;
        rdfs:domain         :sitting ;
        rdfs:label          "Sitting part of session" ;
        rdfs:range          :session ;
        rdfs:subPropertyOf  :event_part_of_dossier .

:opinion_advocate-general_joined_to_case_court
        a                   owl:ObjectProperty ;
        rdfs:comment        "Only in IMMC concext" ;
        rdfs:domain         :opinion_advocate-general ;
        rdfs:label          "Conclusions are part of a case" ;
        rdfs:range          :case_court ;
        rdfs:subPropertyOf  :joined_to ;
        owl:inverseOf       :case_court_has_joined_conclusion_opinion_advocate-general .

:work_contains_subdivision
        a                   owl:ObjectProperty ;
        rdfs:comment        "The subdivision of this work" ;
        rdfs:domain         :work ;
        rdfs:label          "Work contains subdivision" ;
        rdfs:range          :subdivision ;
        rdfs:subPropertyOf  :contains .

:extends_validity_of  a  owl:ObjectProperty ;
        rdfs:label  "Extends validity of" .

<http://publications.europa.eu/resource/authority/corporate-body/ECA>
        a       owl:NamedIndividual .

:affaire_jurisdiction
        a             owl:DatatypeProperty ;
        rdfs:comment  "Jurisdiction part of the Court case identification" ;
        rdfs:label    "Jurisdiction of case" .

:asked_by  a        owl:ObjectProperty ;
        rdfs:label  "Asked by" .

:date_official_journal
        a           owl:DatatypeProperty ;
        rdfs:label  "Date official journal" .

:procurement_public_date_dispatch
        a                   owl:DatatypeProperty ;
        rdfs:domain         :procurement_public ;
        rdfs:label          "Dispatch date" ;
        rdfs:range          xsd:date ;
        rdfs:subPropertyOf  :date_dispatch .

:work_has_expression  a     owl:ObjectProperty ;
        rdfs:comment        "Relevant for legal analysis: true. The work has one or more expressions. Relevant for legal analysis: true" ;
        rdfs:domain         :work ;
        rdfs:label          "Work has expression" ;
        rdfs:range          :expression ;
        rdfs:subPropertyOf  :has .

:grounds  a         owl:DatatypeProperty ;
        rdfs:label  "Grounds" .

:official-journal_legal_effect_paper
        a                   owl:DatatypeProperty ;
        rdfs:comment        "Does the paper version of this OJ issue have legal effect? To be included after the adoption of a regulation on electronic publication of OJ" ;
        rdfs:domain         :official-journal ;
        rdfs:label          "Legal effect for paper version of the Official Journal" ;
        rdfs:range          xsd:boolean ;
        rdfs:subPropertyOf  :legal_effect_paper .

:reference_publication
        a           owl:DatatypeProperty ;
        rdfs:label  "Reference publication" .

:manifestation_case-law
        a                owl:Class ;
        rdfs:comment     "Note: Conciously suppressed are: 1, décision + 2, sommaire proprement dit (avec référence aux affaires précédentes) -" ;
        rdfs:label       "Manifestation of case law" ;
        rdfs:subClassOf  :manifestation ;
        rdfs:subClassOf  [ a                   owl:Restriction ;
                           owl:maxCardinality  "1"^^xsd:nonNegativeInteger ;
                           owl:onProperty      :manifestation_case-law_subject
                         ] ;
        rdfs:subClassOf  [ a                   owl:Restriction ;
                           owl:maxCardinality  "1"^^xsd:nonNegativeInteger ;
                           owl:onProperty      :manifestation_case-law_grounds
                         ] ;
        rdfs:subClassOf  [ a                   owl:Restriction ;
                           owl:maxCardinality  "1"^^xsd:nonNegativeInteger ;
                           owl:onProperty      :manifestation_case-law_endorsements
                         ] ;
        rdfs:subClassOf  [ a                   owl:Restriction ;
                           owl:maxCardinality  "1"^^xsd:nonNegativeInteger ;
                           owl:onProperty      :manifestation_case-law_keywords
                         ] ;
        rdfs:subClassOf  [ a                   owl:Restriction ;
                           owl:maxCardinality  "1"^^xsd:nonNegativeInteger ;
                           owl:onProperty      :manifestation_case-law_parties
                         ] ;
        rdfs:subClassOf  [ a                   owl:Restriction ;
                           owl:maxCardinality  "1"^^xsd:nonNegativeInteger ;
                           owl:onProperty      :manifestation_case-law_costs_decisions
                         ] ;
        rdfs:subClassOf  [ a                   owl:Restriction ;
                           owl:maxCardinality  "1"^^xsd:nonNegativeInteger ;
                           owl:onProperty      :manifestation_case-law_operative_part
                         ] .

:procurement_public_nuts_original_link_title
        a                   owl:DatatypeProperty ;
        rdfs:domain         :procurement_public ;
        rdfs:label          "NUTS orignal title" ;
        rdfs:range          xsd:string ;
        rdfs:subPropertyOf  :nuts_original_link_title .

:cpv_original_reference
        a           owl:DatatypeProperty ;
        rdfs:label  "Cpv original reference" .

:resource_legal_contains_fragment_resource_legal
        a                   owl:ObjectProperty ;
        rdfs:domain         :resource_legal ;
        rdfs:label          "Legal resource contains a legal article" ;
        rdfs:range          :fragment_resource_legal ;
        rdfs:subPropertyOf  :contains ;
        owl:inverseOf       :fragment_resource_legal_part_of_resource_legal .

:act_other_eesc_number_session
        a                   owl:DatatypeProperty ;
        rdfs:comment        "DEPRECATED. Number of session during which this act was debated or voted (EP, EESC, CoR, …). Relevant for legal analysis: true" ;
        rdfs:domain         :act_other_eesc ;
        rdfs:label          "Number of session" ;
        rdfs:range          xsd:string ;
        rdfs:subPropertyOf  :number_session , :act_preparatory_number_session ;
        owl:deprecated      true .

:title_information_additional
        a                   owl:DatatypeProperty ;
        rdfs:label          "Title information additional" ;
        rdfs:subPropertyOf  :title .

:resource_legal_preliminary_question-submitted_by_communication_case_new
        a              owl:ObjectProperty ;
        rdfs:domain    :resource_legal ;
        rdfs:label     "Resource legal preliminary question submitted by communication case new" ;
        rdfs:range     :communication_case_new ;
        owl:inverseOf  :communication_case_new_submits_preliminary_question_resource_legal .

:national_website_link
        a           owl:DatatypeProperty ;
        rdfs:label  "National website link" .

:identifier_court  a  owl:DatatypeProperty ;
        rdfs:label  "Identifier court" .
