<?xml version="1.0" encoding="UTF-8"?>
<rdf:RDF xmlns:rdf="http://www.w3.org/1999/02/22-rdf-syntax-ns#"
         xmlns:at="http://publications.europa.eu/ontology/authority/"
         xmlns:rdfs="http://www.w3.org/2000/01/rdf-schema#"
         xmlns:owl="http://www.w3.org/2002/07/owl#"
         xmlns:skos="http://www.w3.org/2004/02/skos/core#"
         xmlns:atold="http://publications.europa.eu/resource/authority/"
         xmlns:dc="http://purl.org/dc/elements/1.1/"
         xml:base="http://publications.europa.eu/resource/authority/access-right">
   <skos:ConceptScheme rdf:about="http://publications.europa.eu/resource/authority/access-right"
                       at:table.id="access-right"
                       at:table.version.number="20230614-0">
      <at:prefLabel xml:lang="en">Access right</at:prefLabel>
      <rdfs:label xml:lang="en">Access right</rdfs:label>
      <owl:versionInfo>20230614-0</owl:versionInfo>
      <skos:prefLabel xml:lang="en">Access right</skos:prefLabel>
   </skos:ConceptScheme>
   <skos:Concept rdf:about="http://publications.europa.eu/resource/authority/access-right/CONFIDENTIAL"
                 at:deprecated="false">
      <skos:prefLabel xml:lang="bg">поверителен</skos:prefLabel>
      <skos:prefLabel xml:lang="cs">důvěrné</skos:prefLabel>
      <skos:prefLabel xml:lang="da">fortrolig</skos:prefLabel>
      <skos:prefLabel xml:lang="de">vertraulich</skos:prefLabel>
      <skos:prefLabel xml:lang="el">εμπιστευτικό</skos:prefLabel>
      <skos:prefLabel xml:lang="en">confidential</skos:prefLabel>
      <skos:prefLabel xml:lang="es">confidencial</skos:prefLabel>
      <skos:prefLabel xml:lang="et">konfidentsiaalne</skos:prefLabel>
      <skos:prefLabel xml:lang="fi">luottamuksellinen</skos:prefLabel>
      <skos:prefLabel xml:lang="fr">confidentiel</skos:prefLabel>
      <skos:prefLabel xml:lang="ga">rúnda</skos:prefLabel>
      <skos:prefLabel xml:lang="hr">povjerljivo</skos:prefLabel>
      <skos:prefLabel xml:lang="hu">bizalmas</skos:prefLabel>
      <skos:prefLabel xml:lang="it">riservato</skos:prefLabel>
      <skos:prefLabel xml:lang="lt">konfidencialus</skos:prefLabel>
      <skos:prefLabel xml:lang="lv">konfidenciāls</skos:prefLabel>
      <skos:prefLabel xml:lang="mt">kunfidenzjali</skos:prefLabel>
      <skos:prefLabel xml:lang="nl">vertrouwelijk</skos:prefLabel>
      <skos:prefLabel xml:lang="pl">poufny</skos:prefLabel>
      <skos:prefLabel xml:lang="pt">confidencial</skos:prefLabel>
      <skos:prefLabel xml:lang="ro">confidențial</skos:prefLabel>
      <skos:prefLabel xml:lang="sk">dôverné</skos:prefLabel>
      <skos:prefLabel xml:lang="sl">zaupno</skos:prefLabel>
      <skos:prefLabel xml:lang="sv">konfidentiellt</skos:prefLabel>
      <at:authority-code>CONFIDENTIAL</at:authority-code>
      <at:op-code>CONFIDENTIAL</at:op-code>
      <at:start.use>2021-03-17</at:start.use>
      <atold:op-code>CONFIDENTIAL</atold:op-code>
      <dc:identifier>CONFIDENTIAL</dc:identifier>
      <skos:definition xml:lang="en">Information that is not disclosed. Usage note: Disclosure of this data could cause damage to interested parties such as public administrations and businesses. It may refer to personal and professional information as well as to information in the context of business, commerce or trade.</skos:definition>
      <skos:inScheme rdf:resource="http://publications.europa.eu/resource/authority/access-right"/>
      <skos:topConceptOf rdf:resource="http://publications.europa.eu/resource/authority/access-right"/>
   </skos:Concept>
   <skos:Concept rdf:about="http://publications.europa.eu/resource/authority/access-right/NON_PUBLIC"
                 at:deprecated="false">
      <skos:prefLabel xml:lang="bg">непубличен</skos:prefLabel>
      <skos:prefLabel xml:lang="cs">neveřejné</skos:prefLabel>
      <skos:prefLabel xml:lang="da">ikke-offentlig</skos:prefLabel>
      <skos:prefLabel xml:lang="de">nicht öffentlich</skos:prefLabel>
      <skos:prefLabel xml:lang="el">μη δημόσιο</skos:prefLabel>
      <skos:prefLabel xml:lang="en">non-public</skos:prefLabel>
      <skos:prefLabel xml:lang="es">no público</skos:prefLabel>
      <skos:prefLabel xml:lang="et">mitteavalik</skos:prefLabel>
      <skos:prefLabel xml:lang="fi">ei-julkinen</skos:prefLabel>
      <skos:prefLabel xml:lang="fr">non public</skos:prefLabel>
      <skos:prefLabel xml:lang="ga">neamhphoiblí</skos:prefLabel>
      <skos:prefLabel xml:lang="hr">nije za javnu objavu</skos:prefLabel>
      <skos:prefLabel xml:lang="hu">nem nyilvános</skos:prefLabel>
      <skos:prefLabel xml:lang="it">non pubblico</skos:prefLabel>
      <skos:prefLabel xml:lang="lt">neviešas</skos:prefLabel>
      <skos:prefLabel xml:lang="lv">nav publisks</skos:prefLabel>
      <skos:prefLabel xml:lang="mt">mhux pubbliku</skos:prefLabel>
      <skos:prefLabel xml:lang="nl">niet-openbaar</skos:prefLabel>
      <skos:prefLabel xml:lang="pl">niepubliczny</skos:prefLabel>
      <skos:prefLabel xml:lang="pt">não público</skos:prefLabel>
      <skos:prefLabel xml:lang="ro">neaccesibil publicului</skos:prefLabel>
      <skos:prefLabel xml:lang="sk">neverejné</skos:prefLabel>
      <skos:prefLabel xml:lang="sl">nejavno</skos:prefLabel>
      <skos:prefLabel xml:lang="sv">icke-offentligt</skos:prefLabel>
      <at:authority-code>NON_PUBLIC</at:authority-code>
      <at:op-code>NON_PUBLIC</at:op-code>
      <at:start.use>2013-01-01</at:start.use>
      <atold:op-code>NON_PUBLIC</atold:op-code>
      <dc:identifier>NON_PUBLIC</dc:identifier>
      <skos:definition xml:lang="en">Not publicly accessible for privacy, security or other reasons. Usage note: This category may include resources that contain sensitive or personal information.</skos:definition>
      <skos:inScheme rdf:resource="http://publications.europa.eu/resource/authority/access-right"/>
      <skos:topConceptOf rdf:resource="http://publications.europa.eu/resource/authority/access-right"/>
   </skos:Concept>
   <skos:Concept rdf:about="http://publications.europa.eu/resource/authority/access-right/NORMAL"
                 at:deprecated="true">
      <skos:prefLabel xml:lang="bg">нормален</skos:prefLabel>
      <skos:prefLabel xml:lang="cs">obvyklé</skos:prefLabel>
      <skos:prefLabel xml:lang="da">normal</skos:prefLabel>
      <skos:prefLabel xml:lang="de">normal</skos:prefLabel>
      <skos:prefLabel xml:lang="el">κανονικό</skos:prefLabel>
      <skos:prefLabel xml:lang="en">normal</skos:prefLabel>
      <skos:prefLabel xml:lang="es">normal</skos:prefLabel>
      <skos:prefLabel xml:lang="et">tavaline</skos:prefLabel>
      <skos:prefLabel xml:lang="fi">tavanomainen</skos:prefLabel>
      <skos:prefLabel xml:lang="fr">normal</skos:prefLabel>
      <skos:prefLabel xml:lang="ga">normálta</skos:prefLabel>
      <skos:prefLabel xml:lang="hr">tipično</skos:prefLabel>
      <skos:prefLabel xml:lang="hu">normál</skos:prefLabel>
      <skos:prefLabel xml:lang="it">normale</skos:prefLabel>
      <skos:prefLabel xml:lang="lt">normalus</skos:prefLabel>
      <skos:prefLabel xml:lang="lv">parasts</skos:prefLabel>
      <skos:prefLabel xml:lang="mt">normali</skos:prefLabel>
      <skos:prefLabel xml:lang="nl">normaal</skos:prefLabel>
      <skos:prefLabel xml:lang="pl">zwykły</skos:prefLabel>
      <skos:prefLabel xml:lang="pt">normal</skos:prefLabel>
      <skos:prefLabel xml:lang="ro">normal</skos:prefLabel>
      <skos:prefLabel xml:lang="sk">normálne</skos:prefLabel>
      <skos:prefLabel xml:lang="sl">običajno</skos:prefLabel>
      <skos:prefLabel xml:lang="sv">normal åtkomst</skos:prefLabel>
      <at:authority-code>NORMAL</at:authority-code>
      <at:op-code>NORMAL</at:op-code>
      <at:start.use>2009-12-01</at:start.use>
      <atold:op-code>NORMAL</atold:op-code>
      <dc:identifier>NORMAL</dc:identifier>
      <skos:definition xml:lang="en">Publicly accessible. This concept has been used in the schemas of IMMC, the Interinstitutional Metadata Maintenance Committee, as the predecessor of the current concept ‘public’.</skos:definition>
      <skos:inScheme rdf:resource="http://publications.europa.eu/resource/authority/access-right"/>
      <skos:topConceptOf rdf:resource="http://publications.europa.eu/resource/authority/access-right"/>
      <at:end.use>2022-03-16</at:end.use>
   </skos:Concept>
   <skos:Concept rdf:about="http://publications.europa.eu/resource/authority/access-right/OP_DATPRO"
                 at:deprecated="false">
      <skos:prefLabel xml:lang="bg">Неокончателни данни</skos:prefLabel>
      <skos:prefLabel xml:lang="cs">Předběžné údaje</skos:prefLabel>
      <skos:prefLabel xml:lang="da">Midlertidige data</skos:prefLabel>
      <skos:prefLabel xml:lang="de">Vorläufige Daten</skos:prefLabel>
      <skos:prefLabel xml:lang="el">Προσωρινά δεδομένα</skos:prefLabel>
      <skos:prefLabel xml:lang="en">Provisional data</skos:prefLabel>
      <skos:prefLabel xml:lang="es">Datos provisionales</skos:prefLabel>
      <skos:prefLabel xml:lang="et">Esialgsed andmed</skos:prefLabel>
      <skos:prefLabel xml:lang="fi">Alustavat tiedot</skos:prefLabel>
      <skos:prefLabel xml:lang="fr">Données provisoires</skos:prefLabel>
      <skos:prefLabel xml:lang="ga">Sonraí sealadacha</skos:prefLabel>
      <skos:prefLabel xml:lang="hr">Privremeni podaci</skos:prefLabel>
      <skos:prefLabel xml:lang="hu">Ideiglenes adatok</skos:prefLabel>
      <skos:prefLabel xml:lang="it">Dati provvisori</skos:prefLabel>
      <skos:prefLabel xml:lang="lt">Laikinieji duomenys</skos:prefLabel>
      <skos:prefLabel xml:lang="lv">Provizoriski dati</skos:prefLabel>
      <skos:prefLabel xml:lang="mt">Dejta provviżorja</skos:prefLabel>
      <skos:prefLabel xml:lang="nl">Voorlopige gegevens</skos:prefLabel>
      <skos:prefLabel xml:lang="pl">Dane tymczasowe</skos:prefLabel>
      <skos:prefLabel xml:lang="pt">Dados provisórios</skos:prefLabel>
      <skos:prefLabel xml:lang="ro">Date provizorii</skos:prefLabel>
      <skos:prefLabel xml:lang="sk">Predbežné údaje</skos:prefLabel>
      <skos:prefLabel xml:lang="sl">Začasni podatki</skos:prefLabel>
      <skos:prefLabel xml:lang="sv">Tillfälliga uppgifter</skos:prefLabel>
      <at:authority-code>OP_DATPRO</at:authority-code>
      <at:op-code>OP_DATPRO</at:op-code>
      <at:start.use>1952-07-23</at:start.use>
      <atold:op-code>OP_DATPRO</atold:op-code>
      <dc:identifier>OP_DATPRO</dc:identifier>
      <skos:inScheme rdf:resource="http://publications.europa.eu/resource/authority/access-right"/>
      <skos:topConceptOf rdf:resource="http://publications.europa.eu/resource/authority/access-right"/>
   </skos:Concept>
   <skos:Concept rdf:about="http://publications.europa.eu/resource/authority/access-right/PUBLIC"
                 at:deprecated="false">
      <skos:prefLabel xml:lang="bg">публичен</skos:prefLabel>
      <skos:prefLabel xml:lang="cs">veřejné</skos:prefLabel>
      <skos:prefLabel xml:lang="da">offentlig</skos:prefLabel>
      <skos:prefLabel xml:lang="de">öffentlich</skos:prefLabel>
      <skos:prefLabel xml:lang="el">δημόσιο</skos:prefLabel>
      <skos:prefLabel xml:lang="en">public</skos:prefLabel>
      <skos:prefLabel xml:lang="es">público</skos:prefLabel>
      <skos:prefLabel xml:lang="et">avalik</skos:prefLabel>
      <skos:prefLabel xml:lang="fi">julkinen</skos:prefLabel>
      <skos:prefLabel xml:lang="fr">public</skos:prefLabel>
      <skos:prefLabel xml:lang="ga">poiblí</skos:prefLabel>
      <skos:prefLabel xml:lang="hr">za javnu objavu</skos:prefLabel>
      <skos:prefLabel xml:lang="hu">nyilvános</skos:prefLabel>
      <skos:prefLabel xml:lang="it">pubblico</skos:prefLabel>
      <skos:prefLabel xml:lang="lt">viešas</skos:prefLabel>
      <skos:prefLabel xml:lang="lv">publiski pieejams</skos:prefLabel>
      <skos:prefLabel xml:lang="mt">pubbliku</skos:prefLabel>
      <skos:prefLabel xml:lang="nl">openbaar</skos:prefLabel>
      <skos:prefLabel xml:lang="pl">publiczny</skos:prefLabel>
      <skos:prefLabel xml:lang="pt">público</skos:prefLabel>
      <skos:prefLabel xml:lang="ro">public</skos:prefLabel>
      <skos:prefLabel xml:lang="sk">verejné</skos:prefLabel>
      <skos:prefLabel xml:lang="sl">javno</skos:prefLabel>
      <skos:prefLabel xml:lang="sv">offentligt</skos:prefLabel>
      <at:authority-code>PUBLIC</at:authority-code>
      <at:op-code>PUBLIC</at:op-code>
      <at:start.use>2013-01-01</at:start.use>
      <atold:op-code>PUBLIC</atold:op-code>
      <dc:identifier>PUBLIC</dc:identifier>
      <skos:definition xml:lang="en">Publicly accessible by everyone. Usage note: Permissible obstacles include registration and request for API keys, as long as anyone can request such registration and/or API keys.</skos:definition>
      <skos:inScheme rdf:resource="http://publications.europa.eu/resource/authority/access-right"/>
      <skos:topConceptOf rdf:resource="http://publications.europa.eu/resource/authority/access-right"/>
   </skos:Concept>
   <skos:Concept rdf:about="http://publications.europa.eu/resource/authority/access-right/RESTRICTED"
                 at:deprecated="false">
      <skos:prefLabel xml:lang="bg">с ограничен достъп</skos:prefLabel>
      <skos:prefLabel xml:lang="cs">vyhrazeno</skos:prefLabel>
      <skos:prefLabel xml:lang="da">til tjenestebrug</skos:prefLabel>
      <skos:prefLabel xml:lang="de">eingeschränkt</skos:prefLabel>
      <skos:prefLabel xml:lang="el">περιορισμένης χρήσης</skos:prefLabel>
      <skos:prefLabel xml:lang="en">restricted</skos:prefLabel>
      <skos:prefLabel xml:lang="es">restringido</skos:prefLabel>
      <skos:prefLabel xml:lang="et">piiratud</skos:prefLabel>
      <skos:prefLabel xml:lang="fi">rajoitettu</skos:prefLabel>
      <skos:prefLabel xml:lang="fr">restreint</skos:prefLabel>
      <skos:prefLabel xml:lang="ga">teoranta</skos:prefLabel>
      <skos:prefLabel xml:lang="hr">ograničen pristup</skos:prefLabel>
      <skos:prefLabel xml:lang="hu">korlátozott terjesztésű</skos:prefLabel>
      <skos:prefLabel xml:lang="it">limitato</skos:prefLabel>
      <skos:prefLabel xml:lang="lt">taikomi ribojimai</skos:prefLabel>
      <skos:prefLabel xml:lang="lv">ierobežotas pieejamības</skos:prefLabel>
      <skos:prefLabel xml:lang="mt">ristrett</skos:prefLabel>
      <skos:prefLabel xml:lang="nl">beperkt</skos:prefLabel>
      <skos:prefLabel xml:lang="pl">zastrzeżony</skos:prefLabel>
      <skos:prefLabel xml:lang="pt">restrito</skos:prefLabel>
      <skos:prefLabel xml:lang="ro">cu acces restricționat</skos:prefLabel>
      <skos:prefLabel xml:lang="sk">vyhradené</skos:prefLabel>
      <skos:prefLabel xml:lang="sl">interno</skos:prefLabel>
      <skos:prefLabel xml:lang="sv">begränsad åtkomst</skos:prefLabel>
      <at:authority-code>RESTRICTED</at:authority-code>
      <at:op-code>RESTRICTED</at:op-code>
      <at:start.use>2013-01-01</at:start.use>
      <atold:op-code>RESTRICTED</atold:op-code>
      <dc:identifier>RESTRICTED</dc:identifier>
      <skos:definition xml:lang="en">Only available under certain conditions. Usage note: This category may include resources that require payment, resources shared under non-disclosure agreements, resources for which the publisher or owner has not yet decided if they can be publicly released.</skos:definition>
      <skos:inScheme rdf:resource="http://publications.europa.eu/resource/authority/access-right"/>
      <skos:topConceptOf rdf:resource="http://publications.europa.eu/resource/authority/access-right"/>
   </skos:Concept>
   <skos:Concept rdf:about="http://publications.europa.eu/resource/authority/access-right/SENSITIVE"
                 at:deprecated="false">
      <skos:prefLabel xml:lang="bg">чувствителен</skos:prefLabel>
      <skos:prefLabel xml:lang="cs">citlivé</skos:prefLabel>
      <skos:prefLabel xml:lang="da">følsom</skos:prefLabel>
      <skos:prefLabel xml:lang="de">sensibel</skos:prefLabel>
      <skos:prefLabel xml:lang="el">ευαίσθητο</skos:prefLabel>
      <skos:prefLabel xml:lang="en">sensitive</skos:prefLabel>
      <skos:prefLabel xml:lang="es">sensible</skos:prefLabel>
      <skos:prefLabel xml:lang="et">tundlik</skos:prefLabel>
      <skos:prefLabel xml:lang="fi">arkaluonteinen</skos:prefLabel>
      <skos:prefLabel xml:lang="fr">sensible</skos:prefLabel>
      <skos:prefLabel xml:lang="ga">íogair</skos:prefLabel>
      <skos:prefLabel xml:lang="hr">osjetljivo</skos:prefLabel>
      <skos:prefLabel xml:lang="hu">érzékeny</skos:prefLabel>
      <skos:prefLabel xml:lang="it">sensibile</skos:prefLabel>
      <skos:prefLabel xml:lang="lt">neskelbtinas</skos:prefLabel>
      <skos:prefLabel xml:lang="lv">sensitīvs</skos:prefLabel>
      <skos:prefLabel xml:lang="mt">sensittiv</skos:prefLabel>
      <skos:prefLabel xml:lang="nl">gevoelig</skos:prefLabel>
      <skos:prefLabel xml:lang="pl">sensytywny</skos:prefLabel>
      <skos:prefLabel xml:lang="pt">sensível</skos:prefLabel>
      <skos:prefLabel xml:lang="ro">sensibil</skos:prefLabel>
      <skos:prefLabel xml:lang="sk">citlivé</skos:prefLabel>
      <skos:prefLabel xml:lang="sl">občutljivo</skos:prefLabel>
      <skos:prefLabel xml:lang="sv">känsligt</skos:prefLabel>
      <at:authority-code>SENSITIVE</at:authority-code>
      <at:op-code>SENSITIVE</at:op-code>
      <at:start.use>2020-03-18</at:start.use>
      <atold:op-code>SENSITIVE</atold:op-code>
      <dc:identifier>SENSITIVE</dc:identifier>
      <skos:definition xml:lang="en">Sensitive non-classified (SNC) information, information whose unauthorised disclosure could cause damage to the Commission or other interested parties such as businesses, companies, intellectual property or personal data but which is not EU classified information.</skos:definition>
      <skos:definition xml:lang="fr">Informations «sensibles non classifiées» (SNC), informations dont la divulgation non autorisée pourrait causer un préjudice à la Commission ou à d’autres parties intéressées telles que les entreprises, les sociétés, la propriété intellectuelle ou les données à caractère personnel, mais qui ne sont pas des informations classifiées de l’UE.</skos:definition>
      <skos:inScheme rdf:resource="http://publications.europa.eu/resource/authority/access-right"/>
      <skos:topConceptOf rdf:resource="http://publications.europa.eu/resource/authority/access-right"/>
   </skos:Concept>
</rdf:RDF>
